@prefix : <http://iec.ch/TC57/CIM-generic#> .
@prefix dc: <http://purl.org/dc/elements/1.1/> .
@prefix msg: <http://langdale.com.au/2005/Message#> .
@prefix owl: <http://www.w3.org/2002/07/owl#> .
@prefix rdf: <http://www.w3.org/1999/02/22-rdf-syntax-ns#> .
@prefix uml: <http://langdale.com.au/2005/UML#> .
@prefix xml: <http://www.w3.org/XML/1998/namespace> .
@prefix xsd: <http://www.w3.org/2001/XMLSchema#> .
@prefix rdfs: <http://www.w3.org/2000/01/rdf-schema#> .
@base <http://iec.ch/TC57/CIM-generic#> .

<http://iec.ch/TC57/CIM-generic> rdf:type owl:Ontology .

#################################################################
#    Annotation properties
#################################################################

###  http://iec.ch/TC57/CIM-generic#OldTransformerEndInfo.solidInsulationWeight
:OldTransformerEndInfo.solidInsulationWeight rdf:type owl:AnnotationProperty ;
                                             uml:id "_17A5040D-2047-4a64-8D7B-14FE792ADB70" ;
                                             rdfs:comment "Weight of solid insultation in transformer." ;
                                             rdfs:label "solidInsulationWeight" ;
                                             rdfs:domain :OldTransformerEndInfo .


###  http://iec.ch/TC57/CIM-generic#OldTransformerTankInfo.coreCoilsWeight
:OldTransformerTankInfo.coreCoilsWeight rdf:type owl:AnnotationProperty ;
                                        uml:id "_31200834-25CB-4cac-BAC7-CE5BF875DAD8" ;
                                        rdfs:comment "Weight of core and coils in transformer." ;
                                        rdfs:label "coreCoilsWeight" ;
                                        rdfs:domain :OldTransformerTankInfo .


###  http://iec.ch/TC57/CIM-generic#ProductAssetModel.weightTotal
:ProductAssetModel.weightTotal rdf:type owl:AnnotationProperty ;
                               uml:id "_5BA8CFE6-3E0B-4d77-8910-62D0B57A2537" ;
                               rdfs:comment "Total manufactured weight of asset." ;
                               rdfs:label "weightTotal" ;
                               rdfs:domain :ProductAssetModel .


###  http://iec.ch/TC57/CIM-generic#SwitchInfo.gasWeightPerTank
:SwitchInfo.gasWeightPerTank rdf:type owl:AnnotationProperty ;
                             uml:id "_FB310EDA-3064-4783-896C-ECE09394DE3F" ;
                             rdfs:comment "Weight of gas in each tank of SF6 dead tank breaker." ;
                             rdfs:label "gasWeightPerTank" ;
                             rdfs:domain :SwitchInfo .


###  http://langdale.com.au/2005/UML#baseprefix
uml:baseprefix rdf:type owl:AnnotationProperty .


###  http://langdale.com.au/2005/UML#baseuri
uml:baseuri rdf:type owl:AnnotationProperty .


###  http://langdale.com.au/2005/UML#hasInitialValue
uml:hasInitialValue rdf:type owl:AnnotationProperty .


###  http://langdale.com.au/2005/UML#hasMaxCardinality
uml:hasMaxCardinality rdf:type owl:AnnotationProperty .


###  http://langdale.com.au/2005/UML#hasMinCardinality
uml:hasMinCardinality rdf:type owl:AnnotationProperty .


###  http://langdale.com.au/2005/UML#hasMultiplier
uml:hasMultiplier rdf:type owl:AnnotationProperty .


###  http://langdale.com.au/2005/UML#hasStereotype
uml:hasStereotype rdf:type owl:AnnotationProperty .


###  http://langdale.com.au/2005/UML#hasUnits
uml:hasUnits rdf:type owl:AnnotationProperty .


###  http://langdale.com.au/2005/UML#id
uml:id rdf:type owl:AnnotationProperty .


###  http://langdale.com.au/2005/UML#roleALabel
uml:roleALabel rdf:type owl:AnnotationProperty .


###  http://langdale.com.au/2005/UML#roleAOf
uml:roleAOf rdf:type owl:AnnotationProperty .


###  http://langdale.com.au/2005/UML#roleBLabel
uml:roleBLabel rdf:type owl:AnnotationProperty .


###  http://langdale.com.au/2005/UML#roleBOf
uml:roleBOf rdf:type owl:AnnotationProperty .


###  http://langdale.com.au/2005/UML#uriHasPrefix
uml:uriHasPrefix rdf:type owl:AnnotationProperty .


#################################################################
#    Datatypes
#################################################################

###  http://iec.ch/TC57/CIM-generic#ActivePower
:ActivePower rdf:type rdfs:Datatype ;
             uml:hasUnits "W" ;
             uml:id "_E52EDC2D-8972-42c7-A7EB-D8C017E138A4" ;
             rdfs:comment "Product of RMS value of the voltage and the RMS value of the in-phase component of the current." ;
             rdfs:label "ActivePower" ;
             owl:equivalentClass xsd:float .


###  http://iec.ch/TC57/CIM-generic#ActivePowerChangeRate
:ActivePowerChangeRate rdf:type rdfs:Datatype ;
                       uml:hasUnits "WPers" ;
                       uml:id "_C872CC3E-AEC1-4ea2-93C8-0E51DDC2DA30" ;
                       rdfs:comment "Rate of change of active power per time." ;
                       rdfs:label "ActivePowerChangeRate" ;
                       owl:equivalentClass xsd:float .


###  http://iec.ch/TC57/CIM-generic#ActivePowerPerCurrentFlow
:ActivePowerPerCurrentFlow rdf:type rdfs:Datatype ;
                           uml:hasUnits "WPerA" ;
                           uml:id "_D0F4E10E-A379-4a83-A452-974B8D2B45AD" ;
                           rdfs:comment "Active power variation with current flow." ;
                           rdfs:label "ActivePowerPerCurrentFlow" ;
                           owl:equivalentClass xsd:float .


###  http://iec.ch/TC57/CIM-generic#ActivePowerPerFrequency
:ActivePowerPerFrequency rdf:type rdfs:Datatype ;
                         uml:hasUnits "WPers" ;
                         uml:id "_322D4C26-DEB6-4f9b-98CF-BA06ACD58EF8" ;
                         rdfs:comment "Active power variation with frequency." ;
                         rdfs:label "ActivePowerPerFrequency" ;
                         owl:equivalentClass xsd:float .


###  http://iec.ch/TC57/CIM-generic#Admittance
:Admittance rdf:type rdfs:Datatype ;
            uml:hasUnits "S" ;
            uml:id "_30AC6821-E972-456a-8F64-0765D7361767" ;
            rdfs:comment "Ratio of current to voltage." ;
            rdfs:label "Admittance" ;
            owl:equivalentClass xsd:float .


###  http://iec.ch/TC57/CIM-generic#AngleDegrees
:AngleDegrees rdf:type rdfs:Datatype ;
              uml:hasMultiplier "none" ;
              uml:hasUnits "deg" ;
              uml:id "_A633BDC9-A238-4f69-AF1B-FF8A5C2FFCC8" ;
              rdfs:comment "Measurement of angle in degrees." ;
              rdfs:label "AngleDegrees" ;
              owl:equivalentClass xsd:float .


###  http://iec.ch/TC57/CIM-generic#AngleRadians
:AngleRadians rdf:type rdfs:Datatype ;
              uml:hasMultiplier "none" ;
              uml:hasUnits "rad" ;
              uml:id "_E491E83D-03A0-4cad-86D4-30A09EF320F3" ;
              rdfs:comment "Phase angle in radians." ;
              rdfs:label "AngleRadians" ;
              owl:equivalentClass xsd:float .


###  http://iec.ch/TC57/CIM-generic#ApparentPower
:ApparentPower rdf:type rdfs:Datatype ;
               uml:hasUnits "VA" ;
               uml:id "_95576B4A-D9AC-49fc-82ED-CB6DB2CE8584" ;
               rdfs:comment "Product of the RMS value of the voltage and the RMS value of the current." ;
               rdfs:label "ApparentPower" ;
               owl:equivalentClass xsd:float .


###  http://iec.ch/TC57/CIM-generic#Area
:Area rdf:type rdfs:Datatype ;
      uml:hasUnits "m2" ;
      uml:id "_BD3D15F2-CB39-41a5-935D-7B8F490ECBF8" ;
      rdfs:comment "Area." ;
      rdfs:label "Area" ;
      owl:equivalentClass xsd:float .


###  http://iec.ch/TC57/CIM-generic#Bearing
:Bearing rdf:type rdfs:Datatype ;
         uml:hasMultiplier "none" ;
         uml:hasUnits "deg" ;
         uml:id "_FAB258CB-D0F4-49eb-82B5-1E3FE343A1EE" ;
         rdfs:comment "The bearing in degrees (with 360 degrees being True North).  Measured in degrees clockwise from True North.  0 degrees indicates no direction being given." ;
         rdfs:label "Bearing" ;
         owl:equivalentClass xsd:float .


###  http://iec.ch/TC57/CIM-generic#Capacitance
:Capacitance rdf:type rdfs:Datatype ;
             uml:hasUnits "F" ;
             uml:id "_B2C696FA-9529-4b58-9D82-4062406AEACF" ;
             rdfs:comment "Capacitive part of reactance (imaginary part of impedance), at rated frequency." ;
             rdfs:label "Capacitance" ;
             owl:equivalentClass xsd:float .


###  http://iec.ch/TC57/CIM-generic#CapacitancePerLength
:CapacitancePerLength rdf:type rdfs:Datatype ;
                      uml:hasMultiplier "none" ;
                      uml:hasUnits "FPerm" ;
                      uml:id "_7436C3C1-BA51-447f-B351-1C9FAA335847" ;
                      rdfs:comment "Capacitance per unit of length." ;
                      rdfs:label "CapacitancePerLength" ;
                      owl:equivalentClass xsd:float .


###  http://iec.ch/TC57/CIM-generic#Classification
:Classification rdf:type rdfs:Datatype ;
                uml:hasMultiplier "none" ;
                uml:hasUnits "none" ;
                uml:id "_567D00ED-9FD9-4cd1-9B12-70AEA6F11BFC" ;
                rdfs:comment "Classification of level.  Specify as 1..n, with 1 being the most detailed, highest priority, etc as described on the attribute using this data type." ;
                rdfs:label "Classification" ;
                owl:equivalentClass xsd:integer .


###  http://iec.ch/TC57/CIM-generic#Conductance
:Conductance rdf:type rdfs:Datatype ;
             uml:hasUnits "S" ;
             uml:id "_CCE4615A-C403-4c96-8122-26904C128276" ;
             rdfs:comment "Factor by which voltage must be multiplied to give corresponding power lost from a circuit. Real part of admittance." ;
             rdfs:label "Conductance" ;
             owl:equivalentClass xsd:float .


###  http://iec.ch/TC57/CIM-generic#ConductancePerLength
:ConductancePerLength rdf:type rdfs:Datatype ;
                      uml:hasMultiplier "none" ;
                      uml:hasUnits "SPerm" ;
                      uml:id "_0C25DC23-EAD4-4ea0-B0C3-D7C46488E3F8" ;
                      rdfs:comment "Real part of admittance per unit of length." ;
                      rdfs:label "ConductancePerLength" ;
                      owl:equivalentClass xsd:float .


###  http://iec.ch/TC57/CIM-generic#CostPerEnergyUnit
:CostPerEnergyUnit rdf:type rdfs:Datatype ;
                   uml:id "_781B4357-DF24-4f4f-BBE3-8C8CE1C0F2E5" ;
                   rdfs:comment "Cost, in units of currency, per quantity of electrical energy generated." ;
                   rdfs:label "CostPerEnergyUnit" ;
                   owl:equivalentClass xsd:float .


###  http://iec.ch/TC57/CIM-generic#CostPerHeatUnit
:CostPerHeatUnit rdf:type rdfs:Datatype ;
                 uml:id "_E1913AA6-E24F-4b45-BB9B-946567FC7AF6" ;
                 rdfs:comment "Cost, in units of currency, per quantity of heat generated." ;
                 rdfs:label "CostPerHeatUnit" ;
                 owl:equivalentClass xsd:float .


###  http://iec.ch/TC57/CIM-generic#CostPerVolume
:CostPerVolume rdf:type rdfs:Datatype ;
               uml:id "_56D3E01F-B21E-4f00-A8F1-CBC80D384B3B" ;
               rdfs:comment "Cost per unit volume." ;
               rdfs:label "CostPerVolume" ;
               owl:equivalentClass xsd:float .


###  http://iec.ch/TC57/CIM-generic#CostRate
:CostRate rdf:type rdfs:Datatype ;
          uml:id "_A8B9F2B7-69E6-4698-8492-D6A8E70D8755" ;
          rdfs:comment "Cost, in units of currency, per elapsed time." ;
          rdfs:label "CostRate" ;
          owl:equivalentClass xsd:float .


###  http://iec.ch/TC57/CIM-generic#CurrentFlow
:CurrentFlow rdf:type rdfs:Datatype ;
             uml:hasUnits "A" ;
             uml:id "_DC3FD69C-E9B2-440d-A113-BE84B71BA691" ;
             rdfs:comment "Electrical current with sign convention: positive flow is out of the conducting equipment into the connectivity node. Can be both AC and DC." ;
             rdfs:label "CurrentFlow" ;
             owl:equivalentClass xsd:float .


###  http://iec.ch/TC57/CIM-generic#Damping
:Damping rdf:type rdfs:Datatype ;
         uml:hasUnits "onePerHz" ;
         uml:id "_9CD49278-B929-4acf-A09E-43660FD1F7F7" ;
         rdfs:comment "Per-unit active power variation with frequency referenced on the system apparent power base. Typical values are in the range 1,0 - 2,0." ;
         rdfs:label "Damping" ;
         owl:equivalentClass xsd:float .


###  http://iec.ch/TC57/CIM-generic#Displacement
:Displacement rdf:type rdfs:Datatype ;
              uml:hasMultiplier "none" ;
              uml:hasUnits "m" ;
              uml:id "_9B356995-DED3-46c2-8DB7-AE244D4D3644" ;
              rdfs:comment "Unit of displacement relative to a reference position, hence can be negative." ;
              rdfs:label "Displacement" ;
              owl:equivalentClass xsd:float .


###  http://iec.ch/TC57/CIM-generic#Emission
:Emission rdf:type rdfs:Datatype ;
          uml:hasMultiplier "none" ;
          uml:hasUnits "kgPerJ" ;
          uml:id "_E1046D37-77EE-42b0-832A-8AF115835122" ;
          rdfs:comment "Quantity of emission per fuel heat content." ;
          rdfs:label "Emission" ;
          owl:equivalentClass xsd:float .


###  http://iec.ch/TC57/CIM-generic#Frequency
:Frequency rdf:type rdfs:Datatype ;
           uml:hasUnits "Hz" ;
           uml:id "_DD71FE93-4683-440c-8622-A8AA2EB44F6F" ;
           rdfs:comment "Cycles per second." ;
           rdfs:label "Frequency" ;
           owl:equivalentClass xsd:float .


###  http://iec.ch/TC57/CIM-generic#HeatRate
:HeatRate rdf:type rdfs:Datatype ;
          uml:hasUnits "J" ;
          uml:id "_8E0A1478-92E7-445a-9F23-9BCEB17FD303" ;
          rdfs:comment "Heat generated, in energy per time unit of elapsed time." ;
          rdfs:label "HeatRate" ;
          owl:equivalentClass xsd:float .


###  http://iec.ch/TC57/CIM-generic#Hours
:Hours rdf:type rdfs:Datatype ;
       uml:hasMultiplier "none" ;
       uml:hasUnits "h" ;
       uml:id "_C8C67111-A8BF-46d8-B8DB-F0336CD201D1" ;
       rdfs:comment "Time specified in hours." ;
       rdfs:label "Hours" ;
       owl:equivalentClass xsd:float .


###  http://iec.ch/TC57/CIM-generic#Impedance
:Impedance rdf:type rdfs:Datatype ;
           uml:hasUnits "ohm" ;
           uml:id "_3E46E0C6-230A-475b-B15C-B5B4754CDD65" ;
           rdfs:comment "Ratio of voltage to current." ;
           rdfs:label "Impedance" ;
           owl:equivalentClass xsd:float .


###  http://iec.ch/TC57/CIM-generic#Inductance
:Inductance rdf:type rdfs:Datatype ;
            uml:hasUnits "H" ;
            uml:id "_A5C20135-6480-450b-812C-23263BCC8553" ;
            rdfs:comment "Inductive part of reactance (imaginary part of impedance), at rated frequency." ;
            rdfs:label "Inductance" ;
            owl:equivalentClass xsd:float .


###  http://iec.ch/TC57/CIM-generic#InductancePerLength
:InductancePerLength rdf:type rdfs:Datatype ;
                     uml:hasMultiplier "none" ;
                     uml:hasUnits "HPerm" ;
                     uml:id "_256B27BD-003D-4cf9-9BAE-D9AD4CF6D948" ;
                     rdfs:comment "Inductance per unit of length." ;
                     rdfs:label "InductancePerLength" ;
                     owl:equivalentClass xsd:float .


###  http://iec.ch/TC57/CIM-generic#KiloActivePower
:KiloActivePower rdf:type rdfs:Datatype ;
                 uml:hasMultiplier "k" ;
                 uml:hasUnits "W" ;
                 uml:id "_BE17081C-6888-4153-B4AB-A672392B7467" ;
                 rdfs:comment "Active power in kilowatts." ;
                 rdfs:label "KiloActivePower" ;
                 owl:equivalentClass xsd:float .


###  http://iec.ch/TC57/CIM-generic#Length
:Length rdf:type rdfs:Datatype ;
        uml:hasUnits "m" ;
        uml:id "_06F9A3F0-3AE3-4ad1-88F8-06C207238C3B" ;
        rdfs:comment "Unit of length. It shall be a positive value or zero." ;
        rdfs:label "Length" ;
        owl:equivalentClass xsd:float .


###  http://iec.ch/TC57/CIM-generic#MagneticField
:MagneticField rdf:type rdfs:Datatype ;
               uml:hasMultiplier "n" ;
               uml:hasUnits "T" ;
               uml:id "_2C3CA1D1-1DBB-4f95-9BC9-60B0DD26DA65" ;
               rdfs:comment "Magnetic field in nanotesla." ;
               rdfs:label "MagneticField" ;
               owl:equivalentClass xsd:float .


###  http://iec.ch/TC57/CIM-generic#Mass
:Mass rdf:type rdfs:Datatype ;
      uml:hasMultiplier "k" ;
      uml:hasUnits "g" ;
      uml:id "_3090EC66-8B19-4224-A206-00BFE70ECED0" ;
      rdfs:comment "Mass." ;
      rdfs:label "Mass" ;
      owl:equivalentClass xsd:float .


###  http://iec.ch/TC57/CIM-generic#Minutes
:Minutes rdf:type rdfs:Datatype ;
         uml:hasMultiplier "none" ;
         uml:hasUnits "min" ;
         uml:id "_68F89418-6302-42a8-8177-5637B46ED1DB" ;
         rdfs:comment "Time in minutes." ;
         rdfs:label "Minutes" ;
         owl:equivalentClass xsd:float .


###  http://iec.ch/TC57/CIM-generic#Money
:Money rdf:type rdfs:Datatype ;
       uml:id "_5E4B6DE1-9115-4fce-9859-6714580E5C66" ;
       rdfs:comment "Amount of money." ;
       rdfs:label "Money" ;
       owl:equivalentClass xsd:decimal .


###  http://iec.ch/TC57/CIM-generic#MonthDay
:MonthDay rdf:type rdfs:Datatype ;
          uml:id "_06EEB33A-0F70-4c8c-A932-3836A0BF6872" ;
          rdfs:comment "MonthDay format as \"--mm-dd\", which conforms with XSD data type gMonthDay." ;
          rdfs:label "MonthDay" .


###  http://iec.ch/TC57/CIM-generic#PU
:PU rdf:type rdfs:Datatype ;
    uml:hasMultiplier "none" ;
    uml:hasUnits "none" ;
    uml:id "_B47F1EC8-BE4F-47df-9ACA-3F12A128BF85" ;
    rdfs:comment "Per Unit - a positive or negative value referred to a defined base. Values typically range from -10 to +10." ;
    rdfs:label "PU" ;
    owl:equivalentClass xsd:float .


###  http://iec.ch/TC57/CIM-generic#ParticulateDensity
:ParticulateDensity rdf:type rdfs:Datatype ;
                    uml:hasMultiplier "none" ;
                    uml:hasUnits "kgPerm3" ;
                    uml:id "_47AA7054-AC2F-4daf-B509-136A5802F368" ;
                    rdfs:comment "Particulate density as kg/m<sup>3</sup>." ;
                    rdfs:label "ParticulateDensity" ;
                    owl:equivalentClass xsd:float .


###  http://iec.ch/TC57/CIM-generic#PerCent
:PerCent rdf:type rdfs:Datatype ;
         uml:hasMultiplier "none" ;
         uml:hasUnits "none" ;
         uml:id "_8345A4E0-E4BB-45d6-894B-983BB43C4B4F" ;
         rdfs:comment "Percentage on a defined base.   For example, specify as 100 to indicate at the defined base." ;
         rdfs:label "PerCent" ;
         owl:equivalentClass xsd:float .


###  http://iec.ch/TC57/CIM-generic#Pressure
:Pressure rdf:type rdfs:Datatype ;
          uml:hasUnits "Pa" ;
          uml:id "_BBEF7CB4-FBE0-4bc5-9EB4-A3E586C7F34C" ;
          rdfs:comment "Pressure in pascals." ;
          rdfs:label "Pressure" ;
          owl:equivalentClass xsd:float .


###  http://iec.ch/TC57/CIM-generic#Reactance
:Reactance rdf:type rdfs:Datatype ;
           uml:hasUnits "ohm" ;
           uml:id "_F1C90FB4-B7BE-4528-A974-E36BBEAB8616" ;
           rdfs:comment "Reactance (imaginary part of impedance), at rated frequency." ;
           rdfs:label "Reactance" ;
           owl:equivalentClass xsd:float .


###  http://iec.ch/TC57/CIM-generic#ReactancePerLength
:ReactancePerLength rdf:type rdfs:Datatype ;
                    uml:hasMultiplier "none" ;
                    uml:hasUnits "ohmPerm" ;
                    uml:id "_ECCBABE8-F29C-4878-9504-35D08A1E9CA1" ;
                    rdfs:comment "Reactance (imaginary part of impedance) per unit of length, at rated frequency." ;
                    rdfs:label "ReactancePerLength" ;
                    owl:equivalentClass xsd:float .


###  http://iec.ch/TC57/CIM-generic#ReactivePower
:ReactivePower rdf:type rdfs:Datatype ;
               uml:hasUnits "VAr" ;
               uml:id "_C15CB4E4-4430-43ea-AF69-BC3250B1F4A3" ;
               rdfs:comment "Product of RMS value of the voltage and the RMS value of the quadrature component of the current." ;
               rdfs:label "ReactivePower" ;
               owl:equivalentClass xsd:float .


###  http://iec.ch/TC57/CIM-generic#RealEnergy
:RealEnergy rdf:type rdfs:Datatype ;
            uml:hasUnits "Wh" ;
            uml:id "_FD0D7251-962F-4c57-ACFB-C1F578AB6361" ;
            rdfs:comment "Real electrical energy." ;
            rdfs:label "RealEnergy" ;
            owl:equivalentClass xsd:float .


###  http://iec.ch/TC57/CIM-generic#Resistance
:Resistance rdf:type rdfs:Datatype ;
            uml:hasUnits "ohm" ;
            uml:id "_EDB281E6-BBB4-438d-953B-7D746CAF55B5" ;
            rdfs:comment "Resistance (real part of impedance)." ;
            rdfs:label "Resistance" ;
            owl:equivalentClass xsd:float .


###  http://iec.ch/TC57/CIM-generic#ResistancePerLength
:ResistancePerLength rdf:type rdfs:Datatype ;
                     uml:hasMultiplier "none" ;
                     uml:hasUnits "ohmPerm" ;
                     uml:id "_A4EFE5A9-F88A-4d8a-A35F-26D017259C43" ;
                     rdfs:comment "Resistance (real part of impedance) per unit of length." ;
                     rdfs:label "ResistancePerLength" ;
                     owl:equivalentClass xsd:float .


###  http://iec.ch/TC57/CIM-generic#RotationSpeed
:RotationSpeed rdf:type rdfs:Datatype ;
               uml:hasMultiplier "none" ;
               uml:hasUnits "Hz" ;
               uml:id "_D9556FC3-5453-44d9-94C5-07D51D3BAD82" ;
               rdfs:comment "Number of revolutions per second." ;
               rdfs:label "RotationSpeed" ;
               owl:equivalentClass xsd:float .


###  http://iec.ch/TC57/CIM-generic#Seconds
:Seconds rdf:type rdfs:Datatype ;
         uml:hasMultiplier "none" ;
         uml:hasUnits "s" ;
         uml:id "_A2008978-193D-4955-8102-599E43C7CFE4" ;
         rdfs:comment "Time, in seconds." ;
         rdfs:label "Seconds" ;
         owl:equivalentClass xsd:float .


###  http://iec.ch/TC57/CIM-generic#Speed
:Speed rdf:type rdfs:Datatype ;
       uml:hasMultiplier "none" ;
       uml:hasUnits "mPers" ;
       uml:id "_B2B55BF9-D1CD-4a20-8B96-E9509B356C6D" ;
       rdfs:comment "Distance per unit of time." ;
       rdfs:label "Speed" ;
       owl:equivalentClass xsd:float .


###  http://iec.ch/TC57/CIM-generic#Susceptance
:Susceptance rdf:type rdfs:Datatype ;
             uml:hasUnits "S" ;
             uml:id "_F246F97E-529D-4ec3-9F06-BAF4AFD0829B" ;
             rdfs:comment "Imaginary part of admittance." ;
             rdfs:label "Susceptance" ;
             owl:equivalentClass xsd:float .


###  http://iec.ch/TC57/CIM-generic#SusceptancePerLength
:SusceptancePerLength rdf:type rdfs:Datatype ;
                      uml:hasMultiplier "none" ;
                      uml:hasUnits "SPerm" ;
                      uml:id "_59A364BC-34EB-41b6-810C-88484A2D929C" ;
                      rdfs:comment "Imaginary part of admittance per unit of length." ;
                      rdfs:label "SusceptancePerLength" ;
                      owl:equivalentClass xsd:float .


###  http://iec.ch/TC57/CIM-generic#Temperature
:Temperature rdf:type rdfs:Datatype ;
             uml:hasMultiplier "none" ;
             uml:hasUnits "degC" ;
             uml:id "_2C614F42-FED1-4705-82C8-57771A0466CE" ;
             rdfs:comment "Value of temperature in degrees Celsius." ;
             rdfs:label "Temperature" ;
             owl:equivalentClass xsd:float .


###  http://iec.ch/TC57/CIM-generic#Voltage
:Voltage rdf:type rdfs:Datatype ;
         uml:hasUnits "V" ;
         uml:id "_233C330A-11B8-4705-879C-5497380F1D82" ;
         rdfs:comment "Electrical voltage, can be both AC and DC." ;
         rdfs:label "Voltage" ;
         owl:equivalentClass xsd:float .


###  http://iec.ch/TC57/CIM-generic#VoltagePerReactivePower
:VoltagePerReactivePower rdf:type rdfs:Datatype ;
                         uml:hasUnits "VPerVAr" ;
                         uml:id "_00D99B0C-4D20-43b7-AFA4-B0F9746CFE74" ;
                         rdfs:comment "Voltage variation with reactive power." ;
                         rdfs:label "VoltagePerReactivePower" ;
                         owl:equivalentClass xsd:float .


###  http://iec.ch/TC57/CIM-generic#Volume
:Volume rdf:type rdfs:Datatype ;
        uml:hasUnits "m3" ;
        uml:id "_20E0B5CF-6DA4-452c-A366-CBE9FC2DF962" ;
        rdfs:comment "Volume." ;
        rdfs:label "Volume" ;
        owl:equivalentClass xsd:float .


###  http://iec.ch/TC57/CIM-generic#VolumeFlowRate
:VolumeFlowRate rdf:type rdfs:Datatype ;
                uml:hasMultiplier "none" ;
                uml:hasUnits "m3Pers" ;
                uml:id "_0EFCC366-353D-41d8-983D-E16E170F716A" ;
                rdfs:comment "Volume per time." ;
                rdfs:label "VolumeFlowRate" ;
                owl:equivalentClass xsd:float .


###  http://iec.ch/TC57/CIM-generic#WaterLevel
:WaterLevel rdf:type rdfs:Datatype ;
            uml:hasUnits "m" ;
            uml:id "_97337107-69C4-4b94-B996-1375EF171312" ;
            rdfs:comment "Reservoir water level referred to a given datum such as mean sea level." ;
            rdfs:label "WaterLevel" ;
            owl:equivalentClass xsd:float .


###  http://www.w3.org/2001/XMLSchema#date
xsd:date rdf:type rdfs:Datatype .


###  http://www.w3.org/2001/XMLSchema#duration
xsd:duration rdf:type rdfs:Datatype .


###  http://www.w3.org/2001/XMLSchema#time
xsd:time rdf:type rdfs:Datatype .


#################################################################
#    Object Properties
#################################################################

###  http://iec.ch/TC57/CIM-generic#BaseVoltage.ConductingEquipment
:BaseVoltage.ConductingEquipment rdf:type owl:ObjectProperty ;
                                 owl:inverseOf :ConductingEquipment.BaseVoltage ;
                                 rdf:type owl:InverseFunctionalProperty ;
                                 rdfs:domain :BaseVoltage ;
                                 rdfs:range :ConductingEquipment ;
                                 uml:id "_B21687D9-2B46-4880-B016-06CCFA215EC3-A" ;
                                 rdfs:comment "All conducting equipment with this base voltage.  Use only when there is no voltage level container used and only one base voltage applies.  For example, not used for transformers." ;
                                 rdfs:label "ConductingEquipment" .


###  http://iec.ch/TC57/CIM-generic#BaseVoltage.VoltageLevel
:BaseVoltage.VoltageLevel rdf:type owl:ObjectProperty ;
                          owl:inverseOf :VoltageLevel.BaseVoltage ;
                          rdf:type owl:InverseFunctionalProperty ;
                          rdfs:domain :BaseVoltage ;
                          rdfs:range :VoltageLevel ;
                          uml:id "_F610FDC8-D98D-4367-99A9-E9CA1C8A8CC5-B" ;
                          rdfs:comment "The voltage levels having this base voltage." ;
                          rdfs:label "VoltageLevel" .


###  http://iec.ch/TC57/CIM-generic#Bay.Substation
:Bay.Substation rdf:type owl:ObjectProperty ;
                owl:inverseOf :Substation.Bays ;
                rdf:type owl:FunctionalProperty ;
                rdfs:domain :Bay ;
                rdfs:range :Substation ;
                uml:id "_51152F4A-1B03-451f-BA84-6A05A6AE1630-A" ;
                rdfs:comment "Substation containing the bay." ;
                rdfs:label "Substation" .


###  http://iec.ch/TC57/CIM-generic#Bay.VoltageLevel
:Bay.VoltageLevel rdf:type owl:ObjectProperty ;
                  owl:inverseOf :VoltageLevel.Bays ;
                  rdf:type owl:FunctionalProperty ;
                  rdfs:domain :Bay ;
                  rdfs:range :VoltageLevel ;
                  uml:id "_5E328091-5BC1-4fa8-9BA3-F087A215492A-B" ;
                  rdfs:comment "The voltage level containing this bay." ;
                  rdfs:label "VoltageLevel" .


###  http://iec.ch/TC57/CIM-generic#ConductingEquipment.BaseVoltage
:ConductingEquipment.BaseVoltage rdf:type owl:ObjectProperty ,
                                          owl:FunctionalProperty ;
                                 rdfs:domain :ConductingEquipment ;
                                 rdfs:range :BaseVoltage ;
                                 uml:id "_B21687D9-2B46-4880-B016-06CCFA215EC3-B" ;
                                 rdfs:comment "Base voltage of this conducting equipment.  Use only when there is no voltage level container used and only one base voltage applies.  For example, not used for transformers." ;
                                 rdfs:label "BaseVoltage" .


###  http://iec.ch/TC57/CIM-generic#ConductingEquipment.Terminals
:ConductingEquipment.Terminals rdf:type owl:ObjectProperty ;
                               owl:inverseOf :Terminal.ConductingEquipment ;
                               rdf:type owl:InverseFunctionalProperty ;
                               rdfs:domain :ConductingEquipment ;
                               rdfs:range :Terminal ;
                               uml:id "_5FEF5186-7804-4dad-8E18-8C5DB7FCE6B2-B" ;
                               rdfs:comment "Conducting equipment have terminals that may be connected to other conducting equipment terminals via connectivity nodes or topological nodes." ;
                               rdfs:label "Terminals" .


###  http://iec.ch/TC57/CIM-generic#ConnectivityNode.ConnectivityNodeContainer
:ConnectivityNode.ConnectivityNodeContainer rdf:type owl:ObjectProperty ;
                                            owl:inverseOf :ConnectivityNodeContainer.ConnectivityNodes ;
                                            rdf:type owl:FunctionalProperty ;
                                            rdfs:domain :ConnectivityNode ;
                                            rdfs:range :ConnectivityNodeContainer ;
                                            uml:id "_08EEABA6-269C-44a7-8F82-7BBEFE71ADD6-A" ;
                                            rdfs:comment "Container of this connectivity node." ;
                                            rdfs:label "ConnectivityNodeContainer" .


###  http://iec.ch/TC57/CIM-generic#ConnectivityNode.Terminals
:ConnectivityNode.Terminals rdf:type owl:ObjectProperty ;
                            owl:inverseOf :Terminal.ConnectivityNode ;
                            rdf:type owl:InverseFunctionalProperty ;
                            rdfs:domain :ConnectivityNode ;
                            rdfs:range :Terminal ;
                            uml:id "_C7E01609-F4E6-4a6e-8ACF-BDD413E62DE3-B" ;
                            rdfs:comment "Terminals interconnected with zero impedance at a this connectivity node." ;
                            rdfs:label "Terminals" .


###  http://iec.ch/TC57/CIM-generic#ConnectivityNodeContainer.ConnectivityNodes
:ConnectivityNodeContainer.ConnectivityNodes rdf:type owl:ObjectProperty ,
                                                      owl:InverseFunctionalProperty ;
                                             rdfs:domain :ConnectivityNodeContainer ;
                                             rdfs:range :ConnectivityNode ;
                                             uml:id "_08EEABA6-269C-44a7-8F82-7BBEFE71ADD6-B" ;
                                             rdfs:comment "Connectivity nodes which belong to this connectivity node container." ;
                                             rdfs:label "ConnectivityNodes" .


###  http://iec.ch/TC57/CIM-generic#Equipment.AdditionalEquipmentContainer
:Equipment.AdditionalEquipmentContainer rdf:type owl:ObjectProperty ;
                                        owl:inverseOf :EquipmentContainer.AdditionalGroupedEquipment ;
                                        rdfs:domain :Equipment ;
                                        rdfs:range :EquipmentContainer ;
                                        uml:id "_43EA076F-F51B-4617-BC39-6D3939D5CEFD-B" ;
                                        rdfs:comment "Additional equipment container beyond the primary equipment container.  The equipment is contained in another equipment container, but also grouped with this equipment container." ;
                                        rdfs:label "AdditionalEquipmentContainer" .


###  http://iec.ch/TC57/CIM-generic#Equipment.EquipmentContainer
:Equipment.EquipmentContainer rdf:type owl:ObjectProperty ;
                              owl:inverseOf :EquipmentContainer.Equipments ;
                              rdf:type owl:FunctionalProperty ;
                              rdfs:domain :Equipment ;
                              rdfs:range :EquipmentContainer ;
                              uml:id "_68BA73EF-8533-48ba-964A-DE0F722292D2-B" ;
                              rdfs:comment "Container of this equipment." ;
                              rdfs:label "EquipmentContainer" .


###  http://iec.ch/TC57/CIM-generic#EquipmentContainer.AdditionalGroupedEquipment
:EquipmentContainer.AdditionalGroupedEquipment rdf:type owl:ObjectProperty ;
                                               rdfs:domain :EquipmentContainer ;
                                               rdfs:range :Equipment ;
                                               uml:id "_43EA076F-F51B-4617-BC39-6D3939D5CEFD-A" ;
                                               rdfs:comment "The additonal contained equipment.  The equipment belong to the equipment container. The equipment is contained in another equipment container, but also grouped with this equipment container.  Examples include when a switch contained in a substation is also desired to be grouped with a line contianer or when a switch is included in a secondary substation and also grouped in a feeder." ;
                                               rdfs:label "AdditionalGroupedEquipment" .


###  http://iec.ch/TC57/CIM-generic#EquipmentContainer.Equipments
:EquipmentContainer.Equipments rdf:type owl:ObjectProperty ,
                                        owl:InverseFunctionalProperty ;
                               rdfs:domain :EquipmentContainer ;
                               rdfs:range :Equipment ;
                               uml:id "_68BA73EF-8533-48ba-964A-DE0F722292D2-A" ;
                               rdfs:comment "Contained equipment." ;
                               rdfs:label "Equipments" .


###  http://iec.ch/TC57/CIM-generic#GeographicalRegion.Regions
:GeographicalRegion.Regions rdf:type owl:ObjectProperty ;
                            owl:inverseOf :SubGeographicalRegion.Region ;
                            rdf:type owl:InverseFunctionalProperty ;
                            rdfs:domain :GeographicalRegion ;
                            rdfs:range :SubGeographicalRegion ;
                            uml:id "_023E20DF-DF02-4ffb-A047-E5BBDB18AB59-A" ;
                            rdfs:comment "All sub-geographical regions within this geographical region." ;
                            rdfs:label "Regions" .


###  http://iec.ch/TC57/CIM-generic#IdentifiedObject.Names
:IdentifiedObject.Names rdf:type owl:ObjectProperty ;
                        owl:inverseOf :Name.IdentifiedObject ;
                        rdf:type owl:InverseFunctionalProperty ;
                        rdfs:domain :IdentifiedObject ;
                        rdfs:range :Name ;
                        uml:id "_203C47E2-30FB-4c8f-ABEA-1661621CC0A7-B" ;
                        rdfs:comment "All names of this identified object." ;
                        rdfs:label "Names" .


###  http://iec.ch/TC57/CIM-generic#Line.Region
:Line.Region rdf:type owl:ObjectProperty ;
             owl:inverseOf :SubGeographicalRegion.Lines ;
             rdf:type owl:FunctionalProperty ;
             rdfs:domain :Line ;
             rdfs:range :SubGeographicalRegion ;
             uml:id "_BAB73169-D3BE-43c3-A58B-F1B87EAA1239-B" ;
             rdfs:comment "The sub-geographical region of the line." ;
             rdfs:label "Region" .


###  http://iec.ch/TC57/CIM-generic#Name.IdentifiedObject
:Name.IdentifiedObject rdf:type owl:ObjectProperty ,
                                owl:FunctionalProperty ;
                       rdfs:domain :Name ;
                       rdfs:range :IdentifiedObject ;
                       uml:id "_203C47E2-30FB-4c8f-ABEA-1661621CC0A7-A" ;
                       rdfs:comment "Identified object that this name designates." ;
                       rdfs:label "IdentifiedObject" .


###  http://iec.ch/TC57/CIM-generic#Name.NameType
:Name.NameType rdf:type owl:ObjectProperty ;
               owl:inverseOf :NameType.Names ;
               rdf:type owl:FunctionalProperty ;
               rdfs:domain :Name ;
               rdfs:range :NameType ;
               uml:id "_2DF559F1-C2F0-43ff-B7E0-654C3E738FDE-A" ;
               rdfs:comment "Type of this name." ;
               rdfs:label "NameType" .


###  http://iec.ch/TC57/CIM-generic#NameType.Names
:NameType.Names rdf:type owl:ObjectProperty ,
                         owl:InverseFunctionalProperty ;
                rdfs:domain :NameType ;
                rdfs:range :Name ;
                uml:id "_2DF559F1-C2F0-43ff-B7E0-654C3E738FDE-B" ;
                rdfs:comment "All names of this type." ;
                rdfs:label "Names" .


###  http://iec.ch/TC57/CIM-generic#PSRType.PowerSystemResources
:PSRType.PowerSystemResources rdf:type owl:ObjectProperty ;
                              owl:inverseOf :PowerSystemResource.PSRType ;
                              rdf:type owl:InverseFunctionalProperty ;
                              rdfs:domain :PSRType ;
                              rdfs:range :PowerSystemResource ;
                              uml:id "_739158B5-6CE8-473f-87FF-1CDA17078612-B" ;
                              rdfs:comment "Power system resources classified with this power system resource type." ;
                              rdfs:label "PowerSystemResources" .


###  http://iec.ch/TC57/CIM-generic#PowerSystemResource.PSRType
:PowerSystemResource.PSRType rdf:type owl:ObjectProperty ,
                                      owl:FunctionalProperty ;
                             rdfs:domain :PowerSystemResource ;
                             rdfs:range :PSRType ;
                             uml:id "_739158B5-6CE8-473f-87FF-1CDA17078612-A" ;
                             rdfs:comment "Custom classification for this power system resource." ;
                             rdfs:label "PSRType" .


###  http://iec.ch/TC57/CIM-generic#SubGeographicalRegion.Lines
:SubGeographicalRegion.Lines rdf:type owl:ObjectProperty ,
                                      owl:InverseFunctionalProperty ;
                             rdfs:domain :SubGeographicalRegion ;
                             rdfs:range :Line ;
                             uml:id "_BAB73169-D3BE-43c3-A58B-F1B87EAA1239-A" ;
                             rdfs:comment "The lines within the sub-geographical region." ;
                             rdfs:label "Lines" .


###  http://iec.ch/TC57/CIM-generic#SubGeographicalRegion.Region
:SubGeographicalRegion.Region rdf:type owl:ObjectProperty ,
                                       owl:FunctionalProperty ;
                              rdfs:domain :SubGeographicalRegion ;
                              rdfs:range :GeographicalRegion ;
                              uml:id "_023E20DF-DF02-4ffb-A047-E5BBDB18AB59-B" ;
                              rdfs:comment "The geographical region which this sub-geographical region is within." ;
                              rdfs:label "Region" .


###  http://iec.ch/TC57/CIM-generic#SubGeographicalRegion.Substations
:SubGeographicalRegion.Substations rdf:type owl:ObjectProperty ;
                                   owl:inverseOf :Substation.Region ;
                                   rdf:type owl:InverseFunctionalProperty ;
                                   rdfs:domain :SubGeographicalRegion ;
                                   rdfs:range :Substation ;
                                   uml:id "_66E7D72B-2889-483c-80A2-2E51B283F2B1-A" ;
                                   rdfs:comment "The substations in this sub-geographical region." ;
                                   rdfs:label "Substations" .


###  http://iec.ch/TC57/CIM-generic#Substation.Bays
:Substation.Bays rdf:type owl:ObjectProperty ,
                          owl:InverseFunctionalProperty ;
                 rdfs:domain :Substation ;
                 rdfs:range :Bay ;
                 uml:id "_51152F4A-1B03-451f-BA84-6A05A6AE1630-B" ;
                 rdfs:comment "Bays contained in the substation." ;
                 rdfs:label "Bays" .


###  http://iec.ch/TC57/CIM-generic#Substation.Region
:Substation.Region rdf:type owl:ObjectProperty ,
                            owl:FunctionalProperty ;
                   rdfs:domain :Substation ;
                   rdfs:range :SubGeographicalRegion ;
                   uml:id "_66E7D72B-2889-483c-80A2-2E51B283F2B1-B" ;
                   rdfs:comment "The SubGeographicalRegion containing the substation." ;
                   rdfs:label "Region" .


###  http://iec.ch/TC57/CIM-generic#Substation.VoltageLevels
:Substation.VoltageLevels rdf:type owl:ObjectProperty ;
                          owl:inverseOf :VoltageLevel.Substation ;
                          rdf:type owl:InverseFunctionalProperty ;
                          rdfs:domain :Substation ;
                          rdfs:range :VoltageLevel ;
                          uml:id "_0E9E9E28-C575-47c5-BF01-7F4EB8B36D16-A" ;
                          rdfs:comment "The voltage levels within this substation." ;
                          rdfs:label "VoltageLevels" .


###  http://iec.ch/TC57/CIM-generic#Terminal.ConductingEquipment
:Terminal.ConductingEquipment rdf:type owl:ObjectProperty ,
                                       owl:FunctionalProperty ;
                              rdfs:domain :Terminal ;
                              rdfs:range :ConductingEquipment ;
                              uml:id "_5FEF5186-7804-4dad-8E18-8C5DB7FCE6B2-A" ;
                              rdfs:comment "The conducting equipment of the terminal.  Conducting equipment have  terminals that may be connected to other conducting equipment terminals via connectivity nodes or topological nodes." ;
                              rdfs:label "ConductingEquipment" .


###  http://iec.ch/TC57/CIM-generic#Terminal.ConnectivityNode
:Terminal.ConnectivityNode rdf:type owl:ObjectProperty ,
                                    owl:FunctionalProperty ;
                           rdfs:domain :Terminal ;
                           rdfs:range :ConnectivityNode ;
                           uml:id "_C7E01609-F4E6-4a6e-8ACF-BDD413E62DE3-A" ;
                           rdfs:comment "The connectivity node to which this terminal connects with zero impedance." ;
                           rdfs:label "ConnectivityNode" .


###  http://iec.ch/TC57/CIM-generic#Terminal.phases
:Terminal.phases rdf:type owl:ObjectProperty ,
                          owl:FunctionalProperty ;
                 rdfs:domain :Terminal ;
                 rdfs:range :PhaseCode ;
                 uml:id "_8C0E221E-4988-48bf-BFC3-F9FFD7E7E075" ;
                 rdfs:comment """Represents the normal network phasing condition. If the attribute is missing, three phases (ABC) shall be assumed, except for terminals of grounding classes (specializations of EarthFaultCompensator, GroundDisconnector, and Ground) which will be assumed to be N. Therefore, phase code ABCN is explicitly declared when needed, e.g. for star point grounding equipment.
The phase code on terminals connecting same ConnectivityNode or same TopologicalNode as well as for equipment between two terminals shall be consistent.""" ;
                 rdfs:label "phases" .


###  http://iec.ch/TC57/CIM-generic#VoltageLevel.BaseVoltage
:VoltageLevel.BaseVoltage rdf:type owl:ObjectProperty ,
                                   owl:FunctionalProperty ;
                          rdfs:domain :VoltageLevel ;
                          rdfs:range :BaseVoltage ;
                          uml:id "_F610FDC8-D98D-4367-99A9-E9CA1C8A8CC5-A" ;
                          rdfs:comment "The base voltage used for all equipment within the voltage level." ;
                          rdfs:label "BaseVoltage" .


###  http://iec.ch/TC57/CIM-generic#VoltageLevel.Bays
:VoltageLevel.Bays rdf:type owl:ObjectProperty ,
                            owl:InverseFunctionalProperty ;
                   rdfs:domain :VoltageLevel ;
                   rdfs:range :Bay ;
                   uml:id "_5E328091-5BC1-4fa8-9BA3-F087A215492A-A" ;
                   rdfs:comment "The bays within this voltage level." ;
                   rdfs:label "Bays" .


###  http://iec.ch/TC57/CIM-generic#VoltageLevel.Substation
:VoltageLevel.Substation rdf:type owl:ObjectProperty ,
                                  owl:FunctionalProperty ;
                         rdfs:domain :VoltageLevel ;
                         rdfs:range :Substation ;
                         uml:id "_0E9E9E28-C575-47c5-BF01-7F4EB8B36D16-B" ;
                         rdfs:comment "The substation of the voltage level." ;
                         rdfs:label "Substation" .


#################################################################
#    Data properties
#################################################################

###  http://iec.ch/TC57/CIM-generic#ACDCTerminal.connected
:ACDCTerminal.connected rdf:type owl:DatatypeProperty ,
                                 owl:FunctionalProperty ;
                        rdfs:domain :ACDCTerminal ;
                        rdfs:range xsd:boolean ;
                        uml:id "_C97C0B38-C62F-4f03-A3DE-A67F29A6C6DB" ;
                        rdfs:comment """The connected status is related to a bus-branch model and the topological node to terminal relation.  True implies the terminal is connected to the related topological node and false implies it is not. 
In a bus-branch model, the connected status is used to tell if equipment is disconnected without having to change the connectivity described by the topological node to terminal relation. A valid case is that conducting equipment can be connected in one end and open in the other. In particular for an AC line segment, where the reactive line charging can be significant, this is a relevant case.""" ;
                        rdfs:label "connected" .


###  http://iec.ch/TC57/CIM-generic#ACDCTerminal.sequenceNumber
:ACDCTerminal.sequenceNumber rdf:type owl:DatatypeProperty ,
                                      owl:FunctionalProperty ;
                             rdfs:domain :ACDCTerminal ;
                             rdfs:range xsd:integer ;
                             uml:id "_7C7195D3-DFCD-487f-BF92-F359BBE7AFD0" ;
                             rdfs:comment "The orientation of the terminal connections for a multiple terminal conducting equipment.  The sequence numbering starts with 1 and additional terminals should follow in increasing order.   The first terminal is the \"starting point\" for a two terminal branch." ;
                             rdfs:label "sequenceNumber" .


###  http://iec.ch/TC57/CIM-generic#BaseFrequency.frequency
:BaseFrequency.frequency rdf:type owl:DatatypeProperty ,
                                  owl:FunctionalProperty ;
                         rdfs:domain :BaseFrequency ;
                         rdfs:range :Frequency ;
                         uml:id "_80C75B75-855F-44af-9846-BE082114E41E" ;
                         rdfs:comment "The base frequency." ;
                         rdfs:label "frequency" .


###  http://iec.ch/TC57/CIM-generic#BasePower.basePower
:BasePower.basePower rdf:type owl:DatatypeProperty ,
                              owl:FunctionalProperty ;
                     rdfs:domain :BasePower ;
                     rdfs:range :ApparentPower ;
                     uml:id "_9F2DC83B-B801-4b29-BD57-4781BD53A50A" ;
                     rdfs:comment "Value used as base power." ;
                     rdfs:label "basePower" .


###  http://iec.ch/TC57/CIM-generic#BaseVoltage.nominalVoltage
:BaseVoltage.nominalVoltage rdf:type owl:DatatypeProperty ,
                                     owl:FunctionalProperty ;
                            rdfs:domain :BaseVoltage ;
                            rdfs:range :Voltage ;
                            uml:id "_D37DA22A-916B-4a33-88AB-B77C229DB882" ;
                            rdfs:comment "The power system resource's base voltage.  Shall be a positive value and not zero." ;
                            rdfs:label "nominalVoltage" .


###  http://iec.ch/TC57/CIM-generic#Bay.bayEnergyMeasFlag
:Bay.bayEnergyMeasFlag rdf:type owl:DatatypeProperty ,
                                owl:FunctionalProperty ;
                       rdfs:domain :Bay ;
                       rdfs:range xsd:boolean ;
                       uml:id "_26D3924E-0222-4e9a-9373-CD7D256E9B19" ;
                       rdfs:comment "Indicates the presence/absence of energy measurements." ;
                       rdfs:label "bayEnergyMeasFlag" .


###  http://iec.ch/TC57/CIM-generic#Bay.bayPowerMeasFlag
:Bay.bayPowerMeasFlag rdf:type owl:DatatypeProperty ,
                               owl:FunctionalProperty ;
                      rdfs:domain :Bay ;
                      rdfs:range xsd:boolean ;
                      uml:id "_B5F9E0A2-7BE7-4bb1-A035-0F5F849847F0" ;
                      rdfs:comment "Indicates the presence/absence of active/reactive power measurements." ;
                      rdfs:label "bayPowerMeasFlag" .


###  http://iec.ch/TC57/CIM-generic#Breaker.inTransitTime
:Breaker.inTransitTime rdf:type owl:DatatypeProperty ,
                                owl:FunctionalProperty ;
                       rdfs:domain :Breaker ;
                       rdfs:range :Seconds ;
                       uml:id "_9F9445D9-22B1-4328-A4D5-C3B872F33DE2" ;
                       rdfs:comment "The transition time from open to close." ;
                       rdfs:label "inTransitTime" .


###  http://iec.ch/TC57/CIM-generic#Equipment.aggregate
:Equipment.aggregate rdf:type owl:DatatypeProperty ,
                              owl:FunctionalProperty ;
                     rdfs:domain :Equipment ;
                     rdfs:range xsd:boolean ;
                     uml:id "_3C000D48-C67D-4cc3-89D6-5F336420B325" ;
                     rdfs:comment """The aggregate flag provides an alternative way of representing an aggregated (equivalent) element. It is applicable in cases when the dedicated classes for equivalent equipment do not have all of the attributes necessary to represent the required level of detail.  In case the flag is set to “true” the single instance of equipment represents multiple pieces of equipment that have been modelled together as an aggregate equivalent obtained by a network reduction procedure. Examples would be power transformers or synchronous machines operating in parallel modelled as a single aggregate power transformer or aggregate synchronous machine.  
The attribute is not used for EquivalentBranch, EquivalentShunt and EquivalentInjection.""" ;
                     rdfs:label "aggregate" .


###  http://iec.ch/TC57/CIM-generic#Equipment.inService
:Equipment.inService rdf:type owl:DatatypeProperty ,
                              owl:FunctionalProperty ;
                     rdfs:domain :Equipment ;
                     rdfs:range xsd:boolean ;
                     uml:id "_84B66A12-0723-4edf-BC0E-5CD2F4034CC3" ;
                     rdfs:comment "Specifies the availability of the equipment. True means the equipment is available for topology processing, which determines if the equipment is energized or not. False means that the equipment is treated by network applications as if it is not in the model." ;
                     rdfs:label "inService" .


###  http://iec.ch/TC57/CIM-generic#Equipment.networkAnalysisEnabled
:Equipment.networkAnalysisEnabled rdf:type owl:DatatypeProperty ,
                                           owl:FunctionalProperty ;
                                  rdfs:domain :Equipment ;
                                  rdfs:range xsd:boolean ;
                                  uml:id "_0B1D0D20-436A-42a0-AD04-DECFCE5CFCF3" ;
                                  rdfs:comment "The equipment is enabled to participate in network analysis.  If unspecified, the value is assumed to be true." ;
                                  rdfs:label "networkAnalysisEnabled" .


###  http://iec.ch/TC57/CIM-generic#Equipment.normallyInService
:Equipment.normallyInService rdf:type owl:DatatypeProperty ,
                                      owl:FunctionalProperty ;
                             rdfs:domain :Equipment ;
                             rdfs:range xsd:boolean ;
                             uml:id "_410CEA04-CA77-46d9-A093-019230A2DE17" ;
                             rdfs:comment "Specifies the availability of the equipment under normal operating conditions. True means the equipment is available for topology processing, which determines if the equipment is energized or not. False means that the equipment is treated by network applications as if it is not in the model." ;
                             rdfs:label "normallyInService" .


###  http://iec.ch/TC57/CIM-generic#IEC61970CIMVersion.date
:IEC61970CIMVersion.date rdf:type owl:DatatypeProperty ,
                                  owl:FunctionalProperty ;
                         rdfs:range xsd:date ;
                         uml:hasInitialValue "2020-08-24" ;
                         uml:id "_8DADB97F-283D-40c7-A25A-D75E4C0D8507" ;
                         rdfs:comment "Form is YYYY-MM-DD for example for January 5, 2009 it is 2009-01-05." ;
                         rdfs:label "date" .


###  http://iec.ch/TC57/CIM-generic#IdentifiedObject.aliasName
:IdentifiedObject.aliasName rdf:type owl:DatatypeProperty ,
                                     owl:FunctionalProperty ;
                            rdfs:domain :IdentifiedObject ;
                            rdfs:range xsd:string ;
                            uml:id "_D4F8B75D-CDAD-4440-8092-1425101E5ABC" ;
                            rdfs:comment """The aliasName is free text human readable name of the object alternative to IdentifiedObject.name. It may be non unique and may not correlate to a naming hierarchy.
The attribute aliasName is retained because of backwards compatibility between CIM relases. It is however recommended to replace aliasName with the Name class as aliasName is planned for retirement at a future time.""" ;
                            rdfs:label "aliasName" .


###  http://iec.ch/TC57/CIM-generic#IdentifiedObject.description
:IdentifiedObject.description rdf:type owl:DatatypeProperty ,
                                       owl:FunctionalProperty ;
                              rdfs:domain :IdentifiedObject ;
                              rdfs:range xsd:string ;
                              uml:id "_13104BE9-CB1E-4dde-9A52-D7EE95DF7B65" ;
                              rdfs:comment "The description is a free human readable text describing or naming the object. It may be non unique and may not correlate to a naming hierarchy." ;
                              rdfs:label "description" .


###  http://iec.ch/TC57/CIM-generic#IdentifiedObject.mRID
:IdentifiedObject.mRID rdf:type owl:DatatypeProperty ,
                                owl:FunctionalProperty ;
                       rdfs:domain :IdentifiedObject ;
                       rdfs:range xsd:string ;
                       uml:id "_C775F80A-A23D-4f38-AB9D-49D1FA882337" ;
                       rdfs:comment """Master resource identifier issued by a model authority. The mRID is unique within an exchange context. Global uniqueness is easily achieved by using a UUID, as specified in RFC 4122, for the mRID. The use of UUID is strongly recommended.
For CIMXML data files in RDF syntax conforming to IEC 61970-552, the mRID is mapped to rdf:ID or rdf:about attributes that identify CIM object elements.""" ;
                       rdfs:label "mRID" .


###  http://iec.ch/TC57/CIM-generic#IdentifiedObject.name
:IdentifiedObject.name rdf:type owl:DatatypeProperty ,
                                owl:FunctionalProperty ;
                       rdfs:domain :IdentifiedObject ;
                       rdfs:range xsd:string ;
                       uml:id "_870F033B-EDA6-4a32-A5AD-47DCBBFE2997" ;
                       rdfs:comment "The name is any free human readable and possibly non unique text naming the object." ;
                       rdfs:label "name" .


###  http://iec.ch/TC57/CIM-generic#Name.name
:Name.name rdf:type owl:DatatypeProperty ,
                    owl:FunctionalProperty ;
           rdfs:domain :Name ;
           rdfs:range xsd:string ;
           uml:id "_A2162B14-022E-4cda-AC84-B9D32A0C6C00" ;
           rdfs:comment "Any free text that name the object." ;
           rdfs:label "name" .


###  http://iec.ch/TC57/CIM-generic#NameType.description
:NameType.description rdf:type owl:DatatypeProperty ,
                               owl:FunctionalProperty ;
                      rdfs:domain :NameType ;
                      rdfs:range xsd:string ;
                      uml:id "_B831899F-A8DB-470e-B41E-AE8F085A6225" ;
                      rdfs:comment "Description of the name type." ;
                      rdfs:label "description" .


###  http://iec.ch/TC57/CIM-generic#NameType.name
:NameType.name rdf:type owl:DatatypeProperty ,
                        owl:FunctionalProperty ;
               rdfs:domain :NameType ;
               rdfs:range xsd:string ;
               uml:id "_EEC57734-55A8-4d7d-BCBB-44785732CBD8" ;
               rdfs:comment "Name of the name type." ;
               rdfs:label "name" .


###  http://iec.ch/TC57/CIM-generic#ProtectedSwitch.breakingCapacity
:ProtectedSwitch.breakingCapacity rdf:type owl:DatatypeProperty ,
                                           owl:FunctionalProperty ;
                                  rdfs:domain :ProtectedSwitch ;
                                  rdfs:range :CurrentFlow ;
                                  uml:id "_52EB29C5-1F53-46e6-84EC-400C4B5AF75F" ;
                                  rdfs:comment "The maximum fault current a breaking device can break safely under prescribed conditions of use." ;
                                  rdfs:label "breakingCapacity" .


###  http://iec.ch/TC57/CIM-generic#Switch.locked
:Switch.locked rdf:type owl:DatatypeProperty ,
                        owl:FunctionalProperty ;
               rdfs:domain :Switch ;
               rdfs:range xsd:boolean ;
               uml:id "_D72B9A82-CD67-425e-AF36-802920CFAF3F" ;
               rdfs:comment """If true, the switch is locked. The resulting switch state is a combination of locked and Switch.open attributes as follows:
<ul>
	<li>locked=true and Switch.open=true. The resulting state is open and locked;</li>
	<li>locked=false and Switch.open=true. The resulting state is open;</li>
	<li>locked=false and Switch.open=false. The resulting state is closed.</li>
</ul>""" ;
               rdfs:label "locked" .


###  http://iec.ch/TC57/CIM-generic#Switch.normalOpen
:Switch.normalOpen rdf:type owl:DatatypeProperty ,
                            owl:FunctionalProperty ;
                   rdfs:domain :Switch ;
                   rdfs:range xsd:boolean ;
                   uml:id "_42C10E32-018C-4f7d-81E1-3687F5A7FCFD" ;
                   rdfs:comment "The attribute is used in cases when no Measurement for the status value is present. If the Switch has a status measurement the Discrete.normalValue is expected to match with the Switch.normalOpen." ;
                   rdfs:label "normalOpen" .


###  http://iec.ch/TC57/CIM-generic#Switch.open
:Switch.open rdf:type owl:DatatypeProperty ,
                      owl:FunctionalProperty ;
             rdfs:domain :Switch ;
             rdfs:range xsd:boolean ;
             uml:id "_7FC100AA-9641-4d45-AC84-8B90D9FC4D3F" ;
             rdfs:comment "The attribute tells if the switch is considered open when used as input to topology processing." ;
             rdfs:label "open" .


###  http://iec.ch/TC57/CIM-generic#Switch.ratedCurrent
:Switch.ratedCurrent rdf:type owl:DatatypeProperty ,
                              owl:FunctionalProperty ;
                     rdfs:domain :Switch ;
                     rdfs:range :CurrentFlow ;
                     uml:id "_486957C7-D5EF-499f-8CE3-7A2E88765D52" ;
                     rdfs:comment """The maximum continuous current carrying capacity in amps governed by the device material and construction.
The attribute shall be a positive value.""" ;
                     rdfs:label "ratedCurrent" .


###  http://iec.ch/TC57/CIM-generic#Switch.retained
:Switch.retained rdf:type owl:DatatypeProperty ,
                          owl:FunctionalProperty ;
                 rdfs:domain :Switch ;
                 rdfs:range xsd:boolean ;
                 uml:id "_5E9C873C-F052-49f6-9247-D7274CDA570A" ;
                 rdfs:comment "Branch is retained in the topological solution.  The flow through retained switches will normally be calculated in power flow." ;
                 rdfs:label "retained" .


###  http://iec.ch/TC57/CIM-generic#Switch.switchOnCount
:Switch.switchOnCount rdf:type owl:DatatypeProperty ,
                               owl:FunctionalProperty ;
                      rdfs:domain :Switch ;
                      rdfs:range xsd:integer ;
                      uml:id "_0FA70685-F30F-4d40-9CA6-65C5C7AC0543" ;
                      rdfs:comment "The switch on count since the switch was last reset or initialized." ;
                      rdfs:label "switchOnCount" .


###  http://iec.ch/TC57/CIM-generic#Switch.switchOnDate
:Switch.switchOnDate rdf:type owl:DatatypeProperty ,
                              owl:FunctionalProperty ;
                     rdfs:domain :Switch ;
                     rdfs:range xsd:dateTime ;
                     uml:id "_49CABBEB-6179-48ca-A1D3-4D45B67C7058" ;
                     rdfs:comment "The date and time when the switch was last switched on." ;
                     rdfs:label "switchOnDate" .


###  http://iec.ch/TC57/CIM-generic#TapChanger.controlEnabled
:TapChanger.controlEnabled rdf:type owl:DatatypeProperty ,
                                    owl:FunctionalProperty ;
                           rdfs:domain :TapChanger ;
                           rdfs:range xsd:boolean ;
                           uml:id "_1BF7B544-61DC-4fd7-9325-E938A8C364C7" ;
                           rdfs:comment "Specifies the regulation status of the equipment.  True is regulating, false is not regulating." ;
                           rdfs:label "controlEnabled" .


###  http://iec.ch/TC57/CIM-generic#TapChanger.highStep
:TapChanger.highStep rdf:type owl:DatatypeProperty ,
                              owl:FunctionalProperty ;
                     rdfs:domain :TapChanger ;
                     rdfs:range xsd:integer ;
                     uml:id "_F3D83CC1-3BD4-4c27-9782-7FB0DDBAED1F" ;
                     rdfs:comment """Highest possible tap step position, advance from neutral.
The attribute shall be greater than lowStep.""" ;
                     rdfs:label "highStep" .


###  http://iec.ch/TC57/CIM-generic#TapChanger.initialDelay
:TapChanger.initialDelay rdf:type owl:DatatypeProperty ,
                                  owl:FunctionalProperty ;
                         rdfs:domain :TapChanger ;
                         rdfs:range :Seconds ;
                         uml:id "_0AA6B766-F046-494b-9390-05BD55E7879C" ;
                         rdfs:comment "For an LTC, the delay for initial tap changer operation (first step change)." ;
                         rdfs:label "initialDelay" .


###  http://iec.ch/TC57/CIM-generic#TapChanger.lowStep
:TapChanger.lowStep rdf:type owl:DatatypeProperty ,
                             owl:FunctionalProperty ;
                    rdfs:domain :TapChanger ;
                    rdfs:range xsd:integer ;
                    uml:id "_E72756C9-A9EA-41fb-9523-A9E5EC65C109" ;
                    rdfs:comment "Lowest possible tap step position, retard from neutral." ;
                    rdfs:label "lowStep" .


###  http://iec.ch/TC57/CIM-generic#TapChanger.ltcFlag
:TapChanger.ltcFlag rdf:type owl:DatatypeProperty ,
                             owl:FunctionalProperty ;
                    rdfs:domain :TapChanger ;
                    rdfs:range xsd:boolean ;
                    uml:id "_DA8B32CA-3C0B-4913-8EED-F08BF2818AFD" ;
                    rdfs:comment "Specifies whether or not a TapChanger has load tap changing capabilities." ;
                    rdfs:label "ltcFlag" .


###  http://iec.ch/TC57/CIM-generic#TapChanger.neutralStep
:TapChanger.neutralStep rdf:type owl:DatatypeProperty ,
                                 owl:FunctionalProperty ;
                        rdfs:domain :TapChanger ;
                        rdfs:range xsd:integer ;
                        uml:id "_AEF6801E-342A-4a1f-ADC6-C7DAFFED61BC" ;
                        rdfs:comment """The neutral tap step position for this winding.
The attribute shall be equal to or greater than lowStep and equal or less than highStep.
It is the step position where the voltage is neutralU when the other terminals of the transformer are at the ratedU.  If there are other tap changers on the transformer those taps are kept constant at their neutralStep.""" ;
                        rdfs:label "neutralStep" .


###  http://iec.ch/TC57/CIM-generic#TapChanger.neutralU
:TapChanger.neutralU rdf:type owl:DatatypeProperty ,
                              owl:FunctionalProperty ;
                     rdfs:domain :TapChanger ;
                     rdfs:range :Voltage ;
                     uml:id "_773D3CD1-ED8D-4b55-9D8B-93CFB1E9F5B3" ;
                     rdfs:comment """Voltage at which the winding operates at the neutral tap setting. It is the voltage at the terminal of the PowerTransformerEnd associated with the tap changer when all tap changers on the transformer are at their neutralStep position.  Normally neutralU of the tap changer is the same as ratedU of the PowerTransformerEnd, but it can differ in special cases such as when the tapping mechanism is separate from the winding more common on lower voltage transformers.
This attribute is not relevant for PhaseTapChangerAsymmetrical, PhaseTapChangerSymmetrical and PhaseTapChangerLinear.""" ;
                     rdfs:label "neutralU" .


###  http://iec.ch/TC57/CIM-generic#TapChanger.normalStep
:TapChanger.normalStep rdf:type owl:DatatypeProperty ,
                                owl:FunctionalProperty ;
                       rdfs:domain :TapChanger ;
                       rdfs:range xsd:integer ;
                       uml:id "_A0388C6D-808F-4546-A960-9D73692E7B0B" ;
                       rdfs:comment """The tap step position used in \"normal\" network operation for this winding. For a \"Fixed\" tap changer indicates the current physical tap setting.
The attribute shall be equal to or greater than lowStep and equal to or less than highStep.""" ;
                       rdfs:label "normalStep" .


###  http://iec.ch/TC57/CIM-generic#TapChanger.step
:TapChanger.step rdf:type owl:DatatypeProperty ,
                          owl:FunctionalProperty ;
                 rdfs:domain :TapChanger ;
                 rdfs:range xsd:float ;
                 uml:id "_2FA251C7-BB3A-4cf7-9BC7-316171AED7CB" ;
                 rdfs:comment """Tap changer position.
Starting step for a steady state solution. Non integer values are allowed to support continuous tap variables. The reasons for continuous value are to support study cases where no discrete tap changer has yet been designed, a solution where a narrow voltage band forces the tap step to oscillate or to accommodate for a continuous solution as input.
The attribute shall be equal to or greater than lowStep and equal to or less than highStep.""" ;
                 rdfs:label "step" .


###  http://iec.ch/TC57/CIM-generic#TapChanger.subsequentDelay
:TapChanger.subsequentDelay rdf:type owl:DatatypeProperty ,
                                     owl:FunctionalProperty ;
                            rdfs:domain :TapChanger ;
                            rdfs:range :Seconds ;
                            uml:id "_4F65DA6B-7334-4903-AA61-23253E9E5FE6" ;
                            rdfs:comment "For an LTC, the delay for subsequent tap changer operation (second and later step changes)." ;
                            rdfs:label "subsequentDelay" .


###  http://iec.ch/TC57/CIM-generic#VoltageLevel.highVoltageLimit
:VoltageLevel.highVoltageLimit rdf:type owl:DatatypeProperty ,
                                        owl:FunctionalProperty ;
                               rdfs:domain :VoltageLevel ;
                               rdfs:range :Voltage ;
                               uml:id "_D1BAD493-B22A-497f-B6A6-CDFDF46EA012" ;
                               rdfs:comment """The bus bar's high voltage limit.
The limit applies to all equipment and nodes contained in a given VoltageLevel. It is not required that it is exchanged in pair with lowVoltageLimit. It is preferable to use operational VoltageLimit, which prevails, if present.""" ;
                               rdfs:label "highVoltageLimit" .


###  http://iec.ch/TC57/CIM-generic#VoltageLevel.lowVoltageLimit
:VoltageLevel.lowVoltageLimit rdf:type owl:DatatypeProperty ,
                                       owl:FunctionalProperty ;
                              rdfs:domain :VoltageLevel ;
                              rdfs:range :Voltage ;
                              uml:id "_EB17FEAC-CDBA-4bbd-B45E-86D3EA333C08" ;
                              rdfs:comment """The bus bar's low voltage limit.
The limit applies to all equipment and nodes contained in a given VoltageLevel. It is not required that it is exchanged in pair with highVoltageLimit. It is preferable to use operational VoltageLimit, which prevails, if present.""" ;
                              rdfs:label "lowVoltageLimit" .


#################################################################
#    Classes
#################################################################

###  http://iec.ch/TC57/CIM-generic#ACDCTerminal
:ACDCTerminal rdf:type owl:Class ;
              rdfs:subClassOf :IdentifiedObject ;
              uml:id "_D37077B9-3B0C-4c16-8F5F-9A6F2C83A7F2" ;
              rdfs:comment "An electrical connection point (AC or DC) to a piece of conducting equipment. Terminals are connected at physical connection points called connectivity nodes." ;
              rdfs:label "ACDCTerminal" .


###  http://iec.ch/TC57/CIM-generic#BaseFrequency
:BaseFrequency rdf:type owl:Class ;
               rdfs:subClassOf :IdentifiedObject ;
               uml:id "_2FA6A39A-A920-4ab7-92DC-D005DDDBB348" ;
               rdfs:comment "The BaseFrequency class describes a base frequency for a power system network. In case of multiple power networks with different frequencies, e.g. 50 Hz or 60 Hz each network will have its own base frequency class. Hence it is assumed that power system objects having different base frequencies appear in separate documents where each document has a single base frequency instance." ;
               rdfs:label "BaseFrequency" .


###  http://iec.ch/TC57/CIM-generic#BasePower
:BasePower rdf:type owl:Class ;
           rdfs:subClassOf :IdentifiedObject ;
           uml:id "_A10836E5-09FC-4862-B3C3-96D52298E21B" ;
           rdfs:comment "The BasePower class defines the base power used in the per unit calculations." ;
           rdfs:label "BasePower" .


###  http://iec.ch/TC57/CIM-generic#BaseVoltage
:BaseVoltage rdf:type owl:Class ;
             rdfs:subClassOf :IdentifiedObject ;
             uml:id "_2E70DC9D-AEAE-46cc-B20A-C20A636AE9B0" ;
             rdfs:comment "Defines a system base voltage which is referenced." ;
             rdfs:label "BaseVoltage" .


###  http://iec.ch/TC57/CIM-generic#Bay
:Bay rdf:type owl:Class ;
     rdfs:subClassOf :EquipmentContainer ;
     uml:id "_45910062-D4E8-40ee-99EB-FEC14DD9FAB0" ;
     rdfs:comment "A collection of power system resources (within a given substation) including conducting equipment, protection relays, measurements, and telemetry.  A bay typically represents a physical grouping related to modularization of equipment." ;
     rdfs:label "Bay" .


###  http://iec.ch/TC57/CIM-generic#Breaker
:Breaker rdf:type owl:Class ;
         rdfs:subClassOf :ProtectedSwitch ;
         uml:id "_380D92AA-1D80-4e84-A8EE-843DACEB59DD" ;
         rdfs:comment "A mechanical switching device capable of making, carrying, and breaking currents under normal circuit conditions and also making, carrying for a specified time, and breaking currents under specified abnormal circuit conditions e.g.  those of short circuit." ;
         rdfs:label "Breaker" .


###  http://iec.ch/TC57/CIM-generic#ConductingEquipment
:ConductingEquipment rdf:type owl:Class ;
                     rdfs:subClassOf :Equipment ;
                     uml:id "_7C5F19FB-5253-430c-8E53-BDCF7EBCE4C1" ;
                     rdfs:comment "The parts of the AC power system that are designed to carry current or that are conductively connected through terminals." ;
                     rdfs:label "ConductingEquipment" .


###  http://iec.ch/TC57/CIM-generic#ConnectivityNode
:ConnectivityNode rdf:type owl:Class ;
                  rdfs:subClassOf :IdentifiedObject ;
                  uml:id "_8BCACC36-B2DD-4c2a-A2AE-CFDF43731FC2" ;
                  rdfs:comment "Connectivity nodes are points where terminals of AC conducting equipment are connected together with zero impedance." ;
                  rdfs:label "ConnectivityNode" .


###  http://iec.ch/TC57/CIM-generic#ConnectivityNodeContainer
:ConnectivityNodeContainer rdf:type owl:Class ;
                           rdfs:subClassOf :PowerSystemResource ;
                           uml:id "_B985C03E-46A3-4aec-B5B6-FDD983EBE621" ;
                           rdfs:comment "A base class for all objects that may contain connectivity nodes or topological nodes." ;
                           rdfs:label "ConnectivityNodeContainer" .


###  http://iec.ch/TC57/CIM-generic#Equipment
:Equipment rdf:type owl:Class ;
           rdfs:subClassOf :PowerSystemResource ;
           uml:id "_F8DD8DAC-3545-4660-9CA5-794881CC6591" ;
           rdfs:comment "The parts of a power system that are physical devices, electronic or mechanical." ;
           rdfs:label "Equipment" .


###  http://iec.ch/TC57/CIM-generic#EquipmentContainer
:EquipmentContainer rdf:type owl:Class ;
                    rdfs:subClassOf :ConnectivityNodeContainer ;
                    uml:id "_F465B7B4-B488-46c5-8D05-8036F09A03A0" ;
                    rdfs:comment "A modelling construct to provide a root class for containing equipment." ;
                    rdfs:label "EquipmentContainer" .


###  http://iec.ch/TC57/CIM-generic#EquivalentNetwork
:EquivalentNetwork rdf:type owl:Class ;
                   rdfs:subClassOf :ConnectivityNodeContainer ;
                   uml:id "_1FCEE6DF-2D36-4ee8-8CB9-0EFC3F000799" ;
                   rdfs:comment "A class that groups electrical equivalents, including internal nodes, of a network that has been reduced. The ConnectivityNodes contained in the equivalent are intended to reflect internal nodes of the equivalent. The boundary Connectivity nodes where the equivalent connects outside itself are not contained by the equivalent." ;
                   rdfs:label "EquivalentNetwork" .


###  http://iec.ch/TC57/CIM-generic#GeographicalRegion
:GeographicalRegion rdf:type owl:Class ;
                    rdfs:subClassOf :IdentifiedObject ;
                    uml:id "_F935232D-65FF-4720-BAFB-50639B7CA0AB" ;
                    rdfs:comment "A geographical region of a power system network model." ;
                    rdfs:label "GeographicalRegion" .


###  http://iec.ch/TC57/CIM-generic#IdentifiedObject
:IdentifiedObject rdf:type owl:Class ;
                  uml:id "_055C5806-E9D8-4a7a-9307-DAF7C31763C7" ;
                  rdfs:comment "This is a root class to provide common identification for all classes needing identification and naming attributes." ;
                  rdfs:label "IdentifiedObject" .


###  http://iec.ch/TC57/CIM-generic#Line
:Line rdf:type owl:Class ;
      rdfs:subClassOf :EquipmentContainer ;
      uml:id "_43D9D2B8-DA1E-45c4-B99D-EC28FCAB742B" ;
      rdfs:comment "Contains equipment beyond a substation belonging to a power transmission line." ;
      rdfs:label "Line" .


###  http://iec.ch/TC57/CIM-generic#Name
:Name rdf:type owl:Class ;
      uml:id "_D6F3DF4E-3363-48d2-AB61-7872E337C422" ;
      rdfs:comment "The Name class provides the means to define any number of human readable  names for an object. A name is <b>not</b> to be used for defining inter-object relationships. For inter-object relationships instead use the object identification 'mRID'." ;
      rdfs:label "Name" .


###  http://iec.ch/TC57/CIM-generic#NameType
:NameType rdf:type owl:Class ;
          uml:id "_666F94BF-13E3-4947-830F-3A2D4E7CC9FC" ;
          rdfs:comment """Type of name. Possible values for attribute 'name' are implementation dependent but standard profiles may specify types. An enterprise may have multiple IT systems each having its own local name for the same object, e.g. a planning system may have different names from an EMS. An object may also have different names within the same IT system, e.g. localName as defined in CIM version 14. The definition from CIM14 is:
The localName is a human readable name of the object. It is a free text name local to a node in a naming hierarchy similar to a file directory structure. A power system related naming hierarchy may be: Substation, VoltageLevel, Equipment etc. Children of the same parent in such a hierarchy have names that typically are unique among them.""" ;
          rdfs:label "NameType" .


###  http://iec.ch/TC57/CIM-generic#PSRType
:PSRType rdf:type owl:Class ;
         rdfs:subClassOf :IdentifiedObject ;
         uml:id "_CF59539F-A910-4af6-A84D-A52BBA7300CB" ;
         rdfs:comment "Classifying instances of the same class, e.g. overhead and underground ACLineSegments. This classification mechanism is intended to provide flexibility outside the scope of this document, i.e. provide customisation that is non standard." ;
         rdfs:label "PSRType" .


###  http://iec.ch/TC57/CIM-generic#PhaseCode
:PhaseCode rdf:type owl:Class ;
           uml:id "_3687AEED-A1B1-4557-899E-5985D184FCE9" ;
           rdfs:comment """An unordered enumeration of phase identifiers.  Allows designation of phases for both transmission and distribution equipment, circuits and loads.   The enumeration, by itself, does not describe how the phases are connected together or connected to ground.  Ground is not explicitly denoted as a phase.
Residential and small commercial loads are often served from single-phase, or split-phase, secondary circuits. For the example of s12N, phases 1 and 2 refer to hot wires that are 180 degrees out of phase, while N refers to the neutral wire. Through single-phase transformer connections, these secondary circuits may be served from one or two of the primary phases A, B, and C. For three-phase loads, use the A, B, C phase codes instead of s12N.
The integer values are from IEC 61968-9 to support revenue metering applications.""" ;
           rdfs:label "PhaseCode" .


###  http://iec.ch/TC57/CIM-generic#PowerSystemResource
:PowerSystemResource rdf:type owl:Class ;
                     rdfs:subClassOf :IdentifiedObject ;
                     uml:id "_0340C084-3759-40cc-AAF2-386101DE842F" ;
                     rdfs:comment "A power system resource (PSR) can be an item of equipment such as a switch, an equipment container containing many individual items of equipment such as a substation, or an organisational entity such as sub-control area. Power system resources can have measurements associated." ;
                     rdfs:label "PowerSystemResource" .


###  http://iec.ch/TC57/CIM-generic#ProtectedSwitch
:ProtectedSwitch rdf:type owl:Class ;
                 rdfs:subClassOf :Switch ;
                 uml:id "_BADE2A18-37F4-49bf-87BC-A087E4D2E4F7" ;
                 rdfs:comment "A ProtectedSwitch is a switching device that can be operated by ProtectionEquipment." ;
                 rdfs:label "ProtectedSwitch" .


###  http://iec.ch/TC57/CIM-generic#SubGeographicalRegion
:SubGeographicalRegion rdf:type owl:Class ;
                       rdfs:subClassOf :IdentifiedObject ;
                       uml:id "_D3CE44CA-5AED-484b-92A3-89F156425204" ;
                       rdfs:comment "A subset of a geographical region of a power system network model." ;
                       rdfs:label "SubGeographicalRegion" .


###  http://iec.ch/TC57/CIM-generic#Substation
:Substation rdf:type owl:Class ;
            rdfs:subClassOf :EquipmentContainer ;
            uml:id "_D8A14AC5-D17B-4d42-8F12-1B674E5D12D7" ;
            rdfs:comment "A collection of equipment for purposes other than generation or utilization, through which electric energy in bulk is passed for the purposes of switching or modifying its characteristics." ;
            rdfs:label "Substation" .


###  http://iec.ch/TC57/CIM-generic#Switch
:Switch rdf:type owl:Class ;
        rdfs:subClassOf :ConductingEquipment ;
        uml:id "_ACE2DDBB-536E-489a-A3A8-22589256302D" ;
        rdfs:comment "A generic device designed to close, or open, or both, one or more electric circuits.  All switches are two terminal devices including grounding switches. The ACDCTerminal.connected at the two sides of the switch shall not be considered for assessing switch connectivity, i.e. only Switch.open, .normalOpen and .locked are relevant." ;
        rdfs:label "Switch" .


###  http://iec.ch/TC57/CIM-generic#TapChanger
:TapChanger rdf:type owl:Class ;
            rdfs:subClassOf :PowerSystemResource ;
            uml:id "_F43099C0-90EA-47f1-B038-EDE831744C07" ;
            rdfs:comment "Mechanism for changing transformer winding tap positions." ;
            rdfs:label "TapChanger" .


###  http://iec.ch/TC57/CIM-generic#Terminal
:Terminal rdf:type owl:Class ;
          rdfs:subClassOf :ACDCTerminal ;
          uml:id "_1A0F8321-5E77-4d68-BE29-B36FA31549DC" ;
          rdfs:comment "An AC electrical connection point to a piece of conducting equipment. Terminals are connected at physical connection points called connectivity nodes." ;
          rdfs:label "Terminal" .


###  http://iec.ch/TC57/CIM-generic#VoltageLevel
:VoltageLevel rdf:type owl:Class ;
              rdfs:subClassOf :EquipmentContainer ;
              uml:id "_B147BAEA-7339-406b-A8C3-47F85EA0E82A" ;
              rdfs:comment "A collection of equipment at one common system voltage forming a switchgear. The equipment typically consists of breakers, busbars, instrumentation, control, regulation and protection devices as well as assemblies of all these." ;
              rdfs:label "VoltageLevel" .


#################################################################
#    Individuals
#################################################################

###  http://iec.ch/TC57/CIM-generic#PhaseCode.A
:PhaseCode.A rdf:type owl:NamedIndividual ,
                      :PhaseCode ;
             uml:hasInitialValue "128" ;
             uml:id "_EA5174F8-A73C-4f4b-96AA-54EAFB16BC9F" ;
             rdfs:comment "Phase A." ;
             rdfs:label "A" .


###  http://iec.ch/TC57/CIM-generic#PhaseCode.AB
:PhaseCode.AB rdf:type owl:NamedIndividual ,
                       :PhaseCode ;
              uml:hasInitialValue "132" ;
              uml:id "_77216F5E-3863-424c-91CD-4597AE97B61E" ;
              rdfs:comment "Phases A and B." ;
              rdfs:label "AB" .


###  http://iec.ch/TC57/CIM-generic#PhaseCode.ABC
:PhaseCode.ABC rdf:type owl:NamedIndividual ,
                        :PhaseCode ;
               uml:hasInitialValue "224" ;
               uml:id "_5A6F7D82-6A2C-4eb3-90BC-8F77AAD9D50F" ;
               rdfs:comment "Phases A, B, and C." ;
               rdfs:label "ABC" .


###  http://iec.ch/TC57/CIM-generic#PhaseCode.ABCN
:PhaseCode.ABCN rdf:type owl:NamedIndividual ,
                         :PhaseCode ;
                uml:hasInitialValue "225" ;
                uml:id "_8E38EE25-FD5C-4b01-938C-008998EDA526" ;
                rdfs:comment "Phases A, B, C, and N." ;
                rdfs:label "ABCN" .


###  http://iec.ch/TC57/CIM-generic#PhaseCode.ABN
:PhaseCode.ABN rdf:type owl:NamedIndividual ,
                        :PhaseCode ;
               uml:hasInitialValue "193" ;
               uml:id "_C5F9ED62-CB15-4c15-98DB-6593686F63E2" ;
               rdfs:comment "Phases A, B, and neutral." ;
               rdfs:label "ABN" .


###  http://iec.ch/TC57/CIM-generic#PhaseCode.AC
:PhaseCode.AC rdf:type owl:NamedIndividual ,
                       :PhaseCode ;
              uml:hasInitialValue "96" ;
              uml:id "_598C4480-5C39-4889-8BD1-D1D2BCEB4DEA" ;
              rdfs:comment "Phases A and C." ;
              rdfs:label "AC" .


###  http://iec.ch/TC57/CIM-generic#PhaseCode.ACN
:PhaseCode.ACN rdf:type owl:NamedIndividual ,
                        :PhaseCode ;
               uml:hasInitialValue "41" ;
               uml:id "_0396E7F5-6112-49e7-A7C8-7B7FA0214AA7" ;
               rdfs:comment "Phases A, C and neutral." ;
               rdfs:label "ACN" .


###  http://iec.ch/TC57/CIM-generic#PhaseCode.AN
:PhaseCode.AN rdf:type owl:NamedIndividual ,
                       :PhaseCode ;
              uml:hasInitialValue "129" ;
              uml:id "_9B41A289-EDF6-4728-AABE-B11D2E617549" ;
              rdfs:comment "Phases A and neutral." ;
              rdfs:label "AN" .


###  http://iec.ch/TC57/CIM-generic#PhaseCode.B
:PhaseCode.B rdf:type owl:NamedIndividual ,
                      :PhaseCode ;
             uml:hasInitialValue "64" ;
             uml:id "_DF516C67-D4FE-4a6b-9FE7-54E54036C7CA" ;
             rdfs:comment "Phase B." ;
             rdfs:label "B" .


###  http://iec.ch/TC57/CIM-generic#PhaseCode.BC
:PhaseCode.BC rdf:type owl:NamedIndividual ,
                       :PhaseCode ;
              uml:hasInitialValue "66" ;
              uml:id "_8124AC36-FD4D-4b64-A414-6F9B8D350469" ;
              rdfs:comment "Phases B and C." ;
              rdfs:label "BC" .


###  http://iec.ch/TC57/CIM-generic#PhaseCode.BCN
:PhaseCode.BCN rdf:type owl:NamedIndividual ,
                        :PhaseCode ;
               uml:hasInitialValue "97" ;
               uml:id "_F494A423-E865-4c3d-8C83-180728F30A66" ;
               rdfs:comment "Phases B, C, and neutral." ;
               rdfs:label "BCN" .


###  http://iec.ch/TC57/CIM-generic#PhaseCode.BN
:PhaseCode.BN rdf:type owl:NamedIndividual ,
                       :PhaseCode ;
              uml:hasInitialValue "65" ;
              uml:id "_2780D899-5467-4920-8DAA-117051620D3A" ;
              rdfs:comment "Phases B and neutral." ;
              rdfs:label "BN" .


###  http://iec.ch/TC57/CIM-generic#PhaseCode.C
:PhaseCode.C rdf:type owl:NamedIndividual ,
                      :PhaseCode ;
             uml:hasInitialValue "32" ;
             uml:id "_8E5E8952-BD3F-4b06-A218-7A1EE85598D0" ;
             rdfs:comment "Phase C." ;
             rdfs:label "C" .


###  http://iec.ch/TC57/CIM-generic#PhaseCode.CN
:PhaseCode.CN rdf:type owl:NamedIndividual ,
                       :PhaseCode ;
              uml:hasInitialValue "33" ;
              uml:id "_DEB66611-AEAD-4b57-8CBD-65D1931709CE" ;
              rdfs:comment "Phases C and neutral." ;
              rdfs:label "CN" .


###  http://iec.ch/TC57/CIM-generic#PhaseCode.N
:PhaseCode.N rdf:type owl:NamedIndividual ,
                      :PhaseCode ;
             uml:hasInitialValue "16" ;
             uml:id "_177D92A8-237D-4ec7-99BF-6BBE2AA2CE9E" ;
             rdfs:comment "Neutral phase." ;
             rdfs:label "N" .


###  http://iec.ch/TC57/CIM-generic#PhaseCode.X
:PhaseCode.X rdf:type owl:NamedIndividual ,
                      :PhaseCode ;
             uml:hasInitialValue "1024" ;
             uml:id "_18C21147-5A05-4e89-857C-07DED480CDD7" ;
             rdfs:comment "Unknown non-neutral phase." ;
             rdfs:label "X" .


###  http://iec.ch/TC57/CIM-generic#PhaseCode.XN
:PhaseCode.XN rdf:type owl:NamedIndividual ,
                       :PhaseCode ;
              uml:hasInitialValue "1040" ;
              uml:id "_C97339FF-B1B1-4b27-9F89-F1224B83DFCD" ;
              rdfs:comment "Unknown non-neutral phase plus neutral." ;
              rdfs:label "XN" .


###  http://iec.ch/TC57/CIM-generic#PhaseCode.XY
:PhaseCode.XY rdf:type owl:NamedIndividual ,
                       :PhaseCode ;
              uml:hasInitialValue "3072" ;
              uml:id "_88204DE0-8923-4886-8C42-955E3147E39B" ;
              rdfs:comment "Two unknown non-neutral phases." ;
              rdfs:label "XY" .


###  http://iec.ch/TC57/CIM-generic#PhaseCode.XYN
:PhaseCode.XYN rdf:type owl:NamedIndividual ,
                        :PhaseCode ;
               uml:hasInitialValue "3088" ;
               uml:id "_BE6C0B89-4F67-41fa-B56D-1195F07B82E0" ;
               rdfs:comment "Two unknown non-neutral phases plus neutral." ;
               rdfs:label "XYN" .


###  http://iec.ch/TC57/CIM-generic#PhaseCode.none
:PhaseCode.none rdf:type owl:NamedIndividual ,
                         :PhaseCode ;
                uml:hasInitialValue "0" ;
                uml:id "_39811306-A5CF-49f9-9D71-313B1B5BC519" ;
                rdfs:comment "No phases specified." ;
                rdfs:label "none" .


###  http://iec.ch/TC57/CIM-generic#PhaseCode.s1
:PhaseCode.s1 rdf:type owl:NamedIndividual ,
                       :PhaseCode ;
              uml:hasInitialValue "512" ;
              uml:id "_50FB82A9-B3F5-4a7b-AF43-2EC84E06D953" ;
              rdfs:comment "Secondary phase 1." ;
              rdfs:label "s1" .


###  http://iec.ch/TC57/CIM-generic#PhaseCode.s12
:PhaseCode.s12 rdf:type owl:NamedIndividual ,
                        :PhaseCode ;
               uml:hasInitialValue "768" ;
               uml:id "_939E2E11-8FE6-4d66-A048-8F990F9BEBF6" ;
               rdfs:comment "Secondary phase 1 and 2." ;
               rdfs:label "s12" .


###  http://iec.ch/TC57/CIM-generic#PhaseCode.s12N
:PhaseCode.s12N rdf:type owl:NamedIndividual ,
                         :PhaseCode ;
                uml:hasInitialValue "784" ;
                uml:id "_2E31EA79-AFF2-45bf-82E3-DD2DD070FDB6" ;
                rdfs:comment "Secondary phases 1, 2, and neutral." ;
                rdfs:label "s12N" .


###  http://iec.ch/TC57/CIM-generic#PhaseCode.s1N
:PhaseCode.s1N rdf:type owl:NamedIndividual ,
                        :PhaseCode ;
               uml:hasInitialValue "528" ;
               uml:id "_7CBBF307-75C0-4255-B181-0BB16E0B4A23" ;
               rdfs:comment "Secondary phase 1 and neutral." ;
               rdfs:label "s1N" .


###  http://iec.ch/TC57/CIM-generic#PhaseCode.s2
:PhaseCode.s2 rdf:type owl:NamedIndividual ,
                       :PhaseCode ;
              uml:hasInitialValue "256" ;
              uml:id "_DD0F804D-9672-4043-8B7A-9937AC0C3BAB" ;
              rdfs:comment "Secondary phase 2." ;
              rdfs:label "s2" .


###  http://iec.ch/TC57/CIM-generic#PhaseCode.s2N
:PhaseCode.s2N rdf:type owl:NamedIndividual ,
                        :PhaseCode ;
               uml:hasInitialValue "272" ;
               uml:id "_16119B57-3431-4045-A8EB-1618E844A397" ;
               rdfs:comment "Secondary phase 2 and neutral." ;
               rdfs:label "s2N" .


#################################################################
#    Annotations
#################################################################

:ADSInstructionTypeCommitment.SHUT_DOWN uml:id "_84E9D518-0EF0-4c46-860D-BAE56EBC1837" ;
                                        rdfs:label "SHUT_DOWN" .


:ADSInstructionTypeCommitment.START_UP uml:id "_5486F5C0-B53D-432f-8564-363A0F7FEFD4" ;
                                       rdfs:label "START_UP" .


:ADSInstructionTypeOOS.FIXED_CONSTRAINT uml:id "_E27B575E-604C-4bdc-818C-BC4B914DFFA0" ;
                                        rdfs:label "FIXED_CONSTRAINT" .


:ADSInstructionTypeOOS.MAX_CONSTRAINT uml:id "_F11340C3-A991-4c3d-ACEB-467D35AB5870" ;
                                      rdfs:label "MAX_CONSTRAINT" .


:ADSInstructionTypeOOS.MIN_CONSTRAINT uml:id "_0D13000E-6938-4252-AF6F-4F41031EA7DF" ;
                                      rdfs:label "MIN_CONSTRAINT" .


:ASTMStandardEditionKind._00_2005_ uml:id "_8E71FBCF-DBF3-49c9-9967-26454CD26F66" ;
                                   rdfs:comment "00(2005) standard edition." ;
                                   rdfs:label "00(2005)" .


:ASTMStandardEditionKind._00_2005_e1 uml:id "_492864FA-7E00-459c-82D4-6CF125C1B384" ;
                                     rdfs:comment "00(2005)e1 standard edition." ;
                                     rdfs:label "00(2005)e1" .


:ASTMStandardEditionKind._00_2010_ uml:id "_7E2BEAC7-1B86-44ac-A426-5360F245151C" ;
                                   rdfs:comment "00(2010) standard edition." ;
                                   rdfs:label "00(2010)" .


:ASTMStandardEditionKind._01 uml:id "_B80D7E77-038B-4f86-AAC6-C26DCFCDFE63" ;
                             rdfs:comment "01 standard edition." ;
                             rdfs:label "01" .


:ASTMStandardEditionKind._01a_2007_ uml:id "_D1459C58-520F-4614-8A84-D4BA20088BC4" ;
                                    rdfs:comment "01a(2007) standard edition." ;
                                    rdfs:label "01a(2007)" .


:ASTMStandardEditionKind._01e1 uml:id "_547CACFA-AE53-445c-9706-44F26B1B69BA" ;
                               rdfs:comment "01e1 standard edition." ;
                               rdfs:label "01e1" .


:ASTMStandardEditionKind._02 uml:id "_CC5B70F3-1A65-496b-827B-38CD5CC54FD1" ;
                             rdfs:comment "02 standard edition." ;
                             rdfs:label "02" .


:ASTMStandardEditionKind._02_2007_ uml:id "_D05C679E-3ABF-4e5e-AEDE-AD8A2352FA14" ;
                                   rdfs:comment "02(2007) standard edition." ;
                                   rdfs:label "02(2007)" .


:ASTMStandardEditionKind._02_2008_ uml:id "_4695E6BF-1D27-4155-B014-D7756AC3DF35" ;
                                   rdfs:comment "02(2008) standard edition." ;
                                   rdfs:label "02(2008)" .


:ASTMStandardEditionKind._02_2009_ uml:id "_72AFF8DB-D2C3-425a-AC88-EC736CAE706F" ;
                                   rdfs:comment "02(2009) standard edition." ;
                                   rdfs:label "02(2009)" .


:ASTMStandardEditionKind._02_2012_ uml:id "_499EA67F-E4A1-4bc5-B6EF-620DACE97DD5" ;
                                   rdfs:comment "02(2012) standard edition." ;
                                   rdfs:label "02(2012)" .


:ASTMStandardEditionKind._02_2014_ uml:id "_6D8F26A3-CC28-42ab-BC5D-D3F637E641E7" ;
                                   rdfs:comment "02(2014) standard edition." ;
                                   rdfs:label "02(2014)" .


:ASTMStandardEditionKind._02a uml:id "_24756ABA-07F2-4b85-ABE4-B037FF6EFB73" ;
                              rdfs:comment "02a standard edition." ;
                              rdfs:label "02a" .


:ASTMStandardEditionKind._02b uml:id "_CF915DA3-500B-49bf-8411-21ECA901E6BD" ;
                              rdfs:comment "02b standard edition." ;
                              rdfs:label "02b" .


:ASTMStandardEditionKind._02e1 uml:id "_DAB74175-5F48-468e-94C7-D07EA3386A4E" ;
                               rdfs:comment "02e1 standard edition." ;
                               rdfs:label "02e1" .


:ASTMStandardEditionKind._03 uml:id "_1284187C-0C77-48ec-B47B-1E78F816FEE3" ;
                             rdfs:comment "03 standard edition." ;
                             rdfs:label "03" .


:ASTMStandardEditionKind._03_2008_ uml:id "_0BE5F928-B640-4f9d-A293-393DE4A7BC81" ;
                                   rdfs:comment "03(2008) standard edition." ;
                                   rdfs:label "03(2008)" .


:ASTMStandardEditionKind._03_2014_ uml:id "_304E5600-257A-4878-9934-C0A163F9FC43" ;
                                   rdfs:comment "03(2014) standard edition." ;
                                   rdfs:label "03(2014)" .


:ASTMStandardEditionKind._03a uml:id "_7D20D562-285D-4fd5-84E5-20E663410634" ;
                              rdfs:comment "03a standard edition." ;
                              rdfs:label "03a" .


:ASTMStandardEditionKind._04 uml:id "_92CB997D-36E8-46b0-BE5E-63CD43DA85C6" ;
                             rdfs:comment "04 standard edition." ;
                             rdfs:label "04" .


:ASTMStandardEditionKind._04a uml:id "_4E9AF060-E2DD-4a32-8253-616C0C300719" ;
                              rdfs:comment "04a standard edition." ;
                              rdfs:label "04a" .


:ASTMStandardEditionKind._04ae1 uml:id "_60F1113C-C74C-4d74-A692-EC9884AC541C" ;
                                rdfs:comment "04ae1 standard edition." ;
                                rdfs:label "04ae1" .


:ASTMStandardEditionKind._04e1 uml:id "_4C1FDD18-DF21-4c2e-A4FC-8A5194F66313" ;
                               rdfs:comment "04e1 standard edition." ;
                               rdfs:label "04e1" .


:ASTMStandardEditionKind._04e2 uml:id "_0F5E2528-E2ED-47d1-9DE2-E792C46E74D3" ;
                               rdfs:comment "04e2 standard edition." ;
                               rdfs:label "04e2" .


:ASTMStandardEditionKind._05 uml:id "_E692974C-6BFB-432e-97E5-D4F5853FAB52" ;
                             rdfs:comment "05 standard edition." ;
                             rdfs:label "05" .


:ASTMStandardEditionKind._05_2010_ uml:id "_FC587458-2610-4269-86E0-00C3A70D4172" ;
                                   rdfs:comment "05(2010) standard edition." ;
                                   rdfs:label "05(2010)" .


:ASTMStandardEditionKind._05a uml:id "_D1DCB59F-D6F7-422b-A6A7-8514A321E743" ;
                              rdfs:comment "05a standard edition." ;
                              rdfs:label "05a" .


:ASTMStandardEditionKind._05a_2010_ uml:id "_F8553908-77C2-4fe0-9DC2-5AD71584CCEB" ;
                                    rdfs:comment "05a(2010) standard edition." ;
                                    rdfs:label "05a(2010)" .


:ASTMStandardEditionKind._06 uml:id "_0C86EFCA-781B-4a7f-9D5F-11D70F12E1A1" ;
                             rdfs:comment "06 standard edition." ;
                             rdfs:label "06" .


:ASTMStandardEditionKind._07 uml:id "_BAACED6C-A32A-4850-BA14-618BA6F80790" ;
                             rdfs:comment "07 standard edition." ;
                             rdfs:label "07" .


:ASTMStandardEditionKind._07_2013_ uml:id "_2D8A66F7-8686-45cb-BE7B-8AF068F25471" ;
                                   rdfs:comment "07(2013) standard edition." ;
                                   rdfs:label "07(2013)" .


:ASTMStandardEditionKind._08 uml:id "_3748265A-FDA0-40b0-91F1-7876AA50A586" ;
                             rdfs:comment "08 standard edition." ;
                             rdfs:label "08" .


:ASTMStandardEditionKind._08e1 uml:id "_0F2B9507-6F2B-482b-9537-610A11AC6082" ;
                               rdfs:comment "08e1 standard edition." ;
                               rdfs:label "08e1" .


:ASTMStandardEditionKind._09 uml:id "_6CA8E970-C8D5-4c4d-A0BC-491208163B8B" ;
                             rdfs:comment "09 standard edition." ;
                             rdfs:label "09" .


:ASTMStandardEditionKind._09_2013_ uml:id "_8B3383FF-7319-4b40-AD5E-9C1F9A85A435" ;
                                   rdfs:comment "09(2013) standard edition." ;
                                   rdfs:label "09(2013)" .


:ASTMStandardEditionKind._10 uml:id "_BE0A25DB-74EF-4357-9CE9-756D92E67A24" ;
                             rdfs:comment "10 standard edition." ;
                             rdfs:label "10" .


:ASTMStandardEditionKind._10a uml:id "_D054A828-886D-4166-9161-334826F2C07D" ;
                              rdfs:comment "10a standard edition." ;
                              rdfs:label "10a" .


:ASTMStandardEditionKind._11 uml:id "_3E940072-CEB6-4912-B65E-67A30C519454" ;
                             rdfs:comment "11 standard edition." ;
                             rdfs:label "11" .


:ASTMStandardEditionKind._11a uml:id "_1262688E-0F9C-4a92-9E5A-0B93AC21A76B" ;
                              rdfs:comment "11a standard edition." ;
                              rdfs:label "11a" .


:ASTMStandardEditionKind._12 uml:id "_A8FA5C2F-38F6-4142-8E72-65D41B219CD8" ;
                             rdfs:comment "12 standard edition." ;
                             rdfs:label "12" .


:ASTMStandardEditionKind._12a uml:id "_E84C7B7C-C2F3-4729-AD2E-420C70A2C547" ;
                              rdfs:comment "12a standard edition." ;
                              rdfs:label "12a" .


:ASTMStandardEditionKind._12b uml:id "_221DC14C-72C4-4894-A637-5F22A24BED6D" ;
                              rdfs:comment "12b standard edition." ;
                              rdfs:label "12b" .


:ASTMStandardEditionKind._13 uml:id "_48A4934B-9067-486b-9C5A-11E7AF36E548" ;
                             rdfs:comment "13 standard edition." ;
                             rdfs:label "13" .


:ASTMStandardEditionKind._13e1 uml:id "_3718D436-D87F-4b64-B797-7B4AFE418E60" ;
                               rdfs:comment "13e1 standard edition." ;
                               rdfs:label "13e1" .


:ASTMStandardEditionKind._14 uml:id "_61302FE9-D016-40f7-A310-01E61DE66AB6" ;
                             rdfs:comment "14 standard edition." ;
                             rdfs:label "14" .


:ASTMStandardEditionKind._14a uml:id "_A48959D9-7755-4c68-B204-BC3E38849964" ;
                              rdfs:comment "14a standard edition." ;
                              rdfs:label "14a" .


:ASTMStandardEditionKind._14e1 uml:id "_D83C3960-C91F-44ef-8684-9EEEDD6FBFB7" ;
                               rdfs:comment "14e1 standard edition." ;
                               rdfs:label "14e1" .


:ASTMStandardEditionKind._14e2 uml:id "_3E597D0E-5B8D-42de-AAE2-6ECF40862610" ;
                               rdfs:comment "14e2 standard edition." ;
                               rdfs:label "14e2" .


:ASTMStandardEditionKind._15 uml:id "_123F42EB-5D49-4a21-9258-009A9863AD95" ;
                             rdfs:comment "15 standard edition." ;
                             rdfs:label "15" .


:ASTMStandardEditionKind._15a uml:id "_0D89D8ED-2C87-43d7-8880-4A8D41E730BC" ;
                              rdfs:comment "15a standard edition." ;
                              rdfs:label "15a" .


:ASTMStandardEditionKind._65 uml:id "_54A78FE5-DAA3-4e79-B088-4414E6A754CC" ;
                             rdfs:comment "65 standard edition." ;
                             rdfs:label "65" .


:ASTMStandardEditionKind._71 uml:id "_69DD9820-2BFC-427a-907F-B16A2D2EC433" ;
                             rdfs:comment "71 standard edition." ;
                             rdfs:label "71" .


:ASTMStandardEditionKind._74 uml:id "_49917246-D240-4e11-B350-F0A991624D57" ;
                             rdfs:comment "74 standard edition." ;
                             rdfs:label "74" .


:ASTMStandardEditionKind._80e1 uml:id "_48BAA2A9-E851-4a2f-B55C-86B3AD74FD37" ;
                               rdfs:comment "80e1 standard edition." ;
                               rdfs:label "80e1" .


:ASTMStandardEditionKind._82 uml:id "_EBD9656E-1C69-4171-A1BD-36E8ABA8D61B" ;
                             rdfs:comment "82 standard edition." ;
                             rdfs:label "82" .


:ASTMStandardEditionKind._83_1996_e1 uml:id "_EB31ABEF-1D7C-48fa-8B6C-107A42A70AF6" ;
                                     rdfs:comment "83(1996)e1 standard edition." ;
                                     rdfs:label "83(1996)e1" .


:ASTMStandardEditionKind._85 uml:id "_1FC6B816-D0F7-4742-A337-9D8F6B385F62" ;
                             rdfs:comment "85 standard edition." ;
                             rdfs:label "85" .


:ASTMStandardEditionKind._85_1990_e1 uml:id "_5FC570FD-5F8D-403d-BA30-F4CEBAB8CB16" ;
                                     rdfs:comment "85(1990)e1 standard edition." ;
                                     rdfs:label "85(1990)e1" .


:ASTMStandardEditionKind._87_1995_ uml:id "_69881E1E-A36D-4f36-8C5A-9A6EE2266023" ;
                                   rdfs:comment "87(1995) standard edition." ;
                                   rdfs:label "87(1995)" .


:ASTMStandardEditionKind._87e1 uml:id "_ADBB3502-F42A-4d53-B37B-C21F203ECF0F" ;
                               rdfs:comment "87e1 standard edition." ;
                               rdfs:label "87e1" .


:ASTMStandardEditionKind._88 uml:id "_4AA005BE-4D18-419e-BF8D-3C0A287A2C02" ;
                             rdfs:comment "88 standard edition." ;
                             rdfs:label "88" .


:ASTMStandardEditionKind._90e1 uml:id "_F7AD6EAC-78F2-447c-9DB4-8AC4D8EA40CD" ;
                               rdfs:comment "90e1 standard edition." ;
                               rdfs:label "90e1" .


:ASTMStandardEditionKind._91 uml:id "_499240D8-74CA-4845-B5AD-128C07E281E4" ;
                             rdfs:comment "91 standard edition." ;
                             rdfs:label "91" .


:ASTMStandardEditionKind._92 uml:id "_9F714487-5619-4f8a-8C9D-B341F4455EC5" ;
                             rdfs:comment "92 standard edition." ;
                             rdfs:label "92" .


:ASTMStandardEditionKind._94 uml:id "_F82C808B-E574-4420-B494-83BCB350297D" ;
                             rdfs:comment "94 standard edition." ;
                             rdfs:label "94" .


:ASTMStandardEditionKind._94_1999_ uml:id "_393A76C1-DDA2-4698-A158-C932ED9F3ED1" ;
                                   rdfs:comment "94(1999) standard edition." ;
                                   rdfs:label "94(1999)" .


:ASTMStandardEditionKind._94_2004_ uml:id "_DE9031C7-1757-4117-A170-A6B096545B80" ;
                                   rdfs:comment "94(2004) standard edition." ;
                                   rdfs:label "94(2004)" .


:ASTMStandardEditionKind._94_2010_ uml:id "_FC9BC22B-8B02-4ddb-9C40-64A022614730" ;
                                   rdfs:comment "94(2010) standard edition." ;
                                   rdfs:label "94(2010)" .


:ASTMStandardEditionKind._94e1 uml:id "_872D4963-D962-4d2f-B173-9540FF39ED96" ;
                               rdfs:comment "94e1 standard edition." ;
                               rdfs:label "94e1" .


:ASTMStandardEditionKind._95 uml:id "_F660D7A2-E8BF-42eb-97B8-2D76B859878E" ;
                             rdfs:comment "95 standard edition." ;
                             rdfs:label "95" .


:ASTMStandardEditionKind._95_2000_e1 uml:id "_11863897-3E93-46ca-9E5F-B7D505CE7468" ;
                                     rdfs:comment "95(2000)e1 standard edition." ;
                                     rdfs:label "95(2000)e1" .


:ASTMStandardEditionKind._96 uml:id "_60E37299-5F60-461e-90B8-FE3999BBC01B" ;
                             rdfs:comment "96 standard edition." ;
                             rdfs:label "96" .


:ASTMStandardEditionKind._96_2002_e1 uml:id "_609D38A3-1DB0-48ed-9C92-1FA434A93959" ;
                                     rdfs:comment "96(2002)e1 standard edition." ;
                                     rdfs:label "96(2002)e1" .


:ASTMStandardEditionKind._96a uml:id "_AECE6E97-279C-48a8-A042-F8E9521FAEED" ;
                              rdfs:comment "96a standard edition." ;
                              rdfs:label "96a" .


:ASTMStandardEditionKind._96e1 uml:id "_BC789993-A3AC-401d-AFD4-BE1AA7CE3531" ;
                               rdfs:comment "96e1 standard edition." ;
                               rdfs:label "96e1" .


:ASTMStandardEditionKind._97 uml:id "_C6236D3F-F457-44b0-81E6-726637B61A9F" ;
                             rdfs:comment "97 standard edition." ;
                             rdfs:label "97" .


:ASTMStandardEditionKind._97_2002_ uml:id "_07E839ED-6AE6-4188-8A60-18A768EB7DF4" ;
                                   rdfs:comment "97(2002) standard edition." ;
                                   rdfs:label "97(2002)" .


:ASTMStandardEditionKind._97_2003_ uml:id "_96B550A9-B221-4d58-8F41-991D303CC49C" ;
                                   rdfs:comment "97(2003) standard edition." ;
                                   rdfs:label "97(2003)" .


:ASTMStandardEditionKind._97_2008_ uml:id "_8507490C-DEB7-4af4-8B2E-C76E0DC378B8" ;
                                   rdfs:comment "97(2008) standard edition." ;
                                   rdfs:label "97(2008)" .


:ASTMStandardEditionKind._97a uml:id "_E58E931A-8AA1-4973-B510-2EFC5B31B009" ;
                              rdfs:comment "97a standard edition." ;
                              rdfs:label "97a" .


:ASTMStandardEditionKind._97a_2004_ uml:id "_5C3E48A5-0386-4f40-B78A-04C139F44C29" ;
                                    rdfs:comment "97a(2004) standard edition." ;
                                    rdfs:label "97a(2004)" .


:ASTMStandardEditionKind._98 uml:id "_63471520-3CA9-490a-BF67-163FC7AF5007" ;
                             rdfs:comment "98 standard edition." ;
                             rdfs:label "98" .


:ASTMStandardEditionKind._98a uml:id "_D1861806-824C-4722-A5F5-4A8AFA284E05" ;
                              rdfs:comment "98a standard edition." ;
                              rdfs:label "98a" .


:ASTMStandardEditionKind._99 uml:id "_51A57EFC-8C94-42c8-80F5-40AB95A7DBF4" ;
                             rdfs:comment "99 standard edition." ;
                             rdfs:label "99" .


:ASTMStandardEditionKind._99_2004_e1 uml:id "_807093CF-9225-4b19-AB6C-CB62731FB75F" ;
                                     rdfs:comment "99(2004)e1 standard edition." ;
                                     rdfs:label "99(2004)e1" .


:ASTMStandardEditionKind._99_2005_ uml:id "_9331F749-46B7-4087-BA5F-927D7ABAB456" ;
                                   rdfs:comment "99(2005) standard edition." ;
                                   rdfs:label "99(2005)" .


:ASTMStandardEditionKind._99_2009_ uml:id "_2AF29F7E-263E-4367-858B-F1538F914D3F" ;
                                   rdfs:comment "99(2009) standard edition." ;
                                   rdfs:label "99(2009)" .


:ASTMStandardEditionKind._99a uml:id "_BBD4B265-7825-4d9c-8063-79481D451E0F" ;
                              rdfs:comment "99a standard edition." ;
                              rdfs:label "99a" .


:ASTMStandardEditionKind._99a_2004_ uml:id "_E25F80DB-8008-4c8d-AC3D-CCC9E634873C" ;
                                    rdfs:comment "99a(2004) standard edition." ;
                                    rdfs:label "99a(2004)" .


:ASTMStandardEditionKind._99e1 uml:id "_CDEAC077-330A-4781-A86A-A3F3BC5A3CA5" ;
                               rdfs:comment "99e1 standard edition." ;
                               rdfs:label "99e1" .


:ASTMStandardEditionKind._99e2 uml:id "_7AEEED05-DE64-4663-8DFB-76B75C8916C7" ;
                               rdfs:comment "99e2 standard edition." ;
                               rdfs:label "99e2" .


:ASTMStandardEditionKind.none uml:id "_F9E578FF-3D32-465a-85F5-26AB5E3229EE" ;
                              rdfs:comment "No kind of standard." ;
                              rdfs:label "none" .


:ASTMStandardEditionKind.unknown uml:id "_B8FCE4EA-71A8-4f96-A49D-EF4D348B7AD6" ;
                                 rdfs:comment "Unknown kind of standard." ;
                                 rdfs:label "unknown" .


:ASTMStandardKind.D1169 uml:id "_BDA838E2-BC16-4722-9DE7-A01FD0A23565" ;
                        rdfs:comment "Standard Test Method for Specific Resistance (Resistivity) of Electrical Insulating Liquids." ;
                        rdfs:label "D1169" .


:ASTMStandardKind.D1275 uml:id "_520B1325-2E8E-46e5-BDD0-E55ED98D7E37" ;
                        rdfs:comment "Standard Test Method for Corrosive Sulfur in Electrical Insulating Oils." ;
                        rdfs:label "D1275" .


:ASTMStandardKind.D1298 uml:id "_45EBAA7D-1281-4d37-ACB9-31D90A69ECAC" ;
                        rdfs:comment """Standard Test Method for Density, Relative Density, or API Gravity of Crude Petroleum and Liquid Petroleum Products by Hydrometer Method  -or-
Standard Test Method for Density, Relative Density (Specific Gravity), or API Gravity of Crude Petroleum and Liquid Petroleum Products by Hydrometer Method.""" ;
                        rdfs:label "D1298" .


:ASTMStandardKind.D149 uml:id "_4587F9EE-F3E2-4065-A4DC-608C55238E1D" ;
                       rdfs:comment "Standard Test Method for Dielectric Breakdown Voltage and Dielectric Strength of Solid Electrical Insulating Materials at Commercial Power Frequencies." ;
                       rdfs:label "D149" .


:ASTMStandardKind.D1500 uml:id "_E4DED850-65F5-42ca-B163-EF6E59EEA9CB" ;
                        rdfs:comment "Standard Test Method for ASTM Color of Petroleum Products (ASTM Color Scale)." ;
                        rdfs:label "D1500" .


:ASTMStandardKind.D1524 uml:id "_413C5720-2394-42df-9875-A50B3D7A2353" ;
                        rdfs:comment "Standard Test Method for Visual Examination of Used Electrical Insulating Oils of Petroleum Origin in the Field." ;
                        rdfs:label "D1524" .


:ASTMStandardKind.D1533 uml:id "_C510C0FA-D50A-4efa-B5F0-ECF7962EC423" ;
                        rdfs:comment "Standard Test Method for Water in Insulating Liquids by Coulometric Karl Fischer Titration." ;
                        rdfs:label "D1533" .


:ASTMStandardKind.D1816 uml:id "_BF78B213-9EE7-40fb-973D-8C232FE01265" ;
                        rdfs:comment "Standard Test Method for Dielectric Breakdown Voltage of Insulating Liquids Using VDE Electrodes." ;
                        rdfs:label "D1816" .


:ASTMStandardKind.D2029 uml:id "_126DBAFD-7B91-47e3-80D5-75496545A4AA" ;
                        rdfs:comment "Standard Test Methods for Water Vapor Content of Electrical Insulating Gases by Measurement of Dew Point." ;
                        rdfs:label "D2029" .


:ASTMStandardKind.D2112 uml:id "_FFAF595B-6824-481f-84F9-3A951742C8A8" ;
                        rdfs:comment "Standard Test Method for Oxidation Stability of Inhibited Mineral Insulating Oil by Pressure Vessel." ;
                        rdfs:label "D2112" .


:ASTMStandardKind.D2129 uml:id "_A3D11146-E01D-4664-904F-7C3ECED41733" ;
                        rdfs:comment "Standard Test Method for Color of Clear Electrical Insulating Liquids (Platinum-Cobalt Scale)." ;
                        rdfs:label "D2129" .


:ASTMStandardKind.D2140 uml:id "_D23659F8-51E1-441d-96DE-C6666094A564" ;
                        rdfs:comment """Standard Practice for Calculating Carbon-Type Composition of Insulating Oils of Petroleum Origin  -or-
Standard Test Method for Carbon-Type Composition of Insulating Oils of Petroleum Origin.""" ;
                        rdfs:label "D2140" .


:ASTMStandardKind.D2144 uml:id "_B6C6D2AF-6EE0-41b8-979F-10D9DD573E8F" ;
                        rdfs:comment """Standard Practices for Examination of Electrical Insulating Oils by Infrared Absorption  -or-
Standard Test Methods for Examination of Electrical Insulating Oils by Infrared Absorption.""" ;
                        rdfs:label "D2144" .


:ASTMStandardKind.D2668 uml:id "_00504546-78F4-4891-BCE7-0B33305176C7" ;
                        rdfs:comment """Standard Test Method for 2,6-di-tert-Butyl- p-Cresol and 2,6-di-tert-Butyl Phenol in Electrical Insulating Oil by Infrared Absorption  -or-
Standard Test Method for 2,6-Ditertiary-Butyl Para Cresol and 2,6-Ditertiary-Butyl Phenol in Electrical Insulating Oil by Infrared Absorption.""" ;
                        rdfs:label "D2668" .


:ASTMStandardKind.D3612 uml:id "_31EB35FE-B204-4b24-BE81-5D861128714B" ;
                        rdfs:comment "Standard Test Method for Analysis of Gases Dissolved in Electrical Insulating Oil by Gas Chromatography." ;
                        rdfs:label "D3612" .


:ASTMStandardKind.D4052 uml:id "_24BDA1F0-BD2B-4b27-930C-2268930BA2DA" ;
                        rdfs:comment """Standard Test Method for Density, Relative Density, and API Gravity of Liquids by Digital Density Meter  -or-
Standard Test Method for Density and Relative Density of Liquids by Digital Density Meter.""" ;
                        rdfs:label "D4052" .


:ASTMStandardKind.D4059 uml:id "_97CA1A7E-C08F-402a-A756-990C09EFABF5" ;
                        rdfs:comment "Standard Test Method for Analysis of Polychlorinated Biphenyls in Insulating Liquids by Gas Chromatography." ;
                        rdfs:label "D4059" .


:ASTMStandardKind.D4230 uml:id "_2BAE4CD6-3C3C-492e-920A-815BBC11D42C" ;
                        rdfs:comment "Standard Test Method of Measuring Humidity with Cooled-Surface Condensation (Dew-Point) Hygrometer." ;
                        rdfs:label "D4230" .


:ASTMStandardKind.D4243 uml:id "_FDBA07BB-B863-48bd-9FA1-F7F4F68C4CBA" ;
                        rdfs:comment "Standard Test Method for Measurement of Average Viscometric Degree of Polymerization of New and Aged Electrical Papers and Boards." ;
                        rdfs:label "D4243" .


:ASTMStandardKind.D445 uml:id "_3A1116AB-EED3-41de-81F6-29A76C8B4931" ;
                       rdfs:comment """Standard Test Method for Kinematic Viscosity of Transparent and Opaque Liquids (and Calculation of Dynamic Viscosity)  -or-
Standard Method Of Test For Viscosity Of Transparent And Opaque Liquids (Kinematic And Dynamic Viscosities).""" ;
                       rdfs:label "D445" .


:ASTMStandardKind.D4768 uml:id "_36F35B66-AADA-4a68-A4DF-DB41B1B8411B" ;
                        rdfs:comment "Standard Test Method for Analysis of 2,6-Ditertiary-Butyl Para-Cresol and 2,6-Ditertiary-Butyl Phenol in Insulating Liquids by Gas Chromatography." ;
                        rdfs:label "D4768" .


:ASTMStandardKind.D5837 uml:id "_F7E3CDF0-BD8E-4849-8BE8-8C78CE4AB544" ;
                        rdfs:comment "Standard Test Method for Furanic Compounds in Electrical Insulating Liquids by High-Performance Liquid Chromatography (HPLC)." ;
                        rdfs:label "D5837" .


:ASTMStandardKind.D5853 uml:id "_75B78622-F1F8-437a-AE68-5C971E3F10D5" ;
                        rdfs:comment "Standard Test Method for Pour Point of Crude Oils." ;
                        rdfs:label "D5853" .


:ASTMStandardKind.D5949 uml:id "_3DC6643A-5ACD-4bc8-828D-EF783AE6088E" ;
                        rdfs:comment "Standard Test Method for Pour Point of Petroleum Products (Automatic Pressure Pulsing Method)." ;
                        rdfs:label "D5949" .


:ASTMStandardKind.D5950 uml:id "_54DCD366-AD08-4c33-B507-29C21D51F144" ;
                        rdfs:comment "Standard Test Method for Pour Point of Petroleum Products (Automatic Tilt Method)." ;
                        rdfs:label "D5950" .


:ASTMStandardKind.D5985 uml:id "_3A3380A0-A124-41f3-9464-BE45CBBDE912" ;
                        rdfs:comment "Standard Test Method for Pour Point of Petroleum Products (Rotational Method)." ;
                        rdfs:label "D5985" .


:ASTMStandardKind.D6304 uml:id "_B29E4892-37B8-4d51-9AE7-53FD162B16C4" ;
                        rdfs:comment "Standard Test Method for Determination of Water in Petroleum Products, Lubricating Oils, and Additives by Coulometric Karl Fischer Titration." ;
                        rdfs:label "D6304" .


:ASTMStandardKind.D6749 uml:id "_14D28F29-F833-4846-9732-FE5CF4A62B75" ;
                        rdfs:comment "Standard Test Method for Pour Point of Petroleum Products (Automatic Air Pressure Method)." ;
                        rdfs:label "D6749" .


:ASTMStandardKind.D6786 uml:id "_D36911FD-D1B2-4617-8E45-43F1589026C4" ;
                        rdfs:comment "Standard Test Method for Particle Count in Mineral Insulating Oil Using Automatic Optical Particle Counters." ;
                        rdfs:label "D6786" .


:ASTMStandardKind.D6892 uml:id "_DAB88866-B01A-4229-A61C-6887D449AC4F" ;
                        rdfs:comment "Standard Test Method for Pour Point of Petroleum Products (Robotic Tilt Method)." ;
                        rdfs:label "D6892" .


:ASTMStandardKind.D7151 uml:id "_C8221233-0266-4b32-B8C8-9070E62EAFC4" ;
                        rdfs:comment "Standard Test Method for Determination of Elements in Insulating Oils by Inductively Coupled Plasma Atomic Emission Spectrometry (ICP-AES)." ;
                        rdfs:label "D7151" .


:ASTMStandardKind.D7346 uml:id "_B785E03F-52C6-49bd-ADE5-E0869421448B" ;
                        rdfs:comment """Standard Test Method for No Flow Point and Pour Point of Petroleum Products and Liquid Fuels  -or-
Standard Test Method for No Flow Point and Pour Point of Petroleum Products  -or-
Standard Test Method for No Flow Point of Petroleum Products.""" ;
                        rdfs:label "D7346" .


:ASTMStandardKind.D828 uml:id "_F11EEB75-9C59-4085-A95E-D33523E0362D" ;
                       rdfs:comment "Standard Test Method for Tensile Properties of Paper and Paperboard Using Constant-Rate-of-Elongation Apparatus (Withdrawn 2009)." ;
                       rdfs:label "D828" .


:ASTMStandardKind.D877 uml:id "_D2E500C9-3440-4f47-8CFA-4EB856E4B5D6" ;
                       rdfs:comment "Standard Test Method for Dielectric Breakdown Voltage of Insulating Liquids Using Disk Electrodes." ;
                       rdfs:label "D877" .


:ASTMStandardKind.D877_D877M uml:id "_0DA468BD-5566-49ff-8FB5-F9122970CFB1" ;
                             rdfs:comment "Standard Test Method for Dielectric Breakdown Voltage of Insulating Liquids Using Disk Electrodes." ;
                             rdfs:label "D877/D877M" .


:ASTMStandardKind.D92 uml:id "_B1D58CA7-1194-49fd-8972-E704144B8538" ;
                      rdfs:comment """Standard Test Method for Flash and Fire Points by Cleveland Open Cup Tester  -or-
Standard Test Method for Flash and Fire Points by Cleveland Open Cup.""" ;
                      rdfs:label "D92" .


:ASTMStandardKind.D924 uml:id "_890D0E74-B788-426a-8114-DB5840502C87" ;
                       rdfs:comment "Standard Test Method for Dissipation Factor (or Power Factor) and Relative Permittivity (Dielectric Constant) of Electrical Insulating Liquids." ;
                       rdfs:label "D924" .


:ASTMStandardKind.D93 uml:id "_C52F8AE8-DED9-4a99-97D0-5537857DF251" ;
                      rdfs:comment """Standard Test Methods for Flash Point by Pensky-Martens Closed Cup Tester  -or-
Standard Test Method for Flash Point by Pensky-Martens Closed Tester  -or-
Standard Method Of Test For Flash Point by Pensky-Martens Closed Tester.""" ;
                      rdfs:label "D93" .


:ASTMStandardKind.D97 uml:id "_4022FFDE-786F-411d-ABEA-82DD1E1E1947" ;
                      rdfs:comment """Standard Test Method for Pour Point of Petroleum Products  -or-
Standard Test Method for Pour Point of Petroleum Oils.""" ;
                      rdfs:label "D97" .


:ASTMStandardKind.D974 uml:id "_6D0A2EE6-76A1-4fe1-BCDE-590211676CCB" ;
                       rdfs:comment "Standard Test Method for Acid and Base Number by Color-Indicator Titration." ;
                       rdfs:label "D974" .


:AccumulationKind.boundedQuantity uml:hasInitialValue "14" ;
                                  uml:id "_32F41A88-A184-42a8-8D52-DF6F1DC51DDA" ;
                                  rdfs:comment "A time-independent cumulative quantity much like a 'bulkQuantity' or a 'latchingQuantity', except that the accumulation stops at the maximum or minimum values. When the maximum is reached, any additional positive accumulation is discarded, but negative accumulation may be accepted (thus lowering the counter.) Likewise, when the negative bound is reached, any additional negative accumulation is discarded, but positive accumulation is accepted (thus increasing the counter.)" ;
                                  rdfs:label "boundedQuantity" .


:AccumulationKind.bulkQuantity uml:hasInitialValue "1" ;
                               uml:id "_399FA930-B42D-43c3-9D07-61AAB6753CD4" ;
                               rdfs:comment """A value from a register which represents the bulk quantity of a commodity. This quantity is computed as the integral of the commodity usage rate. This value is typically used as the basis for the dial reading at the meter, and as a result, will roll over upon reaching a maximum dial value. 
Note 1: With the metering system, the roll-over behaviour typically implies a roll-under behavior so that the value presented is always a positive value (e.g. unsigned integer or positive decimal.) However, when communicating data between enterprise applications a negative value might occur in a case such as net metering.
Note 2: A 'bulkQuantity' refers primarily to the dial reading and not the consumption over a specific period of time.""" ;
                               rdfs:label "bulkQuantity" .


:AccumulationKind.continuousCumulative uml:hasInitialValue "2" ;
                                       uml:id "_C0ED909E-32CA-458b-ADDC-5C89AF7C5DA2" ;
                                       rdfs:comment """The sum of the previous billing period values and the present period value.
Note: 'continuousCumulative' is commonly used in conjunction with 'demand', and it  would represent the cumulative sum of the previous billing period maximum demand values (as occurring with each demand reset) summed with the present period maximum demand value (which has yet to be reset.)""" ;
                                       rdfs:label "continuousCumulative" .


:AccumulationKind.cumulative uml:hasInitialValue "3" ;
                             uml:id "_BABECDA5-A39C-41ef-A70E-ABAB39A760FD" ;
                             rdfs:comment """The sum of the previous billing period values.
Note: 'cumulative' is commonly used in conjunction with “demand.” Each demand reset causes the maximum demand value for the present billing period (since the last demand reset) to accumulate as an accumulative total of all maximum demands. So instead of 'zeroing' the demand register, a demand reset has the effect of adding the present maximum demand to this accumulating total.""" ;
                             rdfs:label "cumulative" .


:AccumulationKind.deltaData uml:hasInitialValue "4" ;
                            uml:id "_DFA6FB19-2A7C-4aab-9A78-753822D67012" ;
                            rdfs:comment """The difference between the value at the end of the prescribed interval and the beginning of the interval. This is used for incremental interval data. 
Note: One common application would be for load profile data, another use might be to report the number of events within an interval (such as the number of equipment energisations within the specified period of time.)""" ;
                            rdfs:label "deltaData" .


:AccumulationKind.indicating uml:hasInitialValue "6" ;
                             uml:id "_3C61E398-3FC4-430c-AB7B-81B42B91BC92" ;
                             rdfs:comment """As if a needle is swung out on the meter face to a value to indicate the current value.
Note: An 'indicating' value is typically measured over hundreds of milliseconds or greater, or may imply a “pusher” mechanism to capture a value. Compare this to 'instantaneous' which is measured over a shorter period of time.""" ;
                             rdfs:label "indicating" .


:AccumulationKind.instantaneous uml:hasInitialValue "12" ;
                                uml:id "_238008C2-0A22-40b2-B4EB-6B65C9F67C85" ;
                                rdfs:comment """Typically measured over the fastest period of time allowed by the definition of the metric (usually milliseconds or tens of milliseconds.)
Note: 'instantaneous' was moved to attribute #3 in Ed.2 of IEC 61968-9, from attribute #1 in Ed.1 of IEC 61968-9.""" ;
                                rdfs:label "instantaneous" .


:AccumulationKind.latchingQuantity uml:hasInitialValue "13" ;
                                   uml:id "_63214527-EC2F-4b67-88E9-046D41E8ABBD" ;
                                   rdfs:comment """When this description is applied to a metered value, it implies that the value is a time-independent cumulative quantity much like a 'bulkQuantity', except that it latches upon the maximum value upon reaching that value. Any additional accumulation (positive or negative) is discarded until a reset occurs. 
Note: A 'latchingQuantity' may also occur in the downward direction – upon reaching a minimum value. The terms 'maximum' or 'minimum' (for 'aggregate') will usually be included when this type of accumulation behaviour is present. 
When this description is applied to an encoded value (UOM= 'Code'), it implies that the value has one or more bits which are latching. The condition that caused the bit to be set may have long since evaporated.
In either case, the timestamp that accompanies the value may not coincide with the moment the value was initially set.
In both cases a system will need to perform an operation to clear the latched value.""" ;
                                   rdfs:label "latchingQuantity" .


:AccumulationKind.none uml:hasInitialValue "0" ;
                       uml:id "_86370381-DBEA-4802-B068-AB8EEE43D45E" ;
                       rdfs:comment "Not applicable, or implied by the unit of measure." ;
                       rdfs:label "none" .


:AccumulationKind.summation uml:hasInitialValue "9" ;
                            uml:id "_D58C159E-28AF-485e-843C-C13FC94067C0" ;
                            rdfs:comment """A form of accumulation which is selective with respect to time. 
Note : 'summation' could be considered a specialisation of 'bulkQuantity' as it selectively accumulates pulses over a timing pattern (while 'bulkQuantity' accumulates pulses all of the time).""" ;
                            rdfs:label "summation" .


:AccumulationKind.timeDelay uml:hasInitialValue "10" ;
                            uml:id "_BD170B22-4CB4-48a7-B7E5-DDC7F329D97B" ;
                            rdfs:comment "A form of computation which introduces a time delay characteristic to the data value." ;
                            rdfs:label "timeDelay" .


:ActionType.CANCEL uml:id "_E5EA090F-7915-4c33-89A3-9926F4B6D383" ;
                   rdfs:comment "Cancel a trade." ;
                   rdfs:label "CANCEL" .


:AdderType.BASELINE uml:id "_D1E66A1E-075B-4ce0-8057-DCEAA40946FC" ;
                    rdfs:label "BASELINE" .


:AdderType.NEGOTIATED uml:id "_E879A569-DF85-4407-A3C1-A268FFD5A54B" ;
                      rdfs:label "NEGOTIATED" .


:AggregateKind.average uml:hasInitialValue "2" ;
                       uml:id "_D0D4CE63-D116-4285-9739-C0E4AA58B9EF" ;
                       rdfs:comment "The value represents average." ;
                       rdfs:label "average" .


:AggregateKind.excess uml:hasInitialValue "4" ;
                      uml:id "_8E510F94-C290-4a12-B510-E87FA1637768" ;
                      rdfs:comment "The value represents an amount over which a threshold was exceeded." ;
                      rdfs:label "excess" .


:AggregateKind.fifthMaximum uml:hasInitialValue "25" ;
                            uml:id "_715C2F7B-E77B-4356-B28C-C12ABB192647" ;
                            rdfs:comment "The fifth highest value observed." ;
                            rdfs:label "fifthMaximum" .


:AggregateKind.fourthMaximum uml:hasInitialValue "24" ;
                             uml:id "_F912DE09-EE7D-470a-8901-9F7B7F441ECF" ;
                             rdfs:comment "The fourth highest value observed." ;
                             rdfs:label "fourthMaximum" .


:AggregateKind.highThreshold uml:hasInitialValue "5" ;
                             uml:id "_278D72B1-F5EC-4af5-BF68-610B6FC54E0A" ;
                             rdfs:comment "The value represents a programmed high threshold." ;
                             rdfs:label "highThreshold" .


:AggregateKind.lowThreshold uml:hasInitialValue "7" ;
                            uml:id "_3BB9F9E6-E9EA-46db-B0E4-9656F9788AC1" ;
                            rdfs:comment "The value represents a programmed low threshold." ;
                            rdfs:label "lowThreshold" .


:AggregateKind.maximum uml:hasInitialValue "8" ;
                       uml:id "_72B3FA61-59DC-4eed-9026-849B0188CEFD" ;
                       rdfs:comment "The highest value observed." ;
                       rdfs:label "maximum" .


:AggregateKind.minimum uml:hasInitialValue "9" ;
                       uml:id "_9C51BF89-A4AE-41ed-BC37-0441998A6D06" ;
                       rdfs:comment "The smallest value observed." ;
                       rdfs:label "minimum" .


:AggregateKind.nominal uml:hasInitialValue "11" ;
                       uml:id "_68DE4069-31AC-41d5-B7C6-6882B74807FB" ;
                       rdfs:comment "The nominal value." ;
                       rdfs:label "nominal" .


:AggregateKind.none uml:hasInitialValue "0" ;
                    uml:id "_15C5DB87-83D3-48a5-B2C6-A564FF42979F" ;
                    rdfs:comment "Not applicable." ;
                    rdfs:label "none" .


:AggregateKind.normal uml:hasInitialValue "12" ;
                      uml:id "_C4AABDA6-D25C-4e5f-BE44-868E9D58976A" ;
                      rdfs:comment "The normal value." ;
                      rdfs:label "normal" .


:AggregateKind.secondMaximum uml:hasInitialValue "16" ;
                             uml:id "_50D29B59-8085-432d-AFD3-6A337CC4DF62" ;
                             rdfs:comment "The second highest value observed." ;
                             rdfs:label "secondMaximum" .


:AggregateKind.secondMinimum uml:hasInitialValue "17" ;
                             uml:id "_0D5AC330-E006-4bab-9119-860F67A75A75" ;
                             rdfs:comment "The second smallest value observed." ;
                             rdfs:label "secondMinimum" .


:AggregateKind.sum uml:hasInitialValue "26" ;
                   uml:id "_377B8C36-5568-4a13-A139-2B0A6AF1D18B" ;
                   rdfs:comment "The accumulated sum." ;
                   rdfs:label "sum" .


:AggregateKind.thirdMaximum uml:hasInitialValue "23" ;
                            uml:id "_9AE63C4A-2221-419e-9574-B375C7FEE6F2" ;
                            rdfs:comment "The third highest value observed." ;
                            rdfs:label "thirdMaximum" .


:AlarmDisplayType.Appear uml:id "_4A455840-9ACF-4d86-8007-85E6425AF09D" ;
                         rdfs:label "Appear" .


:AlarmDisplayType.Disappear uml:id "_4E9DB412-7B94-456b-8CD7-2F4630042D12" ;
                            rdfs:label "Disappear" .


:AlarmDisplayType.Fleeting uml:id "_ED3726A3-0E63-455d-9CA8-9571175F118B" ;
                           rdfs:label "Fleeting" .


:AllocationEnergyTypeCode.ACNG uml:id "_21F8F7EB-C281-48f7-8C41-272D616EC2F7" ;
                               rdfs:label "ACNG" .


:AllocationEnergyTypeCode.BS uml:id "_D1D8052A-3D26-4695-9D37-420D21ADA516" ;
                             rdfs:label "BS" .


:AllocationEnergyTypeCode.DAPE uml:id "_9F362C89-AB7B-46b7-AB15-317834D48406" ;
                               rdfs:label "DAPE" .


:AllocationEnergyTypeCode.DASE uml:id "_1E702837-C1C7-408e-858F-AB916A16950C" ;
                               rdfs:label "DASE" .


:AllocationEnergyTypeCode.ESRT uml:id "_D4DF1E4C-C4F6-45f1-925A-1A3889268BE8" ;
                               rdfs:label "ESRT" .


:AllocationEnergyTypeCode.ESYS uml:id "_7FA33841-3CA6-464a-8C50-FE273BEA6EE9" ;
                               rdfs:label "ESYS" .


:AllocationEnergyTypeCode.ETC uml:id "_87F640A6-E9E6-4ff5-91BE-CBFCA4DABF9A" ;
                              rdfs:label "ETC" .


:AllocationEnergyTypeCode.HASE uml:id "_47236E18-B746-4201-B273-AD4E43787154" ;
                               rdfs:label "HASE" .


:AllocationEnergyTypeCode.LMPM uml:id "_DCB903B7-2BC6-49c3-8F62-61EBF83883FF" ;
                               rdfs:label "LMPM" .


:AllocationEnergyTypeCode.MINL uml:id "_C4556F89-7E5E-40f7-9767-45145FA542FD" ;
                               rdfs:label "MINL" .


:AllocationEnergyTypeCode.MLE uml:id "_FD2F93D0-0F34-4eb8-8F32-D55E891F0736" ;
                              rdfs:label "MLE" .


:AllocationEnergyTypeCode.MSSLFE uml:id "_3051EC37-8AA1-4d4d-A4A9-E62A5A06F16F" ;
                                 rdfs:label "MSSLFE" .


:AllocationEnergyTypeCode.OE uml:id "_4E396B39-57D4-4343-8F04-B153081F3611" ;
                             rdfs:label "OE" .


:AllocationEnergyTypeCode.OTHER uml:id "_9743082A-BC58-4fb5-A856-96552E49692E" ;
                                rdfs:label "OTHER" .


:AllocationEnergyTypeCode.OVGN uml:id "_64AB4E96-C891-4579-B53F-98ABA034C44E" ;
                               rdfs:label "OVGN" .


:AllocationEnergyTypeCode.PE uml:id "_5111E3ED-E3DC-4632-A459-85BF995A2BD6" ;
                             rdfs:label "PE" .


:AllocationEnergyTypeCode.RCNG uml:id "_E69A541C-53E6-4fe9-B6A6-50262891628B" ;
                               rdfs:label "RCNG" .


:AllocationEnergyTypeCode.RE uml:id "_3A1C7ACE-7543-4a9e-ACBB-7F5055AEC98F" ;
                             rdfs:label "RE" .


:AllocationEnergyTypeCode.RED uml:id "_022F6657-72DA-4e44-AD52-9F0A7368D2D5" ;
                              rdfs:label "RED" .


:AllocationEnergyTypeCode.RMRD uml:id "_04862EAF-DEEA-4237-BBD2-093D21B5F24E" ;
                               rdfs:label "RMRD" .


:AllocationEnergyTypeCode.RMRH uml:id "_FFCCA9BD-CCBD-4675-9DBD-01810EB676B5" ;
                               rdfs:label "RMRH" .


:AllocationEnergyTypeCode.RMRR uml:id "_EC0F9A44-3E0E-4985-9362-C250400F3F8C" ;
                               rdfs:label "RMRR" .


:AllocationEnergyTypeCode.RMRS uml:id "_50C7D5EC-A15D-4e31-862D-31B5A2566313" ;
                               rdfs:label "RMRS" .


:AllocationEnergyTypeCode.RMRT uml:id "_AED689C5-A2F5-4167-BFAC-91C7F07DB352" ;
                               rdfs:label "RMRT" .


:AllocationEnergyTypeCode.RSYS uml:id "_BFE0E28F-5531-47d9-8FA9-21D0F474ECE8" ;
                               rdfs:label "RSYS" .


:AllocationEnergyTypeCode.RTSSE uml:id "_29B92C8B-F463-48e5-955D-ED1118AFF8BD" ;
                                rdfs:label "RTSSE" .


:AllocationEnergyTypeCode.SDWN uml:id "_2B517CFB-0DCB-4e9d-865B-252B43DA9B4C" ;
                               rdfs:label "SDWN" .


:AllocationEnergyTypeCode.SE uml:id "_21CC1ADB-3C30-48c9-9E02-6C4992DBA674" ;
                             rdfs:label "SE" .


:AllocationEnergyTypeCode.SLIC uml:id "_5A3DCA63-9AA8-439f-8A9A-663CC9E70875" ;
                               rdfs:label "SLIC" .


:AllocationEnergyTypeCode.SRE uml:id "_35F70B21-C8A2-428f-B06E-077D249E11BF" ;
                              rdfs:label "SRE" .


:AllocationEnergyTypeCode.STRT uml:id "_53EEC3C8-4023-4daa-A227-73ED2C27DBAB" ;
                               rdfs:label "STRT" .


:AllocationEnergyTypeCode.SUMR uml:id "_C6C5970F-9A9D-4b61-8D58-C44B08430FF5" ;
                               rdfs:label "SUMR" .


:AllocationEnergyTypeCode.TCNG uml:id "_00382BFC-B925-4e25-AE53-E2E16CA8B73C" ;
                               rdfs:label "TCNG" .


:AllocationEnergyTypeCode.TEST uml:id "_4BA981CB-EF29-4bed-A143-53CFC95B7AAF" ;
                               rdfs:label "TEST" .


:AllocationEnergyTypeCode.TOR uml:id "_C137DBE6-1CBA-48b0-B887-60AC2902221F" ;
                              rdfs:label "TOR" .


:AllocationEnergyTypeCode.VS uml:id "_EE0E6E12-F7D4-4a49-BB06-3A00B58ADCE2" ;
                             rdfs:label "VS" .


:AmiBillingReadyKind.amiCapable uml:id "_1A5859D6-149E-4b93-B8B4-09C7E53B57BD" ;
                                rdfs:comment "Usage point is equipped with an AMI capable meter that is not yet currently equipped with a communications module." ;
                                rdfs:label "amiCapable" .


:AmiBillingReadyKind.amiDisabled uml:id "_FD29CB68-66E0-4238-BBB9-0E73322B2292" ;
                                 rdfs:comment "Usage point is equipped with an AMI capable meter; however, the AMI functionality has been disabled or is not being used." ;
                                 rdfs:label "amiDisabled" .


:AmiBillingReadyKind.billingApproved uml:id "_9ADC2417-4D85-4d78-9A54-F2D12C0C1860" ;
                                     rdfs:comment "Usage point is equipped with an operating AMI capable meter and accuracy has been certified for billing purposes." ;
                                     rdfs:label "billingApproved" .


:AmiBillingReadyKind.enabled uml:id "_CF70448A-6855-42fb-B84E-174152DEA3AE" ;
                             rdfs:comment "Usage point is equipped with an AMI capable meter having communications capability." ;
                             rdfs:label "enabled" .


:AmiBillingReadyKind.nonAmi uml:id "_E7C2F2B1-6F4B-40de-8199-8E2E77CFFC89" ;
                            rdfs:comment "Usage point is equipped with a non AMI capable meter." ;
                            rdfs:label "nonAmi" .


:AmiBillingReadyKind.nonMetered uml:id "_5B7ACD6E-011F-4530-B4AC-7501C1C94921" ;
                                rdfs:comment "Usage point is not currently equipped with a meter." ;
                                rdfs:label "nonMetered" .


:AmiBillingReadyKind.operable uml:id "_1E16365F-8608-4895-9DB5-8A8A60ED8813" ;
                              rdfs:comment "Usage point is equipped with an AMI capable meter that is functioning and communicating with the AMI network." ;
                              rdfs:label "operable" .


:AnalogLimitType.BranchLongTerm uml:id "_95B28857-7460-4ba8-AD65-1DBADC4E5D00" ;
                                rdfs:comment "Branch Long Term Limit" ;
                                rdfs:label "BranchLongTerm" .


:AnalogLimitType.BranchMediumTerm uml:id "_D0A2C9E4-CDD2-4b0b-85F2-8AA027BFC710" ;
                                  rdfs:comment "Branch Medium Term Limit" ;
                                  rdfs:label "BranchMediumTerm" .


:AnalogLimitType.BranchShortTerm uml:id "_B0EDA439-C57C-4645-8EE5-3F213D1BD1C7" ;
                                 rdfs:comment "Branch Short Term Limit" ;
                                 rdfs:label "BranchShortTerm" .


:AnalogLimitType.VoltageHigh uml:id "_6276D8BF-F042-4b6c-A79A-F3FDA624386B" ;
                             rdfs:comment "Voltage High Limit" ;
                             rdfs:label "VoltageHigh" .


:AnalogLimitType.VoltageLow uml:id "_AE30CEBB-368D-4b60-8B27-4DA0C76CC35F" ;
                            rdfs:comment "Voltage Low Limit" ;
                            rdfs:label "VoltageLow" .


:AnalogToDigitalLogicKind.eq uml:id "_093BD8B8-4782-43c5-80EE-CDA6DF2F5F45" ;
                             rdfs:comment "Equal (like) comparison operation." ;
                             rdfs:label "eq" .


:AnalogToDigitalLogicKind.ge uml:id "_90E460DE-C7BB-4ea5-8398-6BB17B135F16" ;
                             rdfs:comment "Greater or equal comparison operation." ;
                             rdfs:label "ge" .


:AnalogToDigitalLogicKind.gt uml:id "_9CB66A12-F8B9-4abf-B99A-F09E42A6880C" ;
                             rdfs:comment "Greater than comparison operation." ;
                             rdfs:label "gt" .


:AnalogToDigitalLogicKind.le uml:id "_FB63F810-2A6B-4b69-B1AD-8BE4FF62B22D" ;
                             rdfs:comment "Less or equal comparison operation." ;
                             rdfs:label "le" .


:AnalogToDigitalLogicKind.lt uml:id "_76EE8579-DD6C-42c5-A5DD-4EFBAF2BDC64" ;
                             rdfs:comment "Less than comparison operation." ;
                             rdfs:label "lt" .


:AnalogToDigitalLogicKind.ne uml:id "_2BD79851-4D3E-4d99-81F5-9BFFAD6381EA" ;
                             rdfs:comment "Not equal (unlike) comparison operation." ;
                             rdfs:label "ne" .


:AnalyticKind.agingAnalytic uml:id "_C2C33117-B7FE-4233-A933-7C23B01E520A" ;
                            rdfs:comment "Analytic evaluates aging." ;
                            rdfs:label "agingAnalytic" .


:AnalyticKind.faultAnalytic uml:id "_726154C7-E536-4968-9BC0-2C1AAE3A41C5" ;
                            rdfs:comment "Analytic evaluates fault." ;
                            rdfs:label "faultAnalytic" .


:AnalyticKind.healthAnalytic uml:id "_CF0B2DE7-D41E-4d18-97AA-445AF712C110" ;
                             rdfs:comment "Analytic evaluates asset health." ;
                             rdfs:label "healthAnalytic" .


:AnalyticKind.other uml:id "_E767E08B-69C9-4d39-9A72-1FD1D6BD22E7" ;
                    rdfs:comment "Analytic evaluates other factor." ;
                    rdfs:label "other" .


:AnalyticKind.replacementAnalytic uml:id "_13E1F480-805D-4484-A51A-D12C9C37016A" ;
                                  rdfs:comment "Analytic evaluates need for replacement." ;
                                  rdfs:label "replacementAnalytic" .


:AnalyticKind.riskAnalytic uml:id "_E6D05734-6D4B-4722-8395-91B557285363" ;
                           rdfs:comment "Analytic evaluates risk." ;
                           rdfs:label "riskAnalytic" .


:AnchorKind.concrete uml:id "_321FE6AB-4A05-4552-846A-5812C5C10E3B" ;
                     rdfs:label "concrete" .


:AnchorKind.helix uml:id "_5BEA99D4-3A23-4d3a-9AFC-EF66531B42AF" ;
                  rdfs:label "helix" .


:AnchorKind.multiHelix uml:id "_F4B063EB-1573-448a-BC5F-9B1F05D0A039" ;
                       rdfs:label "multiHelix" .


:AnchorKind.other uml:id "_50D42452-0CF6-4f6c-B241-B55DF6BF6682" ;
                  rdfs:label "other" .


:AnchorKind.rod uml:id "_6CB14A47-7404-4c27-975E-9E76888F09ED" ;
                rdfs:label "rod" .


:AnchorKind.screw uml:id "_FF4B65C4-F75F-4930-8A3F-662E8807A06E" ;
                  rdfs:label "screw" .


:AnchorKind.unknown uml:id "_FD124732-3587-4440-B507-CE77CD9AE702" ;
                    rdfs:label "unknown" .


:AncillaryCommodityType.NONSPIN uml:id "_1F9AF23F-8328-432e-B8E6-450957AF41DE" ;
                                rdfs:comment "non spinning reserve" ;
                                rdfs:label "NONSPIN" .


:AncillaryCommodityType.REGDN uml:id "_07D5E031-00AC-4ac9-B60A-2290E944EB4C" ;
                              rdfs:comment "regulation down" ;
                              rdfs:label "REGDN" .


:AncillaryCommodityType.REGUP uml:id "_DC70C300-636C-4397-BD57-19D4B5E74436" ;
                              rdfs:comment "regulation up" ;
                              rdfs:label "REGUP" .


:AncillaryCommodityType.SPIN uml:id "_BD91A884-323A-4402-A0F7-C6D3FD1113B6" ;
                             rdfs:comment "spinning reserve" ;
                             rdfs:label "SPIN" .


:AnodeType.ACA uml:id "_929C183C-EFBC-450a-933E-746946DB1B1E" ;
               rdfs:comment "Adjacent Control Area" ;
               rdfs:label "ACA" .


:AnodeType.AGR uml:id "_06596BE2-95DF-41f3-9D14-4DE68BC5F41C" ;
               rdfs:comment "Aggregate Generation Resource;" ;
               rdfs:label "AGR" .


:AnodeType.ALR uml:id "_71DB6C1C-3866-4277-82F5-DB0A8ADFE06F" ;
               rdfs:comment "Aggregate Load Resource;" ;
               rdfs:label "ALR" .


:AnodeType.ASR uml:id "_61EE5B26-C05E-4e98-8993-48F336251852" ;
               rdfs:comment "Aggregated System Resource" ;
               rdfs:label "ASR" .


:AnodeType.DER uml:id "_21121CED-7CFD-4db1-B54E-D0ADC11B101E" ;
               rdfs:comment "Distributed Energy Resource." ;
               rdfs:label "DER" .


:AnodeType.ECA uml:id "_68B130B3-3C87-4d62-B635-5F44FC577725" ;
               rdfs:comment "Embedded Control Area" ;
               rdfs:label "ECA" .


:AnodeType.LFZ uml:id "_ADD85D8B-E15B-41eb-B16F-A06A870AD8C9" ;
               rdfs:comment "Load Forecast Zone" ;
               rdfs:label "LFZ" .


:AnodeType.LTAC uml:id "_725B6D04-0D32-4748-BD8F-BD57C4EFC826" ;
                rdfs:comment "Load TransmissionAccessCharge (TAC) Group;" ;
                rdfs:label "LTAC" .


:AnodeType.POD uml:id "_6FFA71B6-8EC5-4cc5-8FBE-C957B4F17620" ;
               rdfs:comment "Point of Delivery;" ;
               rdfs:label "POD" .


:AnodeType.REG uml:id "_2CBCD676-5533-4054-93C3-6EAD45B15B6E" ;
               rdfs:comment "Market Energy/Ancillary Service Region;" ;
               rdfs:label "REG" .


:AnodeType.RUC uml:id "_17F6F84D-F24F-4723-A50E-C003DAEF944C" ;
               rdfs:comment "RUC Zone" ;
               rdfs:label "RUC" .


:AnodeType.SYS uml:id "_B5F1C6CF-0131-4b9c-85F9-221A7C54D78D" ;
               rdfs:comment "System Zone/Region;" ;
               rdfs:label "SYS" .


:ApnodeType.AG uml:id "_8FFFC9D3-5E35-44b7-BBF8-0E30D46C86BF" ;
               rdfs:comment "Aggregated Generation" ;
               rdfs:label "AG" .


:ApnodeType.BUS uml:id "_CC6C6C72-DD18-4a38-9D82-FCC89ABFCEE8" ;
                rdfs:comment "Bus" ;
                rdfs:label "BUS" .


:ApnodeType.CA uml:id "_191A6CAB-46CA-49bf-9400-FF12C8716B79" ;
               rdfs:comment "Control Area" ;
               rdfs:label "CA" .


:ApnodeType.CPZ uml:id "_4BF236DB-57B9-46d8-9401-2DD590D4E4EC" ;
                rdfs:comment "Custom Price Zone" ;
                rdfs:label "CPZ" .


:ApnodeType.DCA uml:id "_17EBD495-E485-4601-95BD-ED81CEFADD80" ;
                rdfs:comment "Designated Congestion Area" ;
                rdfs:label "DCA" .


:ApnodeType.DPZ uml:id "_5A5F528E-9CA0-4398-91E6-7963F0093285" ;
                rdfs:comment "Default Price Zone" ;
                rdfs:label "DPZ" .


:ApnodeType.EHV uml:id "_8B5CD47A-97D3-499d-A08B-8F8BA9AB64DB" ;
                rdfs:comment "500 kV - Extra High Voltage aggregate price nodes" ;
                rdfs:label "EHV" .


:ApnodeType.GA uml:id "_4F379793-6C43-40eb-A3E8-DAD964168374" ;
               rdfs:comment "generic aggregation" ;
               rdfs:label "GA" .


:ApnodeType.GH uml:id "_E025C7AB-7031-4ff6-87ED-A0355BFC4BA8" ;
               rdfs:comment "generic hub" ;
               rdfs:label "GH" .


:ApnodeType.INT uml:id "_63601B12-6E90-4d5f-95E8-A49F9D964869" ;
                rdfs:comment "Interface" ;
                rdfs:label "INT" .


:ApnodeType.SYS uml:id "_AA6A60BA-12A4-45ee-8A33-CF45DF5C6985" ;
                rdfs:comment "System Zone" ;
                rdfs:label "SYS" .


:ApnodeType.TH uml:id "_4DB37CC8-C33D-4cad-8F27-1FD96B67976C" ;
               rdfs:comment "Trading  Hub" ;
               rdfs:label "TH" .


:ApnodeType.ZN uml:id "_4F3412AC-1108-4b49-9EC4-9A7BE287B633" ;
               rdfs:comment "Zone" ;
               rdfs:label "ZN" .


:ApplicationSecurityKind.endToEndSecure uml:id "_97B77F60-CAE5-4d9d-9C95-AB0170C985C2" ;
                                        rdfs:comment "Indicates that E2E-security shall be used in order to allow establishment of an MMS association." ;
                                        rdfs:label "endToEndSecure" .


:ApplicationSecurityKind.nonSecure uml:id "_E4A01C19-4BBC-49f7-98B3-DE9D687226F6" ;
                                   rdfs:comment "Indicates that an application security shall not be used in order to allow establishment of an MSS association." ;
                                   rdfs:label "nonSecure" .


:ApplicationSecurityKind.secure uml:id "_463A0794-00C8-4643-936D-0949911B70DA" ;
                                rdfs:comment "Indicates that the A-security-profile as specified in Clause 11 (or IEC TS 62351-4:2007) shall be used in order to allow establishment of an MMS association." ;
                                rdfs:label "secure" .


:AreaControlMode.CF uml:id "_529C9077-53BA-46fb-8587-CC6D29A7CDC4" ;
                    rdfs:comment "CF = Constant Frequency" ;
                    rdfs:label "CF" .


:AreaControlMode.CTL uml:id "_8CC65B96-9CC2-4bb5-9456-02D069DDE91F" ;
                     rdfs:comment "Constant Tie-Line" ;
                     rdfs:label "CTL" .


:AreaControlMode.OFF uml:id "_FAE5FD94-9BA9-43b9-A0A7-53A2D8DE4DE0" ;
                     rdfs:comment "Off control" ;
                     rdfs:label "OFF" .


:AreaControlMode.TLB uml:id "_FC6A16C8-19D7-4f0a-A1BE-E5ADA2C20B61" ;
                     rdfs:comment "Tie-Line Bias" ;
                     rdfs:label "TLB" .


:AreaKind.borough uml:id "_3929CD68-4876-431c-820C-1B35351C339D" ;
                  rdfs:comment "Enumeration for the type of area defined for the borough" ;
                  rdfs:label "borough" .


:AreaKind.county uml:id "_715CA34A-30C0-41d4-8EB1-2CFA88D71E16" ;
                 rdfs:comment "Enumeration for the type of area defined for the county" ;
                 rdfs:label "county" .


:AreaKind.parish uml:id "_8D29E3D2-4B18-461f-9BF6-B0408BB573CA" ;
                 rdfs:comment "Enumeration for the type of area defined for the parish" ;
                 rdfs:label "parish" .


:AreaKind.serviceArea uml:id "_DC5E0522-266A-4f4e-A719-68214501E399" ;
                      rdfs:comment "Enumeration for the type of area defined for the service area" ;
                      rdfs:label "serviceArea" .


:AreaKind.state uml:id "_7339F7DB-5EA8-4cde-858B-A05EF354C5A4" ;
                rdfs:comment "Enumeration for the type of area defined for the state" ;
                rdfs:label "state" .


:AreaKind.township uml:id "_CE8703F8-3862-4d29-A177-7CE4D7ABEAD5" ;
                   rdfs:comment "Enumeration for the type of area defined for the township" ;
                   rdfs:label "township" .


:AreaKind.ward uml:id "_4492488F-93F7-4cf0-B2B8-C1433A4704BC" ;
               rdfs:comment "Enumeration for the type of area defined for the ward" ;
               rdfs:label "ward" .


:AreaKind.zipcode uml:id "_12E86C0E-2585-4289-9414-7EFB1E6EB1E5" ;
                  rdfs:comment "Enumeration for the type of area defined for the zipcode" ;
                  rdfs:label "zipcode" .


:AssetFailureClassification.defect uml:id "_C59D8E34-F7EE-403c-936F-17B7185B78B1" ;
                                   rdfs:comment "Failure due to defect." ;
                                   rdfs:label "defect" .


:AssetFailureClassification.major uml:id "_ED9CC37C-9C83-4058-988F-9980776E9879" ;
                                  rdfs:comment "Major failure." ;
                                  rdfs:label "major" .


:AssetFailureClassification.majorNeedsReplacement uml:id "_B5B93A54-EFDE-465a-B8D3-2A0AA8686718" ;
                                                  rdfs:comment "Major failure – asset needs to be replaced." ;
                                                  rdfs:label "majorNeedsReplacement" .


:AssetFailureClassification.minor uml:id "_BC3805D1-FE7F-47f4-9710-18AA2BCD6381" ;
                                  rdfs:comment "Minor failure." ;
                                  rdfs:label "minor" .


:AssetFailureMode.failToCarryLoad uml:id "_BC8AFBA8-1F26-49d5-BD0F-6E53E1212263" ;
                                  rdfs:comment "Failure to carry load." ;
                                  rdfs:label "failToCarryLoad" .


:AssetFailureMode.failToClose uml:id "_6984DA56-F93C-4218-804E-6465E1744568" ;
                              rdfs:comment "Failure to close." ;
                              rdfs:label "failToClose" .


:AssetFailureMode.failToInterrupt uml:id "_49587DE4-0847-4316-BE98-37DBF87546FC" ;
                                  rdfs:comment "Failure to interrupt." ;
                                  rdfs:label "failToInterrupt" .


:AssetFailureMode.failToOpen uml:id "_22A59BDA-8CEC-4ac6-BFC8-958E8D47EA9E" ;
                             rdfs:comment "Failure to open." ;
                             rdfs:label "failToOpen" .


:AssetFailureMode.failToProvideInsulationLevel uml:id "_4414E83D-12AD-4488-B6BE-0997E9491C13" ;
                                               rdfs:comment "Failure to provide insulation." ;
                                               rdfs:label "failToProvideInsulationLevel" .


:AssetGroupKind.analysisGroup uml:id "_84E498AF-1A4C-4996-8640-653AB193FF35" ;
                              rdfs:comment "Group is used for analysis purposes." ;
                              rdfs:label "analysisGroup" .


:AssetGroupKind.complianceGroup uml:id "_E4CB5E53-BE1E-4749-A81C-8C2F1A743F50" ;
                                rdfs:comment "Group is used for compliance purposes." ;
                                rdfs:label "complianceGroup" .


:AssetGroupKind.functionalGroup uml:id "_324D043B-837F-47d9-A38C-EDBBF534E336" ;
                                rdfs:comment "Group is used for functional purposes, for example assets which are grouped together because they are part of a for a particular function - such as a group of feeders." ;
                                rdfs:label "functionalGroup" .


:AssetGroupKind.inventoryGroup uml:id "_288A0375-4246-42d0-9CFA-ED7550BBF0AA" ;
                               rdfs:comment "Group is used for inventory purposes." ;
                               rdfs:label "inventoryGroup" .


:AssetGroupKind.other uml:id "_1C1B952C-CE7A-489e-BC8A-38B46AB59C56" ;
                      rdfs:label "other" .


:AssetHazardKind.ambientTempAbove38 uml:id "_E5545CFC-3E9B-41a8-B4F4-4B05E0E28212" ;
                                    rdfs:comment "Subject to ambient temperature above 38 °C." ;
                                    rdfs:label "ambientTempAbove38" .


:AssetHazardKind.ambientTempBelowMinus12 uml:id "_C5731FF5-5B94-4b0e-9C87-EBF1AF2BDE22" ;
                                         rdfs:comment "Subject to ambient temperature of below -12 °C." ;
                                         rdfs:label "ambientTempBelowMinus12" .


:AssetHazardKind.childrenAtPlay uml:id "_EE74DD4C-B4FF-4bd6-8D82-2B65EC8947A7" ;
                                rdfs:comment "Children play in area (stray kite/ball hazard)." ;
                                rdfs:label "childrenAtPlay" .


:AssetHazardKind.fishingArea uml:id "_923E8E6E-B00D-44fb-A376-93181CB77B65" ;
                             rdfs:comment "Fishing in area (fishing pole/line hazard)." ;
                             rdfs:label "fishingArea" .


:AssetHazardKind.other uml:id "_959A89A0-EF9D-40d4-9F73-F9EF28297FBC" ;
                       rdfs:comment "If other, look at type field for more information." ;
                       rdfs:label "other" .


:AssetHazardKind.vegetation uml:id "_5AFC3FEF-5B20-42c7-81A5-4250D7C67CA4" ;
                            rdfs:comment "Vegetation growing below asset that may cause problem." ;
                            rdfs:label "vegetation" .


:AssetKind.breakerAirBlastBreaker uml:id "_64F67AC1-7464-41d9-96A9-8F68298A9CFA" ;
                                  rdfs:comment "Air blast circuit breaker." ;
                                  rdfs:label "breakerAirBlastBreaker" .


:AssetKind.breakerBulkOilBreaker uml:id "_204DFF6B-68C0-478b-A1FC-E44EF6C19885" ;
                                 rdfs:comment "Bulk oil circuit breaker." ;
                                 rdfs:label "breakerBulkOilBreaker" .


:AssetKind.breakerInsulatingStackAssembly uml:id "_245F78CC-F5E6-4fc5-96AE-83CC504ACC89" ;
                                          rdfs:comment "Breaker insulating stack assembly (for live tank breaker)." ;
                                          rdfs:label "breakerInsulatingStackAssembly" .


:AssetKind.breakerMinimumOilBreaker uml:id "_645468F0-B634-40eb-BE39-2D5B0F2003C1" ;
                                    rdfs:comment "Minimum oil circuit breaker." ;
                                    rdfs:label "breakerMinimumOilBreaker" .


:AssetKind.breakerSF6DeadTankBreaker uml:id "_FA31EDE3-9827-4133-8E05-83F189129E55" ;
                                     rdfs:comment "SF6 dead tank breaker." ;
                                     rdfs:label "breakerSF6DeadTankBreaker" .


:AssetKind.breakerSF6LiveTankBreaker uml:id "_E2DF121F-43C4-4f8e-8927-1521902FA1F8" ;
                                     rdfs:comment "SF6 live tank breaker." ;
                                     rdfs:label "breakerSF6LiveTankBreaker" .


:AssetKind.breakerTankAssembly uml:id "_07D76E72-D58C-4c94-8272-5E98825ACAEF" ;
                               rdfs:comment "Breaker tank assembly." ;
                               rdfs:label "breakerTankAssembly" .


:AssetKind.other uml:id "_9AB12E93-A9B7-4fe4-9363-D4DDE5D0A3FD" ;
                 rdfs:comment "Other type of Asset. The type attribute may provide more details in this case." ;
                 rdfs:label "other" .


:AssetKind.transformer uml:id "_4F356D4E-EA3E-4b2b-A8A8-0E259D7AF287" ;
                       rdfs:comment "Transformer." ;
                       rdfs:label "transformer" .


:AssetKind.transformerTank uml:id "_009B1A17-21FF-4e85-85BF-925B30FA7431" ;
                           rdfs:comment "Transformer tank." ;
                           rdfs:label "transformerTank" .


:AssetLifecycleStateKind.disposedOf uml:id "_8AF24D67-5AC4-4865-8F81-359F23CE388D" ;
                                    rdfs:comment "Asset disposed of." ;
                                    rdfs:label "disposedOf" .


:AssetLifecycleStateKind.manufactured uml:id "_28F39F7B-52AF-4795-84B8-3330A88D6B81" ;
                                      rdfs:comment "Asset manufactured." ;
                                      rdfs:label "manufactured" .


:AssetLifecycleStateKind.purchased uml:id "_0109C3B7-DEE5-4643-B17F-1DFF433DDC5D" ;
                                   rdfs:comment "Asset purchased." ;
                                   rdfs:label "purchased" .


:AssetLifecycleStateKind.received uml:id "_28D023DE-3DEE-43db-94A5-CA054BBF71A5" ;
                                  rdfs:comment "Asset received." ;
                                  rdfs:label "received" .


:AssetLifecycleStateKind.retired uml:id "_3912E1A6-E64B-46ee-881D-1B2D7215888A" ;
                                 rdfs:comment "Asset retired." ;
                                 rdfs:label "retired" .


:AssetModelUsageKind.customerSubstation uml:id "_B5F26010-FAE7-4494-8666-D017F621165D" ;
                                        rdfs:comment "Asset model is intended for use in customer substation." ;
                                        rdfs:label "customerSubstation" .


:AssetModelUsageKind.distributionOverhead uml:id "_6ED2A098-34B2-4370-8738-2BF77D514B48" ;
                                          rdfs:comment "Asset model is intended for use in distribution overhead network." ;
                                          rdfs:label "distributionOverhead" .


:AssetModelUsageKind.distributionUnderground uml:id "_1AC16B3C-F46C-45b9-9FF2-BA2C4E280AC7" ;
                                             rdfs:comment "Asset model is intended for use in underground distribution network." ;
                                             rdfs:label "distributionUnderground" .


:AssetModelUsageKind.other uml:id "_CE7FC7BB-7A72-49d5-96E5-80849B98D13D" ;
                           rdfs:comment "Other kind of asset model usage." ;
                           rdfs:label "other" .


:AssetModelUsageKind.streetlight uml:id "_EA2B3AFA-B15E-47f4-81AA-54FA6B763D0C" ;
                                 rdfs:comment "Asset model is intended for use as streetlight." ;
                                 rdfs:label "streetlight" .


:AssetModelUsageKind.substation uml:id "_F0C50BB4-5DA4-47f5-8243-A1222047C338" ;
                                rdfs:comment "Asset model is intended for use in substation." ;
                                rdfs:label "substation" .


:AssetModelUsageKind.transmission uml:id "_BBDFC966-DE68-442e-B61D-71C565225F24" ;
                                  rdfs:comment "Asset model is intended for use in transmission network." ;
                                  rdfs:label "transmission" .


:AssetModelUsageKind.unknown uml:id "_74ED83A2-5135-4e9f-AB90-9C28C5B7795D" ;
                             rdfs:comment "Usage of the asset model is unknown." ;
                             rdfs:label "unknown" .


:AssetStringKind.visualExamRemarks uml:id "_C1EBE9EB-BFB1-4a23-A66C-8E2B6BFBDC8B" ;
                                   rdfs:comment """Remarks related to a visual exam.
Could be used for remarks on oil appearance resulting from visual examination, including sediment, appearance, free water.""" ;
                                   rdfs:label "visualExamRemarks" .


:AssetTemperaturePressureAnalogKind.oilPressureAtValve uml:id "_70FCFD40-A97A-4fc6-86C9-17E719AD73E4" ;
                                                       rdfs:comment "Oil pressure at valve (in KPa)." ;
                                                       rdfs:label "oilPressureAtValve" .


:AssetTemperaturePressureAnalogKind.oilTemperatureAtValve uml:id "_0B9E7C36-612D-4653-A9D3-24D93321F96F" ;
                                                          rdfs:comment "Oil temperature at valve (in °C)." ;
                                                          rdfs:label "oilTemperatureAtValve" .


:AsynchronousMachineKind.generator uml:id "_E653D495-7583-4d27-A25F-AADBBA7D9B8D" ;
                                   rdfs:comment "The Asynchronous Machine is a generator." ;
                                   rdfs:label "generator" .


:AsynchronousMachineKind.motor uml:id "_E6162696-2DA3-413f-AA16-9713D25F040B" ;
                               rdfs:comment "The Asynchronous Machine is a motor." ;
                               rdfs:label "motor" .


:AtmosphericAnalogKind.albedo uml:id "_F7C31D2F-3FC9-46cc-9287-EB11633B39B8" ;
                              rdfs:label "albedo" .


:AtmosphericAnalogKind.ambientTemperature uml:id "_4FE54B9C-C5AB-4f72-BF51-D59B94B1B910" ;
                                          rdfs:comment "The temperature measured b<font color=\"#0f0f0f\">y a thermometer exposed to the air in a place sheltered from direct solar radiation. </font>Also known as \"dry bulb\" because<font color=\"#0f0f0f\"> the air temperature is indicated by a thermometer not affecte</font>d by the moisture of the air." ;
                                          rdfs:label "ambientTemperature" .


:AtmosphericAnalogKind.atmosphericPressure uml:id "_BC2F397D-79F9-4d3e-9874-38736385F173" ;
                                           rdfs:label "atmosphericPressure" .


:AtmosphericAnalogKind.ceiling uml:id "_D7BD1247-0588-4fd1-AF7B-41C06773BB54" ;
                               rdfs:label "ceiling" .


:AtmosphericAnalogKind.dewPoint uml:id "_9A65200F-CB0D-4e54-9FC7-60DF77641567" ;
                                rdfs:comment "The temperature to which air must be cooled at constant pressure and constant water-vapor content in order for saturation to occur. In other words, it is the temperature at which water vapor starts to condense out of the air." ;
                                rdfs:label "dewPoint" .


:AtmosphericAnalogKind.heatIndex uml:id "_E889DA88-ABFB-4c66-8396-6128878D7C0B" ;
                                 rdfs:comment "The temperature of how hot it \"feels like\" for a given combination of warm air temperature and relative humidity." ;
                                 rdfs:label "heatIndex" .


:AtmosphericAnalogKind.horizontalVisibility uml:id "_15E251C6-5E47-4b94-95BA-DDB29EFD683C" ;
                                            rdfs:label "horizontalVisibility" .


:AtmosphericAnalogKind.humidity uml:id "_961A04DA-2A6D-4bf8-98B5-7CC5627F033D" ;
                                rdfs:label "humidity" .


:AtmosphericAnalogKind.ice uml:id "_14B099E9-1584-40f0-8993-BB26C648A6EE" ;
                           rdfs:label "ice" .


:AtmosphericAnalogKind.illuminanceDiffuseHorizontal uml:id "_3C1CD5F6-1832-48e4-B1F8-B0D2B98E0710" ;
                                                    rdfs:label "illuminanceDiffuseHorizontal" .


:AtmosphericAnalogKind.illuminanceDirectNormal uml:id "_88EED2B0-387B-4cd5-BF84-BC3B6495FBC1" ;
                                               rdfs:label "illuminanceDirectNormal" .


:AtmosphericAnalogKind.illuminanceGlobalHorizontal uml:id "_5770A7B8-E33B-4098-A2DB-19FFDE192BB9" ;
                                                   rdfs:label "illuminanceGlobalHorizontal" .


:AtmosphericAnalogKind.irradianceDiffuseHorizonal uml:id "_CDE68F44-2AEF-4fb7-BAFD-A6BDDDF2CAE2" ;
                                                  rdfs:label "irradianceDiffuseHorizonal" .


:AtmosphericAnalogKind.irradianceDirectNormal uml:id "_620FA028-98F6-40b4-B4FA-21F0AA1417A7" ;
                                              rdfs:label "irradianceDirectNormal" .


:AtmosphericAnalogKind.irradianceExtraTerrestrialHorizontal uml:id "_ADF07F5C-4E2F-4e02-A523-0E064AFE7432" ;
                                                            rdfs:label "irradianceExtraTerrestrialHorizontal" .


:AtmosphericAnalogKind.irradianceExtraTerrestrialVertical uml:id "_CE2CD05C-77FD-48a7-9790-E601A531EEFF" ;
                                                          rdfs:label "irradianceExtraTerrestrialVertical" .


:AtmosphericAnalogKind.irradianceGlobalHorizontal uml:id "_BB71B4FF-D561-4290-9806-C8BB579885C1" ;
                                                  rdfs:label "irradianceGlobalHorizontal" .


:AtmosphericAnalogKind.luminanceZenith uml:id "_8BAD88FA-5CDE-49cc-B14E-30AEB55A2F61" ;
                                       rdfs:label "luminanceZenith" .


:AtmosphericAnalogKind.precipitation uml:id "_EED8F27E-A300-4ac2-A1F3-4FE31CCFAE4C" ;
                                     rdfs:label "precipitation" .


:AtmosphericAnalogKind.rain uml:id "_F43421C9-EA43-4bc8-8DA9-C15DA0C2C0C8" ;
                            rdfs:label "rain" .


:AtmosphericAnalogKind.skyCoverageOpaque uml:id "_56E468AF-7A3C-47f6-AD89-A9A39C58B2AD" ;
                                         rdfs:label "skyCoverageOpaque" .


:AtmosphericAnalogKind.skyCoverageTotal uml:id "_DA76CE2B-E30A-43b2-9DB3-40126B665E18" ;
                                        rdfs:label "skyCoverageTotal" .


:AtmosphericAnalogKind.snow uml:id "_1765835F-C903-4b1d-B159-48E0BDCD7C35" ;
                            rdfs:comment "Snow amount over a specified period of time." ;
                            rdfs:label "snow" .


:AtmosphericAnalogKind.verticalVisibility uml:id "_BFE4FB1D-0F10-4e2d-AB91-CAED287EF526" ;
                                          rdfs:label "verticalVisibility" .


:AtmosphericAnalogKind.windChill uml:id "_AEB4943D-73A5-45be-91A9-C0DBA3A09D04" ;
                                 rdfs:comment "The temperature of how cold it \"feels like\" based on the rate of heat loss from exposed skin caused by the effects of wind and cold temperatures." ;
                                 rdfs:label "windChill" .


:AtmosphericAnalogKind.windSpeedGust uml:id "_3B9CA816-E9DD-4d8b-A499-F524781BAA20" ;
                                     rdfs:comment """Maximum instantaneous wind speed in the 10 minute period preceding a moment in time so long as more than 10 knots of difference has been exhibited between peaks and lulls during that 10 minute time period. 
0 value means no gusts during preceding 10 minute period.""" ;
                                     rdfs:label "windSpeedGust" .


:AtmosphericAnalogKind.windSpeedInstantaneous uml:id "_507CC39E-3D99-407b-BDC3-C223A8143CE1" ;
                                              rdfs:comment "Wind speed at a moment in time." ;
                                              rdfs:label "windSpeedInstantaneous" .


:AtmosphericAnalogKind.windSpeedPeak uml:id "_3EF88313-0BC4-4bed-8E93-BAD793562834" ;
                                     rdfs:comment """Peak instantaneous wind speed in the 60 minutes preceding a moment in time as long as peak speed greater than 25 knots.  
0 value means speed did not exceed 25 knots during preceding 60 minutes.""" ;
                                     rdfs:label "windSpeedPeak" .


:AtmosphericAnalogKind.windSpeedSustained uml:id "_5BDCE21C-C0DD-4109-A684-0634C501D7C3" ;
                                          rdfs:comment "Average instantaneous wind speed over the 2-minute time period preceding a moment in time." ;
                                          rdfs:label "windSpeedSustained" .


:AutomaticDispInstTypeCommitment.DR_ADJUSTMENT uml:id "_88D3E8D4-20C0-489a-9093-068E8D6CC8D3" ;
                                               rdfs:comment "Distributed Resource adjustment for a distributed resource that is already deployed (committed)." ;
                                               rdfs:label "DR_ADJUSTMENT" .


:AutomaticDispInstTypeCommitment.DR_DEPLOY uml:id "_363089D0-44BD-4251-97DA-08F1A2D5FBC5" ;
                                           rdfs:comment "Distributed Resource Deployment" ;
                                           rdfs:label "DR_DEPLOY" .


:AutomaticDispInstTypeCommitment.DR_RELEASE uml:id "_E1091FD6-5614-4b21-BC00-2EBAC0863B24" ;
                                            rdfs:comment "Distributed Resource Release" ;
                                            rdfs:label "DR_RELEASE" .


:AutomaticDispInstTypeCommitment.SHUT_DOWN uml:id "_C54CF1F7-CA46-4aae-B9DE-2130AA3DA9D0" ;
                                           rdfs:comment "Shut down instruction type" ;
                                           rdfs:label "SHUT_DOWN" .


:AutomaticDispInstTypeCommitment.START_UP uml:id "_AECF94B1-E588-4524-AE1A-DD7900ECEB33" ;
                                          rdfs:comment "Start up instruction type" ;
                                          rdfs:label "START_UP" .


:AutomaticDispatchMode.CONTINGENCY uml:id "_145F07A8-BC24-4ef9-8BCF-05AC357466E1" ;
                                   rdfs:comment "Contingnency occurance, redispatch of contingency reserves" ;
                                   rdfs:label "CONTINGENCY" .


:AutomaticDispatchMode.INTERVAL uml:id "_E69BDCB2-900A-4e6c-AE51-008E4B4EE47A" ;
                                rdfs:label "INTERVAL" .


:AutomaticDispatchMode.MANUAL uml:id "_9ED4EDCA-C53D-448f-98F6-F44601BEB2E2" ;
                              rdfs:comment "Operator override" ;
                              rdfs:label "MANUAL" .


:BatteryStateKind.charging uml:id "_19F34FA8-CFB2-4bbc-8B63-905A12841965" ;
                           rdfs:comment "Stored energy is increasing." ;
                           rdfs:label "charging" .


:BatteryStateKind.discharging uml:id "_5CD0E68E-41E4-40c8-85CD-498A0BBA1B48" ;
                              rdfs:comment "Stored energy is decreasing." ;
                              rdfs:label "discharging" .


:BatteryStateKind.empty uml:id "_4B8424DA-BED2-454e-BC4A-DAFC677E11B5" ;
                        rdfs:comment "Unable to discharge, and not charging." ;
                        rdfs:label "empty" .


:BatteryStateKind.full uml:id "_9AA779C1-DB12-475b-AB95-2028A9EF2645" ;
                       rdfs:comment "Unable to charge, and not discharging." ;
                       rdfs:label "full" .


:BatteryStateKind.waiting uml:id "_79E0E262-7061-4525-B997-D9234C824409" ;
                          rdfs:comment "Neither charging nor discharging, but able to do so." ;
                          rdfs:label "waiting" .


:BidCalculationBasis.COST_BASED uml:id "_3C8BD9B5-142A-4b59-B2E3-302068248ED2" ;
                                rdfs:comment "Based on unit generation characteristics and a cost of fuel." ;
                                rdfs:label "COST_BASED" .


:BidCalculationBasis.LMP_BASED uml:id "_60982D3F-D14F-4568-86E2-2CB393343FE8" ;
                               rdfs:comment "Based on prices paid at particular pricing location." ;
                               rdfs:label "LMP_BASED" .


:BidCalculationBasis.NEGOTIATED uml:id "_FADE5432-E8BE-4bf0-BD9E-8B2D5619F3E0" ;
                                rdfs:comment "An amount negotiated with the designated Independent Entity." ;
                                rdfs:label "NEGOTIATED" .


:BidMitigationStatus.B uml:id "_C4D0EAF7-C494-40a8-84C9-598EA9485F48" ;
                       rdfs:label "B" .


:BidMitigationStatus.L uml:id "_4792BB9B-5A40-4780-8B68-D52F4281EB61" ;
                       rdfs:label "L" .


:BidMitigationStatus.M uml:id "_490C9A04-7542-4a77-BA29-E7C96D7B9F8F" ;
                       rdfs:label "M" .


:BidMitigationStatus.O uml:id "_A21A8DA5-E6E3-4d9a-8549-F0FE59617E57" ;
                       rdfs:label "O" .


:BidMitigationStatus.R uml:id "_5646D065-FFEC-4a27-9534-66B4E3D0D78E" ;
                       rdfs:label "R" .


:BidMitigationStatus.S uml:id "_86F8419D-B58B-47d6-B678-7C6C50873CB2" ;
                       rdfs:label "S" .


:BidMitigationType.F uml:id "_033EDE23-864E-4751-9BB0-53611D5DC16D" ;
                     rdfs:label "F" .


:BidMitigationType.I uml:id "_F7255C9A-75D1-4a92-8E19-2DC7B1845F2B" ;
                     rdfs:label "I" .


:BidPriceCapType.AS uml:id "_B8F847D2-664E-43a6-886E-6342ADA566F0" ;
                    rdfs:label "AS" .


:BidPriceCapType.ENERGY uml:id "_A226A539-6CD7-4d1b-992A-CEB50BB0E8CE" ;
                        rdfs:label "ENERGY" .


:BidPriceCapType.RUC uml:id "_61D1EE41-146B-4dae-BBF1-7C9BEF82459D" ;
                     rdfs:label "RUC" .


:BidStatusType.CL uml:id "_49098747-2A88-47b8-A1D6-77A8FBEA25DB" ;
                  rdfs:comment "Clean" ;
                  rdfs:label "CL" .


:BidStatusType.CM uml:id "_8BCB7E1F-B2FB-49ce-9F69-CBD97A35923B" ;
                  rdfs:label "CM" .


:BidStatusType.CV uml:id "_E5CF645E-38B1-4233-A269-CE5A7A117D04" ;
                  rdfs:label "CV" .


:BidStatusType.CX uml:id "_49A64F56-232D-4136-AAF4-27E21660C949" ;
                  rdfs:label "CX" .


:BidStatusType.I uml:id "_05B0D64E-4EB5-4590-A72E-F42B533043B9" ;
                 rdfs:label "I" .


:BidStatusType.M uml:id "_1495BE4A-1BFE-4683-83C1-759426CDE994" ;
                 rdfs:label "M" .


:BidStatusType.O uml:id "_892581DE-44E3-4506-A5B3-53181D981B49" ;
                 rdfs:label "O" .


:BidStatusType.RJ uml:id "_E76778FA-5D75-4883-84AC-1FA893EC8F58" ;
                  rdfs:label "RJ" .


:BidStatusType.RP uml:id "_77ED80BF-A4C4-4db7-BBF3-9D3EA8E4150F" ;
                  rdfs:comment "Replicated" ;
                  rdfs:label "RP" .


:BidStatusType.V uml:id "_78899B17-1E27-4a20-A713-6157B99766DF" ;
                 rdfs:label "V" .


:BidType.DEFAULT_ENERGY_BID uml:id "_485E00C2-D4D5-4192-A756-110CA1FF20E5" ;
                            rdfs:label "DEFAULT_ENERGY_BID" .


:BidType.DEFAULT_MINIMUM_LOAD_BID uml:id "_5341E9E9-21FF-474c-B677-7EF93EFFCE9B" ;
                                  rdfs:label "DEFAULT_MINIMUM_LOAD_BID" .


:BidType.DEFAULT_STARTUP_BID uml:id "_2CB5899E-E095-48d9-B2AF-725E1BE9FD3C" ;
                             rdfs:label "DEFAULT_STARTUP_BID" .


:BidTypeRMR.QUALIFIED_PREDISPATCH uml:id "_71A8181E-FA3C-47a9-9EFC-E8D17835749F" ;
                                  rdfs:comment "Output of requirements bid self schedule type." ;
                                  rdfs:label "QUALIFIED_PREDISPATCH" .


:BidTypeRMR.REQUIREMENTS uml:id "_213F51F9-E327-444e-A091-EEE8382D40AE" ;
                         rdfs:comment "Qualified pre-dispatch bid self schedule type." ;
                         rdfs:label "REQUIREMENTS" .


:BillMediaKind.electronic uml:id "_9D40AF79-6BCE-4546-8347-CE426C906A98" ;
                          rdfs:label "electronic" .


:BillMediaKind.other uml:id "_4B3E1B7D-511A-4dac-AB6E-3FAF621EEFC7" ;
                     rdfs:label "other" .


:BillMediaKind.paper uml:id "_96375195-3F19-4e72-B221-BE5667F4D01A" ;
                     rdfs:label "paper" .


:BoilerControlMode.coordinated uml:id "_036BAB41-592D-433b-B36F-092A7D6E2330" ;
                               rdfs:comment "Coordinated." ;
                               rdfs:label "coordinated" .


:BoilerControlMode.following uml:id "_3CD1CFD7-EE28-41ac-9047-1B4C3B36ABBA" ;
                             rdfs:comment "Following." ;
                             rdfs:label "following" .


:BreakerApplicationKind.busBreaker uml:id "_4FA244F8-1694-4747-9447-FA257ADFDE3B" ;
                                   rdfs:comment "Bus breaker." ;
                                   rdfs:label "busBreaker" .


:BreakerApplicationKind.busTieBreaker uml:id "_342FF631-EEB2-4d74-A885-D97702020173" ;
                                      rdfs:comment "Bus tie breaker." ;
                                      rdfs:label "busTieBreaker" .


:BreakerApplicationKind.capacitorOrReactorBankBreaker uml:id "_1BC876E5-0C72-49dd-917D-47697F53214B" ;
                                                      rdfs:comment "Capacitor or reactor breaker." ;
                                                      rdfs:label "capacitorOrReactorBankBreaker" .


:BreakerApplicationKind.feederBreaker uml:id "_791AEB01-5504-45ce-B008-4A45D2C728F4" ;
                                      rdfs:comment "Feeder breaker." ;
                                      rdfs:label "feederBreaker" .


:BreakerApplicationKind.other uml:id "_2412CD72-B6DC-40e0-A74D-F9F413521864" ;
                              rdfs:comment "Other type of breaker application." ;
                              rdfs:label "other" .


:BreakerApplicationKind.spare uml:id "_F770F3AE-6956-41b6-A8DE-9BA9382FEF1E" ;
                              rdfs:comment "Spare breaker." ;
                              rdfs:label "spare" .


:BreakerApplicationKind.stepUpTransformerBreakerFossil uml:id "_0CE3C176-B0FC-4fe9-8466-DA7F5A03D47F" ;
                                                       rdfs:comment "Step-up transformer breaker for fossil generator." ;
                                                       rdfs:label "stepUpTransformerBreakerFossil" .


:BreakerApplicationKind.stepUpTransformerBreakerHydro uml:id "_8BBD5334-7024-4df4-BB94-6E7DD153D881" ;
                                                      rdfs:comment "Step-up transformer breaker for hydro generator." ;
                                                      rdfs:label "stepUpTransformerBreakerHydro" .


:BreakerApplicationKind.stepUpTransformerBreakerNuclear uml:id "_4FE9C0BF-BDD7-46fa-9BAF-47CEF7A5E106" ;
                                                        rdfs:comment "Step-up transformer breaker for nuclear generator." ;
                                                        rdfs:label "stepUpTransformerBreakerNuclear" .


:BreakerApplicationKind.stepUpTransformerBreakerPumpedStorage uml:id "_5540B1FB-605A-42ad-88F9-12D1D562BD88" ;
                                                              rdfs:comment "Step-up transformer breaker for pumped storage." ;
                                                              rdfs:label "stepUpTransformerBreakerPumpedStorage" .


:BreakerApplicationKind.substationTransformerBreaker uml:id "_E27B9F71-639C-4aa2-AEB0-F3C158F2BD60" ;
                                                     rdfs:comment "Substation transformer breaker." ;
                                                     rdfs:label "substationTransformerBreaker" .


:BreakerApplicationKind.transmissionFlowGateLineBreaker uml:id "_2B479A74-AD9E-4530-BDF0-3036FA2F0090" ;
                                                        rdfs:comment "Transmission flow gate line breaker." ;
                                                        rdfs:label "transmissionFlowGateLineBreaker" .


:BreakerApplicationKind.transmissionLineBreaker uml:id "_8C8FF9FE-0B1B-462d-A459-FF5BD1AC68D3" ;
                                                rdfs:comment "Transmission line breaker." ;
                                                rdfs:label "transmissionLineBreaker" .


:BreakerApplicationKind.transmissionTieLineBreaker uml:id "_84E245C8-B94C-4076-81AF-1BECF0D14836" ;
                                                   rdfs:comment "Transmission tie line breaker." ;
                                                   rdfs:label "transmissionTieLineBreaker" .


:BreakerConfiguration.breakerAndAHalf uml:id "_0B0C09C4-66E5-48db-85B5-7BBCB3FB2759" ;
                                      rdfs:comment "Breaker and a half." ;
                                      rdfs:label "breakerAndAHalf" .


:BreakerConfiguration.doubleBreaker uml:id "_8D041086-6214-4bc0-8351-D8A680FEC6E3" ;
                                    rdfs:comment "Double breaker." ;
                                    rdfs:label "doubleBreaker" .


:BreakerConfiguration.noBreaker uml:id "_00F5D8BD-3E07-4371-B7A3-29276B241276" ;
                                rdfs:comment "No breaker." ;
                                rdfs:label "noBreaker" .


:BreakerConfiguration.singleBreaker uml:id "_44DB9F68-B210-48a4-9625-F25A2CB91A8C" ;
                                    rdfs:comment "Single breaker." ;
                                    rdfs:label "singleBreaker" .


:BreakerFailureReasonKind.SF6BlastValveFailure uml:id "_F75C1CC3-1525-4910-8EBA-9CF3011AB144" ;
                                               rdfs:comment "SF6 blast valve failure." ;
                                               rdfs:label "SF6BlastValveFailure" .


:BreakerFailureReasonKind.SF6PufferFailure uml:id "_1AE66382-078A-472a-9563-4383B19508F2" ;
                                           rdfs:comment "SF6 puffer valve failure." ;
                                           rdfs:label "SF6PufferFailure" .


:BreakerFailureReasonKind.blastValveFailure uml:id "_30D60A7E-E991-4fc6-B21E-70BFBB425D5D" ;
                                            rdfs:comment "Blast valve failure." ;
                                            rdfs:label "blastValveFailure" .


:BreakerFailureReasonKind.bushingFailure uml:id "_0C2E4CDF-CA9E-4043-9744-D16A8CE5929D" ;
                                         rdfs:comment "Bushing failure." ;
                                         rdfs:label "bushingFailure" .


:BreakerFailureReasonKind.closeCoilOpenShortedFailed uml:id "_598C82C0-1BD0-458f-B62A-4716F7CDD835" ;
                                                     rdfs:comment "Close coil open shorted failure." ;
                                                     rdfs:label "closeCoilOpenShortedFailed" .


:BreakerFailureReasonKind.contaminatedAir uml:id "_40FC0A16-177F-4dc3-ADF8-8A8AC8970E4D" ;
                                          rdfs:comment "Contaminated air." ;
                                          rdfs:label "contaminatedAir" .


:BreakerFailureReasonKind.contaminatedArcChutes uml:id "_A4BCADEA-5A86-49f1-BE9B-4DF1829FB387" ;
                                                rdfs:comment "Contaminated arc chutes." ;
                                                rdfs:label "contaminatedArcChutes" .


:BreakerFailureReasonKind.contaminatedGas uml:id "_F8BD9B53-5B89-45ea-8537-5C2881E649EB" ;
                                          rdfs:comment "Contaminated gas." ;
                                          rdfs:label "contaminatedGas" .


:BreakerFailureReasonKind.contaminatedGasAir uml:id "_D96E9F2F-10EA-4943-8271-C9C9B0F97922" ;
                                             rdfs:comment "Contaminated gas or air." ;
                                             rdfs:label "contaminatedGasAir" .


:BreakerFailureReasonKind.controlCircuitFailure uml:id "_FD4B790B-BB62-481c-834A-D830D73BD35A" ;
                                                rdfs:comment "Control circuit failure." ;
                                                rdfs:label "controlCircuitFailure" .


:BreakerFailureReasonKind.degradedLubrication uml:id "_E7C04C52-E42D-4c34-8EDC-6226AA91F8B1" ;
                                              rdfs:comment "Degraded lubrication." ;
                                              rdfs:label "degradedLubrication" .


:BreakerFailureReasonKind.externalOrInternalContamination uml:id "_635231A2-A6EA-4a16-B927-4907A25B0294" ;
                                                          rdfs:comment "External or internal contamination." ;
                                                          rdfs:label "externalOrInternalContamination" .


:BreakerFailureReasonKind.highPressureAirPlant uml:id "_6F6FE842-77C2-4692-8851-9ADAF60B772B" ;
                                               rdfs:comment "High pressure air plant." ;
                                               rdfs:label "highPressureAirPlant" .


:BreakerFailureReasonKind.highResistanceLoadPath uml:id "_14814CF1-0523-48dc-ADC5-B1518DA4A37F" ;
                                                 rdfs:comment "High resistance load path." ;
                                                 rdfs:label "highResistanceLoadPath" .


:BreakerFailureReasonKind.highResistancePath uml:id "_DB42A410-F347-4887-BCC4-67FB2747ED48" ;
                                             rdfs:comment "High resistance path." ;
                                             rdfs:label "highResistancePath" .


:BreakerFailureReasonKind.interrupterContactFailure uml:id "_266CD3BD-A7D4-4cda-AFD7-9AAF3028E9FF" ;
                                                    rdfs:comment "Interrupter contact failure." ;
                                                    rdfs:label "interrupterContactFailure" .


:BreakerFailureReasonKind.interrupterFailure uml:id "_119D2755-1EE4-444a-AFC5-F6A512FF1C99" ;
                                             rdfs:comment "Interrupter failure." ;
                                             rdfs:label "interrupterFailure" .


:BreakerFailureReasonKind.linkageFailure uml:id "_9FAC53B6-5CF0-4489-B539-73D9EB0452F9" ;
                                         rdfs:comment "Linkage failure." ;
                                         rdfs:label "linkageFailure" .


:BreakerFailureReasonKind.lossOfOil uml:id "_E69F5C96-B3CC-4f57-AB73-189F070BA74F" ;
                                    rdfs:comment "Loss of oil." ;
                                    rdfs:label "lossOfOil" .


:BreakerFailureReasonKind.lossOfVacuum uml:id "_9C68430E-7EF3-499d-9499-969960EA5D02" ;
                                       rdfs:comment "Loss of vacuum." ;
                                       rdfs:label "lossOfVacuum" .


:BreakerFailureReasonKind.lowGasPressure uml:id "_1A86799C-29CF-49c9-921D-5FF2901268D1" ;
                                         rdfs:comment "Low gas pressure." ;
                                         rdfs:label "lowGasPressure" .


:BreakerFailureReasonKind.mechanismFailure uml:id "_1AF7B0DB-E199-4396-BF95-2FAFAF6787AE" ;
                                           rdfs:comment "Blast valve failure." ;
                                           rdfs:label "mechanismFailure" .


:BreakerFailureReasonKind.mechanismOrLinkageFailure uml:id "_2B69A66D-1E27-4015-AEBA-84BA097AEDED" ;
                                                    rdfs:comment "Mechanism or linkage failure." ;
                                                    rdfs:label "mechanismOrLinkageFailure" .


:BreakerFailureReasonKind.oilRelatedFailure uml:id "_8B7758DC-059B-42a9-99E1-60B2CBA41E62" ;
                                            rdfs:comment "Oil-related failure." ;
                                            rdfs:label "oilRelatedFailure" .


:BreakerFailureReasonKind.poorOilQuality uml:id "_AE5C859C-3972-4fb9-AD23-971A091DF1A9" ;
                                         rdfs:comment "Poor oil quality." ;
                                         rdfs:label "poorOilQuality" .


:BreakerFailureReasonKind.rackingMechanismFailure uml:id "_71B4D41D-E47C-4b62-A51B-B19694D76A72" ;
                                                  rdfs:comment "Racking mechanism failure." ;
                                                  rdfs:label "rackingMechanismFailure" .


:BreakerFailureReasonKind.resistorFailure uml:id "_CA6CD667-DC2F-4b9d-AF5B-024F7FA4AE65" ;
                                          rdfs:comment "Resistor failure." ;
                                          rdfs:label "resistorFailure" .


:BreakerFailureReasonKind.resistorGradingCapacitorFailure uml:id "_33D82F13-D3F4-4649-A83C-C7DCA99C9E7D" ;
                                                          rdfs:comment "Resistor grading capacitor failure." ;
                                                          rdfs:label "resistorGradingCapacitorFailure" .


:BreakerFailureReasonKind.solidDielectricFailure uml:id "_4E8628FE-8199-49e2-9F55-CC4B4146857D" ;
                                                 rdfs:comment "Solid dielectric failure." ;
                                                 rdfs:label "solidDielectricFailure" .


:BreakerFailureReasonKind.storedEnergyFailure uml:id "_F67A3E04-02F7-4078-8385-967AAEA98C98" ;
                                              rdfs:comment "Stored energy failure." ;
                                              rdfs:label "storedEnergyFailure" .


:BreakerFailureReasonKind.tripCoilOpenShortedFailed uml:id "_5168F141-0FA3-4f48-A286-39806DF28301" ;
                                                    rdfs:comment "Trip coil open shorted failure." ;
                                                    rdfs:label "tripCoilOpenShortedFailed" .


:BreakerMaintenanceKind.externalOutOfService uml:id "_F5FCE584-3E21-4639-A56A-A34F7AC7C767" ;
                                             rdfs:comment "External out-of-service inspection and maintenance." ;
                                             rdfs:label "externalOutOfService" .


:BreakerMaintenanceKind.internalOutOfService uml:id "_57B6C89F-DBBB-4e87-AB83-473AC3377D75" ;
                                             rdfs:comment "Internal (interrupter) inspection and maintenance (breaker out of service)." ;
                                             rdfs:label "internalOutOfService" .


:BreakerMaintenanceKind.interrupterOverhaul uml:id "_158D75EA-8DF1-4fdc-8658-25C51D6B5B1E" ;
                                            rdfs:comment "Overhaul of breaker interrupter unit." ;
                                            rdfs:label "interrupterOverhaul" .


:BreakerRepairItemKind.SF6GasLeak uml:id "_6EF4F61C-7371-4a16-AEEA-C33EDFB90FC8" ;
                                  rdfs:comment "SF6 gas leak repair." ;
                                  rdfs:label "SF6GasLeak" .


:BreakerRepairItemKind.airCompressor uml:id "_0FC7B2AC-13B8-4421-843C-09D82D9283E0" ;
                                     rdfs:comment "Air compressor repair." ;
                                     rdfs:label "airCompressor" .


:BreakerRepairItemKind.auxiliarySwitchAndLinkage uml:id "_765E9B4D-3EFB-408a-BD4E-36E4D344D5A1" ;
                                                 rdfs:comment "Auxiliary switch and linkage repair." ;
                                                 rdfs:label "auxiliarySwitchAndLinkage" .


:BreakerRepairItemKind.busConnection uml:id "_F4A920ED-2048-40bb-AFA9-8A4F5D208E07" ;
                                     rdfs:comment "Bus connection repair." ;
                                     rdfs:label "busConnection" .


:BreakerRepairItemKind.checkValve uml:id "_F218AEBC-2752-4114-86F2-32D93105B8D9" ;
                                  rdfs:comment "Check valve repair." ;
                                  rdfs:label "checkValve" .


:BreakerRepairItemKind.closeCoil uml:id "_DFEB79AD-55B7-421e-A048-5050F76E6C21" ;
                                 rdfs:comment "Close coil repair." ;
                                 rdfs:label "closeCoil" .


:BreakerRepairItemKind.contactor uml:id "_28593F12-179B-4a07-9E06-6DCF7B1E7B38" ;
                                 rdfs:comment "Contactor repair." ;
                                 rdfs:label "contactor" .


:BreakerRepairItemKind.controlCircuit uml:id "_48FE5505-F845-4c4a-8474-B580958F193D" ;
                                      rdfs:comment "Control circuit repair." ;
                                      rdfs:label "controlCircuit" .


:BreakerRepairItemKind.corrosion uml:id "_E647042E-9A24-4962-A24E-9847257EF246" ;
                                 rdfs:comment "Corrosion repair." ;
                                 rdfs:label "corrosion" .


:BreakerRepairItemKind.gasDensitySupervision uml:id "_9D70E59A-B77B-4b9e-A9E2-853A2546BBE3" ;
                                             rdfs:comment "Gas density supervision repair." ;
                                             rdfs:label "gasDensitySupervision" .


:BreakerRepairItemKind.heaterOrThermostat uml:id "_1E0C0CE0-1955-4671-8F25-9FB6791C70DC" ;
                                          rdfs:comment "Heater or thermostat repair." ;
                                          rdfs:label "heaterOrThermostat" .


:BreakerRepairItemKind.hydraulicFluidLeak uml:id "_7A440D56-E870-41cb-B0D9-95523DADDEAD" ;
                                          rdfs:comment "Hydraulic fluid leak repair." ;
                                          rdfs:label "hydraulicFluidLeak" .


:BreakerRepairItemKind.interrupterAssembly uml:id "_C356BC95-3673-4ee1-B4C1-5E4979528A07" ;
                                           rdfs:comment "Interrupter assembly repair." ;
                                           rdfs:label "interrupterAssembly" .


:BreakerRepairItemKind.other uml:id "_7BA92C88-9ABF-45d3-B503-5C4E986A9F9D" ;
                             rdfs:comment "Other type of repair." ;
                             rdfs:label "other" .


:BreakerRepairItemKind.positionIndicator uml:id "_F3B0D423-453E-4444-9C73-6BF505E4ACA0" ;
                                         rdfs:comment "Position indicator repair." ;
                                         rdfs:label "positionIndicator" .


:BreakerRepairItemKind.pressureSwitch uml:id "_43C27BDF-C086-40a7-9C98-2C25C18B4742" ;
                                      rdfs:comment "Pressure switch repair." ;
                                      rdfs:label "pressureSwitch" .


:BreakerRepairItemKind.pumpOrMotor uml:id "_3D419495-6544-4532-851B-B8FD3F871B85" ;
                                   rdfs:comment "Pump or motor repair." ;
                                   rdfs:label "pumpOrMotor" .


:BreakerRepairItemKind.relay uml:id "_798D9F89-D529-433e-8BA2-639E167D63B9" ;
                             rdfs:comment "Relay repair." ;
                             rdfs:label "relay" .


:BreakerRepairItemKind.storedEnergySystem uml:id "_4848DA7A-EE14-4f31-8A69-E702FF19ADDA" ;
                                          rdfs:comment "Stored energy system repair." ;
                                          rdfs:label "storedEnergySystem" .


:BreakerRepairItemKind.tripCoil uml:id "_4EB5C04D-B6E6-4298-9687-E300630545FC" ;
                                rdfs:comment "Trip coil repair." ;
                                rdfs:label "tripCoil" .


:BreakerRepairItemKind.tripControlValve uml:id "_BA2C3D1E-6EF1-455b-90F0-15FBA02D48A7" ;
                                        rdfs:comment "Trip control valve repair." ;
                                        rdfs:label "tripControlValve" .


:BreakerRepairItemKind.wiring uml:id "_1173068F-6C90-4d1f-9442-D06B4860D0D6" ;
                              rdfs:comment "Wiring repair." ;
                              rdfs:label "wiring" .


:BusbarConfiguration.doubleBus uml:id "_4818CA4D-1A75-4e80-9364-CF5DF7873944" ;
                               rdfs:comment "Double bus." ;
                               rdfs:label "doubleBus" .


:BusbarConfiguration.mainWithTransfer uml:id "_8DC02787-5BEC-4701-A919-193EEB5A6656" ;
                                      rdfs:comment "Main bus with transfer bus." ;
                                      rdfs:label "mainWithTransfer" .


:BusbarConfiguration.ringBus uml:id "_51ADB6A4-ED54-49e2-95C0-85BF285C3C8F" ;
                             rdfs:comment "Ring bus." ;
                             rdfs:label "ringBus" .


:BusbarConfiguration.singleBus uml:id "_C252873E-93AB-4837-BFA2-72F7ED949063" ;
                               rdfs:comment "Single bus." ;
                               rdfs:label "singleBus" .


:BushingInsulationKind.compound uml:id "_9D9E8358-AB7A-4422-8953-3DBDCB84F82C" ;
                                rdfs:comment "Compound." ;
                                rdfs:label "compound" .


:BushingInsulationKind.oilImpregnatedPaper uml:id "_10CD10DB-B4DC-4a26-AA55-5FF2BC8EEC16" ;
                                           rdfs:comment "Oil impregnated paper." ;
                                           rdfs:label "oilImpregnatedPaper" .


:BushingInsulationKind.other uml:id "_92800D2C-7E59-4f6c-8565-B6E4F0AFC163" ;
                             rdfs:comment "Other." ;
                             rdfs:label "other" .


:BushingInsulationKind.resinBondedPaper uml:id "_2DE129E3-F2CD-4b33-BC93-643531E13034" ;
                                        rdfs:comment "Resin bonded paper." ;
                                        rdfs:label "resinBondedPaper" .


:BushingInsulationKind.resinImpregnatedPaper uml:id "_7CAAF319-98A0-4acf-A256-7405FFFB4990" ;
                                             rdfs:comment "Resin impregnated paper." ;
                                             rdfs:label "resinImpregnatedPaper" .


:BushingInsulationKind.solidPorcelain uml:id "_6C222A3A-CD9D-46b0-B6E3-7017F736EB4B" ;
                                      rdfs:comment "Solid porcelain." ;
                                      rdfs:label "solidPorcelain" .


:BushingInsulationPfTestKind.c1 uml:id "_9F16553C-1F0F-4dc4-B0FC-9A02AA952BAF" ;
                                rdfs:comment "Power factor tap-to-ground." ;
                                rdfs:label "c1" .


:BushingInsulationPfTestKind.c2 uml:id "_3D315ACC-4149-4e7a-9C1F-1322CECD015A" ;
                                rdfs:comment "Power factor tap-to-conductor." ;
                                rdfs:label "c2" .


:CIGREStandardEditionKind._2000 uml:id "_EE8F128C-A7A4-421d-AF8E-F5258C786C95" ;
                                rdfs:comment "2000 standard edition." ;
                                rdfs:label "2000" .


:CIGREStandardEditionKind.none uml:id "_CB550EE8-038C-4413-9030-D48F1B870F8E" ;
                               rdfs:comment "No standard edition." ;
                               rdfs:label "none" .


:CIGREStandardEditionKind.unknown uml:id "_EC568586-4BEF-48e9-A26C-9D4EA7AAE9FF" ;
                                  rdfs:comment "Unknown standard edition." ;
                                  rdfs:label "unknown" .


:CIGREStandardKind.TB_170 uml:id "_499DC4AF-688D-4a03-AF28-D8ED14C2CAF7" ;
                          rdfs:comment "CIGRE Technical Brochure 170 Static Electrification in Power Transformers." ;
                          rdfs:label "TB 170" .


:CRRCategoryType.NSR uml:id "_D77268DB-C24F-4a63-8CAE-D683A246761B" ;
                     rdfs:comment "Network Service" ;
                     rdfs:label "NSR" .


:CRRCategoryType.PTP uml:id "_CC2F4EAC-6FE5-46df-BD67-FF94B9969B1B" ;
                     rdfs:comment "Point to Point" ;
                     rdfs:label "PTP" .


:CRRHedgeType.OBLIGATION uml:id "_535CCF93-0DC6-447e-9ABA-7D10C49BDFE9" ;
                         rdfs:label "OBLIGATION" .


:CRRHedgeType.OPTION uml:id "_15D9CCC4-A640-4a62-90A5-1534EBECCD0A" ;
                     rdfs:label "OPTION" .


:CRRRoleType.BUYER uml:id "_3384C5FD-8154-48d8-B552-EFEADCEAB119" ;
                   rdfs:label "BUYER" .


:CRRRoleType.OWNER uml:id "_CFA1234F-3BC7-420b-BB56-339F2094F834" ;
                   rdfs:label "OWNER" .


:CRRRoleType.SELLER uml:id "_16D5DE62-21E5-402a-BDC1-5A02FC9C900F" ;
                    rdfs:label "SELLER" .


:CRRSegmentType.AUC uml:id "_95760A4C-CC9F-4427-B125-C25CB10CC35D" ;
                    rdfs:label "AUC" .


:CRRSegmentType.CAP uml:id "_7D49A152-C6EE-4970-921B-4AB479AEBBF7" ;
                    rdfs:label "CAP" .


:CRRSegmentType.CF uml:id "_D86465B6-F729-4dac-B772-CEE217F681D5" ;
                   rdfs:label "CF" .


:CRRSegmentType.CVR uml:id "_F5EECC95-3613-4693-837D-6584FE3462B6" ;
                    rdfs:comment "Converted rights." ;
                    rdfs:label "CVR" .


:CRRSegmentType.ETC uml:id "_56A5FD8C-510D-4f63-BD91-672D1E7B4141" ;
                    rdfs:comment "Existing Transmission Contract." ;
                    rdfs:label "ETC" .


:CRRSegmentType.LSE uml:id "_9965F5FF-AA24-4bab-ABCD-325F0E4DEBED" ;
                    rdfs:comment "Load Serving Entity." ;
                    rdfs:label "LSE" .


:CRRSegmentType.MT uml:id "_765292DC-3EF7-495f-BCB2-6ECCD211AF47" ;
                   rdfs:comment "Merchant transmission." ;
                   rdfs:label "MT" .


:CRRSegmentType.TOR uml:id "_54345270-CCE5-494c-939B-0DC995B0DA53" ;
                    rdfs:comment "Transmission Ownership Rights." ;
                    rdfs:label "TOR" .


:CableConstructionKind.compacted uml:id "_2735D553-3002-4c0d-A41D-77481121912B" ;
                                 rdfs:comment "Compacted cable." ;
                                 rdfs:label "compacted" .


:CableConstructionKind.compressed uml:id "_9D6C8350-5DA8-44a8-B2FF-0881164ABBC0" ;
                                  rdfs:comment "Compressed cable." ;
                                  rdfs:label "compressed" .


:CableConstructionKind.other uml:id "_49CD656B-5879-448f-AD49-C147DF7F04CC" ;
                             rdfs:comment "Other kind of cable construction." ;
                             rdfs:label "other" .


:CableConstructionKind.sector uml:id "_AF3E84D0-807D-402a-8F51-5DFF43410CB5" ;
                              rdfs:comment "Sector cable." ;
                              rdfs:label "sector" .


:CableConstructionKind.segmental uml:id "_7C253CC1-E1E1-477b-8B68-13145A7C3358" ;
                                 rdfs:comment "Segmental cable." ;
                                 rdfs:label "segmental" .


:CableConstructionKind.solid uml:id "_BD226CFC-1363-4f43-BAD6-3A7D241A6516" ;
                             rdfs:comment "Solid cable." ;
                             rdfs:label "solid" .


:CableConstructionKind.stranded uml:id "_F216BAE7-708B-4ebd-B5D4-17F24C8D5AA9" ;
                                rdfs:comment "Stranded cable." ;
                                rdfs:label "stranded" .


:CableOuterJacketKind.insulating uml:id "_1580FECE-B730-43a3-8570-826EB7B2897A" ;
                                 rdfs:comment "Insulating cable outer jacket." ;
                                 rdfs:label "insulating" .


:CableOuterJacketKind.linearLowDensityPolyethylene uml:id "_3B06AF70-4A3B-4037-98B4-4267191D6D24" ;
                                                   rdfs:comment "Linear low density polyethylene cable outer jacket." ;
                                                   rdfs:label "linearLowDensityPolyethylene" .


:CableOuterJacketKind.none uml:id "_3DA67FCE-74C5-4658-9684-C283A4E62B67" ;
                           rdfs:comment "Cable has no outer jacket." ;
                           rdfs:label "none" .


:CableOuterJacketKind.other uml:id "_81181A29-4B97-45b0-97D8-A1A4688C6302" ;
                            rdfs:comment "Pther kind of cable outer jacket." ;
                            rdfs:label "other" .


:CableOuterJacketKind.polyethylene uml:id "_FF1B423A-B3C1-4d13-B1B6-C6B6C7BCC60E" ;
                                   rdfs:comment "Polyethylene cable outer jacket." ;
                                   rdfs:label "polyethylene" .


:CableOuterJacketKind.pvc uml:id "_EE8265E9-086E-4ef1-B1E8-2B35958F50CE" ;
                          rdfs:comment "PVC cable outer jacket." ;
                          rdfs:label "pvc" .


:CableOuterJacketKind.semiconducting uml:id "_D9C413D2-019A-4e6b-8312-0508670EA545" ;
                                     rdfs:comment "Semiconducting cable outer jacket." ;
                                     rdfs:label "semiconducting" .


:CableShieldMaterialKind.aluminum uml:id "_722C6A25-1A40-491f-A9E5-6C3DA2AC6729" ;
                                  rdfs:comment "Aluminum cable shield." ;
                                  rdfs:label "aluminum" .


:CableShieldMaterialKind.copper uml:id "_12EF202C-F149-4f7c-B8DA-A9CE642AEB41" ;
                                rdfs:comment "Copper cable shield." ;
                                rdfs:label "copper" .


:CableShieldMaterialKind.lead uml:id "_902A2C27-89D6-48cb-BAEB-3C2DD386DF0C" ;
                              rdfs:comment "Lead cable shield." ;
                              rdfs:label "lead" .


:CableShieldMaterialKind.other uml:id "_EF55175B-8D53-4d0c-BD36-88FC7A3DEBE4" ;
                               rdfs:comment "Other kind of cable shield material." ;
                               rdfs:label "other" .


:CableShieldMaterialKind.steel uml:id "_1B36E1B2-B960-4994-9795-841C3C18D30A" ;
                               rdfs:comment "Steel cable shield." ;
                               rdfs:label "steel" .


:CalculationIntervalUnitKind.cycle uml:id "_13B61A3C-5544-4cc5-8B43-1EA43B7BE644" ;
                                   rdfs:comment "Period expressed in cycles." ;
                                   rdfs:label "cycle" .


:CalculationIntervalUnitKind.day uml:id "_21E466BC-49FB-4879-A6BC-5FEC2FA69C2D" ;
                                 rdfs:comment "Period expressed in days." ;
                                 rdfs:label "day" .


:CalculationIntervalUnitKind.hour uml:id "_DB85C617-16AC-422c-81CE-A7D8FD1A91D3" ;
                                  rdfs:comment "Period expressed in hours." ;
                                  rdfs:label "hour" .


:CalculationIntervalUnitKind.milliSecond uml:id "_EE757E07-87B5-480f-9E00-B7969E05A944" ;
                                         rdfs:comment "Period expressed in milli-seconds." ;
                                         rdfs:label "milliSecond" .


:CalculationIntervalUnitKind.minute uml:id "_C7B9C8CD-CFC8-4787-B340-F58C74315D06" ;
                                    rdfs:comment "Period expressed in minutes." ;
                                    rdfs:label "minute" .


:CalculationIntervalUnitKind.month uml:id "_24443448-EAA9-4891-91CB-81EE4E5D41EE" ;
                                   rdfs:comment "Period expressed in months." ;
                                   rdfs:label "month" .


:CalculationIntervalUnitKind.perCycle uml:id "_6BE554C5-8A84-4026-BAA0-69DDAF256277" ;
                                      rdfs:comment "Period expressed in per-cycle." ;
                                      rdfs:label "perCycle" .


:CalculationIntervalUnitKind.season uml:id "_6F054307-C44C-48a1-BFA0-9F085BD93EC0" ;
                                    rdfs:comment "Period expressed in seasons." ;
                                    rdfs:label "season" .


:CalculationIntervalUnitKind.second uml:id "_B0F50EAA-E0F5-428a-8A02-35D75D9F0220" ;
                                    rdfs:comment "Period expressed in seconds." ;
                                    rdfs:label "second" .


:CalculationIntervalUnitKind.week uml:id "_EE536F4F-389E-43c1-A790-EDB2CEAC1296" ;
                                  rdfs:comment "Period expressed in weeks." ;
                                  rdfs:label "week" .


:CalculationIntervalUnitKind.year uml:id "_752DC03C-0570-4ee2-A371-6BEB1A6BE7E2" ;
                                  rdfs:comment "Period expressed in years." ;
                                  rdfs:label "year" .


:CalculationKind.div uml:id "_44380763-1E53-4bee-9DCB-5ED5A3E28D75" ;
                     rdfs:comment "Division operation the input values (operands)." ;
                     rdfs:label "div" .


:CalculationKind.mul uml:id "_AE100BFB-D6AE-44f4-BE5C-0FBB3F0A32B4" ;
                     rdfs:comment "Multiplication operation the input values (operands)." ;
                     rdfs:label "mul" .


:CalculationKind.sqrt uml:id "_CE420801-4EF4-488d-A0A5-D4A230931877" ;
                      rdfs:comment "Square root operator - only one input value (operands)." ;
                      rdfs:label "sqrt" .


:CalculationKind.sum uml:id "_7CAEF807-9455-418e-8374-8F626E7DE19F" ;
                     rdfs:comment "Summation operation over the input values (operands)." ;
                     rdfs:label "sum" .


:CalculationModeKind.period uml:id "_D5D527CE-1E3F-4a35-8614-C20F624980DE" ;
                            rdfs:comment "Calcuation is for fixed period." ;
                            rdfs:label "period" .


:CalculationModeKind.sliding uml:id "_5618A0F1-10AD-40bf-A287-7AFCE4F62CCB" ;
                             rdfs:comment "Calculation is for sliding period." ;
                             rdfs:label "sliding" .


:CalculationModeKind.total uml:id "_DE3A2882-F75F-43f5-9C12-A65345BBA158" ;
                           rdfs:comment "Calculation is for total period." ;
                           rdfs:label "total" .


:CalculationTechniqueKind.average uml:id "_464224C2-0F34-42d4-8284-3EC29BE71E9A" ;
                                  rdfs:comment "Result is average value for period." ;
                                  rdfs:label "average" .


:CalculationTechniqueKind.maximum uml:id "_89FF1DAD-7B49-43cf-80E7-16F7320E7A34" ;
                                  rdfs:comment "Result is maximum value for period." ;
                                  rdfs:label "maximum" .


:CalculationTechniqueKind.minimum uml:id "_C37136E1-21D7-4480-9C08-7F1A6F9FB96C" ;
                                  rdfs:comment "Result is minimum value for period." ;
                                  rdfs:label "minimum" .


:CalculationTechniqueKind.trueRMS uml:id "_FA73E284-C45D-462a-A35C-0FEF69550891" ;
                                  rdfs:comment "Result is RMS value for period." ;
                                  rdfs:label "trueRMS" .


:ChargeKind.auxiliaryCharge uml:id "_2F1EAFE1-E83E-4adc-A420-911CC63D4274" ;
                            rdfs:comment "Any other charge which is not a consumptionCharge or demandCharge. For example: debt recovery, arrears, standing charge or charge for another service such as street lighting." ;
                            rdfs:label "auxiliaryCharge" .


:ChargeKind.consumptionCharge uml:id "_B1F74271-06BB-4a98-9524-0FDB71F71ABB" ;
                              rdfs:comment "The charge levied for the actual usage of the service, normally expressed in terms of a tariff. For example: usage x price per kWh = total charge for consumption." ;
                              rdfs:label "consumptionCharge" .


:ChargeKind.demandCharge uml:id "_33EBD778-E57F-4c4f-AEB3-1FD25FD6D964" ;
                         rdfs:comment "The charge related to the usage within a defined time interval, normally expressed in terms of a tariff. For example: a maximum-demand tariff will levy an additional charge on top of the consumption charge if the usage exceeds a defined limit per hour." ;
                         rdfs:label "demandCharge" .


:ChargeKind.other uml:id "_59011684-2316-491c-9315-3E9827A7BE4B" ;
                  rdfs:comment "Other kind of charge." ;
                  rdfs:label "other" .


:ChargeKind.taxCharge uml:id "_8CB6CA84-373D-4700-8F4C-2C15AA98D5E7" ;
                      rdfs:comment "Any charge that is classified as a tax of a kind. For example: VAT, GST, TV tax, etc." ;
                      rdfs:label "taxCharge" .


:CheckOutType.AFTER_THE_FACT uml:id "_BEE41C74-ABDF-4182-96B3-82F202BEF625" ;
                             rdfs:label "AFTER_THE_FACT" .


:CheckOutType.PRE_HOUR uml:id "_201DCC41-A8E6-4f4f-B8B8-C1F07F68DE4E" ;
                       rdfs:label "PRE_HOUR" .


:CheckOutType.PRE_SCHEDULE uml:id "_0E2A1B61-9FFE-461f-AD2C-1B3CE9A34C21" ;
                           rdfs:label "PRE_SCHEDULE" .


:ChequeKind.bankOrder uml:id "_761F35F2-99F9-4ee0-A8FB-CD82B69E2440" ;
                      rdfs:comment "Payment order used by a bank." ;
                      rdfs:label "bankOrder" .


:ChequeKind.other uml:id "_E68A776E-E0B0-4269-A463-738743BAAB72" ;
                  rdfs:comment "Other kind of cheque." ;
                  rdfs:label "other" .


:ChequeKind.postalOrder uml:id "_B5AC951B-0033-4b4a-B74A-189EEAB73111" ;
                        rdfs:comment "Payment order used by institutions other than banks." ;
                        rdfs:label "postalOrder" .


:CleanTradeProductType.APN uml:id "_252A5724-BC88-468f-8999-BEBC5106339D" ;
                           rdfs:comment "Energy Trades at Aggregated Pricing Nodes" ;
                           rdfs:label "APN" .


:CleanTradeProductType.CPT uml:id "_575E0B7B-D8F7-465f-B99E-78ED48E74E17" ;
                           rdfs:comment "Converted Physical Energy Trade" ;
                           rdfs:label "CPT" .


:CleanTradeProductType.NRT uml:id "_D5ADA39F-360A-4158-B8A2-A9FD8F56487A" ;
                           rdfs:comment "Non-Spinning Reserve Trade" ;
                           rdfs:label "NRT" .


:CleanTradeProductType.PHY uml:id "_07C26D98-DB13-4bc5-8D3D-6AC92BBC46C9" ;
                           rdfs:comment "Physical Energy Tra" ;
                           rdfs:label "PHY" .


:CleanTradeProductType.RDT uml:id "_CBD848D7-A005-4cf8-88B5-BB1FFD9224C3" ;
                           rdfs:comment "Regulation Down Trade" ;
                           rdfs:label "RDT" .


:CleanTradeProductType.RUT uml:id "_AB57CE07-8718-45e0-B461-E01E3BEEF30F" ;
                           rdfs:comment "Regulation Up Trade" ;
                           rdfs:label "RUT" .


:CleanTradeProductType.SRT uml:id "_AB1A5DE2-5ABC-40a8-8F20-6014B2014F74" ;
                           rdfs:comment "Spinning Reserve Trade" ;
                           rdfs:label "SRT" .


:ClearanceActionKind.issue uml:id "_92B91793-784A-487f-ACED-3F7D8A69BA37" ;
                           rdfs:comment "Issue clearance." ;
                           rdfs:label "issue" .


:ClearanceActionKind.release uml:id "_04F4B5A7-5A44-48dd-8637-F603EAD2C510" ;
                             rdfs:comment "Release clearance." ;
                             rdfs:label "release" .


:ClearanceActionKind.update uml:id "_831A7582-9199-409c-96F5-1F83E93C159D" ;
                            rdfs:comment "Update clearance." ;
                            rdfs:label "update" .


:CloudKind.altoCumulus uml:id "_9C8D79CF-8B5B-4726-A502-208EFAB9A13D" ;
                       rdfs:label "altoCumulus" .


:CloudKind.altoStratus uml:id "_4E1A921A-447B-40e5-8F7E-6B8CA623B144" ;
                       rdfs:label "altoStratus" .


:CloudKind.cirroCumulus uml:id "_ED2BE614-7767-4a1c-AD39-640EEE988429" ;
                        rdfs:label "cirroCumulus" .


:CloudKind.cirroStratus uml:id "_46FAE592-9178-4272-B843-473588158091" ;
                        rdfs:label "cirroStratus" .


:CloudKind.cirrus uml:id "_6A7D1D76-C754-41d4-8F0D-F98C07CEC7D2" ;
                  rdfs:label "cirrus" .


:CloudKind.cumuloNimbus uml:id "_8EB07A9F-4310-453a-86B2-F78A151E0D5B" ;
                        rdfs:label "cumuloNimbus" .


:CloudKind.cumulus uml:id "_05447D08-67C9-402b-8695-0782655111F7" ;
                   rdfs:label "cumulus" .


:CloudKind.nimboStratus uml:id "_106F6D69-6062-4720-922F-8F893462D07B" ;
                        rdfs:label "nimboStratus" .


:CloudKind.other uml:id "_F60ABC70-B85D-400f-BB50-90C15D82CA57" ;
                 rdfs:label "other" .


:CloudKind.stratoCumulus uml:id "_14DAAAA6-BF9F-46b5-B41D-415602269EBC" ;
                         rdfs:label "stratoCumulus" .


:CloudKind.stratus uml:id "_D4D08403-EA33-48f4-9DC1-EC7D67C66BE8" ;
                   rdfs:label "stratus" .


:CloudKind.toweringCumulus uml:id "_F969C27E-9FC7-444a-9D6D-8C3EBC955F02" ;
                           rdfs:label "toweringCumulus" .


:ComDirectionKind.biDirectional uml:id "_B143F713-C9FA-41b6-8169-EFC12FFB9190" ;
                                rdfs:comment "Communication with the device is bi-directional." ;
                                rdfs:label "biDirectional" .


:ComDirectionKind.fromDevice uml:id "_2613B7DA-88BB-48e7-84B5-51660B9C703E" ;
                             rdfs:comment "Communication is from device." ;
                             rdfs:label "fromDevice" .


:ComDirectionKind.toDevice uml:id "_04263A1C-FAB4-414d-A9CB-757127539690" ;
                           rdfs:comment "Communication is to device." ;
                           rdfs:label "toDevice" .


:ComTechnologyKind.cellular uml:id "_0381F4E6-5BF8-49f8-ABC8-4859232EAA0F" ;
                            rdfs:comment "Communicates using a public cellular radio network. A specific variant of 'rf'." ;
                            rdfs:label "cellular" .


:ComTechnologyKind.ethernet uml:id "_2AB21062-8E90-4eae-80C2-CCEA4522AC62" ;
                            rdfs:comment "Communicates using one or more of a family of frame-based computer networking technologies conforming to the IEEE 802.3 standard." ;
                            rdfs:label "ethernet" .


:ComTechnologyKind.homePlug uml:id "_58085034-38A5-4a4c-BCCC-C65F168B07DF" ;
                            rdfs:comment "Communicates using power line communication technologies conforming to the standards established by the HomePlug Powerline Alliance. A specific variant of 'plc'." ;
                            rdfs:label "homePlug" .


:ComTechnologyKind.pager uml:id "_41E95511-E5C1-417a-B317-005A4D586DAD" ;
                         rdfs:comment "Communicates using a public one-way or two-way radio-based paging network. A specific variant of 'rf'." ;
                         rdfs:label "pager" .


:ComTechnologyKind.phone uml:id "_E23519E7-AA3B-448c-A77C-4C60AC6D0274" ;
                         rdfs:comment "Communicates using a basic, wireline telephone system." ;
                         rdfs:label "phone" .


:ComTechnologyKind.plc uml:id "_96059140-9F25-4634-8549-04CB327BFDDE" ;
                       rdfs:comment "Communicates using power line communication technologies." ;
                       rdfs:label "plc" .


:ComTechnologyKind.rf uml:id "_EE14239D-87FF-48f2-B26A-BDACA9901E08" ;
                      rdfs:comment "Communicates using private or public radio-based technology." ;
                      rdfs:label "rf" .


:ComTechnologyKind.rfMesh uml:id "_0A7C7A0F-951A-4244-8C95-FF5B0E3B27E4" ;
                          rdfs:comment "Communicates using a mesh radio technology. A specific variant of 'rf'." ;
                          rdfs:label "rfMesh" .


:ComTechnologyKind.zigbee uml:id "_A0DF5D95-1355-432e-AEB0-CB22E842730B" ;
                          rdfs:comment "Communicates using radio communication technologies conforming to the standards established by the ZigBee. A specific variant of 'rf'." ;
                          rdfs:label "zigbee" .


:CommitmentType.ISO uml:id "_BD15AFC7-3EF9-49ec-BF27-951587505ACB" ;
                    rdfs:label "ISO" .


:CommitmentType.SELF uml:id "_8C75BC58-C27B-4d97-8128-61AAC19BEAE6" ;
                     rdfs:label "SELF" .


:CommitmentType.UC uml:id "_6AF267B4-B970-403a-8D7D-4C362042EB51" ;
                   rdfs:label "UC" .


:CommodityKind.air uml:hasInitialValue "4" ;
                   uml:id "_96DEA7BE-8DA8-446f-AA9A-AC6DB4ABBCAD" ;
                   rdfs:comment "Atmospheric air" ;
                   rdfs:label "air" .


:CommodityKind.carbon uml:hasInitialValue "19" ;
                      uml:id "_D5095FDD-E537-4418-86D2-E78D2AA3D9F0" ;
                      rdfs:comment "The element has an atomic number of 6." ;
                      rdfs:label "carbon" .


:CommodityKind.ch4 uml:hasInitialValue "17" ;
                   uml:id "_B0F613C1-5D3E-48f3-98C1-EAFA12F7BEBA" ;
                   rdfs:comment "Methane CH4" ;
                   rdfs:label "ch4" .


:CommodityKind.co2 uml:hasInitialValue "18" ;
                   uml:id "_025D4E4F-F092-48fa-B390-40F3701903C4" ;
                   rdfs:comment "Carbon Dioxide CO2" ;
                   rdfs:label "co2" .


:CommodityKind.communication uml:hasInitialValue "3" ;
                             uml:id "_3C79F608-85DD-45ef-9085-1396FE0D6EB9" ;
                             rdfs:comment "A measurement of the communication infrastructure itself." ;
                             rdfs:label "communication" .


:CommodityKind.coolingFluid uml:hasInitialValue "13" ;
                            uml:id "_FC7C1BCC-7C39-4834-BE44-36E4D769A9FB" ;
                            rdfs:comment "The cool fluid returns warmer than when it was sent. The heat conveyed may be metered." ;
                            rdfs:label "coolingFluid" .


:CommodityKind.electricityPrimaryMetered uml:hasInitialValue "2" ;
                                         uml:id "_F6E81EFA-FEE7-4c53-96EB-5B3A3536D638" ;
                                         rdfs:comment "It is possible for a meter to be outfitted with an external VT and/or CT. The meter might not be aware of these devices, and the display not compensate for their presence. Ultimately, when these scalars are applied, the value that represents the service value is called the “primary metered” value. The “index” in sub-category 3 mirrors those of sub-category 0." ;
                                         rdfs:label "electricityPrimaryMetered" .


:CommodityKind.electricitySecondaryMetered uml:hasInitialValue "1" ;
                                           uml:id "_718BB312-7C16-430c-9F9F-CB80A1E62334" ;
                                           rdfs:comment "All types of metered quantities. This type of reading comes from the meter and represents a “secondary” metered value." ;
                                           rdfs:label "electricitySecondaryMetered" .


:CommodityKind.hch uml:hasInitialValue "20" ;
                   uml:id "_94A30E00-5AF4-40ef-A718-9DF4DCDC0708" ;
                   rdfs:comment "Hexachlorocyclohexane HCH" ;
                   rdfs:label "hch" .


:CommodityKind.heatingFluid uml:hasInitialValue "12" ;
                            uml:id "_D48E36F6-A36F-497c-A246-707BBEAA36C1" ;
                            rdfs:comment "This fluid is likely in liquid form. It is not necessarily water or water based. The warm fluid returns cooler than when it was sent. The heat conveyed may be metered." ;
                            rdfs:label "heatingFluid" .


:CommodityKind.insulativeGas uml:hasInitialValue "5" ;
                             uml:id "_E968DC07-265E-41cc-A95E-332E57D0615F" ;
                             rdfs:comment "(SF6 is found separately below.)" ;
                             rdfs:label "insulativeGas" .


:CommodityKind.insulativeOil uml:hasInitialValue "6" ;
                             uml:id "_1D5CA370-2F97-4b5f-9B43-DF72A2800243" ;
                             rdfs:comment "Oil that is used in transformers to provide insulation and heat conduction." ;
                             rdfs:label "insulativeOil" .


:CommodityKind.internet uml:hasInitialValue "24" ;
                        uml:id "_77E021BB-7E43-481c-A4A8-A7E30BACBC66" ;
                        rdfs:comment "Internet service" ;
                        rdfs:label "internet" .


:CommodityKind.naturalGas uml:hasInitialValue "7" ;
                          uml:id "_B8873BB8-19FE-4772-8BE9-5F8165E6E0BE" ;
                          rdfs:comment "A naturally occurring hydrocarbon  gas mixture." ;
                          rdfs:label "naturalGas" .


:CommodityKind.none uml:hasInitialValue "0" ;
                    uml:id "_95036860-E113-4c13-8713-E7EFF95F94A4" ;
                    rdfs:comment "Not Applicable" ;
                    rdfs:label "none" .


:CommodityKind.nonpotableWater uml:hasInitialValue "14" ;
                               uml:id "_AB92C5ED-069C-4dc7-A7CE-78508603C28A" ;
                               rdfs:comment "Reclaimed water – possibly used for irrigation but not sufficiently treated to be considered safe for drinking." ;
                               rdfs:label "nonpotableWater" .


:CommodityKind.nox uml:hasInitialValue "15" ;
                   uml:id "_A1FDCAF2-1E6F-4cbc-9679-654CB60BF052" ;
                   rdfs:comment "Nitrous Oxides NOX" ;
                   rdfs:label "nox" .


:CommodityKind.pfc uml:hasInitialValue "21" ;
                   uml:id "_4C337D73-5FF2-4c7d-AEFA-EB7FF337CD8F" ;
                   rdfs:comment "Perfluorocarbons PFC" ;
                   rdfs:label "pfc" .


:CommodityKind.potableWater uml:hasInitialValue "9" ;
                            uml:id "_EB71070B-1354-4dce-8AA0-DA1D226BA29D" ;
                            rdfs:comment "Drinkable water" ;
                            rdfs:label "potableWater" .


:CommodityKind.propane uml:hasInitialValue "8" ;
                       uml:id "_DCAB146D-8B07-4b5d-8F4D-02822AB956B0" ;
                       rdfs:comment "The formula is C3H8" ;
                       rdfs:label "propane" .


:CommodityKind.refuse uml:hasInitialValue "25" ;
                      uml:id "_CF5DE8FB-9F20-4deb-B338-FD5959C2172A" ;
                      rdfs:comment "trash" ;
                      rdfs:label "refuse" .


:CommodityKind.sf6 uml:hasInitialValue "22" ;
                   uml:id "_48BACD9E-5890-427e-9CF0-69F845479FDD" ;
                   rdfs:comment "Sulfurhexafluoride SF6" ;
                   rdfs:label "sf6" .


:CommodityKind.so2 uml:hasInitialValue "16" ;
                   uml:id "_DFEB7875-592C-42f6-947D-DDAEB6449B9D" ;
                   rdfs:comment "Sulfur Dioxide SO2" ;
                   rdfs:label "so2" .


:CommodityKind.steam uml:hasInitialValue "10" ;
                     uml:id "_96D401ED-3C83-4c22-AD27-430FFE930D53" ;
                     rdfs:comment "Water in steam form, usually used for heating." ;
                     rdfs:label "steam" .


:CommodityKind.tvLicence uml:hasInitialValue "23" ;
                         uml:id "_D337EA63-CFE7-4b95-8A80-4562594E8DEF" ;
                         rdfs:comment "Television" ;
                         rdfs:label "tvLicence" .


:CommodityKind.wasteWater uml:hasInitialValue "11" ;
                          uml:id "_D7396F86-F54F-48c2-8F60-84EA8A566391" ;
                          rdfs:comment "(Sewerage)" ;
                          rdfs:label "wasteWater" .


:CompositeSwitchKind.escoThrowOver uml:id "_9839F383-4C31-42b3-AC06-BD0A76C8F307" ;
                                   rdfs:label "escoThrowOver" .


:CompositeSwitchKind.gral uml:id "_FA359723-E719-4372-95EF-5AD352E50D2E" ;
                          rdfs:label "gral" .


:CompositeSwitchKind.other uml:id "_43098CBF-5123-4744-8DF5-458D4C1FE644" ;
                           rdfs:label "other" .


:CompositeSwitchKind.ral uml:id "_9CBEE8D0-2CED-4eed-A172-A316FD155B08" ;
                         rdfs:label "ral" .


:CompositeSwitchKind.regulatorBypass uml:id "_A456FDC2-1DB7-4e65-B434-7572BC318272" ;
                                     rdfs:label "regulatorBypass" .


:CompositeSwitchKind.throwOver uml:id "_F34B4D4F-BB87-4c07-8BEF-EA081483574F" ;
                               rdfs:label "throwOver" .


:CompositeSwitchKind.ugMultiSwitch uml:id "_819876BC-0B73-4180-8C07-78DA9C88C91E" ;
                                   rdfs:label "ugMultiSwitch" .


:ConditionFactorKind.accountAllocation uml:id "_48809184-89E0-4a14-BE67-65BB64A9A0B8" ;
                                       rdfs:label "accountAllocation" .


:ConditionFactorKind.labor uml:id "_422B882F-1B4B-4e9b-89DF-A0B2F2242D77" ;
                           rdfs:label "labor" .


:ConditionFactorKind.material uml:id "_F7009183-6923-4da1-8640-BD5B17812D5C" ;
                              rdfs:label "material" .


:ConditionFactorKind.other uml:id "_C10A3AC8-7C1A-4a76-BD7D-D0752854C8FD" ;
                           rdfs:label "other" .


:ConditionFactorKind.travel uml:id "_0B5303D3-E38D-405c-A7D2-6DC82351DEBF" ;
                            rdfs:label "travel" .


:ConstraintLimitType.MAXIMUM uml:id "_E59D1EFD-CA0B-49ec-ACE8-1F8287A9B29B" ;
                             rdfs:label "MAXIMUM" .


:ConstraintLimitType.MINIMUM uml:id "_7F8F866D-D9C7-4a5c-A299-E4A6A819EABD" ;
                             rdfs:label "MINIMUM" .


:ConstraintRampType.FAST uml:id "_3378A528-18CC-4b01-A5D4-96D0EF2D2DE1" ;
                         rdfs:label "FAST" .


:ConstraintRampType.SLOW uml:id "_08A6FB04-E930-4729-AEA3-23DCDBB6C2DF" ;
                         rdfs:label "SLOW" .


:ContingencyEquipmentStatusKind.inService uml:id "_52DCF9EB-B100-4dc2-B0BE-82ADA309922E" ;
                                          rdfs:comment "The equipment is to be put into service." ;
                                          rdfs:label "inService" .


:ContingencyEquipmentStatusKind.outOfService uml:id "_F296EA90-0E39-4a44-8E31-D31EE6106CB6" ;
                                             rdfs:comment "The equipment is to be taken out of service." ;
                                             rdfs:label "outOfService" .


:ContractType.CVR uml:id "_656DAF3E-967D-4927-938B-32B603D6133A" ;
                  rdfs:comment "CVR - Converted contract." ;
                  rdfs:label "CVR" .


:ContractType.ETC uml:id "_953ED153-0420-4bc1-A792-83B235D5B278" ;
                  rdfs:comment "ETC - Existing Transmission Contract" ;
                  rdfs:label "ETC" .


:ContractType.O uml:id "_A49468B9-4905-413c-AB46-8E0DCDA97263" ;
                rdfs:comment "O - Other" ;
                rdfs:label "O" .


:ContractType.RMR uml:id "_A8352BC5-59FF-419c-B653-2C56845CBEE9" ;
                  rdfs:comment "RMR - Reliability Must Run Contract" ;
                  rdfs:label "RMR" .


:ContractType.RMT uml:id "_6B9BBF1C-BC6E-4f39-9878-36638D5237D9" ;
                  rdfs:comment "RMT - RMT Contract" ;
                  rdfs:label "RMT" .


:ContractType.TE uml:id "_83109E91-0FED-4948-A614-B4D69C302E1C" ;
                 rdfs:comment "TE - Transmission Export" ;
                 rdfs:label "TE" .


:ContractType.TI uml:id "_36C5DC29-42B3-49cf-918A-ADB63308C9A1" ;
                 rdfs:comment "TI - Transmission Import" ;
                 rdfs:label "TI" .


:ContractType.TOR uml:id "_C948431C-09A9-4b9a-99D3-928ECC97E804" ;
                  rdfs:comment "TOR - Transmission Ownership Right" ;
                  rdfs:label "TOR" .


:ControlAreaTypeKind.AGC uml:id "_8BA47D6C-F682-4daa-931F-EA232E22DA14" ;
                         rdfs:comment "Used for automatic generation control." ;
                         rdfs:label "AGC" .


:ControlAreaTypeKind.Forecast uml:id "_51A131DD-63D8-4f4c-83C9-29EF59E44962" ;
                              rdfs:comment "Used for load forecast." ;
                              rdfs:label "Forecast" .


:ControlAreaTypeKind.Interchange uml:id "_94213EA0-368A-49c1-8028-9A905159C854" ;
                                 rdfs:comment "Used for interchange specification or control." ;
                                 rdfs:label "Interchange" .


:CoolantType.air uml:id "_2FBCC200-0408-41d6-8CEE-E179F67B7D47" ;
                 rdfs:comment "Air." ;
                 rdfs:label "air" .


:CoolantType.hydrogenGas uml:id "_17676572-09DD-43d7-B586-6FE9616CE56E" ;
                         rdfs:comment "Hydrogen gas." ;
                         rdfs:label "hydrogenGas" .


:CoolantType.water uml:id "_037AFDDD-4C06-4531-B227-53B16C4327A8" ;
                   rdfs:comment "Water." ;
                   rdfs:label "water" .


:CoolingKind.forcedAir uml:id "_D147AC5A-8720-4f39-90A7-7706AD8FE238" ;
                       rdfs:label "forcedAir" .


:CoolingKind.forcedOilAndAir uml:id "_0FD94E57-DE34-464c-87B4-6D44D2AC4F8A" ;
                             rdfs:label "forcedOilAndAir" .


:CoolingKind.other uml:id "_CFE99F39-8EF0-4225-B9AD-DE22DC059C41" ;
                   rdfs:label "other" .


:CoolingKind.selfCooling uml:id "_8C520ABE-D202-4be1-BE64-828848D473FA" ;
                         rdfs:label "selfCooling" .


:CorporateStandardKind.experimental uml:id "_A96F7F0E-0C5E-4208-904F-D122561B96F0" ;
                                    rdfs:comment "Asset model is used experimentally." ;
                                    rdfs:label "experimental" .


:CorporateStandardKind.other uml:id "_A65A8664-53EB-48e0-8C22-C7150493394C" ;
                             rdfs:comment "Other kind of corporate standard for the asset model." ;
                             rdfs:label "other" .


:CorporateStandardKind.standard uml:id "_406E95D0-49CB-487e-84CC-F6C247D1D2C8" ;
                                rdfs:comment "Asset model is used as corporate standard." ;
                                rdfs:label "standard" .


:CorporateStandardKind.underEvaluation uml:id "_B7D01BD9-6427-4914-9745-78EDB2B6A0CD" ;
                                       rdfs:comment "Asset model usage is under evaluation." ;
                                       rdfs:label "underEvaluation" .


:CostBasis.BIDC uml:id "_382359D5-DF07-4531-A16E-99755138CEFA" ;
                rdfs:label "BIDC" .


:CostBasis.PRXC uml:id "_163741B0-62BD-4bf5-85A9-2E5025832BCD" ;
                rdfs:label "PRXC" .


:CostBasis.REGC uml:id "_A73A6403-F3B2-4ece-B5F0-E9332CB9C283" ;
                rdfs:label "REGC" .


:CoverageCodeKind.brief uml:id "_18369290-A8EB-4156-B6EF-2A75E30F93FB" ;
                        rdfs:label "brief" .


:CoverageCodeKind.frequent uml:id "_1C108A21-3775-478c-B573-04D0B7D8761E" ;
                           rdfs:label "frequent" .


:CoverageCodeKind.intermittant uml:id "_1388C8DE-CF15-426e-9247-19C9106E9C6F" ;
                               rdfs:label "intermittant" .


:CoverageCodeKind.isolated uml:id "_52A8B952-6726-4e53-906F-F8CA791AE3DC" ;
                           rdfs:label "isolated" .


:CoverageCodeKind.numerous uml:id "_CAA8B0B8-BA59-4eee-A738-3034F56EC90E" ;
                           rdfs:label "numerous" .


:CoverageCodeKind.occasional uml:id "_2A2B94A9-5BFA-407f-98AA-27F4F332C80D" ;
                             rdfs:label "occasional" .


:CoverageCodeKind.partly uml:id "_611E6979-73DD-4304-8942-8AC3198CF012" ;
                         rdfs:label "partly" .


:CoverageCodeKind.patchy uml:id "_1D24F216-3616-4ce3-85B2-4FC6BDC13DAC" ;
                         rdfs:label "patchy" .


:CoverageCodeKind.periodsOf uml:id "_7534E68B-B76E-445c-B3C4-3234BE49447A" ;
                            rdfs:label "periodsOf" .


:CoverageCodeKind.scattered uml:id "_A51EBC9F-54E5-4ed6-872E-17682A66CED7" ;
                            rdfs:label "scattered" .


:CoverageCodeKind.widespread uml:id "_7F190721-6297-4997-A490-43329921D448" ;
                             rdfs:label "widespread" .


:CrewStatusKind.arrived uml:id "_8CC94FC5-1D69-4967-8619-2B2060A069BE" ;
                        rdfs:comment "the crew is on site at the outage location" ;
                        rdfs:label "arrived" .


:CrewStatusKind.assigned uml:id "_53E018DA-D710-4f09-BF9F-00002BD6B676" ;
                         rdfs:comment "the crew has been assigned to work on a task" ;
                         rdfs:label "assigned" .


:CrewStatusKind.awaitingCrewAssignment uml:id "_35D2334A-1728-4adb-9359-A7F3D7DA9C47" ;
                                       rdfs:comment "Indicates that the work is awaiting one or more crews to be assigned" ;
                                       rdfs:label "awaitingCrewAssignment" .


:CrewStatusKind.enroute uml:id "_A558BDCD-994E-4835-AB38-81DC1080F516" ;
                        rdfs:comment "the crew has been dispatched to work on an outage" ;
                        rdfs:label "enroute" .


:CrewStatusKind.fieldComplete uml:id "_DF4869BC-D3EB-4613-A89B-0282E5289E20" ;
                              rdfs:comment "the crew has corrected the outage in the field.  The equipment or other devices may not be energized at this time." ;
                              rdfs:label "fieldComplete" .


:CsOperatingModeKind.inverter uml:id "_4468886F-11CB-49aa-9074-C1F8DF9567DC" ;
                              rdfs:comment "Operating as inverter, which is the power receiving end." ;
                              rdfs:label "inverter" .


:CsOperatingModeKind.rectifier uml:id "_E887FDBD-34CA-4523-A6FE-9DFFE716287E" ;
                               rdfs:comment "Operating as rectifier, which is the power sending end." ;
                               rdfs:label "rectifier" .


:CsPpccControlKind.activePower uml:id "_C8635C3D-D432-4f8f-BF38-470EFEF07A78" ;
                               rdfs:comment "Control is active power control at AC side, at point of common coupling. Target is provided by ACDCConverter.targetPpcc." ;
                               rdfs:label "activePower" .


:CsPpccControlKind.dcCurrent uml:id "_0EF84B22-6683-4531-9627-F98AF4E25A21" ;
                             rdfs:comment "Control is DC current  with target value provided by CsConverter.targetIdc." ;
                             rdfs:label "dcCurrent" .


:CsPpccControlKind.dcVoltage uml:id "_1E4AB43E-B899-4f70-B996-A90291CB1003" ;
                             rdfs:comment "Control is DC voltage  with target value provided by ACDCConverter.targetUdc." ;
                             rdfs:label "dcVoltage" .


:Currency.AED uml:hasInitialValue "784" ;
              uml:id "_8311768F-16AF-4e99-938E-A7312455ADCD" ;
              rdfs:comment "United Arab Emirates dirham." ;
              rdfs:label "AED" .


:Currency.AFN uml:hasInitialValue "971" ;
              uml:id "_FB01059D-0487-4902-BCDB-601DE52F9459" ;
              rdfs:comment "Afghan afghani." ;
              rdfs:label "AFN" .


:Currency.ALL uml:hasInitialValue "008" ;
              uml:id "_D63F2DD9-38ED-4576-90EF-A3C6AC696D25" ;
              rdfs:comment "Albanian lek." ;
              rdfs:label "ALL" .


:Currency.AMD uml:hasInitialValue "051" ;
              uml:id "_4AEDF1C1-57C9-407f-9C63-EC2BFD7C7CB7" ;
              rdfs:comment "Armenian dram." ;
              rdfs:label "AMD" .


:Currency.ANG uml:hasInitialValue "532" ;
              uml:id "_33CD80A9-E051-47e0-BA68-F73AB5303660" ;
              rdfs:comment "Netherlands Antillean guilder." ;
              rdfs:label "ANG" .


:Currency.AOA uml:hasInitialValue "973" ;
              uml:id "_1592F28E-1DDF-4818-B2DB-74A5513CDEC6" ;
              rdfs:comment "Angolan kwanza." ;
              rdfs:label "AOA" .


:Currency.ARS uml:hasInitialValue "032" ;
              uml:id "_A37D65B0-6D69-4510-A379-C78BECA6A8CD" ;
              rdfs:comment "Argentine peso." ;
              rdfs:label "ARS" .


:Currency.AUD uml:hasInitialValue "036" ;
              uml:id "_B68ED9D0-E666-4c95-B4C8-3A2C8760C838" ;
              rdfs:comment "Australian dollar." ;
              rdfs:label "AUD" .


:Currency.AWG uml:hasInitialValue "533" ;
              uml:id "_F3D56893-E43C-4c64-A521-D8251B1D5B48" ;
              rdfs:comment "Aruban florin." ;
              rdfs:label "AWG" .


:Currency.AZN uml:hasInitialValue "944" ;
              uml:id "_F5BF1908-D42F-4c60-ACB1-035341951BD0" ;
              rdfs:comment "Azerbaijani manat." ;
              rdfs:label "AZN" .


:Currency.BAM uml:hasInitialValue "977" ;
              uml:id "_6CB82B96-D67F-40b0-B4E3-0385F61DB8F2" ;
              rdfs:comment "Bosnia and Herzegovina convertible mark." ;
              rdfs:label "BAM" .


:Currency.BBD uml:hasInitialValue "052" ;
              uml:id "_28CFBF64-16AB-45f8-AE26-2C8FBEF9B20F" ;
              rdfs:comment "Barbados dollar." ;
              rdfs:label "BBD" .


:Currency.BDT uml:hasInitialValue "050" ;
              uml:id "_74510D41-0967-4633-80E9-14BF51A24D3E" ;
              rdfs:comment "Bangladeshi taka." ;
              rdfs:label "BDT" .


:Currency.BGN uml:hasInitialValue "975" ;
              uml:id "_F57CC213-32B9-4120-8A78-0FB728D120FD" ;
              rdfs:comment "Bulgarian lev." ;
              rdfs:label "BGN" .


:Currency.BHD uml:hasInitialValue "048" ;
              uml:id "_1BC0AA85-5F9D-46ef-B4C2-CE7027781E56" ;
              rdfs:comment "Bahraini dinar." ;
              rdfs:label "BHD" .


:Currency.BIF uml:hasInitialValue "108" ;
              uml:id "_E9AAD0D3-7F9D-4997-8141-DD6128E5B2CA" ;
              rdfs:comment "Burundian franc." ;
              rdfs:label "BIF" .


:Currency.BMD uml:hasInitialValue "060" ;
              uml:id "_CA3A6A9C-31DC-4168-ACDE-E1EF5DA3F577" ;
              rdfs:comment "Bermudian dollar (customarily known as Bermuda dollar)." ;
              rdfs:label "BMD" .


:Currency.BND uml:hasInitialValue "096" ;
              uml:id "_994BFD2E-0601-4d44-B269-194EBD9B9E88" ;
              rdfs:comment "Brunei dollar." ;
              rdfs:label "BND" .


:Currency.BOB uml:hasInitialValue "068" ;
              uml:id "_96D55A3A-96D8-4359-B483-FD18C50CA078" ;
              rdfs:comment "Boliviano." ;
              rdfs:label "BOB" .


:Currency.BOV uml:hasInitialValue "984" ;
              uml:id "_A1FF6C66-4F30-4581-91D9-E8CC013BECD2" ;
              rdfs:comment "Bolivian Mvdol (funds code)." ;
              rdfs:label "BOV" .


:Currency.BRL uml:hasInitialValue "986" ;
              uml:id "_E903CA31-6CD7-4633-89C6-DB537F497A50" ;
              rdfs:comment "Brazilian real." ;
              rdfs:label "BRL" .


:Currency.BSD uml:hasInitialValue "044" ;
              uml:id "_5BDDE8D1-7D3A-448e-AAB7-B809F772F790" ;
              rdfs:comment "Bahamian dollar." ;
              rdfs:label "BSD" .


:Currency.BTN uml:hasInitialValue "064" ;
              uml:id "_6DD99146-0FA9-4bed-8551-436F4250AEB4" ;
              rdfs:comment "Bhutanese ngultrum." ;
              rdfs:label "BTN" .


:Currency.BWP uml:hasInitialValue "072" ;
              uml:id "_A262A244-582D-4e21-AB35-53207EB676A5" ;
              rdfs:comment "Botswana pula." ;
              rdfs:label "BWP" .


:Currency.BYR uml:hasInitialValue "974" ;
              uml:id "_D717C166-A730-4cdc-829F-6609963A3AD5" ;
              rdfs:comment "Belarusian ruble." ;
              rdfs:label "BYR" .


:Currency.BZD uml:hasInitialValue "084" ;
              uml:id "_67148F2D-1E44-4fc4-BDED-F067ED615541" ;
              rdfs:comment "Belize dollar." ;
              rdfs:label "BZD" .


:Currency.CAD uml:hasInitialValue "124" ;
              uml:id "_60DEBBD0-791B-4542-ABF6-8550366541E4" ;
              rdfs:comment "Canadian dollar." ;
              rdfs:label "CAD" .


:Currency.CDF uml:hasInitialValue "976" ;
              uml:id "_09A4D7FD-DF6C-4476-92BE-45902704EF0B" ;
              rdfs:comment "Congolese franc." ;
              rdfs:label "CDF" .


:Currency.CHF uml:hasInitialValue "756" ;
              uml:id "_5EFD5A2E-31B9-4aea-84D5-914F1C0A31DC" ;
              rdfs:comment "Swiss franc." ;
              rdfs:label "CHF" .


:Currency.CLF uml:hasInitialValue "990" ;
              uml:id "_20CAB3A7-59D7-4bfd-A67F-89C803936FDE" ;
              rdfs:comment "Unidad de Fomento (funds code), Chile." ;
              rdfs:label "CLF" .


:Currency.CLP uml:hasInitialValue "152" ;
              uml:id "_3C66B994-20A3-45a3-94ED-28738DD41344" ;
              rdfs:comment "Chilean peso." ;
              rdfs:label "CLP" .


:Currency.CNY uml:hasInitialValue "156" ;
              uml:id "_550E5C6A-B558-4710-A97A-431C6BB83570" ;
              rdfs:comment "Chinese yuan." ;
              rdfs:label "CNY" .


:Currency.COP uml:hasInitialValue "170" ;
              uml:id "_EDB86E9A-63B1-4423-817C-BAB5A05D9DAF" ;
              rdfs:comment "Colombian peso." ;
              rdfs:label "COP" .


:Currency.COU uml:hasInitialValue "970" ;
              uml:id "_B9FC64A5-B33B-4376-AEE7-54FC483BE070" ;
              rdfs:comment "Unidad de Valor Real." ;
              rdfs:label "COU" .


:Currency.CRC uml:hasInitialValue "188" ;
              uml:id "_2952CAAC-62A1-4b65-8FE3-FD55A4E679C2" ;
              rdfs:comment "Costa Rican colon." ;
              rdfs:label "CRC" .


:Currency.CUC uml:hasInitialValue "931" ;
              uml:id "_A0EC7C95-2C97-4db8-A48F-2CBAF5CA9A34" ;
              rdfs:comment "Cuban convertible peso." ;
              rdfs:label "CUC" .


:Currency.CUP uml:hasInitialValue "192" ;
              uml:id "_734DB065-9B4B-4050-A6A7-7CF77B9A815C" ;
              rdfs:comment "Cuban peso." ;
              rdfs:label "CUP" .


:Currency.CVE uml:hasInitialValue "132" ;
              uml:id "_D70453A7-76B5-4068-8A7E-1ED3539380E3" ;
              rdfs:comment "Cape Verde escudo." ;
              rdfs:label "CVE" .


:Currency.CZK uml:hasInitialValue "203" ;
              uml:id "_D5273F1C-3077-490b-ADAE-F7C7B78E8645" ;
              rdfs:comment "Czech koruna." ;
              rdfs:label "CZK" .


:Currency.DJF uml:hasInitialValue "262" ;
              uml:id "_93B97152-61E3-4181-8D8B-89D3E6462250" ;
              rdfs:comment "Djiboutian franc." ;
              rdfs:label "DJF" .


:Currency.DKK uml:hasInitialValue "208" ;
              uml:id "_34DF27B9-64EE-43bb-BE02-F596A5597F4E" ;
              rdfs:comment "Danish krone." ;
              rdfs:label "DKK" .


:Currency.DOP uml:hasInitialValue "214" ;
              uml:id "_127EECB6-674B-4e97-8720-7D7AF2321011" ;
              rdfs:comment "Dominican peso." ;
              rdfs:label "DOP" .


:Currency.DZD uml:hasInitialValue "012" ;
              uml:id "_934E831F-DE3F-48aa-BABC-DB31FE9B2161" ;
              rdfs:comment "Algerian dinar." ;
              rdfs:label "DZD" .


:Currency.EEK uml:hasInitialValue "233" ;
              uml:id "_618FEB6C-A37E-4123-86D2-926014E12DBF" ;
              rdfs:comment "Estonian kroon." ;
              rdfs:label "EEK" .


:Currency.EGP uml:hasInitialValue "818" ;
              uml:id "_DCAC1DBC-24C0-4b81-A6C7-404445948EA8" ;
              rdfs:comment "Egyptian pound." ;
              rdfs:label "EGP" .


:Currency.ERN uml:hasInitialValue "232" ;
              uml:id "_D9B4813C-E737-41ca-BCC5-D3F709B608AA" ;
              rdfs:comment "Eritrean nakfa." ;
              rdfs:label "ERN" .


:Currency.ETB uml:hasInitialValue "230" ;
              uml:id "_4D239045-36DB-47ca-AD25-DC0767B702D2" ;
              rdfs:comment "Ethiopian birr." ;
              rdfs:label "ETB" .


:Currency.EUR uml:hasInitialValue "978" ;
              uml:id "_C3D20097-F8ED-4a1f-A9F0-6DF9E427E2BB" ;
              rdfs:comment "Euro." ;
              rdfs:label "EUR" .


:Currency.FJD uml:hasInitialValue "242" ;
              uml:id "_078B47FC-790C-4a80-8C9D-30087552BD79" ;
              rdfs:comment "Fiji dollar." ;
              rdfs:label "FJD" .


:Currency.FKP uml:hasInitialValue "238" ;
              uml:id "_FFD30DFB-C207-4997-96E7-A0274F6DB9C1" ;
              rdfs:comment "Falkland Islands pound." ;
              rdfs:label "FKP" .


:Currency.GBP uml:hasInitialValue "826" ;
              uml:id "_006204B2-3B69-49f1-87B0-99312D364461" ;
              rdfs:comment "Pound sterling." ;
              rdfs:label "GBP" .


:Currency.GEL uml:hasInitialValue "981" ;
              uml:id "_43CDA5FE-3792-4187-995A-C28FCFE4B0A6" ;
              rdfs:comment "Georgian lari." ;
              rdfs:label "GEL" .


:Currency.GHS uml:hasInitialValue "936" ;
              uml:id "_C762140A-49DF-4c09-9D98-5673E48F95A9" ;
              rdfs:comment "Ghanaian cedi." ;
              rdfs:label "GHS" .


:Currency.GIP uml:hasInitialValue "929" ;
              uml:id "_D1FE9E47-C3AB-48c5-8941-05758FB8C73A" ;
              rdfs:comment "Gibraltar pound." ;
              rdfs:label "GIP" .


:Currency.GMD uml:hasInitialValue "270" ;
              uml:id "_CD90076F-18D6-405c-B248-6B166EAA42D2" ;
              rdfs:comment "Gambian dalasi." ;
              rdfs:label "GMD" .


:Currency.GNF uml:hasInitialValue "324" ;
              uml:id "_3C97A67D-C22B-49c1-B45D-B3830CB2C13C" ;
              rdfs:comment "Guinean franc." ;
              rdfs:label "GNF" .


:Currency.GTQ uml:hasInitialValue "320" ;
              uml:id "_C3E7DE88-4BA3-4163-90B2-CF3C04007DB3" ;
              rdfs:comment "Guatemalan quetzal." ;
              rdfs:label "GTQ" .


:Currency.GYD uml:hasInitialValue "328" ;
              uml:id "_8D072E8C-EEC7-4b87-9F42-3BEA2B33700F" ;
              rdfs:comment "Guyanese dollar." ;
              rdfs:label "GYD" .


:Currency.HKD uml:hasInitialValue "344" ;
              uml:id "_BE4C99E3-6486-4818-937D-671741A07115" ;
              rdfs:comment "Hong Kong dollar." ;
              rdfs:label "HKD" .


:Currency.HNL uml:hasInitialValue "340" ;
              uml:id "_D29BC449-C8B9-47ec-BDBD-DF15B269B65F" ;
              rdfs:comment "Honduran lempira." ;
              rdfs:label "HNL" .


:Currency.HRK uml:hasInitialValue "191" ;
              uml:id "_EC700002-6F09-4a69-BE82-A2D2E94B9E10" ;
              rdfs:comment "Croatian kuna." ;
              rdfs:label "HRK" .


:Currency.HTG uml:hasInitialValue "332" ;
              uml:id "_5B8C90EA-50EC-4d5b-8120-570F98DB11D9" ;
              rdfs:comment "Haitian gourde." ;
              rdfs:label "HTG" .


:Currency.HUF uml:hasInitialValue "348" ;
              uml:id "_A9FC7F7B-BD91-4cfc-BA7D-0FB991824F36" ;
              rdfs:comment "Hungarian forint." ;
              rdfs:label "HUF" .


:Currency.IDR uml:hasInitialValue "360" ;
              uml:id "_1A0A4950-3866-4eb0-888B-712F87BE8ACD" ;
              rdfs:comment "Indonesian rupiah." ;
              rdfs:label "IDR" .


:Currency.ILS uml:hasInitialValue "376" ;
              uml:id "_6B94E8B6-2848-4ed1-8B2C-C033013642B5" ;
              rdfs:comment "Israeli new sheqel." ;
              rdfs:label "ILS" .


:Currency.INR uml:hasInitialValue "356" ;
              uml:id "_08E2A85B-7695-414e-B468-DE797E59EDCA" ;
              rdfs:comment "Indian rupee." ;
              rdfs:label "INR" .


:Currency.IQD uml:hasInitialValue "368" ;
              uml:id "_3CFF7B10-1EF6-4c8d-A9DA-CAFEE767CA11" ;
              rdfs:comment "Iraqi dinar." ;
              rdfs:label "IQD" .


:Currency.IRR uml:hasInitialValue "364" ;
              uml:id "_90A33AC2-32A7-496b-9B02-00D30F9425E7" ;
              rdfs:comment "Iranian rial." ;
              rdfs:label "IRR" .


:Currency.ISK uml:hasInitialValue "352" ;
              uml:id "_C576CCC9-AD7D-4c0d-A72E-A491AB26C8AF" ;
              rdfs:comment "Icelandic króna." ;
              rdfs:label "ISK" .


:Currency.JMD uml:hasInitialValue "388" ;
              uml:id "_ABCE69F9-8E78-4515-9E2A-FA4C70D70418" ;
              rdfs:comment "Jamaican dollar." ;
              rdfs:label "JMD" .


:Currency.JOD uml:hasInitialValue "400" ;
              uml:id "_E8CB7ED5-6DD2-4f9a-B320-6BC5C118C10B" ;
              rdfs:comment "Jordanian dinar." ;
              rdfs:label "JOD" .


:Currency.JPY uml:hasInitialValue "392" ;
              uml:id "_5471E94F-BE53-4ee9-A711-2AC90244D1D4" ;
              rdfs:comment "Japanese yen." ;
              rdfs:label "JPY" .


:Currency.KES uml:hasInitialValue "404" ;
              uml:id "_4F5A5DBE-D0B7-4b5b-9CB6-809C3850DBE0" ;
              rdfs:comment "Kenyan shilling." ;
              rdfs:label "KES" .


:Currency.KGS uml:hasInitialValue "417" ;
              uml:id "_03306F76-3BEE-48ef-BB80-478F197550E7" ;
              rdfs:comment "Kyrgyzstani som." ;
              rdfs:label "KGS" .


:Currency.KHR uml:hasInitialValue "116" ;
              uml:id "_D5B86766-EB12-45df-8172-A94A04940BF8" ;
              rdfs:comment "Cambodian riel." ;
              rdfs:label "KHR" .


:Currency.KMF uml:hasInitialValue "174" ;
              uml:id "_50D48764-48CE-464c-9E48-38503CC6F25A" ;
              rdfs:comment "Comoro franc." ;
              rdfs:label "KMF" .


:Currency.KPW uml:hasInitialValue "408" ;
              uml:id "_8B1467AD-623E-4020-A26E-4AA27C3C6075" ;
              rdfs:comment "North Korean won." ;
              rdfs:label "KPW" .


:Currency.KRW uml:hasInitialValue "410" ;
              uml:id "_CB7B371F-F72E-477f-A3F6-8FEFEFD7A99D" ;
              rdfs:comment "South Korean won." ;
              rdfs:label "KRW" .


:Currency.KWD uml:hasInitialValue "414" ;
              uml:id "_2394B184-0E47-447f-A13C-0C69A2706198" ;
              rdfs:comment "Kuwaiti dinar." ;
              rdfs:label "KWD" .


:Currency.KYD uml:hasInitialValue "136" ;
              uml:id "_D88FF880-FC0B-4ef3-9CEA-40D459A40539" ;
              rdfs:comment "Cayman Islands dollar." ;
              rdfs:label "KYD" .


:Currency.KZT uml:hasInitialValue "398" ;
              uml:id "_E2399A59-2B6E-45f9-9FAC-E4D799D64A0C" ;
              rdfs:comment "Kazakhstani tenge." ;
              rdfs:label "KZT" .


:Currency.LAK uml:hasInitialValue "418" ;
              uml:id "_7B9EEDAD-83FD-4147-B2B8-671D73B87678" ;
              rdfs:comment "Lao kip." ;
              rdfs:label "LAK" .


:Currency.LBP uml:hasInitialValue "422" ;
              uml:id "_69A852C5-ED56-48ff-A08A-893E6B52D7C8" ;
              rdfs:comment "Lebanese pound." ;
              rdfs:label "LBP" .


:Currency.LKR uml:hasInitialValue "144" ;
              uml:id "_39F04FBC-7A7B-4f82-8D11-60391EDCBDFA" ;
              rdfs:comment "Sri Lanka rupee." ;
              rdfs:label "LKR" .


:Currency.LRD uml:hasInitialValue "430" ;
              uml:id "_7ADF3BC1-033D-4dc7-B2FE-629CCD1240CD" ;
              rdfs:comment "Liberian dollar." ;
              rdfs:label "LRD" .


:Currency.LSL uml:hasInitialValue "426" ;
              uml:id "_9F868853-D68D-481b-A785-A430A0B9AF9E" ;
              rdfs:comment "Lesotho loti." ;
              rdfs:label "LSL" .


:Currency.LTL uml:hasInitialValue "440" ;
              uml:id "_63A336EE-9B6E-417a-A25E-85C2DA15EF35" ;
              rdfs:comment "Lithuanian litas." ;
              rdfs:label "LTL" .


:Currency.LVL uml:hasInitialValue "428" ;
              uml:id "_89A13F2D-9FC3-4218-8573-89653B8FD5AC" ;
              rdfs:comment "Latvian lats." ;
              rdfs:label "LVL" .


:Currency.LYD uml:hasInitialValue "434" ;
              uml:id "_E470BDA3-9985-4b92-ABEC-B4B35F3176D2" ;
              rdfs:comment "Libyan dinar." ;
              rdfs:label "LYD" .


:Currency.MAD uml:hasInitialValue "504" ;
              uml:id "_DF5743DB-E0B2-4dea-9419-BAD992BD9E8A" ;
              rdfs:comment "Moroccan dirham." ;
              rdfs:label "MAD" .


:Currency.MDL uml:hasInitialValue "498" ;
              uml:id "_0DDF9E55-B409-428a-A68F-783623DE7101" ;
              rdfs:comment "Moldovan leu." ;
              rdfs:label "MDL" .


:Currency.MGA uml:hasInitialValue "969" ;
              uml:id "_AA41FDC6-714F-4ceb-813C-5383624A7E17" ;
              rdfs:comment "Malagasy ariary." ;
              rdfs:label "MGA" .


:Currency.MKD uml:hasInitialValue "807" ;
              uml:id "_5EE0BC1C-E12E-4357-8C9C-308693E9B604" ;
              rdfs:comment "Macedonian denar." ;
              rdfs:label "MKD" .


:Currency.MMK uml:hasInitialValue "104" ;
              uml:id "_9B82E309-721E-46fc-9A2A-7B39C741A3D5" ;
              rdfs:comment "Myanma kyat." ;
              rdfs:label "MMK" .


:Currency.MNT uml:hasInitialValue "496" ;
              uml:id "_A795B587-AD16-4a4a-B8D5-64C42499C69A" ;
              rdfs:comment "Mongolian tugrik." ;
              rdfs:label "MNT" .


:Currency.MOP uml:hasInitialValue "446" ;
              uml:id "_BDA58344-8BD8-4b8a-B625-452623B8F726" ;
              rdfs:comment "Macanese pataca." ;
              rdfs:label "MOP" .


:Currency.MRO uml:hasInitialValue "478" ;
              uml:id "_4562AF34-2197-4b1f-95BA-9E9227445DF9" ;
              rdfs:comment "Mauritanian ouguiya." ;
              rdfs:label "MRO" .


:Currency.MUR uml:hasInitialValue "480" ;
              uml:id "_44EDF874-F3D7-4e82-B28C-D023F1194499" ;
              rdfs:comment "Mauritian rupee." ;
              rdfs:label "MUR" .


:Currency.MVR uml:hasInitialValue "462" ;
              uml:id "_1F2F920D-CD52-47d0-AC8D-C538B5C21AB6" ;
              rdfs:comment "Maldivian rufiyaa." ;
              rdfs:label "MVR" .


:Currency.MWK uml:hasInitialValue "454" ;
              uml:id "_BE3EC824-D76D-43ba-81CE-1AE454F922C4" ;
              rdfs:comment "Malawian kwacha." ;
              rdfs:label "MWK" .


:Currency.MXN uml:hasInitialValue "484" ;
              uml:id "_D1D1FC8D-DA05-4e23-B014-57071E0F0018" ;
              rdfs:comment "Mexican peso." ;
              rdfs:label "MXN" .


:Currency.MYR uml:hasInitialValue "458" ;
              uml:id "_B1DC20F0-1417-40ee-AEA3-26ADF3BDDBE8" ;
              rdfs:comment "Malaysian ringgit." ;
              rdfs:label "MYR" .


:Currency.MZN uml:hasInitialValue "943" ;
              uml:id "_22188237-E195-4385-9246-27371700629A" ;
              rdfs:comment "Mozambican metical." ;
              rdfs:label "MZN" .


:Currency.NAD uml:hasInitialValue "516" ;
              uml:id "_E0DC0D79-C74B-415e-BB1B-DD49A784E030" ;
              rdfs:comment "Namibian dollar." ;
              rdfs:label "NAD" .


:Currency.NGN uml:hasInitialValue "566" ;
              uml:id "_D3F3C26B-CC43-4c17-9986-98F0FD50337F" ;
              rdfs:comment "Nigerian naira." ;
              rdfs:label "NGN" .


:Currency.NIO uml:hasInitialValue "558" ;
              uml:id "_EC9DF490-2CCA-4f91-ACE9-C5D570FA2393" ;
              rdfs:comment "Cordoba oro." ;
              rdfs:label "NIO" .


:Currency.NOK uml:hasInitialValue "578" ;
              uml:id "_E6F2DF01-C818-41e4-85DD-7607D1060F79" ;
              rdfs:comment "Norwegian krone." ;
              rdfs:label "NOK" .


:Currency.NPR uml:hasInitialValue "524" ;
              uml:id "_5A687CAD-5670-4cb7-B013-ED56004592D0" ;
              rdfs:comment "Nepalese rupee." ;
              rdfs:label "NPR" .


:Currency.NZD uml:hasInitialValue "554" ;
              uml:id "_9F158607-8615-434f-8DC5-7BE0EE7932D8" ;
              rdfs:comment "New Zealand dollar." ;
              rdfs:label "NZD" .


:Currency.OMR uml:hasInitialValue "512" ;
              uml:id "_B5F0D3C0-4A76-497a-8D57-7346A8A4FF60" ;
              rdfs:comment "Omani rial." ;
              rdfs:label "OMR" .


:Currency.PAB uml:hasInitialValue "590" ;
              uml:id "_1C281135-BD47-4d3b-9BAF-24F62343F378" ;
              rdfs:comment "Panamanian balboa." ;
              rdfs:label "PAB" .


:Currency.PEN uml:hasInitialValue "604" ;
              uml:id "_D77761B6-BD9A-48b7-8647-F969174B827B" ;
              rdfs:comment "Peruvian nuevo sol." ;
              rdfs:label "PEN" .


:Currency.PGK uml:hasInitialValue "598" ;
              uml:id "_49C0D37A-F1C2-4b89-8825-67A202FAF1C1" ;
              rdfs:comment "Papua New Guinean kina." ;
              rdfs:label "PGK" .


:Currency.PHP uml:hasInitialValue "608" ;
              uml:id "_28D08385-3612-421a-9892-6D5B7F0F5755" ;
              rdfs:comment "Philippine peso." ;
              rdfs:label "PHP" .


:Currency.PKR uml:hasInitialValue "586" ;
              uml:id "_0C43307C-30C1-48e1-A5F5-F7815FD1061B" ;
              rdfs:comment "Pakistani rupee." ;
              rdfs:label "PKR" .


:Currency.PLN uml:hasInitialValue "985" ;
              uml:id "_E1502883-E84C-4b69-8754-0E0D8F6F0541" ;
              rdfs:comment "Polish zloty." ;
              rdfs:label "PLN" .


:Currency.PYG uml:hasInitialValue "600" ;
              uml:id "_FE57212E-2EB2-4ca9-BA01-D0B0B89EB39E" ;
              rdfs:comment "Paraguayan guaraní." ;
              rdfs:label "PYG" .


:Currency.QAR uml:hasInitialValue "634" ;
              uml:id "_518AE7C8-AABE-4514-86E7-B1E98ABE8666" ;
              rdfs:comment "Qatari rial." ;
              rdfs:label "QAR" .


:Currency.RON uml:hasInitialValue "946" ;
              uml:id "_1965570A-1DF4-447f-A71B-90023BEAC168" ;
              rdfs:comment "Romanian new leu." ;
              rdfs:label "RON" .


:Currency.RSD uml:hasInitialValue "941" ;
              uml:id "_77012A2B-0161-41e8-AB66-CCB6960BF0E7" ;
              rdfs:comment "Serbian dinar." ;
              rdfs:label "RSD" .


:Currency.RUB uml:hasInitialValue "643" ;
              uml:id "_A677E20A-9FF6-4cd7-88FF-A862704AB5A9" ;
              rdfs:comment "Russian rouble." ;
              rdfs:label "RUB" .


:Currency.RWF uml:hasInitialValue "646" ;
              uml:id "_C8036589-4CFD-4467-8FCE-4B3EADCE7FDE" ;
              rdfs:comment "Rwandan franc." ;
              rdfs:label "RWF" .


:Currency.SAR uml:hasInitialValue "682" ;
              uml:id "_C3A5DF37-CB42-4ef7-88B4-548557EC41B8" ;
              rdfs:comment "Saudi riyal." ;
              rdfs:label "SAR" .


:Currency.SBD uml:hasInitialValue "090" ;
              uml:id "_CD30CB39-454B-4bfe-8273-79AD119DCD0A" ;
              rdfs:comment "Solomon Islands dollar." ;
              rdfs:label "SBD" .


:Currency.SCR uml:hasInitialValue "690" ;
              uml:id "_61803DBD-73B1-4b87-8CD3-4CA3979170ED" ;
              rdfs:comment "Seychelles rupee." ;
              rdfs:label "SCR" .


:Currency.SDG uml:hasInitialValue "938" ;
              uml:id "_1E0C75F9-76EE-4476-AB27-6D80D5F6BEF3" ;
              rdfs:comment "Sudanese pound." ;
              rdfs:label "SDG" .


:Currency.SEK uml:hasInitialValue "752" ;
              uml:id "_7AD17FA7-8042-468a-9A4E-5A31A4F24858" ;
              rdfs:comment "Swedish krona/kronor." ;
              rdfs:label "SEK" .


:Currency.SGD uml:hasInitialValue "702" ;
              uml:id "_052FA818-D6EE-497e-9F6E-FA732781A281" ;
              rdfs:comment "Singapore dollar." ;
              rdfs:label "SGD" .


:Currency.SHP uml:hasInitialValue "654" ;
              uml:id "_524D8445-4F6D-42d9-B8D3-8E879FD58D48" ;
              rdfs:comment "Saint Helena pound." ;
              rdfs:label "SHP" .


:Currency.SLL uml:hasInitialValue "694" ;
              uml:id "_205D4979-6002-406a-A6B5-221F6776ED70" ;
              rdfs:comment "Sierra Leonean leone." ;
              rdfs:label "SLL" .


:Currency.SOS uml:hasInitialValue "706" ;
              uml:id "_C53B8253-FBFB-429f-BF42-5D498E2B5FF7" ;
              rdfs:comment "Somali shilling." ;
              rdfs:label "SOS" .


:Currency.SRD uml:hasInitialValue "968" ;
              uml:id "_D0B98BEE-00E7-4b90-BB2C-D8408C5F0A27" ;
              rdfs:comment "Surinamese dollar." ;
              rdfs:label "SRD" .


:Currency.STD uml:hasInitialValue "678" ;
              uml:id "_084AC846-EC27-4458-BD38-023AC6DC37AB" ;
              rdfs:comment "São Tomé and Príncipe dobra." ;
              rdfs:label "STD" .


:Currency.SYP uml:hasInitialValue "760" ;
              uml:id "_F25FA2B4-6A4C-4438-BC83-6AE73E69B688" ;
              rdfs:comment "Syrian pound." ;
              rdfs:label "SYP" .


:Currency.SZL uml:hasInitialValue "748" ;
              uml:id "_66A2C3AE-1447-49cd-B92E-C3A29F1B9A7B" ;
              rdfs:comment "Lilangeni." ;
              rdfs:label "SZL" .


:Currency.THB uml:hasInitialValue "764" ;
              uml:id "_C511B839-D3F0-4e15-BD80-F9F1E1EA4FA3" ;
              rdfs:comment "Thai baht." ;
              rdfs:label "THB" .


:Currency.TJS uml:hasInitialValue "972" ;
              uml:id "_AE51E72D-CCB5-4870-9FD4-51A55259C6DF" ;
              rdfs:comment "Tajikistani somoni." ;
              rdfs:label "TJS" .


:Currency.TMT uml:hasInitialValue "934" ;
              uml:id "_C862B797-6B08-45f6-93E9-F561F63FCE04" ;
              rdfs:comment "Turkmenistani manat." ;
              rdfs:label "TMT" .


:Currency.TND uml:hasInitialValue "788" ;
              uml:id "_D7CA53B9-8DBF-45a9-9D7E-9F989A5F9B93" ;
              rdfs:comment "Tunisian dinar." ;
              rdfs:label "TND" .


:Currency.TOP uml:hasInitialValue "776" ;
              uml:id "_36E56606-AFB8-4f89-BC80-7C7AC374AF1C" ;
              rdfs:comment "Tongan pa'anga." ;
              rdfs:label "TOP" .


:Currency.TRY uml:hasInitialValue "949" ;
              uml:id "_2158C7AC-F5AD-4f0e-BC14-8CB3E969A689" ;
              rdfs:comment "Turkish lira." ;
              rdfs:label "TRY" .


:Currency.TTD uml:hasInitialValue "780" ;
              uml:id "_02F344FD-F2C4-4daa-A3C4-D23CEB062C9C" ;
              rdfs:comment "Trinidad and Tobago dollar." ;
              rdfs:label "TTD" .


:Currency.TWD uml:hasInitialValue "901" ;
              uml:id "_5BA60238-098D-4a4c-BBB0-674669A73713" ;
              rdfs:comment "New Taiwan dollar." ;
              rdfs:label "TWD" .


:Currency.TZS uml:hasInitialValue "834" ;
              uml:id "_76249704-5DD8-47f5-8DAC-2EAA6E24FE28" ;
              rdfs:comment "Tanzanian shilling." ;
              rdfs:label "TZS" .


:Currency.UAH uml:hasInitialValue "980" ;
              uml:id "_4E68F4B3-C55C-4e8d-89C1-ADE21CBD0672" ;
              rdfs:comment "Ukrainian hryvnia." ;
              rdfs:label "UAH" .


:Currency.UGX uml:hasInitialValue "800" ;
              uml:id "_EEFD1900-19F1-4760-BDED-DE34161C9F32" ;
              rdfs:comment "Ugandan shilling." ;
              rdfs:label "UGX" .


:Currency.USD uml:hasInitialValue "840" ;
              uml:id "_F8F87BEA-4269-49de-B28F-8DC130EC9AAC" ;
              rdfs:comment "United States dollar." ;
              rdfs:label "USD" .


:Currency.UYU uml:hasInitialValue "858" ;
              uml:id "_03676FCF-6C91-465f-8A8E-4E571BCE9BDD" ;
              rdfs:comment "Uruguayan peso." ;
              rdfs:label "UYU" .


:Currency.UZS uml:hasInitialValue "860" ;
              uml:id "_887E3DEF-310A-4f6b-89D9-DBBA9059E978" ;
              rdfs:comment "Uzbekistan som." ;
              rdfs:label "UZS" .


:Currency.VEF uml:hasInitialValue "937" ;
              uml:id "_3CAF99DC-92D0-4808-A1EB-03AE3F8F8391" ;
              rdfs:comment "Venezuelan bolívar fuerte." ;
              rdfs:label "VEF" .


:Currency.VND uml:hasInitialValue "704" ;
              uml:id "_E2D7E769-E4E7-42a5-86D3-E2B0B44033D1" ;
              rdfs:comment "Vietnamese Dong." ;
              rdfs:label "VND" .


:Currency.VUV uml:hasInitialValue "548" ;
              uml:id "_FDC3A68E-4BA2-4b69-A0FD-1209C3C5AC3E" ;
              rdfs:comment "Vanuatu vatu." ;
              rdfs:label "VUV" .


:Currency.WST uml:hasInitialValue "882" ;
              uml:id "_1E764ADE-1E5F-42ed-B4D6-937E133B689F" ;
              rdfs:comment "Samoan tala." ;
              rdfs:label "WST" .


:Currency.XAF uml:hasInitialValue "950" ;
              uml:id "_1AA2CC12-FACD-436c-AD73-FED872AA7770" ;
              rdfs:comment "CFA franc BEAC." ;
              rdfs:label "XAF" .


:Currency.XCD uml:hasInitialValue "951" ;
              uml:id "_214A7E04-0943-4f38-AFD6-3BE0580483A0" ;
              rdfs:comment "East Caribbean dollar." ;
              rdfs:label "XCD" .


:Currency.XOF uml:hasInitialValue "952" ;
              uml:id "_EFB2A7B8-B9C9-4c9c-A244-9D10086829AF" ;
              rdfs:comment "CFA Franc BCEAO." ;
              rdfs:label "XOF" .


:Currency.XPF uml:hasInitialValue "953" ;
              uml:id "_1083709A-0F74-4a5d-A9CD-DA129B5853D5" ;
              rdfs:comment "CFP franc." ;
              rdfs:label "XPF" .


:Currency.YER uml:hasInitialValue "886" ;
              uml:id "_B7ECDF90-9201-40eb-9B03-A8698A81AE3C" ;
              rdfs:comment "Yemeni rial." ;
              rdfs:label "YER" .


:Currency.ZAR uml:hasInitialValue "710" ;
              uml:id "_73C9E782-D310-4f6f-943E-05382AE412FF" ;
              rdfs:comment "South African rand." ;
              rdfs:label "ZAR" .


:Currency.ZMK uml:hasInitialValue "894" ;
              uml:id "_C1A242CF-29D6-44a6-9EF5-A16DF42A2C2C" ;
              rdfs:comment "Zambian kwacha." ;
              rdfs:label "ZMK" .


:Currency.ZWL uml:hasInitialValue "932" ;
              uml:id "_DCF62BC1-0B87-44a6-9DEA-A241F73BA296" ;
              rdfs:comment "Zimbabwe dollar." ;
              rdfs:label "ZWL" .


:CurrentStatusSC.ACTIVE uml:id "_D99F06E5-09C9-44bc-8769-CA84E41C4D44" ;
                        rdfs:label "ACTIVE" .


:CurrentStatusSC.INACTIVE uml:id "_6CC2D3CB-2B80-4da8-94BE-5BD55A4DCB4B" ;
                          rdfs:label "INACTIVE" .


:CurveStyle.constantYValue uml:id "_FC48CB26-36DB-4228-8203-0B5F1CDF4A73" ;
                           rdfs:comment "The Y-axis values are assumed constant until the next curve point and prior to the first curve point." ;
                           rdfs:label "constantYValue" .


:CurveStyle.straightLineYValues uml:id "_C87B3CE1-F526-4e92-A292-0238CA829EA0" ;
                                rdfs:comment "The Y-axis values are assumed to be a straight line between values.  Also known as linear interpolation." ;
                                rdfs:label "straightLineYValues" .


:CustomerBillingKind.consolidatedEss uml:id "_39A91264-B15E-404f-9574-132CB0827D0B" ;
                                     rdfs:comment "Consolidated bill from energy service supplier (ESS)." ;
                                     rdfs:label "consolidatedEss" .


:CustomerBillingKind.consolidatedUdc uml:id "_98DD2388-CD25-49ae-AAD0-5D8676258208" ;
                                     rdfs:comment "Consolidated bill from utility distribution company (UDC)." ;
                                     rdfs:label "consolidatedUdc" .


:CustomerBillingKind.other uml:id "_292B7ACC-47D8-4f18-A324-B2F3F4425BD5" ;
                           rdfs:label "other" .


:CustomerBillingKind.separateEssUdc uml:id "_AB5DF4A3-6DBA-4404-8730-32F96D2297E0" ;
                                    rdfs:comment "Separate bills from ESS and UDC." ;
                                    rdfs:label "separateEssUdc" .


:CustomerKind.commercialIndustrial uml:id "_EC2ED083-2201-478d-B1A6-86DBAEA90845" ;
                                   rdfs:comment "Commercial industrial customer." ;
                                   rdfs:label "commercialIndustrial" .


:CustomerKind.energyServiceScheduler uml:id "_B82F97A2-DEF2-4a5b-B483-A250EC222B81" ;
                                     rdfs:comment "Customer as energy service scheduler." ;
                                     rdfs:label "energyServiceScheduler" .


:CustomerKind.energyServiceSupplier uml:id "_FFBBED52-2D6E-4eb1-AEF5-D232600FFB93" ;
                                    rdfs:comment "Customer as energy service supplier." ;
                                    rdfs:label "energyServiceSupplier" .


:CustomerKind.enterprise uml:id "_59A143B2-3F2E-4a71-96A1-5E6BDB5AD175" ;
                         rdfs:comment "Enterprise customer" ;
                         rdfs:label "enterprise" .


:CustomerKind.internalUse uml:id "_08F89276-2BCD-4707-A33C-37906D4F2177" ;
                          rdfs:comment "Internal use customer." ;
                          rdfs:label "internalUse" .


:CustomerKind.other uml:id "_77F956BF-AD13-44b5-8CC6-E6F5AC29474B" ;
                    rdfs:comment "Other kind of customer." ;
                    rdfs:label "other" .


:CustomerKind.pumpingLoad uml:id "_754B8EEB-8A10-4024-8CA3-E3ACECBD84B6" ;
                          rdfs:comment "Pumping load customer." ;
                          rdfs:label "pumpingLoad" .


:CustomerKind.regionalOperator uml:id "_6BD3C61D-00C7-47bc-B1C8-07C3B453FE72" ;
                               rdfs:comment "Regional Operator customer" ;
                               rdfs:label "regionalOperator" .


:CustomerKind.residential uml:id "_8BF12334-C823-49f4-9363-2DE043980AE6" ;
                          rdfs:comment "Residential customer." ;
                          rdfs:label "residential" .


:CustomerKind.residentialAndCommercial uml:id "_6A17FEE4-95A0-4d29-AF9A-863B63410AFE" ;
                                       rdfs:comment "Residential and commercial customer." ;
                                       rdfs:label "residentialAndCommercial" .


:CustomerKind.residentialAndStreetlight uml:id "_DB100B72-C153-47ae-9E44-255DD4B84BDA" ;
                                        rdfs:comment "Residential and streetlight customer." ;
                                        rdfs:label "residentialAndStreetlight" .


:CustomerKind.residentialFarmService uml:id "_463934FD-988D-46b6-B1D2-00854AABDB2A" ;
                                     rdfs:comment "Residential farm service customer." ;
                                     rdfs:label "residentialFarmService" .


:CustomerKind.residentialStreetlightOthers uml:id "_A66F5FB0-F221-402a-A663-E5573E90C010" ;
                                           rdfs:comment "Residential streetlight or other related customer." ;
                                           rdfs:label "residentialStreetlightOthers" .


:CustomerKind.subsidiary uml:id "_25A9FB6D-F363-4474-A3AD-0BF9C41FEEB7" ;
                         rdfs:comment "Subsidiary customer" ;
                         rdfs:label "subsidiary" .


:CustomerKind.windMachine uml:id "_576A1B72-9FB2-45f8-8064-5FE18E5B5023" ;
                          rdfs:comment "Wind machine customer." ;
                          rdfs:label "windMachine" .


:DAMMarketType.DAM uml:id "_56D6B5E1-BB8C-4a98-AFC1-C345954DD74F" ;
                   rdfs:label "DAM" .


:DCConverterOperatingModeKind.bipolar uml:id "_AAAD7D9F-9637-4dfc-95BC-0980D8C08508" ;
                                      rdfs:comment "Bipolar operation." ;
                                      rdfs:label "bipolar" .


:DCConverterOperatingModeKind.monopolarGroundReturn uml:id "_ACBACA8D-7817-4bb6-9775-7025BF6DFE29" ;
                                                    rdfs:comment "Monopolar operation with ground return." ;
                                                    rdfs:label "monopolarGroundReturn" .


:DCConverterOperatingModeKind.monopolarMetallicReturn uml:id "_941FD023-3DAB-4c02-9F05-E4A56F884CA4" ;
                                                      rdfs:comment "Monopolar operation with metallic return." ;
                                                      rdfs:label "monopolarMetallicReturn" .


:DCPolarityKind.middle uml:id "_05BB3BFF-DB86-48b8-84D2-2C60BE4A89FE" ;
                       rdfs:comment "Middle pole. The converter terminal is the midpoint in a bipolar or symmetric monopole configuration. The midpoint can be grounded and/or have a metallic return." ;
                       rdfs:label "middle" .


:DCPolarityKind.negative uml:id "_398B4A2E-72D3-482e-B61A-20AC1CEC80E6" ;
                         rdfs:comment "Negative pole. The converter terminal is intended to operate at a negative voltage relative the midpoint or positive terminal." ;
                         rdfs:label "negative" .


:DCPolarityKind.positive uml:id "_9E7235FE-D9EA-4f9d-BB58-8FDAE5188207" ;
                         rdfs:comment "Positive pole. The converter terminal is intended to operate at a positive voltage relative the midpoint or negative terminal." ;
                         rdfs:label "positive" .


:DERParameterKind.activePower uml:hasInitialValue "2" ;
                              uml:id "_16846A16-80B1-410b-BDDF-3C8A816CB6E9" ;
                              rdfs:comment "The amount of power being used, measured in Watts." ;
                              rdfs:label "activePower" .


:DERParameterKind.apparentPower uml:hasInitialValue "1" ;
                                uml:id "_F637F32F-F3A8-4698-A605-EBE478971F6F" ;
                                rdfs:comment "The combination of reactive power and active power, and is the product of voltage and current without reference to the phase angle." ;
                                rdfs:label "apparentPower" .


:DERParameterKind.decreasingRampRate uml:hasInitialValue "11" ;
                                     uml:id "_D4314977-8AB6-491d-B138-032D89D5518E" ;
                                     rdfs:comment "An indication of whether the ramp rate associated with a curve is negative." ;
                                     rdfs:label "decreasingRampRate" .


:DERParameterKind.highFilterBiDirectionalRegulation uml:hasInitialValue "4" ;
                                                    uml:id "_FFF8F724-58AE-412d-BE7A-E2D25B2A547F" ;
                                                    rdfs:comment "AC voltage regulation of high frequency" ;
                                                    rdfs:label "highFilterBiDirectionalRegulation" .


:DERParameterKind.highFilterDownRegulation uml:hasInitialValue "8" ;
                                           uml:id "_989D2F3F-AB15-41cf-981C-7FC775A6FCB0" ;
                                           rdfs:comment "High Pass Frequency Regulation downwards." ;
                                           rdfs:label "highFilterDownRegulation" .


:DERParameterKind.highFilterUpRegulation uml:hasInitialValue "6" ;
                                         uml:id "_9F7E46C8-B921-4120-98C1-C8AFC29C0DB3" ;
                                         rdfs:comment "High Pass Frequency Regulation upwards." ;
                                         rdfs:label "highFilterUpRegulation" .


:DERParameterKind.increasingRampRate uml:hasInitialValue "10" ;
                                     uml:id "_DC389771-ECB1-4fba-AD22-7062EA4BEC37" ;
                                     rdfs:comment "An indication of whether the ramp rate associated with a curve is positive." ;
                                     rdfs:label "increasingRampRate" .


:DERParameterKind.lowFilterBiDirectionalRegulation uml:hasInitialValue "5" ;
                                                   uml:id "_1153C4D8-5FBB-411f-898F-8F66900EB543" ;
                                                   rdfs:comment "Used to filter out the sinosuidal disturbances to the grid." ;
                                                   rdfs:label "lowFilterBiDirectionalRegulation" .


:DERParameterKind.lowFilterDownRegulation uml:hasInitialValue "9" ;
                                          uml:id "_D53EFD5E-ADD6-415c-AEC7-D7ECD9F2F3CA" ;
                                          rdfs:comment "Low Pass Frequency Regulation downwards." ;
                                          rdfs:label "lowFilterDownRegulation" .


:DERParameterKind.lowFilterUpRegulation uml:hasInitialValue "7" ;
                                        uml:id "_E7994ABD-F21E-4da0-8EE6-6FBA9ED6D9C7" ;
                                        rdfs:comment "Low Pass Frequency Regulation upwards." ;
                                        rdfs:label "lowFilterUpRegulation" .


:DERParameterKind.reactivePower uml:hasInitialValue "3" ;
                                uml:id "_EDDAE413-7BC8-479f-8CE0-9B8D196C2A5B" ;
                                rdfs:comment "The measure of reactance, measured in Vars." ;
                                rdfs:label "reactivePower" .


:DERParameterKind.voltage uml:hasInitialValue "12" ;
                          uml:id "_3EB87DF4-5242-4fc8-B1AC-88A8DF89CCB8" ;
                          rdfs:comment "The measure of difference in potential between two points, measured in Volts." ;
                          rdfs:label "voltage" .


:DERUnitSymbol.A uml:hasInitialValue "5" ;
                 uml:id "_7A9AC903-BD3E-4f5d-8C29-6C343D7D5E29" ;
                 rdfs:comment "Current in Ampere." ;
                 rdfs:label "A" .


:DERUnitSymbol.Ah uml:hasInitialValue "106" ;
                  uml:id "_C5456A5A-C31B-4fb6-A2F5-04D727CA2DF1" ;
                  rdfs:comment "Ampere-hours, Ampere-hours." ;
                  rdfs:label "Ah" .


:DERUnitSymbol.As uml:hasInitialValue "68" ;
                  uml:id "_0B81B14F-8427-4f74-A191-F0F3A8E91064" ;
                  rdfs:comment "Ampere seconds (A·s)." ;
                  rdfs:label "As" .


:DERUnitSymbol.Btu uml:hasInitialValue "132" ;
                   uml:id "_4272AE09-251E-44d5-97D8-DBB7DC50D99B" ;
                   rdfs:comment "Energy, British Thermal Unit." ;
                   rdfs:label "Btu" .


:DERUnitSymbol.Hz uml:hasInitialValue "33" ;
                  uml:id "_0B4DB8BE-FF24-479c-B066-0F5785433049" ;
                  rdfs:comment "Frequency in Hertz (1/s)." ;
                  rdfs:label "Hz" .


:DERUnitSymbol.Q uml:hasInitialValue "100" ;
                 uml:id "_5AAEE5FB-FD71-4d90-98B7-F243410E8789" ;
                 rdfs:comment "Quantity power, Q." ;
                 rdfs:label "Q" .


:DERUnitSymbol.Qh uml:hasInitialValue "101" ;
                  uml:id "_C7E89DB8-40F6-4555-8D3A-E1181DC8DA0A" ;
                  rdfs:comment "Quantity energy, Qh." ;
                  rdfs:label "Qh" .


:DERUnitSymbol.V uml:hasInitialValue "29" ;
                 uml:id "_7F2A4D6F-A670-47a6-B904-385DF96D8BDF" ;
                 rdfs:comment "Electric potential in Volt (W/A)." ;
                 rdfs:label "V" .


:DERUnitSymbol.VA uml:hasInitialValue "61" ;
                  uml:id "_AC621C92-D10D-4327-A43E-AC55D1B4EA41" ;
                  rdfs:comment "Apparent power in Volt Ampere (See also real power and reactive power.)" ;
                  rdfs:label "VA" .


:DERUnitSymbol.VAh uml:hasInitialValue "71" ;
                   uml:id "_D86E2C84-3496-42cf-A9B7-9C458C442405" ;
                   rdfs:comment "Apparent energy in Volt Ampere hours." ;
                   rdfs:label "VAh" .


:DERUnitSymbol.VAr uml:hasInitialValue "63" ;
                   uml:id "_978031C4-430D-4c95-907C-6BB23BD29E64" ;
                   rdfs:comment """Reactive power in Volt Ampere reactive. The “reactive” or “imaginary” component of electrical power (VIsin(phi)). (See also real power and apparent power).
Note: Different meter designs use different methods to arrive at their results. Some meters may compute reactive power as an arithmetic value, while others compute the value vectorially. The data consumer should determine the method in use and the suitability of the measurement for the intended purpose.""" ;
                   rdfs:label "VAr" .


:DERUnitSymbol.VArh uml:hasInitialValue "73" ;
                    uml:id "_73A57724-8DC2-48b5-8087-1F6DF19A04E3" ;
                    rdfs:comment "Reactive energy in Volt Ampere reactive hours." ;
                    rdfs:label "VArh" .


:DERUnitSymbol.VPerVA uml:hasInitialValue "153" ;
                      uml:id "_305F5C22-1D7C-43aa-89F1-792DEDBA7938" ;
                      rdfs:comment "Power factor, PF, the ratio of the active power to the apparent power. Note: The sign convention used for power factor will differ between IEC meters and EEI (ANSI) meters. It is assumed that the data consumers understand the type of meter being used and agree on the sign convention in use at any given utility." ;
                      rdfs:label "VPerVA" .


:DERUnitSymbol.VPerVAr uml:id "_C6315AC6-FE12-4cb6-B5AE-C2229F89DBF2" ;
                       rdfs:comment "Power factor, PF, the ratio of the active power to the apparent power. Note: The sign convention used for power factor will differ between IEC meters and EEI (ANSI) meters. It is assumed that the data consumers understand the type of meter being used and agree on the sign convention in use at any given utility." ;
                       rdfs:label "VPerVAr" .


:DERUnitSymbol.Vh uml:hasInitialValue "280" ;
                  uml:id "_986EFCBC-ACFF-4fee-92C2-E797D9B4C075" ;
                  rdfs:comment "Volt-hour, Volt hours." ;
                  rdfs:label "Vh" .


:DERUnitSymbol.Vs uml:hasInitialValue "66" ;
                  uml:id "_5F8BE774-D837-4c05-A670-8865D62CA98E" ;
                  rdfs:comment "Volt second (Ws/A)." ;
                  rdfs:label "Vs" .


:DERUnitSymbol.W uml:hasInitialValue "38" ;
                 uml:id "_88827AD2-825E-4561-835A-FCC66786029F" ;
                 rdfs:comment "Real power in Watt (J/s). Electrical power may have real and reactive components. The real portion of electrical power (I²R or VIcos(phi)), is expressed in Watts. (See also apparent power and reactive power.)" ;
                 rdfs:label "W" .


:DERUnitSymbol.WPerA uml:id "_FDA22034-0417-468a-B6BA-99F47A3B2B9A" ;
                     rdfs:comment "Active power per current flow, watt per Ampere." ;
                     rdfs:label "WPerA" .


:DERUnitSymbol.WPers uml:hasInitialValue "81" ;
                     uml:id "_CF56506A-6925-4011-B563-B25A7B50CDCF" ;
                     rdfs:comment "Ramp rate in Watt per second." ;
                     rdfs:label "WPers" .


:DERUnitSymbol.Wh uml:hasInitialValue "72" ;
                  uml:id "_AECB659C-2929-4fd4-9CB6-611FEB942AE4" ;
                  rdfs:comment "Real energy in Watt hours." ;
                  rdfs:label "Wh" .


:DERUnitSymbol.deg uml:hasInitialValue "9" ;
                   uml:id "_0402C11E-2D61-4e84-B620-785C4BCFFE29" ;
                   rdfs:comment "Plane angle in degrees." ;
                   rdfs:label "deg" .


:DERUnitSymbol.degC uml:hasInitialValue "23" ;
                    uml:id "_5702078E-2D9F-4441-9D76-5AFBBEF47ABA" ;
                    rdfs:comment """Relative temperature in degrees Celsius.
In the SI unit system the symbol is ºC. Electric charge is measured in coulomb that has the unit symbol C. To distinguish degree Celsius form coulomb the symbol used in the UML is degC. Reason for not using ºC is the special character º is difficult to manage in software.""" ;
                    rdfs:label "degC" .


:DERUnitSymbol.h uml:hasInitialValue "84" ;
                 uml:id "_EBF5C74E-A549-45ca-A24C-E1756F0CB824" ;
                 rdfs:comment "Time, hour = 60 min = 3600 s." ;
                 rdfs:label "h" .


:DERUnitSymbol.min uml:hasInitialValue "85" ;
                   uml:id "_DF1873F1-242E-4af4-9E9F-435AC692BFBF" ;
                   rdfs:comment "Time, minute  = 60 s." ;
                   rdfs:label "min" .


:DERUnitSymbol.ohm uml:hasInitialValue "30" ;
                   uml:id "_7210C686-6570-4986-91A9-439908D873F6" ;
                   rdfs:comment "Electric resistance in ohm (V/A)." ;
                   rdfs:label "ohm" .


:DERUnitSymbol.ohmPerm uml:id "_1C636B7F-E4DA-49e2-8E45-AEA912B85644" ;
                       rdfs:comment "Electric resistance per length in ohm per metre ((V/A)/m)." ;
                       rdfs:label "ohmPerm" .


:DERUnitSymbol.ohmm uml:hasInitialValue "102" ;
                    uml:id "_2D664514-077E-4aee-8122-AFB07985B33C" ;
                    rdfs:comment "resistivity, Ohm metre, (rho)." ;
                    rdfs:label "ohmm" .


:DERUnitSymbol.onePerHz uml:id "_93D18B7A-147C-4b9c-9CB8-91486487AD51" ;
                        rdfs:comment "Reciprocal of frequency (1/Hz)." ;
                        rdfs:label "onePerHz" .


:DERUnitSymbol.s uml:hasInitialValue "4" ;
                 uml:id "_427AE896-5C28-4244-AC66-01B9BEBF1CF0" ;
                 rdfs:comment "Time in seconds." ;
                 rdfs:label "s" .


:DERUnitSymbol.therm uml:hasInitialValue "169" ;
                     uml:id "_7BE76D3D-808C-4771-BC8B-5C5F5DCA273D" ;
                     rdfs:comment "Energy, Therm." ;
                     rdfs:label "therm" .


:DINStandardEditionKind._1985 uml:id "_EE91301E-96D2-446a-82F3-1BBF8A6CAB6E" ;
                              rdfs:comment "1985 standard edition." ;
                              rdfs:label "1985" .


:DINStandardEditionKind.none uml:id "_06B2CE9F-588E-4048-9DE7-8593FFF6F644" ;
                             rdfs:comment "No standard edition." ;
                             rdfs:label "none" .


:DINStandardEditionKind.unknown uml:id "_BD10835E-942F-4fc0-846B-5C1F43AE5013" ;
                                rdfs:comment "Unknown standard edition." ;
                                rdfs:label "unknown" .


:DINStandardKind._51353 uml:id "_BEF784C3-0C79-445f-B3F7-E6B9261C20D1" ;
                        rdfs:comment "Testing of insulating oils; detection of corrosive sulfur; silver strip test." ;
                        rdfs:label "51353" .


:DemographicKind.other uml:id "_71AC187C-F9B4-44e9-B115-DC13871025CF" ;
                       rdfs:label "other" .


:DemographicKind.rural uml:id "_E4DC627B-8653-44c3-A8B8-0BB848A9403E" ;
                       rdfs:label "rural" .


:DemographicKind.urban uml:id "_3BBBAB00-F35D-4f18-84C4-701BEC60674F" ;
                       rdfs:label "urban" .


:DependencyKind.mutuallyExclusive uml:id "_6FD4EB93-7C76-4fb2-852F-D7B757F09279" ;
                                  rdfs:label "mutuallyExclusive" .


:DependencyKind.required uml:id "_D2ED798D-6450-412c-83C1-DB19C24F93B6" ;
                         rdfs:label "required" .


:DeploymentStateKind.inService uml:id "_A79605AE-1FDE-4ce6-B0A8-CC72C003E6B3" ;
                               rdfs:comment "Asset in service in deployment location." ;
                               rdfs:label "inService" .


:DeploymentStateKind.installed uml:id "_E60BF94D-CEDA-4c1c-AED5-5FD421354FCF" ;
                               rdfs:comment "Asset installed in deployment location." ;
                               rdfs:label "installed" .


:DeploymentStateKind.notYetInstalled uml:id "_627634B0-2A41-4a49-B2E4-CEA6841D0E4B" ;
                                     rdfs:comment "Asset not yet installed in deployment location." ;
                                     rdfs:label "notYetInstalled" .


:DeploymentStateKind.outOfService uml:id "_32292C31-E903-42d6-9DD2-82158F90753A" ;
                                  rdfs:comment "Asset out of service, but in deployment location." ;
                                  rdfs:label "outOfService" .


:DeploymentStateKind.removed uml:id "_E2BE4454-DDC6-4d4f-97EB-30C2232B82A4" ;
                             rdfs:comment "Asset removed from deployment location." ;
                             rdfs:label "removed" .


:DesignKind.asBuilt uml:id "_2B622818-B982-49e6-AFC0-21364C0F58E7" ;
                    rdfs:label "asBuilt" .


:DesignKind.estimated uml:id "_BC90302C-9240-4719-ADF4-C5EFC251C1C1" ;
                      rdfs:label "estimated" .


:DesignKind.other uml:id "_329D5311-29A2-41c8-9439-379E6847B7E8" ;
                  rdfs:label "other" .


:DispatchAcceptStatus.ACCEPT uml:id "_1071F454-0B01-4d88-B1A9-D4D4B53BDFC2" ;
                             rdfs:label "ACCEPT" .


:DispatchAcceptStatus.CANNOT uml:id "_9ED8C001-83F5-4ff1-96C4-905BDC3AF661" ;
                             rdfs:label "CANNOT" .


:DispatchAcceptStatus.DECLINE uml:id "_DA97D25B-DB8E-48ce-9EE0-458D3BE852C9" ;
                              rdfs:label "DECLINE" .


:DispatchAcceptStatus.NON_RESPONSE uml:id "_CE2988E2-7F9E-4178-A17C-D8AA14CEE3F8" ;
                                   rdfs:label "NON_RESPONSE" .


:DispatchAcceptStatus.OK uml:id "_DCABCC4E-140A-48f6-8807-8FC491B45A1A" ;
                         rdfs:label "OK" .


:DispatchAcceptStatus.PARTIAL uml:id "_3DF8C302-06D0-4474-B8D7-6C4991B3831C" ;
                              rdfs:label "PARTIAL" .


:DispatchResponseType.ACCEPT uml:id "_67686126-E2CB-4e48-992F-1EACB8CE3A75" ;
                             rdfs:label "ACCEPT" .


:DispatchResponseType.DECLINE uml:id "_EA86A318-3546-4df4-B0DC-0A93FCE89462" ;
                              rdfs:label "DECLINE" .


:DispatchResponseType.NON_RESPONSE uml:id "_D5478280-898C-42ae-B75E-C2076DCC0124" ;
                                   rdfs:label "NON_RESPONSE" .


:DispatchResponseType.PARTIAL uml:id "_22C3C156-2898-44fb-B72B-4386353EEC14" ;
                              rdfs:label "PARTIAL" .


:DispatchTransactionType.Purchase uml:id "_C43B78C4-4061-4a6d-8888-2256590E1C01" ;
                                  rdfs:label "Purchase" .


:DispatchTransactionType.Sale uml:id "_7102FB8C-5965-48b6-9EC9-2711603AD86C" ;
                              rdfs:label "Sale" .


:DobleStandardEditionKind.none uml:id "_D365D144-68E2-4fcf-B9A9-6E50739DE4A2" ;
                               rdfs:comment "No edition." ;
                               rdfs:label "none" .


:DobleStandardEditionKind.unknown uml:id "_FBBC3B95-21AB-4897-93C0-4C27835E6A8D" ;
                                  rdfs:comment "Unknown edition." ;
                                  rdfs:label "unknown" .


:DobleStandardKind.methanol uml:id "_3E9C24E8-2A00-4e7f-ADE6-1F119F7F4A07" ;
                            rdfs:comment "Doble test for methanol." ;
                            rdfs:label "methanol" .


:DroopSignalFeedbackKind.electricalPower uml:id "_BC2A261C-5068-4631-B279-99A4F9E0BB68" ;
                                         rdfs:comment "Electrical power feedback (connection indicated as 1 in the block diagrams of models, e.g. GovCT1, GovCT2)." ;
                                         rdfs:label "electricalPower" .


:DroopSignalFeedbackKind.fuelValveStroke uml:id "_D95E8F20-CE3E-40bd-A1E2-840A5BCE31D5" ;
                                         rdfs:comment "Fuel valve stroke feedback (true stroke) (connection indicated as 2 in the block diagrams of model, e.g. GovCT1, GovCT2)." ;
                                         rdfs:label "fuelValveStroke" .


:DroopSignalFeedbackKind.governorOutput uml:id "_42BC2DD8-FD94-4cc6-AC91-F6F216D77A1F" ;
                                        rdfs:comment "Governor output feedback (requested stroke) (connection indicated as 3 in the block diagrams of models, e.g. GovCT1, GovCT2)." ;
                                        rdfs:label "governorOutput" .


:DroopSignalFeedbackKind.none uml:id "_C7116843-752E-4c73-B359-E75742ADE854" ;
                              rdfs:comment "No droop signal feedback, is isochronous governor." ;
                              rdfs:label "none" .


:EPAStandardEditionKind.A uml:id "_67A8D173-9DFA-4895-8C3C-8DE4202932F3" ;
                          rdfs:comment "Standard edition A." ;
                          rdfs:label "A" .


:EPAStandardEditionKind.none uml:id "_9A744E76-F1D4-492a-924D-E49949AA73B7" ;
                             rdfs:comment "No standard edition." ;
                             rdfs:label "none" .


:EPAStandardEditionKind.unknown uml:id "_58A8B8ED-677E-4239-81D5-EC62223BCF1A" ;
                                rdfs:comment "Unknown standard edition." ;
                                rdfs:label "unknown" .


:EPAStandardKind._8082 uml:id "_E0F67E32-9C8F-4ee5-8EB7-5293B70F3D65" ;
                       rdfs:comment "Polychlorinated Biphenyls (PCBs) by Gas Chromatography." ;
                       rdfs:label "8082" .


:ERTConfidenceKind.high uml:id "_EC986F30-302E-4878-9F23-CBC5B06D5726" ;
                        rdfs:comment "there is a high confidence that the ERT will be accomplished" ;
                        rdfs:label "high" .


:ERTConfidenceKind.low uml:id "_0BB19AB3-97BF-4e32-B6D0-088799866080" ;
                       rdfs:comment "there is a low confidence that the ERT will be accomplished." ;
                       rdfs:label "low" .


:EmissionType.carbonDioxide uml:id "_3A38B1C7-DD00-48b8-944B-489B28AC27A3" ;
                            rdfs:comment "Carbon dioxide." ;
                            rdfs:label "carbonDioxide" .


:EmissionType.carbonDisulfide uml:id "_27FBACE6-1691-47bb-8EED-0F36BB97B019" ;
                              rdfs:comment "Carbon disulfide." ;
                              rdfs:label "carbonDisulfide" .


:EmissionType.chlorine uml:id "_30F01FEF-25A6-4ed2-88C2-1B946BE9F667" ;
                       rdfs:comment "Chlorine." ;
                       rdfs:label "chlorine" .


:EmissionType.hydrogenSulfide uml:id "_54FAC8F0-49CD-4fe0-9AE2-404E630ED5FD" ;
                              rdfs:comment "Hydrogen sulfide." ;
                              rdfs:label "hydrogenSulfide" .


:EmissionType.nitrogenOxide uml:id "_65B3C938-9474-4876-A9C2-0EFC9A4E5E30" ;
                            rdfs:comment "Nitrogen oxide." ;
                            rdfs:label "nitrogenOxide" .


:EmissionType.sulfurDioxide uml:id "_330E0354-FC40-4a19-B79C-9476E052537E" ;
                            rdfs:comment "Sulfur dioxide." ;
                            rdfs:label "sulfurDioxide" .


:EmissionValueSource.calculated uml:id "_5C476043-4FEB-4865-AE0B-0A957DCBE044" ;
                                rdfs:comment "Calculated." ;
                                rdfs:label "calculated" .


:EmissionValueSource.measured uml:id "_4E6AD84B-AD5A-4788-A299-9BBF0EBDC6A7" ;
                              rdfs:comment "Measured." ;
                              rdfs:label "measured" .


:EndDeviceFunctionKind.autonomousDst uml:id "_89185290-3ABB-4929-8102-E26E02AB7A97" ;
                                     rdfs:comment "Autonomous application of daylight saving time (DST)." ;
                                     rdfs:label "autonomousDst" .


:EndDeviceFunctionKind.demandResponse uml:id "_25940B91-4EDC-44bc-8BF2-7D2FFC0C27B8" ;
                                      rdfs:comment "Demand response functions." ;
                                      rdfs:label "demandResponse" .


:EndDeviceFunctionKind.electricMetering uml:id "_C2C830B2-6688-4e2c-B8A9-C19699937ABF" ;
                                        rdfs:comment "Electricity metering." ;
                                        rdfs:label "electricMetering" .


:EndDeviceFunctionKind.gasMetering uml:id "_DD6A2F15-32F6-4cd2-8344-0B68A6B133EA" ;
                                   rdfs:comment "Gas metering." ;
                                   rdfs:label "gasMetering" .


:EndDeviceFunctionKind.metrology uml:id "_60C7E244-4C14-427d-9884-EB81E742B371" ;
                                 rdfs:comment "Presentation of metered values to a user or another system (always a function of a meter, but might not be supported by a load control unit)." ;
                                 rdfs:label "metrology" .


:EndDeviceFunctionKind.onRequestRead uml:id "_AA742E86-0366-4fcf-BE07-BE973FEF0BE5" ;
                                     rdfs:comment "On-request reads." ;
                                     rdfs:label "onRequestRead" .


:EndDeviceFunctionKind.outageHistory uml:id "_00A999B1-5594-478d-ABC7-24D20AB7E033" ;
                                     rdfs:comment "Reporting historical power interruption data." ;
                                     rdfs:label "outageHistory" .


:EndDeviceFunctionKind.relaysProgramming uml:id "_E60E6DF7-0E1F-49b2-A219-47FA09233379" ;
                                         rdfs:comment "Support for one or more relays that may be programmable in the meter (and tied to TOU, time pulse, load control or other functions)." ;
                                         rdfs:label "relaysProgramming" .


:EndDeviceFunctionKind.reverseFlow uml:id "_51C01548-842F-4d92-BB5F-52B46F3EE8C8" ;
                                   rdfs:comment "Detection and monitoring of reverse flow." ;
                                   rdfs:label "reverseFlow" .


:EndDeviceFunctionKind.waterMetering uml:id "_1B2B3A3D-8041-4f2b-A538-B4A70F159225" ;
                                     rdfs:comment "Water metering." ;
                                     rdfs:label "waterMetering" .


:EnergyPriceIndexType.BOTH uml:id "_618E030E-C1A4-4530-8E4D-9BFE7EC5D57A" ;
                           rdfs:label "BOTH" .


:EnergyPriceIndexType.RETAIL uml:id "_04CA382D-1E55-4380-8F9A-31CB848598FD" ;
                             rdfs:label "RETAIL" .


:EnergyPriceIndexType.WHOLESALE uml:id "_75DCBF8C-F60E-4697-B615-B7C2C45AC719" ;
                                rdfs:label "WHOLESALE" .


:EnergyProductType.DYN uml:id "_7BC0044E-A62D-44ff-844C-0D9F2DC1884A" ;
                       rdfs:comment "Dynamic" ;
                       rdfs:label "DYN" .


:EnergyProductType.FIRM uml:id "_8D6A544A-51D7-4584-9EBE-3F40BBA0BF20" ;
                        rdfs:comment "Firm" ;
                        rdfs:label "FIRM" .


:EnergyProductType.NFRM uml:id "_8F523AF2-46C9-48a8-8E7E-9EB445DCD33B" ;
                        rdfs:comment "Non Firm" ;
                        rdfs:label "NFRM" .


:EnergyProductType.WHL uml:id "_90FE3401-1EE9-4225-8ECB-7B88274A5909" ;
                       rdfs:comment "Wheeling" ;
                       rdfs:label "WHL" .


:EnergyTransactionType.approve uml:id "_6B8894C2-9131-4213-9F82-0DA151E04186" ;
                               rdfs:comment "Approve" ;
                               rdfs:label "approve" .


:EnergyTransactionType.deny uml:id "_C8F7969E-94CA-4313-BDAA-43869A7423AB" ;
                            rdfs:comment "Deny" ;
                            rdfs:label "deny" .


:EnergyTransactionType.study uml:id "_9F4ED503-4E1A-460f-A703-B8BC65EE6442" ;
                             rdfs:comment "Study" ;
                             rdfs:label "study" .


:EnergyTypeCode.DABE uml:id "_C792829A-AE02-47e1-A4A5-00EC8BCE821B" ;
                     rdfs:label "DABE" .


:EnergyTypeCode.DAPE uml:id "_97F745E6-475A-4128-84AA-85D11545A674" ;
                     rdfs:label "DAPE" .


:EnergyTypeCode.DASE uml:id "_88B3625D-E11C-4243-BFC6-3FE04C72FD07" ;
                     rdfs:label "DASE" .


:EnergyTypeCode.DMLE uml:id "_C4ABC213-ECA2-4819-8A8C-73C33753C1DE" ;
                     rdfs:label "DMLE" .


:EnergyTypeCode.DSSE uml:id "_1862577C-AD95-49a4-95D5-5D018074D69C" ;
                     rdfs:label "DSSE" .


:EnergyTypeCode.EDE uml:id "_E3EC007B-D3A2-4122-BAF1-7B791D68754F" ;
                    rdfs:label "EDE" .


:EnergyTypeCode.HASE uml:id "_C76DBEF3-62B6-4aa3-8E65-709E6CB9858C" ;
                     rdfs:label "HASE" .


:EnergyTypeCode.MLE uml:id "_D6E89F06-1109-41ad-A757-0363AE434A4F" ;
                    rdfs:label "MLE" .


:EnergyTypeCode.MSSLFE uml:id "_586DF6CD-66D9-4a24-BF47-DE2B5AE6207B" ;
                       rdfs:label "MSSLFE" .


:EnergyTypeCode.OE uml:id "_9B4358B1-8259-450b-B00C-968DD9B5EB77" ;
                   rdfs:label "OE" .


:EnergyTypeCode.PE uml:id "_A1B265AD-541E-43a2-9AF0-9A299C96B40E" ;
                   rdfs:label "PE" .


:EnergyTypeCode.RE uml:id "_F53BC610-F2BF-4dba-9C0E-6AAB82116117" ;
                   rdfs:label "RE" .


:EnergyTypeCode.RED uml:id "_D7287F00-9152-4adf-822E-24EA8AC00AF7" ;
                    rdfs:label "RED" .


:EnergyTypeCode.RMRE uml:id "_B67535FF-EF13-45c3-B5BA-28C73729F957" ;
                     rdfs:label "RMRE" .


:EnergyTypeCode.RTSSE uml:id "_C2E46EA1-53E5-4f57-8D55-53CD7E31F5BE" ;
                      rdfs:label "RTSSE" .


:EnergyTypeCode.SE uml:id "_4AE02265-C422-4ffc-918B-7C36A5E88292" ;
                   rdfs:label "SE" .


:EnergyTypeCode.SRE uml:id "_A6812534-0C0A-4285-A6F7-9BD76D7B76DA" ;
                    rdfs:label "SRE" .


:EnergyTypeCode.TEE uml:id "_D2C7FCE1-3505-4f64-9CDB-BDBC3A993D8A" ;
                    rdfs:label "TEE" .


:EnergyTypeKind.ConsumerLoad uml:id "_C738867D-4693-4286-867F-861FB8A30460" ;
                             rdfs:label "ConsumerLoad" .


:EnergyTypeKind.IndustrialLoad uml:id "_77AF1E70-4145-483e-98E0-429E85846C6B" ;
                               rdfs:label "IndustrialLoad" .


:EnergyTypeKind.Other uml:id "_EAC4E5FD-FC38-4a11-A1DA-22A3A0A4BCF7" ;
                      rdfs:label "Other" .


:EnergyTypeKind.PVpark uml:id "_81C32E01-A018-4946-A7F3-545FEFFBF0F4" ;
                       rdfs:label "PVpark" .


:EnergyTypeKind.WindPark uml:id "_BDD60AA4-3664-4745-BA20-A78CCEA7468E" ;
                         rdfs:label "WindPark" .


:EnvironmentalDiscreteKind.cloudCover uml:id "_48420231-0ED9-4eb4-9044-A51AB391ED3D" ;
                                      rdfs:comment "Cloud cover in octa." ;
                                      rdfs:label "cloudCover" .


:EquipmentStatusType.In uml:id "_F63F1D22-FFE2-493c-8807-DC4EA4CD0ADF" ;
                        rdfs:comment "Equipment is in." ;
                        rdfs:label "In" .


:EquipmentStatusType.Out uml:id "_CB939500-A150-4e40-BC2C-190E8E2EBF54" ;
                         rdfs:comment "Equipment is out." ;
                         rdfs:label "Out" .


:ErpAccountKind.estimate uml:id "_F7DBB07C-4DE9-4f10-B3E2-DBD2C78895C3" ;
                         rdfs:label "estimate" .


:ErpAccountKind.normal uml:id "_F773052E-96B2-4a76-93D3-222ABD43D867" ;
                       rdfs:label "normal" .


:ErpAccountKind.reversal uml:id "_F0F3E268-6254-4cd0-93C9-D186D8E5923D" ;
                         rdfs:label "reversal" .


:ErpAccountKind.statistical uml:id "_A5534DDC-9263-420d-82CC-8BEE9CF14909" ;
                            rdfs:label "statistical" .


:ErpInvoiceKind.purchase uml:id "_67D7AA0A-0221-444d-8A06-2C572A5F3EB1" ;
                         rdfs:label "purchase" .


:ErpInvoiceKind.sale uml:id "_84878F2E-3F1D-49e6-A5DA-B7C05A9AD640" ;
                     rdfs:label "sale" .


:ErpInvoiceLineItemKind.initial uml:id "_BC996AFA-AAB6-4931-9DD8-EA8849CCB8D0" ;
                                rdfs:label "initial" .


:ErpInvoiceLineItemKind.other uml:id "_0D84BC3E-6F30-424c-A8D2-B043C293F118" ;
                              rdfs:label "other" .


:ErpInvoiceLineItemKind.recalculation uml:id "_06E8B37B-10EE-44e6-828F-5B1A80D5CB28" ;
                                      rdfs:label "recalculation" .


:ExcIEEEST1AUELselectorKind.ignoreUELsignal uml:id "_559092A6-4A5E-4770-8565-FF15421513CC" ;
                                            rdfs:comment "Ignore UEL signal." ;
                                            rdfs:label "ignoreUELsignal" .


:ExcIEEEST1AUELselectorKind.inputAddedToErrorSignal uml:id "_0167BCCC-21F3-4f5d-8DD7-0F3121597F8F" ;
                                                    rdfs:comment "UEL input added to error signal." ;
                                                    rdfs:label "inputAddedToErrorSignal" .


:ExcIEEEST1AUELselectorKind.inputHVgateErrorSignal uml:id "_DF248D9F-D976-4c79-A740-E1AB4C2EE954" ;
                                                   rdfs:comment "UEL input HV gate with error signal." ;
                                                   rdfs:label "inputHVgateErrorSignal" .


:ExcIEEEST1AUELselectorKind.inputHVgateVoltageOutput uml:id "_87F6AC0B-8BAE-4846-A7D3-88449AE441F2" ;
                                                     rdfs:comment "UEL input HV gate with voltage regulator output." ;
                                                     rdfs:label "inputHVgateVoltageOutput" .


:ExcREXSFeedbackSignalKind.fieldCurrent uml:id "_20B5EA6E-9205-4b2a-A9D2-D87DE23F2E91" ;
                                        rdfs:comment "The exciter field current is used." ;
                                        rdfs:label "fieldCurrent" .


:ExcREXSFeedbackSignalKind.fieldVoltage uml:id "_F1321EE5-BA25-4ff0-8170-9C6BB353C6B8" ;
                                        rdfs:comment "The voltage regulator output voltage is used. It is the same as exciter field voltage." ;
                                        rdfs:label "fieldVoltage" .


:ExcREXSFeedbackSignalKind.outputVoltage uml:id "_77C43C4E-60C1-448f-88C2-F3C339747521" ;
                                         rdfs:comment "The output voltage of the exciter is used." ;
                                         rdfs:label "outputVoltage" .


:ExcST6BOELselectorKind.afterUEL uml:id "_9E3FE06F-CA3A-4170-A559-6586DF11FF44" ;
                                 rdfs:comment "The connection is after UEL. Corresponds to <i>OELin</i> = 2 on the ExcST6B diagram." ;
                                 rdfs:label "afterUEL" .


:ExcST6BOELselectorKind.beforeUEL uml:id "_26C343DF-DEE4-4c49-B64A-FE4704AE4C7D" ;
                                  rdfs:comment "The connection is before UEL. Corresponds to <i>OELin</i> = 1 on the ExcST6B diagram." ;
                                  rdfs:label "beforeUEL" .


:ExcST6BOELselectorKind.noOELinput uml:id "_123C25C6-1786-4cfb-826D-F45069298025" ;
                                   rdfs:comment "No OEL input is used. Corresponds to <i>OELin</i> not = 1 and not = 2 on the ExcST6B diagram. Original ExcST6B model would have called this <i>OELin</i> = 0." ;
                                   rdfs:label "noOELinput" .


:ExcST7BOELselectorKind.addVref uml:id "_C4866047-697D-477a-B572-C858FE0C3477" ;
                                rdfs:comment "The signal is added to <i>Vref</i>.  Corresponds to <i>OELin</i> = 1 on the ExcST7B diagram." ;
                                rdfs:label "addVref" .


:ExcST7BOELselectorKind.inputLVgate uml:id "_6F4F940D-1730-4555-B3DE-0843F9A6A8B0" ;
                                    rdfs:comment "The signal is connected into the input <i>LVGate</i>. Corresponds to <i>OELin</i> = 2 on the ExcST7B diagram." ;
                                    rdfs:label "inputLVgate" .


:ExcST7BOELselectorKind.noOELinput uml:id "_2BC3480F-7146-4a72-89B7-1E72D021533C" ;
                                   rdfs:comment "No OEL input is used. Corresponds to <i>OELin</i> not = 1 and not = 2 and not = 3 on the ExcST7B diagram. Original ExcST7B model would have called this <i>OELin</i> = 0." ;
                                   rdfs:label "noOELinput" .


:ExcST7BOELselectorKind.outputLVgate uml:id "_1A8BEBCF-ABA1-4dd7-87B2-32FB6C469A00" ;
                                     rdfs:comment "The signal is connected into the output <i>LVGate</i>.  Corresponds to <i>OELin</i> = 3 on the ExcST7B diagram." ;
                                     rdfs:label "outputLVgate" .


:ExcST7BUELselectorKind.addVref uml:id "_484B9178-2FF5-40c7-BC72-98F0BCB06A29" ;
                                rdfs:comment "The signal is added to <i>Vref</i>. Corresponds to <i>UELin</i> = 1 on the ExcST7B diagram." ;
                                rdfs:label "addVref" .


:ExcST7BUELselectorKind.inputHVgate uml:id "_0601B4EF-4E06-49ec-BEBC-5991132231E6" ;
                                    rdfs:comment "The signal is connected into the input <i>HVGate</i>.  Corresponds to <i>UELin</i> = 2 on the ExcST7B diagram." ;
                                    rdfs:label "inputHVgate" .


:ExcST7BUELselectorKind.noUELinput uml:id "_17EC1C75-1ECE-4bdc-BD5D-453C0626C03B" ;
                                   rdfs:comment "No UEL input is used.  Corresponds to <i>UELin</i> not = 1 and not = 2 and not = 3 on the ExcST7B diagram. Original ExcST7B model would have called this <i>UELin</i> = 0." ;
                                   rdfs:label "noUELinput" .


:ExcST7BUELselectorKind.outputHVgate uml:id "_E69D40DF-4CDF-486f-A4F8-D323F2D87DA1" ;
                                     rdfs:comment "The signal is connected into the output <i>HVGate</i>.  Corresponds to <i>UELin</i> = 3 on the ExcST7B diagram." ;
                                     rdfs:label "outputHVgate" .


:ExecutionType.DA uml:id "_2A9F2715-E924-435d-9E7D-B9108E9BDF0D" ;
                  rdfs:comment "Day Ahead" ;
                  rdfs:label "DA" .


:ExecutionType.HASP uml:id "_9630866A-2872-4844-AA17-37D76DB6E5EF" ;
                    rdfs:comment "Real TIme Hour Ahead Execution" ;
                    rdfs:label "HASP" .


:ExecutionType.RTD uml:id "_2FE092F5-B88F-4dd6-9A74-B3E7D32F3DB2" ;
                   rdfs:comment "Real Time Dispatch" ;
                   rdfs:label "RTD" .


:ExecutionType.RTPD uml:id "_113E94E7-BAFB-4e2d-8109-F30C718FAF31" ;
                    rdfs:comment "Real Time Pre-dispatch" ;
                    rdfs:label "RTPD" .


:FACTSDeviceKind.statcom uml:id "_A81C68C3-49E6-4f08-836A-FF6BAF663CC7" ;
                         rdfs:comment "Static synchronous compensator." ;
                         rdfs:label "statcom" .


:FACTSDeviceKind.svc uml:id "_0BD922B5-5E5C-4255-AB32-8888C7508ECE" ;
                     rdfs:comment "Static VAr compensator." ;
                     rdfs:label "svc" .


:FACTSDeviceKind.tcpar uml:id "_04BF8754-86EE-448f-9121-6CF8BC1CBFE6" ;
                       rdfs:comment "Thyristor-controlled phase-angle regulator." ;
                       rdfs:label "tcpar" .


:FACTSDeviceKind.tcsc uml:id "_5475CE0E-2D5F-479c-9B1A-82FDE57C0605" ;
                      rdfs:comment "Thyristor-controlled series capacitor." ;
                      rdfs:label "tcsc" .


:FACTSDeviceKind.tcvl uml:id "_FC54D9A2-BE08-48d9-BA43-AAD8D0EA9030" ;
                      rdfs:comment "Thyristor-controlled voltage limiter." ;
                      rdfs:label "tcvl" .


:FACTSDeviceKind.tsbr uml:id "_6AE5268E-0487-43be-8AED-0A5C2C6BF983" ;
                      rdfs:comment "Thyristor-switched braking resistor." ;
                      rdfs:label "tsbr" .


:FACTSDeviceKind.tssc uml:id "_08BE63AA-8E2B-4f50-9CC9-BA99533F2FAE" ;
                      rdfs:comment "Thyristor-switched series capacitor." ;
                      rdfs:label "tssc" .


:FACTSDeviceKind.upfc uml:id "_7DE813CF-898B-4174-9815-0E55C6B4DB01" ;
                      rdfs:comment "Unified power flow controller." ;
                      rdfs:label "upfc" .


:FScale.five uml:id "_B6CE21C4-206F-4ffb-B4A8-2B8F4EF1D9D6" ;
             rdfs:comment "Over 200 mph 3-second gust." ;
             rdfs:label "five" .


:FScale.four uml:id "_9F2C3F06-566E-48e4-81BE-E96C4B13ED05" ;
             rdfs:comment "166-200 mph 3-second gust." ;
             rdfs:label "four" .


:FScale.minusNine uml:id "_C58CB0C9-8DDC-4fe0-96F8-6F637C6A20BF" ;
                  rdfs:comment "Unknown." ;
                  rdfs:label "minusNine" .


:FScale.one uml:id "_41738BD9-42E6-4fdd-BE91-4269D53B29C9" ;
            rdfs:comment "86-110 mph 3-second gust." ;
            rdfs:label "one" .


:FScale.three uml:id "_EF5CCCFB-0DBB-4951-87C6-902DA6D7CB14" ;
              rdfs:comment "136-165 mph 3-second gust." ;
              rdfs:label "three" .


:FScale.two uml:id "_A43B85BA-B8A0-42e2-9744-36B1B6FDD07D" ;
            rdfs:comment "111-135 mph 3-second gust." ;
            rdfs:label "two" .


:FScale.zero uml:id "_2DA63F9D-7EF4-414d-8D2E-54618ADBB66B" ;
             rdfs:comment "65-85 mph 3-second gust." ;
             rdfs:label "zero" .


:FacilityKind.distributionPoleTop uml:id "_1B8A8E2A-5F92-47a3-BEF8-81132D38388C" ;
                                  rdfs:comment "Distribution pole top." ;
                                  rdfs:label "distributionPoleTop" .


:FacilityKind.substationDistribution uml:id "_E7CE089E-70FC-4778-B994-867E827EEA8F" ;
                                     rdfs:comment "Distribution substation." ;
                                     rdfs:label "substationDistribution" .


:FacilityKind.substationFossilPlant uml:id "_DA3FF0DC-3997-4461-AFBB-68237F433F0A" ;
                                    rdfs:comment "Fossil plant substation." ;
                                    rdfs:label "substationFossilPlant" .


:FacilityKind.substationHydroPlant uml:id "_F35BF7D4-D8BE-4ea4-9745-CA88394227EE" ;
                                   rdfs:comment "Hydro plant substation." ;
                                   rdfs:label "substationHydroPlant" .


:FacilityKind.substationNuclearPlant uml:id "_D2879425-A999-4912-B276-05D7C4F90E05" ;
                                     rdfs:comment "Nuclear plant substation." ;
                                     rdfs:label "substationNuclearPlant" .


:FacilityKind.substationSubTransmission uml:id "_6DE7DE36-4555-43b5-ABD9-884BD1C6BDE2" ;
                                        rdfs:comment "Subtransmission substation." ;
                                        rdfs:label "substationSubTransmission" .


:FacilityKind.substationTransmission uml:id "_55457CBB-825F-4f25-BFCE-DD75B54E19F6" ;
                                     rdfs:comment "Transmission substation." ;
                                     rdfs:label "substationTransmission" .


:FailureIsolationMethodKind.breakerOperation uml:id "_06661926-D180-416c-8D65-A1612577FA6B" ;
                                             rdfs:comment "Isolated via breaker operation." ;
                                             rdfs:label "breakerOperation" .


:FailureIsolationMethodKind.burnedInTheClear uml:id "_EECE93A8-ED38-44c3-AEE1-7165D32AC3BD" ;
                                             rdfs:comment "Isolated by equipment burning in the clear." ;
                                             rdfs:label "burnedInTheClear" .


:FailureIsolationMethodKind.fuse uml:id "_3D29DEE3-27DA-4064-8632-38C72564C562" ;
                                 rdfs:comment "Isolated by fuse." ;
                                 rdfs:label "fuse" .


:FailureIsolationMethodKind.manuallyIsolated uml:id "_270BD360-091B-4ab5-9303-2618A17F3CEC" ;
                                             rdfs:comment "Isolated by manual operation." ;
                                             rdfs:label "manuallyIsolated" .


:FailureIsolationMethodKind.other uml:id "_1EC7CF42-99C2-4d26-AC5C-F12D161DDFC3" ;
                                  rdfs:comment "Isolated by other action." ;
                                  rdfs:label "other" .


:FaultIndicatorResetKind.automatic uml:id "_3911F5AE-C79B-4de1-AD6E-1CEE19755DB1" ;
                                   rdfs:label "automatic" .


:FaultIndicatorResetKind.manual uml:id "_80A7AB2F-D6AF-4b99-A25F-29E605FF7E45" ;
                                rdfs:label "manual" .


:FaultIndicatorResetKind.other uml:id "_4060BA6B-AE6A-4e6e-9118-6D9E21463ACD" ;
                               rdfs:label "other" .


:FaultIndicatorResetKind.remote uml:id "_C290C62F-E51E-4fad-A010-02399EB8839B" ;
                                rdfs:label "remote" .


:FlagTypeRMR.N uml:id "_C4A525C9-E823-4cf1-8C55-ADDEC1D7E0A5" ;
               rdfs:comment "'N' - not an RMR unit" ;
               rdfs:label "N" .


:FlagTypeRMR._1 uml:id "_47FF9B69-84E9-4365-858C-5E4736558216" ;
                rdfs:comment "'1' - RMR Condition 1 unit" ;
                rdfs:label "1" .


:FlagTypeRMR._2 uml:id "_AEF47561-C2FB-49fd-BD1A-4835A0FEDAA8" ;
                rdfs:comment "'2' - RMR Condition 2 unit" ;
                rdfs:label "2" .


:FlowDirectionKind.forward uml:hasInitialValue "1" ;
                           uml:id "_CD793FD7-51EF-410b-8F30-123CD3F6E989" ;
                           rdfs:comment """\"Delivered,\" or \"Imported\" as defined 61968-2.
Forward Active Energy is a positive kWh value as one would naturally expect to find as energy is supplied by the utility and consumed at the service.
Forward Reactive Energy is a positive VArh value as one would naturally expect to find in the presence of inductive loading.
In polyphase metering, the forward energy register is incremented when the sum of the phase energies is greater than zero:
<img src=\"HTS_1.PNG\" width=\"209\" height=\"16\" border=\"0\" alt=\"graphic\"/>""" ;
                           rdfs:label "forward" .


:FlowDirectionKind.lagging uml:hasInitialValue "2" ;
                           uml:id "_94EA88FF-0299-48cf-90F3-074DFF34EC23" ;
                           rdfs:comment """Typically used to describe that a power factor is lagging the reference value. 
Note 1: When used to describe VA, “lagging” describes a form of measurement where reactive power is considered in all four quadrants, but real power is considered only in quadrants I and IV.
Note 2: When used to describe power factor, the term “Lagging” implies that the PF is negative. The term “lagging” in this case takes the place of the negative sign. If a signed PF value is to be passed by the data producer, then the direction of flow enumeration zero (none) should be used in order to avoid the possibility of creating an expression that employs a double negative. The data consumer should be able to tell from the sign of the data if the PF is leading or lagging. This principle is analogous to the concept that “Reverse” energy is an implied negative value, and to publish a negative reverse value would be ambiguous.
Note 3: Lagging power factors typically indicate inductive loading.""" ;
                           rdfs:label "lagging" .


:FlowDirectionKind.leading uml:hasInitialValue "3" ;
                           uml:id "_E34D26B3-6DE2-4cd4-BD6E-30221A5D516B" ;
                           rdfs:comment """Typically used to describe that a power factor is leading the reference value.
Note: Leading power factors typically indicate capacitive loading.""" ;
                           rdfs:label "leading" .


:FlowDirectionKind.net uml:hasInitialValue "4" ;
                       uml:id "_710A918A-8F9B-45c6-B0CE-114D2743954E" ;
                       rdfs:comment """|Forward| - |Reverse|, See 61968-2.

Note: In some systems, the value passed as a “net” value could become negative. In other systems the value passed as a “net” value is always a positive number, and rolls-over and rolls-under as needed.""" ;
                       rdfs:label "net" .


:FlowDirectionKind.none uml:hasInitialValue "0" ;
                        uml:id "_FFA0B12F-050B-4ba8-A9B5-B4B6332A8EC8" ;
                        rdfs:comment "Not Applicable (N/A)" ;
                        rdfs:label "none" .


:FlowDirectionKind.q1minusQ4 uml:hasInitialValue "9" ;
                             uml:id "_0BE7A9F1-B563-4d5c-82FC-08121925B92D" ;
                             rdfs:comment "Q1 minus Q4" ;
                             rdfs:label "q1minusQ4" .


:FlowDirectionKind.q1plusQ2 uml:hasInitialValue "5" ;
                            uml:id "_B3C84D0D-C497-4798-8FEF-E8D15AF898F3" ;
                            rdfs:comment "Reactive positive quadrants. (The term “lagging” is preferred.)" ;
                            rdfs:label "q1plusQ2" .


:FlowDirectionKind.q1plusQ3 uml:hasInitialValue "7" ;
                            uml:id "_7276E72B-3337-4d25-921B-5AD2AC7C97F5" ;
                            rdfs:comment "Quadrants 1 and 3" ;
                            rdfs:label "q1plusQ3" .


:FlowDirectionKind.q1plusQ4 uml:hasInitialValue "8" ;
                            uml:id "_0F22200A-A507-4c74-A7C2-AF654813DD1C" ;
                            rdfs:comment "Quadrants 1 and 4 usually represent forward active energy" ;
                            rdfs:label "q1plusQ4" .


:FlowDirectionKind.q2minusQ3 uml:hasInitialValue "12" ;
                             uml:id "_A81A05BE-5DED-47e0-B3ED-D7D4C742691F" ;
                             rdfs:comment "Q2 minus Q3" ;
                             rdfs:label "q2minusQ3" .


:FlowDirectionKind.q2plusQ3 uml:hasInitialValue "10" ;
                            uml:id "_F53D76DF-03AF-41b7-8CEC-94F6BD6AD694" ;
                            rdfs:comment "Quadrants 2 and 3 usually represent reverse active energy" ;
                            rdfs:label "q2plusQ3" .


:FlowDirectionKind.q2plusQ4 uml:hasInitialValue "11" ;
                            uml:id "_995C631E-A068-447c-85F5-A6F0D3B57664" ;
                            rdfs:comment "Quadrants 2 and 4" ;
                            rdfs:label "q2plusQ4" .


:FlowDirectionKind.q3minusQ2 uml:hasInitialValue "14" ;
                             uml:id "_CB577B09-2DFF-49c7-9A45-833EE066E945" ;
                             rdfs:comment "Q3 minus Q2" ;
                             rdfs:label "q3minusQ2" .


:FlowDirectionKind.q3plusQ4 uml:hasInitialValue "13" ;
                            uml:id "_E8172E8F-3A81-4389-831F-5F470E201FAC" ;
                            rdfs:comment "Reactive negative quadrants. (The term “leading” is preferred.)" ;
                            rdfs:label "q3plusQ4" .


:FlowDirectionKind.quadrant1 uml:hasInitialValue "15" ;
                             uml:id "_37C6835D-D3A8-411c-90D3-35A3A32720F8" ;
                             rdfs:comment "Q1 only" ;
                             rdfs:label "quadrant1" .


:FlowDirectionKind.quadrant2 uml:hasInitialValue "16" ;
                             uml:id "_97D06D32-09EB-47a3-B003-E384C2763045" ;
                             rdfs:comment "Q2 only" ;
                             rdfs:label "quadrant2" .


:FlowDirectionKind.quadrant3 uml:hasInitialValue "17" ;
                             uml:id "_ACA00D9F-02DA-4bb0-94D7-63623EBB865E" ;
                             rdfs:comment "Q3 only" ;
                             rdfs:label "quadrant3" .


:FlowDirectionKind.quadrant4 uml:hasInitialValue "18" ;
                             uml:id "_8D2ECAE0-6EBD-4b5c-84F3-02960D9DEDC0" ;
                             rdfs:comment "Q4 only" ;
                             rdfs:label "quadrant4" .


:FlowDirectionKind.reverse uml:hasInitialValue "19" ;
                           uml:id "_7234A8E8-7C70-44d4-A497-95D2E2A7A293" ;
                           rdfs:comment """Reverse Active Energy is equivalent to \"Received,\" or \"Exported\" as defined in 61968-2.
Reverse Active Energy is a positive kWh value as one would expect to find when energy is backfed by the service onto the utility network.
Reverse Reactive Energy is a positive VArh value as one would expect to find in the presence of capacitive loading and a leading Power Factor.
In polyphase metering, the reverse energy register is incremented when the sum of the phase energies is less than zero:
<img src=\"HTS_1.PNG\" width=\"209\" height=\"16\" border=\"0\" alt=\"graphic\"/>
Note: The value passed as a reverse value is always a positive value. It is understood by the label “reverse” that it represents negative flow.""" ;
                           rdfs:label "reverse" .


:FlowDirectionKind.total uml:hasInitialValue "20" ;
                         uml:id "_DA938311-D058-496b-A6D2-5686F4D52512" ;
                         rdfs:comment """|Forward| + |Reverse|, See 61968-2.
The sum of the commodity in all quadrants Q1+Q2+Q3+Q4.
In polyphase metering, the total energy register is incremented when the absolute value of the sum of the phase energies is greater than zero:
<img src=\"HTS_1.PNG\" width=\"217\" height=\"16\" border=\"0\" alt=\"graphic\"/>""" ;
                         rdfs:label "total" .


:FlowDirectionKind.totalByPhase uml:hasInitialValue "21" ;
                                uml:id "_03FEC082-6E82-40bb-BD2B-5E881A9153B6" ;
                                rdfs:comment """In polyphase metering, the total by phase energy register is incremented when the sum of the absolute values of the phase energies is greater than zero:
<img src=\"HTS_1.PNG\" width=\"234\" height=\"16\" border=\"0\" alt=\"graphic\"/>
In single phase metering, the formulas for “Total” and “Total by phase” collapse to the same expression. For communication purposes however, the “Total” enumeration should be used with single phase meter data.""" ;
                                rdfs:label "totalByPhase" .


:FlowDirectionType.Forward uml:id "_3710B80E-1200-4491-B0C2-7151A873E74B" ;
                           rdfs:comment "Forward direction." ;
                           rdfs:label "Forward" .


:FlowDirectionType.Reverse uml:id "_B472A601-A911-49e5-B001-78A407B4B74A" ;
                           rdfs:comment "Reverse direction." ;
                           rdfs:label "Reverse" .


:FrancisGovernorControlKind.electromechanicalElectrohydraulic uml:id "_A6361EFE-054B-4ad3-96BC-A12067766DB7" ;
                                                              rdfs:comment "Electromechanical and electrohydraulic regulator (Cflag=3)." ;
                                                              rdfs:label "electromechanicalElectrohydraulic" .


:FrancisGovernorControlKind.mechanicHydraulicTransientFeedback uml:id "_F8F54CFB-B7B4-4889-9A34-B9D25BFEABE6" ;
                                                               rdfs:comment "Mechanic-hydraulic regulator with transient feedback (Cflag=2)." ;
                                                               rdfs:label "mechanicHydraulicTransientFeedback" .


:FrancisGovernorControlKind.mechanicHydrolicTachoAccelerator uml:id "_628C3010-E835-4b2d-AAA6-C44F09B9B815" ;
                                                             rdfs:comment "Mechanic-hydraulic regulator with tacho-accelerometer (Cflag = 1)." ;
                                                             rdfs:label "mechanicHydrolicTachoAccelerator" .


:FuelSource.BGAS uml:id "_E0427B18-C8E2-4f7a-9D7E-80703535A198" ;
                 rdfs:comment "Bio Gas (Landfill, Sewage, Digester, etc.)" ;
                 rdfs:label "BGAS" .


:FuelSource.BIOM uml:id "_FBD9AF03-11AC-40c3-8382-2D101D7ED850" ;
                 rdfs:comment "Biomass" ;
                 rdfs:label "BIOM" .


:FuelSource.COAL uml:id "_A65E7474-2A90-4bec-848C-0A007AA98FE9" ;
                 rdfs:comment "Coal" ;
                 rdfs:label "COAL" .


:FuelSource.DIST uml:id "_C4A436EB-1915-48ff-B935-FFC31453B603" ;
                 rdfs:label "DIST" .


:FuelSource.GAS uml:id "_51C39BFF-B9FF-459e-B3EF-472E28D88D81" ;
                rdfs:label "GAS" .


:FuelSource.GEOT uml:id "_D54DDB78-A2CB-4d4f-8687-D8CF3E81409C" ;
                 rdfs:comment "GeoThermal" ;
                 rdfs:label "GEOT" .


:FuelSource.HRCV uml:id "_57B5AEB5-C9F9-451e-AAE2-F64C21377E08" ;
                 rdfs:label "HRCV" .


:FuelSource.NG uml:id "_733A69FE-9000-45cf-9AA6-1A9FD6743132" ;
               rdfs:comment "Natural Gas" ;
               rdfs:label "NG" .


:FuelSource.NNG uml:id "_F788EFF2-4BA8-4e64-AAF0-4E085053CB5F" ;
                rdfs:comment "Non-Natural Gas" ;
                rdfs:label "NNG" .


:FuelSource.NONE uml:id "_9E85CA32-0527-437d-99EB-FA207B936850" ;
                 rdfs:label "NONE" .


:FuelSource.NUCL uml:id "_9F508CEF-0012-4f63-81C6-352D85760D26" ;
                 rdfs:comment "Nuclear" ;
                 rdfs:label "NUCL" .


:FuelSource.OIL uml:id "_604B2B03-BE98-4b36-B30B-7194E71082D8" ;
                rdfs:label "OIL" .


:FuelSource.OTHR uml:id "_EFBB22A2-300F-43f3-971C-4F725A947F93" ;
                 rdfs:comment "Other" ;
                 rdfs:label "OTHR" .


:FuelSource.SOLR uml:id "_687D0F0E-9827-4322-BB16-A828233FF14F" ;
                 rdfs:comment "Solar" ;
                 rdfs:label "SOLR" .


:FuelSource.WAST uml:id "_862129C4-8F60-4ddb-B4A1-75B416EA2B8D" ;
                 rdfs:comment "Waste to Energy" ;
                 rdfs:label "WAST" .


:FuelSource.WATR uml:id "_1DB47B93-1D35-4ca5-9A34-D704EC5DE7D3" ;
                 rdfs:comment "Water" ;
                 rdfs:label "WATR" .


:FuelSource.WIND uml:id "_1EE3B826-A7F5-4712-8F3F-01ED68EC1FF7" ;
                 rdfs:comment "Wind" ;
                 rdfs:label "WIND" .


:FuelType.brownCoalLignite uml:id "_A5DEF850-4095-4c6f-822A-70E2C3A2004B" ;
                           rdfs:comment "Brown coal lignite." ;
                           rdfs:label "brownCoalLignite" .


:FuelType.coal uml:id "_48574203-A20C-471d-86F8-40A310D86D9C" ;
               rdfs:comment "Generic coal, not including lignite type." ;
               rdfs:label "coal" .


:FuelType.coalDerivedGas uml:id "_A54D2137-25F9-4e6c-8911-9D168CEA13B0" ;
                         rdfs:comment "Coal derived gas." ;
                         rdfs:label "coalDerivedGas" .


:FuelType.gas uml:id "_A584C64F-24D8-456e-849B-A836063EB741" ;
              rdfs:comment "Natural gas." ;
              rdfs:label "gas" .


:FuelType.hardCoal uml:id "_18FE649C-B794-4ced-AFCD-8FDDA6DDCF80" ;
                   rdfs:comment "Hard coal." ;
                   rdfs:label "hardCoal" .


:FuelType.lignite uml:id "_740E6D2B-C458-4553-B915-458358AE74A8" ;
                  rdfs:comment "The fuel is lignite coal.  Note that this is a special type of coal, so the other enum of coal is reserved for hard coal types or if the exact type of coal is not known." ;
                  rdfs:label "lignite" .


:FuelType.oil uml:id "_B8642718-8910-450f-B0F8-6FAFB7AE4E7B" ;
              rdfs:comment "Oil." ;
              rdfs:label "oil" .


:FuelType.oilShale uml:id "_59454BB2-4DFB-459f-9CC2-8F20D3201589" ;
                   rdfs:comment "Oil Shale." ;
                   rdfs:label "oilShale" .


:FuelType.other uml:id "_ECB2760B-5351-4506-9B61-1921945E171C" ;
                rdfs:comment "Any fuel type not included in the rest of the enumerated value." ;
                rdfs:label "other" .


:FuelType.peat uml:id "_FB22A039-D8DB-40bb-B5DD-FEEC6E3DA434" ;
               rdfs:comment "Peat." ;
               rdfs:label "peat" .


:GateLogicKind.and uml:id "_3294F454-7555-4da2-ABA3-2D1082306483" ;
                   rdfs:comment "A logical AND operation. True when all input are true." ;
                   rdfs:label "and" .


:GateLogicKind.nand uml:id "_5135B7ED-80E3-4484-90F5-29A0ADA2F9B7" ;
                    rdfs:comment "A logical NAND operation. False when all input are true." ;
                    rdfs:label "nand" .


:GateLogicKind.nor uml:id "_AA8B0FDC-1F10-428d-B4D1-8EF586685EE3" ;
                   rdfs:comment "A logical NOR operation. False when one or more input are true." ;
                   rdfs:label "nor" .


:GateLogicKind.not uml:id "_ED49693E-176B-4bab-9612-10B18FFB3FA1" ;
                   rdfs:comment "A logical NOT operation. Only one input and true input will give false out and false in will give true out. An inverter." ;
                   rdfs:label "not" .


:GateLogicKind.or uml:id "_3181B9BA-C507-4c6b-A24F-9CF1460986B6" ;
                  rdfs:comment "A logical OR operation. True when one or more input are true." ;
                  rdfs:label "or" .


:GateLogicKind.xnor uml:id "_57D32F58-2F60-411e-A14E-6A8BBB3CBACF" ;
                    rdfs:comment "A logical XNOR operation. The function is the inverse of the exclusive OR (XOR) gate. All input false or true will give true. Otherwise false." ;
                    rdfs:label "xnor" .


:GateLogicKind.xor uml:id "_4AE8A92E-060A-4678-B472-271DF3203B3B" ;
                   rdfs:comment "A logical XOR operation.  All input false or true will give false. Otherwise true." ;
                   rdfs:label "xor" .


:GeneratorControlMode.pulse uml:id "_86003E6B-2E51-439f-B483-DC6898431E72" ;
                            rdfs:comment "Pulse control mode." ;
                            rdfs:label "pulse" .


:GeneratorControlMode.setpoint uml:id "_27334956-C1AD-4ba5-96A4-84E29F956435" ;
                               rdfs:comment "Setpoint control mode." ;
                               rdfs:label "setpoint" .


:GeneratorControlSource.offAGC uml:id "_DD41B9BB-A11A-4b4a-A4C6-4B462E41DDE0" ;
                               rdfs:comment "Off of automatic generation control (AGC)." ;
                               rdfs:label "offAGC" .


:GeneratorControlSource.onAGC uml:id "_5ADBF694-909C-487c-9134-2295C1A3E8E6" ;
                              rdfs:comment "On automatic generation control (AGC)." ;
                              rdfs:label "onAGC" .


:GeneratorControlSource.plantControl uml:id "_F4C5FBF2-28B3-437f-85EF-F574071C790C" ;
                                     rdfs:comment "Plant is controlling." ;
                                     rdfs:label "plantControl" .


:GeneratorControlSource.unavailable uml:id "_BFBC77D6-2D86-48c1-B93F-9293533DCD34" ;
                                    rdfs:comment "Not available." ;
                                    rdfs:label "unavailable" .


:GenericNonLinearLoadModelKind.exponentialRecovery uml:id "_6E645C61-4229-4d95-8E10-2200FEF19D41" ;
                                                   rdfs:comment "Exponential recovery model." ;
                                                   rdfs:label "exponentialRecovery" .


:GenericNonLinearLoadModelKind.loadAdaptive uml:id "_DE516437-5564-4f69-BC30-EDAFBE685E94" ;
                                            rdfs:comment "Load adaptive model." ;
                                            rdfs:label "loadAdaptive" .


:GeosphericAnalogKind.lightningDensity uml:id "_16D8CCB2-EC26-4a23-A076-66449B807D4A" ;
                                       rdfs:comment "Flash rate in strikes/hour/km<sup>2</sup>." ;
                                       rdfs:label "lightningDensity" .


:GeosphericAnalogKind.seismicEastWest uml:id "_4D8E1140-A53A-4406-A904-FD3BAD1DA9E7" ;
                                      rdfs:label "seismicEastWest" .


:GeosphericAnalogKind.seismicNorthSouth uml:id "_D7848E12-FB06-4b2b-B53F-353D88B297F5" ;
                                        rdfs:label "seismicNorthSouth" .


:GeosphericAnalogKind.seismicVertical uml:id "_F5BF2676-7444-4115-8E6C-CCB790693F29" ;
                                      rdfs:label "seismicVertical" .


:GeosphericAnalogKind.snowPackDepth uml:id "_DDAA7C0F-13E4-4149-B7F6-B84345724AF2" ;
                                    rdfs:label "snowPackDepth" .


:GeosphericAnalogKind.temperature uml:id "_1A7F75E1-5FCD-4900-B09B-EF2B7DC51F1B" ;
                                  rdfs:label "temperature" .


:GovHydro4ModelKind.francisPelton uml:id "_B07B361E-CA8F-4433-B86C-E065EA2CDBDA" ;
                                  rdfs:comment "Francis or Pelton model." ;
                                  rdfs:label "francisPelton" .


:GovHydro4ModelKind.kaplan uml:id "_C55953FA-6545-4f55-9CB6-97FDC94F1F05" ;
                           rdfs:comment "Kaplan model." ;
                           rdfs:label "kaplan" .


:GovHydro4ModelKind.simple uml:id "_4FF834A7-38D6-4440-83EE-6111ED481385" ;
                           rdfs:comment "Simple model." ;
                           rdfs:label "simple" .


:HydroEnergyConversionKind.generator uml:id "_2BEF7548-AC7A-47f6-8AFB-D8FD5594FC5A" ;
                                     rdfs:comment "Able to generate power, but not able to pump water for energy storage." ;
                                     rdfs:label "generator" .


:HydroEnergyConversionKind.pumpAndGenerator uml:id "_3965BBB3-D7F3-4a66-82A7-BB51C80B93CD" ;
                                            rdfs:comment "Able to both generate power and pump water for energy storage." ;
                                            rdfs:label "pumpAndGenerator" .


:HydroPlantStorageKind.pumpedStorage uml:id "_BE3E5F7B-A1C9-4b87-8B73-8A3502814C19" ;
                                     rdfs:comment "Pumped storage." ;
                                     rdfs:label "pumpedStorage" .


:HydroPlantStorageKind.runOfRiver uml:id "_62BDEA10-C6A6-4107-9567-CE47AAD0E560" ;
                                  rdfs:comment "Run of river." ;
                                  rdfs:label "runOfRiver" .


:HydroPlantStorageKind.storage uml:id "_7B020F75-B69C-4fe7-A06E-B47EB5E4316F" ;
                               rdfs:comment "Storage." ;
                               rdfs:label "storage" .


:HydroTurbineKind.francis uml:id "_08B0B97B-5C23-4a52-95D7-B97A28E4BFD2" ;
                          rdfs:comment "Francis." ;
                          rdfs:label "francis" .


:HydroTurbineKind.kaplan uml:id "_A132B48C-1981-425d-ABA0-888B87DD1BB3" ;
                         rdfs:comment "Kaplan." ;
                         rdfs:label "kaplan" .


:HydroTurbineKind.pelton uml:id "_F7A8B1D2-22DB-450d-8A83-D21AC557BE19" ;
                         rdfs:comment "Pelton." ;
                         rdfs:label "pelton" .


:HydrosphericAnalogKind.floodLevel uml:id "_2D00B88D-8831-4e21-B324-A7F2F4575929" ;
                                   rdfs:label "floodLevel" .


:HydrosphericAnalogKind.stormSurgeHeight uml:id "_6127D110-1979-4aad-89D0-8C58216ACB47" ;
                                         rdfs:label "stormSurgeHeight" .


:HydrosphericAnalogKind.surfaceTemperature uml:id "_1F42CB38-B2EE-4157-8BED-9CD3BF4BD682" ;
                                           rdfs:label "surfaceTemperature" .


:HydrosphericAnalogKind.waterTemperature uml:id "_5612E922-E82E-4fe1-A946-3E261B672D1B" ;
                                         rdfs:label "waterTemperature" .


:HydrosphericAnalogKind.waveHeight uml:id "_5646466D-9C1A-4e25-9044-139C64DB951A" ;
                                   rdfs:label "waveHeight" .


:ICCPAccessPrivilegeKind.readOnly uml:id "_3D227F82-FAA2-443e-BF9D-11B833D56EC3" ;
                                  rdfs:comment "Indicates that the remote is not allowed to change the value of the ICCPPoint." ;
                                  rdfs:label "readOnly" .


:ICCPAccessPrivilegeKind.readWrite uml:id "_D2DCEFAB-B7C8-4879-A23A-12F2DA28E7A2" ;
                                   rdfs:comment "Indicates that the remote can not only get the value, but may also change the value of the ICCP Point." ;
                                   rdfs:label "readWrite" .


:ICCPPointKind.discrete uml:id "_CAC01C8F-AF3C-46ed-BC32-BCD0F25F39AE" ;
                        rdfs:comment "Indicates that an ICCP discrete type is to be conveyed." ;
                        rdfs:label "discrete" .


:ICCPPointKind.packedProtectionEvent uml:id "_69EE703E-1530-4188-89C7-049534854D58" ;
                                     rdfs:comment "Indicates that an ICCP packed Protection Event is to be conveyed." ;
                                     rdfs:label "packedProtectionEvent" .


:ICCPPointKind.real uml:id "_BCAE2A02-D851-444a-8983-C2F2C017A8F0" ;
                    rdfs:comment "Indicates that an ICCP real type is to be conveyed." ;
                    rdfs:label "real" .


:ICCPPointKind.singleProtectionEvent uml:id "_2F27C9F8-55BA-4a14-8466-5306BF3856AA" ;
                                     rdfs:comment "Indicates that an ICCP single Protection Event  type is to be conveyed." ;
                                     rdfs:label "singleProtectionEvent" .


:ICCPPointKind.state uml:id "_0365C0D5-6134-4798-B9B1-9DA50D9453B5" ;
                     rdfs:comment "Indicates that an ICCP state type is to be conveyed." ;
                     rdfs:label "state" .


:ICCPPointKind.stateSupplemental uml:id "_41821425-CA04-408d-A5CC-8B6712378AAE" ;
                                 rdfs:comment "Indicates that an ICCP state supplemental type is to be conveyed." ;
                                 rdfs:label "stateSupplemental" .


:ICCPQualityKind.extended uml:id "_BCAB25F4-4D61-4fa5-BA85-D1700494BF67" ;
                          rdfs:comment "Indicates that only extended information is to be provided." ;
                          rdfs:label "extended" .


:ICCPQualityKind.extendedwithQualityTime uml:id "_72463474-1088-4bec-86E6-74B2C4DC877D" ;
                                         rdfs:comment "Provides quality, timestamp, and extended information." ;
                                         rdfs:label "extendedwithQualityTime" .


:ICCPQualityKind.none uml:id "_8ED33AF9-9BB8-4c92-955A-2212386EBD25" ;
                      rdfs:comment "Indicates that no quality is conveyed with the ICCP point." ;
                      rdfs:label "none" .


:ICCPQualityKind.qualityAndTime uml:id "_3315A761-4AE5-4716-BB0F-C096EEEA083A" ;
                                rdfs:comment "Indicates that quality and a timestamp are to be provided." ;
                                rdfs:label "qualityAndTime" .


:ICCPQualityKind.qualityOnly uml:id "_BD8502A8-E49B-40e9-9957-D93C4F889E37" ;
                             rdfs:comment "Indicates that only quality is to be provided." ;
                             rdfs:label "qualityOnly" .


:ICCPScopeKind.iCC uml:id "_C51D23B8-119D-46ba-8525-B2CB963D76C0" ;
                   rdfs:comment "Inter-Control Centre scope – available for exchange between the control centres in the bilateral table." ;
                   rdfs:label "iCC" .


:ICCPScopeKind.vCC uml:id "_C9BFD40B-5151-4a57-9423-08E21004EBB6" ;
                   rdfs:comment "Virtual Control Centre Scope – globally available." ;
                   rdfs:label "vCC" .


:IECStandardEditionKind._1963 uml:id "_6C40DD5F-EEC2-4db4-941B-C17385861F61" ;
                              rdfs:comment "1963 edition." ;
                              rdfs:label "1963" .


:IECStandardEditionKind._1967 uml:id "_ACF457D4-C318-4c58-848E-DB4C9C06105D" ;
                              rdfs:comment "1967 edition." ;
                              rdfs:label "1967" .


:IECStandardEditionKind._1973 uml:id "_0A9F53B1-8D38-494d-984F-34FDFEDAB3FC" ;
                              rdfs:comment "1973 edition." ;
                              rdfs:label "1973" .


:IECStandardEditionKind._1974 uml:id "_5FF2DEC1-F0A5-4cd7-A445-70CB232780E4" ;
                              rdfs:comment "1974 edition." ;
                              rdfs:label "1974" .


:IECStandardEditionKind._1977 uml:id "_EFF13CB9-A4E9-45dd-8BD8-1FCE43121154" ;
                              rdfs:comment "1977 edition." ;
                              rdfs:label "1977" .


:IECStandardEditionKind._1978 uml:id "_6F53E5C1-A3F9-4fc0-BCCC-41D6A63DD3C5" ;
                              rdfs:comment "1978 edition." ;
                              rdfs:label "1978" .


:IECStandardEditionKind._1979 uml:id "_2ECD5FF4-1590-4439-9210-556F9E2B1F6E" ;
                              rdfs:comment "1979 edition." ;
                              rdfs:label "1979" .


:IECStandardEditionKind._1985 uml:id "_2EC67A28-9880-4140-885B-E447EF622C96" ;
                              rdfs:comment "1985 edition." ;
                              rdfs:label "1985" .


:IECStandardEditionKind._1989 uml:id "_59764745-EC73-45f3-B32B-34CC461EB258" ;
                              rdfs:comment "1989 edition." ;
                              rdfs:label "1989" .


:IECStandardEditionKind._1992 uml:id "_FC285C33-424F-4c6d-86EF-0F3F3037483B" ;
                              rdfs:comment "1992 edition." ;
                              rdfs:label "1992" .


:IECStandardEditionKind._1992_AMD1_2004 uml:id "_B3D5B8FD-8789-49cc-BB51-4B1B6A3A01E7" ;
                                        rdfs:comment "1992/AMD1:2004 edition." ;
                                        rdfs:label "1992/AMD1:2004" .


:IECStandardEditionKind._1992_COR1_1992 uml:id "_A421FB2D-F914-43d0-BD70-9871661C1ECC" ;
                                        rdfs:comment "1992/COR1:1992 edition." ;
                                        rdfs:label "1992/COR1:1992" .


:IECStandardEditionKind._1993 uml:id "_6408E23E-521D-453f-B7FE-6F68AB10D0E7" ;
                              rdfs:comment "1993 edition." ;
                              rdfs:label "1993" .


:IECStandardEditionKind._1995 uml:id "_F6F560F7-F343-4ecc-955F-935D6E4DE92F" ;
                              rdfs:comment "1995 edition." ;
                              rdfs:label "1995" .


:IECStandardEditionKind._1997 uml:id "_250F5AD3-B5CD-4dc2-9B67-7C0CD555C011" ;
                              rdfs:comment "1997 edition." ;
                              rdfs:label "1997" .


:IECStandardEditionKind._1998 uml:id "_05A74BEA-920E-4329-BD5D-FE9E90E029E3" ;
                              rdfs:comment "1998 edition." ;
                              rdfs:label "1998" .


:IECStandardEditionKind._2004 uml:id "_42970755-F31B-43ba-B11D-5DF2CC42C27E" ;
                              rdfs:comment "2004 edition." ;
                              rdfs:label "2004" .


:IECStandardEditionKind._2004_AMD1_2007 uml:id "_2DB7F596-4CA0-471d-8489-BABC58A14F40" ;
                                        rdfs:comment "2004/AMD1:2007 edition." ;
                                        rdfs:label "2004/AMD1:2007" .


:IECStandardEditionKind._2004_AMD1_2007CSV uml:id "_D05BF832-5BD0-487e-BA3F-6CAB7C2ED64B" ;
                                           rdfs:comment "2004/AMD1:2007CSV edition." ;
                                           rdfs:label "2004/AMD1:2007CSV" .


:IECStandardEditionKind._2005 uml:id "_83B8A508-9C62-4932-BC28-97FE211FB403" ;
                              rdfs:comment "2005 edition." ;
                              rdfs:label "2005" .


:IECStandardEditionKind._2007 uml:id "_366342B9-3F23-4d40-8825-38D9C9483C76" ;
                              rdfs:comment "2007 edition." ;
                              rdfs:label "2007" .


:IECStandardEditionKind._2008 uml:id "_59A2835A-D246-49e9-9ECF-665503B5751A" ;
                              rdfs:comment "2008 edition." ;
                              rdfs:label "2008" .


:IECStandardEditionKind._2010 uml:id "_31F782D4-570D-4e76-AC68-87C24E967552" ;
                              rdfs:comment "2010 edition." ;
                              rdfs:label "2010" .


:IECStandardEditionKind._2011 uml:id "_E60793A5-9F55-4633-8312-3B8C1BB49C0B" ;
                              rdfs:comment "2011 edition." ;
                              rdfs:label "2011" .


:IECStandardEditionKind._2012 uml:id "_E9AC03BF-07A0-4fc1-8EAF-0E99818C49E6" ;
                              rdfs:comment "2012 edition." ;
                              rdfs:label "2012" .


:IECStandardEditionKind._2013 uml:id "_4374CC1D-CB96-48dd-8554-4D18A15631A6" ;
                              rdfs:comment "2013 edition." ;
                              rdfs:label "2013" .


:IECStandardEditionKind._2013_COR_2013 uml:id "_21F1B9DD-5635-4955-BC70-2700405BEBE6" ;
                                       rdfs:comment "2013/COR:2013 edition." ;
                                       rdfs:label "2013/COR:2013" .


:IECStandardEditionKind.none uml:id "_36EFE84B-2EE9-4631-AE9A-DA16B135D4FC" ;
                             rdfs:comment "No edition." ;
                             rdfs:label "none" .


:IECStandardEditionKind.unknown uml:id "_BEB9F61F-4E47-4759-8665-4E087A9CC221" ;
                                rdfs:comment "Unknown edition." ;
                                rdfs:label "unknown" .


:IECStandardKind._60156 uml:id "_FB1C4E31-440F-4cff-844F-D7A5F6DC6AF2" ;
                        rdfs:comment "Insulating liquids - Determination of the breakdown voltage at power frequency - Test method." ;
                        rdfs:label "60156" .


:IECStandardKind._60243-1 uml:id "_F18E897E-6F33-4016-A339-127492AF9BD5" ;
                          rdfs:comment "Electric strength of insulating materials - Test methods - Part 1: Tests at power frequencies." ;
                          rdfs:label "60243-1" .


:IECStandardKind._60243-2 uml:id "_6110D1B7-9389-4f6d-9E09-567216EB7D41" ;
                          rdfs:comment "Electric strength of insulating materials - Test methods - Part 2: Additional requirements for tests using direct voltage." ;
                          rdfs:label "60243-2" .


:IECStandardKind._60243-3 uml:id "_C5323E68-4987-4cdb-B258-681095C8ADC2" ;
                          rdfs:comment "Electric strength of insulating materials - Test methods - Part 3: Additional requirements for 1,2/50 µs impulse tests." ;
                          rdfs:label "60243-3" .


:IECStandardKind._60247 uml:id "_BC32E158-944B-47ca-A983-BDF6F57A21FD" ;
                        rdfs:comment """Insulating liquids - Measurement of relative permittivity, dielectric dissipation factor (tan d) and d.c. resistivity  -or-
Measurement of relative permittivity, dielectric dissipation factor and d.c. resistivity of insulating liquids  -or-
Recommended test cells for measuring the resistivity of insulating liquids and methods of cleaning the cells.""" ;
                        rdfs:label "60247" .


:IECStandardKind._60422 uml:id "_D156A8FF-05D3-4a02-80AD-90B82E0B3638" ;
                        rdfs:comment "Mineral insulating oils in electrical equipment - Supervision and maintenance guidance." ;
                        rdfs:label "60422" .


:IECStandardKind._60450 uml:id "_371C1052-92D6-4bfd-BFF8-5287754AECC0" ;
                        rdfs:comment "Measurement of the average viscometric degree of polymerization of new and aged cellulosic electrically insulating materials." ;
                        rdfs:label "60450" .


:IECStandardKind._60567 uml:id "_6DE8D074-80C5-41c1-8C95-1E00437864D4" ;
                        rdfs:comment """Oil-filled electrical equipment - Sampling of gases and analysis of free and dissolved gasses - Guidance  -or-
Oil-filled electrical equipment - Sampling of gases and of oil for analysis of free and dissolved gases - Guidance  -or-
Guide for the sampling of gases and of oil form oil-filled electrical equipment and for the analysis of free and dissolved gases.""" ;
                        rdfs:label "60567" .


:IECStandardKind._60666 uml:id "_805CAC3D-3CEB-46b3-9C2E-5901FCB817D1" ;
                        rdfs:comment """Detection and determination of specified additives in mineral insulating oils  -or-
Detection and determination of specified anti-oxidant additives in insulating oils.""" ;
                        rdfs:label "60666" .


:IECStandardKind._60814 uml:id "_1F623371-B981-4349-8341-9C0B283FF25E" ;
                        rdfs:comment "Insulating liquids - Oil-impregnated paper and pressboard - Determination of water by automatic coulometric Karl Fischer titration." ;
                        rdfs:label "60814" .


:IECStandardKind._60970 uml:id "_3114A245-3F26-4217-8508-6BFD26D92CFD" ;
                        rdfs:comment """Insulating liquids - Methods for counting and sizing particles  -or-
Methods for counting and sizing particles in insulating liquids.""" ;
                        rdfs:label "60970" .


:IECStandardKind._60997 uml:id "_8439596B-813B-420d-A97E-E8BC2535E489" ;
                        rdfs:comment """Determination of polychlorinated biphenyls (PCBs) in mineral insulating oils by packed column gas chromatography (GC).
Withdrawn.""" ;
                        rdfs:label "60997" .


:IECStandardKind._61125 uml:id "_D109DE8F-7C7D-444e-8A26-33E32CB5A35E" ;
                        rdfs:comment "Unused hydrocarbon based insulating liquids - Test methods for evaluating the oxidation stability." ;
                        rdfs:label "61125" .


:IECStandardKind._61198 uml:id "_97527D59-A690-4722-AC91-81E738186806" ;
                        rdfs:comment "Mineral insulating oils - Methods for the determination of 2-furfural and related compounds." ;
                        rdfs:label "61198" .


:IECStandardKind._61619 uml:id "_56AD72DB-1A18-43a7-ABB1-DB5A5C726F46" ;
                        rdfs:comment "Insulating liquids - Contamination by polychlorinated biphenyls (PCBs) - Method of determination by capillary column gas chromatography." ;
                        rdfs:label "61619" .


:IECStandardKind._61868 uml:id "_3FDEC366-2C13-480d-817C-E62523D893E3" ;
                        rdfs:comment "Mineral insulating oils – Determination of kinematic viscosity at very low temperatures." ;
                        rdfs:label "61868" .


:IECStandardKind._62535 uml:id "_57FD7C74-46DC-4c7c-AA33-DBA703DC5EC8" ;
                        rdfs:comment "Insulating liquids – Test method for detection of potentially corrosive sulphur in used and unused insulating oil." ;
                        rdfs:label "62535" .


:IECStandardKind._62697-1 uml:id "_F9A106D9-1756-4f32-A836-F75BFE098A96" ;
                          rdfs:comment "Test methods for quantitative determination of corrosive sulfur compounds in unused and used insulating liquids - Part 1: Test method for quantitative determination of dibenzyldisulfide (DBDS)." ;
                          rdfs:label "62697-1" .


:IECStandardKind._62770 uml:id "_0F37F434-5CC8-43dc-BBCB-12A0814E7958" ;
                        rdfs:comment "Fluids for electrotechnical applications – Unused natural esters for transformers and similar electrical equipment." ;
                        rdfs:label "62770" .


:IEEEStandardEditionKind._1978 uml:id "_C48DE724-26A7-44bd-BB82-2211318C01C3" ;
                               rdfs:comment "1978 standard edition." ;
                               rdfs:label "1978" .


:IEEEStandardEditionKind._1995 uml:id "_781594C5-996E-4b52-A567-B71C7DB024F0" ;
                               rdfs:comment "1995 standard edition." ;
                               rdfs:label "1995" .


:IEEEStandardEditionKind.none uml:id "_656296F3-4690-4d32-A9AC-EC9CC88D53E1" ;
                              rdfs:comment "No standard edition." ;
                              rdfs:label "none" .


:IEEEStandardEditionKind.unknown uml:id "_B8D79C61-F556-4476-87F2-362C779D84BF" ;
                                 rdfs:comment "Unknown standard edition." ;
                                 rdfs:label "unknown" .


:IEEEStandardKind._62 uml:id "_87F8704C-DE01-4a2d-AAC8-FF671EDAFC56" ;
                      rdfs:comment """IEEE Guide for Diagnostic Field Testing of Electric Power Apparatus - Part 1: Oil Filled Power Transformers, Regulators, and Reactors -or-
IEEE Guide for Field Testing Power Apparatus Insulation.""" ;
                      rdfs:label "62" .


:IPAddressKind.iPv4 uml:id "_C6E2D879-BD9B-480f-B88C-177152D07A87" ;
                    rdfs:comment "Indicates that IPv4 dotted decimal notation is in use." ;
                    rdfs:label "iPv4" .


:IPAddressKind.iPv6 uml:id "_8FC243AE-6376-439f-8FB1-8BE08FF478D0" ;
                    rdfs:comment "Indicates that an IPv6 dotted decimal is in use." ;
                    rdfs:label "iPv6" .


:ISOStandardEditionKind._1973 uml:id "_EF88839F-468A-4458-A717-AF45A85E88BD" ;
                              rdfs:comment "1973 standard edition." ;
                              rdfs:label "1973" .


:ISOStandardEditionKind._1974 uml:id "_68D54C41-1FF0-4df6-B329-A054959AAE95" ;
                              rdfs:comment "1974 standard edition." ;
                              rdfs:label "1974" .


:ISOStandardEditionKind._1976 uml:id "_305E1FE7-E0E6-4216-B54E-538751FECD46" ;
                              rdfs:comment "1976 standard edition." ;
                              rdfs:label "1976" .


:ISOStandardEditionKind._1983 uml:id "_C6B5BC71-056E-4e84-A399-C9989D9DC72B" ;
                              rdfs:comment "1983 standard edition." ;
                              rdfs:label "1983" .


:ISOStandardEditionKind._1985 uml:id "_CF00A108-C167-4338-8943-6DFBE46C8141" ;
                              rdfs:comment "1985 standard edition." ;
                              rdfs:label "1985" .


:ISOStandardEditionKind._1988 uml:id "_F213E179-6DC7-434f-A573-B286B3E60DDA" ;
                              rdfs:comment "1988 standard edition." ;
                              rdfs:label "1988" .


:ISOStandardEditionKind._1992 uml:id "_65757644-E100-415a-A6FA-61070B293B8E" ;
                              rdfs:comment "1992 standard edition." ;
                              rdfs:label "1992" .


:ISOStandardEditionKind._1993 uml:id "_FBACB0A8-4F16-4bb6-84B2-6E29D7E153E9" ;
                              rdfs:comment "1993 standard edition." ;
                              rdfs:label "1993" .


:ISOStandardEditionKind._1994 uml:id "_76A7CAE4-767E-487a-BB9A-74E6CA65AD75" ;
                              rdfs:comment "1994 standard edition." ;
                              rdfs:label "1994" .


:ISOStandardEditionKind._1994_Cor1_1997 uml:id "_46C29A8B-7D65-4c48-B67B-375DAA93418E" ;
                                        rdfs:comment "1994/Cor1:1997 standard edition." ;
                                        rdfs:label "1994/Cor1:1997" .


:ISOStandardEditionKind._1998 uml:id "_E6B765CA-0256-48d7-BF3A-F4B5E1150C7C" ;
                              rdfs:comment "1998 standard edition." ;
                              rdfs:label "1998" .


:ISOStandardEditionKind._2000 uml:id "_50C9162E-DB9A-416b-A59B-F29C467AB5F4" ;
                              rdfs:comment "2000 standard edition." ;
                              rdfs:label "2000" .


:ISOStandardEditionKind._2002 uml:id "_76D79666-6437-417b-A719-54F9488AE2B4" ;
                              rdfs:comment "2002 standard edition." ;
                              rdfs:label "2002" .


:ISOStandardEditionKind._2005 uml:id "_6EA02042-5B56-481c-9D7A-E01066296B06" ;
                              rdfs:comment "2005 standard edition." ;
                              rdfs:label "2005" .


:ISOStandardEditionKind._2008 uml:id "_D776E6B6-6CBD-4b01-8C6F-81D7BD1FBB4C" ;
                              rdfs:comment "2008 standard edition." ;
                              rdfs:label "2008" .


:ISOStandardEditionKind.none uml:id "_BDACDF86-1F57-44c8-9A3C-AC6868B7ED3C" ;
                             rdfs:comment "No standard edition." ;
                             rdfs:label "none" .


:ISOStandardEditionKind.unknown uml:id "_E108B7AE-5430-47a0-B3C6-CFD22F39BA7A" ;
                                rdfs:comment "Unknown standard edition." ;
                                rdfs:label "unknown" .


:ISOStandardKind._1924 uml:id "_038CABD9-D397-404f-9AA7-F86D74E7A62C" ;
                       rdfs:comment "Paper and board -- Determination of tensile strength." ;
                       rdfs:label "1924" .


:ISOStandardKind._1924-1 uml:id "_211EC0AB-ADE7-40ac-80EA-FBE9AA5A4966" ;
                         rdfs:comment "Paper and board -- Determination of tensile properties -- Part 1: Constant rate of loading method." ;
                         rdfs:label "1924-1" .


:ISOStandardKind._1924-2 uml:id "_F88FCE9F-5932-463c-B297-50401665FA3D" ;
                         rdfs:comment """Paper and board -- Determination of tensile properties -- Part 2: Constant rate of elongation method (20 mm/min)  -or-
Paper and board -- Determination of tensile properties -- Part 2: Constant rate of elongation method.""" ;
                         rdfs:label "1924-2" .


:ISOStandardKind._1924-3 uml:id "_02EBBC00-9D9C-45be-8CCB-0A9BE005DF4A" ;
                         rdfs:comment "Paper and board -- Determination of tensile properties -- Part 3: Constant rate of elongation method (100 mm/min)." ;
                         rdfs:label "1924-3" .


:ISOStandardKind._2592 uml:id "_E4DD2545-ACAC-482e-ABF6-F830B1EB3B2B" ;
                       rdfs:comment "Determination of flash and fire points -- Cleveland open cup method (copied directly from ASTM D92)." ;
                       rdfs:label "2592" .


:ISOStandardKind._2719 uml:id "_A8857633-0860-4853-A03E-7D080F705D5B" ;
                       rdfs:comment """Determination of flash point -- Pensky-Martens closed cup method (copied directly from ASTM D93)  -or-
Petroleum products and lubricants -- Determination of flash point -- Pensky-Martens closed cup method (copied directly from ASTM D93)  -or-
Petroleum products -- Determination of flash point -- Pensky-Martens closed cup method (copied directly from ASTM D93).""" ;
                       rdfs:label "2719" .


:ISOStandardKind._3016 uml:id "_683E0BD5-B0B6-4bfb-B5D2-2A68B40B7A6D" ;
                       rdfs:comment """Petroleum products -- Determination of pour point  -or-
Petroleum oils -- Determination of pour point.""" ;
                       rdfs:label "3016" .


:ISOStandardKind._3104 uml:id "_87851F07-10A9-49ee-8F5C-780717B18384" ;
                       rdfs:comment "Petroleum products -- Transparent and opaque liquids -- Determination of kinematic viscosity and calculation of dynamic viscosity." ;
                       rdfs:label "3104" .


:ISOStandardKind._3675 uml:id "_084666C0-E494-4050-B517-C344E8802C7E" ;
                       rdfs:comment """Crude petroleum and liquid petroleum products -- Laboratory determination of density -- Hydrometer method  -or-
Crude petroleum and liquid petroleum products -- Laboratory determination of density or relative density -- Hydrometer method.""" ;
                       rdfs:label "3675" .


:IfdBaseKind.ifag uml:id "_7C8FAC4A-E06D-4cef-A07D-F6A953EB89BD" ;
                  rdfs:comment "Air gap line mode." ;
                  rdfs:label "ifag" .


:IfdBaseKind.iffl uml:id "_94A0A534-CDD3-4cf6-8B58-0ADD44897655" ;
                  rdfs:comment "Full load system mode." ;
                  rdfs:label "iffl" .


:IfdBaseKind.ifnl uml:id "_43B52704-9509-44bc-80D8-CFFF578F695E" ;
                  rdfs:comment "No load system with saturation mode." ;
                  rdfs:label "ifnl" .


:InUseStateKind.inUse uml:id "_11E437C2-410A-4b92-A930-B8FF66A4B722" ;
                      rdfs:comment "Asset is deployed (in use) or is being put into use." ;
                      rdfs:label "inUse" .


:InUseStateKind.notReadyForUse uml:id "_9F7FC0C7-8DCA-4016-8E17-E1C0855470B9" ;
                               rdfs:comment "Asset is not ready to be put into use." ;
                               rdfs:label "notReadyForUse" .


:InUseStateKind.readyForUse uml:id "_94AE9535-ACD7-4cad-ACA9-D0B476B11CB1" ;
                            rdfs:comment "Asset is ready to be put into use." ;
                            rdfs:label "readyForUse" .


:InputSignalKind.branchCurrent uml:id "_EA532B35-5113-49e8-9394-7A91FDA6C9D7" ;
                               rdfs:comment "Input signal is amplitude of remote branch current." ;
                               rdfs:label "branchCurrent" .


:InputSignalKind.busFrequency uml:id "_41AFCD63-391E-4207-8B2B-46DBFD9DA43C" ;
                              rdfs:comment "Input signal is bus voltage fr<font color=\"#0f0f0f\">equency.  This could be a terminal frequency or remote frequency.</font>" ;
                              rdfs:label "busFrequency" .


:InputSignalKind.busFrequencyDeviation uml:id "_05B69A90-D260-4f3f-B50C-C8CA58C23660" ;
                                       rdfs:comment "Input signal is deviation of bus voltage frequ<font color=\"#0f0f0f\">ency.  This could be a terminal frequency deviation or remote frequency deviation.</font>" ;
                                       rdfs:label "busFrequencyDeviation" .


:InputSignalKind.busVoltage uml:id "_ADF7172C-4782-435d-BCB6-8F77B8228143" ;
                            rdfs:comment "Input signal <font color=\"#0f0f0f\">is bus voltage.  This could be a terminal voltage or remote voltage.</font>" ;
                            rdfs:label "busVoltage" .


:InputSignalKind.busVoltageDerivative uml:id "_7257D0BA-639A-4c57-B1A6-B16C8B4A5413" ;
                                      rdfs:comment "Input signal is derivative of bus voltag<font color=\"#0f0f0f\">e.  This could be a terminal voltage derivative or remote voltage derivative.</font>" ;
                                      rdfs:label "busVoltageDerivative" .


:InputSignalKind.fieldCurrent uml:id "_2686F02C-A18A-49f8-A9EB-67492C02D8E3" ;
                              rdfs:comment "Input signal is generator field current." ;
                              rdfs:label "fieldCurrent" .


:InputSignalKind.generatorAcceleratingPower uml:id "_34DD5A5C-2473-47c3-B770-96AA87561AA6" ;
                                            rdfs:comment "Input signal is generator accelerating power." ;
                                            rdfs:label "generatorAcceleratingPower" .


:InputSignalKind.generatorElectricalPower uml:id "_858F5C6A-A7C5-435f-8254-D8CE92928486" ;
                                          rdfs:comment "Input signal is generator electrical power on rated <i>S</i>." ;
                                          rdfs:label "generatorElectricalPower" .


:InputSignalKind.generatorMechanicalPower uml:id "_A75FF07F-1834-4878-93CC-D2769DF9C6C6" ;
                                          rdfs:comment "Input signal is generator mechanical power." ;
                                          rdfs:label "generatorMechanicalPower" .


:InputSignalKind.rotorAngularFrequencyDeviation uml:id "_35873D9C-65AB-4ad0-80E1-A71AC07B91D6" ;
                                                rdfs:comment "Input signal is rotor or shaft angular frequency deviation." ;
                                                rdfs:label "rotorAngularFrequencyDeviation" .


:InputSignalKind.rotorSpeed uml:id "_55B94FB1-BF83-4636-B004-54286AB61A17" ;
                            rdfs:comment "Input signal is rotor or shaft speed (angular frequency)." ;
                            rdfs:label "rotorSpeed" .


:InspectionAnalogKind.airPressureHPSystemReading uml:id "_C8D05575-CF9B-4dc1-809F-020F9F90CC0A" ;
                                                 rdfs:comment "Analog value represents High Pressure system air pressure." ;
                                                 rdfs:label "airPressureHPSystemReading" .


:InspectionAnalogKind.airPressureLPSystemReading uml:id "_46FBE798-84A1-409b-87C7-DEC98CD137CC" ;
                                                 rdfs:comment "Analog value represents Low Pressure system air pressure." ;
                                                 rdfs:label "airPressureLPSystemReading" .


:InspectionAnalogKind.airPressureReading uml:id "_697A35EB-DAF0-4d91-BA07-27CBEA21D045" ;
                                         rdfs:comment "Analog value represents air pressure." ;
                                         rdfs:label "airPressureReading" .


:InspectionAnalogKind.compressorHourMeterReading uml:id "_C946674D-E3F7-4beb-BE3D-0F5D3047E449" ;
                                                 rdfs:comment "Analog value represents reading from compressor hour meter." ;
                                                 rdfs:label "compressorHourMeterReading" .


:InspectionAnalogKind.sF6PressureReading uml:id "_1A251ABC-F75E-4576-9A35-9A9B2BB75C95" ;
                                         rdfs:comment "Analog value represents SF6 gas pressure." ;
                                         rdfs:label "sF6PressureReading" .


:InspectionDiscreteKind.bushingOilLevelsOK uml:id "_26A07024-E8C9-49de-B820-796087C21F97" ;
                                           rdfs:comment "Are bushing oil levels OK?" ;
                                           rdfs:label "bushingOilLevelsOK" .


:InspectionDiscreteKind.checkOilLevelOK uml:id "_BB3D5FE7-AB46-4c73-A12C-9DD6208EE6A9" ;
                                        rdfs:comment "Check oil level OK?" ;
                                        rdfs:label "checkOilLevelOK" .


:InspectionDiscreteKind.controlCabinetHeaterOn uml:id "_8661753A-2EEC-4b50-87C1-500AD33DF35F" ;
                                               rdfs:comment "Is the control cabinet heater on?" ;
                                               rdfs:label "controlCabinetHeaterOn" .


:InspectionDiscreteKind.gasIndicatorNormal uml:id "_A301BA6C-4FF2-4286-B174-362599883C31" ;
                                           rdfs:comment "Is the circuit switcher gas indicator normal?" ;
                                           rdfs:label "gasIndicatorNormal" .


:InspectionDiscreteKind.hydraulicFluidLevelOK uml:id "_8590E228-356A-4bf0-A1CE-1B9B76F59476" ;
                                              rdfs:comment "Hydraulic fluid level OK?" ;
                                              rdfs:label "hydraulicFluidLevelOK" .


:InspectionDiscreteKind.hydraulicOilLevelOK uml:id "_70FF69F1-3ACE-45c0-9C79-4EC04A1C8A49" ;
                                            rdfs:comment "Is the hydraulic oil level OK? Can apply to any individual pole." ;
                                            rdfs:label "hydraulicOilLevelOK" .


:InspectionDiscreteKind.lowToHighPressureCount uml:id "_B2F50519-0295-4182-8A9A-044C3B563273" ;
                                               rdfs:comment "Count of ??." ;
                                               rdfs:label "lowToHighPressureCount" .


:InspectionDiscreteKind.motorOperationsCount uml:id "_90B38379-EFAF-4e90-B30F-142DFF2904BD" ;
                                             rdfs:comment "Count of motor operations." ;
                                             rdfs:label "motorOperationsCount" .


:InspectionDiscreteKind.oilTankLevelsOK uml:id "_CB488747-8299-4b00-9783-8082D62E91C8" ;
                                        rdfs:comment "Are the oil tank levels OK?" ;
                                        rdfs:label "oilTankLevelsOK" .


:InspectionDiscreteKind.operationCount uml:id "_E278D34E-5008-4ba5-BA16-7116BC6725F5" ;
                                       rdfs:comment "Count of operations." ;
                                       rdfs:label "operationCount" .


:InspectionDiscreteKind.pumpMotorOperationCount uml:id "_DCD0DA78-7D31-4869-AB3C-6EAA87195EF1" ;
                                                rdfs:comment "Count of pump motor operations." ;
                                                rdfs:label "pumpMotorOperationCount" .


:InspectionDiscreteKind.springPressureReadingOK uml:id "_C35955CF-DD43-4319-A82A-02CB18F84EF3" ;
                                                rdfs:comment "Is the spring pressure reading OK? Can apply to whole breaker or any individual pole." ;
                                                rdfs:label "springPressureReadingOK" .


:InspectionDiscreteKind.visibleDamageOrLeaks uml:id "_5915F358-4EB7-4868-8943-087CC7612EAE" ;
                                             rdfs:comment "Any visible damage and/or oil/air/SF6 leaks?." ;
                                             rdfs:label "visibleDamageOrLeaks" .


:IntensityCodeKind.heavy uml:id "_5C10B536-BE0A-4207-AADB-D6B4919B66E8" ;
                         rdfs:label "heavy" .


:IntensityCodeKind.light uml:id "_C91C763D-DF3D-490a-BEA6-99D4FA6A15C1" ;
                         rdfs:label "light" .


:IntensityCodeKind.veryHeavy uml:id "_F3AB44A4-D010-488a-A4B7-D2C0999E77F9" ;
                             rdfs:label "veryHeavy" .


:IntensityCodeKind.veryLight uml:id "_2197CD09-4DDB-4792-AF2E-CD0D47E17BB4" ;
                             rdfs:label "veryLight" .


:InterTieDirection.E uml:id "_9B132EC1-7471-46b5-9DAE-F706D912335A" ;
                     rdfs:comment "Export." ;
                     rdfs:label "E" .


:InterTieDirection.I uml:id "_35CD5C12-3FBF-450e-995B-263794822645" ;
                     rdfs:comment "Import." ;
                     rdfs:label "I" .


:InterruptingMediumKind.airBlast uml:id "_439D64B2-44BF-4356-BABD-35CF23C7DD1A" ;
                                 rdfs:comment "Air blast." ;
                                 rdfs:label "airBlast" .


:InterruptingMediumKind.airMagnetic uml:id "_32245187-CE72-4d0e-9FA1-86837885C9ED" ;
                                    rdfs:comment "Air magnetic." ;
                                    rdfs:label "airMagnetic" .


:InterruptingMediumKind.bulkOil uml:id "_ED69C14F-5D6C-4e6c-BE73-B27A9281D597" ;
                                rdfs:comment "Bulk oil." ;
                                rdfs:label "bulkOil" .


:InterruptingMediumKind.gasSinglePressure uml:id "_9FD11CC8-2CF9-4932-9C5E-94F0749D4622" ;
                                          rdfs:comment "Gas single pressure." ;
                                          rdfs:label "gasSinglePressure" .


:InterruptingMediumKind.gasTwoPressure uml:id "_F3CDEEB2-B785-4ffc-ABCC-EDB354DDFCBC" ;
                                       rdfs:comment "Gas two pressure." ;
                                       rdfs:label "gasTwoPressure" .


:InterruptingMediumKind.minimumOil uml:id "_0E05A09C-F553-4332-BA29-D6C0E2ACA13D" ;
                                   rdfs:comment "Minimum oil." ;
                                   rdfs:label "minimumOil" .


:InterruptingMediumKind.vacuum uml:id "_8A6B23DC-D402-4075-B940-700632ACA3D8" ;
                               rdfs:comment "Vacuum." ;
                               rdfs:label "vacuum" .


:JobFlagType.CREATED uml:id "_CA98E320-D1A1-447d-BCF7-8C80199C6D6A" ;
                     rdfs:label "CREATED" .


:JobFlagType.DELETED uml:id "_9F3E3C7D-39AA-4f3e-9BED-31713D86BB5C" ;
                     rdfs:label "DELETED" .


:JobFlagType.MODIFIED uml:id "_66FEB25D-CB7A-4db3-8483-CE6F1E2458B2" ;
                      rdfs:label "MODIFIED" .


:JobScheduleType.CRITICAL uml:id "_8F49D069-7ECD-4188-9E73-10BC7CA5F0F3" ;
                          rdfs:label "CRITICAL" .


:JobScheduleType.NONCRITICAL uml:id "_FA8F410A-80DA-492f-853A-AAC80AD95073" ;
                             rdfs:label "NONCRITICAL" .


:JobStartEndType.END uml:id "_C8DCE124-4544-4ce8-B2DB-C565987C8C0B" ;
                     rdfs:label "END" .


:JobStartEndType.NA uml:id "_4AB8F0EB-1230-4ba7-88CF-F86C960F0661" ;
                    rdfs:label "NA" .


:JobStartEndType.START uml:id "_92081147-2EF6-4509-863F-4791DE776839" ;
                       rdfs:label "START" .


:JointConfigurationKind.other uml:id "_58F6042A-5F4B-4c9d-AF42-E7004EDF54A0" ;
                              rdfs:label "other" .


:JointConfigurationKind.wires1to1 uml:id "_AC2CE61E-F33E-401f-9FF8-BE73E458C745" ;
                                  rdfs:label "wires1to1" .


:JointConfigurationKind.wires2to1 uml:id "_DAF59B3A-D567-44b7-8BD3-B43C8EEED312" ;
                                  rdfs:label "wires2to1" .


:JointConfigurationKind.wires3to1 uml:id "_D125FC51-3FE1-46a9-BF7C-CC58C8BC2211" ;
                                  rdfs:label "wires3to1" .


:JointFillKind.airNoFilling uml:id "_6DA48504-873F-4af4-B794-4D931FE9C4A8" ;
                            rdfs:label "airNoFilling" .


:JointFillKind.asphaltic uml:id "_E984DAFF-A8A0-4b3e-BD42-022E592562C4" ;
                         rdfs:label "asphaltic" .


:JointFillKind.bluefill254 uml:id "_908E4924-90A4-4d43-A252-BF2EA0FC2B02" ;
                           rdfs:label "bluefill254" .


:JointFillKind.epoxy uml:id "_9EF99651-A0F5-40ed-81B0-748BCB2B3CB8" ;
                     rdfs:label "epoxy" .


:JointFillKind.insoluseal uml:id "_9CFAE881-3753-4a98-B1FC-E57B8FF06441" ;
                          rdfs:label "insoluseal" .


:JointFillKind.noFillPrefab uml:id "_18AD660B-1C46-4ef5-AB8E-5C2E1883CD2F" ;
                            rdfs:label "noFillPrefab" .


:JointFillKind.noVoid uml:id "_4DB06DA1-CF67-429e-81D1-F1ECC7C7BF2B" ;
                      rdfs:label "noVoid" .


:JointFillKind.oil uml:id "_2FAA85E6-724F-4732-AC5E-494F6D8C43DB" ;
                   rdfs:label "oil" .


:JointFillKind.other uml:id "_B4C8A436-28EA-4bc1-83B7-73AD5ED75FD4" ;
                     rdfs:label "other" .


:JointFillKind.petrolatum uml:id "_D19861D8-B783-4291-9AA7-AD823797BAB1" ;
                          rdfs:label "petrolatum" .


:LFCResourceType.GEN uml:id "_7FAB9B8B-7532-45b0-9FA4-6298B99D7FF3" ;
                     rdfs:label "GEN" .


:LFCResourceType.PUMP uml:id "_3606DFF3-D324-4b28-9B8B-C29453FEE6E8" ;
                      rdfs:label "PUMP" .


:LaborelecStandardEditionKind.none uml:id "_8EAE8589-7F4C-457f-B6F3-86739BAC9176" ;
                                   rdfs:comment "No standard edition." ;
                                   rdfs:label "none" .


:LaborelecStandardEditionKind.unknown uml:id "_7B57D3A6-E478-46b8-A76E-AA3200619E66" ;
                                      rdfs:comment "Unknown standard edition." ;
                                      rdfs:label "unknown" .


:LaborelecStandardKind.methanol uml:id "_8F5FBE00-AD7B-43f2-96AD-217C455D87EA" ;
                                rdfs:comment "Laborelec test for methanol." ;
                                rdfs:label "methanol" .


:LandPropertyKind.building uml:id "_67DCE805-4247-4ad7-B365-62D0787C624C" ;
                           rdfs:comment "Site enclosed within a building." ;
                           rdfs:label "building" .


:LandPropertyKind.customerPremise uml:id "_496053EF-0382-42cc-A0AC-19FAAA6F2659" ;
                                  rdfs:comment "Site with a customer." ;
                                  rdfs:label "customerPremise" .


:LandPropertyKind.depot uml:id "_9C30687D-9953-4dc7-A51E-670014F23FBC" ;
                        rdfs:comment "Storehouse for supplies that also serves as a station for supporting crews." ;
                        rdfs:label "depot" .


:LandPropertyKind.external uml:id "_39552784-6DB4-4f92-ACB7-D45728C21028" ;
                           rdfs:comment "Property owned or used by an external party that is not a customer." ;
                           rdfs:label "external" .


:LandPropertyKind.gridSupplyPoint uml:id "_38548786-DB4F-47b2-A804-8ECDCFD1D709" ;
                                  rdfs:comment "Substation where the distribution and transmission networks meet and hence have mixed ownership and mixed operational control." ;
                                  rdfs:label "gridSupplyPoint" .


:LandPropertyKind.store uml:id "_612C0577-35D6-43d1-96BC-A4D6374B8FF5" ;
                        rdfs:comment "Place of storage (e.g., a warehouse) to put aside, or accumulate, material and equipment for use when needed." ;
                        rdfs:label "store" .


:LandPropertyKind.substation uml:id "_A5A09EE3-5DDE-45b4-BDD8-9CE2C39FBBED" ;
                             rdfs:comment "Transmission network switchyard." ;
                             rdfs:label "substation" .


:LoadFollowingCapacityType.DOWN uml:id "_8B1226B5-7E32-485e-9432-8612E6396267" ;
                                rdfs:label "DOWN" .


:LoadFollowingCapacityType.UP uml:id "_CE7FE6A3-0323-4003-9150-39DC3A70417E" ;
                              rdfs:label "UP" .


:LoadForecastType.LFZ uml:id "_8D14D495-45C6-4986-AB4A-ACEC57D6ADC0" ;
                      rdfs:comment "Load forecast zone." ;
                      rdfs:label "LFZ" .


:LoadForecastType.LZMS uml:id "_31BD165F-1498-48a5-9BE1-F6EB29A11217" ;
                       rdfs:comment "Metered sub system zone." ;
                       rdfs:label "LZMS" .


:LocationKind.center uml:id "_48F9D82B-2E5C-4fc6-8FFD-3452747E4F42" ;
                     rdfs:comment "The center of a phenomenon. Will typically be used with a Location with a single PositionPoint instance." ;
                     rdfs:label "center" .


:LocationKind.extent uml:id "_84105F6B-7EC8-41c9-A54B-73646078A162" ;
                     rdfs:comment "The area or line of a phenomenon, not the center. Will typically be used with a Location with multiple PositionPoint instances." ;
                     rdfs:label "extent" .


:LocationKind.primary uml:id "_1F2896EE-F037-4a98-B5D9-1F4AE9227124" ;
                      rdfs:comment "Primary area to which an environmental alert applies." ;
                      rdfs:label "primary" .


:LocationKind.secondary uml:id "_80D1D265-3034-4723-87ED-B0FD7F2E2AC4" ;
                        rdfs:comment "Secondary area to which an environmental alert applies." ;
                        rdfs:label "secondary" .


:LookUpTableFunctionKind.additionalQcurrent uml:id "_AA661E5D-4401-4389-AC25-124FFFD607A8" ;
                                            rdfs:label "additionalQcurrent" .


:LookUpTableFunctionKind.vdcol uml:id "_27865F62-75B8-4890-8C34-E14411877CB9" ;
                               rdfs:label "vdcol" .


:MPMTestIdentifierType._1 uml:id "_FDC66BF1-A6BD-4eea-B570-491325115632" ;
                          rdfs:comment "1 - Global Price Test." ;
                          rdfs:label "1" .


:MPMTestIdentifierType._2 uml:id "_8D2B54DF-3AD8-4a18-AE1C-DA9B72759D7C" ;
                          rdfs:comment "2 - Global Conduct Test." ;
                          rdfs:label "2" .


:MPMTestIdentifierType._3 uml:id "_E50EEB6E-78DD-4a7a-B7D0-23DF2F40971C" ;
                          rdfs:comment "3 - Global Impact Test." ;
                          rdfs:label "3" .


:MPMTestIdentifierType._4 uml:id "_511EFF13-F58F-4ee6-B523-65A7CD349616" ;
                          rdfs:comment "4 - Local Price Test." ;
                          rdfs:label "4" .


:MPMTestIdentifierType._5 uml:id "_EF7331F0-C5BC-40f6-BDE1-EE5EA363B982" ;
                          rdfs:comment "5 - Local Conduct Test." ;
                          rdfs:label "5" .


:MPMTestIdentifierType._6 uml:id "_A820611B-740C-409e-AA9A-0A754E1347F1" ;
                          rdfs:comment "6 - Local Impact Test." ;
                          rdfs:label "6" .


:MPMTestMethodType.ALTERNATE uml:id "_3767513C-D390-421c-B566-09767EE6C7E8" ;
                             rdfs:comment "Alternate." ;
                             rdfs:label "ALTERNATE" .


:MPMTestMethodType.NORMAL uml:id "_071E16C4-EC06-4c17-97C8-3FE0A1D2FE7D" ;
                          rdfs:comment "Normal." ;
                          rdfs:label "NORMAL" .


:MPMTestOutcome.D uml:id "_2682B075-D08A-480d-AEFE-4BCBCD2DA6EA" ;
                  rdfs:comment "Disabled" ;
                  rdfs:label "D" .


:MPMTestOutcome.F uml:id "_BAE18119-8F79-48c1-B646-4FC1D5B70416" ;
                  rdfs:comment "Failed" ;
                  rdfs:label "F" .


:MPMTestOutcome.P uml:id "_424596AA-F856-47ef-944C-37AB4E29E056" ;
                  rdfs:comment "Passed" ;
                  rdfs:label "P" .


:MPMTestOutcome.S uml:id "_F45936F6-6934-41c4-98FC-B9BED6A2DEB0" ;
                  rdfs:comment "Skipped" ;
                  rdfs:label "S" .


:MQSCHGType.ADD uml:id "_9AD56F7C-4DB4-4b3e-BBCD-AA0FF37FD185" ;
                rdfs:label "ADD" .


:MQSCHGType.CHG uml:id "_C6E1D0AA-E653-46e1-8ADE-874BF869C382" ;
                rdfs:label "CHG" .


:MQSDELType.ADD uml:id "_8AD03AB0-8584-41c4-8DAB-C8C2822E71B5" ;
                rdfs:label "ADD" .


:MQSDELType.CHG uml:id "_28F0D965-155B-4f82-A4BD-7EE8CC32A0FE" ;
                rdfs:label "CHG" .


:MQSDELType.DEL uml:id "_33CE8BA7-B545-4e47-BBDF-8E85356A890E" ;
                rdfs:label "DEL" .


:MQSInstructionSource.ACT uml:id "_E606B8DC-9E76-4681-AC5A-D5B0AB7210F8" ;
                          rdfs:label "ACT" .


:MQSInstructionSource.INS uml:id "_170F3937-9051-44e5-8FFA-89B32A5D5E63" ;
                          rdfs:label "INS" .


:MacroPeriodKind.billingPeriod uml:hasInitialValue "8" ;
                               uml:id "_28162C5F-9EFB-409b-8225-74B78FCF5FD8" ;
                               rdfs:comment "Captured during the billing period starting at midnight of the first day of the billing period (as defined by the billing cycle day). If during the current billing period, it specifies a period from the start of the current billing period until \"now\"." ;
                               rdfs:label "billingPeriod" .


:MacroPeriodKind.daily uml:hasInitialValue "11" ;
                       uml:id "_6C5410FE-15C4-45e4-8A0E-82A4096B2755" ;
                       rdfs:comment "Daily period starting at midnight. If for the current day, this specifies the time from midnight to \"now\"." ;
                       rdfs:label "daily" .


:MacroPeriodKind.monthly uml:hasInitialValue "13" ;
                         uml:id "_2D1A8FB6-F055-4722-83CD-5F635DA9A53B" ;
                         rdfs:comment "Monthly period starting at midnight on the first day of the month. If within the current month, this specifies the period from the start of the month until \"now.\"" ;
                         rdfs:label "monthly" .


:MacroPeriodKind.none uml:hasInitialValue "0" ;
                      uml:id "_C6DD668D-8A3B-4c0f-BF18-FAE2795C13DD" ;
                      rdfs:comment "Not applicable." ;
                      rdfs:label "none" .


:MacroPeriodKind.seasonal uml:hasInitialValue "22" ;
                          uml:id "_E16B0E47-C091-4102-8DB4-B720B51C41C5" ;
                          rdfs:comment "A season of time spanning multiple months. E.g. \"Summer,\" \"Spring,\" \"Fall,\" and \"Winter\" based cycle. If within the current season, it specifies the period from the start of the current season until \"now.\"" ;
                          rdfs:label "seasonal" .


:MacroPeriodKind.specifiedPeriod uml:hasInitialValue "32" ;
                                 uml:id "_6FD557E1-D896-4b49-A78B-8DE8F6B82670" ;
                                 rdfs:comment "For the period defined by the start and end of the TimePeriod element in the message." ;
                                 rdfs:label "specifiedPeriod" .


:MacroPeriodKind.weekly uml:hasInitialValue "24" ;
                        uml:id "_DCA2FC51-06DF-4c01-8B48-D0856FB531B5" ;
                        rdfs:comment "Weekly period starting at midnight on the first day of the week and ending the instant before midnight the last day of the week. If within the current week, it specifies the period from the start of the week until \"now.\"" ;
                        rdfs:label "weekly" .


:MarketEventStatusKind.active uml:id "_4C2BB19C-52F4-4e4a-9BF9-FCFBA2004FAD" ;
                              rdfs:comment """The status of the event is currently in a active state.
Active (when sysdate is equal or greater than to planned start time)""" ;
                              rdfs:label "active" .


:MarketEventStatusKind.cancelled uml:id "_D1CB8463-1E0C-43c1-9659-FE5BFD1B42A6" ;
                                 rdfs:comment """The status of the event is currently in a cancelled state.
Cancelled (stopped before planned start time or planned end time)""" ;
                                 rdfs:label "cancelled" .


:MarketEventStatusKind.completed uml:id "_0BE48B1A-92DC-4b2b-ADD3-E9735F0321FA" ;
                                 rdfs:comment """The status of the event is currently in a completed state.
Complete (when sysdate is equal to the release time)""" ;
                                 rdfs:label "completed" .


:MarketEventStatusKind.planned uml:id "_BE413E48-A31E-44f6-889C-E4EDD2E45CC5" ;
                               rdfs:comment """The status of the event is currently in a planned state.
Planned (sysdate is less than planned start time)""" ;
                               rdfs:label "planned" .


:MarketProductSelfSchedType.ETC uml:id "_3247DD84-D4B6-4b1d-B9C0-E98636E8F96D" ;
                                rdfs:comment "Existing Transmission Contract." ;
                                rdfs:label "ETC" .


:MarketProductSelfSchedType.LPT uml:id "_9667293F-931E-429d-8F09-95C381A7F31D" ;
                                rdfs:comment "Low price taker." ;
                                rdfs:label "LPT" .


:MarketProductSelfSchedType.PT uml:id "_2ED80949-CC54-4bb0-9C17-BADEEA697806" ;
                               rdfs:comment "Price taker." ;
                               rdfs:label "PT" .


:MarketProductSelfSchedType.RA uml:id "_44B27D30-E018-4427-B5F5-CAE48C7B3B02" ;
                               rdfs:comment "Resource adequacy." ;
                               rdfs:label "RA" .


:MarketProductSelfSchedType.RGMR uml:id "_EA731F57-231A-4522-BE53-E77B5C7DE1CF" ;
                                 rdfs:comment "Regulatory must run." ;
                                 rdfs:label "RGMR" .


:MarketProductSelfSchedType.RMR uml:id "_A5AB1431-B8E9-488a-BB18-48B8D8A6C56E" ;
                                rdfs:comment "Reliability Must Run." ;
                                rdfs:label "RMR" .


:MarketProductSelfSchedType.RMT uml:id "_44727B77-9603-497d-A746-DACE6A7D790F" ;
                                rdfs:comment "Reliability must take." ;
                                rdfs:label "RMT" .


:MarketProductSelfSchedType.SP uml:id "_0EE88180-E190-4676-B9AB-905ABFE754E7" ;
                               rdfs:comment "Self provision." ;
                               rdfs:label "SP" .


:MarketProductSelfSchedType.TOR uml:id "_59A5180A-2003-45c5-B29B-396173559A5D" ;
                                rdfs:comment "Transmission Ownership Right." ;
                                rdfs:label "TOR" .


:MarketProductType.EN uml:id "_84FDD6C9-9164-4db2-9D18-8EECAC447C21" ;
                      rdfs:comment "energy type" ;
                      rdfs:label "EN" .


:MarketProductType.LFD uml:id "_2E6263D4-2AAD-4a37-AFE8-279BFAB0A798" ;
                       rdfs:comment "Load following down" ;
                       rdfs:label "LFD" .


:MarketProductType.LFU uml:id "_CBD339B7-E081-4f57-982F-10D07957C3CD" ;
                       rdfs:comment "Load following up" ;
                       rdfs:label "LFU" .


:MarketProductType.NR uml:id "_AAC473EC-8B17-4ce8-9C37-C128EFF445BD" ;
                      rdfs:comment "non spinning reserve" ;
                      rdfs:label "NR" .


:MarketProductType.RC uml:id "_4F694BBC-9CD5-49e7-B5B7-417A5150E557" ;
                      rdfs:comment "Residual Unit Commitment" ;
                      rdfs:label "RC" .


:MarketProductType.RD uml:id "_41FBA785-6B63-4f90-B22B-E55AB80ED8FA" ;
                      rdfs:comment "regulation down" ;
                      rdfs:label "RD" .


:MarketProductType.REG uml:id "_9F43267F-10A6-494f-8122-E50723D913C7" ;
                       rdfs:comment "Regulation" ;
                       rdfs:label "REG" .


:MarketProductType.RU uml:id "_87151667-13A8-495b-B332-044839661E8D" ;
                      rdfs:comment "regulation up" ;
                      rdfs:label "RU" .


:MarketProductType.SR uml:id "_5A5F9766-1686-4062-9277-CE70A4EB97A3" ;
                      rdfs:comment "spinning reserve" ;
                      rdfs:label "SR" .


:MarketProductTypeAsReq.AS uml:id "_2CC70FE0-F349-43e2-BDC8-9DD0F0AE0A66" ;
                           rdfs:label "AS" .


:MarketProductTypeAsReq.NR uml:id "_B038941C-3CDC-437f-A354-C818DA8B6291" ;
                           rdfs:comment "non spinning reserve" ;
                           rdfs:label "NR" .


:MarketProductTypeAsReq.RD uml:id "_4E11B343-DEFE-44ba-995E-6D25BE73C961" ;
                           rdfs:comment "regulation down" ;
                           rdfs:label "RD" .


:MarketProductTypeAsReq.RU uml:id "_9D6B9050-8F20-4a71-A928-A4EBD6073A72" ;
                           rdfs:comment "regulation up" ;
                           rdfs:label "RU" .


:MarketProductTypeAsReq.SR uml:id "_CA75DF6A-0F81-4c98-A1AB-D1740C4BA88A" ;
                           rdfs:comment "spinning reserve" ;
                           rdfs:label "SR" .


:MarketRoleKind.BalanceResponsibleParty uml:id "_C3AAFCCE-2962-407b-B63E-29590C2914A1" ;
                                        rdfs:comment """A party that has a contract proving financial security and identifying balance responsibility with the Imbalance Settlement Responsible of the Market Balance Area entitling the party to operate in the market. This is the only role allowing a party to nominate energy on a wholesale level.
<b><i>Additional information:</i></b>
The meaning of the word \"balance\" in this context signifies that the quantity contracted to provide or to consume shall be equal to the quantity really provided or consumed. Equivalent to \"Program responsible party\" in the Netherlands. Equivalent to \"Balance group manager\" in Germany. Equivalent to \"market agent\" in Spain.""" ;
                                        rdfs:label "BalanceResponsibleParty" .


:MarketRoleKind.BalanceSupplier uml:id "_C78D24CF-E285-4270-965B-5728D3B695C5" ;
                                rdfs:comment """A party that markets the difference between actual metered energy consumption and the energy bought with firm energy contracts by the Party Connected to the Grid. In addition the Balance Supplier markets any difference with the firm energy contract (of the Party Connected to the Grid) and the metered production.
<b><i>Additional information:</i></b>
There is only one Balance Supplier for each Accounting Point.""" ;
                                rdfs:label "BalanceSupplier" .


:MarketRoleKind.BillingAgent uml:id "_89884C08-822F-41a3-82E2-EDF24B5A9408" ;
                             rdfs:comment "The party responsible for invoicing a concerned party." ;
                             rdfs:label "BillingAgent" .


:MarketRoleKind.BlockEnergyTrader uml:id "_D1FFF02D-6B19-4b61-84FD-E81DB80EB8B3" ;
                                  rdfs:comment "A party that is selling or buying energy on a firm basis (a fixed volume per market time period)." ;
                                  rdfs:label "BlockEnergyTrader" .


:MarketRoleKind.CapacityCoordinator uml:id "_07C9BB84-2FFC-440d-BD2A-CA570A6011A7" ;
                                    rdfs:comment "A party, acting on behalf of the System Operators involved, responsible for establishing a coordinated Offered Capacity and/or Net Transfer Capacity (NTC) and/or Available Transfer Capacity (ATC) between several Market Balance Areas." ;
                                    rdfs:label "CapacityCoordinator" .


:MarketRoleKind.CapacityTrader uml:id "_02736890-4C9D-4f0c-BEF5-CEC6C6A2947D" ;
                               rdfs:comment """A party that has a contract to participate in the Capacity Market to acquire capacity through a Transmission Capacity Allocator.

The capacity may be acquired on behalf of an Interconnection Trade Responsible or for sale on secondary capacity markets.""" ;
                               rdfs:label "CapacityTrader" .


:MarketRoleKind.Consumer uml:id "_5F4CF05F-EDF9-40d6-AD2E-5CF8B617D222" ;
                         rdfs:comment """A party that consumes electricity.
<b><i>Additional information:</i></b>
This is a Type of Party Connected to the Grid.""" ;
                         rdfs:label "Consumer" .


:MarketRoleKind.ConsumptionResponsibleParty uml:id "_E374757E-BCB6-4615-823C-3F2FD03DA6F3" ;
                                            rdfs:comment """A party who can be brought to rights, legally and financially, for any imbalance between enegry nominated and consumed for all associated Accounting Points.
<b><i>Additional information:</i></b>
This is a type of Balance Responsible Party.""" ;
                                            rdfs:label "ConsumptionResponsibleParty" .


:MarketRoleKind.ControlAreaOperator uml:id "_5FE2B642-B6A7-45ca-8B6F-80B6B3C0D470" ;
                                    rdfs:comment """Responsible for :
1. The coordination of exchange programs between its related Market Balance Areas and for the exchanges between its associated Control Areas.
2. The load frequency control for its own area.
3. The coordination of the correction of time deviations.""" ;
                                    rdfs:label "ControlAreaOperator" .


:MarketRoleKind.ControlBlockOperator uml:id "_13E5A3B1-E672-4e46-96C2-141E63500859" ;
                                     rdfs:comment """Responsible for :
1. The coordination of exchanges between its associated Control Blocks and the organisation of the coordination of exchange programs between its related Control Areas.
2. The load frequency control within its own block and ensuring that its Control Areas respect their obligations in respect to load frequency control and time deviation.
3. The organisation of the settlement and/or compensation between its Control Areas.""" ;
                                     rdfs:label "ControlBlockOperator" .


:MarketRoleKind.CoordinationCenterOperator uml:id "_5C328593-F3DE-48f7-9952-E6D4771886E7" ;
                                           rdfs:comment """Responsible for :
1. The coordination of exchange programs between its related Control Blocks and for the exchanges between its associated Coordination Center Zones.
2. Ensuring that its Control Blocks respect their obligations in respect to load frequency control.
3. Calculating the time deviation in cooperation with the associated coordination centers.
4. Carrying out the settlement and/or compensation between its Control Blocks and against the other Coordination Center Zones.""" ;
                                           rdfs:label "CoordinationCenterOperator" .


:MarketRoleKind.GridAccessProvider uml:id "_EA8B33C1-4301-4788-8AC9-69AA5129A049" ;
                                   rdfs:comment "A party responsible for providing access to the grid through an Accounting Point and its use for energy consumption or production to the Party Connected to the Grid." ;
                                   rdfs:label "GridAccessProvider" .


:MarketRoleKind.GridOperator uml:id "_9C7A11A9-11B9-4737-BF28-D021A67BB9A4" ;
                             rdfs:comment "A party that operates one or more grids." ;
                             rdfs:label "GridOperator" .


:MarketRoleKind.ImbalanceSettlementResponsible uml:id "_F77A0704-FAE2-477c-802F-B41D94F8D339" ;
                                               rdfs:comment """A party that is responsible for settlement of the difference between the contracted quantities and the realised quantities of energy products for the Balance Responsible Parties in a Market Balance Area.
Note:
The Imbalance Settlement Responsible has not the responsibility to invoice. The Imbalance Settlement Responsible may delegate the invoicing responsibility to a more generic role such as a Billing Agent.""" ;
                                               rdfs:label "ImbalanceSettlementResponsible" .


:MarketRoleKind.InterconnectionTradeResponsible uml:id "_6B56CF05-A488-4a93-8EB1-02E2393458EE" ;
                                                rdfs:comment """Is a Balance Responsible Party or depends on one. They are recognized by the Nomination Validator for the nomination of already allocated capacity.
<b><i>Additional information:</i></b>
This is a type of Balance Responsible Party.""" ;
                                                rdfs:label "InterconnectionTradeResponsible" .


:MarketRoleKind.MOLResponsible uml:id "_3C9539D6-111F-43e3-8B62-B529FBDEBBB7" ;
                               rdfs:comment "Responsible for the management of the available tenders for all Acquiring System Operators to establish the order of the reserve capacity that can be activated." ;
                               rdfs:label "MOLResponsible" .


:MarketRoleKind.MarketInformationAggregator uml:id "_EBE5F0AA-F215-440d-BFAD-1B7CBBDB05FA" ;
                                            rdfs:comment """Market Information Aggregator, A party that provides market related information that has been compiled from the figures supplied by different actors in the market. This information may also be published or distributed for general use.
<b><i>Note:</i></b>
The Market Information Aggregator may receive information from any market participant that is relevant for publication or distribution.""" ;
                                            rdfs:label "MarketInformationAggregator" .


:MarketRoleKind.MarketOperator uml:id "_502E0B4B-A89A-413d-89ED-FDD192274734" ;
                               rdfs:comment "The unique power exchange of trades for the actual delivery of energy that receives the bids from the Balance Responsible Parties that have a contract to bid. The Market Operator determines the market energy price for the Market Balance Area after applying technical constraints from the System Operator. It may also establish the price for the reconciliation within a Metering Grid Area." ;
                               rdfs:label "MarketOperator" .


:MarketRoleKind.MeterAdministrator uml:id "_1D3A8167-ECE2-42b8-9454-8CDB35A41C49" ;
                                   rdfs:comment "A party responsible for keeping a database of meters." ;
                                   rdfs:label "MeterAdministrator" .


:MarketRoleKind.MeterOperator uml:id "_FAA20AD9-FB5B-4501-A787-97D0DD3D190C" ;
                              rdfs:comment "A party responsible for installing, maintaining, testing, certifying and decommissioning physical meters." ;
                              rdfs:label "MeterOperator" .


:MarketRoleKind.MeteredDataAggregator uml:id "_2C5A1408-092A-454e-B08C-E188B64D8D66" ;
                                      rdfs:comment "A party responsible for the establishment and qualification of metered data from the Metered Data Responsible. This data is aggregated according to a defined set of market rules." ;
                                      rdfs:label "MeteredDataAggregator" .


:MarketRoleKind.MeteredDataCollector uml:id "_A40556A4-583A-45bf-A2D1-4760B3F18324" ;
                                     rdfs:comment "A party responsible for meter reading and quality control of the reading." ;
                                     rdfs:label "MeteredDataCollector" .


:MarketRoleKind.MeteredDataResponsible uml:id "_8585EAA7-125E-439e-A242-3488CEA7D086" ;
                                       rdfs:comment "A party responsible for the establishment and validation of metered data based on the collected data received from the Metered Data Collector. The party is responsible for the history of metered data for a Metering Point." ;
                                       rdfs:label "MeteredDataResponsible" .


:MarketRoleKind.MeteringPointAdministrator uml:id "_D874249D-7BA9-4766-93FB-69D566D569B5" ;
                                           rdfs:comment "A party responsible for registering the parties linked to the metering points in a Metering Grid Area. They are also responsible for maintaining the Metering Point technical specifications. They are responsible for creating and terminating metering points." ;
                                           rdfs:label "MeteringPointAdministrator" .


:MarketRoleKind.NominationValidator uml:id "_6ECFA6CF-938D-4ab3-A439-E4950CE7AECE" ;
                                    rdfs:comment "Has the responsibility of ensuring that all capacity nominated is within the allowed limits and confirming all valid nominations to all involved parties. They inform the Interconnection Trade Responsible of the maximum nominated capacity allowed. Depending on market rules for a given interconnection the corresponding System Operators may appoint one Nomination Validator." ;
                                    rdfs:label "NominationValidator" .


:MarketRoleKind.PartyConnectedToTheGrid uml:id "_0A55202E-7915-4d74-B842-0872C94551CC" ;
                                        rdfs:comment "A party that contracts for the right to consume or produce electricity at an Accounting Point." ;
                                        rdfs:label "PartyConnectedToTheGrid" .


:MarketRoleKind.Producer uml:id "_0A69244F-6CA0-4041-A4B7-2B936282C568" ;
                         rdfs:comment """A party that produces electricity.
<b><i>Additional information:</i></b>
This is a type of Party Connected to the Grid.""" ;
                         rdfs:label "Producer" .


:MarketRoleKind.ProductionResponsibleParty uml:id "_5295D5CD-7B08-4a2c-A9B2-B378EC2379DA" ;
                                           rdfs:comment """A party who can be brought to rights, legally and financially, for any imbalance between energy nominated and produced for all associated Accounting Points.
<b><i>Additional information:</i></b>
This is a type of Balance Responsible Party.""" ;
                                           rdfs:label "ProductionResponsibleParty" .


:MarketRoleKind.ReconciliationAccountable uml:id "_D8B612FD-28C2-4f05-848B-673540A80EA8" ;
                                          rdfs:comment "A party that is financially accountable for the reconciled volume of energy products for a profiled Accounting Point." ;
                                          rdfs:label "ReconciliationAccountable" .


:MarketRoleKind.ReconciliationResponsible uml:id "_ED6D640F-0676-4936-B789-0CE8B7B53B8C" ;
                                          rdfs:comment """A party that is responsible for reconciling, within a Metering Grid Area, the volumes used in the imbalance settlement process for profiled Accounting Points and the actual metered quantities.
Note:
The Reconciliation Responsible may delegate the invoicing responsibility to a more generic role such as a Billing Agent.""" ;
                                          rdfs:label "ReconciliationResponsible" .


:MarketRoleKind.ReserveAllocator uml:id "_11ACC95C-C10D-4f92-9B3C-A79A0BAAF98B" ;
                                 rdfs:comment "Informs the market of reserve requirements, receives tenders against the requirements and in compliance with the prequalification criteria, determines what tenders meet requirements and assigns tenders." ;
                                 rdfs:label "ReserveAllocator" .


:MarketRoleKind.ResourceProvider uml:id "_7BC08364-DBDA-4270-9EBA-F9CCC2F9C80B" ;
                                 rdfs:comment "A role that manages a resource object and provides the schedules for it" ;
                                 rdfs:label "ResourceProvider" .


:MarketRoleKind.SchedulingCoordinator uml:id "_CDE73D24-C773-4f2b-96B5-81F2BED00CF6" ;
                                      rdfs:comment "A party that is responsible for the schedule information and its exchange on behalf of a Balance Responsible Party. For example in the Polish market a Scheduling Coordinator is responsible for information interchange for scheduling and settlement." ;
                                      rdfs:label "SchedulingCoordinator" .


:MarketRoleKind.SystemOperator uml:id "_33BE69AC-8297-44f5-B851-558A8A8AA806" ;
                               rdfs:comment """A party that is responsible for a stable power system operation
(including the organisation of physical balance) through a transmission grid in a geographical area. The System Operator will also determine and be responsible for cross border capacity and exchanges. If necessary they may reduce allocated capacity to ensure operational stability. Transmission as mentioned above means \"the transport of electricity on the extra high or high voltage network with a view to its delivery to final customers or to distributors. Operation of transmission includes as well the tasks of system operation concerning its management of energy flows, reliability of the system and availability of all necessary system services.\" (definition taken from the ENTSO-E RGCE Operation handbook Glossary).
<b><i>Note: </i></b>additional obligations may be imposed through local market rules.""" ;
                               rdfs:label "SystemOperator" .


:MarketRoleKind.TradeResponsibleParty uml:id "_7F3CFB82-BCF0-4d92-A2D0-66B430A492EA" ;
                                      rdfs:comment """A party who can be brought to rights, legally and financially, for any imbalance between energy nominated and consumed for all associated Accounting Points.
<b><i>Note:</i></b>
A power exchange without any privileged responsibilities acts as a Trade Responsible Party.
<b><i>Additional information:</i></b>
This is a type of Balance Responsible Party.""" ;
                                      rdfs:label "TradeResponsibleParty" .


:MarketRoleKind.TransmissionCapacityAllocator uml:id "_2D069218-BCC1-4d3f-A09C-3FC861E8EF69" ;
                                              rdfs:comment """Manages the allocation of transmission capacity for an Allocated Capacity Area.
<b><i>For explicit auctions:</i></b>
The Transmission Capacity Allocator manages, on behalf of the System Operators, the allocation of available transmission capacity for an Allocated capacity Area. They offer the available transmission capacity to the market, allocates the available transmission capacity to individual Capacity Traders and calculates the billing amount of already allocated capacities to the Capacity Traders.""" ;
                                              rdfs:label "TransmissionCapacityAllocator" .


:MarketRoleKind.balancingAuthority uml:id "_6F8E5D0C-AA40-4652-84ED-734FE0456570" ;
                                   rdfs:comment "Balancing authority." ;
                                   rdfs:label "balancingAuthority" .


:MarketRoleKind.competitiveRetailer uml:id "_47422C7D-9502-434b-A65F-93BE7F5C7A64" ;
                                    rdfs:comment "Competitive retailer." ;
                                    rdfs:label "competitiveRetailer" .


:MarketRoleKind.complianceMonitor uml:id "_55D7DADB-E06D-40c3-9523-46AF9D210630" ;
                                  rdfs:comment "Compliance monitor." ;
                                  rdfs:label "complianceMonitor" .


:MarketRoleKind.distributionProvider uml:id "_1D7318DD-9F0A-4696-AD89-E38B341E8289" ;
                                     rdfs:comment "Distribution provider." ;
                                     rdfs:label "distributionProvider" .


:MarketRoleKind.energyServiceConsumer uml:id "_7DBB846A-EF6A-47a4-95B1-E9498A09ACF5" ;
                                      rdfs:comment "Energy service consumer." ;
                                      rdfs:label "energyServiceConsumer" .


:MarketRoleKind.generatorOperator uml:id "_46D65467-7BCA-4297-8EAB-33972815ABC4" ;
                                  rdfs:comment "Generator merchant operator." ;
                                  rdfs:label "generatorOperator" .


:MarketRoleKind.generatorOwner uml:id "_AD6BC660-035D-42e8-A3B6-40E275A44252" ;
                               rdfs:comment "Generator merchant owner." ;
                               rdfs:label "generatorOwner" .


:MarketRoleKind.interchangeAuthority uml:id "_1BB3808E-DD50-4b18-94E2-4260BA6D00EB" ;
                                     rdfs:comment "Interchange authority." ;
                                     rdfs:label "interchangeAuthority" .


:MarketRoleKind.loadServingEntity uml:id "_E08742CC-D417-4316-8F4F-14A94AA3062D" ;
                                  rdfs:comment "Load serving entity." ;
                                  rdfs:label "loadServingEntity" .


:MarketRoleKind.planningAuthority uml:id "_7CCC8875-5825-4beb-AB81-7C79D07586F9" ;
                                  rdfs:comment "Planning authority." ;
                                  rdfs:label "planningAuthority" .


:MarketRoleKind.purchasingSellingEntity uml:id "_6A3633A7-C229-4a45-8902-EF16F1E7F8FF" ;
                                        rdfs:comment "Purchasing selling entity." ;
                                        rdfs:label "purchasingSellingEntity" .


:MarketRoleKind.reliabilityAuthority uml:id "_FE1C5B36-D7F5-44b4-9148-460099C3B111" ;
                                     rdfs:comment "Reliability authority." ;
                                     rdfs:label "reliabilityAuthority" .


:MarketRoleKind.resourcePlanner uml:id "_DECFE64A-128D-4fab-88FF-FEFF49BA9669" ;
                                rdfs:comment "Resource planner." ;
                                rdfs:label "resourcePlanner" .


:MarketRoleKind.standardsDeveloper uml:id "_145C576B-7AEC-41a6-A042-14D96D8D284A" ;
                                   rdfs:comment "Standards developer." ;
                                   rdfs:label "standardsDeveloper" .


:MarketRoleKind.transmissionOperator uml:id "_01891C0C-584C-4ef9-B912-AFFF978864B5" ;
                                     rdfs:comment "Transmission operator." ;
                                     rdfs:label "transmissionOperator" .


:MarketRoleKind.transmissionOwner uml:id "_4644887E-B97D-4f8c-9202-EB28D140DAB7" ;
                                  rdfs:comment "Transmission owner." ;
                                  rdfs:label "transmissionOwner" .


:MarketRoleKind.transmissionPlanner uml:id "_391C235F-10F4-431b-B99F-47C1DF90529B" ;
                                    rdfs:comment "Transmission planner." ;
                                    rdfs:label "transmissionPlanner" .


:MarketRoleKind.transmissionServiceProvider uml:id "_782264D2-A4DA-438e-9C0A-74AE63AC1917" ;
                                            rdfs:comment "Transmission service provider." ;
                                            rdfs:label "transmissionServiceProvider" .


:MarketScheduleServices.retrieveDefaultBidCurves uml:id "_7B8AE87C-DBFA-429f-B709-B18CFF5C1B07" ;
                                                 rdfs:label "retrieveDefaultBidCurves" .


:MarketScheduleServices.retrieveMPMResults uml:id "_E682D0D6-D08E-41ee-92A6-814BECC08875" ;
                                           rdfs:label "retrieveMPMResults" .


:MarketScheduleServices.retrieveMarketAwards uml:id "_FDDFF250-969C-4ded-B643-F90CBF4749D0" ;
                                             rdfs:label "retrieveMarketAwards" .


:MarketScheduleServices.retrieveSchedulePrices uml:id "_FD40E494-5006-4153-8C9A-D0D091DBBFA2" ;
                                               rdfs:label "retrieveSchedulePrices" .


:MarketScheduleServices.retrieveStartUpShutDownInstructions uml:id "_E80C54F1-0F55-4f3c-AE50-5DE95F2C56C6" ;
                                                            rdfs:label "retrieveStartUpShutDownInstructions" .


:MarketStatementDescription.DAILY_INITIAL_CREDIT uml:id "_C10A8321-A95A-4599-86B7-45C92A1B4763" ;
                                                 rdfs:label "DAILY_INITIAL_CREDIT" .


:MarketStatementDescription.DAILY_INITIAL_MARKET uml:id "_F59526BC-DB61-4af9-8837-D6C0D04E70CD" ;
                                                 rdfs:label "DAILY_INITIAL_MARKET" .


:MarketStatementDescription.DAILY_RECALC_MARKET uml:id "_2F7B123B-4769-4d4f-B1AC-B5271A6EB53D" ;
                                                rdfs:label "DAILY_RECALC_MARKET" .


:MarketStatementDescription.MONTHLY_INITIAL_MARKET uml:id "_97F00589-DE57-4b78-B405-3B0E29EC6413" ;
                                                   rdfs:label "MONTHLY_INITIAL_MARKET" .


:MarketStatementDescription.MONTHLY_RECALC_MARKET uml:id "_5C4FA3CE-DCBD-4ceb-B255-290EDBA9FE58" ;
                                                  rdfs:label "MONTHLY_RECALC_MARKET" .


:MarketStatementDocStatus.APPROVED uml:id "_315D7F8F-E6FD-46e6-B883-3C5C8534FD2D" ;
                                   rdfs:label "APPROVED" .


:MarketStatementDocStatus.CANCELLED uml:id "_D4B7FA95-EDEA-4a57-82CA-1FDCCFB5BDCD" ;
                                    rdfs:label "CANCELLED" .


:MarketStatementDocType.CREDIT uml:id "_91FBE1AC-3FF6-4872-8944-CEABD56ACAF6" ;
                               rdfs:label "CREDIT" .


:MarketStatementDocType.MARKET_INITIAL uml:id "_5E013820-A7D8-4c30-9A39-F39B3997D7B3" ;
                                       rdfs:label "MARKET_INITIAL" .


:MarketStatementDocType.MARKET_RECALC uml:id "_39E196A2-664D-49ee-AAAC-7C1210098BCB" ;
                                      rdfs:label "MARKET_RECALC" .


:MarketStatementLineItemAliasName.CHARGE_CODE_INTERVAL_DETAIL uml:id "_F1450606-E0F3-4a4c-9BA0-348751736D99" ;
                                                              rdfs:label "CHARGE_CODE_INTERVAL_DETAIL" .


:MarketStatementLineItemAliasName.CHARGE_CODE_INTERVAL_TOTAL uml:id "_F68050B4-7262-4fd9-87F5-24A67465DEC3" ;
                                                             rdfs:label "CHARGE_CODE_INTERVAL_TOTAL" .


:MarketStatementLineItemAliasName.CHARGE_CODE_SUMMARY uml:id "_B07C77C4-2A17-46b6-BA9D-182D6364289B" ;
                                                      rdfs:label "CHARGE_CODE_SUMMARY" .


:MarketStatementLineItemAliasName.CHARGE_GROUP uml:id "_670CA605-301D-4800-8223-456D19A2C95C" ;
                                               rdfs:label "CHARGE_GROUP" .


:MarketStatementLineItemAliasName.PARENT_CHARGE_GROUP uml:id "_4F59B72D-237C-4f8f-B603-4CFE96D00F6F" ;
                                                      rdfs:label "PARENT_CHARGE_GROUP" .


:MarketStatementLineItemAliasName.TRADE_DATE uml:id "_3E50D4A6-C1C0-4cbd-A032-BA5595E68694" ;
                                             rdfs:label "TRADE_DATE" .


:MarketType.DAM uml:id "_891C81EB-EFFA-4daf-88A7-7C23075ABDC1" ;
                rdfs:comment "Day ahead market." ;
                rdfs:label "DAM" .


:MarketType.HAM uml:id "_CC7C140B-8ADC-406a-9A2B-DB818199FCCB" ;
                rdfs:comment "Hour Ahead Market." ;
                rdfs:label "HAM" .


:MarketType.RTM uml:id "_D86CA228-F06F-404e-B74C-D7C2F0BFF312" ;
                rdfs:comment "Real time market." ;
                rdfs:label "RTM" .


:MarketType.RUC uml:id "_F0871DEA-187F-4824-94B9-7DF280295FBE" ;
                rdfs:comment "Residual Unit Commitment." ;
                rdfs:label "RUC" .


:MeasurementKind-Old.alarm uml:hasInitialValue "118" ;
                           uml:id "_6C8B2687-1D40-4e3a-9B9C-A3F8644D5D95" ;
                           rdfs:comment "A measurement related to an alarm" ;
                           rdfs:label "alarm" .


:MeasurementKind-Old.apTitle uml:hasInitialValue "91" ;
                             uml:id "_E825E37B-4095-4d8a-A211-A07CCD91B81C" ;
                             rdfs:comment "An application name which is making or has made a request" ;
                             rdfs:label "apTitle" .


:MeasurementKind-Old.apparentPowerFactor uml:hasInitialValue "2" ;
                                         uml:id "_BA83F63C-2564-4638-84DC-7350CEB0B514" ;
                                         rdfs:comment "The ratio of real energy (usually net Wh) to apparent energy (kVAh)" ;
                                         rdfs:label "apparentPowerFactor" .


:MeasurementKind-Old.applicationContext uml:hasInitialValue "90" ;
                                        uml:id "_4510F633-563E-491d-A2BD-0380BB4DE654" ;
                                        rdfs:comment "Information that describes the logical context in which a request, measurement, or command is made." ;
                                        rdfs:label "applicationContext" .


:MeasurementKind-Old.assetNumber uml:hasInitialValue "92" ;
                                 uml:id "_57473841-FEAA-4dca-8152-0A4A09EB2279" ;
                                 rdfs:comment "An asset identifier" ;
                                 rdfs:label "assetNumber" .


:MeasurementKind-Old.audibleVolume uml:hasInitialValue "154" ;
                                   uml:id "_CB1FF935-EB13-4734-9FB3-DA31CB9B0A86" ;
                                   rdfs:comment "Sound" ;
                                   rdfs:label "audibleVolume" .


:MeasurementKind-Old.bandwidth uml:hasInitialValue "93" ;
                               uml:id "_DAF8FBF9-15C9-4282-85FE-7FEDF48E9D5A" ;
                               rdfs:comment "A measurement of dataflow" ;
                               rdfs:label "bandwidth" .


:MeasurementKind-Old.batteryCarryover uml:hasInitialValue "119" ;
                                      uml:id "_02C2B75D-BC48-4685-A51D-4EB94DDA594E" ;
                                      rdfs:comment "An estimate of the battery ride through capacity" ;
                                      rdfs:label "batteryCarryover" .


:MeasurementKind-Old.batteryVoltage uml:hasInitialValue "94" ;
                                    uml:id "_29F131A7-174F-4299-87F0-BC059795754C" ;
                                    rdfs:comment "Battery voltage" ;
                                    rdfs:label "batteryVoltage" .


:MeasurementKind-Old.billCarryover uml:hasInitialValue "152" ;
                                   uml:id "_1F0B5020-1561-46fb-83BA-AEDBAAE5CA48" ;
                                   rdfs:comment "Customer’s bill for the (Currency)" ;
                                   rdfs:label "billCarryover" .


:MeasurementKind-Old.billLastPeriod uml:hasInitialValue "150" ;
                                    uml:id "_238314AF-66D5-4f28-BB47-77CC1EE8CD1E" ;
                                    rdfs:comment "Customer’s bill for the previous billing period (Currency)" ;
                                    rdfs:label "billLastPeriod" .


:MeasurementKind-Old.billToDate uml:hasInitialValue "151" ;
                                uml:id "_D00D6DAB-606B-4489-9231-DA15F89D997D" ;
                                rdfs:comment "Customer’s bill, as known thus far within the present billing period (Currency)" ;
                                rdfs:label "billToDate" .


:MeasurementKind-Old.broadcastAddress uml:hasInitialValue "95" ;
                                      uml:id "_6E58A65E-C33C-4561-8DC5-093D28ACC446" ;
                                      rdfs:comment "A message target address implying all endpoint units within range of a particular sender" ;
                                      rdfs:label "broadcastAddress" .


:MeasurementKind-Old.connectionFee uml:hasInitialValue "153" ;
                                   uml:id "_BA7AE343-2EEF-4f18-837E-000094403938" ;
                                   rdfs:comment "Monthly fee for connection to commodity." ;
                                   rdfs:label "connectionFee" .


:MeasurementKind-Old.currency uml:hasInitialValue "3" ;
                              uml:id "_6F3A41C1-8410-40e4-A082-827662CD8B9D" ;
                              rdfs:comment "funds" ;
                              rdfs:label "currency" .


:MeasurementKind-Old.current uml:hasInitialValue "4" ;
                             uml:id "_05F18CF5-02BA-4f08-BF37-01DCEC4F8C72" ;
                             rdfs:comment "The flow of electrons" ;
                             rdfs:label "current" .


:MeasurementKind-Old.currentAngle uml:hasInitialValue "5" ;
                                  uml:id "_33E3DB8A-467A-4020-8B5C-00E6C23B563B" ;
                                  rdfs:comment "A phase current zerocross timing measurement releative to a reference voltage zerocross" ;
                                  rdfs:label "currentAngle" .


:MeasurementKind-Old.currentImbalance uml:hasInitialValue "6" ;
                                      uml:id "_2F62FF9C-F7CC-4866-B020-D1DD1B52BBD9" ;
                                      rdfs:comment "A measurement of the departure of a phase current relative to the average current of all phases" ;
                                      rdfs:label "currentImbalance" .


:MeasurementKind-Old.dataOverflowAlarm uml:hasInitialValue "120" ;
                                       uml:id "_AE457323-87B0-462e-9BA4-A3F30B7D3FD6" ;
                                       rdfs:comment "An indication of or measurement of a loss of data" ;
                                       rdfs:label "dataOverflowAlarm" .


:MeasurementKind-Old.date uml:hasInitialValue "7" ;
                          uml:id "_C549663E-B2BF-46f0-B5D5-9937243B8D04" ;
                          rdfs:comment "A measurement of the date and/or time in a clock, or a time stamp indicating when data was captured, when a maximum or minimum occurred, or to commemorate some other important aspect of a measurement" ;
                          rdfs:label "date" .


:MeasurementKind-Old.demand uml:hasInitialValue "8" ;
                            uml:id "_C20A56AC-E45E-4514-9EFD-52BB4E25F5B4" ;
                            rdfs:comment "The measurement of maximum power flow which is computed as energy usage over time, the dimensions of which are defined by a tariff" ;
                            rdfs:label "demand" .


:MeasurementKind-Old.demandLimit uml:hasInitialValue "121" ;
                                 uml:id "_E4B2920D-29E3-478c-9927-5ED0D2BCA21D" ;
                                 rdfs:comment "A threshold setting that determines the trip point that if exceeded would trigger a demand limiting action or alarm" ;
                                 rdfs:label "demandLimit" .


:MeasurementKind-Old.demandReset uml:hasInitialValue "122" ;
                                 uml:id "_95573EB2-A799-484e-A625-43C2F65AA18E" ;
                                 rdfs:comment "A count of the number of times demand has been reset (remotely, locally, and/or automatically.)" ;
                                 rdfs:label "demandReset" .


:MeasurementKind-Old.deviceAddressType1 uml:hasInitialValue "96" ;
                                        uml:id "_7ED5F11D-085A-43de-A968-8A32226D076D" ;
                                        rdfs:comment "Endpoint target address Type1" ;
                                        rdfs:label "deviceAddressType1" .


:MeasurementKind-Old.deviceAddressType2 uml:hasInitialValue "97" ;
                                        uml:id "_BFFFE45F-DB44-490b-A8DB-4CE4A339DFA5" ;
                                        rdfs:comment "Endpoint target address Type2" ;
                                        rdfs:label "deviceAddressType2" .


:MeasurementKind-Old.deviceAddressType3 uml:hasInitialValue "98" ;
                                        uml:id "_F3FB951F-6C19-4545-B7B5-DE4CA5CEA7F4" ;
                                        rdfs:comment "Endpoint target address Type3" ;
                                        rdfs:label "deviceAddressType3" .


:MeasurementKind-Old.deviceAddressType4 uml:hasInitialValue "99" ;
                                        uml:id "_5417B8B5-99E7-46bf-B131-1D2069CB96B1" ;
                                        rdfs:comment "Endpoint target address Type4" ;
                                        rdfs:label "deviceAddressType4" .


:MeasurementKind-Old.deviceClass uml:hasInitialValue "100" ;
                                 uml:id "_B6571D72-5988-4ac2-8EF9-7B8AC824E35B" ;
                                 rdfs:comment "A unique identifier for the Endpoint’s configuration" ;
                                 rdfs:label "deviceClass" .


:MeasurementKind-Old.diagnostic uml:hasInitialValue "123" ;
                                uml:id "_BE297427-3ED8-498d-BF3E-42D4E50C232F" ;
                                rdfs:comment "A measurement related to equipment diagnostics" ;
                                rdfs:label "diagnostic" .


:MeasurementKind-Old.distance uml:hasInitialValue "9" ;
                              uml:id "_13775785-7ED7-4bbd-8B7E-DED8A3C25200" ;
                              rdfs:comment "A linear distance or range radius" ;
                              rdfs:label "distance" .


:MeasurementKind-Old.distortionPowerFactor uml:hasInitialValue "64" ;
                                           uml:id "_0462B2F4-FD07-4415-B1A6-D3A6A9979EA3" ;
                                           rdfs:comment "The ratio of the distortion VAh to the apparent VAh" ;
                                           rdfs:label "distortionPowerFactor" .


:MeasurementKind-Old.distortionVoltAmp uml:hasInitialValue "10" ;
                                       uml:id "_604F5826-FBC9-44f4-A2B8-FE6C2075E13F" ;
                                       rdfs:comment "A measurement in which a V<sup>2</sup> I<sup>2</sup> term has both real and reactive components removed leaving only distortion. For example, distortion VAh = Sqrt( (V<sup>2</sup>h)(I<sup>2</sup>h) – (Wh)<sup>2</sup> – (VArh)<sup>2</sup>)" ;
                                       rdfs:label "distortionVoltAmp" .


:MeasurementKind-Old.electronicSerialNumber uml:hasInitialValue "101" ;
                                            uml:id "_6A5CC0FB-D82D-4649-A3B7-D83512B96514" ;
                                            rdfs:comment "A device serial number" ;
                                            rdfs:label "electronicSerialNumber" .


:MeasurementKind-Old.emergencyLimit uml:hasInitialValue "124" ;
                                    uml:id "_0983F9B7-67DD-49d7-BB9A-45F4099BF2F1" ;
                                    rdfs:comment "A setting that indicates an emergency limit" ;
                                    rdfs:label "emergencyLimit" .


:MeasurementKind-Old.encoderTamper uml:hasInitialValue "125" ;
                                   uml:id "_D3B27A43-E89E-4a7e-85AB-0C76D3388FA0" ;
                                   rdfs:comment "An indication of tampering with a meter encoder" ;
                                   rdfs:label "encoderTamper" .


:MeasurementKind-Old.endDeviceID uml:hasInitialValue "102" ;
                                 uml:id "_91BC7C38-8FF7-422d-8AA4-1F3FF91D0623" ;
                                 rdfs:comment "A unique identifier of the endDevice – the device providing measurements or under control of the network" ;
                                 rdfs:label "endDeviceID" .


:MeasurementKind-Old.energization uml:hasInitialValue "11" ;
                                  uml:id "_AC84FA97-D5D9-4a95-A00A-565106829D50" ;
                                  rdfs:comment "Pertaining to the presence of voltage" ;
                                  rdfs:label "energization" .


:MeasurementKind-Old.energizationLoadSide uml:hasInitialValue "13" ;
                                          uml:id "_B38B0458-A7AA-4df0-BA6D-062ED8B41986" ;
                                          rdfs:comment "Measuring the presence or absence of voltage on the load side of an electricity meter" ;
                                          rdfs:label "energizationLoadSide" .


:MeasurementKind-Old.energy uml:hasInitialValue "12" ;
                            uml:id "_3FCDCE57-6938-4bde-8E2C-9BD8B3110A5C" ;
                            rdfs:comment "Scalar quantity which may be increased or decreased in a system when it receives or produces work, respectively" ;
                            rdfs:label "energy" .


:MeasurementKind-Old.fan uml:hasInitialValue "14" ;
                         uml:id "_754A8001-FED9-4810-AE5A-EA384FACDF84" ;
                         rdfs:comment "A forced air moving device" ;
                         rdfs:label "fan" .


:MeasurementKind-Old.frequency uml:hasInitialValue "15" ;
                               uml:id "_D21F8662-8A64-4139-B1C0-4FE4FF5C6786" ;
                               rdfs:comment "Reciprocal of the period" ;
                               rdfs:label "frequency" .


:MeasurementKind-Old.frequencyExcursion uml:hasInitialValue "81" ;
                                        uml:id "_6A85458C-6392-4316-AC22-1EAE98D93ECF" ;
                                        rdfs:comment "A measurement of the departure of the frequency from the nominal frequency" ;
                                        rdfs:label "frequencyExcursion" .


:MeasurementKind-Old.fund uml:hasInitialValue "16" ;
                          uml:id "_6771B1C4-1584-4858-9688-BF698815EA1F" ;
                          rdfs:comment "Duplicate with “currency”" ;
                          rdfs:label "fund" .


:MeasurementKind-Old.groupAddressType1 uml:hasInitialValue "103" ;
                                       uml:id "_6F477B54-975C-4661-B849-5206996AD234" ;
                                       rdfs:comment "Group target address Type1" ;
                                       rdfs:label "groupAddressType1" .


:MeasurementKind-Old.groupAddressType2 uml:hasInitialValue "104" ;
                                       uml:id "_BD0E9162-2B97-436d-BFCE-2FFB7FE19EC9" ;
                                       rdfs:comment "Group target address Type2" ;
                                       rdfs:label "groupAddressType2" .


:MeasurementKind-Old.groupAddressType3 uml:hasInitialValue "105" ;
                                       uml:id "_6ABF306E-BB8D-4da5-A9DF-9F58D0561C38" ;
                                       rdfs:comment "Group target address Type3" ;
                                       rdfs:label "groupAddressType3" .


:MeasurementKind-Old.groupAddressType4 uml:hasInitialValue "106" ;
                                       uml:id "_669C3AA5-4710-455b-B775-90D8837ECD52" ;
                                       rdfs:comment "Group target address Type4" ;
                                       rdfs:label "groupAddressType4" .


:MeasurementKind-Old.ieee1366ASAI uml:hasInitialValue "17" ;
                                  uml:id "_6E3DDB1C-10C9-4dd8-9746-E8FE7F8EF4BA" ;
                                  rdfs:comment "A measurement of IEEE-1366 Average Service Availability Index" ;
                                  rdfs:label "ieee1366ASAI" .


:MeasurementKind-Old.ieee1366ASIDI uml:hasInitialValue "18" ;
                                   uml:id "_2669BDC6-6D2E-4d92-9754-DFF39CDC1BFD" ;
                                   rdfs:comment "A measurement of the IEEE-1366 Average Service Interruption Duration Index" ;
                                   rdfs:label "ieee1366ASIDI" .


:MeasurementKind-Old.ieee1366ASIFI uml:hasInitialValue "19" ;
                                   uml:id "_C6F53A6D-6286-4bca-B0E9-BE2B4714AD06" ;
                                   rdfs:comment "A measurement of the IEEE-1366 Average Service Interruption Frequency Index" ;
                                   rdfs:label "ieee1366ASIFI" .


:MeasurementKind-Old.ieee1366CAIDI uml:hasInitialValue "20" ;
                                   uml:id "_00A21C74-8B31-4400-B038-EB2DB587478F" ;
                                   rdfs:comment "A measurement of the IEEE-1366 Customer average interruption duration index" ;
                                   rdfs:label "ieee1366CAIDI" .


:MeasurementKind-Old.ieee1366CAIFI uml:hasInitialValue "21" ;
                                   uml:id "_BA162247-652E-484a-B91B-29F66E9B65C9" ;
                                   rdfs:comment "A measurement of the IEEE-1366 Customer average interruption frequency index" ;
                                   rdfs:label "ieee1366CAIFI" .


:MeasurementKind-Old.ieee1366CEMIn uml:hasInitialValue "22" ;
                                   uml:id "_494C0DC9-987D-4c17-AE3D-7F801F190873" ;
                                   rdfs:comment "A measurement of the IEEE-1366 Customers Experiencing Multiple Interruptions" ;
                                   rdfs:label "ieee1366CEMIn" .


:MeasurementKind-Old.ieee1366CEMSMIn uml:hasInitialValue "23" ;
                                     uml:id "_305ED7F6-05BE-45fb-ABA7-82055B452C45" ;
                                     rdfs:comment "A measurement of the IEEE-1366 Customers Experiencing Multiple Sustained and Momentary Interruptions" ;
                                     rdfs:label "ieee1366CEMSMIn" .


:MeasurementKind-Old.ieee1366CTAIDI uml:hasInitialValue "24" ;
                                    uml:id "_28D6D607-389C-4240-BC00-EC9025BDC4E1" ;
                                    rdfs:comment "A measurement of the IEEE-1366 Customer Total Average Interruption Duration Index" ;
                                    rdfs:label "ieee1366CTAIDI" .


:MeasurementKind-Old.ieee1366MAIFI uml:hasInitialValue "25" ;
                                   uml:id "_4B1EA76A-3CE6-464f-BB78-60CDF6521ACA" ;
                                   rdfs:comment "A measurement of the IEEE-1366 Momentary Average Interruption Frequency Index" ;
                                   rdfs:label "ieee1366MAIFI" .


:MeasurementKind-Old.ieee1366MAIFIe uml:hasInitialValue "26" ;
                                    uml:id "_1D522D8E-E75C-419b-88B9-EE2B86813F2B" ;
                                    rdfs:comment "A measurement of the IEEE-1366 Momentary Average event Interruption Frequency Index" ;
                                    rdfs:label "ieee1366MAIFIe" .


:MeasurementKind-Old.ieee1366MomentaryInterruption uml:hasInitialValue "126" ;
                                                   uml:id "_603E2B31-DFA0-4acf-91D5-697ADC8F2E98" ;
                                                   rdfs:comment "IEEE-1366 Momentary Interruption count" ;
                                                   rdfs:label "ieee1366MomentaryInterruption" .


:MeasurementKind-Old.ieee1366MomentaryInterruptionEvent uml:hasInitialValue "127" ;
                                                        uml:id "_7C8D87BE-253E-42c3-9C84-159BE29036B5" ;
                                                        rdfs:comment "IEEE-1366 Momentary Interruption event count" ;
                                                        rdfs:label "ieee1366MomentaryInterruptionEvent" .


:MeasurementKind-Old.ieee1366SAIDI uml:hasInitialValue "27" ;
                                   uml:id "_BA3016F8-312B-4ab9-9006-F6AC10573B28" ;
                                   rdfs:comment "IEEE-1366 System Average Interruption Duration Index" ;
                                   rdfs:label "ieee1366SAIDI" .


:MeasurementKind-Old.ieee1366SAIFI uml:hasInitialValue "28" ;
                                   uml:id "_D682C37A-A02F-49af-8E7F-821CF904F6FA" ;
                                   rdfs:comment "IEEE-1366 System Average Interruption Frequency Index" ;
                                   rdfs:label "ieee1366SAIFI" .


:MeasurementKind-Old.ieee1366SustainedInterruption uml:hasInitialValue "128" ;
                                                   uml:id "_D6B9909F-1796-4bbe-8DD5-27EBC89B0AA5" ;
                                                   rdfs:comment "IEEE-1366 Sustained Interruption duration" ;
                                                   rdfs:label "ieee1366SustainedInterruption" .


:MeasurementKind-Old.interruptionBehaviour uml:hasInitialValue "129" ;
                                           uml:id "_61AEA8AE-988D-494c-B69B-8E96E8A13EBC" ;
                                           rdfs:comment "A measurement related to power interruptions (Note: often an interruption count or duration.)" ;
                                           rdfs:label "interruptionBehaviour" .


:MeasurementKind-Old.inversionTamper uml:hasInitialValue "130" ;
                                     uml:id "_03D0D557-B268-43b4-BF11-F620B0F17C45" ;
                                     rdfs:comment "A measurement related to inversion tamper (Note: typically a count of inversions)" ;
                                     rdfs:label "inversionTamper" .


:MeasurementKind-Old.ipAddress uml:hasInitialValue "107" ;
                               uml:id "_5F88F15E-4C0D-40f1-A1A0-DADE31C21DE3" ;
                               rdfs:comment "An IP address for the endpoint" ;
                               rdfs:label "ipAddress" .


:MeasurementKind-Old.lineLoss uml:hasInitialValue "31" ;
                              uml:id "_FB72B8D9-6FAF-4954-8D56-0D0240D45FCD" ;
                              rdfs:comment "An energy, power, voltage, or current loss attributed to transmission or distribution line impedance" ;
                              rdfs:label "lineLoss" .


:MeasurementKind-Old.loadInterrupt uml:hasInitialValue "131" ;
                                   uml:id "_32E63FA5-999B-43c8-AFE8-215EB567B122" ;
                                   rdfs:comment "A measurement related to load interruption (Note: typically a load interruption count or measurement of duration)" ;
                                   rdfs:label "loadInterrupt" .


:MeasurementKind-Old.loadShed uml:hasInitialValue "132" ;
                              uml:id "_EAA4F356-D88B-499d-97E1-0D4C62BA2F97" ;
                              rdfs:comment "A measurement related to load shed (Note: typically a load shed count or load shed duration)" ;
                              rdfs:label "loadShed" .


:MeasurementKind-Old.loss uml:hasInitialValue "32" ;
                          uml:id "_F9F5922B-EC74-4245-B68F-5C815A519D64" ;
                          rdfs:comment "A quantity lost due to “technical” reasons (such as line loss) or “non-technical” reasons (such as theft.)" ;
                          rdfs:label "loss" .


:MeasurementKind-Old.macAddress uml:hasInitialValue "108" ;
                                uml:id "_2374A673-05AE-49d9-962B-3C15DFD09664" ;
                                rdfs:comment "A MAC address for the endpoint" ;
                                rdfs:label "macAddress" .


:MeasurementKind-Old.maintenance uml:hasInitialValue "133" ;
                                 uml:id "_1526ABEA-0CCC-4982-A159-7ED127F8F8A7" ;
                                 rdfs:comment "A measurement related to the pending maintenance of equipment" ;
                                 rdfs:label "maintenance" .


:MeasurementKind-Old.mfgAssignedConfigurationID uml:hasInitialValue "109" ;
                                                uml:id "_1E4E20E3-B637-4aa4-ABA0-AA17F8C791DE" ;
                                                rdfs:comment "The configuration given to a device at time of manufacture" ;
                                                rdfs:label "mfgAssignedConfigurationID" .


:MeasurementKind-Old.mfgAssignedPhysicalSerialNumber uml:hasInitialValue "110" ;
                                                     uml:id "_FD54DCB6-CBF2-46c6-A6AE-896BCD7C9336" ;
                                                     rdfs:comment "The serial number assigned to a device at time of manufacture" ;
                                                     rdfs:label "mfgAssignedPhysicalSerialNumber" .


:MeasurementKind-Old.mfgAssignedProductNumber uml:hasInitialValue "111" ;
                                              uml:id "_EA5C93C2-4DBD-4d1b-879C-8C298CE72652" ;
                                              rdfs:comment "The product number assigned to a device at time of manufacture" ;
                                              rdfs:label "mfgAssignedProductNumber" .


:MeasurementKind-Old.mfgAssignedUniqueCommunicationAddress uml:hasInitialValue "112" ;
                                                           uml:id "_7E1B0F06-FDFD-4439-BA1A-2370A74606DC" ;
                                                           rdfs:comment "A communication address assigned to a device at time of manufacture" ;
                                                           rdfs:label "mfgAssignedUniqueCommunicationAddress" .


:MeasurementKind-Old.multiCastAddress uml:hasInitialValue "113" ;
                                      uml:id "_F1B90ACC-27EF-41bd-A74F-EC3979D978B0" ;
                                      rdfs:comment "A message target address implying a large group of endpoint units within range of a particular sender" ;
                                      rdfs:label "multiCastAddress" .


:MeasurementKind-Old.negativeSequence uml:hasInitialValue "33" ;
                                      uml:id "_CFBBC6FE-34D2-4f80-84C0-086892621114" ;
                                      rdfs:comment "A quantity that has a rotation sequence which is opposite to that of the power system" ;
                                      rdfs:label "negativeSequence" .


:MeasurementKind-Old.none uml:hasInitialValue "0" ;
                          uml:id "_08F0E83B-C7C3-45d3-B46F-A19160432454" ;
                          rdfs:comment "Not Applicable" ;
                          rdfs:label "none" .


:MeasurementKind-Old.oneWayAddress uml:hasInitialValue "114" ;
                                   uml:id "_4ED4C6B9-28AE-4576-908C-B27BF2C81D5A" ;
                                   rdfs:comment "A communication address of a network endpoint used in one-way communication" ;
                                   rdfs:label "oneWayAddress" .


:MeasurementKind-Old.phasorPowerFactor uml:hasInitialValue "34" ;
                                       uml:id "_497C2B1B-EB0D-449d-8474-7D516E4BBF25" ;
                                       rdfs:comment "The ratio of real energy (usually net Wh) to phasor apparent energy (kVAh)" ;
                                       rdfs:label "phasorPowerFactor" .


:MeasurementKind-Old.phasorReactivePower uml:hasInitialValue "35" ;
                                         uml:id "_2F0A4A03-955A-406c-9C6A-C0BB3D471FEA" ;
                                         rdfs:comment "The ratio of real energy (usually net Wh) to phasor reactive energy (kVAh)" ;
                                         rdfs:label "phasorReactivePower" .


:MeasurementKind-Old.physicalTamper uml:hasInitialValue "134" ;
                                    uml:id "_3BEFBA44-D4E9-4020-91DE-3A0C5A4961FE" ;
                                    rdfs:comment "A measurement related to physical tampering (Note: typically a tamper count)" ;
                                    rdfs:label "physicalTamper" .


:MeasurementKind-Old.positiveSequence uml:hasInitialValue "36" ;
                                      uml:id "_79AE04D2-30E7-4122-89CA-1E776144BA5E" ;
                                      rdfs:comment "A quantity that has a rotation sequence in agreement with that of the power system" ;
                                      rdfs:label "positiveSequence" .


:MeasurementKind-Old.power uml:hasInitialValue "37" ;
                           uml:id "_4F755EEA-2CE5-4085-A47E-6031ACAECBB6" ;
                           rdfs:comment "The derivative of energy with respect to time, where the energy is being transferred or transformed." ;
                           rdfs:label "power" .


:MeasurementKind-Old.powerFactor uml:hasInitialValue "38" ;
                                 uml:id "_A36B46E7-C148-494c-B8E0-55AE972ABA38" ;
                                 rdfs:comment "The ratio of real energy (usually net Wh) to apparent energy (kVAh)" ;
                                 rdfs:label "powerFactor" .


:MeasurementKind-Old.powerLossTamper uml:hasInitialValue "135" ;
                                     uml:id "_8DFE2BC4-015A-4b7d-8919-88CE4C0E788C" ;
                                     rdfs:comment "Tamper indicated while power was out" ;
                                     rdfs:label "powerLossTamper" .


:MeasurementKind-Old.powerOutage uml:hasInitialValue "136" ;
                                 uml:id "_A38D0D4E-AC6B-4ed4-BD67-98FB5201D0CF" ;
                                 rdfs:comment "A measurement related to power outages (Note: typically a status)" ;
                                 rdfs:label "powerOutage" .


:MeasurementKind-Old.powerQuality uml:hasInitialValue "137" ;
                                  uml:id "_F1ACB75A-5E8A-4352-B741-BE5E02F420E1" ;
                                  rdfs:comment "A measurement related to power quality" ;
                                  rdfs:label "powerQuality" .


:MeasurementKind-Old.powerRestoration uml:hasInitialValue "138" ;
                                      uml:id "_93D99A01-63DB-45da-9F13-2E0A89EA8CC1" ;
                                      rdfs:comment "A measurement related to power restoration (Note: typically a status)" ;
                                      rdfs:label "powerRestoration" .


:MeasurementKind-Old.programmed uml:hasInitialValue "139" ;
                                uml:id "_83720109-5466-43cc-A456-17F0700AB395" ;
                                rdfs:comment "A measurement related to device programming (Note: typically a status measurement)" ;
                                rdfs:label "programmed" .


:MeasurementKind-Old.pushbutton uml:hasInitialValue "140" ;
                                uml:id "_225B66FD-C137-49ec-B03D-BF758C15B4AE" ;
                                rdfs:comment "A measurement related to pushbutton (Note: typically a status or count)" ;
                                rdfs:label "pushbutton" .


:MeasurementKind-Old.quantityPower uml:hasInitialValue "40" ;
                                   uml:id "_836F9982-399A-4657-B030-E845F9959C8E" ;
                                   rdfs:comment "A power measurement of Qh, where Qh is defined to be half of the sum of the Wh measurements on each phase plus the squareroot of 3 over two times the sum of the VArh measurements on each phase." ;
                                   rdfs:label "quantityPower" .


:MeasurementKind-Old.relayActivation uml:hasInitialValue "141" ;
                                     uml:id "_847F3395-2761-4e1c-B775-10CA6E9A6EFE" ;
                                     rdfs:comment "A measurement related to relay activations" ;
                                     rdfs:label "relayActivation" .


:MeasurementKind-Old.relayCycle uml:hasInitialValue "142" ;
                                uml:id "_A1CF7FB7-0C24-4093-95F0-3D813686C26A" ;
                                rdfs:comment "A measurement related to relay cycling (Note1: one open and one closure together is one cycle, Note2: Usually expressed as a count)" ;
                                rdfs:label "relayCycle" .


:MeasurementKind-Old.removalTamper uml:hasInitialValue "143" ;
                                   uml:id "_42178AE0-F862-4315-A705-52E6F54CC351" ;
                                   rdfs:comment "An indication of equipment tampering that shows equipment was moved or opened" ;
                                   rdfs:label "removalTamper" .


:MeasurementKind-Old.reprogrammingTamper uml:hasInitialValue "144" ;
                                         uml:id "_6A50557B-1EF4-46cd-9527-174E9E8CB98A" ;
                                         rdfs:comment "An indication of equipment tampering that shows equipment has been reprogrammed" ;
                                         rdfs:label "reprogrammingTamper" .


:MeasurementKind-Old.reverseRotationTamper uml:hasInitialValue "145" ;
                                           uml:id "_BAF309EF-8871-4047-8194-AF1B6F4E364C" ;
                                           rdfs:comment "An indication of tampering as evidenced by reverse power flow" ;
                                           rdfs:label "reverseRotationTamper" .


:MeasurementKind-Old.sag uml:hasInitialValue "41" ;
                         uml:id "_4B3C1891-0C67-4dea-89D5-EA1BA53758DA" ;
                         rdfs:comment "A temporary dip in the supply voltage below the nominal value" ;
                         rdfs:label "sag" .


:MeasurementKind-Old.signalStrength uml:hasInitialValue "115" ;
                                    uml:id "_EE19117A-B381-477f-B63E-5FB1C3784933" ;
                                    rdfs:comment "A measurement of RF signal strength" ;
                                    rdfs:label "signalStrength" .


:MeasurementKind-Old.signaltoNoiseRatio uml:hasInitialValue "117" ;
                                        uml:id "_A8E6E355-7E78-4ce0-982D-173BBC6F5D04" ;
                                        rdfs:comment "A measurement of received (RF) signal strength divided by the (RF) noise floor" ;
                                        rdfs:label "signaltoNoiseRatio" .


:MeasurementKind-Old.swell uml:hasInitialValue "42" ;
                           uml:id "_4EB7228B-B195-4897-8C22-29C329B79B75" ;
                           rdfs:comment "A temporary rise of the supply voltage over the nominal value" ;
                           rdfs:label "swell" .


:MeasurementKind-Old.switchArmed uml:hasInitialValue "146" ;
                                 uml:id "_3D054223-C66E-412f-AF1A-C0C214B70936" ;
                                 rdfs:comment "A measurement of the switch arm condition" ;
                                 rdfs:label "switchArmed" .


:MeasurementKind-Old.switchDisabled uml:hasInitialValue "147" ;
                                    uml:id "_FA6FD67C-7718-49b0-9556-FB8AB442F95C" ;
                                    rdfs:comment "A measurement of the switch enablement status" ;
                                    rdfs:label "switchDisabled" .


:MeasurementKind-Old.switchPosition uml:hasInitialValue "43" ;
                                    uml:id "_AE71D007-449C-4e08-A840-0ED91B612F21" ;
                                    rdfs:comment "A physical or logical switch position status which includes “opened” and “closed”, but for some products may also include “armed,” or other states that indicate a temporary state due to some condition." ;
                                    rdfs:label "switchPosition" .


:MeasurementKind-Old.tamper uml:hasInitialValue "148" ;
                            uml:id "_E94034CD-5049-4d3a-AACB-D4A1DD69E48F" ;
                            rdfs:comment "An indication of equipment tampering" ;
                            rdfs:label "tamper" .


:MeasurementKind-Old.tapPosition uml:hasInitialValue "44" ;
                                 uml:id "_BE3A7871-BBAB-4062-ABB0-FE57ED94653F" ;
                                 rdfs:comment "Tap changer position" ;
                                 rdfs:label "tapPosition" .


:MeasurementKind-Old.tariffRate uml:hasInitialValue "45" ;
                                uml:id "_EAFE4042-BFDC-47ec-9C60-30BB5D78A381" ;
                                rdfs:comment "An energy price defined in a contract. The rate might be a price for energy, for power (usually expressed as a demand value), or some other measurement. The rate might be currency based, or as a code, or as a component of a larger tariff description." ;
                                rdfs:label "tariffRate" .


:MeasurementKind-Old.temperature uml:hasInitialValue "46" ;
                                 uml:id "_96B51394-477A-4c12-AEFB-CAE77B9548EB" ;
                                 rdfs:comment "A quantity proportional to the energy of a system" ;
                                 rdfs:label "temperature" .


:MeasurementKind-Old.totalHarmonicDistortion uml:hasInitialValue "47" ;
                                             uml:id "_86060EB8-E954-408c-917E-ACF92BECA2F5" ;
                                             rdfs:comment "The ratio of the sum of the harmonics to the fundamental. (THD may measure either voltage or current, and may isolated to a given phase)" ;
                                             rdfs:label "totalHarmonicDistortion" .


:MeasurementKind-Old.transformerLoss uml:hasInitialValue "48" ;
                                     uml:id "_55CD35FD-5292-48a6-BEDC-7FC2B44516EC" ;
                                     rdfs:comment "A measurement of the energy or power loss in a transformer due to inefficiency" ;
                                     rdfs:label "transformerLoss" .


:MeasurementKind-Old.twoWayAddress uml:hasInitialValue "116" ;
                                   uml:id "_6CE82411-9D77-484a-AB61-7900A0544532" ;
                                   rdfs:comment "A communication address used for bidirectional communication" ;
                                   rdfs:label "twoWayAddress" .


:MeasurementKind-Old.unipedeVoltageDip10to15 uml:hasInitialValue "49" ;
                                             uml:id "_05F37E9F-82E8-45b7-B3D1-38246D9A25BB" ;
                                             rdfs:comment "A voltage dip classification per EN50160 or a similar national standard measuring the number of dips in the 10-15% range" ;
                                             rdfs:label "unipedeVoltageDip10to15" .


:MeasurementKind-Old.unipedeVoltageDip15to30 uml:hasInitialValue "50" ;
                                             uml:id "_A4088A97-7701-47cc-B208-D68B7B3A2406" ;
                                             rdfs:comment "A voltage dip classification per EN50160 or a similar national standard measuring the number of dips in the 15-30% range" ;
                                             rdfs:label "unipedeVoltageDip15to30" .


:MeasurementKind-Old.unipedeVoltageDip30to60 uml:hasInitialValue "51" ;
                                             uml:id "_62751B85-7EA7-4cc8-B7FA-DAFF2A55C626" ;
                                             rdfs:comment "A voltage dip classification per EN50160 or a similar national standard measuring the number of dips in the 30-60% range" ;
                                             rdfs:label "unipedeVoltageDip30to60" .


:MeasurementKind-Old.unipedeVoltageDip60to90 uml:hasInitialValue "52" ;
                                             uml:id "_49865D9B-5D7F-4623-881A-93445FE35A36" ;
                                             rdfs:comment "A voltage dip classification per EN50160 or a similar national standard measuring the number of dips in the 60-90% rangeA voltage dip classification per EN50160 or a similar national standard measuring the number of dips in the 60-90% range" ;
                                             rdfs:label "unipedeVoltageDip60to90" .


:MeasurementKind-Old.unipedeVoltageDip90to100 uml:hasInitialValue "53" ;
                                              uml:id "_711CBD95-4440-4c92-AB0E-B9A44CDBEF3D" ;
                                              rdfs:comment "A voltage dip classification per EN50160 or a similar national standard measuring the number of dips in the 90-100% range" ;
                                              rdfs:label "unipedeVoltageDip90to100" .


:MeasurementKind-Old.voltage uml:hasInitialValue "54" ;
                             uml:id "_0524E69D-0003-4c31-A82C-E11FA10A0109" ;
                             rdfs:comment "The difference in electric potential between two points" ;
                             rdfs:label "voltage" .


:MeasurementKind-Old.voltageAngle uml:hasInitialValue "55" ;
                                  uml:id "_54917B63-C018-4cb8-8101-17108C7F7772" ;
                                  rdfs:comment "A phase voltage zerocross timing measurement relative to a reference voltage zerocross" ;
                                  rdfs:label "voltageAngle" .


:MeasurementKind-Old.voltageExcursion uml:hasInitialValue "56" ;
                                      uml:id "_BA724B94-B323-45d7-A699-015DDB29D6DE" ;
                                      rdfs:comment "A measurement of the departure of the voltage from the nominal voltage" ;
                                      rdfs:label "voltageExcursion" .


:MeasurementKind-Old.voltageImbalance uml:hasInitialValue "57" ;
                                      uml:id "_0C05B252-7E96-4e6e-ABD4-C77E920268F1" ;
                                      rdfs:comment "A measurement of the departure of a phase voltage relative to the average voltage of all phases." ;
                                      rdfs:label "voltageImbalance" .


:MeasurementKind-Old.volume uml:hasInitialValue "58" ;
                            uml:id "_9DCEADE6-0346-44a4-BFF4-3D74A81B7CD4" ;
                            rdfs:comment "fluid volume" ;
                            rdfs:label "volume" .


:MeasurementKind-Old.volumetricFlow uml:hasInitialValue "155" ;
                                    uml:id "_32B0BB6B-0A25-41aa-87AC-CC6B38E3C6F5" ;
                                    rdfs:comment "A fluid flow rate" ;
                                    rdfs:label "volumetricFlow" .


:MeasurementKind-Old.watchdogTimeout uml:hasInitialValue "149" ;
                                     uml:id "_E1540CF3-7AA7-446f-9664-3BE5E88272B1" ;
                                     rdfs:comment "A reset triggered by a hardware “watchdog” circuit" ;
                                     rdfs:label "watchdogTimeout" .


:MeasurementKind-Old.zeroFlowDuration uml:hasInitialValue "59" ;
                                      uml:id "_A3ED4F79-4357-43ba-9951-8F8FD7C35BDA" ;
                                      rdfs:comment "The amount of time that current flow drops to a zero level or level below the ability of the sensor to sense" ;
                                      rdfs:label "zeroFlowDuration" .


:MeasurementKind-Old.zeroSequence uml:hasInitialValue "60" ;
                                  uml:id "_9789087D-2349-44a8-AF4A-BBF29AA19EFA" ;
                                  rdfs:comment "The zero sequence current is the vector sum of the phase currents" ;
                                  rdfs:label "zeroSequence" .


:MeasurementKind.alarm uml:hasInitialValue "118" ;
                       uml:id "_D32DC4BC-02FA-43d4-9DE0-87E785613089" ;
                       rdfs:comment "A measurement related to an alarm" ;
                       rdfs:label "alarm" .


:MeasurementKind.apTitle uml:hasInitialValue "91" ;
                         uml:id "_D17C0D61-D81A-44c0-A8F9-B0EAC52D9D1D" ;
                         rdfs:comment "An application name which is making or has made a request" ;
                         rdfs:label "apTitle" .


:MeasurementKind.apparentPowerFactor uml:hasInitialValue "2" ;
                                     uml:id "_332C806F-5FEA-4876-B2D0-1E2B2EDFCB7E" ;
                                     rdfs:comment "The ratio of real energy (usually net Wh) to apparent energy (kVAh)" ;
                                     rdfs:label "apparentPowerFactor" .


:MeasurementKind.applicationContext uml:hasInitialValue "90" ;
                                    uml:id "_448CCEE3-D58E-4520-A409-C58602442331" ;
                                    rdfs:comment "Information that describes the logical context in which a request, measurement, or command is made." ;
                                    rdfs:label "applicationContext" .


:MeasurementKind.assetNumber uml:hasInitialValue "92" ;
                             uml:id "_3E23139F-3E37-42db-A779-4486E528D920" ;
                             rdfs:comment "An asset identifier" ;
                             rdfs:label "assetNumber" .


:MeasurementKind.audibleVolume uml:hasInitialValue "154" ;
                               uml:id "_8F833E6C-A268-49c4-8BEF-E8B4589C6A52" ;
                               rdfs:comment "Sound" ;
                               rdfs:label "audibleVolume" .


:MeasurementKind.bandwidth uml:hasInitialValue "93" ;
                           uml:id "_A6BC0D5B-1EEC-43a6-8B3D-1649B14BA4ED" ;
                           rdfs:comment "A measurement of dataflow" ;
                           rdfs:label "bandwidth" .


:MeasurementKind.batteryCarryover uml:hasInitialValue "119" ;
                                  uml:id "_AA4E5B98-C924-4e18-BF6F-73263ACD023C" ;
                                  rdfs:comment "An estimate of the battery ride through capacity" ;
                                  rdfs:label "batteryCarryover" .


:MeasurementKind.batteryVoltage uml:hasInitialValue "94" ;
                                uml:id "_3CB1ACC9-0257-4307-81B5-90B489EF52AF" ;
                                rdfs:comment "Battery voltage" ;
                                rdfs:label "batteryVoltage" .


:MeasurementKind.billCarryover uml:hasInitialValue "152" ;
                               uml:id "_E6F8CEEB-DFFE-48a9-8783-220911A848BF" ;
                               rdfs:comment "Customer’s bill for the (Currency)" ;
                               rdfs:label "billCarryover" .


:MeasurementKind.billLastPeriod uml:hasInitialValue "150" ;
                                uml:id "_1D0E0160-B201-40e5-A351-BEABB8B37A79" ;
                                rdfs:comment "Customer’s bill for the previous billing period (Currency)" ;
                                rdfs:label "billLastPeriod" .


:MeasurementKind.billToDate uml:hasInitialValue "151" ;
                            uml:id "_BDB5188F-21E7-40a9-9599-2D48508441AE" ;
                            rdfs:comment "Customer’s bill, as known thus far within the present billing period (Currency)" ;
                            rdfs:label "billToDate" .


:MeasurementKind.broadcastAddress uml:hasInitialValue "95" ;
                                  uml:id "_50E0511B-A8B7-4392-A393-D217C369F4F4" ;
                                  rdfs:comment "A message target address implying all endpoint units within range of a particular sender" ;
                                  rdfs:label "broadcastAddress" .


:MeasurementKind.connectionFee uml:hasInitialValue "153" ;
                               uml:id "_143ED7A9-05BD-46c9-89E3-9B9841821A0C" ;
                               rdfs:comment "Monthly fee for connection to commodity." ;
                               rdfs:label "connectionFee" .


:MeasurementKind.currency uml:hasInitialValue "3" ;
                          uml:id "_4D44C69B-20C4-4ef6-B900-4B06DD34B4B6" ;
                          rdfs:comment "funds" ;
                          rdfs:label "currency" .


:MeasurementKind.current uml:hasInitialValue "4" ;
                         uml:id "_2DBF1AC5-CFDF-48ff-AD49-42DB977742A3" ;
                         rdfs:comment "The flow of electrons" ;
                         rdfs:label "current" .


:MeasurementKind.currentAngle uml:hasInitialValue "5" ;
                              uml:id "_FAAD09FA-2DFE-4b99-97F5-4ACC4FDA2B4A" ;
                              rdfs:comment "A phase current zerocross timing measurement releative to a reference voltage zerocross" ;
                              rdfs:label "currentAngle" .


:MeasurementKind.currentImbalance uml:hasInitialValue "6" ;
                                  uml:id "_D2A0A528-9CF0-4309-82D8-119179C79700" ;
                                  rdfs:comment "A measurement of the departure of a phase current relative to the average current of all phases" ;
                                  rdfs:label "currentImbalance" .


:MeasurementKind.dataOverflowAlarm uml:hasInitialValue "120" ;
                                   uml:id "_AAC6CB70-C3AC-487f-8492-12E0A30AC807" ;
                                   rdfs:comment "An indication of or measurement of a loss of data" ;
                                   rdfs:label "dataOverflowAlarm" .


:MeasurementKind.date uml:hasInitialValue "7" ;
                      uml:id "_58910ACA-8C45-43e8-8FF3-113D18DA33C6" ;
                      rdfs:comment "A measurement of the date and/or time in a clock, or a time stamp indicating when data was captured, when a maximum or minimum occurred, or to commemorate some other important aspect of a measurement" ;
                      rdfs:label "date" .


:MeasurementKind.demand uml:hasInitialValue "8" ;
                        uml:id "_B623A543-24D7-4131-8B77-620BEE0E9EBC" ;
                        rdfs:comment "The measurement of maximum power flow which is computed as energy usage over time, the dimensions of which are defined by a tariff" ;
                        rdfs:label "demand" .


:MeasurementKind.demandLimit uml:hasInitialValue "121" ;
                             uml:id "_1447A684-D06C-4a76-997F-710C9B357AAE" ;
                             rdfs:comment "A threshold setting that determines the trip point that if exceeded would trigger a demand limiting action or alarm" ;
                             rdfs:label "demandLimit" .


:MeasurementKind.demandReset uml:hasInitialValue "122" ;
                             uml:id "_1FB13730-9463-4156-B48B-E50DFE6ACA15" ;
                             rdfs:comment "A count of the number of times demand has been reset (remotely, locally, and/or automatically.)" ;
                             rdfs:label "demandReset" .


:MeasurementKind.deviceAddressType1 uml:hasInitialValue "96" ;
                                    uml:id "_7AAEB292-79F8-48dd-BB70-2375E3118645" ;
                                    rdfs:comment "Endpoint target address Type1" ;
                                    rdfs:label "deviceAddressType1" .


:MeasurementKind.deviceAddressType2 uml:hasInitialValue "97" ;
                                    uml:id "_5B50C60C-43F5-4203-BE99-4298D62BF1BB" ;
                                    rdfs:comment "Endpoint target address Type2" ;
                                    rdfs:label "deviceAddressType2" .


:MeasurementKind.deviceAddressType3 uml:hasInitialValue "98" ;
                                    uml:id "_3A7CC033-0FC9-4740-B81F-697DD63E9286" ;
                                    rdfs:comment "Endpoint target address Type3" ;
                                    rdfs:label "deviceAddressType3" .


:MeasurementKind.deviceAddressType4 uml:hasInitialValue "99" ;
                                    uml:id "_55741C62-4803-4c54-A988-C560FEDE72D2" ;
                                    rdfs:comment "Endpoint target address Type4" ;
                                    rdfs:label "deviceAddressType4" .


:MeasurementKind.deviceClass uml:hasInitialValue "100" ;
                             uml:id "_47AE570D-9EFF-4ee4-BEA7-F0CB1695EB8B" ;
                             rdfs:comment "A unique identifier for the Endpoint’s configuration" ;
                             rdfs:label "deviceClass" .


:MeasurementKind.diagnostic uml:hasInitialValue "123" ;
                            uml:id "_B2B45200-7882-4a7d-84EA-D24E9F5E448C" ;
                            rdfs:comment "A measurement related to equipment diagnostics" ;
                            rdfs:label "diagnostic" .


:MeasurementKind.distance uml:hasInitialValue "9" ;
                          uml:id "_141C9F04-2B61-49cf-B1D2-6285E608C46C" ;
                          rdfs:comment "A linear distance or range radius" ;
                          rdfs:label "distance" .


:MeasurementKind.distortionPowerFactor uml:hasInitialValue "64" ;
                                       uml:id "_7C23883A-BE32-4dff-BA9D-41A60218ED40" ;
                                       rdfs:comment "The ratio of the distortion VAh to the apparent VAh" ;
                                       rdfs:label "distortionPowerFactor" .


:MeasurementKind.distortionVoltAmp uml:hasInitialValue "10" ;
                                   uml:id "_359E3726-E5D7-4a8b-B426-82F2DA4EDF29" ;
                                   rdfs:comment "A measurement in which a V<sup>2</sup> I<sup>2</sup> term has both real and reactive components removed leaving only distortion. For example, distortion VAh = Sqrt( (V<sup>2</sup>h)(I<sup>2</sup>h) – (Wh)<sup>2</sup> – (VArh)<sup>2</sup>)" ;
                                   rdfs:label "distortionVoltAmp" .


:MeasurementKind.electronicSerialNumber uml:hasInitialValue "101" ;
                                        uml:id "_EF2BDD35-9A5D-473e-B089-B4AD7F1AD5FB" ;
                                        rdfs:comment "A device serial number" ;
                                        rdfs:label "electronicSerialNumber" .


:MeasurementKind.emergencyLimit uml:hasInitialValue "124" ;
                                uml:id "_DED9D37F-CD65-4664-8DEB-649FA72878AF" ;
                                rdfs:comment "A setting that indicates an emergency limit" ;
                                rdfs:label "emergencyLimit" .


:MeasurementKind.encoderTamper uml:hasInitialValue "125" ;
                               uml:id "_7A0D0649-AAB0-4509-85D7-823F5026B7FB" ;
                               rdfs:comment "An indication of tampering with a meter encoder" ;
                               rdfs:label "encoderTamper" .


:MeasurementKind.endDeviceID uml:hasInitialValue "102" ;
                             uml:id "_8CA9C488-13FE-48a3-BA1A-CC7D323A5D43" ;
                             rdfs:comment "A unique identifier of the endDevice – the device providing measurements or under control of the network" ;
                             rdfs:label "endDeviceID" .


:MeasurementKind.energization uml:hasInitialValue "11" ;
                              uml:id "_C03EE2F4-363B-4c64-8C54-FBAACBBB92FA" ;
                              rdfs:comment "Pertaining to the presence of voltage" ;
                              rdfs:label "energization" .


:MeasurementKind.energizationLoadSide uml:hasInitialValue "13" ;
                                      uml:id "_33D486F1-78DE-48ac-9451-0AE77B614DBF" ;
                                      rdfs:comment "Measuring the presence or absence of voltage on the load side of an electricity meter" ;
                                      rdfs:label "energizationLoadSide" .


:MeasurementKind.energy uml:hasInitialValue "12" ;
                        uml:id "_EA45E289-4D08-4881-B24B-2CB23C387A8C" ;
                        rdfs:comment "Scalar quantity which may be increased or decreased in a system when it receives or produces work, respectively" ;
                        rdfs:label "energy" .


:MeasurementKind.fan uml:hasInitialValue "14" ;
                     uml:id "_D6CE215D-13CC-4b97-8B24-1985A5FFFF03" ;
                     rdfs:comment "A forced air moving device" ;
                     rdfs:label "fan" .


:MeasurementKind.frequency uml:hasInitialValue "15" ;
                           uml:id "_F4A6BFD3-63D1-4eb8-88F7-127E41CD1343" ;
                           rdfs:comment "Reciprocal of the period" ;
                           rdfs:label "frequency" .


:MeasurementKind.frequencyExcursion uml:hasInitialValue "81" ;
                                    uml:id "_29543891-1038-4b1c-90C4-CE2D6C439B1C" ;
                                    rdfs:comment "A measurement of the departure of the frequency from the nominal frequency" ;
                                    rdfs:label "frequencyExcursion" .


:MeasurementKind.fund uml:hasInitialValue "16" ;
                      uml:id "_C208959B-931E-40a1-ABE6-FA54B8AE50C1" ;
                      rdfs:comment "Duplicate with “currency”" ;
                      rdfs:label "fund" .


:MeasurementKind.groupAddressType1 uml:hasInitialValue "103" ;
                                   uml:id "_AFC31615-DD48-4f48-98D1-F74298A9000E" ;
                                   rdfs:comment "Group target address Type1" ;
                                   rdfs:label "groupAddressType1" .


:MeasurementKind.groupAddressType2 uml:hasInitialValue "104" ;
                                   uml:id "_BF1D614C-3C8C-4f90-8CA5-6CD6B3053D13" ;
                                   rdfs:comment "Group target address Type2" ;
                                   rdfs:label "groupAddressType2" .


:MeasurementKind.groupAddressType3 uml:hasInitialValue "105" ;
                                   uml:id "_47957668-BD85-46be-9E41-22F7A0872522" ;
                                   rdfs:comment "Group target address Type3" ;
                                   rdfs:label "groupAddressType3" .


:MeasurementKind.groupAddressType4 uml:hasInitialValue "106" ;
                                   uml:id "_39871014-B296-4208-81FC-235CAC4A7BBA" ;
                                   rdfs:comment "Group target address Type4" ;
                                   rdfs:label "groupAddressType4" .


:MeasurementKind.ieee1366ASAI uml:hasInitialValue "17" ;
                              uml:id "_679F87B9-672D-4b71-9DE0-4A58B117EFAE" ;
                              rdfs:comment "A measurement of IEEE-1366 Average Service Availability Index" ;
                              rdfs:label "ieee1366ASAI" .


:MeasurementKind.ieee1366ASIDI uml:hasInitialValue "18" ;
                               uml:id "_D28E0CDD-241A-4c1e-AFB7-78D11B9A14CB" ;
                               rdfs:comment "A measurement of the IEEE-1366 Average Service Interruption Duration Index" ;
                               rdfs:label "ieee1366ASIDI" .


:MeasurementKind.ieee1366ASIFI uml:hasInitialValue "19" ;
                               uml:id "_2D9C0562-147A-455b-891C-C03C954291C5" ;
                               rdfs:comment "A measurement of the IEEE-1366 Average Service Interruption Frequency Index" ;
                               rdfs:label "ieee1366ASIFI" .


:MeasurementKind.ieee1366CAIDI uml:hasInitialValue "20" ;
                               uml:id "_07D8D38B-8034-45aa-A26A-E182CF68B0D7" ;
                               rdfs:comment "A measurement of the IEEE-1366 Customer average interruption duration index" ;
                               rdfs:label "ieee1366CAIDI" .


:MeasurementKind.ieee1366CAIFI uml:hasInitialValue "21" ;
                               uml:id "_05B5CABA-15B4-46a0-86D1-E836395221BD" ;
                               rdfs:comment "A measurement of the IEEE-1366 Customer average interruption frequency index" ;
                               rdfs:label "ieee1366CAIFI" .


:MeasurementKind.ieee1366CEMIn uml:hasInitialValue "22" ;
                               uml:id "_3669B68B-8796-4d93-8A36-DBC0287289DA" ;
                               rdfs:comment "A measurement of the IEEE-1366 Customers Experiencing Multiple Interruptions" ;
                               rdfs:label "ieee1366CEMIn" .


:MeasurementKind.ieee1366CEMSMIn uml:hasInitialValue "23" ;
                                 uml:id "_6DC129C7-B611-4905-89DC-E13AB77689B5" ;
                                 rdfs:comment "A measurement of the IEEE-1366 Customers Experiencing Multiple Sustained and Momentary Interruptions" ;
                                 rdfs:label "ieee1366CEMSMIn" .


:MeasurementKind.ieee1366CTAIDI uml:hasInitialValue "24" ;
                                uml:id "_2ADB0562-75FC-4a0f-BF00-C5B722A75F25" ;
                                rdfs:comment "A measurement of the IEEE-1366 Customer Total Average Interruption Duration Index" ;
                                rdfs:label "ieee1366CTAIDI" .


:MeasurementKind.ieee1366MAIFI uml:hasInitialValue "25" ;
                               uml:id "_B838FCE1-2F54-4e6b-81AE-B2C8A506C151" ;
                               rdfs:comment "A measurement of the IEEE-1366 Momentary Average Interruption Frequency Index" ;
                               rdfs:label "ieee1366MAIFI" .


:MeasurementKind.ieee1366MAIFIe uml:hasInitialValue "26" ;
                                uml:id "_1CA8B83B-C845-410e-85DB-69079E33FD5F" ;
                                rdfs:comment "A measurement of the IEEE-1366 Momentary Average event Interruption Frequency Index" ;
                                rdfs:label "ieee1366MAIFIe" .


:MeasurementKind.ieee1366MomentaryInterruption uml:hasInitialValue "126" ;
                                               uml:id "_E7108C59-F66C-4307-A64D-CB3D7BA8A906" ;
                                               rdfs:comment "IEEE-1366 Momentary Interruption count" ;
                                               rdfs:label "ieee1366MomentaryInterruption" .


:MeasurementKind.ieee1366MomentaryInterruptionEvent uml:hasInitialValue "127" ;
                                                    uml:id "_518B6C7F-1148-46b3-8D16-522E2F8DF3D1" ;
                                                    rdfs:comment "IEEE-1366 Momentary Interruption event count" ;
                                                    rdfs:label "ieee1366MomentaryInterruptionEvent" .


:MeasurementKind.ieee1366SAIDI uml:hasInitialValue "27" ;
                               uml:id "_7997359A-3628-4b27-B09C-3ECF48158018" ;
                               rdfs:comment "IEEE-1366 System Average Interruption Duration Index" ;
                               rdfs:label "ieee1366SAIDI" .


:MeasurementKind.ieee1366SAIFI uml:hasInitialValue "28" ;
                               uml:id "_800FA18F-FB1F-4bec-B245-600B21A06632" ;
                               rdfs:comment "IEEE-1366 System Average Interruption Frequency Index" ;
                               rdfs:label "ieee1366SAIFI" .


:MeasurementKind.ieee1366SustainedInterruption uml:hasInitialValue "128" ;
                                               uml:id "_F36865D9-D5A0-4a99-B428-194C0F646BEE" ;
                                               rdfs:comment "IEEE-1366 Sustained Interruption duration" ;
                                               rdfs:label "ieee1366SustainedInterruption" .


:MeasurementKind.interruptionBehaviour uml:hasInitialValue "129" ;
                                       uml:id "_0E076338-B0E2-442b-B9E0-2F1DE33CEE0A" ;
                                       rdfs:comment "A measurement related to power interruptions (Note: often an interruption count or duration.)" ;
                                       rdfs:label "interruptionBehaviour" .


:MeasurementKind.inversionTamper uml:hasInitialValue "130" ;
                                 uml:id "_4AC407A1-3EA6-4973-90EB-56E83C07BFAE" ;
                                 rdfs:comment "A measurement related to inversion tamper (Note: typically a count of inversions)" ;
                                 rdfs:label "inversionTamper" .


:MeasurementKind.ipAddress uml:hasInitialValue "107" ;
                           uml:id "_A576D2C5-4998-4dab-8428-6C87086CD35D" ;
                           rdfs:comment "An IP address for the endpoint" ;
                           rdfs:label "ipAddress" .


:MeasurementKind.lineLoss uml:hasInitialValue "31" ;
                          uml:id "_99A89CDC-2BE5-41c2-82FE-AF4DACD9227F" ;
                          rdfs:comment "An energy, power, voltage, or current loss attributed to transmission or distribution line impedance" ;
                          rdfs:label "lineLoss" .


:MeasurementKind.loadInterrupt uml:hasInitialValue "131" ;
                               uml:id "_FA3BE6A9-B11E-44ce-BD14-00EC0AF12388" ;
                               rdfs:comment "A measurement related to load interruption (Note: typically a load interruption count or measurement of duration)" ;
                               rdfs:label "loadInterrupt" .


:MeasurementKind.loadShed uml:hasInitialValue "132" ;
                          uml:id "_0C378073-D82B-4a7c-B9C8-A5AB44486D64" ;
                          rdfs:comment "A measurement related to load shed (Note: typically a load shed count or load shed duration)" ;
                          rdfs:label "loadShed" .


:MeasurementKind.loss uml:hasInitialValue "32" ;
                      uml:id "_235E70E6-0991-4be0-B251-DB3CB29380A5" ;
                      rdfs:comment "A quantity lost due to “technical” reasons (such as line loss) or “non-technical” reasons (such as theft.)" ;
                      rdfs:label "loss" .


:MeasurementKind.macAddress uml:hasInitialValue "108" ;
                            uml:id "_B41F4768-4893-432c-9741-A4F8765CB6A3" ;
                            rdfs:comment "A MAC address for the endpoint" ;
                            rdfs:label "macAddress" .


:MeasurementKind.maintenance uml:hasInitialValue "133" ;
                             uml:id "_3979DF56-4AAD-4847-9CAC-5373229F0DBD" ;
                             rdfs:comment "A measurement related to the pending maintenance of equipment" ;
                             rdfs:label "maintenance" .


:MeasurementKind.mfgAssignedConfigurationID uml:hasInitialValue "109" ;
                                            uml:id "_95DBFC71-B668-40eb-8B9F-859F76650FD9" ;
                                            rdfs:comment "The configuration given to a device at time of manufacture" ;
                                            rdfs:label "mfgAssignedConfigurationID" .


:MeasurementKind.mfgAssignedPhysicalSerialNumber uml:hasInitialValue "110" ;
                                                 uml:id "_6EC29DA4-8E19-42f1-B23C-B4E55C61BA21" ;
                                                 rdfs:comment "The serial number assigned to a device at time of manufacture" ;
                                                 rdfs:label "mfgAssignedPhysicalSerialNumber" .


:MeasurementKind.mfgAssignedProductNumber uml:hasInitialValue "111" ;
                                          uml:id "_7ED846A8-A288-4a2f-934A-79C9A9510EDA" ;
                                          rdfs:comment "The product number assigned to a device at time of manufacture" ;
                                          rdfs:label "mfgAssignedProductNumber" .


:MeasurementKind.mfgAssignedUniqueCommunicationAddress uml:hasInitialValue "112" ;
                                                       uml:id "_F47AE525-C294-4fa7-91C6-7610412BD94E" ;
                                                       rdfs:comment "A communication address assigned to a device at time of manufacture" ;
                                                       rdfs:label "mfgAssignedUniqueCommunicationAddress" .


:MeasurementKind.multiCastAddress uml:hasInitialValue "113" ;
                                  uml:id "_A62D2617-4D58-4b07-AE3E-AA33248CC99F" ;
                                  rdfs:comment "A message target address implying a large group of endpoint units within range of a particular sender" ;
                                  rdfs:label "multiCastAddress" .


:MeasurementKind.negativeSequence uml:hasInitialValue "33" ;
                                  uml:id "_38445DD5-4319-44ca-927E-79B2FD9D3165" ;
                                  rdfs:comment "A quantity that has a rotation sequence which is opposite to that of the power system" ;
                                  rdfs:label "negativeSequence" .


:MeasurementKind.none uml:hasInitialValue "0" ;
                      uml:id "_4C0BD4D4-AFFC-4ea7-A89E-87336EB05A1C" ;
                      rdfs:comment "Not Applicable" ;
                      rdfs:label "none" .


:MeasurementKind.oneWayAddress uml:hasInitialValue "114" ;
                               uml:id "_6A5222D9-8C8F-43cc-9406-F0770DD44BB4" ;
                               rdfs:comment "A communication address of a network endpoint used in one-way communication" ;
                               rdfs:label "oneWayAddress" .


:MeasurementKind.phasorPowerFactor uml:hasInitialValue "34" ;
                                   uml:id "_1816A65B-775F-43d7-BB41-7B9002F7E72F" ;
                                   rdfs:comment "The ratio of real energy (usually net Wh) to phasor apparent energy (kVAh)" ;
                                   rdfs:label "phasorPowerFactor" .


:MeasurementKind.phasorReactivePower uml:hasInitialValue "35" ;
                                     uml:id "_3242C057-16FB-4651-8549-C80C91609AD2" ;
                                     rdfs:comment "The ratio of real energy (usually net Wh) to phasor reactive energy (kVAh)" ;
                                     rdfs:label "phasorReactivePower" .


:MeasurementKind.physicalTamper uml:hasInitialValue "134" ;
                                uml:id "_520178FB-0673-472e-8C4E-4D06B7DDDC7D" ;
                                rdfs:comment "A measurement related to physical tampering (Note: typically a tamper count)" ;
                                rdfs:label "physicalTamper" .


:MeasurementKind.positiveSequence uml:hasInitialValue "36" ;
                                  uml:id "_B541DEDA-348A-47ff-AFB3-116B15B69420" ;
                                  rdfs:comment "A quantity that has a rotation sequence in agreement with that of the power system" ;
                                  rdfs:label "positiveSequence" .


:MeasurementKind.power uml:hasInitialValue "37" ;
                       uml:id "_AB174BBE-5978-47df-B405-69BB1EDA941B" ;
                       rdfs:comment "The derivative of energy with respect to time, where the energy is being transferred or transformed." ;
                       rdfs:label "power" .


:MeasurementKind.powerFactor uml:hasInitialValue "38" ;
                             uml:id "_E729773A-9EFA-477e-95AA-56EC4185CAFE" ;
                             rdfs:comment "The ratio of real energy (usually net Wh) to apparent energy (kVAh)" ;
                             rdfs:label "powerFactor" .


:MeasurementKind.powerLossTamper uml:hasInitialValue "135" ;
                                 uml:id "_030178D7-9E80-4e8c-B45F-84CE5B781431" ;
                                 rdfs:comment "Tamper indicated while power was out" ;
                                 rdfs:label "powerLossTamper" .


:MeasurementKind.powerOutage uml:hasInitialValue "136" ;
                             uml:id "_48F74079-682C-43c0-9D56-00D9023EA93B" ;
                             rdfs:comment "A measurement related to power outages (Note: typically a status)" ;
                             rdfs:label "powerOutage" .


:MeasurementKind.powerQuality uml:hasInitialValue "137" ;
                              uml:id "_DFE9A103-23B9-45e3-A412-A00D23A7803C" ;
                              rdfs:comment "A measurement related to power quality" ;
                              rdfs:label "powerQuality" .


:MeasurementKind.powerRestoration uml:hasInitialValue "138" ;
                                  uml:id "_13E6C9EA-1916-4e34-99E5-4C5E4DC2126D" ;
                                  rdfs:comment "A measurement related to power restoration (Note: typically a status)" ;
                                  rdfs:label "powerRestoration" .


:MeasurementKind.programmed uml:hasInitialValue "139" ;
                            uml:id "_F61029FA-3E6A-44c9-B98F-B67AF8157829" ;
                            rdfs:comment "A measurement related to device programming (Note: typically a status measurement)" ;
                            rdfs:label "programmed" .


:MeasurementKind.pushbutton uml:hasInitialValue "140" ;
                            uml:id "_9D6C3D97-B79F-4a0c-8313-E175E782ED58" ;
                            rdfs:comment "A measurement related to pushbutton (Note: typically a status or count)" ;
                            rdfs:label "pushbutton" .


:MeasurementKind.quantityPower uml:hasInitialValue "40" ;
                               uml:id "_E99E99B6-4085-448e-88FF-E3C298B0EF9C" ;
                               rdfs:comment "A power measurement of Qh, where Qh is defined to be half of the sum of the Wh measurements on each phase plus the squareroot of 3 over two times the sum of the VArh measurements on each phase." ;
                               rdfs:label "quantityPower" .


:MeasurementKind.relayActivation uml:hasInitialValue "141" ;
                                 uml:id "_4F1F9A22-23F7-4c73-9499-40DC7447F73C" ;
                                 rdfs:comment "A measurement related to relay activations" ;
                                 rdfs:label "relayActivation" .


:MeasurementKind.relayCycle uml:hasInitialValue "142" ;
                            uml:id "_68CA6B16-AF2B-4344-AAEA-66B043F25A48" ;
                            rdfs:comment "A measurement related to relay cycling (Note1: one open and one closure together is one cycle, Note2: Usually expressed as a count)" ;
                            rdfs:label "relayCycle" .


:MeasurementKind.removalTamper uml:hasInitialValue "143" ;
                               uml:id "_23CF4C81-1F2C-4083-8489-C762A6C69969" ;
                               rdfs:comment "An indication of equipment tampering that shows equipment was moved or opened" ;
                               rdfs:label "removalTamper" .


:MeasurementKind.reprogrammingTamper uml:hasInitialValue "144" ;
                                     uml:id "_DE949299-1231-4d10-9225-1A3DCB35E6F0" ;
                                     rdfs:comment "An indication of equipment tampering that shows equipment has been reprogrammed" ;
                                     rdfs:label "reprogrammingTamper" .


:MeasurementKind.reverseRotationTamper uml:hasInitialValue "145" ;
                                       uml:id "_6D9E051E-87EC-47f6-8AEA-098E0473E173" ;
                                       rdfs:comment "An indication of tampering as evidenced by reverse power flow" ;
                                       rdfs:label "reverseRotationTamper" .


:MeasurementKind.sag uml:hasInitialValue "41" ;
                     uml:id "_56A5E1E6-192A-4037-9908-6C9FF4E25F23" ;
                     rdfs:comment "A temporary dip in the supply voltage below the nominal value" ;
                     rdfs:label "sag" .


:MeasurementKind.signalStrength uml:hasInitialValue "115" ;
                                uml:id "_6EC66522-9A9E-4627-9C40-4039C18C1286" ;
                                rdfs:comment "A measurement of RF signal strength" ;
                                rdfs:label "signalStrength" .


:MeasurementKind.signaltoNoiseRatio uml:hasInitialValue "117" ;
                                    uml:id "_E2146344-B0E4-4fc4-B8B5-012D1BDBFEAA" ;
                                    rdfs:comment "A measurement of received (RF) signal strength divided by the (RF) noise floor" ;
                                    rdfs:label "signaltoNoiseRatio" .


:MeasurementKind.swell uml:hasInitialValue "42" ;
                       uml:id "_02576DA4-0B95-4f60-8E54-58BD5666A6A7" ;
                       rdfs:comment "A temporary rise of the supply voltage over the nominal value" ;
                       rdfs:label "swell" .


:MeasurementKind.switchArmed uml:hasInitialValue "146" ;
                             uml:id "_BA5C27F9-EAD7-4107-841E-693275CA84C9" ;
                             rdfs:comment "A measurement of the switch arm condition" ;
                             rdfs:label "switchArmed" .


:MeasurementKind.switchDisabled uml:hasInitialValue "147" ;
                                uml:id "_386C8A1D-1276-44af-A679-DA4277DA55BF" ;
                                rdfs:comment "A measurement of the switch enablement status" ;
                                rdfs:label "switchDisabled" .


:MeasurementKind.switchPosition uml:hasInitialValue "43" ;
                                uml:id "_4B61E2AD-2D85-499f-9F25-A63A66FEDE74" ;
                                rdfs:comment "A physical or logical switch position status which includes “opened” and “closed”, but for some products may also include “armed,” or other states that indicate a temporary state due to some condition." ;
                                rdfs:label "switchPosition" .


:MeasurementKind.tamper uml:hasInitialValue "148" ;
                        uml:id "_7302B137-F855-4f59-A8F2-12B621B480C2" ;
                        rdfs:comment "An indication of equipment tampering" ;
                        rdfs:label "tamper" .


:MeasurementKind.tapPosition uml:hasInitialValue "44" ;
                             uml:id "_9ADCA092-ED69-4e47-9F1C-517A412A00C8" ;
                             rdfs:comment "Tap changer position" ;
                             rdfs:label "tapPosition" .


:MeasurementKind.tariffRate uml:hasInitialValue "45" ;
                            uml:id "_E2983F71-CC21-4587-9C20-59F73A827110" ;
                            rdfs:comment "An energy price defined in a contract. The rate might be a price for energy, for power (usually expressed as a demand value), or some other measurement. The rate might be currency based, or as a code, or as a component of a larger tariff description." ;
                            rdfs:label "tariffRate" .


:MeasurementKind.temperature uml:hasInitialValue "46" ;
                             uml:id "_E5B2F4A0-0784-4002-89C4-B2A309481C9C" ;
                             rdfs:comment "A quantity proportional to the energy of a system" ;
                             rdfs:label "temperature" .


:MeasurementKind.totalHarmonicDistortion uml:hasInitialValue "47" ;
                                         uml:id "_5427FFED-E750-46a3-A5ED-DF1C4A6922EE" ;
                                         rdfs:comment "The ratio of the sum of the harmonics to the fundamental. (THD may measure either voltage or current, and may isolated to a given phase)" ;
                                         rdfs:label "totalHarmonicDistortion" .


:MeasurementKind.transformerLoss uml:hasInitialValue "48" ;
                                 uml:id "_43FD0915-12DA-4c01-BBE2-1F8B931204DA" ;
                                 rdfs:comment "A measurement of the energy or power loss in a transformer due to inefficiency" ;
                                 rdfs:label "transformerLoss" .


:MeasurementKind.twoWayAddress uml:hasInitialValue "116" ;
                               uml:id "_190CEA9A-CE1A-487b-A4E2-71EDCC5C4215" ;
                               rdfs:comment "A communication address used for bidirectional communication" ;
                               rdfs:label "twoWayAddress" .


:MeasurementKind.unipedeVoltageDip10to15 uml:hasInitialValue "49" ;
                                         uml:id "_B46E361A-1053-4730-B1F7-13CEA389C0F3" ;
                                         rdfs:comment "A voltage dip classification per EN50160 or a similar national standard measuring the number of dips in the 10-15% range" ;
                                         rdfs:label "unipedeVoltageDip10to15" .


:MeasurementKind.unipedeVoltageDip15to30 uml:hasInitialValue "50" ;
                                         uml:id "_0FB5517D-3A53-4138-9A78-2CE2F59EC14A" ;
                                         rdfs:comment "A voltage dip classification per EN50160 or a similar national standard measuring the number of dips in the 15-30% range" ;
                                         rdfs:label "unipedeVoltageDip15to30" .


:MeasurementKind.unipedeVoltageDip30to60 uml:hasInitialValue "51" ;
                                         uml:id "_566EEB85-1B8D-4030-AD2A-8651FA73C45C" ;
                                         rdfs:comment "A voltage dip classification per EN50160 or a similar national standard measuring the number of dips in the 30-60% range" ;
                                         rdfs:label "unipedeVoltageDip30to60" .


:MeasurementKind.unipedeVoltageDip60to90 uml:hasInitialValue "52" ;
                                         uml:id "_BCA45FB4-D18E-4222-9B76-619FE9D8C2B8" ;
                                         rdfs:comment "A voltage dip classification per EN50160 or a similar national standard measuring the number of dips in the 60-90% rangeA voltage dip classification per EN50160 or a similar national standard measuring the number of dips in the 60-90% range" ;
                                         rdfs:label "unipedeVoltageDip60to90" .


:MeasurementKind.unipedeVoltageDip90to100 uml:hasInitialValue "53" ;
                                          uml:id "_C51156E4-4AB4-4e71-8249-937CF2036524" ;
                                          rdfs:comment "A voltage dip classification per EN50160 or a similar national standard measuring the number of dips in the 90-100% range" ;
                                          rdfs:label "unipedeVoltageDip90to100" .


:MeasurementKind.voltage uml:hasInitialValue "54" ;
                         uml:id "_15350EB8-8B4D-4d09-9347-F16B6D422543" ;
                         rdfs:comment "The difference in electric potential between two points" ;
                         rdfs:label "voltage" .


:MeasurementKind.voltageAngle uml:hasInitialValue "55" ;
                              uml:id "_91EE923C-1F9A-4b29-B41F-66932111CBA6" ;
                              rdfs:comment "A phase voltage zerocross timing measurement relative to a reference voltage zerocross" ;
                              rdfs:label "voltageAngle" .


:MeasurementKind.voltageExcursion uml:hasInitialValue "56" ;
                                  uml:id "_883DC8A3-2510-4cb9-81B9-781EEE07F136" ;
                                  rdfs:comment "A measurement of the departure of the voltage from the nominal voltage" ;
                                  rdfs:label "voltageExcursion" .


:MeasurementKind.voltageImbalance uml:hasInitialValue "57" ;
                                  uml:id "_E8EB098A-818B-46fa-AA7D-25D8BCBC9E53" ;
                                  rdfs:comment "A measurement of the departure of a phase voltage relative to the average voltage of all phases." ;
                                  rdfs:label "voltageImbalance" .


:MeasurementKind.volume uml:hasInitialValue "58" ;
                        uml:id "_6563A061-FA70-42ab-8956-BA4EA4B12249" ;
                        rdfs:comment "fluid volume" ;
                        rdfs:label "volume" .


:MeasurementKind.volumetricFlow uml:hasInitialValue "155" ;
                                uml:id "_3B2D00A7-C88D-4070-BE84-61ED3AEBB87C" ;
                                rdfs:comment "A fluid flow rate" ;
                                rdfs:label "volumetricFlow" .


:MeasurementKind.watchdogTimeout uml:hasInitialValue "149" ;
                                 uml:id "_A01BEBD5-4071-4054-A03B-DED25DA6B1D7" ;
                                 rdfs:comment "A reset triggered by a hardware “watchdog” circuit" ;
                                 rdfs:label "watchdogTimeout" .


:MeasurementKind.zeroFlowDuration uml:hasInitialValue "59" ;
                                  uml:id "_524A726F-AFA8-4c40-A294-A1E212806698" ;
                                  rdfs:comment "The amount of time that current flow drops to a zero level or level below the ability of the sensor to sense" ;
                                  rdfs:label "zeroFlowDuration" .


:MeasurementKind.zeroSequence uml:hasInitialValue "60" ;
                              uml:id "_D21E3C33-046F-4037-BA7B-03FEC18C91B5" ;
                              rdfs:comment "The zero sequence current is the vector sum of the phase currents" ;
                              rdfs:label "zeroSequence" .


:MeasurementTypeEMS.ACE uml:id "_0FA0B70E-B0B3-4950-ADEA-51006178823A" ;
                        rdfs:label "ACE" .


:MeasurementTypeEMS.GMOL uml:id "_57EF2852-62CF-4ff8-837B-3ECB59BD9BCB" ;
                         rdfs:label "GMOL" .


:MeasurementTypeEMS.GNOL uml:id "_9ED2A822-6B02-4d66-9B23-36B0F547B26F" ;
                         rdfs:label "GNOL" .


:MeasurementTypeEMS.GO uml:id "_4D7E5067-F201-4561-9990-6E884C861C2C" ;
                       rdfs:label "GO" .


:MeasurementTypeEMS.GR uml:id "_0712319C-5F8C-482e-9170-643FAE255A3C" ;
                       rdfs:label "GR" .


:MeasurementTypeEMS.GS uml:id "_799D8013-F4E8-4172-96A9-043A882C525A" ;
                       rdfs:label "GS" .


:MeasurementTypeEMS.INADV uml:id "_B5D73677-D880-44ba-9A7D-008E2C7C890B" ;
                          rdfs:label "INADV" .


:MeasurementTypeEMS.OARL uml:id "_1E5EC7EC-0D1B-40de-9DD2-237189AEC425" ;
                         rdfs:label "OARL" .


:MeasurementTypeEMS.PF uml:id "_EEA27A15-26B8-4721-A4F3-3DB1F3D48658" ;
                       rdfs:label "PF" .


:MeasurementTypeEMS.PIAL uml:id "_14D3339E-3F29-42fc-AA00-1F548C83545C" ;
                         rdfs:label "PIAL" .


:MeasurementTypeEMS.PIL uml:id "_A00F6BD6-9947-412f-A60C-E58AC8F0F265" ;
                        rdfs:label "PIL" .


:MeasurementTypeEMS.PIML uml:id "_AE387939-FB22-4e61-B82C-EFB09D47C9F6" ;
                         rdfs:label "PIML" .


:MeasurementTypeEMS.POAL uml:id "_EA03C42C-0AB3-4448-8CD2-C337AE09451E" ;
                         rdfs:label "POAL" .


:MeasurementTypeEMS.POL uml:id "_097C6448-17B5-491a-8DCA-0FB47AF2972E" ;
                        rdfs:label "POL" .


:MeasurementTypeEMS.PP uml:id "_0DB7C1D0-C76F-400b-B310-D19CC9B97F27" ;
                       rdfs:label "PP" .


:MeasurementTypeEMS.SL uml:id "_252ACA0D-1FE6-4409-B6A3-2FB09E740BDB" ;
                       rdfs:label "SL" .


:MeasuringPeriodKind.fifteenMinute uml:hasInitialValue "2" ;
                                   uml:id "_D6F06CAD-18C9-42d8-B9CA-B4510C490D1D" ;
                                   rdfs:comment "15-minute" ;
                                   rdfs:label "fifteenMinute" .


:MeasuringPeriodKind.fiveMinute uml:hasInitialValue "6" ;
                                uml:id "_035A25E5-6AB6-4c0d-9F0B-51D0008468CE" ;
                                rdfs:comment "5-minute" ;
                                rdfs:label "fiveMinute" .


:MeasuringPeriodKind.fixedBlock10Min uml:hasInitialValue "54" ;
                                     uml:id "_4B9E4326-E713-4699-A8C5-F39FDBC372E8" ;
                                     rdfs:comment "10-minute Fixed Block" ;
                                     rdfs:label "fixedBlock10Min" .


:MeasuringPeriodKind.fixedBlock15Min uml:hasInitialValue "53" ;
                                     uml:id "_FF8E972C-1C3E-4f40-A8A2-21A3CFA846B6" ;
                                     rdfs:comment "15-minute Fixed Block" ;
                                     rdfs:label "fixedBlock15Min" .


:MeasuringPeriodKind.fixedBlock1Min uml:hasInitialValue "56" ;
                                    uml:id "_C1B1F10A-0D80-419d-B0E4-529254D5AE82" ;
                                    rdfs:comment "1-minute Fixed Block" ;
                                    rdfs:label "fixedBlock1Min" .


:MeasuringPeriodKind.fixedBlock20Min uml:hasInitialValue "52" ;
                                     uml:id "_E2E2DE00-07AE-44fa-B2A9-B314E19E6B4E" ;
                                     rdfs:comment "20-minute Fixed Block" ;
                                     rdfs:label "fixedBlock20Min" .


:MeasuringPeriodKind.fixedBlock30Min uml:hasInitialValue "51" ;
                                     uml:id "_60A8C17B-21E4-4c63-B678-D76C410E8B76" ;
                                     rdfs:comment "30-minute Fixed Block" ;
                                     rdfs:label "fixedBlock30Min" .


:MeasuringPeriodKind.fixedBlock5Min uml:hasInitialValue "55" ;
                                    uml:id "_425B16A1-D79F-4194-99AB-C8DF00838CD4" ;
                                    rdfs:comment "5-minute Fixed Block" ;
                                    rdfs:label "fixedBlock5Min" .


:MeasuringPeriodKind.fixedBlock60Min uml:hasInitialValue "50" ;
                                     uml:id "_03AF44AE-3CDF-4f9b-B555-3E7A3C21E82C" ;
                                     rdfs:comment "60-minute Fixed Block" ;
                                     rdfs:label "fixedBlock60Min" .


:MeasuringPeriodKind.none uml:hasInitialValue "0" ;
                          uml:id "_FD4D33BC-3EC1-4919-A63F-FB7A8A81E70D" ;
                          rdfs:comment "Not applicable." ;
                          rdfs:label "none" .


:MeasuringPeriodKind.oneMinute uml:hasInitialValue "3" ;
                               uml:id "_E9FC29CB-8963-4e4f-9D05-B6B7623D1973" ;
                               rdfs:comment "1-minute" ;
                               rdfs:label "oneMinute" .


:MeasuringPeriodKind.present uml:hasInitialValue "15" ;
                             uml:id "_2C3BBDC9-D044-4da8-98E7-A30DBBEFD232" ;
                             rdfs:comment "Within the present period of time" ;
                             rdfs:label "present" .


:MeasuringPeriodKind.previous uml:hasInitialValue "16" ;
                              uml:id "_D7A26C99-5F5E-4630-9D4D-0093EE51C739" ;
                              rdfs:comment "Shifted within the previous monthly cycle and data set" ;
                              rdfs:label "previous" .


:MeasuringPeriodKind.rollingBlock10MinIntvl1MinSubIntvl uml:hasInitialValue "76" ;
                                                        uml:id "_80729BDD-6E54-4315-A46F-1C7E6DEA4481" ;
                                                        rdfs:comment "10-minute Rolling Block with 1-minute sub-intervals" ;
                                                        rdfs:label "rollingBlock10MinIntvl1MinSubIntvl" .


:MeasuringPeriodKind.rollingBlock10MinIntvl2MinSubIntvl uml:hasInitialValue "75" ;
                                                        uml:id "_9C0B7FA4-1728-42ac-8660-B52F7FF214CC" ;
                                                        rdfs:comment "10-minute Rolling Block with 2-minute sub-intervals" ;
                                                        rdfs:label "rollingBlock10MinIntvl2MinSubIntvl" .


:MeasuringPeriodKind.rollingBlock10MinIntvl5MinSubIntvl uml:hasInitialValue "74" ;
                                                        uml:id "_55EE1F3C-E336-4977-BEA2-735627D947D9" ;
                                                        rdfs:comment "10-minute Rolling Block with 5-minute sub-intervals" ;
                                                        rdfs:label "rollingBlock10MinIntvl5MinSubIntvl" .


:MeasuringPeriodKind.rollingBlock15MinIntvl1MinSubIntvl uml:hasInitialValue "73" ;
                                                        uml:id "_1A8CF1B9-6B10-4a67-B66C-6FB0391BD734" ;
                                                        rdfs:comment "15-minute Rolling Block with 1-minute sub-intervals" ;
                                                        rdfs:label "rollingBlock15MinIntvl1MinSubIntvl" .


:MeasuringPeriodKind.rollingBlock15MinIntvl3MinSubIntvl uml:hasInitialValue "72" ;
                                                        uml:id "_5F3B4D4C-A2EF-4a15-848E-8446F357358E" ;
                                                        rdfs:comment "15-minute Rolling Block with 3-minute sub-intervals" ;
                                                        rdfs:label "rollingBlock15MinIntvl3MinSubIntvl" .


:MeasuringPeriodKind.rollingBlock15MinIntvl5MinSubIntvl uml:hasInitialValue "71" ;
                                                        uml:id "_02859A96-6A9B-4059-92E9-D35E8FCFE795" ;
                                                        rdfs:comment "15-minute Rolling Block with 5-minute sub-intervals" ;
                                                        rdfs:label "rollingBlock15MinIntvl5MinSubIntvl" .


:MeasuringPeriodKind.rollingBlock30MinIntvl10MinSubIntvl uml:hasInitialValue "66" ;
                                                         uml:id "_50BF1585-FFC2-4a0e-84C5-DFF0431C65BC" ;
                                                         rdfs:comment "30-minute Rolling Block with 10-minute sub-intervals" ;
                                                         rdfs:label "rollingBlock30MinIntvl10MinSubIntvl" .


:MeasuringPeriodKind.rollingBlock30MinIntvl15MinSubIntvl uml:hasInitialValue "65" ;
                                                         uml:id "_17B2B4EA-B1FC-4fc0-93A8-DCC85B394C13" ;
                                                         rdfs:comment "30-minute Rolling Block with 15-minute sub-intervals" ;
                                                         rdfs:label "rollingBlock30MinIntvl15MinSubIntvl" .


:MeasuringPeriodKind.rollingBlock30MinIntvl2MinSubIntvl uml:hasInitialValue "70" ;
                                                        uml:id "_09A15EB1-45C5-4ef4-AB64-A36D34694C13" ;
                                                        rdfs:comment "30-minute Rolling Block with 2-minute sub-intervals" ;
                                                        rdfs:label "rollingBlock30MinIntvl2MinSubIntvl" .


:MeasuringPeriodKind.rollingBlock30MinIntvl3MinSubIntvl uml:hasInitialValue "69" ;
                                                        uml:id "_DECD7909-66E5-4e90-84A7-26C550779BCC" ;
                                                        rdfs:comment "30-minute Rolling Block with 3-minute sub-intervals" ;
                                                        rdfs:label "rollingBlock30MinIntvl3MinSubIntvl" .


:MeasuringPeriodKind.rollingBlock30MinIntvl5MinSubIntvl uml:hasInitialValue "68" ;
                                                        uml:id "_E4655F7C-69FE-48e7-9CB8-A7EE26A5C2E8" ;
                                                        rdfs:comment "30-minute Rolling Block with 5-minute sub-intervals." ;
                                                        rdfs:label "rollingBlock30MinIntvl5MinSubIntvl" .


:MeasuringPeriodKind.rollingBlock30MinIntvl6MinSubIntvl uml:hasInitialValue "67" ;
                                                        uml:id "_AADD0246-C750-492c-B0D0-CFFD49FA2FC3" ;
                                                        rdfs:comment "30-minute Rolling Block with 6-minute sub-intervals" ;
                                                        rdfs:label "rollingBlock30MinIntvl6MinSubIntvl" .


:MeasuringPeriodKind.rollingBlock5MinIntvl1MinSubIntvl uml:hasInitialValue "77" ;
                                                       uml:id "_46FC902F-1526-4e05-90AE-462779745425" ;
                                                       rdfs:comment "5-minute Rolling Block with 1-minute sub-intervals" ;
                                                       rdfs:label "rollingBlock5MinIntvl1MinSubIntvl" .


:MeasuringPeriodKind.rollingBlock60MinIntvl10MinSubIntvl uml:hasInitialValue "61" ;
                                                         uml:id "_D17B3727-8E4A-4344-927F-29E312B9FC07" ;
                                                         rdfs:comment "60-minute Rolling Block with 10-minute sub-intervals" ;
                                                         rdfs:label "rollingBlock60MinIntvl10MinSubIntvl" .


:MeasuringPeriodKind.rollingBlock60MinIntvl12MinSubIntvl uml:hasInitialValue "60" ;
                                                         uml:id "_C3D911B2-0EC8-459e-B27D-8C0CD3917C69" ;
                                                         rdfs:comment "60-minute Rolling Block with 12-minute sub-intervals" ;
                                                         rdfs:label "rollingBlock60MinIntvl12MinSubIntvl" .


:MeasuringPeriodKind.rollingBlock60MinIntvl15MinSubIntvl uml:hasInitialValue "59" ;
                                                         uml:id "_11186874-64B9-4b12-8BAD-D094049618BB" ;
                                                         rdfs:comment "60-minute Rolling Block with 15-minute sub-intervals" ;
                                                         rdfs:label "rollingBlock60MinIntvl15MinSubIntvl" .


:MeasuringPeriodKind.rollingBlock60MinIntvl20MinSubIntvl uml:hasInitialValue "58" ;
                                                         uml:id "_12A9FDE0-6E63-4c4b-B0C1-99C1498BAD9F" ;
                                                         rdfs:comment "60-minute Rolling Block with 20-minute sub-intervals" ;
                                                         rdfs:label "rollingBlock60MinIntvl20MinSubIntvl" .


:MeasuringPeriodKind.rollingBlock60MinIntvl30MinSubIntvl uml:hasInitialValue "57" ;
                                                         uml:id "_4B5CD310-43A1-449c-A8F6-8A5D967809B7" ;
                                                         rdfs:comment "60-minute Rolling Block with 30-minute sub-intervals" ;
                                                         rdfs:label "rollingBlock60MinIntvl30MinSubIntvl" .


:MeasuringPeriodKind.rollingBlock60MinIntvl4MinSubIntvl uml:hasInitialValue "64" ;
                                                        uml:id "_87E5F8B5-BC33-4cf0-B5FF-AA00BFE2B33B" ;
                                                        rdfs:comment "60-minute Rolling Block with 4-minute sub-intervals" ;
                                                        rdfs:label "rollingBlock60MinIntvl4MinSubIntvl" .


:MeasuringPeriodKind.rollingBlock60MinIntvl5MinSubIntvl uml:hasInitialValue "63" ;
                                                        uml:id "_F7D738DD-991D-41d0-ACA8-7EBE050725C6" ;
                                                        rdfs:comment "60-minute Rolling Block with 5-minute sub-intervals" ;
                                                        rdfs:label "rollingBlock60MinIntvl5MinSubIntvl" .


:MeasuringPeriodKind.rollingBlock60MinIntvl6MinSubIntvl uml:hasInitialValue "62" ;
                                                        uml:id "_ABD861D9-2A96-46fb-BB20-8DB0398E4556" ;
                                                        rdfs:comment "60-minute Rolling Block with 6-minute sub-intervals" ;
                                                        rdfs:label "rollingBlock60MinIntvl6MinSubIntvl" .


:MeasuringPeriodKind.sixtyMinute uml:hasInitialValue "7" ;
                                 uml:id "_87EA2C65-C6EC-45b5-8240-E478D2951D8D" ;
                                 rdfs:comment "60-minute" ;
                                 rdfs:label "sixtyMinute" .


:MeasuringPeriodKind.tenMinute uml:hasInitialValue "1" ;
                               uml:id "_9118A5F7-C0D1-4e25-8C90-7E58E237AA7C" ;
                               rdfs:comment "10-minute" ;
                               rdfs:label "tenMinute" .


:MeasuringPeriodKind.thirtyMinute uml:hasInitialValue "5" ;
                                  uml:id "_BAE50016-8363-490a-9BEC-ADDD4D25303A" ;
                                  rdfs:comment "30-minute" ;
                                  rdfs:label "thirtyMinute" .


:MeasuringPeriodKind.threeMinute uml:hasInitialValue "14" ;
                                 uml:id "_1C373062-F881-42bc-8EDB-EB29B082D3CC" ;
                                 rdfs:comment "3-minute" ;
                                 rdfs:label "threeMinute" .


:MeasuringPeriodKind.twentyMinute uml:hasInitialValue "31" ;
                                  uml:id "_AEADF8B1-8239-4360-B86C-EBE77218365C" ;
                                  rdfs:comment "20-minute interval" ;
                                  rdfs:label "twentyMinute" .


:MeasuringPeriodKind.twentyfourHour uml:hasInitialValue "4" ;
                                    uml:id "_F330DEE2-455E-45a5-B6D0-FF8A83912F87" ;
                                    rdfs:comment "24-hour" ;
                                    rdfs:label "twentyfourHour" .


:MeasuringPeriodKind.twoMinute uml:hasInitialValue "10" ;
                               uml:id "_CE9A4ADD-E32A-4471-BB5C-1B18DDE7BD5E" ;
                               rdfs:comment "2-minute" ;
                               rdfs:label "twoMinute" .


:MediumKind.SF6 uml:id "_DF7BF9ED-BCB9-4e1c-9B4C-33AB52B81700" ;
                rdfs:comment "Medium is SF6." ;
                rdfs:label "SF6" .


:MediumKind.SF6CF4 uml:id "_4661C9CD-9C00-4b59-82E9-E7D6044F405A" ;
                   rdfs:comment "Medium is SF6CF4." ;
                   rdfs:label "SF6CF4" .


:MediumKind.SF6N2 uml:id "_99F5728F-1618-4f4c-82C1-04A7F55F7C23" ;
                  rdfs:comment "Medium is SF6N2." ;
                  rdfs:label "SF6N2" .


:MediumKind.air uml:id "_C3038E60-FBA6-4499-B567-25B7BDA528D8" ;
                rdfs:comment "Medium is air." ;
                rdfs:label "air" .


:MediumKind.gas uml:id "_AA7F3DEB-B805-4dbe-BB34-13C7073D49C9" ;
                rdfs:comment "Medium is gas." ;
                rdfs:label "gas" .


:MediumKind.liquid uml:id "_C4CEFD70-56D3-4edb-84B0-E4973AA3A1FE" ;
                   rdfs:comment "Medium is liquid." ;
                   rdfs:label "liquid" .


:MediumKind.mineralOil uml:id "_15DFC023-8E5A-4fb3-A697-991C381F80FD" ;
                       rdfs:comment "Medium is mineral oil." ;
                       rdfs:label "mineralOil" .


:MediumKind.solid uml:id "_4D23B971-5C5E-4798-BD1E-0E65920C3D01" ;
                  rdfs:comment "Medium is solid." ;
                  rdfs:label "solid" .


:MeterMultiplierKind.ctRatio uml:id "_5CF26FCC-C93E-42e3-9199-8ECEE905CEBE" ;
                             rdfs:comment "Current transformer ratio used to convert associated quantities to real measurements." ;
                             rdfs:label "ctRatio" .


:MeterMultiplierKind.kE uml:id "_04F87E33-EFA9-46c8-84AE-FF608FF3E610" ;
                        rdfs:comment "Test constant." ;
                        rdfs:label "kE" .


:MeterMultiplierKind.kH uml:id "_9F98A4FA-F8F7-403b-A2E0-DDCEB442D097" ;
                        rdfs:comment "Meter kh (watthour) constant. The number of watthours that must be applied to the meter to cause one disk revolution for an electromechanical meter or the number of watthours represented by one increment pulse for an electronic meter." ;
                        rdfs:label "kH" .


:MeterMultiplierKind.kR uml:id "_79D140FB-40E1-49ab-B547-9C04DFE6CD9B" ;
                        rdfs:comment "Register multiplier. The number to multiply the register reading by in order to get kWh." ;
                        rdfs:label "kR" .


:MeterMultiplierKind.ptRatio uml:id "_518587B2-0F99-4f5e-A3FD-990234AB31E3" ;
                             rdfs:comment "Potential transformer ratio used to convert associated quantities to real measurements." ;
                             rdfs:label "ptRatio" .


:MeterMultiplierKind.transformerRatio uml:id "_6C6C20A7-B87F-4f67-96F2-3C752E5FC3B3" ;
                                      rdfs:comment "Product of the CT ratio and PT ratio." ;
                                      rdfs:label "transformerRatio" .


:MktAccountKind.estimate uml:id "_D4B2F902-D305-4f78-85E0-A9E0EE37735F" ;
                         rdfs:label "estimate" .


:MktAccountKind.normal uml:id "_B5303E13-E217-4b2e-9F81-8F9A3C83886C" ;
                       rdfs:label "normal" .


:MktAccountKind.reversal uml:id "_3FAD5137-496A-4d70-BCF4-1CE734C0A184" ;
                         rdfs:label "reversal" .


:MktAccountKind.statistical uml:id "_1B860D7A-EED5-42cc-A673-6FEB822A51BD" ;
                            rdfs:label "statistical" .


:MktBillMediaKind.electronic uml:id "_3444A4A4-A234-4eba-90D8-E7899BB6CDA2" ;
                             rdfs:label "electronic" .


:MktBillMediaKind.other uml:id "_A883656D-E14E-451c-83B5-97CC1CEC13E2" ;
                        rdfs:label "other" .


:MktBillMediaKind.paper uml:id "_4A84C70E-BBC0-4423-B132-21B8C024AF48" ;
                        rdfs:label "paper" .


:MktInvoiceLineItemKind.initial uml:id "_CE02D575-68E5-4c34-97BB-C257910ADAA8" ;
                                rdfs:label "initial" .


:MktInvoiceLineItemKind.other uml:id "_5359109E-9CA5-4438-B8FF-10CD7C697C16" ;
                              rdfs:label "other" .


:MktInvoiceLineItemKind.recalculation uml:id "_CD86A29F-B313-4177-9803-4A299DD912B9" ;
                                      rdfs:label "recalculation" .


:MktSubClassType.Branch_Group_Derates uml:id "_B0748A31-6B84-4fb4-88AB-B7DFBFEA3F71" ;
                                      rdfs:label "Branch_Group_Derates" .


:MktSubClassType.Day_Ahead_Final_Market_Info uml:id "_2454CB72-19E5-44f7-8D45-653E1F41A53C" ;
                                             rdfs:label "Day_Ahead_Final_Market_Info" .


:MktSubClassType.Day_Ahead_Forecast_Information uml:id "_317BB24D-A41C-4f3e-A01D-05899872F77D" ;
                                                rdfs:label "Day_Ahead_Forecast_Information" .


:MktSubClassType.Day_Ahead_Interim_Market_Info uml:id "_45BCBE7D-ED94-4ca3-A2D4-744D49ADCD4C" ;
                                               rdfs:label "Day_Ahead_Interim_Market_Info" .


:MktSubClassType.Day_Ahead_RMR uml:id "_40F50181-25A9-4497-A6F6-36E3CA79907A" ;
                               rdfs:label "Day_Ahead_RMR" .


:MktSubClassType.Forecasted_UDC_Direct_Access_Load uml:id "_0A57D14D-1863-4d53-A4E0-E5D213A036E3" ;
                                                   rdfs:label "Forecasted_UDC_Direct_Access_Load" .


:MktSubClassType.Hour_Ahead_Market_Info uml:id "_F51F15AA-AAC5-484a-A4F1-CBD3C83A57D6" ;
                                        rdfs:label "Hour_Ahead_Market_Info" .


:MktSubClassType.Hourly_Expost_Market_Info uml:id "_9EDA9C91-E50E-48ae-AAB9-A968F6E5CCDD" ;
                                           rdfs:label "Hourly_Expost_Market_Info" .


:MktSubClassType.Public_Bid_Data uml:id "_67F61CAF-B6F1-448b-B7EA-0699FBAE8F1F" ;
                                 rdfs:label "Public_Bid_Data" .


:MktSubClassType.TTC_ATC_Forecast_Information uml:id "_9BBAE60F-FD55-46ef-8E37-8F0FFAEB7E54" ;
                                              rdfs:label "TTC/ATC_Forecast_Information" .


:MktSubClassType.TTC_ATC_Hourly_Forecast uml:id "_00CE4FBD-34B0-438b-9F64-9D5E61803B29" ;
                                         rdfs:label "TTC/ATC_Hourly_Forecast" .


:MktSubClassType.Ten_Min_Expost_Market_Info uml:id "_D7661E86-B02D-4429-9EE3-18FE5BC4A3D4" ;
                                            rdfs:label "Ten_Min_Expost_Market_Info" .


:NotificationTriggerKind.etrChange uml:id "_775E6A45-3F58-4ce8-9A1D-CCD38F954693" ;
                                   rdfs:comment "Notify customer if estimated restoration time changes." ;
                                   rdfs:label "etrChange" .


:NotificationTriggerKind.informDispatched uml:id "_FCF11AD0-2E2E-4090-8159-7DFCCB5D436F" ;
                                          rdfs:comment "Notify customer that a crew has been dispatched to investigate the problem." ;
                                          rdfs:label "informDispatched" .


:NotificationTriggerKind.initialEtr uml:id "_E9A8A82A-DF8D-45bc-9F78-18CC88889579" ;
                                    rdfs:comment "Notify customer for the first time that estimated restoration time is available." ;
                                    rdfs:label "initialEtr" .


:NotificationTriggerKind.powerOut uml:id "_11257F70-AD72-4382-B39D-EEC832576F1E" ;
                                  rdfs:comment "Notify customer of planned outage." ;
                                  rdfs:label "powerOut" .


:NotificationTriggerKind.powerRestored uml:id "_8AC6D3E4-059C-4bd2-BAD5-53802F86E8B5" ;
                                       rdfs:comment "Notify customer when power has been restored." ;
                                       rdfs:label "powerRestored" .


:OASISBidReportType.BIDS_PUBLIC uml:id "_18021C7D-99BE-4279-A88A-A9E0985226CB" ;
                                rdfs:label "BIDS_PUBLIC" .


:OASISDataItems.AS_CLEAR_ASMP_IFM uml:id "_2E8CFF15-E5B6-4191-982D-B86351F30165" ;
                                  rdfs:label "AS_CLEAR_ASMP_IFM" .


:OASISDataItems.AS_CLEAR_ASMP_RTM uml:id "_48DBC876-EA71-472c-BAE7-51B975659882" ;
                                  rdfs:label "AS_CLEAR_ASMP_RTM" .


:OASISDataItems.AS_CLEAR_COST_IFM uml:id "_9DDB4483-C773-477b-9E64-434701A0E25F" ;
                                  rdfs:label "AS_CLEAR_COST_IFM" .


:OASISDataItems.AS_CLEAR_COST_RTM uml:id "_08E90DC9-335E-4b7d-ABC8-6173E1551CF2" ;
                                  rdfs:label "AS_CLEAR_COST_RTM" .


:OASISDataItems.AS_CLEAR_MW_IFM uml:id "_37FC4749-7088-4e95-B76A-B6FFF824B59F" ;
                                rdfs:label "AS_CLEAR_MW_IFM" .


:OASISDataItems.AS_CLEAR_MW_RTM uml:id "_521A08EE-1E39-4ce2-B5A4-2AE20FE04577" ;
                                rdfs:label "AS_CLEAR_MW_RTM" .


:OASISDataItems.AS_GEN_TOTAL_MW_IFM uml:id "_C8B542B9-8757-4c8c-B5C1-AEAFCFAD4D2A" ;
                                    rdfs:label "AS_GEN_TOTAL_MW_IFM" .


:OASISDataItems.AS_GEN_TOTAL_MW_RTM uml:id "_32D17334-EB68-45f7-8D43-FD0C80DDB257" ;
                                    rdfs:label "AS_GEN_TOTAL_MW_RTM" .


:OASISDataItems.AS_IMP_TOTAL_MW_IFM uml:id "_714C30C8-05B6-42a8-ACDE-E3EC4BE64DD5" ;
                                    rdfs:label "AS_IMP_TOTAL_MW_IFM" .


:OASISDataItems.AS_IMP_TOTAL_MW_RTM uml:id "_5E2F989B-AFC4-4045-A320-3E52460BB9C9" ;
                                    rdfs:label "AS_IMP_TOTAL_MW_RTM" .


:OASISDataItems.AS_LOAD_TOTAL_MW_IFM uml:id "_F5BAC623-64D8-4317-9BE0-B5357638F3FD" ;
                                     rdfs:label "AS_LOAD_TOTAL_MW_IFM" .


:OASISDataItems.AS_LOAD_TOTAL_MW_RTM uml:id "_F736A69A-7F6A-4b75-9965-CDAAE07EA9D2" ;
                                     rdfs:label "AS_LOAD_TOTAL_MW_RTM" .


:OASISDataItems.AS_REGION_REQ_MAX uml:id "_A4A68180-5223-45e8-863E-E3CB8FB57A33" ;
                                  rdfs:label "AS_REGION_REQ_MAX" .


:OASISDataItems.AS_REGION_REQ_MIN uml:id "_1B765314-5A49-4729-9B07-956CD0C572C9" ;
                                  rdfs:label "AS_REGION_REQ_MIN" .


:OASISDataItems.AS_REGION_value uml:id "_BAFB24A0-70BD-482d-A72D-88F70A09C3EF" ;
                                rdfs:label "AS_REGION_value" .


:OASISDataItems.AS_SELF_MW_IFM uml:id "_B5749992-2766-4486-ACD8-02511D973D00" ;
                               rdfs:label "AS_SELF_MW_IFM" .


:OASISDataItems.AS_SELF_MW_RTM uml:id "_4D5EEC4E-A5E1-42b5-9C33-8A92E17E8078" ;
                               rdfs:label "AS_SELF_MW_RTM" .


:OASISDataItems.AS_TOTAL_MW uml:id "_9A2CE2CD-F409-43be-BC58-2A412F8B5421" ;
                            rdfs:label "AS_TOTAL_MW" .


:OASISDataItems.AS_TOTAL_MW_IFM uml:id "_257A914F-4FC7-406b-8FE1-12A36535692A" ;
                                rdfs:label "AS_TOTAL_MW_IFM" .


:OASISDataItems.AS_TOTAL_MW_RTM uml:id "_43868FFD-AA45-48bb-A8BF-D75F47C45748" ;
                                rdfs:label "AS_TOTAL_MW_RTM" .


:OASISDataItems.AS_TYPE uml:id "_D78BFF46-D910-4d9d-B024-B53FDFEA8D3B" ;
                        rdfs:label "AS_TYPE" .


:OASISDataItems.AS_USER_RATE uml:id "_4C080795-5CB7-4c64-B61E-0848D21A50CE" ;
                             rdfs:label "AS_USER_RATE" .


:OASISDataItems.CA_value uml:id "_0CD1AA78-28D6-4766-A61F-FE8524CDE2A7" ;
                         rdfs:label "CA_value" .


:OASISDataItems.CMMT_MINLOAD_MLC uml:id "_CEE6EEA4-9A94-48de-970C-2F93817106E4" ;
                                 rdfs:label "CMMT_MINLOAD_MLC" .


:OASISDataItems.CMMT_MINLOAD_MW uml:id "_E7357460-7603-43f6-8B26-213F823B6BF5" ;
                                rdfs:label "CMMT_MINLOAD_MW" .


:OASISDataItems.CMMT_RA_MLC uml:id "_036A7F3E-B07B-4356-A7A6-CD412B85C055" ;
                            rdfs:label "CMMT_RA_MLC" .


:OASISDataItems.CMMT_RA_MW uml:id "_C8D43172-7B85-4ade-BE38-9C3963DDE7CE" ;
                           rdfs:label "CMMT_RA_MW" .


:OASISDataItems.CMMT_RA_START_COST uml:id "_30304291-D682-436e-8BF4-C04B0D447E49" ;
                                   rdfs:label "CMMT_RA_START_COST" .


:OASISDataItems.CMMT_RA_UNITS uml:id "_AD4DD57D-3E94-431c-9777-D34C46B06F52" ;
                              rdfs:label "CMMT_RA_UNITS" .


:OASISDataItems.CMMT_TOTAL_MW uml:id "_EDB4940D-CCA0-48be-A10D-AEE406EADC7C" ;
                              rdfs:label "CMMT_TOTAL_MW" .


:OASISDataItems.CMMT_TOTAL_START_COST uml:id "_FB439EC5-0718-4ed5-B7D6-A0DD1737734E" ;
                                      rdfs:label "CMMT_TOTAL_START_COST" .


:OASISDataItems.CMMT_TOTAL_UNITS uml:id "_275D9B5D-4BBD-4a36-B595-E88D98766B2D" ;
                                 rdfs:label "CMMT_TOTAL_UNITS" .


:OASISDataItems.CRR_CAT uml:id "_27BDE6D2-F88B-4205-BAF3-F0E99F6F76F5" ;
                        rdfs:label "CRR_CAT" .


:OASISDataItems.CRR_MARKET_value uml:id "_070963AD-54A5-4a60-A1A9-164E8F26975B" ;
                                 rdfs:label "CRR_MARKET_value" .


:OASISDataItems.CRR_MW uml:id "_04782716-A95E-4926-99B7-D5A6A02BEB08" ;
                       rdfs:label "CRR_MW" .


:OASISDataItems.CRR_NSR uml:id "_7DAE537B-ECAE-4436-A120-B12FB1ED9772" ;
                        rdfs:label "CRR_NSR" .


:OASISDataItems.CRR_OPTION uml:id "_1766F92D-2E3C-4fa6-80A6-C6E03A4B55D4" ;
                           rdfs:label "CRR_OPTION" .


:OASISDataItems.CRR_OWNER uml:id "_0CB22477-0F0D-41ab-9EA9-EDB0B6D1EF7C" ;
                          rdfs:label "CRR_OWNER" .


:OASISDataItems.CRR_SEGMENT uml:id "_0F47BB99-F9A0-4b3d-BA54-668E54947588" ;
                            rdfs:label "CRR_SEGMENT" .


:OASISDataItems.CRR_TERM uml:id "_B78149BB-4F0E-4c7b-8639-3BCC666C7D94" ;
                         rdfs:label "CRR_TERM" .


:OASISDataItems.CRR_TOU uml:id "_16544807-F1A8-4630-9706-EF944B10F43D" ;
                        rdfs:label "CRR_TOU" .


:OASISDataItems.CRR_TYPE uml:id "_48ECB90A-2B4D-4086-A964-C665A9DB06F4" ;
                         rdfs:label "CRR_TYPE" .


:OASISDataItems.ENE_EA_DA uml:id "_073705D0-AEC7-4cba-A333-1275CC5944CA" ;
                          rdfs:label "ENE_EA_DA" .


:OASISDataItems.ENE_EA_EXCEPT uml:id "_98D778F5-C29F-46d2-BE92-2D2C2D8E9B86" ;
                              rdfs:label "ENE_EA_EXCEPT" .


:OASISDataItems.ENE_EA_HASP uml:id "_8DE1B880-1055-4bc3-8BCF-481DD31F8D41" ;
                            rdfs:label "ENE_EA_HASP" .


:OASISDataItems.ENE_EA_MLE uml:id "_7A21BF8C-7CD3-4a97-8A5C-25B7E3E815BF" ;
                           rdfs:label "ENE_EA_MLE" .


:OASISDataItems.ENE_EA_MSSLF uml:id "_5A36CCD1-26BC-4a6c-8EAB-AAADDA7A9B75" ;
                             rdfs:label "ENE_EA_MSSLF" .


:OASISDataItems.ENE_EA_OPTIMAL uml:id "_6C6A5CC7-244E-451a-AE28-BECF953F2248" ;
                               rdfs:label "ENE_EA_OPTIMAL" .


:OASISDataItems.ENE_EA_RAMP_DEV uml:id "_D06BF3B9-24BA-420b-9FCE-62E7B96A6D3C" ;
                                rdfs:label "ENE_EA_RAMP_DEV" .


:OASISDataItems.ENE_EA_RAMP_STD uml:id "_1E991D65-3474-4214-8DA8-96261557E233" ;
                                rdfs:label "ENE_EA_RAMP_STD" .


:OASISDataItems.ENE_EA_RESIDUAL uml:id "_E1D190E7-3D8F-4c0f-B050-D81B117B3472" ;
                                rdfs:label "ENE_EA_RESIDUAL" .


:OASISDataItems.ENE_EA_RMR uml:id "_D9186BC8-24B6-45a6-AFA5-0626476FCE7D" ;
                           rdfs:label "ENE_EA_RMR" .


:OASISDataItems.ENE_EA_SELF uml:id "_2B81F461-C161-4e9e-8ED9-A7459DE8C6A6" ;
                            rdfs:label "ENE_EA_SELF" .


:OASISDataItems.ENE_EA_SLIC uml:id "_8D1D8C4F-1344-493f-9AC0-FC1719A1E6A1" ;
                            rdfs:label "ENE_EA_SLIC" .


:OASISDataItems.ENE_EXP_CLEAR_HASP uml:id "_33B98FA2-CFB7-49d6-83A3-5261714A555A" ;
                                   rdfs:label "ENE_EXP_CLEAR_HASP" .


:OASISDataItems.ENE_EXP_CLEAR_IFM uml:id "_DC8D38AB-4F13-4c0c-BA42-1919C9822FF7" ;
                                  rdfs:label "ENE_EXP_CLEAR_IFM" .


:OASISDataItems.ENE_EXP_CLEAR_RTM uml:id "_FC4380BD-10B4-438a-994C-AD70641B3327" ;
                                  rdfs:label "ENE_EXP_CLEAR_RTM" .


:OASISDataItems.ENE_GEN_CLEAR_HASP uml:id "_EC1C50F9-C708-4803-9F93-4434374F7376" ;
                                   rdfs:label "ENE_GEN_CLEAR_HASP" .


:OASISDataItems.ENE_GEN_CLEAR_IFM uml:id "_8084580F-AA87-4526-8207-29E65EA3A15C" ;
                                  rdfs:label "ENE_GEN_CLEAR_IFM" .


:OASISDataItems.ENE_GEN_CLEAR_RTM uml:id "_295DF91B-BD3C-4913-9176-31A40EEB376C" ;
                                  rdfs:label "ENE_GEN_CLEAR_RTM" .


:OASISDataItems.ENE_IMP_CLEAR_HASP uml:id "_C73FE58F-20E4-4296-BD09-8CBE5C91826F" ;
                                   rdfs:label "ENE_IMP_CLEAR_HASP" .


:OASISDataItems.ENE_IMP_CLEAR_IFM uml:id "_21C664D5-AE09-4e37-A24E-9D4A0BC8898A" ;
                                  rdfs:label "ENE_IMP_CLEAR_IFM" .


:OASISDataItems.ENE_IMP_CLEAR_RTM uml:id "_2D0D0668-7357-42d7-8D17-26C2A1577A52" ;
                                  rdfs:label "ENE_IMP_CLEAR_RTM" .


:OASISDataItems.ENE_LOAD_ACTUAL uml:id "_FC5ED093-0418-4ffb-B498-745C85C2E9F8" ;
                                rdfs:label "ENE_LOAD_ACTUAL" .


:OASISDataItems.ENE_LOAD_CLEAR_HASP uml:id "_E3523D98-12B9-44c1-AC52-1F2DCE418A6C" ;
                                    rdfs:label "ENE_LOAD_CLEAR_HASP" .


:OASISDataItems.ENE_LOAD_CLEAR_IFM uml:id "_69375CA9-8DE6-41e3-B201-C83753ABF346" ;
                                   rdfs:label "ENE_LOAD_CLEAR_IFM" .


:OASISDataItems.ENE_LOAD_CLEAR_RTM uml:id "_4ED04167-4E5B-4a2b-BA9A-9E1F1235B10E" ;
                                   rdfs:label "ENE_LOAD_CLEAR_RTM" .


:OASISDataItems.ENE_LOAD_FCST uml:id "_2B253B65-EB44-42f2-855E-CA3E2CCAED1F" ;
                              rdfs:label "ENE_LOAD_FCST" .


:OASISDataItems.ENE_PEAK_HOUR uml:id "_51149821-CAB8-433a-BE67-FA9362FEA810" ;
                              rdfs:label "ENE_PEAK_HOUR" .


:OASISDataItems.ENE_PEAK_LOAD uml:id "_0338BDF5-6679-43a2-9C23-2B27A0204F88" ;
                              rdfs:label "ENE_PEAK_LOAD" .


:OASISDataItems.FUEL_REGION_value uml:id "_E758E815-122C-4e25-ABDE-1C3E668322B3" ;
                                  rdfs:label "FUEL_REGION_value" .


:OASISDataItems.INVT_DATETIME uml:id "_74A003DD-4AD4-457e-B2F3-BB999B772F00" ;
                              rdfs:label "INVT_DATETIME" .


:OASISDataItems.LOAD_ACTUAL uml:id "_91B9803A-555E-47b1-B56F-407E8DB9372E" ;
                            rdfs:label "LOAD_ACTUAL" .


:OASISDataItems.LOAD_CLEAR_RTM uml:id "_B038256E-1660-4142-85BD-9CC3AF510505" ;
                               rdfs:label "LOAD_CLEAR_RTM" .


:OASISDataItems.LOSS_TOTAL_COST_HASP uml:id "_AB51AB38-3C5D-424e-83AC-707D100C804D" ;
                                     rdfs:label "LOSS_TOTAL_COST_HASP" .


:OASISDataItems.LOSS_TOTAL_COST_RTM uml:id "_C9B7D55A-63FD-42d2-BC6B-3E28FCF40ADE" ;
                                    rdfs:label "LOSS_TOTAL_COST_RTM" .


:OASISDataItems.LOSS_TOTAL_MW_HASP uml:id "_2F455BBA-9B45-4078-AF26-9C51D00AAD1D" ;
                                   rdfs:label "LOSS_TOTAL_MW_HASP" .


:OASISDataItems.LOSS_TOTAL_MW_RTM uml:id "_7A5390BA-2A05-462f-87C6-6AD3A12E3BE1" ;
                                  rdfs:label "LOSS_TOTAL_MW_RTM" .


:OASISDataItems.MPM_FLAG uml:id "_4EDA2810-F86B-43a5-9BEA-D33EDA0325CE" ;
                         rdfs:label "MPM_FLAG" .


:OASISDataItems.OP_RSRV_TOTAL uml:id "_FF1020A7-1497-4d86-93AA-5264E2109016" ;
                              rdfs:label "OP_RSRV_TOTAL" .


:OASISDataItems.PRC_NG uml:id "_CAE3C8F7-E277-42bc-A1E2-97D1C0A17461" ;
                       rdfs:label "PRC_NG" .


:OASISDataItems.PRC_SHADOW uml:id "_5341F983-4F0C-48e9-B467-CAA1A139DC64" ;
                           rdfs:label "PRC_SHADOW" .


:OASISDataItems.RATING_ATC uml:id "_60D742DF-091B-41e7-87DD-5FFA67058F6C" ;
                           rdfs:label "RATING_ATC" .


:OASISDataItems.RMR_DETER_DAM uml:id "_7FC6AAF5-1ACC-44ff-AB2A-45BC758C6582" ;
                              rdfs:label "RMR_DETER_DAM" .


:OASISDataItems.RMR_DETER_HASP uml:id "_23DD2C8F-7CC1-481a-8C5F-02C3B4D45E70" ;
                               rdfs:label "RMR_DETER_HASP" .


:OASISDataItems.RMR_DISPATCH_DAM uml:id "_5106A14C-0022-4e88-AD02-B7BBBF863590" ;
                                 rdfs:label "RMR_DISPATCH_DAM" .


:OASISDataItems.RMR_DISPATCH_HASP uml:id "_A5B1B54A-E5A1-42d6-AC27-5FA3C5A46ECC" ;
                                  rdfs:label "RMR_DISPATCH_HASP" .


:OASISDataItems.RMR_TOTAL uml:id "_AFCBC8AF-F454-49a1-BCFA-F638D5953B18" ;
                          rdfs:label "RMR_TOTAL" .


:OASISDataItems.RMR_TOTAL_AVAIL uml:id "_43DF13E3-4047-44dc-B15A-53AC038FD9C8" ;
                                rdfs:label "RMR_TOTAL_AVAIL" .


:OASISDataItems.RUC_GEN_CLEAR_RUC uml:id "_B2C9FB6E-DF77-4cfe-B115-4AD059ABEB8D" ;
                                  rdfs:label "RUC_GEN_CLEAR_RUC" .


:OASISDataItems.RUC_IMP_CLEAR_RUC uml:id "_13692770-5299-4ac0-AB72-7A90F5F5E3EF" ;
                                  rdfs:label "RUC_IMP_CLEAR_RUC" .


:OASISDataItems.RUC_LOAD_CLEAR_RUC uml:id "_28328698-AE40-45b6-96A5-6DD0DCA888DF" ;
                                   rdfs:label "RUC_LOAD_CLEAR_RUC" .


:OASISDataItems.RUC_ZONE_value uml:id "_B0921A65-6B7E-4b56-B8EB-7E58A7748A7E" ;
                               rdfs:label "RUC_ZONE_value" .


:OASISDataItems.TAC_AREA_value uml:id "_A84AE2C9-8A9E-4745-9A77-3ACCDE3106C6" ;
                               rdfs:label "TAC_AREA_value" .


:OASISDataItems.TINTRFCE_value uml:id "_C2751E36-8AFF-4d6d-9AF6-7D850C401E9A" ;
                               rdfs:label "TINTRFCE_value" .


:OASISDataItems.TRNS_AS_IMPORT uml:id "_57008B36-61FB-45b9-8D35-9CA735DF54D0" ;
                               rdfs:label "TRNS_AS_IMPORT" .


:OASISDataItems.TRNS_ENE_IMPORT uml:id "_FBF66399-ECE7-4836-917A-BDDA227C0164" ;
                                rdfs:label "TRNS_ENE_IMPORT" .


:OASISDataItems.TRNS_EQUIP_value uml:id "_7F7F3C58-9C27-47f9-953C-B3B94E81DA7B" ;
                                 rdfs:label "TRNS_EQUIP_value" .


:OASISDataItems.TRNS_RATING_CBM uml:id "_E38A48C6-5CBA-4f34-9555-6D8984745E49" ;
                                rdfs:label "TRNS_RATING_CBM" .


:OASISDataItems.TRNS_RATING_DIRECTION uml:id "_E0711C9E-F059-49d6-8323-A5F022F5F59B" ;
                                      rdfs:label "TRNS_RATING_DIRECTION" .


:OASISDataItems.TRNS_RATING_OTC uml:id "_AD2FA295-3E0F-4e51-91B7-615548A22C06" ;
                                rdfs:label "TRNS_RATING_OTC" .


:OASISDataItems.TRNS_RATING_OTC_DERATE uml:id "_20A4ECEC-E3CF-4a2c-B112-9A1AEB47922A" ;
                                       rdfs:label "TRNS_RATING_OTC_DERATE" .


:OASISDataItems.TRNS_RATING_TTC uml:id "_AB623898-24A8-451b-BC52-65E013308666" ;
                                rdfs:label "TRNS_RATING_TTC" .


:OASISDataItems.TRNS_TI_value uml:id "_0BC4577F-1271-447c-9F68-BCAB09DC8133" ;
                              rdfs:label "TRNS_TI_value" .


:OASISDataItems.TRNS_TR_ENTMTS uml:id "_99DBC1EA-0DEE-4b3c-B7F0-34D8C3A4BFC8" ;
                               rdfs:label "TRNS_TR_ENTMTS" .


:OASISDataItems.TRNS_TR_USEAGE uml:id "_594DC69D-776B-46cc-8BA4-4DE5FCDCEC67" ;
                               rdfs:label "TRNS_TR_USEAGE" .


:OASISErrCode._1000 uml:id "_C986739E-C86E-4da5-98A0-72AF4935C47F" ;
                    rdfs:label "1000" .


:OASISErrCode._1001 uml:id "_A8649B2E-EC90-4e11-88DD-A197D60C5B7F" ;
                    rdfs:label "1001" .


:OASISErrCode._1002 uml:id "_8E2AD261-A921-4508-A780-FF2D8D7F60EB" ;
                    rdfs:label "1002" .


:OASISErrCode._1003 uml:id "_B4D3D296-DF22-472e-8D29-ECAA620A1658" ;
                    rdfs:label "1003" .


:OASISErrCode._1004 uml:id "_A56485DA-9489-40ca-AABA-177BFEFD21A2" ;
                    rdfs:label "1004" .


:OASISErrCode._1005 uml:id "_B9F5A68C-EAA1-4d60-BA50-E9C797430D7D" ;
                    rdfs:label "1005" .


:OASISErrCode._1006 uml:id "_25AAA862-252A-4e53-B04B-82435385A09F" ;
                    rdfs:label "1006" .


:OASISErrCode._1007 uml:id "_8F7F8A7D-329E-4f3b-9C1A-7C8D0542C470" ;
                    rdfs:label "1007" .


:OASISErrCode._1008 uml:id "_20FBEF8E-E763-47c6-A0F3-28143F7EB32D" ;
                    rdfs:label "1008" .


:OASISErrCode._1009 uml:id "_3E458A89-1AEE-4ee2-A7C2-28C78C01F819" ;
                    rdfs:label "1009" .


:OASISErrCode._1010 uml:id "_45142394-638A-4819-AE00-165E1B8216BB" ;
                    rdfs:label "1010" .


:OASISErrDescription.Data_can_be_requested_for_period_of_31_days_only uml:id "_7838A32F-3704-42df-B34A-F6FDB1A3B7CD" ;
                                                                      rdfs:label "Data can be requested for period of 31 days only" .


:OASISErrDescription.Exceptions_in_reading_and_writing_of_XML_files uml:id "_B6DBEA9A-CFED-4ae5-AE40-0300095C641F" ;
                                                                    rdfs:label "Exceptions in reading and writing of XML files" .


:OASISErrDescription.Invalid_date_format__please_use_valid_date_format uml:id "_611AFA4F-B38E-46f2-8B4E-D8EF1B1A4C33" ;
                                                                       rdfs:label "Invalid date format, please use valid date format" .


:OASISErrDescription.No_data_returned_for_the_specified_selection uml:id "_9D2D920A-C6FB-46de-81D5-9C0C3916F7E8" ;
                                                                  rdfs:label "No data returned for the specified selection" .


:OASISErrDescription.Out_of_memory_exception uml:id "_DF99D021-20BA-414f-B047-4A16A1E5B82B" ;
                                             rdfs:label "Out of memory exception" .


:OASISErrDescription.Report_name_does_not_exit__please_use_valid_report_name uml:id "_89AF40DD-8AE2-4947-B74E-1F870F24570B" ;
                                                                             rdfs:label "Report name does not exit, please use valid report name" .


:OASISErrDescription.Required_file_does_not_exist uml:id "_95DA1954-9FC5-494d-8FF8-DA924C530792" ;
                                                  rdfs:label "Required file does not exist" .


:OASISErrDescription.System_Error uml:id "_6EC0E8B2-4065-43fe-B086-48F0B67C6260" ;
                                  rdfs:label "System Error" .


:OASISErrDescription.Timed_out_waiting_for_query_response uml:id "_6B42E03B-7A4E-4f79-B76A-AB1C79DD8050" ;
                                                          rdfs:label "Timed out waiting for query response" .


:OASISErrDescription.Validation_exception_during_transformation_of_XML uml:id "_A6359D27-2EE7-4b63-89F5-930B32E809BD" ;
                                                                       rdfs:label "Validation exception during transformation of XML" .


:OASISIntervalType.BEGINNING uml:id "_7A75AF40-D20B-4cf8-B66D-5A4C53029E66" ;
                             rdfs:label "BEGINNING" .


:OASISIntervalType.ENDING uml:id "_A5DB6B5C-AC20-48b1-A12B-E664B4E4B212" ;
                          rdfs:label "ENDING" .


:OASISMarketType.All uml:id "_67200F17-1B4E-46ff-874B-8FA398CB5282" ;
                     rdfs:label "All" .


:OASISMarketType.HASP uml:id "_DA52FA87-FFFE-4f91-80DE-89D45E92F159" ;
                      rdfs:label "HASP" .


:OASISMarketType.IFM uml:id "_5E255E83-FFC0-4009-A048-BBA343087B9C" ;
                     rdfs:label "IFM" .


:OASISMarketType.N_A uml:id "_82DDC1B9-A1BE-408e-8111-36A97CE0D2EB" ;
                     rdfs:label "N/A" .


:OASISMarketType.RTM uml:id "_7CAB301C-0EC8-43f2-9534-9F5004384E4F" ;
                     rdfs:label "RTM" .


:OASISMarketType.RUC uml:id "_1ACB976D-66FD-4bfb-933A-ADF6D089E23E" ;
                     rdfs:label "RUC" .


:OASISMasterType.ATL_APNODE uml:id "_7E0CA6F5-030A-413a-938D-732DA4529CAD" ;
                            rdfs:label "ATL_APNODE" .


:OASISMasterType.ATL_AS_REGION uml:id "_CEA744C5-2B0D-4aae-80CC-26B14DEF3336" ;
                               rdfs:label "ATL_AS_REGION" .


:OASISMasterType.ATL_AS_REGION_MAP uml:id "_7B808D00-C8FE-40a1-A856-FDBAF654BED0" ;
                                   rdfs:label "ATL_AS_REGION_MAP" .


:OASISMasterType.ATL_HUB uml:id "_FA36F4CE-B6DC-4d55-A371-8D4A6BD31B90" ;
                         rdfs:label "ATL_HUB" .


:OASISMasterType.ATL_LAP uml:id "_7EE9A877-C73A-412e-AFDC-3F7E735C88EE" ;
                         rdfs:label "ATL_LAP" .


:OASISMasterType.ATL_LDF uml:id "_64B42CC6-6573-4821-A47A-2D88821F84FA" ;
                         rdfs:label "ATL_LDF" .


:OASISMasterType.ATL_PNODE uml:id "_E2F83E42-427A-4c63-9574-45DBC9DC7BE2" ;
                           rdfs:label "ATL_PNODE" .


:OASISMasterType.ATL_PNODE_MAP uml:id "_9EFD9A90-6E3B-47b4-9672-670B4727FE0D" ;
                               rdfs:label "ATL_PNODE_MAP" .


:OASISMasterType.ATL_PUB uml:id "_93733BE2-6729-40f6-B88B-CA7E452B4D19" ;
                         rdfs:label "ATL_PUB" .


:OASISMasterType.ATL_PUB_SCHED uml:id "_BFF4AE5B-AFA4-460f-8C51-4C91721E6A05" ;
                               rdfs:label "ATL_PUB_SCHED" .


:OASISMasterType.ATL_RESOURCE uml:id "_04D24827-0BCE-4921-9A94-12D067A59EED" ;
                              rdfs:label "ATL_RESOURCE" .


:OASISMasterType.ATL_RUC_ZONE uml:id "_22960D28-CC9B-4bd4-94C4-B6B574A9FD1A" ;
                              rdfs:label "ATL_RUC_ZONE" .


:OASISMasterType.ATL_RUC_ZONE_MAP uml:id "_0BAA6A21-0C44-427a-A69B-C915D045122C" ;
                                  rdfs:label "ATL_RUC_ZONE_MAP" .


:OASISMasterType.ATL_STAT uml:id "_BF040F44-1AB7-47bb-A39D-E2368C8CEFE5" ;
                          rdfs:label "ATL_STAT" .


:OASISMasterType.ATL_TAC_AREA uml:id "_9F7239F7-28C3-411f-A521-4FF75CCF8F6C" ;
                              rdfs:label "ATL_TAC_AREA" .


:OASISMasterType.ATL_TAC_AREA_MAP uml:id "_1943DB54-782D-4108-B160-0AB3581007B9" ;
                                  rdfs:label "ATL_TAC_AREA_MAP" .


:OASISMasterType.ATL_TI uml:id "_F13ACE5D-3311-4ab9-90FE-A3FB6892EECA" ;
                        rdfs:label "ATL_TI" .


:OASISMasterType.ATL_TIEPOINT uml:id "_DF9A2AC0-7217-4982-AD20-ECAB42DD8691" ;
                              rdfs:label "ATL_TIEPOINT" .


:OASISMasterType.ATL_XREF uml:id "_961B0A52-D629-414a-A2B4-92F9B9DFD952" ;
                          rdfs:label "ATL_XREF" .


:OASISMeasType.FACTOR uml:id "_56429AA9-A280-495a-BCB9-D76FCB1D5B32" ;
                      rdfs:label "FACTOR" .


:OASISMeasType.FLAG uml:id "_E8B65F78-DAA5-4e1c-9685-44B2455C9231" ;
                    rdfs:label "FLAG" .


:OASISMeasType.INTEGER uml:id "_FE78990C-1F68-4d05-B564-94D04FE8F980" ;
                       rdfs:label "INTEGER" .


:OASISMeasType.MW uml:id "_339C93A7-547D-4de4-8E7B-E26A489E843E" ;
                  rdfs:label "MW" .


:OASISMeasType.MWh uml:id "_781CE34A-5B6C-40fb-B341-DFEF47816A2B" ;
                   rdfs:label "MWh" .


:OASISMeasType.US_ uml:id "_BC6E1FD8-7FDA-4ff4-B646-182111BE5BE6" ;
                   rdfs:label "US$" .


:OASISMeasType.US__MW uml:id "_9CBB2EBF-97E8-4516-86FC-4188CE427A6B" ;
                      rdfs:label "US$/MW" .


:OASISMeasType.US__MWh uml:id "_090D37CE-759A-4c79-9936-C4398FF7EC63" ;
                       rdfs:label "US$/MWh" .


:OASISMeasType._ uml:id "_B9832992-2022-4f15-A831-D6E9B30EB3E3" ;
                 rdfs:label "%" .


:OASISReportType.AS_DA_RESULT uml:id "_8955B217-9509-4476-B6A9-1A9737AB8C3D" ;
                              rdfs:label "AS_DA_RESULT" .


:OASISReportType.AS_OP_RSRV uml:id "_013C3489-2F56-4d2d-9789-8585D590A9A8" ;
                            rdfs:label "AS_OP_RSRV" .


:OASISReportType.AS_REQ uml:id "_16631B8B-6486-494a-8B04-D356B36BE46C" ;
                        rdfs:label "AS_REQ" .


:OASISReportType.AS_RTM_RESULT uml:id "_6825AFA9-1B31-4ae7-B52F-5DB8860A3CA7" ;
                               rdfs:label "AS_RTM_RESULT" .


:OASISReportType.BIDS_PUBLIC uml:id "_3481F87A-B4CC-466b-85ED-D9094CC14235" ;
                             rdfs:label "BIDS_PUBLIC" .


:OASISReportType.CMMT_RA_MLC uml:id "_82420050-AB03-4032-B757-8966990E3888" ;
                             rdfs:label "CMMT_RA_MLC" .


:OASISReportType.CMMT_RMR uml:id "_E4AB8091-E2CE-4cfc-ABE9-2E9DB281F6C3" ;
                          rdfs:label "CMMT_RMR" .


:OASISReportType.CRR_CLEARING uml:id "_A5614979-9D5F-438c-A579-915E2EF79A8B" ;
                              rdfs:label "CRR_CLEARING" .


:OASISReportType.CRR_INVENTORY uml:id "_EC971F76-6FEC-4c99-A144-72A0910BF891" ;
                               rdfs:label "CRR_INVENTORY" .


:OASISReportType.ENE_EA uml:id "_46301463-ABC4-4eec-BA83-FAE8DB6FF301" ;
                        rdfs:label "ENE_EA" .


:OASISReportType.ENE_HASP uml:id "_D85AF969-E14D-4104-98C1-93FBFB6E43F5" ;
                          rdfs:label "ENE_HASP" .


:OASISReportType.ENE_IFM uml:id "_53D2DFB2-959F-4f7b-B357-478A70A65145" ;
                         rdfs:label "ENE_IFM" .


:OASISReportType.ENE_MPM uml:id "_715317F3-7BC4-43d0-9447-A2A1AD4127F3" ;
                         rdfs:label "ENE_MPM" .


:OASISReportType.ENE_RTM uml:id "_4C30E21C-CD97-4385-927E-F1D988712DC8" ;
                         rdfs:label "ENE_RTM" .


:OASISReportType.ENE_RUC uml:id "_AC4DD8D0-B4B2-459a-80F7-15714A8A7BAE" ;
                         rdfs:label "ENE_RUC" .


:OASISReportType.LOSS_DA_HASP uml:id "_F37C10BD-396D-4a5e-BE42-826D37DC6348" ;
                              rdfs:label "LOSS_DA_HASP" .


:OASISReportType.LOSS_RTM uml:id "_33DCFBCF-9E3B-4e68-A131-01E1325BBA34" ;
                          rdfs:label "LOSS_RTM" .


:OASISReportType.PRC_AS uml:id "_B6DC23AE-2E50-4990-BB19-034E63F1DDA7" ;
                        rdfs:label "PRC_AS" .


:OASISReportType.PRC_CNSTR uml:id "_C9EAB6F0-CA89-44ff-AE83-6DA7766AE6F9" ;
                           rdfs:label "PRC_CNSTR" .


:OASISReportType.PRC_FUEL uml:id "_686ECF58-5E09-4c8d-923F-AF3C24D752B3" ;
                          rdfs:label "PRC_FUEL" .


:OASISReportType.PRC_HRLY_LMP uml:id "_918D8904-1AF3-4996-B00D-9F98FC593D4D" ;
                              rdfs:label "PRC_HRLY_LMP" .


:OASISReportType.PRC_INTVL_LMP uml:id "_1213AFB9-4FC1-4159-916A-83030C56EB12" ;
                               rdfs:label "PRC_INTVL_LMP" .


:OASISReportType.SLD_FCST uml:id "_9B9B3C0F-0009-4878-947A-780E259A3F6D" ;
                          rdfs:label "SLD_FCST" .


:OASISReportType.SLD_FCST_PEAK uml:id "_95B54F49-E58F-43ca-8352-F101DA8837F4" ;
                               rdfs:label "SLD_FCST_PEAK" .


:OASISReportType.SLD_MKTS uml:id "_35847140-CCB3-451b-96E0-169C8519404A" ;
                          rdfs:label "SLD_MKTS" .


:OASISReportType.TRNS_ATC uml:id "_CCD0D373-1073-4006-8D67-A5E6941E1F50" ;
                          rdfs:label "TRNS_ATC" .


:OASISReportType.TRNS_OUTAGE uml:id "_051BD6ED-0738-46a3-A8D7-8F76F58E903A" ;
                             rdfs:label "TRNS_OUTAGE" .


:OASISReportType.TRNS_USAGE uml:id "_02BD54BA-6448-41f2-8903-DCD574869D92" ;
                            rdfs:label "TRNS_USAGE" .


:OASISStatusType.Data_Transfer_Procedure_Initiated uml:id "_6E9421EA-1B6D-4751-BEF8-ADCF623164E7" ;
                                                   rdfs:label "Data_Transfer_Procedure_Initiated" .


:OASISStatusType.Data_Transfer_Succesful uml:id "_7E0F0AAB-90B1-400c-97AF-39CFFC4B2A52" ;
                                         rdfs:label "Data_Transfer_Succesful" .


:OASISStatusType.Forced_Termination uml:id "_7EC533D0-8B75-48d8-876C-021D5CD58897" ;
                                    rdfs:label "Forced_Termination" .


:OASISStatusType.Obsolete uml:id "_901E9AB5-0506-4086-AD64-B670C04FD4C1" ;
                          rdfs:label "Obsolete" .


:OASISStatusType.Push_Failed uml:id "_3CAB7B92-80DA-475d-9164-9A37CDB57264" ;
                             rdfs:label "Push_Failed" .


:OASISStatusType.Valid uml:id "_61A40579-ACCF-4eb0-A555-48E9228E52B6" ;
                       rdfs:label "Valid" .


:OilAnalysisFluidAnalogKind.acidNumber uml:id "_EA62968A-5836-4912-96FC-D1B2066EC918" ;
                                       rdfs:comment "Acid neutralization number (in milligram of KOH/gram)." ;
                                       rdfs:label "acidNumber" .


:OilAnalysisFluidAnalogKind.additiveDBDS uml:id "_348F2398-5748-4dc0-A2CF-0CA495441945" ;
                                         rdfs:comment "Dibenzyl disulfide (DBDS) concentration (in ppm, specificially in milligram/kilogram)." ;
                                         rdfs:label "additiveDBDS" .


:OilAnalysisFluidAnalogKind.aromatics uml:id "_8DE4C341-723B-44c5-9EFF-FB49D6B9F8EA" ;
                                      rdfs:comment "Concentration of aromatic compounds determined using infrared spectroscopy (in percent)." ;
                                      rdfs:label "aromatics" .


:OilAnalysisFluidAnalogKind.carbonyl uml:id "_8071333D-BBFF-4d8e-B4CF-ED26FAD85499" ;
                                     rdfs:comment "Concentration of carbonyl compounds (aldehydes and ketones) determined using infrared spectroscopy (in percent)." ;
                                     rdfs:label "carbonyl" .


:OilAnalysisFluidAnalogKind.density uml:id "_7D9CF1D6-DB57-442e-8596-5E64A181F4D9" ;
                                    rdfs:comment "Density (in gram/millilitre)." ;
                                    rdfs:label "density" .


:OilAnalysisFluidAnalogKind.dielectricBreakdown uml:id "_6E579A27-6C31-4a23-96FA-FFB537C8A4D4" ;
                                                rdfs:comment "Dielectric breakdown, for electrode gap size and temperature specified by selected standard  (in kV)." ;
                                                rdfs:label "dielectricBreakdown" .


:OilAnalysisFluidAnalogKind.dissipationFactor uml:id "_10310F7C-E017-4ae2-9AF4-1AF5D55ADC71" ;
                                              rdfs:comment "Fluid dissipation factor in absolute value, not a percentage. (Multiplying this value by 100 would result in dissipation factor percent)." ;
                                              rdfs:label "dissipationFactor" .


:OilAnalysisFluidAnalogKind.dissipationFactorPercent uml:id "_14443118-BE6B-4030-A2F4-F250623CC4C5" ;
                                                     rdfs:comment "Fluid dissipation factor (in percent). Commonly used in Asia. Dissipation factor is also known as loss factor or tan delta." ;
                                                     rdfs:label "dissipationFactorPercent" .


:OilAnalysisFluidAnalogKind.duration61125MethodC uml:id "_E4BDAD84-6AB0-406a-BB77-726250FD48E9" ;
                                                 rdfs:comment "Duration of oxidation stablity test performed according to IEC 61125, method C. This value should accompany values resulting from testing according to IEC 61125, method C to allow interpretation. Standard specified values are: 164, 332, and 500, but others can be used if agreed upon." ;
                                                 rdfs:label "duration61125MethodC" .


:OilAnalysisFluidAnalogKind.firePoint uml:id "_88C700D3-1CF7-49fc-AF7E-3B216DB0E76B" ;
                                      rdfs:comment "Fire point (in °C). Fire point is when fire is sustained (oil catches fire). Can only be done by means of open cup test, which is commonly used in US." ;
                                      rdfs:label "firePoint" .


:OilAnalysisFluidAnalogKind.flashPointClosedCup uml:id "_DCDC3FC8-0FF6-48e0-8481-6CB822DC246D" ;
                                                rdfs:comment "Flash point (in °C) determined via closed cup test. Flash point occurs when enough vapors have accumulated to sustain a flash. Closed cup is used in Europe." ;
                                                rdfs:label "flashPointClosedCup" .


:OilAnalysisFluidAnalogKind.flashPointOpenCup uml:id "_5717DFAC-6AA3-439c-AF80-2383593F35A2" ;
                                              rdfs:comment "Flash point (in °C) determined via open cup test. Flash point occurs when enough vapors have accumulated to sustain a flash. Open cup is used in US." ;
                                              rdfs:label "flashPointOpenCup" .


:OilAnalysisFluidAnalogKind.inductionTime uml:id "_4C7519DB-230F-422d-B528-97CA2B58B91D" ;
                                          rdfs:comment "Oxidation induction time (in hours). Typically performed on new oil,but can be done on used oil." ;
                                          rdfs:label "inductionTime" .


:OilAnalysisFluidAnalogKind.inhibitor61125MethodC uml:id "_31B73E18-783C-4ea0-B3BE-FB3932F4878A" ;
                                                  rdfs:comment "Amount of inhibitor used in oxidation stablity test performed according to IEC 61125, method C. This value should accompany values resulting from testing according to IEC 61125, method  C to allow interpretation." ;
                                                  rdfs:label "inhibitor61125MethodC" .


:OilAnalysisFluidAnalogKind.interfacialTension uml:id "_D7C9525A-5061-4496-A50D-44E79E7D322C" ;
                                               rdfs:comment "Interfacial tension (in dyne/centimetre or milliNewton/metre, which are the same)." ;
                                               rdfs:label "interfacialTension" .


:OilAnalysisFluidAnalogKind.kinematicViscosity uml:id "_D7137F7C-2881-457d-8393-A05821F19E68" ;
                                               rdfs:comment "Kinematic viscosity (in millimetre2/second). Kinematic viscosity is the ratio of - absolute (or dynamic) viscosity to density." ;
                                               rdfs:label "kinematicViscosity" .


:OilAnalysisFluidAnalogKind.oxidation uml:id "_515348B1-0E0D-4ccb-8E09-A4195CC31512" ;
                                      rdfs:comment "Measure of oxidation stability (in hours)." ;
                                      rdfs:label "oxidation" .


:OilAnalysisFluidAnalogKind.oxidationInhibitorD2668 uml:id "_D227B5FC-FCE5-4776-9D09-0FEE9E6F2706" ;
                                                    rdfs:comment "2,6-ditertiary-butyl para-cresol and 2,6-ditertiary-butyl phenol concentration (in percent by weight)." ;
                                                    rdfs:label "oxidationInhibitorD2668" .


:OilAnalysisFluidAnalogKind.oxidationInhibitorDBP uml:id "_BFC0A627-0D2F-4b32-8FDA-9A02C72AEDB9" ;
                                                  rdfs:comment "2,6-ditertiary-butyl phenol (DBP) oxidation inhibitor concentration (in percent by weight)." ;
                                                  rdfs:label "oxidationInhibitorDBP" .


:OilAnalysisFluidAnalogKind.oxidationInhibitorDBPC uml:id "_55583D98-5A0F-4cba-9CE3-82E86D899035" ;
                                                   rdfs:comment "2,6-ditertiarybutyl para-cresol (DBPC) oxidation inhibitor concentration (in percent by weight)." ;
                                                   rdfs:label "oxidationInhibitorDBPC" .


:OilAnalysisFluidAnalogKind.passivatorBTA uml:id "_FFF7B11A-49C9-45cc-AF9C-880575B68238" ;
                                          rdfs:comment "Metal passivator BTA content (in milligram/kilogram)." ;
                                          rdfs:label "passivatorBTA" .


:OilAnalysisFluidAnalogKind.passivatorContent uml:id "_E0753296-A772-4444-BB51-A67E9F2CC8F3" ;
                                              rdfs:comment "Total passivator content (in milligram/kilogram)." ;
                                              rdfs:label "passivatorContent" .


:OilAnalysisFluidAnalogKind.passivatorIrgamet39 uml:id "_8EF918C2-5374-44d1-A6B0-CBC8CAD24133" ;
                                                rdfs:comment "Irgamet 39 metal passivator content (in ppm, specifically milligram/kilogram)." ;
                                                rdfs:label "passivatorIrgamet39" .


:OilAnalysisFluidAnalogKind.passivatorTTA uml:id "_83D3CF86-D8F4-4c9a-919D-82A0EB3C5685" ;
                                          rdfs:comment "Metal passivator TTA (Irgamet39 in solid form) content (in milligram/kilogram)." ;
                                          rdfs:label "passivatorTTA" .


:OilAnalysisFluidAnalogKind.petroleumOrigin uml:id "_440F6C36-3BC3-41fc-8FE0-A07E549AD208" ;
                                            rdfs:comment "Characterization of the carbon-type composition of insulating oils by petroleum origin." ;
                                            rdfs:label "petroleumOrigin" .


:OilAnalysisFluidAnalogKind.pourPoint uml:id "_6F9848EC-066F-4195-85F7-A66AD42AF418" ;
                                      rdfs:comment "Pour point (in °C). The pour point of a liquid is the temperature at which it becomes semi solid and loses its flow characteristics." ;
                                      rdfs:label "pourPoint" .


:OilAnalysisFluidAnalogKind.pourPointAutomatic uml:id "_163297AB-0341-4a14-9572-FB241DE6E728" ;
                                               rdfs:comment "Pour point (in °C) determined by automatic method. The pour point of a liquid is the temperature at which it becomes semi solid and loses its flow characteristics." ;
                                               rdfs:label "pourPointAutomatic" .


:OilAnalysisFluidAnalogKind.powerFactorPercent uml:id "_E3056614-86DA-47a2-9928-58E512BF58E0" ;
                                               rdfs:comment "Fluid power factor at specified temperature (in percent). Commonly used in US. (Note: Fluid power factor is very similar to fluid dissapation factor, but fluid power factor is cosine of the phase angle between an AC voltage applied to oil and the resulting current (where dissipation factor is the tangent). For values up to 0.005, fluid power factor and dissapation factor are very close. There is a conversion equation between the two)." ;
                                               rdfs:label "powerFactorPercent" .


:OilAnalysisFluidAnalogKind.resistivity uml:id "_859EE86C-2EDD-40cd-AAC5-AF9C3257295E" ;
                                        rdfs:comment "Resistivity at 90°C (in gigohm-metre)." ;
                                        rdfs:label "resistivity" .


:OilAnalysisFluidAnalogKind.sedimentAndSludgePercent uml:id "_A843C22C-1A80-46e5-8449-5B3059CEFD86" ;
                                                     rdfs:comment "Sediment and sludge (in percent)." ;
                                                     rdfs:label "sedimentAndSludgePercent" .


:OilAnalysisFluidAnalogKind.sludge uml:id "_5F669E6A-2BE1-491f-9A43-F6B1FD8B61D1" ;
                                   rdfs:comment "Sludge (in percent by mass). Typically performed on new oil,but can be done on used oil." ;
                                   rdfs:label "sludge" .


:OilAnalysisFluidAnalogKind.solubleAcids uml:id "_52381B9E-55E3-4fdb-9E01-C6D743ED208C" ;
                                         rdfs:comment "Soluble acids  (in milligram of KOH/gram). Typically performed on new oil,but can be done on used oil." ;
                                         rdfs:label "solubleAcids" .


:OilAnalysisFluidAnalogKind.specificGravity uml:id "_53990F3A-B60E-49db-AEEF-543D0CEE6D16" ;
                                            rdfs:comment "Specific gravity corrected to 15°C. Also known as relative density. It is a ratio of density of tested oil to density of water at a specific temperature." ;
                                            rdfs:label "specificGravity" .


:OilAnalysisFluidAnalogKind.staticElectrification uml:id "_6BB070EC-F9A8-46cd-B9F1-6BEF3DB2CFD0" ;
                                                  rdfs:comment "Static electrification tendency (in microcoulombs per metre3). Also called static charging tendency and electrostatic charging tendency (ECT)." ;
                                                  rdfs:label "staticElectrification" .


:OilAnalysisFluidAnalogKind.totalAcids uml:id "_64510F91-6AD6-4d69-AA89-8358309FD2B9" ;
                                       rdfs:comment "Total acids (soluble plus volatile) (in milligram of KOH/gram). Typically performed on new oil,but can be done on used oil." ;
                                       rdfs:label "totalAcids" .


:OilAnalysisFluidAnalogKind.volatileAcids uml:id "_8F4A4022-A015-44b8-B70B-63062F12ACB2" ;
                                          rdfs:comment "Volatile acids (in milligram of KOH/gram). Typically performed on new oil,but can be done on used oil." ;
                                          rdfs:label "volatileAcids" .


:OilAnalysisFluidDiscreteKind.colorNumber uml:id "_47B514FF-F464-4e62-90CE-CEFCCAA496E2" ;
                                          rdfs:comment """Fluid color index number.  Color numbers are expressed in 0.5 intervals and value specified is  \"less-than\". For example, a value of '2.5' means the color index number is between 2.0 and 2.5.
Possible values: 0.5, 1.0, 1.5, 2.0, 2.5, 3.0, 3.5, 4.0, 4.5, 5.0, 5.5, 6.0, 6.5, 7.0, 7.5, 8.0.""" ;
                                          rdfs:label "colorNumber" .


:OilAnalysisFluidDiscreteKind.colorNumberPlatinumCobaltScale uml:id "_1B07B7C0-0BBF-4720-BE97-F983A56953E0" ;
                                                             rdfs:comment """Fluid color index on the platinum cobalt scale. 
Possible values: 5, 10, 15, 20, 25, 30, 35, 40, 50, 60, 70, 100, 150, 200, 250, 300, 350, 400, 450.""" ;
                                                             rdfs:label "colorNumberPlatinumCobaltScale" .


:OilAnalysisFluidDiscreteKind.corrosiveSulphurBy51353 uml:id "_315CA497-944C-42a0-9496-A7523CA85EC2" ;
                                                      rdfs:comment """Corrosive sulphur test result using silver strip test.
Possible values: absent, present.""" ;
                                                      rdfs:label "corrosiveSulphurBy51353" .


:OilAnalysisFluidDiscreteKind.corrosiveSulphurBy62535 uml:id "_AEFD7B93-FC55-45a1-9D4A-BA0BC783D178" ;
                                                      rdfs:comment """Corrosive sulphur test result using covered (copper) conductor deposition test.
Possible values: potentiallyCorrosive, nonCorrosive.""" ;
                                                      rdfs:label "corrosiveSulphurBy62535" .


:OilAnalysisFluidDiscreteKind.corrosiveSulphurByD1275 uml:id "_50CD2F88-BB28-4ea5-8E28-259278AC0647" ;
                                                      rdfs:comment """Corrosive sulphur test result using bare copper strip test.
Possible values: corrosive, nonCorrosive.""" ;
                                                      rdfs:label "corrosiveSulphurByD1275" .


:OilAnalysisFluidDiscreteKind.sludgePrecipitation uml:id "_9A8C7490-BE9C-403c-9028-B6B038EAAB87" ;
                                                  rdfs:comment """Sludge precipitation test results.
Possible values: present, notPresent.""" ;
                                                  rdfs:label "sludgePrecipitation" .


:OilAnalysisFluidDiscreteKind.tarnishLevel uml:id "_1DA9473F-9733-4b10-8CD9-FA4EB83E70DF" ;
                                           rdfs:comment """Tarnish level indicated by corrosive sulphur test.
Possible values: 1A, 1B, 2A, 2B, 2C, 2D, 2E, 3A, 3B, 4A, 4B, 4C.""" ;
                                           rdfs:label "tarnishLevel" .


:OilAnalysisGasAnalogKind.acetylene uml:id "_D757B45E-1A01-4eda-983B-B00C1E3ABF71" ;
                                    rdfs:comment "C2H2 concentration (in ppm, specifically in microlitre/litre)." ;
                                    rdfs:label "acetylene" .


:OilAnalysisGasAnalogKind.butane uml:id "_8FA00F89-C563-4f6a-A724-813779AFFB1C" ;
                                 rdfs:comment "C4H10 concentration (in ppm, specifically in microlitre/litre)." ;
                                 rdfs:label "butane" .


:OilAnalysisGasAnalogKind.carbon uml:id "_BAA8601B-D854-4cb7-B43A-62A11724DB69" ;
                                 rdfs:comment "C? concentration (in ppm, specifically in microlitre/litre)." ;
                                 rdfs:label "carbon" .


:OilAnalysisGasAnalogKind.carbon3 uml:id "_FD66D149-B950-4a3c-8E94-8D5D2B12F925" ;
                                  rdfs:comment "C3 concentration (in ppm, specifically in microlitre/litre)." ;
                                  rdfs:label "carbon3" .


:OilAnalysisGasAnalogKind.carbon4 uml:id "_47D2CCF6-8BF3-4bfa-97CD-1CE2F6DF61ED" ;
                                  rdfs:comment "C4 concentration (in ppm, specifically in microlitre/litre)." ;
                                  rdfs:label "carbon4" .


:OilAnalysisGasAnalogKind.carbonDioxide uml:id "_3CFB3884-BCE4-4e01-BDFC-EF5B74320700" ;
                                        rdfs:comment "CO2 concentration (in ppm, specifically in microlitre/litre)." ;
                                        rdfs:label "carbonDioxide" .


:OilAnalysisGasAnalogKind.carbonMonoxide uml:id "_EC4225E4-10CC-432c-A855-48CD2FDD8C62" ;
                                         rdfs:comment "CO concentration (in ppm, specifically in microlitre/litre)." ;
                                         rdfs:label "carbonMonoxide" .


:OilAnalysisGasAnalogKind.equivalentTCGPercent uml:id "_9B15B421-69B6-47b2-96B6-4C811143D0A8" ;
                                               rdfs:comment """Equivalent Total Combustible Gas (ETCG) percent.
An estimate, calculated from the dissolved-gas concentrations and the oil sample temperature, of what the TCG would be in a gas space in equilibrium with the oil. ETCG reflects what the TCG would be in air spaces near the oil.""" ;
                                               rdfs:label "equivalentTCGPercent" .


:OilAnalysisGasAnalogKind.estimatedSafeHandlingLimit uml:id "_D6A254A2-816D-47a2-A4A0-E7A1AA451AF6" ;
                                                     rdfs:comment """Estimated Safe Handling Limit (ESHL) (in percent). Estimated safe handling limit is an estimate of the lower flammability limit (LFL) of the combustible gas mixture which the dissolved gas in the oil would give off by the oil if exposed to air. 
Expressed in percent like the equivalent total combustible gas percent, it is calculated from the dissolved-gas concentrations, the oil sample temperature, and the lower flammability limits of the individual combustible gases.""" ;
                                                     rdfs:label "estimatedSafeHandlingLimit" .


:OilAnalysisGasAnalogKind.ethane uml:id "_A9B4300D-FB25-4898-8CFD-AE3949929F58" ;
                                 rdfs:comment "C2H6 concentration (in ppm, specifically in microlitre/litre)." ;
                                 rdfs:label "ethane" .


:OilAnalysisGasAnalogKind.ethylene uml:id "_F3747D79-11C0-4757-A542-8498D4127999" ;
                                   rdfs:comment "C2H4 concentration (in ppm, specifically in microlitre/litre)." ;
                                   rdfs:label "ethylene" .


:OilAnalysisGasAnalogKind.hydran uml:id "_C6BC71B4-C7C8-432b-B9F6-54DF65F63687" ;
                                 rdfs:comment """Measured composite of dissolved fault gas concentrations (in ppm, specifically in microlitre/litre). Relative sensitivity
- H2: 100 % of concentration
- CO: 15 ± 4 % of concentration
- C2H2: 8 ± 2 % of concentration
- C2H4: 1.5 ± 0.5 % of concentration.""" ;
                                 rdfs:label "hydran" .


:OilAnalysisGasAnalogKind.hydranPredicted uml:id "_8240D451-33B1-417e-BDFD-ED4F7803D3BB" ;
                                          rdfs:comment """Predicted hydran value (in ppm, specifically in microlitre/litre), calculated based on individual measured dissolved gas concentrations.
- H2: 100 % of concentration
- CO: 15 ± 4 % of concentration
- C2H2: 8 ± 2 % of concentration
- C2H4: 1.5 ± 0.5 % of concentration""" ;
                                          rdfs:label "hydranPredicted" .


:OilAnalysisGasAnalogKind.hydrogen uml:id "_69B8250F-0E6C-4db1-B6D6-A532243DA5A5" ;
                                   rdfs:comment "H2 concentration (in ppm, specifically in microlitre/litre)." ;
                                   rdfs:label "hydrogen" .


:OilAnalysisGasAnalogKind.isobutane uml:id "_30B0ECE9-507A-4620-BBB8-8A36B263F982" ;
                                    rdfs:comment "isoC4 (C4H10) concentration (in ppm, specifically in microlitre/litre). Isobutane is also known as methylpropane." ;
                                    rdfs:label "isobutane" .


:OilAnalysisGasAnalogKind.methane uml:id "_87B8A5B3-259E-4a71-AD91-71345085515A" ;
                                  rdfs:comment "CH4 concentration (in ppm, specifically in microlitre/litre)." ;
                                  rdfs:label "methane" .


:OilAnalysisGasAnalogKind.nitrogen uml:id "_D6B5FF9F-1720-4f78-AEEF-8BACB0EF00D5" ;
                                   rdfs:comment "N2 concentration (in ppm, specifically in microlitre/litre)." ;
                                   rdfs:label "nitrogen" .


:OilAnalysisGasAnalogKind.oxygen uml:id "_9179BBA2-489B-40c9-B97F-E899A4CFED32" ;
                                 rdfs:comment "O2 concentration (in ppm, specifically in microlitre/litre)." ;
                                 rdfs:label "oxygen" .


:OilAnalysisGasAnalogKind.propane uml:id "_43AD7A4F-7613-4fcd-8B51-6C62FD3CD90D" ;
                                  rdfs:comment "C3H8 concentration (in ppm, specifically in microlitre/litre)." ;
                                  rdfs:label "propane" .


:OilAnalysisGasAnalogKind.propene uml:id "_18ED09E8-916A-4a46-97BA-71214DE98105" ;
                                  rdfs:comment "C3H6 concentration (in ppm, specifically in microlitre/litre)." ;
                                  rdfs:label "propene" .


:OilAnalysisGasAnalogKind.totalCombustibleGasPercent uml:id "_59569A7A-B7B7-4de7-BF4D-8582DD24AFA3" ;
                                                     rdfs:comment "Total Combustible Gas (TCG) measured in headspace (in percent by volume)." ;
                                                     rdfs:label "totalCombustibleGasPercent" .


:OilAnalysisGasAnalogKind.totalDissolvedCombustibleGas uml:id "_E97A1E46-CE98-4be1-BCB3-75F60A695FC8" ;
                                                       rdfs:comment "Total dissolved combustible gas concentration (in ppm, specifically in microlitre/litre). Calculated by adding the ppm of combustible gasses: hydrogen (H2), methane (CH4), ethane (C2H6), ethylene (C2H4), acetylene (C2H2), and carbon monoxide (CO)." ;
                                                       rdfs:label "totalDissolvedCombustibleGas" .


:OilAnalysisGasAnalogKind.totalDissolvedGasPercent uml:id "_B7A63877-2518-44cc-9153-37A32056F92D" ;
                                                   rdfs:comment "Total dissolved gas in oil (in percent by volume). Derived from the total area of all the gas peaks in the chromatogram." ;
                                                   rdfs:label "totalDissolvedGasPercent" .


:OilAnalysisGasAnalogKind.totalHeatGas uml:id "_5DC499DF-E61E-4986-BA0F-1BF2CF889100" ;
                                       rdfs:comment "Sum of concentrations of methane, ethane, and ethylene (in ppm, specifically in microlitre/litre). Used in some diagnostic gas ratios, especially THG/acetylene, which compares “heat gas” to “arcing gas.”" ;
                                       rdfs:label "totalHeatGas" .


:OilAnalysisGasAnalogKind.totalPartialPressure uml:id "_D834A885-C0A9-45b3-9536-7DEFDF7E2C32" ;
                                               rdfs:comment """Total partial pressure (in Pa).
Calculated value reflecting total of partial pressures of all combustible gasses.""" ;
                                               rdfs:label "totalPartialPressure" .


:OilAnalysisMetalsAnalogKind.aluminum uml:id "_17DCA08D-62B6-4148-9B9E-E313AC70B4AC" ;
                                      rdfs:comment "Aluminum concentration (in ppb, specifically in microgram/litre)." ;
                                      rdfs:label "aluminum" .


:OilAnalysisMetalsAnalogKind.aluminumParticulate uml:id "_F46760EB-7042-424d-914E-9FADB9A002AB" ;
                                                 rdfs:comment "Aluminum concentration of particles larger than 0.45 microns  (in ppb,specifically in microgram/litre)." ;
                                                 rdfs:label "aluminumParticulate" .


:OilAnalysisMetalsAnalogKind.barium uml:id "_762E4BD5-6BF7-4791-8FAD-EBA3D37B7E10" ;
                                    rdfs:comment "Barium concentration (in ppb, specifically in microgram/litre)." ;
                                    rdfs:label "barium" .


:OilAnalysisMetalsAnalogKind.boron uml:id "_72161B34-917C-44e4-B9A1-1FBFAAC5AD9C" ;
                                   rdfs:comment "Boron concentration (in ppb, specifically in microgram/litre)." ;
                                   rdfs:label "boron" .


:OilAnalysisMetalsAnalogKind.cadmium uml:id "_49B16F68-43AA-4fcd-AED1-B786D46A7AE2" ;
                                     rdfs:comment "Cadmium concentration (in ppb, specifically in microgram/litre)." ;
                                     rdfs:label "cadmium" .


:OilAnalysisMetalsAnalogKind.calcium uml:id "_0172B0DC-DCF5-48bb-AD04-7656ED1535E4" ;
                                     rdfs:comment "Calcium concentration (in ppb, specifically in microgram/litre)." ;
                                     rdfs:label "calcium" .


:OilAnalysisMetalsAnalogKind.chromium uml:id "_7D087ACE-558C-46c0-8A53-1F06A0C82B3F" ;
                                      rdfs:comment "Chromium concentration (in ppb, specifically in microgram/litre)." ;
                                      rdfs:label "chromium" .


:OilAnalysisMetalsAnalogKind.copper uml:id "_1CCE608D-DC85-444a-A16F-85E381C8F009" ;
                                    rdfs:comment "Copper concentration (in ppb, specifically in microgram/litre)." ;
                                    rdfs:label "copper" .


:OilAnalysisMetalsAnalogKind.copperParticulate uml:id "_9A628B6D-BD54-49e6-A59B-E84CB4049EB1" ;
                                               rdfs:comment "Copper concentration of particles larger than 0.45 microns  (in ppb,specifically in microgram/litre)." ;
                                               rdfs:label "copperParticulate" .


:OilAnalysisMetalsAnalogKind.iron uml:id "_9F595E14-F28E-4925-862F-C8A7726C2B04" ;
                                  rdfs:comment "Iron concentration (in ppb, specifically in microgram/litre)." ;
                                  rdfs:label "iron" .


:OilAnalysisMetalsAnalogKind.ironParticulate uml:id "_9D33052E-0563-4f02-A18C-0C634638CBD8" ;
                                             rdfs:comment "Iron concentration of particles larger than 0.45 microns (in ppb, specifically in microgram/litre)." ;
                                             rdfs:label "ironParticulate" .


:OilAnalysisMetalsAnalogKind.lead uml:id "_F9A54FFB-6B17-4d3e-88A6-3A9060D0D6FE" ;
                                  rdfs:comment "Lead concentration (in ppb, specifically in microgram/litre)." ;
                                  rdfs:label "lead" .


:OilAnalysisMetalsAnalogKind.leadParticulate uml:id "_280F0251-EBA9-41e0-B23A-B4DEC74E9FBE" ;
                                             rdfs:comment "Lead concentration of particles larger than 0.45 microns (in ppb, specifically in microgram/litre)." ;
                                             rdfs:label "leadParticulate" .


:OilAnalysisMetalsAnalogKind.lithium uml:id "_BC7DB6A9-1F3C-4e1a-B3F8-C080ACF60D2B" ;
                                     rdfs:comment "Lithium concentration (in ppb, specifically in microgram/litre)." ;
                                     rdfs:label "lithium" .


:OilAnalysisMetalsAnalogKind.magnesium uml:id "_0E2FAF32-F948-45e0-975D-F2373BD69979" ;
                                       rdfs:comment "Magnesium concentration (in ppb, specifically in microgram/litre)." ;
                                       rdfs:label "magnesium" .


:OilAnalysisMetalsAnalogKind.molybdenum uml:id "_753E261C-2C69-4541-B9D9-5A7B4D41EBB5" ;
                                        rdfs:comment "Molybdenum concentration (in ppb, specifically in microgram/litre)." ;
                                        rdfs:label "molybdenum" .


:OilAnalysisMetalsAnalogKind.nickel uml:id "_89189794-32FB-4a4d-BA21-0B6CF4F91795" ;
                                    rdfs:comment "Nickel concentration (in ppb, specifically in microgram/litre)." ;
                                    rdfs:label "nickel" .


:OilAnalysisMetalsAnalogKind.phosphorus uml:id "_73689953-2083-4f9e-96F1-A8D037932AAB" ;
                                        rdfs:comment "Phosphorus concentration (in ppb, specifically in microgram/litre)." ;
                                        rdfs:label "phosphorus" .


:OilAnalysisMetalsAnalogKind.silicon uml:id "_70F85A0A-C182-4bf4-B8EF-6DCB432FC79B" ;
                                     rdfs:comment "Silicon concentration (in ppb, specifically in microgram/litre)." ;
                                     rdfs:label "silicon" .


:OilAnalysisMetalsAnalogKind.silver uml:id "_C8527BE1-A94E-47ff-BD57-BBA548FF42A2" ;
                                    rdfs:comment "Silver concentration (in ppb, specifically in microgram/litre)." ;
                                    rdfs:label "silver" .


:OilAnalysisMetalsAnalogKind.silverParticulate uml:id "_062B08F8-82A6-466b-BCED-72BCABB350C6" ;
                                               rdfs:comment "Silver concentration of particles larger than 0.45 microns (in ppb, specifically in microgram/litre)." ;
                                               rdfs:label "silverParticulate" .


:OilAnalysisMetalsAnalogKind.sodium uml:id "_0BA34E08-C4B6-4035-AC38-ACC9301C678C" ;
                                    rdfs:comment "Sodium concentration (in ppb, specifically in microgram/litre)." ;
                                    rdfs:label "sodium" .


:OilAnalysisMetalsAnalogKind.tin uml:id "_FD171027-DC47-4a48-9A05-BD6E21C3E45B" ;
                                 rdfs:comment "Tin concentration (in ppb, specifically in microgram/litre)." ;
                                 rdfs:label "tin" .


:OilAnalysisMetalsAnalogKind.titanium uml:id "_13CD8AA7-F0D6-4262-A932-AB292E665BE8" ;
                                      rdfs:comment "Titanium concentration (in ppb, specifically in microgram/litre)." ;
                                      rdfs:label "titanium" .


:OilAnalysisMetalsAnalogKind.tungsten uml:id "_9F966012-108B-496f-A399-E39D7F50F68E" ;
                                      rdfs:comment "Tungsten concentration (in ppb, specifically in microgram/litre)." ;
                                      rdfs:label "tungsten" .


:OilAnalysisMetalsAnalogKind.vanadium uml:id "_32889D93-83D0-4e61-A2C2-5F5FDF14152C" ;
                                      rdfs:comment "Vanadium concentration (in ppb, specifically in microgram/litre)." ;
                                      rdfs:label "vanadium" .


:OilAnalysisMetalsAnalogKind.zinc uml:id "_70A2B5AC-9580-4edf-AEC3-08BB84A14204" ;
                                  rdfs:comment "Zinc concentration (in ppb, specifically in microgram/litre)." ;
                                  rdfs:label "zinc" .


:OilAnalysisMetalsAnalogKind.zincParticulate uml:id "_472236F7-C8F7-41f7-B6DC-0FBF382A7E5C" ;
                                             rdfs:comment "Zinc concentration of particles larger than 0.45 microns (in ppb, specifically in microgram/litre)." ;
                                             rdfs:label "zincParticulate" .


:OilAnalysisMoistureAnalogKind.dewPoint uml:id "_4FDA2D66-EDBE-474c-A873-38BE9CA39010" ;
                                        rdfs:comment "Dew point (in °C). Is usually a negative value." ;
                                        rdfs:label "dewPoint" .


:OilAnalysisMoistureAnalogKind.relativeSaturation uml:id "_18C50D2D-9673-4aec-A152-0765E797C91A" ;
                                                  rdfs:comment "Relative saturation of water in fluid (in percent)." ;
                                                  rdfs:label "relativeSaturation" .


:OilAnalysisMoistureAnalogKind.relativeSaturationCalculated uml:id "_65D8B50E-0102-4a32-8A4B-A9E5D0D426BC" ;
                                                            rdfs:comment "Calculated relative saturation of water in fluid (in percent)." ;
                                                            rdfs:label "relativeSaturationCalculated" .


:OilAnalysisMoistureAnalogKind.waterContent uml:id "_6B374D99-6372-4af3-B8ED-AA2D8C1FC9CD" ;
                                            rdfs:comment "Moisture measured via coulometric Karl Fischer titration (in ppm, specifically milligram/kilogram)." ;
                                            rdfs:label "waterContent" .


:OilAnalysisMoistureAnalogKind.waterContentMonitoredViaAluminumOxide uml:id "_50ECF030-05FA-4ed1-B2F3-D9BBB8597192" ;
                                                                     rdfs:comment "Water content by aluminum oxide sensor (in ppm, specifically milligram/kilogram)." ;
                                                                     rdfs:label "waterContentMonitoredViaAluminumOxide" .


:OilAnalysisMoistureAnalogKind.waterContentMonitoredViaCapacitance uml:id "_946F3767-AD07-49bb-B1D4-D6974E72909E" ;
                                                                   rdfs:comment "Water content by capacitance sensor (in ppm, specifically milligram/kilogram)." ;
                                                                   rdfs:label "waterContentMonitoredViaCapacitance" .


:OilAnalysisMoistureAnalogKind.waterContentMonitoredViaInfrared uml:id "_2A92752E-FFE4-431e-9580-EBEAB277E31E" ;
                                                                rdfs:comment "Water content by infrared sensor (in ppm, specifically milligram/kilogram)." ;
                                                                rdfs:label "waterContentMonitoredViaInfrared" .


:OilAnalysisMoistureAnalogKind.waterContentMonitoredViaOther uml:id "_CEC833FE-C79C-44c8-B382-2F599A35B3DA" ;
                                                             rdfs:comment "Water content by other sensor (in ppm, specifically milligram/kilogram)." ;
                                                             rdfs:label "waterContentMonitoredViaOther" .


:OilAnalysisPCBAnalogKind.aroclor1016 uml:id "_A28795EE-953F-4f0c-8307-B7E56800B9F3" ;
                                      rdfs:comment "Concentration of Aroclor 1016 (in ppm, specifically in mg/kg)." ;
                                      rdfs:label "aroclor1016" .


:OilAnalysisPCBAnalogKind.aroclor1221 uml:id "_5F3DE9EE-CF65-43eb-A462-DA095A2BC4DB" ;
                                      rdfs:comment "Concentration of Aroclor 1221 (in ppm, specifically in mg/kg)." ;
                                      rdfs:label "aroclor1221" .


:OilAnalysisPCBAnalogKind.aroclor1242 uml:id "_8097DF99-75A3-4132-A566-79DAFA51A7C0" ;
                                      rdfs:comment "Concentration of Aroclor 1242 (in ppm, specifically in mg/kg)." ;
                                      rdfs:label "aroclor1242" .


:OilAnalysisPCBAnalogKind.aroclor1254 uml:id "_446426F1-9751-4204-9939-FEE4E1C95E5F" ;
                                      rdfs:comment "Concentration of Aroclor 1254 (in ppm, specifically in mg/kg)." ;
                                      rdfs:label "aroclor1254" .


:OilAnalysisPCBAnalogKind.aroclor1260 uml:id "_C5171055-5800-433f-8AB0-C3A3BAB98538" ;
                                      rdfs:comment "Concentration of Aroclor 1260 (in ppm, specifically in mg/kg)." ;
                                      rdfs:label "aroclor1260" .


:OilAnalysisPCBAnalogKind.totalPCB uml:id "_81470642-F1AB-4053-8226-0B72C5C2D5EC" ;
                                   rdfs:comment "Total arochlor (PCB) content (in ppm, specifically in mg/kg). Is the sum of Aroclor 1221, Aroclor 1242, Aroclor 1254, Aroclor 1260, Aroclor 1016." ;
                                   rdfs:label "totalPCB" .


:OilAnalysisPCBDiscreteKind.testKitPCB uml:id "_861A70F8-2810-4ed7-83F0-59827C8CDF4A" ;
                                       rdfs:comment "Possible values:  <blank>, <50, >50." ;
                                       rdfs:label "testKitPCB" .


:OilAnalysisPaperAnalogKind.acetylfuran uml:id "_A076A658-82BC-4bb8-A0B8-9C0DB7EC0C50" ;
                                        rdfs:comment "2-acetylfuran (2ACF) (in ppb). Also known as: 2-acetylfuran, furyl methyl ketone, 2-furyl methyl ketone, methyl 2-furyl ketone, and 1-(2-furanyl)ethanone." ;
                                        rdfs:label "acetylfuran" .


:OilAnalysisPaperAnalogKind.degreeOfPolymerization uml:id "_584EC2A1-D383-4e02-BEEA-631686EC49A3" ;
                                                   rdfs:comment "Direct measurement of degree of polymerization (DP) (unitless)." ;
                                                   rdfs:label "degreeOfPolymerization" .


:OilAnalysisPaperAnalogKind.degreeOfPolymerizationCalculated uml:id "_986495CC-A919-4b2e-AF60-6D516184F3B2" ;
                                                             rdfs:comment "Calculated degree of polymerization (DP) calculated using the Chendong equation (unitless)." ;
                                                             rdfs:label "degreeOfPolymerizationCalculated" .


:OilAnalysisPaperAnalogKind.ethanol uml:id "_D7969551-DCE1-4f96-B717-913113BF0EEF" ;
                                    rdfs:comment "Concentration of ethanol (in ppb, specifically microgram/kilogram)." ;
                                    rdfs:label "ethanol" .


:OilAnalysisPaperAnalogKind.furfural uml:id "_0346BDA9-5F5B-4d4a-9F30-1B03AEC3E449" ;
                                     rdfs:comment "2-furaldehyde (2FAL) (in ppb). Also known as: 2-furfural, 2-furaldehyde, 2-furanaldehyde, fural, furfuraldehyde, furaldehyde, and 2-furancarboxaldehyde." ;
                                     rdfs:label "furfural" .


:OilAnalysisPaperAnalogKind.furfurylAlcohol uml:id "_FBA23766-2F78-4eea-94CC-EB08A04D1CAD" ;
                                            rdfs:comment "Furfuryl alcohol (2FOL) (in ppb). Also known as: 2-furyl alcohol, 2-furfurol, 2-furylmethanol, 2-hydroxymethylfuran, 2-furancarbinol, furancarbinol, 2-furanmethanol, furanmethanol, furfural alcohol, and alpha-furylcarbinol." ;
                                            rdfs:label "furfurylAlcohol" .


:OilAnalysisPaperAnalogKind.hydroxymethylfurfural uml:id "_F270D195-B6B4-4a9c-8EC4-7FD3AAC49E3B" ;
                                                  rdfs:comment "5-hydroxymethyl-2-furaldehyde (5H2F) (in ppb). Also known as: 5-hydroxymethyl-2-furfural, 5-hydroxymethyl-2-furaldehyde, 5-hydroxymethylfurfuraldehyde, and 5-hydroxymethylfurfural." ;
                                                  rdfs:label "hydroxymethylfurfural" .


:OilAnalysisPaperAnalogKind.methanol uml:id "_084035F9-F071-46a2-BB07-A94E1FC405F3" ;
                                     rdfs:comment "Concentration of methanol (in ppb, specifically microgram/kilogram)." ;
                                     rdfs:label "methanol" .


:OilAnalysisPaperAnalogKind.methylfurfural uml:id "_F697DD40-AD0D-4f5b-A829-6F2839CEF7B5" ;
                                           rdfs:comment "5-methyl-2-furaldehyde (5M2F) (in ppb). Also known as: 5-methyl-2-furfural, 5-methyl-2-furaldehyde, 5-methyl-2-furfuraldehyde, and 5-methylfurfural." ;
                                           rdfs:label "methylfurfural" .


:OilAnalysisPaperAnalogKind.solidInsulationDielectricStrength uml:id "_9F6CB3D7-68F3-4144-BC21-891B0C5F1A77" ;
                                                              rdfs:comment "Dielectric breakdown of solid electrical insulating materials (in kV)." ;
                                                              rdfs:label "solidInsulationDielectricStrength" .


:OilAnalysisPaperAnalogKind.tensileStrength uml:id "_3BE11B10-FB4F-455f-B9BC-4DD9E233F3A0" ;
                                            rdfs:comment "Tensile strength (in kilonewtons/metre)." ;
                                            rdfs:label "tensileStrength" .


:OilAnalysisPaperAnalogKind.totalFuran uml:id "_23C788DC-BD88-4474-BB28-4CF458B88ED6" ;
                                       rdfs:comment "Total furan (in ppb). Is the total of the concentrations of 5-hydroxymethyl-2-furaldehyde (5H2F), furfuryl alcohol (2FOL), 2-furaldehyde (2FAL), 2-acetylfuran (2ACF), 5-methyl-2-furaldehyde (5M2F)." ;
                                       rdfs:label "totalFuran" .


:OilAnalysisParticleAnalogKind.carbonPercent uml:id "_7E5477A1-717F-40c2-A994-CAC82E3460E2" ;
                                             rdfs:comment "Percent of particles which are carbon." ;
                                             rdfs:label "carbonPercent" .


:OilAnalysisParticleAnalogKind.count100Plus uml:id "_83B5CE60-B87E-4a18-8FDA-9174FA526DE8" ;
                                            rdfs:comment "Count of particles 100 microns and larger in a 1 millilitre sample." ;
                                            rdfs:label "count100Plus" .


:OilAnalysisParticleAnalogKind.count10Plus uml:id "_37037689-A25F-46eb-A03B-377E77F665BE" ;
                                           rdfs:comment "Count of particles 10 microns and larger in a 1 millilitre sample." ;
                                           rdfs:label "count10Plus" .


:OilAnalysisParticleAnalogKind.count14Plus uml:id "_F9A2C61C-CA7C-4e83-BA96-DDFF88016C85" ;
                                           rdfs:comment "Count of particles 14 microns and larger in a 1 millilitre sample." ;
                                           rdfs:label "count14Plus" .


:OilAnalysisParticleAnalogKind.count15Plus uml:id "_DFE34C41-2794-42f2-85AF-7D9BD748E3C9" ;
                                           rdfs:comment "Count of particles 15 microns and larger in a 1 millilitre sample." ;
                                           rdfs:label "count15Plus" .


:OilAnalysisParticleAnalogKind.count21Plus uml:id "_87ABB61C-CF9E-4eb0-BD21-2E55AF15DEF5" ;
                                           rdfs:comment "Count of particles 21 microns and larger in a 1 millilitre sample." ;
                                           rdfs:label "count21Plus" .


:OilAnalysisParticleAnalogKind.count25Plus uml:id "_A3251E03-D5E2-43d1-98CF-D7E553899876" ;
                                           rdfs:comment "Count of particles 25 microns and larger in a 1 millilitre sample." ;
                                           rdfs:label "count25Plus" .


:OilAnalysisParticleAnalogKind.count2Plus uml:id "_57F2E7CD-82AB-4007-805F-75EB227E6515" ;
                                          rdfs:comment "Count of particles 2 microns and larger in a 1 millilitre sample." ;
                                          rdfs:label "count2Plus" .


:OilAnalysisParticleAnalogKind.count38Plus uml:id "_9D27BF17-B560-4963-9767-5C23E5867A08" ;
                                           rdfs:comment "Count of particles 38 microns and larger in a 1 millilitre sample." ;
                                           rdfs:label "count38Plus" .


:OilAnalysisParticleAnalogKind.count4Plus uml:id "_047DF64A-51D3-4c29-B440-17137F69995F" ;
                                          rdfs:comment "Count of particles 4 microns and larger in a 1 millilitre sample." ;
                                          rdfs:label "count4Plus" .


:OilAnalysisParticleAnalogKind.count50Plus uml:id "_9D5C842D-CC06-4804-BA81-5F4AC9E8BBDD" ;
                                           rdfs:comment "Count of particles 50 microns and larger in a 1 millilitre sample." ;
                                           rdfs:label "count50Plus" .


:OilAnalysisParticleAnalogKind.count5Plus uml:id "_812E35B4-2FF3-46e1-8485-D24B4FD04F58" ;
                                          rdfs:comment "Count of particles 5 microns and larger in a 1 millilitre sample." ;
                                          rdfs:label "count5Plus" .


:OilAnalysisParticleAnalogKind.count6Plus uml:id "_2CA82AC8-FAB8-45d8-A32B-2955157B12FA" ;
                                          rdfs:comment "Count of particles 6 microns and larger in a 1 millilitre sample." ;
                                          rdfs:label "count6Plus" .


:OilAnalysisParticleAnalogKind.count70Plus uml:id "_69FF824C-AAB7-43a9-ACC9-A165F2F6EBD5" ;
                                           rdfs:comment "Count of particles 70 microns and larger in a 1 millilitre sample." ;
                                           rdfs:label "count70Plus" .


:OilAnalysisParticleAnalogKind.fibrePercent uml:id "_A9B745E7-1D84-4507-AB0E-A5FDBF6FF20B" ;
                                            rdfs:comment "Percent of particles which are fibres." ;
                                            rdfs:label "fibrePercent" .


:OilAnalysisParticleAnalogKind.metalPercent uml:id "_E0F10A4B-6DD3-49eb-B1E8-D32A834D1F07" ;
                                            rdfs:comment "Percent of particles which are metal." ;
                                            rdfs:label "metalPercent" .


:OilAnalysisParticleAnalogKind.otherPercent uml:id "_C8E19E3E-DE56-428e-BE46-7E7B4545E3A5" ;
                                            rdfs:comment "Percent of particles which are 'other'." ;
                                            rdfs:label "otherPercent" .


:OilAnalysisParticleDiscreteKind.opacity uml:id "_5177807E-E432-4f65-B5EC-F9DA8566A1A7" ;
                                         rdfs:comment """Opacity of oil.
Possible values: any integer.""" ;
                                         rdfs:label "opacity" .


:OilPreservationKind.conservator uml:id "_44468FDF-C4CB-4009-8705-0BD6913907E4" ;
                                 rdfs:label "conservator" .


:OilPreservationKind.freeBreathing uml:id "_91047A63-123F-4e79-B978-915993393481" ;
                                   rdfs:label "freeBreathing" .


:OilPreservationKind.nitrogenBlanket uml:id "_7ADCF0D8-FAB0-45fe-9832-763BA8D473E5" ;
                                     rdfs:label "nitrogenBlanket" .


:OilPreservationKind.other uml:id "_5D27AC3C-794B-4fbd-8761-0C42E4208C60" ;
                           rdfs:label "other" .


:OilSampleLocation.oilDrainageDevice uml:id "_BA582242-B982-4797-96E4-F962ABBA20FB" ;
                                     rdfs:comment "Sample from oil drainage device." ;
                                     rdfs:label "oilDrainageDevice" .


:OilSampleLocation.oilSampleValve uml:id "_78E02C57-D480-46c7-97FB-4BCE6E297962" ;
                                  rdfs:comment "Sample from oil sample valve." ;
                                  rdfs:label "oilSampleValve" .


:OilSampleLocation.other uml:id "_DFED0D11-8F3E-4be3-BAFD-74453B34901D" ;
                         rdfs:comment "Sample from other location." ;
                         rdfs:label "other" .


:OilTemperatureSource.infraredGun uml:id "_E6EFCA57-C82C-4ee9-B977-F0E48B707F0C" ;
                                  rdfs:comment "Oil temperature from infrared gun." ;
                                  rdfs:label "infraredGun" .


:OilTemperatureSource.other uml:id "_BE3FF80D-2962-49de-BE7F-90F70EE1BF69" ;
                            rdfs:comment "Oil temperature from other souce." ;
                            rdfs:label "other" .


:OilTemperatureSource.topOilTemperatureGauge uml:id "_385BE143-64A3-4a91-AA3D-4E1B7D07EC2B" ;
                                             rdfs:comment "Oil temperature from top oil temperature gauge." ;
                                             rdfs:label "topOilTemperatureGauge" .


:OnOff.OFF uml:id "_8317AAAF-E696-4f4d-AA5F-2874B62B8BA8" ;
           rdfs:label "OFF" .


:OnOff.ON uml:id "_D5222E54-0451-499a-A8D8-10D39D5CBED6" ;
          rdfs:label "ON" .


:OperatingMechanismKind.capacitorTrip uml:id "_91566335-73B3-4962-AD98-8ED4D1E96F4A" ;
                                      rdfs:comment "Capacitor trip mechanism." ;
                                      rdfs:label "capacitorTrip" .


:OperatingMechanismKind.hydraulic uml:id "_8C776FD3-1DD0-4e28-A633-E5DEA4C770E7" ;
                                  rdfs:comment "Hydraulic mechanism." ;
                                  rdfs:label "hydraulic" .


:OperatingMechanismKind.pneudraulic uml:id "_A59CDB4F-9E17-40a7-B48E-45FF323AA5FA" ;
                                    rdfs:comment "Pneudraulic mechanism." ;
                                    rdfs:label "pneudraulic" .


:OperatingMechanismKind.pneumatic uml:id "_5488E724-D43E-4c80-BF95-696A82A3FB4A" ;
                                  rdfs:comment "Pneumatic mechanism." ;
                                  rdfs:label "pneumatic" .


:OperatingMechanismKind.solenoid uml:id "_D5D6DEBE-7D83-4db2-8F14-A0D915166610" ;
                                 rdfs:comment "Solenoid mechanism." ;
                                 rdfs:label "solenoid" .


:OperatingMechanismKind.spring uml:id "_29994947-AF3C-4653-B4C7-37F9643D34BD" ;
                               rdfs:comment "Spring mechanism." ;
                               rdfs:label "spring" .


:OperatingMechanismKind.springHandCrank uml:id "_A4AF5A3E-D8F2-48f1-A1B8-73CB6965AEC7" ;
                                        rdfs:comment "Spring hand-crank mechanism." ;
                                        rdfs:label "springHandCrank" .


:OperatingMechanismKind.springHydraulic uml:id "_BCB70AEF-9FAA-4c5c-B3C5-C52719A6B513" ;
                                        rdfs:comment "Spring hydraulic mechanism." ;
                                        rdfs:label "springHydraulic" .


:OperatingMechanismKind.springMotor uml:id "_C36B74D4-2D36-4984-9BE2-96A617F3E6F2" ;
                                    rdfs:comment "Spring motor mechanism." ;
                                    rdfs:label "springMotor" .


:OperationalLimitDirectionKind.absoluteValue uml:id "_C37E3F49-FDC5-4924-A75A-7A4B7D05C856" ;
                                             rdfs:comment "An absoluteValue limit means that a monitored absolute value above the limit value is a violation." ;
                                             rdfs:label "absoluteValue" .


:OperationalLimitDirectionKind.high uml:id "_DEB6E936-5033-4498-989C-D433460E5D3E" ;
                                    rdfs:comment "High means that a monitored value above the limit value is a violation.   If applied to a terminal flow, the positive direction is into the terminal." ;
                                    rdfs:label "high" .


:OperationalLimitDirectionKind.low uml:id "_1A441FD0-B158-4b91-A4F9-2F83E7EBA2B2" ;
                                   rdfs:comment "Low means a monitored value below the limit is a violation.  If applied to a terminal flow, the positive direction is into the terminal." ;
                                   rdfs:label "low" .


:OrganisationCode.BILL_TO uml:id "_BEFE95F4-26E6-4c55-89C3-D90DF7CC8316" ;
                          rdfs:label "BILL_TO" .


:OrganisationCode.PAY_TO uml:id "_20AC10BF-F46A-4771-83B1-C88AD43422BC" ;
                         rdfs:label "PAY_TO" .


:OrganisationCode.PROVIDED_BY uml:id "_0E9D0A8F-F5F8-4d66-AB08-585D7B772597" ;
                              rdfs:label "PROVIDED_BY" .


:OrganisationCode.SOLD_TO uml:id "_9E87CA03-C6A0-49a0-8773-8C277B35C9CE" ;
                          rdfs:label "SOLD_TO" .


:OrganisationType.CUSTOMER uml:id "_755C4158-0E07-4c6e-AD71-07EF3CF2A026" ;
                           rdfs:label "CUSTOMER" .


:OrganisationType.RTO uml:id "_67BA88D5-17C2-4a50-A771-D198F59BB75F" ;
                      rdfs:label "RTO" .


:OrientationKind.negative uml:id "_6D82C240-A79A-4526-8D68-5EB815024164" ;
                          rdfs:comment "For 2D diagrams, a negative orientation gives the left-hand orientation (favoured by computer graphics displays) with X values increasing from left to right and Y values increasing from top to bottom.   This is also known as a left hand orientation." ;
                          rdfs:label "negative" .


:OrientationKind.positive uml:id "_860B40F5-247F-42ae-9737-7FE0EC735E60" ;
                          rdfs:comment "For 2D diagrams, a positive orientation will result in X values increasing from left to right and Y values increasing from bottom to top.  This is also known as a right hand orientation." ;
                          rdfs:label "positive" .


:OutageCauseKind.animal uml:id "_6A838872-9EF8-4d63-9C8E-1843DE84D1CC" ;
                        rdfs:comment "This outage was caused by an animal is was unplanned.  As such it is treated as a forced outage and is probably classified as \"trouble\" with a Trouble Ticket as well as a work/service order.  The primary difference between this and an unplanned outage is the reason for the outage.  If an animal caused this and perished as a result, the utility may have other actions that are required to be taken by the EPA or other groups with whom the utility has an agreement." ;
                        rdfs:label "animal" .


:OutageCauseKind.lightingStrike uml:id "_815AEFC6-65C1-4542-B332-A7624897CE80" ;
                                rdfs:comment "Outage is caused by a lighting strike" ;
                                rdfs:label "lightingStrike" .


:OutageCauseKind.lineDown uml:id "_C5493BB6-87C3-4a7b-A960-1193D6B9D548" ;
                          rdfs:comment "The outage is caused by a line down" ;
                          rdfs:label "lineDown" .


:OutageCauseKind.poleDown uml:id "_8A6D9D6D-1EA9-4ba2-8DFA-33AA85571B0B" ;
                          rdfs:comment "The outage is caused by a pole down" ;
                          rdfs:label "poleDown" .


:OutageCauseKind.treeDown uml:id "_1F2D83D5-38A8-4925-BE4C-D2D741C089E3" ;
                          rdfs:comment "The outage is caused by a tree down" ;
                          rdfs:label "treeDown" .


:OutageStatusKind.closed uml:id "_7AD31E5D-F74F-4d20-883B-8F37F3F9674A" ;
                         rdfs:comment "The outage has been fully restored, the crews have been released and the outage is shown as closed" ;
                         rdfs:label "closed" .


:OutageStatusKind.confirmed uml:id "_C25C7C45-AC9E-492c-AC84-68A1C56F7730" ;
                            rdfs:comment "the outage has been verified" ;
                            rdfs:label "confirmed" .


:OutageStatusKind.partiallyRestored uml:id "_DABA1CC0-3186-47a9-A1CB-3567E15739F3" ;
                                    rdfs:comment "Some of the usage points affected by the outage have been restored but other usage points are still out of power." ;
                                    rdfs:label "partiallyRestored" .


:OutageStatusKind.predicted uml:id "_4BB374BE-D703-4f05-8B67-209BC2BD3CA6" ;
                            rdfs:comment "the outage may not be real since it has not been verified - it is only thought to be an outage." ;
                            rdfs:label "predicted" .


:OutageStatusKind.restored uml:id "_CF0793F6-AC4F-4c31-BF02-A8CB5561A60C" ;
                           rdfs:comment "All usage points associated with the outage have been restored" ;
                           rdfs:label "restored" .


:PSREventKind.inService uml:id "_0BED646D-9B8E-414d-A839-985B3FCE06B8" ;
                        rdfs:comment "Power system resource state change to in service." ;
                        rdfs:label "inService" .


:PSREventKind.other uml:id "_AF8D6D63-7555-4599-9373-48C99361041B" ;
                    rdfs:comment "Other power system resource state change." ;
                    rdfs:label "other" .


:PSREventKind.outOfService uml:id "_35587599-4E23-472e-9884-059331D3413E" ;
                           rdfs:comment "Power system resource state change to out of service." ;
                           rdfs:label "outOfService" .


:PSREventKind.pendingAdd uml:id "_D08E54ED-D1FB-4fe7-AB1D-6D39615186AB" ;
                         rdfs:comment "Power system resource state change to pending add." ;
                         rdfs:label "pendingAdd" .


:PSREventKind.pendingRemove uml:id "_13C5B546-C97A-4168-A19E-8FEA5167FED3" ;
                            rdfs:comment "Power system resource state change to pending remove." ;
                            rdfs:label "pendingRemove" .


:PSREventKind.pendingReplace uml:id "_5BC2039C-C41D-48f8-BD82-D823A3CE3F81" ;
                             rdfs:comment "Power system resource state change to pending replace." ;
                             rdfs:label "pendingReplace" .


:PSREventKind.unknown uml:id "_4B4EE721-021C-4d27-88CE-0AE70B0A4CE4" ;
                      rdfs:comment "Unknown power system resource state change." ;
                      rdfs:label "unknown" .


:ParticipationCategoryMPM.L uml:id "_C57DA898-83BE-4b5f-B48A-CB695FF4F22F" ;
                            rdfs:label "L" .


:ParticipationCategoryMPM.N uml:id "_5BFC27F8-7F56-448a-A345-81DA5F59F3BB" ;
                            rdfs:label "N" .


:ParticipationCategoryMPM.S uml:id "_80813ED0-7F84-45cc-8A85-634F1CCDE8FD" ;
                            rdfs:label "S" .


:ParticipationCategoryMPM.Y uml:id "_7C2E5A54-A21C-436d-9A77-C94E07477BBC" ;
                            rdfs:label "Y" .


:PassIndicatorType.DA uml:id "_C27F9DF9-1FEC-45f1-A6B2-AC21F81152BE" ;
                      rdfs:comment "Day Ahead" ;
                      rdfs:label "DA" .


:PassIndicatorType.HA-SCUC uml:id "_98899724-42B5-443e-8B59-9DAB3B80F145" ;
                           rdfs:comment "Hour Ahead Security Constrained Unit Commitment" ;
                           rdfs:label "HA-SCUC" .


:PassIndicatorType.MPM-1 uml:id "_3571C009-9F21-4bd9-A211-7C6DDC2AB36D" ;
                         rdfs:comment "Market Power Mitigation Pass 1" ;
                         rdfs:label "MPM-1" .


:PassIndicatorType.MPM-2 uml:id "_D96663A7-147F-45a3-AD20-D54D52229203" ;
                         rdfs:comment "Market Power Mitigation Pass 2" ;
                         rdfs:label "MPM-2" .


:PassIndicatorType.MPM-3 uml:id "_A20138CA-2268-4121-B49F-28B02D440A94" ;
                         rdfs:comment "Market Power Mitigation Pass 3" ;
                         rdfs:label "MPM-3" .


:PassIndicatorType.MPM-4 uml:id "_DBDB0279-3DB6-4e8c-BA93-BB35737A24FB" ;
                         rdfs:comment "Market Power Mitigation Pass 4" ;
                         rdfs:label "MPM-4" .


:PassIndicatorType.RTED uml:id "_0E0B0D6B-93C7-4c97-A4DC-B0BF5FAB081E" ;
                        rdfs:comment "Real Time Economic Dispatch" ;
                        rdfs:label "RTED" .


:PassIndicatorType.RTPD uml:id "_70D24C43-D27B-4366-99D4-773904682700" ;
                        rdfs:comment "Real Time Pre Dispatch" ;
                        rdfs:label "RTPD" .


:PassIndicatorType.RUC uml:id "_282BCB80-3D13-47e1-94F1-49A3FEDE13C6" ;
                       rdfs:comment "Residual Unit Commitment" ;
                       rdfs:label "RUC" .


:PetersenCoilModeKind.automaticPositioning uml:id "_0420A9CF-DFDA-4acc-B5D2-C297FAD7A7EE" ;
                                           rdfs:comment "Automatic positioning." ;
                                           rdfs:label "automaticPositioning" .


:PetersenCoilModeKind.fixed uml:id "_7C2450DE-D888-4741-A3B2-6598BE34F25E" ;
                            rdfs:comment "Fixed position." ;
                            rdfs:label "fixed" .


:PetersenCoilModeKind.manual uml:id "_279C3FB6-957B-4817-9ACE-1CCBE44C3D83" ;
                             rdfs:comment "Manual positioning." ;
                             rdfs:label "manual" .


:PhaseConnectedFaultKind.lineOpen uml:id "_9D8DAA9D-0BC6-4f21-9E79-942AE0908070" ;
                                  rdfs:comment "The fault is when the conductor path is broken between two terminals. Additional coexisting faults may be required if the broken conductor also causes connections to grounds or other lines or phases." ;
                                  rdfs:label "lineOpen" .


:PhaseConnectedFaultKind.lineToGround uml:id "_D1E5958A-98F4-49f3-9C1E-AA42781D5B9E" ;
                                      rdfs:comment "The fault connects the indicated phases to ground. The line to line fault impedance is not used and assumed infinite. The full ground impedance is connected between each phase specified in the fault and ground, but not between the phases." ;
                                      rdfs:label "lineToGround" .


:PhaseConnectedFaultKind.lineToLine uml:id "_9A278CD5-0F0C-4b56-930C-34CE03649D27" ;
                                    rdfs:comment "The fault connects the specified phases together without a connection to ground. The ground impedance of this fault is ignored. The line to line impedance is connected between each of the phases specified in the fault. For example three times for a three phase fault, one time for a two phase fault.  A single phase fault should not be specified." ;
                                    rdfs:label "lineToLine" .


:PhaseConnectedFaultKind.lineToLineToGround uml:id "_98041BF3-DBA9-4d80-AE9A-D52C72ACDAB0" ;
                                            rdfs:comment "The fault connects the indicated phases to ground and to each other. The line to line impedance is connected between each of the phases specified in the fault in a full mesh. For example three times for a three phase fault, one time for a two phase fault. A single phase fault should not be specified. The full ground impedance is connected between each phase specified in the fault and ground." ;
                                            rdfs:label "lineToLineToGround" .


:PhaseShuntConnectionKind.D uml:hasInitialValue "1" ;
                            uml:id "_BB7AE92B-4282-499f-A237-2EFB5550CF18" ;
                            rdfs:comment "Delta connection." ;
                            rdfs:label "D" .


:PhaseShuntConnectionKind.G uml:hasInitialValue "5" ;
                            uml:id "_9B904A86-646C-4eb0-AC5A-C855B6963581" ;
                            rdfs:comment "Ground connection; use when explicit connection to ground needs to be expressed in combination with the phase code, such as for electrical wire/cable or for meters." ;
                            rdfs:label "G" .


:PhaseShuntConnectionKind.I uml:hasInitialValue "4" ;
                            uml:id "_B1808795-7E5F-440e-A7D2-68D61720928F" ;
                            rdfs:comment "Independent winding, for single-phase connections." ;
                            rdfs:label "I" .


:PhaseShuntConnectionKind.Y uml:hasInitialValue "2" ;
                            uml:id "_78F5E336-DE68-4bcd-8E5D-D60B2D772116" ;
                            rdfs:comment "Wye connection." ;
                            rdfs:label "Y" .


:PhaseShuntConnectionKind.Yn uml:hasInitialValue "3" ;
                             uml:id "_4204851F-78EC-4f27-AEF3-587D5A6D43ED" ;
                             rdfs:comment "Wye, with neutral brought out for grounding." ;
                             rdfs:label "Yn" .


:PinBranchGroupKind.activePower uml:id "_4B8ABF82-7789-4db0-A0E0-746D3BFC8D76" ;
                                rdfs:comment "Active power in the branch group." ;
                                rdfs:label "activePower" .


:PinBranchGroupKind.reactivePower uml:id "_E85C2AFB-94D2-4a61-AF0D-D26EA7E3744D" ;
                                  rdfs:comment "Reactive power in the branch group." ;
                                  rdfs:label "reactivePower" .


:PinEquipmentKind.activePowerLimit uml:id "_1FA22B75-D95A-40fd-B873-4B2B665556EA" ;
                                   rdfs:comment "Compare load flow result against the active limit for active power for the given equipment." ;
                                   rdfs:label "activePowerLimit" .


:PinEquipmentKind.apparentPowerLimit uml:id "_A8A9669B-FC34-4585-854F-FE0E7253734B" ;
                                     rdfs:comment "Compare load flow result against the active limit for apparent power for the given equipment." ;
                                     rdfs:label "apparentPowerLimit" .


:PinEquipmentKind.connected uml:id "_2CE1D76F-674E-440f-933C-A23AC1BB0E7D" ;
                            rdfs:comment "Check if all terminal on the equipment is connected." ;
                            rdfs:label "connected" .


:PinEquipmentKind.currentLimit uml:id "_BA7E9107-A354-4481-A0CC-9C3A5BCA2F7D" ;
                               rdfs:comment "Compare load flow result against the active current limit for the equipment." ;
                               rdfs:label "currentLimit" .


:PinEquipmentKind.inService uml:id "_BB7FEF75-898C-492c-A2C5-2025359F85D6" ;
                            rdfs:comment "Check if equipment is in service, True if in service otherwise false." ;
                            rdfs:label "inService" .


:PinEquipmentKind.ratedCurrent uml:id "_901676EC-7A3C-4153-B6FA-DBF80512F875" ;
                               rdfs:comment "Compare load flow result against rated current on the equipment (switch)." ;
                               rdfs:label "ratedCurrent" .


:PinEquipmentKind.voltageLimit uml:id "_D332FA38-D0BE-4b18-86D1-36A58291C5E9" ;
                               rdfs:comment "Compare load flow result against the active voltage limit for the equipment." ;
                               rdfs:label "voltageLimit" .


:PinTerminalKind.activePower uml:id "_5C716C7B-B930-4b51-A02C-6731F9C7AEED" ;
                             rdfs:comment "Active Power on the Terminal." ;
                             rdfs:label "activePower" .


:PinTerminalKind.apparentPower uml:id "_ECC1F568-D75F-4e3d-B418-81A21D8D7E80" ;
                               rdfs:comment "Apparent Power on the Terminal." ;
                               rdfs:label "apparentPower" .


:PinTerminalKind.reactivePower uml:id "_13A962FA-D94D-4f28-B9A4-17CF1EAFECF5" ;
                               rdfs:comment "Reactive Power on the Terminal." ;
                               rdfs:label "reactivePower" .


:PinTerminalKind.voltage uml:id "_55790E55-C496-4a60-AB26-149F6686AEB0" ;
                         rdfs:comment "Voltage on the Terminal." ;
                         rdfs:label "voltage" .


:PoleBaseKind.asphalt uml:id "_31D20CB5-C814-4965-BD5C-B79D9AF627A2" ;
                      rdfs:label "asphalt" .


:PoleBaseKind.cement uml:id "_7A4F578A-2AD1-4d5e-866D-7BDCCF0D4F31" ;
                     rdfs:label "cement" .


:PoleBaseKind.dirt uml:id "_0841FF5D-16CA-4a2a-9D9E-6799C33CC2D6" ;
                   rdfs:label "dirt" .


:PoleBaseKind.other uml:id "_F41D75A1-4E9D-48e6-B846-5A6D35EF593C" ;
                    rdfs:label "other" .


:PoleBaseKind.unknown uml:id "_E20B6327-A5D2-4afe-BAE9-289D70558D8C" ;
                      rdfs:label "unknown" .


:PolePreservativeKind.cellon uml:id "_A2EA2FA2-1485-490b-BDA3-3CD1D2438F90" ;
                             rdfs:label "cellon" .


:PolePreservativeKind.chemonite uml:id "_8CB4DBB9-8375-42b6-9DA4-C29F31E57CDE" ;
                                rdfs:label "chemonite" .


:PolePreservativeKind.creosote uml:id "_C1514E50-98C7-4511-A391-D19681D82FA8" ;
                               rdfs:label "creosote" .


:PolePreservativeKind.naphthena uml:id "_717910B6-037F-42c7-8A05-A9A482A0EB7E" ;
                                rdfs:label "naphthena" .


:PolePreservativeKind.other uml:id "_3546A7B9-AAEB-483f-A59C-2D9373C3E143" ;
                            rdfs:label "other" .


:PolePreservativeKind.penta uml:id "_71380ED0-F52C-4aab-A2DC-6CEC05CC4686" ;
                            rdfs:label "penta" .


:PolePreservativeKind.unknown uml:id "_2FC4A079-5104-4aec-A31E-3863FD0E9608" ;
                              rdfs:label "unknown" .


:PoleTreatmentKind.butt uml:id "_86CAB461-E417-48fb-AE02-D44961FD6038" ;
                        rdfs:label "butt" .


:PoleTreatmentKind.full uml:id "_7D17719A-C580-48b9-8EF1-A3939226DC76" ;
                        rdfs:label "full" .


:PoleTreatmentKind.grayStain uml:id "_D46F9F7F-1C7C-46e0-A008-F02E98D0D64C" ;
                             rdfs:label "grayStain" .


:PoleTreatmentKind.greenStain uml:id "_B36B51BD-55CF-4d35-A760-12D9A3999EAA" ;
                              rdfs:label "greenStain" .


:PoleTreatmentKind.natural uml:id "_4B94C982-FB02-4568-9CC7-6CD1E09EE8AB" ;
                           rdfs:label "natural" .


:PoleTreatmentKind.other uml:id "_907F4C1C-0D88-45c7-8BB9-6B308200841C" ;
                         rdfs:label "other" .


:PoleTreatmentKind.penta uml:id "_581D336E-6187-4f39-9F55-1AC25F03DB23" ;
                         rdfs:label "penta" .


:PoleTreatmentKind.unknown uml:id "_E58EFF04-5D7D-4537-9CF1-B13084F169F8" ;
                           rdfs:label "unknown" .


:PotentialTransformerKind.capacitiveCoupling uml:id "_79BD0A18-3776-4e24-A1E3-892D9282521C" ;
                                             rdfs:comment "The potential transformer is using capacitive coupling to create secondary voltage." ;
                                             rdfs:label "capacitiveCoupling" .


:PotentialTransformerKind.inductive uml:id "_12D1E9BA-EEE1-4e7b-B541-B68DBAD67316" ;
                                    rdfs:comment "The potential transformer is using induction coils to create secondary voltage." ;
                                    rdfs:label "inductive" .


:PriceSetFlag.N uml:id "_B27CD0FE-55CB-4c21-B881-37E0D5A10810" ;
                rdfs:label "N" .


:PriceSetFlag.S uml:id "_9BA66A24-5312-4961-A992-47DA30B9546B" ;
                rdfs:label "S" .


:PriceSetFlag.Y uml:id "_E2E6B20E-E24E-4bfd-9B1C-B10B82B2E239" ;
                rdfs:label "Y" .


:PriceTypeKind.capacity uml:id "_494B44FF-E452-48a2-948D-D9971DFD4ADE" ;
                        rdfs:label "capacity" .


:PriceTypeKind.congestion uml:id "_3FAB4EA1-8E89-4960-9416-C7E17F38C649" ;
                          rdfs:label "congestion" .


:PriceTypeKind.delivery uml:id "_4A77CB5C-DE76-4320-B78E-C919D428EA5A" ;
                        rdfs:label "delivery" .


:PriceTypeKind.loss uml:id "_0DF6DFF6-C44D-449b-A99D-CCEEC663C702" ;
                    rdfs:label "loss" .


:PriceTypeKind.mileage uml:id "_F22056B0-071C-44c2-BFB9-5D7CB11F28C4" ;
                       rdfs:label "mileage" .


:PriceTypeKind.system uml:id "_EAFCBB60-124D-4a10-8948-6E052DFFC96A" ;
                      rdfs:label "system" .


:PriceTypeKind.total uml:id "_007473BE-0665-4619-9D1E-59F1781D0F7B" ;
                     rdfs:label "total" .


:ProcedureKind.diagnosis uml:id "_B4EEEAA5-C3A6-4dc2-ADBA-61F3418FC54E" ;
                         rdfs:comment "Diagnosis procedure." ;
                         rdfs:label "diagnosis" .


:ProcedureKind.inspection uml:id "_34182161-5EB5-4641-B07B-6A17ED569570" ;
                          rdfs:comment "Inspection procedure." ;
                          rdfs:label "inspection" .


:ProcedureKind.maintenance uml:id "_3E821F9E-89FE-43f7-8889-489B582E74F3" ;
                           rdfs:comment "Maintenance procedure." ;
                           rdfs:label "maintenance" .


:ProcedureKind.other uml:id "_42AC1AFC-7EF1-4947-B2DA-C71EF2AF72D9" ;
                     rdfs:comment "Other procedure." ;
                     rdfs:label "other" .


:ProcedureKind.test uml:id "_21C67CBB-313E-45d5-9569-9B61A2BD6E15" ;
                    rdfs:comment "Test procedure." ;
                    rdfs:label "test" .


:ProjectStatusKind.cancelled uml:id "_8DB13B5B-7E69-4ee5-82E8-C9C0E58EA5E1" ;
                             rdfs:label "cancelled" .


:ProjectStatusKind.closed uml:id "_FF011FD6-C4CE-4da8-8FA0-CA62F984D683" ;
                          rdfs:label "closed" .


:ProjectStatusKind.draft uml:id "_989B9186-7078-438f-A2E0-5B9897CDDEA8" ;
                         rdfs:label "draft" .


:ProjectStatusKind.frozen uml:id "_E405B658-EB96-41cc-8F12-AA68AF19E188" ;
                          rdfs:label "frozen" .


:ProtectiveActionAdjustmentKind.byPercentage uml:id "_8C25683F-4822-4d54-9F44-54DDD0FB6B74" ;
                                             rdfs:comment "The adjustment is in percentage of the active value." ;
                                             rdfs:label "byPercentage" .


:ProtectiveActionAdjustmentKind.byValue uml:id "_533E9ED9-C4E1-4c5b-99F9-93DC74554FA2" ;
                                        rdfs:comment "The adjustment is in given by a value that defined the changes that will be done to the active value." ;
                                        rdfs:label "byValue" .


:ProtectiveActionAdjustmentKind.measurement uml:id "_F148ECFB-3B36-41fb-9F48-77E78108FC10" ;
                                            rdfs:comment "The equipment will operating on a value given by a measurement." ;
                                            rdfs:label "measurement" .


:ProtectiveActionAdjustmentKind.setValue uml:id "_D6C00622-4AA1-4625-86A6-70D758C6D52E" ;
                                         rdfs:comment "The equipment will operate on the new value." ;
                                         rdfs:label "setValue" .


:PurposeFlagType.M uml:id "_DECD0EB4-7450-4c82-8C01-993B8B97A80B" ;
                   rdfs:label "M" .


:PurposeFlagType.R uml:id "_19104108-1220-444b-A907-6C7C28C25D14" ;
                   rdfs:label "R" .


:RampCurveType._0 uml:id "_8EF01E39-F3B1-43b5-AF63-0CB7585DFFCE" ;
                  rdfs:comment "Fixed ramp rate independent of rate function unit MW output" ;
                  rdfs:label "0" .


:RampCurveType._1 uml:id "_92B022BA-8AF4-44e8-A7C0-27DE6621ECBE" ;
                  rdfs:comment "Static ramp rates as a function of unit MW output only" ;
                  rdfs:label "1" .


:RampCurveType._2 uml:id "_392FD8BE-A293-447a-A118-67F032BC1A4D" ;
                  rdfs:comment "Dynamic ramp rates as a function of unit MW output and ramping time" ;
                  rdfs:label "2" .


:RampRateCondition.BEST uml:id "_CB755C64-A2A6-4af9-9497-E7282F8C02A3" ;
                        rdfs:label "BEST" .


:RampRateCondition.NA uml:id "_FCEC1981-B42E-4801-B496-A2E2DA1CB02F" ;
                      rdfs:comment "not applicable" ;
                      rdfs:label "NA" .


:RampRateCondition.NORMAL uml:id "_0B90C498-47C9-4dcc-8A61-05FF615F2AA2" ;
                          rdfs:label "NORMAL" .


:RampRateCondition.WORST uml:id "_FB0F6D6C-FFC0-4192-88DF-F3240C6EC478" ;
                         rdfs:label "WORST" .


:RampRateType.INTERTIE uml:id "_7A6702A8-B8D7-43f8-8A43-A2798E28A656" ;
                       rdfs:comment "Intertie ramp rate." ;
                       rdfs:label "INTERTIE" .


:RampRateType.LD_DROP uml:id "_11B5352F-6DC7-4f5e-BB35-4BB034EFE48E" ;
                      rdfs:comment "Load drop ramp rate." ;
                      rdfs:label "LD_DROP" .


:RampRateType.LD_PICKUP uml:id "_00BC8032-8654-45a9-9D49-445086D1CF28" ;
                        rdfs:comment "Load pick up rate." ;
                        rdfs:label "LD_PICKUP" .


:RampRateType.OP uml:id "_2C3F2698-584E-42c3-AEC2-C8625FDB50D3" ;
                 rdfs:comment "Operational ramp rate." ;
                 rdfs:label "OP" .


:RampRateType.OP_RES uml:id "_7585C660-FE66-4c47-A347-28315A490BA6" ;
                     rdfs:comment "Operating reserve ramp rate." ;
                     rdfs:label "OP_RES" .


:RampRateType.REG uml:id "_69842421-78FD-43f9-9BE0-642E9A93AE35" ;
                  rdfs:comment "Regulating ramp rate." ;
                  rdfs:label "REG" .


:RandomisationKind.default uml:id "_28F2A4D6-D3F1-4505-8C4B-27B4285F513D" ;
                           rdfs:comment "Randomisation of start and/or end times involving the operation of one or more devices is controlled by default settings for the device(s)." ;
                           rdfs:label "default" .


:RandomisationKind.end uml:id "_81A71A6C-FD52-42dc-801F-6994A3CDCF84" ;
                       rdfs:comment "End time of an event or control action affecting one or more devices is randomised to prevent simultaneous operation." ;
                       rdfs:label "end" .


:RandomisationKind.none uml:id "_8AA87276-306D-44d3-B217-7C38E51BE204" ;
                        rdfs:comment "Neither the start time nor the end time of an event or control action affecting one or more devices is randomised." ;
                        rdfs:label "none" .


:RandomisationKind.start uml:id "_5F840059-4252-4ed6-983C-5C5F9C52EC2A" ;
                         rdfs:comment "Start time of an event or control action affecting one or more multiple devices is randomised." ;
                         rdfs:label "start" .


:RandomisationKind.startAndEnd uml:id "_ECF539C1-7136-46fa-9049-DD80BB3210DF" ;
                               rdfs:comment "Both the start time and the end time of an event or control action affecting one or more devices are randomised to prevent simultaneous operation." ;
                               rdfs:label "startAndEnd" .


:ReadingReasonKind.billing uml:id "_09401BE6-FE52-4ea5-A24A-F41856E49CEB" ;
                           rdfs:comment "Reading(s) taken or to be taken in response to a billing-related inquiry by a customer or other party. A variant of 'inquiry'." ;
                           rdfs:label "billing" .


:ReadingReasonKind.demandReset uml:id "_BFE93BAB-5090-44d1-B007-60F586394D11" ;
                               rdfs:comment "Reading(s) taken or to be taken in conjunction with the resetting of one or more demand registers in a meter." ;
                               rdfs:label "demandReset" .


:ReadingReasonKind.inquiry uml:id "_058CBE99-8C7D-4845-9198-88353070D22D" ;
                           rdfs:comment "Reading(s) taken or to be taken in response to an inquiry by a customer or other party." ;
                           rdfs:label "inquiry" .


:ReadingReasonKind.installation uml:id "_9CA1F132-A17F-4742-AD9E-C6EE7C240E3B" ;
                                rdfs:comment "Reading(s) taken or to be taken in conjunction with installation of a meter." ;
                                rdfs:label "installation" .


:ReadingReasonKind.loadManagement uml:id "_F92A3C79-CC78-482a-B0ED-AB79101CF541" ;
                                  rdfs:comment "Reading(s) taken or to be taken to support management of loads on distribution networks or devices." ;
                                  rdfs:label "loadManagement" .


:ReadingReasonKind.loadResearch uml:id "_DBEF3365-7D15-4c37-8A9E-D9F2633AD687" ;
                                rdfs:comment "Reading(s) taken or to be taken to support research and analysis of loads on distribution networks or devices." ;
                                rdfs:label "loadResearch" .


:ReadingReasonKind.moveIn uml:id "_74701108-3C53-415b-B0B0-19DD4B9C8422" ;
                          rdfs:comment "Reading(s) taken or to be taken in conjunction with a customer move-in event." ;
                          rdfs:label "moveIn" .


:ReadingReasonKind.moveOut uml:id "_125F5BB7-4B21-4e16-99C0-FA3ED897CBE0" ;
                           rdfs:comment "Reading(s) taken or to be taken in conjunction with a customer move-out event." ;
                           rdfs:label "moveOut" .


:ReadingReasonKind.other uml:id "_81BDD9E5-1086-47a5-B25C-DD9DFAC8BE9D" ;
                         rdfs:comment "Reading(s) taken or to be taken for some other reason or purpose." ;
                         rdfs:label "other" .


:ReadingReasonKind.removal uml:id "_945EA388-BBA1-4678-B0A5-437E15FFC2A5" ;
                           rdfs:comment "Reading(s) taken or to be taken in conjunction with removal of a meter." ;
                           rdfs:label "removal" .


:ReadingReasonKind.serviceConnect uml:id "_8692463B-89B4-4638-9CB9-B5F7D6D4981B" ;
                                  rdfs:comment "Reading(s) taken or to be taken in conjunction with a connection or re-connection of service." ;
                                  rdfs:label "serviceConnect" .


:ReadingReasonKind.serviceDisconnect uml:id "_02139504-E7A5-439f-B3A6-B5DDE7DA6410" ;
                                     rdfs:comment "Reading(s) taken or to be taken in conjunction with a disconnection of service." ;
                                     rdfs:label "serviceDisconnect" .


:RegulatingControlModeKind.activePower uml:id "_23C9B050-DB74-4e78-9212-041967CED311" ;
                                       rdfs:comment "Active power is specified." ;
                                       rdfs:label "activePower" .


:RegulatingControlModeKind.admittance uml:id "_83F69075-D350-4d2c-92B3-50D45A81B4B3" ;
                                      rdfs:comment "Admittance is specified." ;
                                      rdfs:label "admittance" .


:RegulatingControlModeKind.currentFlow uml:id "_D83AA372-A200-4733-B949-55A809B646A2" ;
                                       rdfs:comment "Current flow is specified." ;
                                       rdfs:label "currentFlow" .


:RegulatingControlModeKind.powerFactor uml:id "_A87A2181-9C85-44c6-BC3D-475CF25AD958" ;
                                       rdfs:comment "Power factor is specified." ;
                                       rdfs:label "powerFactor" .


:RegulatingControlModeKind.reactivePower uml:id "_A7F50821-D173-4ff1-96AC-7E854C3ACFF5" ;
                                         rdfs:comment "Reactive power is specified." ;
                                         rdfs:label "reactivePower" .


:RegulatingControlModeKind.temperature uml:id "_93B6C68E-61A6-4d4d-9C47-B3A366DF03DF" ;
                                       rdfs:comment "Control switches on/off based on the local temperature (i.e., a thermostat)." ;
                                       rdfs:label "temperature" .


:RegulatingControlModeKind.timeScheduled uml:id "_558EACEC-1091-4287-88D2-ED67E6966AF0" ;
                                         rdfs:comment "Control switches on/off by time of day. The times may change on the weekend, or in different seasons." ;
                                         rdfs:label "timeScheduled" .


:RegulatingControlModeKind.voltage uml:id "_563504F4-8FFE-4006-8A61-4820A3502302" ;
                                   rdfs:comment "Voltage is specified." ;
                                   rdfs:label "voltage" .


:RegulationBranchKind.breaker uml:id "_6174DE04-2654-4823-985E-52C8D2EC711F" ;
                              rdfs:label "breaker" .


:RegulationBranchKind.fuse uml:id "_26A41C3C-64CF-497e-9F1F-56E08D0018D8" ;
                           rdfs:label "fuse" .


:RegulationBranchKind.line uml:id "_76D76D68-1859-43ca-B6F1-85FE86906F69" ;
                           rdfs:label "line" .


:RegulationBranchKind.other uml:id "_D48DE01F-619B-4541-AFF7-DFD91403EB04" ;
                            rdfs:label "other" .


:RegulationBranchKind.recloser uml:id "_C96483D4-3293-4a3e-AE76-FAB62500C90D" ;
                               rdfs:label "recloser" .


:RegulationBranchKind.sectionner uml:id "_84B959E5-C71C-456f-B243-411880B0CD6E" ;
                                 rdfs:label "sectionner" .


:RegulationBranchKind.switch uml:id "_E8CAF199-AFC0-46af-8484-ADBB623A6090" ;
                             rdfs:label "switch" .


:RegulationBranchKind.transformer uml:id "_C9B2D6B2-42C0-4fd0-9985-26DF85C76D32" ;
                                  rdfs:label "transformer" .


:RelativeDisplacementKind.centreEarth uml:id "_C55CBB28-B6F8-4f04-A7C0-F7C8E59D3AD6" ;
                                      rdfs:label "centreEarth" .


:RelativeDisplacementKind.ground uml:id "_5AE55206-50AE-4d31-B491-D39E79DE756D" ;
                                 rdfs:label "ground" .


:RelativeDisplacementKind.seaLevel uml:id "_70A96BF3-AD87-4725-81C7-18C26A1271DF" ;
                                   rdfs:label "seaLevel" .


:RemedialActionSchemeKind.rAP uml:id "_841B98AA-E6BE-46de-877B-6B203BC9929F" ;
                              rdfs:comment "Remedial Action Plan (RAP)." ;
                              rdfs:label "rAP" .


:RemedialActionSchemeKind.rAS uml:id "_BCC849F2-CE8B-49f5-9347-F1C0D5B99015" ;
                              rdfs:comment "Remedial Action Scheme (RAS)." ;
                              rdfs:label "rAS" .


:RemoteSignalKind.remoteBranchCurrentAmplitude uml:id "_C49FE8D2-9333-4728-B57E-F9DB826A4757" ;
                                               rdfs:comment "Input is branch current amplitude from remote terminal bus." ;
                                               rdfs:label "remoteBranchCurrentAmplitude" .


:RemoteSignalKind.remoteBusFrequency uml:id "_C6DF2D38-4523-42d8-9934-7C24B7F01D5E" ;
                                     rdfs:comment "Input is frequency from remote terminal bus." ;
                                     rdfs:label "remoteBusFrequency" .


:RemoteSignalKind.remoteBusFrequencyDeviation uml:id "_D3F46905-3B27-401f-840B-8AFFBE0EA043" ;
                                              rdfs:comment "Input is frequency deviation from remote terminal bus." ;
                                              rdfs:label "remoteBusFrequencyDeviation" .


:RemoteSignalKind.remoteBusVoltage uml:id "_A9AD26D4-D7B8-4dd1-B5B1-90ECF07AD473" ;
                                   rdfs:comment "Input is voltage from remote terminal bus." ;
                                   rdfs:label "remoteBusVoltage" .


:RemoteSignalKind.remoteBusVoltageAmplitude uml:id "_ADC6015D-1B75-4967-B9C1-7497E00BD416" ;
                                            rdfs:comment "Input is voltage amplitude from remote terminal bus." ;
                                            rdfs:label "remoteBusVoltageAmplitude" .


:RemoteSignalKind.remoteBusVoltageAmplitudeDerivative uml:id "_A3DA99C1-FC9E-4ae3-9DC8-F51A15BF38B8" ;
                                                      rdfs:comment "Input is branch current amplitude derivative from remote terminal bus." ;
                                                      rdfs:label "remoteBusVoltageAmplitudeDerivative" .


:RemoteSignalKind.remoteBusVoltageFrequency uml:id "_2F466BEB-1E65-4226-933C-341820F28D03" ;
                                            rdfs:comment "Input is voltage frequency from remote terminal bus." ;
                                            rdfs:label "remoteBusVoltageFrequency" .


:RemoteSignalKind.remoteBusVoltageFrequencyDeviation uml:id "_97379F4C-D3FC-460d-BCF1-2C189D9E8712" ;
                                                     rdfs:comment "Input is voltage frequency deviation from remote terminal bus." ;
                                                     rdfs:label "remoteBusVoltageFrequencyDeviation" .


:RemoteSignalKind.remotePuBusVoltageDerivative uml:id "_FF2F5379-4C06-43bc-AEB4-79F6A051BA14" ;
                                               rdfs:comment "Input is PU voltage derivative from remote terminal bus." ;
                                               rdfs:label "remotePuBusVoltageDerivative" .


:RemoteUnitType.ControlCenter uml:id "_A70EC582-6B62-4b43-8D83-AAA23EE4A510" ;
                              rdfs:comment "Control centre." ;
                              rdfs:label "ControlCenter" .


:RemoteUnitType.IED uml:id "_2FAC3243-3420-4667-B5DD-DD59D1F07345" ;
                    rdfs:comment "Intelligent electronic device (IED)." ;
                    rdfs:label "IED" .


:RemoteUnitType.RTU uml:id "_C9761387-5835-4c50-8FFC-1F3291CD3B65" ;
                    rdfs:comment "Remote terminal unit." ;
                    rdfs:label "RTU" .


:RemoteUnitType.SubstationControlSystem uml:id "_EF67D5C8-C18E-432e-8C52-DE99E5935742" ;
                                        rdfs:comment "Substation control system." ;
                                        rdfs:label "SubstationControlSystem" .


:ReportingMethodKind.automated uml:id "_0A3570DC-2C56-4bf9-A3BC-1E250E4739FB" ;
                               rdfs:comment "Station automatically reports." ;
                               rdfs:label "automated" .


:ReportingMethodKind.manual uml:id "_9B0A5C6D-EEA6-4fc1-AC5D-3AFB350E5663" ;
                            rdfs:comment "Station must be physically visited to gather observations." ;
                            rdfs:label "manual" .


:ReportingMethodKind.queried uml:id "_55141AE8-E9E7-4119-97B9-6B1679D56DBA" ;
                             rdfs:comment "Station must be queried to obtain observations." ;
                             rdfs:label "queried" .


:RequestorRmrTest.ISO uml:id "_EC33FEBB-FF63-4198-B438-8B152B97249C" ;
                      rdfs:label "ISO" .


:RequestorRmrTest.MP uml:id "_901CEDF4-6D98-4dee-93DC-9AA8EEB6A7C6" ;
                     rdfs:label "MP" .


:ReserveRequirementType.CONT uml:id "_2ED7AAF3-D1CE-4bff-8D5B-E7C3AADB6190" ;
                             rdfs:comment "Contingency" ;
                             rdfs:label "CONT" .


:ReserveRequirementType.OPRSV uml:id "_F065C0E5-814C-4731-865B-A0FF13B929BC" ;
                              rdfs:comment "Operating Reserve" ;
                              rdfs:label "OPRSV" .


:ReserveRequirementType.REG uml:id "_A62AB657-033E-481d-A150-9BA19FF62D37" ;
                            rdfs:comment "Regulation" ;
                            rdfs:label "REG" .


:ResourceAssnType.CSNK uml:id "_E1A26E38-B082-4006-8D27-CB95976B7B07" ;
                       rdfs:label "CSNK" .


:ResourceAssnType.CSRC uml:id "_952CC0F6-4423-4393-BC62-A6FE83D4806A" ;
                       rdfs:label "CSRC" .


:ResourceAssnType.LSE uml:id "_DDBEE3AC-92E3-4de0-8F9C-5FEEA1D174E2" ;
                      rdfs:label "LSE" .


:ResourceAssnType.RMR uml:id "_ABF73CE4-7ED8-4978-B471-23D2836BC035" ;
                      rdfs:label "RMR" .


:ResourceAssnType.SC uml:id "_6C05AB4E-4B4C-4fe4-87DA-B0DABD385AB7" ;
                     rdfs:label "SC" .


:ResourceCapacityType.FO uml:id "_405DF98D-8549-46e1-A20C-92BADEE6A817" ;
                         rdfs:comment "Flexible Offer." ;
                         rdfs:label "FO" .


:ResourceCapacityType.MO uml:id "_B4EC320E-2AAA-4642-A3D9-8CB1C0582C73" ;
                         rdfs:comment "Must Offer." ;
                         rdfs:label "MO" .


:ResourceCapacityType.NR uml:id "_E49F573F-9AA9-4002-9CC8-BF09D749BAB0" ;
                         rdfs:comment "Non spinning reserve." ;
                         rdfs:label "NR" .


:ResourceCapacityType.RA uml:id "_6C55D24A-4C20-4d2c-8AD4-36CBA39C11F2" ;
                         rdfs:comment "Resource Adequacy." ;
                         rdfs:label "RA" .


:ResourceCapacityType.RD uml:id "_BDCF6571-EC59-4b68-97AE-DD2592A6D1D1" ;
                         rdfs:comment "Regulation Down." ;
                         rdfs:label "RD" .


:ResourceCapacityType.RMR uml:id "_3CC88E37-0DF1-4291-8F39-093DD48C5380" ;
                          rdfs:comment "Reliability Must Run." ;
                          rdfs:label "RMR" .


:ResourceCapacityType.RU uml:id "_C431AFAB-FE3D-47ad-9DE7-B3F76A1786FE" ;
                         rdfs:comment "Regulation Up." ;
                         rdfs:label "RU" .


:ResourceCapacityType.SR uml:id "_F2E22B52-9E13-4ebb-88C5-54FD0910D8E9" ;
                         rdfs:comment "Spinning reserve." ;
                         rdfs:label "SR" .


:ResourceCertificationCategory.DAM uml:id "_EEA14BB5-0C46-4928-AFD1-E8602A6B793E" ;
                                   rdfs:label "DAM" .


:ResourceCertificationCategory.GT uml:id "_0E46739C-B680-4320-BB8F-76716350FF7F" ;
                                  rdfs:comment "Generic" ;
                                  rdfs:label "GT" .


:ResourceCertificationCategory.RC uml:id "_D268FB6A-DA08-4637-98D0-94E4DA584FA4" ;
                                  rdfs:label "RC" .


:ResourceCertificationCategory.RTM uml:id "_D5D472A2-E5B9-4271-B106-F46900291BC2" ;
                                   rdfs:label "RTM" .


:ResourceCertificationKind.BLACKSTART uml:id "_7F815B7D-4C21-4238-A603-398434985122" ;
                                      rdfs:comment "Black start" ;
                                      rdfs:label "BLACKSTART" .


:ResourceCertificationKind.Capacity uml:id "_E897D16F-796B-4f45-B1DC-ADA5CFFED6A5" ;
                                    rdfs:label "Capacity" .


:ResourceCertificationKind.DemandSideResponse uml:id "_871DA605-AB36-4479-AFED-E0FED8B0D5C5" ;
                                              rdfs:comment "Demand Side Reponse (DSR)" ;
                                              rdfs:label "DemandSideResponse" .


:ResourceCertificationKind.Energy uml:id "_219290EC-60A8-43a5-9201-BEB72D4C2420" ;
                                  rdfs:label "Energy" .


:ResourceCertificationKind.IntermittentResource uml:id "_8DD28F31-D87A-41dc-87E2-E76A6FE68F75" ;
                                                rdfs:comment "Intermittent resource" ;
                                                rdfs:label "IntermittentResource" .


:ResourceCertificationKind.NonSpinningReserve uml:id "_06E99502-D384-4016-A07A-135341EA9260" ;
                                              rdfs:comment "Non Spinning Reserve (NR, NONSPIN)" ;
                                              rdfs:label "NonSpinningReserve" .


:ResourceCertificationKind.RegulationDown uml:id "_1576E704-0207-40aa-B956-D46B2A199B7D" ;
                                          rdfs:comment "Regulation Down (RD, REGDN)" ;
                                          rdfs:label "RegulationDown" .


:ResourceCertificationKind.RegulationUp uml:id "_C18C59F7-A569-4c59-9A60-801E482592E5" ;
                                        rdfs:comment "Regulation Up (RU, REGUP)" ;
                                        rdfs:label "RegulationUp" .


:ResourceCertificationKind.ReliabilityMustRun uml:id "_601F121C-5038-421c-B526-91789899CC6B" ;
                                              rdfs:comment "Reliability Must Run (RMR)" ;
                                              rdfs:label "ReliabilityMustRun" .


:ResourceCertificationKind.ReliabilityUnitCommitment uml:id "_CB9D7A1D-CFC1-4a41-9947-857071DC166D" ;
                                                     rdfs:comment "Reliability unit commitment (RUC)" ;
                                                     rdfs:label "ReliabilityUnitCommitment" .


:ResourceCertificationKind.SpinningReserve uml:id "_C21007EE-E737-4356-81E2-45FA81F950E4" ;
                                           rdfs:comment "Spinning Reserve (SR, RRSPIN)" ;
                                           rdfs:label "SpinningReserve" .


:ResourceCertificationKind.SynchronousCondenser uml:id "_C1A4372C-0DA5-443f-A744-02233F6B6229" ;
                                                rdfs:comment "Synchronous Condenser (SYNCCOND)" ;
                                                rdfs:label "SynchronousCondenser" .


:ResourceCertificationType.GT uml:id "_81D89297-3A1F-415d-BD86-2BB8E0736E04" ;
                              rdfs:comment "Generic Type" ;
                              rdfs:label "GT" .


:ResourceCertificationType.IR uml:id "_62336D5B-DDE5-4d06-9E32-40499043A297" ;
                              rdfs:comment "Intermittent Resource" ;
                              rdfs:label "IR" .


:ResourceCertificationType.NR uml:id "_789D6DBF-3289-4bdb-918C-2DF3B5578E92" ;
                              rdfs:comment """Generic
Regulation
Spinning
Non-spinning
Intermittent Resource""" ;
                              rdfs:label "NR" .


:ResourceCertificationType.RG uml:id "_4B9FEA56-345F-476a-9C83-25621E2F9F3D" ;
                              rdfs:comment "Regulating" ;
                              rdfs:label "RG" .


:ResourceCertificationType.SR uml:id "_4352FA85-E196-46d7-9D00-3FC838A4BCCF" ;
                              rdfs:comment "Spinning Reserve" ;
                              rdfs:label "SR" .


:ResourceLimitIndicator.LOWER uml:id "_CF547BDC-DA9E-40f2-9ECB-0E6DFAD3D68F" ;
                              rdfs:label "LOWER" .


:ResourceLimitIndicator.UPPER uml:id "_79E8ED6A-DD7D-444e-B1F0-C69BB877E7DB" ;
                              rdfs:label "UPPER" .


:ResourceRegistrationStatus.Active uml:id "_6DD1BFAE-F76F-46f9-BF9B-C9C2B28A359F" ;
                                   rdfs:comment "Resource registration is active" ;
                                   rdfs:label "Active" .


:ResourceRegistrationStatus.Decommissioned uml:id "_4061C09F-B7F7-4f19-B557-BD47637103BA" ;
                                           rdfs:comment "Resource registration status is decommissioned" ;
                                           rdfs:label "Decommissioned" .


:ResourceRegistrationStatus.Mothballed uml:id "_AC33702B-C6EC-49fa-BB2B-04C4C7AA46D5" ;
                                       rdfs:comment "Resource registration has been suspended" ;
                                       rdfs:label "Mothballed" .


:ResourceRegistrationStatus.Planned uml:id "_AE4F7E67-BEC9-4298-8404-ED705A8697AE" ;
                                    rdfs:comment "Registration status is in the planning stage" ;
                                    rdfs:label "Planned" .


:ResultsConstraintType.Actual uml:id "_5C60DD53-9B42-4e5b-93D6-44F35E175EE9" ;
                              rdfs:comment "Actual." ;
                              rdfs:label "Actual" .


:ResultsConstraintType.Contingency uml:id "_90ECA92B-3B94-4ffb-9078-B4872950CCB5" ;
                                   rdfs:comment "Contingency." ;
                                   rdfs:label "Contingency" .


:ResultsConstraintType.FG_act uml:id "_EA4A49E9-04DF-4fe4-BC3C-0F8D0E3D1CFA" ;
                              rdfs:comment "Flowgate actual base case" ;
                              rdfs:label "FG_act" .


:ResultsConstraintType.Interface uml:id "_4B735140-B468-4e65-A97A-E4F94CF625C4" ;
                                 rdfs:comment "Interface." ;
                                 rdfs:label "Interface" .


:RetiredReasonKind.environmental uml:id "_93C1426C-D3E5-4d69-956E-DA85EB30A7E6" ;
                                 rdfs:comment "Retired due to environmental reasons." ;
                                 rdfs:label "environmental" .


:RetiredReasonKind.excessiveMaintenance uml:id "_365EF4C8-7EC1-4328-B01B-E81EF2500D3D" ;
                                        rdfs:comment "Retired due to excessive maintainance issues." ;
                                        rdfs:label "excessiveMaintenance" .


:RetiredReasonKind.facilitiesUpgrade uml:id "_EDE28E56-E708-4428-A6D0-35DB1230461B" ;
                                     rdfs:comment "Retired due to facility upgrade." ;
                                     rdfs:label "facilitiesUpgrade" .


:RetiredReasonKind.failed uml:id "_297E10AD-46C6-4ec9-9B34-7A7F438014E9" ;
                          rdfs:comment "Retired because of failure." ;
                          rdfs:label "failed" .


:RetiredReasonKind.obsolescence uml:id "_B9F097FD-782A-4f56-A47C-3FD08BCA531B" ;
                                rdfs:comment "Retired due to obsolescence." ;
                                rdfs:label "obsolescence" .


:RetiredReasonKind.other uml:id "_A6ED8064-9321-461e-AA0C-67FEE3F00053" ;
                         rdfs:comment "Retired due to other reasons." ;
                         rdfs:label "other" .


:RetiredReasonKind.sold uml:id "_97A6F21C-E45F-4d86-84AD-724745CE3B8F" ;
                        rdfs:comment "Retired and sold." ;
                        rdfs:label "sold" .


:RevenueKind.commercial uml:id "_3F11FCF7-BB43-43eb-8C68-FCFA84C28228" ;
                        rdfs:comment "Commercial revenue." ;
                        rdfs:label "commercial" .


:RevenueKind.industrial uml:id "_A863A2D9-DE9E-4505-9A5D-81EE54FC0934" ;
                        rdfs:comment "Industrial revenue." ;
                        rdfs:label "industrial" .


:RevenueKind.irrigation uml:id "_84545366-9BBF-42c3-A57C-7F0619C3176E" ;
                        rdfs:comment "Irrigation revenue." ;
                        rdfs:label "irrigation" .


:RevenueKind.nonResidential uml:id "_010E8E86-7A0E-4ced-A464-7D4852453839" ;
                            rdfs:comment "Non-residential revenue." ;
                            rdfs:label "nonResidential" .


:RevenueKind.other uml:id "_4F23130D-2BC1-4874-9355-5BB460BECDC2" ;
                   rdfs:comment "Other revenue kind." ;
                   rdfs:label "other" .


:RevenueKind.residential uml:id "_24E5488F-4E2C-4dde-A82A-A44977329DE3" ;
                         rdfs:comment "Residential revenue." ;
                         rdfs:label "residential" .


:RevenueKind.streetLight uml:id "_14E83C5D-CCD8-4d25-B086-A56E81F95FB3" ;
                         rdfs:comment "Streetlight revenue." ;
                         rdfs:label "streetLight" .


:RevisionKind.added uml:id "_5FEBE367-88B7-4955-AD96-7D84C5CDC17C" ;
                    rdfs:label "added" .


:RevisionKind.void uml:id "_4690314B-C5AA-49a6-B6FB-81B1F4E50494" ;
                   rdfs:label "void" .


:RiskScoreKind.customerRisk uml:id "_BA90BF1F-788F-4154-92E8-B0623B9FCD00" ;
                            rdfs:comment "Customer risk score." ;
                            rdfs:label "customerRisk" .


:RiskScoreKind.financialRisk uml:id "_37E40816-D083-483f-88DF-9BA68D251EDC" ;
                             rdfs:comment "Financial risk score." ;
                             rdfs:label "financialRisk" .


:RiskScoreKind.safetyRisk uml:id "_0E3994A5-849C-4bc5-80DF-E580AD1FC616" ;
                          rdfs:comment "Safety risk score." ;
                          rdfs:label "safetyRisk" .


:RotorKind.roundRotor uml:id "_67CB8B97-107B-40bc-8BFD-21812D8CCE2D" ;
                      rdfs:comment "Round rotor type of synchronous machine." ;
                      rdfs:label "roundRotor" .


:RotorKind.salientPole uml:id "_3D4CFF27-DA7C-4073-B80B-790D600A5036" ;
                       rdfs:comment "Salient pole type of synchronous machine." ;
                       rdfs:label "salientPole" .


:SVCControlMode.reactivePower uml:id "_1090360B-E8A3-4e71-B538-629F660CB01B" ;
                              rdfs:comment "Reactive power control." ;
                              rdfs:label "reactivePower" .


:SVCControlMode.voltage uml:id "_34BA1F29-A5C7-4f29-89FF-B8186FCF7B87" ;
                        rdfs:comment "Voltage control." ;
                        rdfs:label "voltage" .


:SampleContainerType.glassCan uml:id "_A022AA80-D1EF-48d9-B0C9-BC243A6DCD2B" ;
                              rdfs:comment "Glass can container." ;
                              rdfs:label "glassCan" .


:SampleContainerType.metalCan uml:id "_D7D5BCA6-5BB5-42b1-9A06-FD06E43CFE5B" ;
                              rdfs:comment "Metal can container." ;
                              rdfs:label "metalCan" .


:SampleContainerType.syringe uml:id "_5938B3A5-8254-4d88-922A-14E1E38B5EE4" ;
                             rdfs:comment "Syringe." ;
                             rdfs:label "syringe" .


:ScaleKind.exponential uml:id "_332B5C30-08A4-4e89-84C8-D215E949DFAC" ;
                       rdfs:comment "Exponential scale." ;
                       rdfs:label "exponential" .


:ScaleKind.linear uml:id "_A0DCBD6C-A616-44a6-BE00-BAFAFED94E8D" ;
                  rdfs:comment "Linear scale." ;
                  rdfs:label "linear" .


:SchedClassType.F uml:id "_8F28E40A-BE99-4fdc-8A0F-8C0FB91A465B" ;
                  rdfs:label "F" .


:SchedClassType.P uml:id "_D91DCF8F-AFFB-433a-8924-E7CFE27C5C17" ;
                  rdfs:label "P" .


:SchedClassType.R uml:id "_E0149A66-D0F6-4ffc-A7E2-CEB756CB19EF" ;
                  rdfs:label "R" .


:SealConditionKind.broken uml:id "_24F77781-F3C9-4862-AF1E-AF413F8E0C43" ;
                          rdfs:comment "Seal is broken." ;
                          rdfs:label "broken" .


:SealConditionKind.locked uml:id "_3D0A12C2-3CF1-4821-AB3C-7F646ACF4934" ;
                          rdfs:comment "Seal is locked." ;
                          rdfs:label "locked" .


:SealConditionKind.missing uml:id "_DB741A15-5087-4fc9-8C22-E46B268E43F6" ;
                           rdfs:comment "Seal is missing." ;
                           rdfs:label "missing" .


:SealConditionKind.open uml:id "_D14BA5DD-8A6D-4cf4-837F-553119D2CA28" ;
                        rdfs:comment "Seal is open." ;
                        rdfs:label "open" .


:SealConditionKind.other uml:id "_0B1562FA-592F-4a8c-AC96-06DBA12A3194" ;
                         rdfs:comment "Other kind of seal condition." ;
                         rdfs:label "other" .


:SealKind.lead uml:id "_F5621AC0-6891-4a99-ACC0-4B5FBC69D8ED" ;
               rdfs:comment "Lead seal." ;
               rdfs:label "lead" .


:SealKind.lock uml:id "_609E80A5-1B4C-4dfa-80D9-2457F4B0846B" ;
               rdfs:comment "Lock seal." ;
               rdfs:label "lock" .


:SealKind.other uml:id "_1C12FE57-1A7E-43f3-9FD0-849EBD08FD08" ;
                rdfs:comment "Other kind of seal." ;
                rdfs:label "other" .


:SealKind.steel uml:id "_9BD65DAC-06E2-4117-A850-1F076F52E20D" ;
                rdfs:comment "Steel seal." ;
                rdfs:label "steel" .


:SegmentCurveType.CONSULTATIVE uml:id "_4E191ABB-4BA8-4c84-BC80-B1DAF017E057" ;
                               rdfs:label "CONSULTATIVE" .


:SegmentCurveType.COST uml:id "_014C9B4A-2343-44b1-8CF8-77831D8C5555" ;
                       rdfs:label "COST" .


:SelfSchedReferenceType.ETC uml:id "_49205AF0-D100-4c00-99B9-85502ABB7E5B" ;
                            rdfs:comment "Existing transmission contract." ;
                            rdfs:label "ETC" .


:SelfSchedReferenceType.TOR uml:id "_2A9C5C05-F87E-4d66-B643-D981638B5E5D" ;
                            rdfs:comment "Transmission ownership right." ;
                            rdfs:label "TOR" .


:SelfSchedTypeCleanBid.BAS uml:id "_73FE9AAC-7DC0-4c61-BD2E-19D014DB8570" ;
                           rdfs:label "BAS" .


:SelfSchedTypeCleanBid.ETC uml:id "_FF45B09C-ECE4-43a1-8EBD-1C91F6AD7FE5" ;
                           rdfs:label "ETC" .


:SelfSchedTypeCleanBid.IFM uml:id "_0F60909D-7AC3-4cc6-A6A7-89BDC0AB8C33" ;
                           rdfs:label "IFM" .


:SelfSchedTypeCleanBid.LOF uml:id "_C05288FD-AC61-4e11-9C43-BC7A062B9C4E" ;
                           rdfs:label "LOF" .


:SelfSchedTypeCleanBid.LPT uml:id "_1D4D3176-7F4D-4105-8D91-0F31205EBDC3" ;
                           rdfs:label "LPT" .


:SelfSchedTypeCleanBid.PT uml:id "_CFDA88B0-7DCE-44ee-B10A-2764798FD5FF" ;
                          rdfs:label "PT" .


:SelfSchedTypeCleanBid.RA uml:id "_7E9E7FBB-7727-4442-BC95-8F9568653924" ;
                          rdfs:comment "RA Obligations" ;
                          rdfs:label "RA" .


:SelfSchedTypeCleanBid.RMT uml:id "_0D10027B-C981-4795-982A-1CB77645AC7B" ;
                           rdfs:label "RMT" .


:SelfSchedTypeCleanBid.SP uml:id "_32C520AC-9CE0-4bd4-A8EF-090BAB632840" ;
                          rdfs:comment "Self-Provision" ;
                          rdfs:label "SP" .


:SelfSchedTypeCleanBid.TOR uml:id "_2BF1554E-0155-4146-AFAD-F954E89E1629" ;
                           rdfs:label "TOR" .


:SelfSchedTypeCleanBid.WHL uml:id "_EB6BFE36-8341-4cad-95B4-9A32F204ABC2" ;
                           rdfs:label "WHL" .


:SelfSchedTypeRawBid.BAS uml:id "_AFCEBF48-8017-4c7c-A3B3-626C475C10A1" ;
                         rdfs:label "BAS" .


:SelfSchedTypeRawBid.ETC uml:id "_128BEA1C-F08F-4264-A493-AC2B371A9DF3" ;
                         rdfs:label "ETC" .


:SelfSchedTypeRawBid.LOF uml:id "_BC24C35F-48CF-45b9-A86C-CAF529075D52" ;
                         rdfs:label "LOF" .


:SelfSchedTypeRawBid.LPT uml:id "_0F73B998-642B-46d3-9744-7B9FB339DD0D" ;
                         rdfs:label "LPT" .


:SelfSchedTypeRawBid.PT uml:id "_F90327F9-5926-4f36-8CD0-6AF837F28A0A" ;
                        rdfs:label "PT" .


:SelfSchedTypeRawBid.RA uml:id "_DB8F0DCF-F7ED-4b10-A050-1359EE4D2A60" ;
                        rdfs:comment "RA Obligations" ;
                        rdfs:label "RA" .


:SelfSchedTypeRawBid.RMT uml:id "_4012001F-7258-4c69-ACE7-5D1FADFBCE01" ;
                         rdfs:label "RMT" .


:SelfSchedTypeRawBid.SP uml:id "_3E0BE79A-C7E9-4c6c-976E-0618E164CC38" ;
                        rdfs:comment "Self-Provision" ;
                        rdfs:label "SP" .


:SelfSchedTypeRawBid.TOR uml:id "_80E3370C-8FC7-4490-A2E8-F110E3524069" ;
                         rdfs:label "TOR" .


:SelfSchedTypeRawBid.WHL uml:id "_32AB532D-F943-4d34-8785-1B1795719C61" ;
                         rdfs:label "WHL" .


:SelfScheduleBreakdownType.ETC uml:id "_99DCC81B-438A-4643-84E2-68194F67AAF4" ;
                               rdfs:comment "Existing transmission contract." ;
                               rdfs:label "ETC" .


:SelfScheduleBreakdownType.LPT uml:id "_6DD5221B-EEC5-4c40-A546-590FBFF4C8ED" ;
                               rdfs:comment "Low price taker." ;
                               rdfs:label "LPT" .


:SelfScheduleBreakdownType.TOR uml:id "_511B0078-3A69-4783-8B7C-6CC2E1E2857D" ;
                               rdfs:comment "Transmission ownership right." ;
                               rdfs:label "TOR" .


:SelfScheduleType.BAS uml:id "_2B6A306B-C1DE-40d7-8671-C59AA137AE49" ;
                      rdfs:comment "Base Schedule" ;
                      rdfs:label "BAS" .


:SelfScheduleType.ETC uml:id "_595D5F81-623F-40ed-A84C-E2ED32D390B2" ;
                      rdfs:label "ETC" .


:SelfScheduleType.IFM uml:id "_7B361B1F-ABD8-4b14-B784-8808DB996FC1" ;
                      rdfs:label "IFM" .


:SelfScheduleType.LOF uml:id "_95BD61E0-0875-44c5-B6EF-46042D0636F0" ;
                      rdfs:comment "Lay-off schedule" ;
                      rdfs:label "LOF" .


:SelfScheduleType.ORFC uml:id "_58776BDA-808F-48a8-8C34-795246613DBD" ;
                       rdfs:label "ORFC" .


:SelfScheduleType.PT uml:id "_99F046A7-4103-475a-A359-BD19728675B6" ;
                     rdfs:label "PT" .


:SelfScheduleType.PUMP_ETC uml:id "_B2A5F062-6172-4cf4-9B75-C6ED5F230C67" ;
                           rdfs:label "PUMP_ETC" .


:SelfScheduleType.PUMP_TOR uml:id "_E6CDCE4C-A18E-4305-B377-89C9FE185F34" ;
                           rdfs:label "PUMP_TOR" .


:SelfScheduleType.RA uml:id "_A7170F2D-9F2D-41fc-BDE3-6EDA12EB19B1" ;
                     rdfs:comment "RA Obligations" ;
                     rdfs:label "RA" .


:SelfScheduleType.RGMR uml:id "_C212A076-AB49-45e0-93CA-7E5C621CD226" ;
                       rdfs:label "RGMR" .


:SelfScheduleType.RMR uml:id "_4426F2E9-6D96-4162-81CC-F33628D323DD" ;
                      rdfs:label "RMR" .


:SelfScheduleType.RMT uml:id "_30CB3C2D-2BBB-4239-A44F-1888B278AFD1" ;
                      rdfs:label "RMT" .


:SelfScheduleType.RUC uml:id "_45BC35BE-880A-47a3-A80E-7CA7590799B2" ;
                      rdfs:label "RUC" .


:SelfScheduleType.SP uml:id "_7D27275C-A8E1-4c67-AB7B-99198E432AA1" ;
                     rdfs:comment "Self-Provision" ;
                     rdfs:label "SP" .


:SelfScheduleType.TOR uml:id "_CFD2B9EE-1BB4-4f3b-AD48-3BEA16EC9C98" ;
                      rdfs:label "TOR" .


:SelfScheduleType.WHL uml:id "_9B485B3D-97BF-422a-AA30-D7B768939118" ;
                      rdfs:label "WHL" .


:SelfScheduleTypeMB.RMR uml:id "_EBAEAF0C-EF0F-4eb7-A701-E37E12D65922" ;
                        rdfs:label "RMR" .


:ServiceKind.air uml:id "_6EA2B7D5-877E-40f9-A417-2540E85DB19C" ;
                 rdfs:comment "Air service." ;
                 rdfs:label "air" .


:ServiceKind.electricity uml:id "_7F85E37C-53E2-4945-B940-7AFF43790F0D" ;
                         rdfs:comment "Electricity service." ;
                         rdfs:label "electricity" .


:ServiceKind.gas uml:id "_29A7BD4A-0D46-4974-BD81-5B3C9675EB6D" ;
                 rdfs:comment "Gas service." ;
                 rdfs:label "gas" .


:ServiceKind.heat uml:id "_70542D24-37A9-4815-ABF0-08DBD4466147" ;
                  rdfs:comment "Heat service." ;
                  rdfs:label "heat" .


:ServiceKind.heatingFluid uml:id "_872097F7-04A9-4183-8B84-5AB064173457" ;
                          rdfs:comment "Heating fluid service." ;
                          rdfs:label "heatingFluid" .


:ServiceKind.internet uml:id "_89425E98-6977-4c45-A1D5-2503401443BF" ;
                      rdfs:comment "Internet service." ;
                      rdfs:label "internet" .


:ServiceKind.naturalGas uml:id "_C9194C7B-CAC6-451c-8B33-9EFC7EE9D52B" ;
                        rdfs:comment "Natural gas service." ;
                        rdfs:label "naturalGas" .


:ServiceKind.other uml:id "_D68430F7-15F7-411d-BB9C-2F621E810228" ;
                   rdfs:comment "Other kind of service." ;
                   rdfs:label "other" .


:ServiceKind.propane uml:id "_5CBFA9A4-11D9-428e-A61E-B4966F202D4A" ;
                     rdfs:comment "Propane service." ;
                     rdfs:label "propane" .


:ServiceKind.rates uml:id "_EFD8A796-7B1E-4d44-8C65-BFECC4CABBC2" ;
                   rdfs:comment "Rates (e.g. tax, charge, toll, duty, tariff, etc.) service." ;
                   rdfs:label "rates" .


:ServiceKind.refuse uml:id "_A9EF0C5F-F8D5-4835-9AFC-7638A4897D21" ;
                    rdfs:comment "Refuse (waster) service." ;
                    rdfs:label "refuse" .


:ServiceKind.sewerage uml:id "_AE59843D-C3DF-4411-BEC5-39C9B7889501" ;
                      rdfs:comment "Sewerage service." ;
                      rdfs:label "sewerage" .


:ServiceKind.steam uml:id "_BAC861E1-7AA2-44a2-BDCE-644F80C624DD" ;
                   rdfs:comment "Steam service." ;
                   rdfs:label "steam" .


:ServiceKind.time uml:id "_43D17447-FF5C-4002-B5BA-69C6B0C8DC55" ;
                  rdfs:comment "Time service." ;
                  rdfs:label "time" .


:ServiceKind.tvLicence uml:id "_05AF4975-59AC-416b-8819-D5AEC405FC7D" ;
                       rdfs:comment "TV license service." ;
                       rdfs:label "tvLicence" .


:ServiceKind.water uml:id "_4A2E4707-7C89-44b8-AB92-AFAA39137545" ;
                   rdfs:comment "Water service." ;
                   rdfs:label "water" .


:ServiceMultiplierKind.ctRatio uml:id "_8CCE45CF-9B38-4236-9B61-F2C3CA587FC8" ;
                               rdfs:comment "Current transformer ratio used to convert associated quantities to real measurements." ;
                               rdfs:label "ctRatio" .


:ServiceMultiplierKind.ptRatio uml:id "_F768471A-51F5-4093-8E9F-0E84AD144DF8" ;
                               rdfs:comment "Voltage transformer ratio used to convert associated quantities to real measurements." ;
                               rdfs:label "ptRatio" .


:ServiceMultiplierKind.transformerRatio uml:id "_5CF72AAB-CB7C-4cd0-9F45-1A597458FC3D" ;
                                        rdfs:comment "Product of the CT ratio and PT ratio." ;
                                        rdfs:label "transformerRatio" .


:ServiceRequestKind.connect uml:id "_3FA4216F-8D0F-4431-BC82-527FC8EAA23F" ;
                            rdfs:comment "Physically connect the service." ;
                            rdfs:label "connect" .


:ServiceRequestKind.construction uml:id "_8D54A546-D558-4f4a-9956-9E08914DCE06" ;
                                 rdfs:comment "The construction work requested." ;
                                 rdfs:label "construction" .


:ServiceRequestKind.disconnect uml:id "_393EAA45-F074-4d5a-9B7E-11F96BD3D2E5" ;
                               rdfs:comment "Physically disconnect the service." ;
                               rdfs:label "disconnect" .


:ServiceRequestKind.inspection uml:id "_B46F330B-57F7-437a-BEC7-A351FED8156C" ;
                               rdfs:comment "Inspection work." ;
                               rdfs:label "inspection" .


:ServiceRequestKind.newservice uml:id "_FA9567F1-823D-4646-A10A-B3773C54A163" ;
                               rdfs:comment "A new service is requested by the customer" ;
                               rdfs:label "newservice" .


:ServiceRequestKind.other uml:id "_B9E44DCD-DBE4-4dfe-890E-D0075166BF20" ;
                          rdfs:comment "Other kind of work." ;
                          rdfs:label "other" .


:ServiceRequestKind.reconnect uml:id "_84DE3CB2-18EA-4c2f-822E-220F1E646221" ;
                              rdfs:comment "Physically reconnect the service." ;
                              rdfs:label "reconnect" .


:ServiceRequestKind.repair uml:id "_999D4469-232D-43e9-A6FC-73964D88CE63" ;
                           rdfs:comment "Repair work." ;
                           rdfs:label "repair" .


:ServiceRequestKind.replace uml:id "_200EBC4F-458D-43c1-81AD-EF78BAEA1B3E" ;
                            rdfs:comment "replace an asset" ;
                            rdfs:label "replace" .


:ServiceRequestKind.test uml:id "_AB40C564-85E2-4e48-AEA5-3293DF4E6556" ;
                         rdfs:comment "Test work." ;
                         rdfs:label "test" .


:ServiceRequestKind.turn-off uml:id "_DF415607-C772-4fd7-AAE2-DBD792B56C2F" ;
                             rdfs:comment "Temporarily turn off the service but leave the connection in place." ;
                             rdfs:label "turn-off" .


:ServiceRequestKind.turn-on uml:id "_E7CD4647-C612-4a1e-8D7A-EE4807C6E3B4" ;
                            rdfs:comment "Turn on the service." ;
                            rdfs:label "turn-on" .


:ShortCircuitRotorKind.salientPole1 uml:id "_C6224E17-3C55-41b4-96B0-A7D760836509" ;
                                    rdfs:comment "Salient pole 1 in IEC 60909." ;
                                    rdfs:label "salientPole1" .


:ShortCircuitRotorKind.salientPole2 uml:id "_45389D96-7D96-435f-B054-391491734D26" ;
                                    rdfs:comment "Salient pole 2 in IEC 60909." ;
                                    rdfs:label "salientPole2" .


:ShortCircuitRotorKind.turboSeries1 uml:id "_C330D074-B02F-46e4-B49E-2F5AAF36FFE0" ;
                                    rdfs:comment "Turbo Series 1 in IEC 60909." ;
                                    rdfs:label "turboSeries1" .


:ShortCircuitRotorKind.turboSeries2 uml:id "_F5BECE1F-74CA-4c01-8AD2-6093E28CC2AF" ;
                                    rdfs:comment "Turbo series 2 in IEC 60909." ;
                                    rdfs:label "turboSeries2" .


:ShuntImpedanceControlKind.fixed uml:id "_E2EEC3F1-49C1-4d81-BB2B-09839E687C37" ;
                                 rdfs:label "fixed" .


:ShuntImpedanceControlKind.localOnly uml:id "_4AE4E7F0-DF5A-4f36-B980-F7F60E44EC5D" ;
                                     rdfs:label "localOnly" .


:ShuntImpedanceControlKind.remoteOnly uml:id "_29DDFAFE-5682-49f8-B9AA-F80ADBE3FA20" ;
                                      rdfs:label "remoteOnly" .


:ShuntImpedanceControlKind.remoteWithLocalOverride uml:id "_7B40D412-6D0F-4f91-A609-07ACC7DFDD8B" ;
                                                   rdfs:label "remoteWithLocalOverride" .


:ShuntImpedanceLocalControlKind.current uml:id "_59C4859C-A809-4cbc-A9C5-AF2DCF5DC8E6" ;
                                        rdfs:label "current" .


:ShuntImpedanceLocalControlKind.none uml:id "_A9E6A720-8379-4788-93E8-8669DF42B249" ;
                                     rdfs:label "none" .


:ShuntImpedanceLocalControlKind.powerFactor uml:id "_0423B958-8C0F-4ee3-BAFD-F949A9C07892" ;
                                            rdfs:label "powerFactor" .


:ShuntImpedanceLocalControlKind.reactivePower uml:id "_57531641-5175-4c05-AA18-6141E897E0EB" ;
                                              rdfs:label "reactivePower" .


:ShuntImpedanceLocalControlKind.temperature uml:id "_59E3E447-A9CF-484d-A056-4D6E52E2BE91" ;
                                            rdfs:label "temperature" .


:ShuntImpedanceLocalControlKind.time uml:id "_0027B6DD-FEFC-49b9-9C6C-3945C9B3B565" ;
                                     rdfs:label "time" .


:ShuntImpedanceLocalControlKind.voltage uml:id "_8550A25E-2926-423f-A26F-E3FE0CB36E2B" ;
                                        rdfs:label "voltage" .


:SinglePhaseKind.A uml:id "_C02D22F4-5CA2-437e-9F27-95F4BFC8B870" ;
                   rdfs:comment "Phase A." ;
                   rdfs:label "A" .


:SinglePhaseKind.B uml:id "_321F86C8-F9F3-4a29-B0C8-BE4329CC578A" ;
                   rdfs:comment "Phase B." ;
                   rdfs:label "B" .


:SinglePhaseKind.C uml:id "_75A291F3-4B98-4d53-ADC8-6A8C31AEBF8D" ;
                   rdfs:comment "Phase C." ;
                   rdfs:label "C" .


:SinglePhaseKind.N uml:id "_544E8D1F-5B68-4435-8096-1BA22C0AC0BA" ;
                   rdfs:comment "Neutral." ;
                   rdfs:label "N" .


:SinglePhaseKind.s1 uml:id "_DFA995B4-25EF-448a-973F-A013ADC35EA7" ;
                    rdfs:comment "Secondary phase 1." ;
                    rdfs:label "s1" .


:SinglePhaseKind.s2 uml:id "_B1ED33EE-4FE9-48c2-A80B-25B1A8576E26" ;
                    rdfs:comment "Secondary phase 2." ;
                    rdfs:label "s2" .


:SkillLevelKind.apprentice uml:id "_84B8E457-6590-4d5d-8060-B0F847F93A11" ;
                           rdfs:label "apprentice" .


:SkillLevelKind.master uml:id "_03D4595F-C2A2-4ced-9C89-E47BE1AA3C3F" ;
                       rdfs:label "master" .


:SkillLevelKind.other uml:id "_A09B1665-0095-4b5b-9BB8-AC9420B00613" ;
                      rdfs:label "other" .


:SkillLevelKind.standard uml:id "_9E2D8894-497F-4705-99FD-D5D45F95AC48" ;
                         rdfs:label "standard" .


:Source.DEFAULTED uml:id "_A72974EF-B5C3-4d7b-8CA5-3C16B95E4A1C" ;
                  rdfs:comment "The value contains a default value." ;
                  rdfs:label "DEFAULTED" .


:Source.PROCESS uml:id "_1BA84003-B2F9-4264-97A4-C7A0AD5541D1" ;
                rdfs:comment "The value is provided by input from the process I/O or being calculated from some function." ;
                rdfs:label "PROCESS" .


:Source.SUBSTITUTED uml:id "_AFA40328-DD9C-4cd1-BB9B-4AC747AF3117" ;
                    rdfs:comment "The value is provided by input of an operator or by an automatic source." ;
                    rdfs:label "SUBSTITUTED" .


:SourceSinkFlag.CSNK uml:id "_5875D1FC-3543-48b0-AFE7-0E3E0A89DE1B" ;
                     rdfs:label "CSNK" .


:SourceSinkFlag.CSRC uml:id "_EBC677F3-DD28-4bd3-897A-DD44B93551A3" ;
                     rdfs:label "CSRC" .


:SourceSinkType.Neither uml:id "_877AA270-EF3B-4d45-A240-7901310A34FE" ;
                        rdfs:label "Neither" .


:SourceSinkType.Sink uml:id "_DC2E1C7C-659C-4c94-9A37-6D169CF8B82A" ;
                     rdfs:label "Sink" .


:SourceSinkType.Source uml:id "_E0542BA6-140D-4eb7-8E83-961562953215" ;
                       rdfs:label "Source" .


:SpaceAnalogKind.magneticFieldDirection uml:id "_E827C7EB-B9FB-4f6d-8004-9A43BA187E51" ;
                                        rdfs:label "magneticFieldDirection" .


:SpaceAnalogKind.magneticFieldStrength uml:id "_1BEF64C9-72D6-4e2a-A720-5884AE778DD4" ;
                                       rdfs:label "magneticFieldStrength" .


:SpinningEventNameType.EASTERN uml:id "_57669F56-1591-4eb8-A92E-C5C5C7744197" ;
                               rdfs:label "EASTERN" .


:SpinningEventNameType.PJM uml:id "_10C81FCB-4AA3-483e-AD8B-CDADB06A8FE0" ;
                           rdfs:label "PJM" .


:SpinningEventNameType.RFC-SR uml:id "_12AA8018-F28B-47a8-8C74-65798754AC77" ;
                              rdfs:label "RFC-SR" .


:SpinningEventNameType.SOUTH-S uml:id "_21BFC07D-92C7-4ce9-8211-4955E6E4511A" ;
                               rdfs:label "SOUTH-S" .


:SpinningEventType.AA uml:id "_5569BB81-07B2-45a6-979F-1A704621F0FB" ;
                      rdfs:label "AA" .


:SpinningEventType.CA uml:id "_4133A2EF-39F8-47ba-9345-4E5C85AFD71F" ;
                      rdfs:label "CA" .


:SpinningEventType.RZ uml:id "_4A563DAC-C63D-4d80-A403-B16B2BD84F2A" ;
                      rdfs:label "RZ" .


:StaticLoadModelKind.constantZ uml:id "_B1BBDC91-9A07-4bad-9063-52E92C620FC6" ;
                               rdfs:comment "The load is represented as a constant impedance.  ConstantZ equations are used  for active and reactive power and no attributes are required." ;
                               rdfs:label "constantZ" .


:StaticLoadModelKind.exponential uml:id "_514F69B7-F201-40b6-A6EE-D54CDB2A09B0" ;
                                 rdfs:comment """This model is an exponential representation of the load. Exponential equations for active and reactive power are used and the following attributes are required:
kp1, kp2, kp3, kpf, ep1, ep2, ep3
kq1, kq2, kq3, kqf, eq1, eq2, eq3.""" ;
                                 rdfs:label "exponential" .


:StaticLoadModelKind.zIP1 uml:id "_D902D0A5-4BA2-423a-B1AA-FCC601F95001" ;
                          rdfs:comment """This model integrates the frequency-dependent load (primarily motors).  ZIP1 equations for active and reactive power are used and the following attributes are required:
kp1, kp2, kp3, kpf
kq1, kq2, kq3, kqf.""" ;
                          rdfs:label "zIP1" .


:StaticLoadModelKind.zIP2 uml:id "_33B98922-364D-47a8-992D-5EF6DE24F0EC" ;
                          rdfs:comment """This model separates the frequency-dependent load (primarily motors) from other load.  ZIP2 equations for active and reactive power are used and the following attributes are required:
kp1, kp2, kp3, kq4, kpf
kq1, kq2, kq3, kq4, kqf.""" ;
                          rdfs:label "zIP2" .


:StreetlightLampKind.highPressureSodium uml:id "_6288DB78-C40C-42cc-A0B2-31B2835A1555" ;
                                        rdfs:label "highPressureSodium" .


:StreetlightLampKind.mercuryVapor uml:id "_8EE3F5B7-CC88-41d4-ACC6-317426F195CB" ;
                                  rdfs:label "mercuryVapor" .


:StreetlightLampKind.metalHalide uml:id "_7950134B-7889-4378-9590-D3D2CE552AA3" ;
                                 rdfs:label "metalHalide" .


:StreetlightLampKind.other uml:id "_1F4B7C50-3902-434c-B6D8-543542AF4903" ;
                           rdfs:label "other" .


:StructureMaterialKind.concrete uml:id "_3C9441EE-16E2-4e19-A998-70F6929D0BB9" ;
                                rdfs:label "concrete" .


:StructureMaterialKind.other uml:id "_478A01F9-B40C-4ecf-A476-B0D58CF5E754" ;
                             rdfs:label "other" .


:StructureMaterialKind.steel uml:id "_3BDCE7BB-70EA-4bd8-9183-768E4F6E6BDE" ;
                             rdfs:label "steel" .


:StructureMaterialKind.wood uml:id "_C3D3746E-7135-4836-96CF-AFF53CC0AA47" ;
                            rdfs:label "wood" .


:StructureSupportKind.anchor uml:id "_E8DBBCAC-5BF8-4242-AF88-0055B09949C0" ;
                             rdfs:label "anchor" .


:StructureSupportKind.guy uml:id "_E2F2C63E-073C-423d-AFC3-15A088DB2651" ;
                          rdfs:label "guy" .


:SupplierKind.lse uml:id "_F8249DFD-3B4F-4bb9-8FEA-011EDFF53695" ;
                  rdfs:comment "Load Serving Entity" ;
                  rdfs:label "lse" .


:SupplierKind.mdma uml:id "_83236180-1B98-4e79-B9AD-63111CB7AAD5" ;
                   rdfs:comment "Meter Data Management Agent (MDMA) reads meters, validates meter data, and estimates missing data to be used in various applications" ;
                   rdfs:label "mdma" .


:SupplierKind.msp uml:id "_2983E6CC-5243-4499-807E-16AEA952110F" ;
                  rdfs:comment "Managed service provider (MSP) delivers services, such as network, application, infrastructure and security, via ongoing and regular support and active administration" ;
                  rdfs:label "msp" .


:SupplierKind.other uml:id "_8B8FB194-E726-45df-9EA8-599524E26A75" ;
                    rdfs:comment "Other kind of supplier." ;
                    rdfs:label "other" .


:SupplierKind.retailer uml:id "_965EE54C-D4E5-4b6a-A6B3-8D9B2A4618F8" ;
                       rdfs:comment "Entity that sells the service, but does not deliver to the customer; applies to the deregulated markets." ;
                       rdfs:label "retailer" .


:SupplierKind.utility uml:id "_D8BF1314-1DA4-4522-B101-25B6100F041C" ;
                      rdfs:comment "Entity that delivers the service to the customer." ;
                      rdfs:label "utility" .


:SwitchActionKind.close uml:id "_3492915F-C6CA-4315-ADC6-B3CBF8240948" ;
                        rdfs:comment "Close the switch." ;
                        rdfs:label "close" .


:SwitchActionKind.disableReclosing uml:id "_E5F6008A-56A0-4f1f-BB3E-86D94F6A360D" ;
                                   rdfs:comment "Disable (automatic) switch reclosing." ;
                                   rdfs:label "disableReclosing" .


:SwitchActionKind.enableReclosing uml:id "_86E39986-025E-400b-B435-93EB055DCD20" ;
                                  rdfs:comment "Enable (automatic) switch reclosing." ;
                                  rdfs:label "enableReclosing" .


:SwitchActionKind.open uml:id "_6A4C2BE8-9771-457b-9011-D9023B75840F" ;
                       rdfs:comment "Open the switch." ;
                       rdfs:label "open" .


:SwitchStatusType.Closed uml:id "_DB8AF56A-9984-474f-840B-4C3B1132576E" ;
                         rdfs:comment "Closed status." ;
                         rdfs:label "Closed" .


:SwitchStatusType.Open uml:id "_99FE3FFC-2570-4e44-AE1B-304CA36679D9" ;
                       rdfs:comment "Open status." ;
                       rdfs:label "Open" .


:SynchronousMachineKind.condenser uml:id "_AB175867-D096-4c32-9722-1B571D44A22E" ;
                                  rdfs:comment "Indicates the synchronous machine can operate as a condenser." ;
                                  rdfs:label "condenser" .


:SynchronousMachineKind.generator uml:id "_EC04A0D2-3B94-4d7b-B3F1-F2A3321B7BC4" ;
                                  rdfs:comment "Indicates the synchronous machine can operate as a generator." ;
                                  rdfs:label "generator" .


:SynchronousMachineKind.generatorOrCondenser uml:id "_1077F20F-1198-4e1b-87A6-5BAAA6B34F72" ;
                                             rdfs:comment "Indicates the synchronous machine can operate as a generator or as a condenser." ;
                                             rdfs:label "generatorOrCondenser" .


:SynchronousMachineKind.generatorOrCondenserOrMotor uml:id "_E147ABB7-F0AA-4ddc-9DAF-14BF3F50DA4F" ;
                                                    rdfs:comment "Indicates the synchronous machine can operate as a generator or as a condenser or as a motor." ;
                                                    rdfs:label "generatorOrCondenserOrMotor" .


:SynchronousMachineKind.generatorOrMotor uml:id "_653D9CA7-A063-4851-9E36-B7B85BE1BE10" ;
                                         rdfs:comment "Indicates the synchronous machine can operate as a generator or as a motor." ;
                                         rdfs:label "generatorOrMotor" .


:SynchronousMachineKind.motor uml:id "_C5DA8C90-AC9E-48b6-A58A-DF9A0352F3A0" ;
                              rdfs:comment "Indicates the synchronous machine can operate as a motor." ;
                              rdfs:label "motor" .


:SynchronousMachineKind.motorOrCondenser uml:id "_F1D15583-2559-4100-B262-83DB325BA34F" ;
                                         rdfs:comment "Indicates the synchronous machine can operate as a motor or as a condenser." ;
                                         rdfs:label "motorOrCondenser" .


:SynchronousMachineModelKind.subtransient uml:id "_D2B83ED1-6190-4d28-B8E7-4227C3C9F4DC" ;
                                          rdfs:comment "Subtransient synchronous machine model." ;
                                          rdfs:label "subtransient" .


:SynchronousMachineModelKind.subtransientSimplified uml:id "_3A6850C7-98D5-4f40-8A3D-4A7E868646EC" ;
                                                    rdfs:comment "Simplified version of subtransient synchronous machine model where magnetic coupling between the direct- and quadrature- axes is ignored." ;
                                                    rdfs:label "subtransientSimplified" .


:SynchronousMachineModelKind.subtransientSimplifiedDirectAxis uml:id "_4AC186DC-E7A7-4064-A694-2B08B9AB3463" ;
                                                              rdfs:comment "Simplified version of a subtransient synchronous machine model with no damper circuit on the direct-axis." ;
                                                              rdfs:label "subtransientSimplifiedDirectAxis" .


:SynchronousMachineModelKind.subtransientTypeF uml:id "_47A8D174-4052-46b2-B7EC-60F89AF73616" ;
                                               rdfs:comment "WECC type F variant of subtransient synchronous machine model." ;
                                               rdfs:label "subtransientTypeF" .


:SynchronousMachineModelKind.subtransientTypeJ uml:id "_11F5A58F-E9C4-4922-8C3A-B3548106982F" ;
                                               rdfs:comment "WECC type J variant of subtransient synchronous machine model." ;
                                               rdfs:label "subtransientTypeJ" .


:SynchronousMachineOperatingMode.condenser uml:id "_4138AC1B-4414-4b66-BFA5-953427ABCA45" ;
                                           rdfs:comment "Operating as condenser." ;
                                           rdfs:label "condenser" .


:SynchronousMachineOperatingMode.generator uml:id "_BC2CBA19-B1E8-498a-A688-965827939158" ;
                                           rdfs:comment "Operating as generator." ;
                                           rdfs:label "generator" .


:SynchronousMachineOperatingMode.motor uml:id "_C66DF514-4509-4123-B2FB-C834F58BDAE3" ;
                                       rdfs:comment "Operating as motor." ;
                                       rdfs:label "motor" .


:SystemType.OASIS uml:id "_1614F4FA-DC58-4748-AEFA-C6A5A3C353E1" ;
                  rdfs:label "OASIS" .


:TAPPIStandardEditionKind._2009 uml:id "_866762AB-80D1-4cc5-918F-603AAC6212D7" ;
                                rdfs:comment "2009 standard edition." ;
                                rdfs:label "2009" .


:TAPPIStandardEditionKind.none uml:id "_679360AA-4175-481a-BCD8-5B12022AAFBD" ;
                               rdfs:comment "No standard edition." ;
                               rdfs:label "none" .


:TAPPIStandardEditionKind.unknown uml:id "_8AC947B6-D624-4f24-9DC5-608D01E70C2B" ;
                                  rdfs:comment "Unknown standard edition." ;
                                  rdfs:label "unknown" .


:TAPPIStandardKind.T494 uml:id "_39735D76-E128-4ae8-8082-ADC61EDF59A9" ;
                        rdfs:comment "Tensile properties of paper and paperboard(using constant rate of elongation apparatus), Test Method TAPPI/ANSI T 494 om-13." ;
                        rdfs:label "T494" .


:TRType.CHAIN uml:id "_7EC5F6D5-6BF2-4264-BA1A-9CEF645F1901" ;
              rdfs:comment "TR chain" ;
              rdfs:label "CHAIN" .


:TRType.INDIVIDUAL uml:id "_2BAA1F74-5482-4e66-8A97-B9E70517BC1D" ;
                   rdfs:comment "Individual TR" ;
                   rdfs:label "INDIVIDUAL" .


:TagActionKind.place uml:id "_1F2B4888-B888-4453-87C4-FF46E0BF28A9" ;
                     rdfs:comment "Place the tag." ;
                     rdfs:label "place" .


:TagActionKind.remove uml:id "_5589EE0A-54B5-4c67-A575-76B57246B24E" ;
                      rdfs:comment "Remove the tag." ;
                      rdfs:label "remove" .


:TagActionKind.verify uml:id "_8A8D68F1-45FB-4e1d-9F2F-400A797ACB9D" ;
                      rdfs:comment "Verify the tag." ;
                      rdfs:label "verify" .


:TempEquipActionKind.connect uml:id "_A85F295B-6F75-4993-B5D6-8985A1376E75" ;
                             rdfs:comment "Connect the temp equipment to its terminal" ;
                             rdfs:label "connect" .


:TempEquipActionKind.disconnect uml:id "_9339ED3C-0246-4e08-B5E6-A1336053C123" ;
                                rdfs:comment "Disconnect the temp equipment from its terminal" ;
                                rdfs:label "disconnect" .


:TempEquipActionKind.place uml:id "_7963F759-746C-4bc0-AEC7-6CF5CD8D24A7" ;
                           rdfs:comment "Place the jumper (close) or the cut (open)." ;
                           rdfs:label "place" .


:TempEquipActionKind.remove uml:id "_6D0261B3-86EF-4d7a-B612-E429DD2757B0" ;
                            rdfs:comment "Remove the jumper (open) or the cut (close)." ;
                            rdfs:label "remove" .


:TenderKind.card uml:id "_EB9C23F6-71E3-4cc8-8E01-F0D70826C5BA" ;
                 rdfs:comment "Payment method by means of a credit or debit card." ;
                 rdfs:label "card" .


:TenderKind.cash uml:id "_B76A01E5-26C2-4dc6-A20F-5FBEDBFECE23" ;
                 rdfs:comment "Payment method by means of cash." ;
                 rdfs:label "cash" .


:TenderKind.cheque uml:id "_2F7326F2-1F28-4e7e-8675-57AD5A2C115A" ;
                   rdfs:comment "Payment method by means of a cheque." ;
                   rdfs:label "cheque" .


:TenderKind.other uml:id "_CF959005-095D-45b5-A172-3AD3265A4E81" ;
                  rdfs:comment "Other payment method such as electronic finds transfer." ;
                  rdfs:label "other" .


:TenderKind.unspecified uml:id "_790101EC-F330-454f-94CB-59761E1C67BF" ;
                        rdfs:comment "Payment method is not known." ;
                        rdfs:label "unspecified" .


:TestKind.equalTo uml:id "_E5E79651-7C27-4bf2-A184-073C288EC394" ;
                  rdfs:label "equalTo" .


:TestKind.greaterThan uml:id "_6C844909-3462-44e5-8F8A-CADB305421A5" ;
                      rdfs:label "greaterThan" .


:TestKind.greaterThanOrEqualTo uml:id "_A0449644-F621-4910-82BC-69313F63E8B9" ;
                               rdfs:label "greaterThanOrEqualTo" .


:TestKind.lessThan uml:id "_F7342CD5-A8DF-43d5-8C7A-45F1683641EC" ;
                   rdfs:label "lessThan" .


:TestKind.lessThanOrEqualTo uml:id "_C36070E8-A220-47be-9CFD-16C35FE5900B" ;
                            rdfs:label "lessThanOrEqualTo" .


:TestMethod.D1275A uml:id "_1492AD6C-7FC1-419b-858D-3164BA0AE8AF" ;
                   rdfs:comment "D1275A method." ;
                   rdfs:label "D1275A" .


:TestMethod.D1275B uml:id "_EA5F9250-615F-44de-88A8-85BF52E8CB63" ;
                   rdfs:comment "D1275B method." ;
                   rdfs:label "D1275B" .


:TestMethod.D3612A uml:id "_E650E64D-3338-4982-8985-0B48A62F3F48" ;
                   rdfs:comment "D3612A method." ;
                   rdfs:label "D3612A" .


:TestMethod.D3612B uml:id "_33061CDE-F0E2-456c-82E4-675DF511209C" ;
                   rdfs:comment "D3612B method." ;
                   rdfs:label "D3612B" .


:TestMethod.D3612C uml:id "_2FDB250C-E5A4-416e-8C82-F6BD26F25898" ;
                   rdfs:comment "D3612C method." ;
                   rdfs:label "D3612C" .


:TestMethod._60567ByDisplacement uml:id "_DF88F1D5-FCD9-44a2-BA45-9E87CAEB4658" ;
                                 rdfs:comment "60567 by displacement method." ;
                                 rdfs:label "60567ByDisplacement" .


:TestMethod._60567ByPartition uml:id "_80D2E977-655D-449d-A16B-5B2C2A04520D" ;
                              rdfs:comment "60567 by partition method." ;
                              rdfs:label "60567ByPartition" .


:TestMethod._60567ByVacuum uml:id "_768C23E8-CF13-4921-9F90-D550A2DB9C15" ;
                           rdfs:comment "60567 by vacuum method." ;
                           rdfs:label "60567ByVacuum" .


:TestMethod._60970Automatic uml:id "_57D5F352-0502-44d5-AFEE-C074AA9FB95E" ;
                            rdfs:comment "Automatic method." ;
                            rdfs:label "60970Automatic" .


:TestMethod._60970Manual1 uml:id "_A5057FB6-9915-40bb-A4E7-6A676A088A28" ;
                          rdfs:comment "Manual method 1." ;
                          rdfs:label "60970Manual1" .


:TestMethod._60970Manual2 uml:id "_CEC3A5A0-4F0E-4e0c-9BA7-DBD1FECCDA50" ;
                          rdfs:comment "Manual method 2." ;
                          rdfs:label "60970Manual2" .


:TestMethod._61125A uml:id "_6EEF5CEA-3C50-466c-9E79-22AEC47A840F" ;
                    rdfs:comment "61125A method." ;
                    rdfs:label "61125A" .


:TestMethod._61125B uml:id "_1E68C35F-2919-4068-9BA3-585C95D2A8B5" ;
                    rdfs:comment "61125B method." ;
                    rdfs:label "61125B" .


:TestMethod._61125C uml:id "_24C8FDA4-8CF2-44d2-8479-47308684A0E8" ;
                    rdfs:comment "61125C method." ;
                    rdfs:label "61125C" .


:TestMethod._62270AnnexA uml:id "_33BAA4B6-2E09-4c1a-9E55-39E21A7CD27F" ;
                         rdfs:comment "62270 Annex A method." ;
                         rdfs:label "62270AnnexA" .


:TestMethod._62535AnnexA uml:id "_4824E07B-F510-42a3-8657-A4D89ACB324E" ;
                         rdfs:comment "62535 Annex A method." ;
                         rdfs:label "62535AnnexA" .


:TestMethod._62535Main uml:id "_22753C2E-740A-4900-AD4A-16543E706A5D" ;
                       rdfs:comment "62535 main method." ;
                       rdfs:label "62535Main" .


:TestReason.postOilTreatment uml:id "_10758EB0-1E39-4d04-A5F9-2A537B1BB051" ;
                             rdfs:comment "Test after oil treatment." ;
                             rdfs:label "postOilTreatment" .


:TestReason.postOperationFault uml:id "_07435789-F631-42f7-B535-DBC56CB030C3" ;
                               rdfs:comment "Test after operation fault." ;
                               rdfs:label "postOperationFault" .


:TestReason.postRepair uml:id "_245106B8-8BB4-4d87-96DB-6B3312241910" ;
                       rdfs:comment "Test after repair." ;
                       rdfs:label "postRepair" .


:TestReason.routine uml:id "_81745C5B-8821-4382-9F02-5CF947360DA0" ;
                    rdfs:comment "Routine test." ;
                    rdfs:label "routine" .


:TestVariantKind._0C uml:id "_E55D9D27-FFC5-4a4f-9298-A9E13DCA5476" ;
                     rdfs:comment "Testing done at temperature of 0°C." ;
                     rdfs:label "0C" .


:TestVariantKind._100C uml:id "_E71C37D6-C2DF-42e8-92C3-D418946E91FF" ;
                       rdfs:comment "Testing done at temperature of  100°C." ;
                       rdfs:label "100C" .


:TestVariantKind._164hours uml:id "_82137C06-6409-4190-B360-A106F37ECCB3" ;
                           rdfs:comment "Measurements taken at 164 hours." ;
                           rdfs:label "164hours" .


:TestVariantKind._1mm uml:id "_38F63DD2-1DD1-4450-B29A-FDD5F3D9FB66" ;
                      rdfs:comment "Specimen of 1 mm thickness used in testing." ;
                      rdfs:label "1mm" .


:TestVariantKind._25C uml:id "_CF2513D1-6E62-4c1b-8564-A7CD30AAFE9C" ;
                      rdfs:comment "Testing done at temperature of  25°C." ;
                      rdfs:label "25C" .


:TestVariantKind._2mm uml:id "_8E5ED28F-123F-4fed-B828-1A1B8A5012DD" ;
                      rdfs:comment "Specimen of 2 mm thickness used in testing." ;
                      rdfs:label "2mm" .


:TestVariantKind._30C uml:id "_65AEAB95-EEDA-46d9-B797-2ECECB73CCF2" ;
                      rdfs:comment "Testing done at temperature of 30°C." ;
                      rdfs:label "30C" .


:TestVariantKind._40C uml:id "_32F7242A-1BC1-4d15-ACA3-06D2963DBFC5" ;
                      rdfs:comment "Testing done at temperature of 40°C." ;
                      rdfs:label "40C" .


:TestVariantKind._72hours uml:id "_A6F50234-20EB-4edd-A06D-AC80A73590A3" ;
                          rdfs:comment "Measurements taken at 72 hours." ;
                          rdfs:label "72hours" .


:TestVariantKind.minus30C uml:id "_0D56AD99-0AA6-4591-9204-29E419012920" ;
                          rdfs:comment "Testing done at temperature of -30°C." ;
                          rdfs:label "minus30C" .


:TestVariantKind.minus40C uml:id "_51F39982-607D-48df-890D-C08F4D08FD5A" ;
                          rdfs:comment "Testing done at temperature of -40°C." ;
                          rdfs:label "minus40C" .


:TimeIntervalKind.D uml:hasInitialValue "3" ;
                    uml:id "_C07A0BF9-11C9-4ed6-AE95-0A19DEA01D99" ;
                    rdfs:comment "Day" ;
                    rdfs:label "D" .


:TimeIntervalKind.M uml:hasInitialValue "2" ;
                    uml:id "_C94268B9-71F8-49fa-9D85-4985053F3E84" ;
                    rdfs:comment "Month" ;
                    rdfs:label "M" .


:TimeIntervalKind.Y uml:hasInitialValue "1" ;
                    uml:id "_9F43F113-B47E-459b-B0C8-3C751EFD3843" ;
                    rdfs:comment "Year" ;
                    rdfs:label "Y" .


:TimeIntervalKind.h uml:hasInitialValue "4" ;
                    uml:id "_A3361B00-3D72-4b97-B457-4292B65D6EA4" ;
                    rdfs:comment "Hour" ;
                    rdfs:label "h" .


:TimeIntervalKind.m uml:hasInitialValue "5" ;
                    uml:id "_3D949A55-3AA5-4498-A2AB-AA8974BAE280" ;
                    rdfs:comment "Minute" ;
                    rdfs:label "m" .


:TimeIntervalKind.s uml:hasInitialValue "6" ;
                    uml:id "_7457AF6C-8640-4c8a-85D2-87C11898044A" ;
                    rdfs:comment "Second" ;
                    rdfs:label "s" .


:TimeOfUse.OFF uml:id "_4D774394-42E4-4200-B3BF-CE893AA30688" ;
               rdfs:comment "Time of use spans only the off peak hours of the day." ;
               rdfs:label "OFF" .


:TimeOfUse.ON uml:id "_9C383024-9360-4804-A45D-096111963E57" ;
              rdfs:comment "Time of use spans only the on peak hours of the day." ;
              rdfs:label "ON" .


:TimeOfUse._24HR uml:id "_22E0AE7A-C07A-48fc-8A22-1B64249CE481" ;
                 rdfs:comment "Time of use spans the entire day, 24 hours." ;
                 rdfs:label "24HR" .


:TimePeriodUnit.days uml:id "_E320A2D6-5EBE-4a1f-900C-00C76137BDB9" ;
                     rdfs:label "days" .


:TimePeriodUnit.hours uml:id "_B2861A11-FEB4-407c-B915-234AA74C0AD6" ;
                      rdfs:label "hours" .


:TimePeriodUnit.minutes uml:id "_E7DAE93F-3B21-48f0-95CD-5D9F9B4D4F8E" ;
                        rdfs:label "minutes" .


:TimePeriodUnit.months uml:id "_B9CFEC0E-E1B2-4e83-9848-D5B44B094FC6" ;
                       rdfs:label "months" .


:TimePeriodUnit.seconds uml:id "_0917C0D7-DD4D-4afd-8187-88ABACE6EB58" ;
                        rdfs:label "seconds" .


:TimePeriodUnit.weeks uml:id "_10C5D223-B544-42dd-B5E4-11736234708A" ;
                      rdfs:label "weeks" .


:TimeZoneType.PPT uml:id "_7391CC41-8C1B-4a6d-9EB7-B87B9512810B" ;
                  rdfs:label "PPT" .


:TowerConstructionKind.suspension uml:id "_8E4C7375-37F8-4b4e-B708-6DDB1253A96E" ;
                                  rdfs:label "suspension" .


:TowerConstructionKind.tension uml:id "_8B89CFF7-DB29-4632-8D8D-32DEE264CAF5" ;
                               rdfs:label "tension" .


:TradeProductType.APN uml:id "_E0016452-D191-48bc-9533-899BD0465C96" ;
                      rdfs:comment "Energy Trades at Aggregated Pricing Nodes" ;
                      rdfs:label "APN" .


:TradeProductType.CAP uml:id "_EA2686A6-AFC4-4632-905D-8EBD9D35AF45" ;
                      rdfs:comment "Capacity type trade" ;
                      rdfs:label "CAP" .


:TradeProductType.NRT uml:id "_3CEA8060-928C-4907-A763-501F200601C5" ;
                      rdfs:comment "Non-Spinning Reserve Trade" ;
                      rdfs:label "NRT" .


:TradeProductType.PHY uml:id "_258939C5-EB12-492b-807B-16F435C2D04B" ;
                      rdfs:comment "Physical Energy Tra" ;
                      rdfs:label "PHY" .


:TradeProductType.RDT uml:id "_888EE4F7-0921-4bd7-87C2-6CB82D7D2C4F" ;
                      rdfs:comment "Regulation Down Trade" ;
                      rdfs:label "RDT" .


:TradeProductType.RUT uml:id "_75207216-0165-489e-B315-00821A960691" ;
                      rdfs:comment "Regulation Up Trade" ;
                      rdfs:label "RUT" .


:TradeProductType.SRT uml:id "_F6E55637-66CB-49f1-A2D0-1AEBCE3C8DBD" ;
                      rdfs:comment "Spinning Reserve Trade" ;
                      rdfs:label "SRT" .


:TradeStatusType.CI uml:id "_3C6AD60E-E234-49c6-A060-FF679E166E8D" ;
                    rdfs:label "CI" .


:TradeStatusType.CM uml:id "_3363021F-709F-40e5-8FF3-B6F9ABC5CA8A" ;
                    rdfs:label "CM" .


:TradeStatusType.CV uml:id "_B71C58A2-235F-4f87-91D5-21AE5F6B8D0B" ;
                    rdfs:label "CV" .


:TradeStatusType.CX uml:id "_488782A2-49FA-445f-897C-35A0201FD12E" ;
                    rdfs:label "CX" .


:TradeStatusType.I uml:id "_92C11A8D-1822-46f0-A1CE-41D33655A708" ;
                   rdfs:label "I" .


:TradeStatusType.M uml:id "_141B1E04-49F0-4c6b-A68C-C2BABB01ED46" ;
                   rdfs:label "M" .


:TradeStatusType.MT uml:id "_74A2ED7D-00E1-4fd3-8E59-9635836AE96C" ;
                    rdfs:label "MT" .


:TradeStatusType.O uml:id "_47172D34-3A20-4233-AE11-9FD6867B6FF2" ;
                   rdfs:label "O" .


:TradeStatusType.RJ uml:id "_E25FB5E6-02AD-42bc-8CA7-B8849DF94AC6" ;
                    rdfs:label "RJ" .


:TradeStatusType.U uml:id "_E55E1057-5AD9-48bd-8EF2-63A77B6BD400" ;
                   rdfs:label "U" .


:TradeStatusType.V uml:id "_4455793E-623A-43a4-91FC-A57FAF32C090" ;
                   rdfs:label "V" .


:TradeType.AST uml:id "_617D05A1-2FC0-48a6-97A2-FE2F739B51C1" ;
               rdfs:comment "Ancillary Services Trade." ;
               rdfs:label "AST" .


:TradeType.IST uml:id "_0B562154-C774-473e-B2DD-ACC435874123" ;
               rdfs:comment "InterSC Trade." ;
               rdfs:label "IST" .


:TradeType.UCT uml:id "_00C840ED-00F9-40e9-A0E5-4BF9537FF36E" ;
               rdfs:comment "Unit Commitment Trade." ;
               rdfs:label "UCT" .


:TransactionKind.accountPayment uml:id "_E46E5360-A240-44c6-9506-17B5AB2C2BD7" ;
                                rdfs:comment "Payment against a specified account." ;
                                rdfs:label "accountPayment" .


:TransactionKind.auxiliaryChargePayment uml:id "_56BAFDD2-5B84-4ddc-8FCF-D7683645C581" ;
                                        rdfs:comment "Payment against a specified auxiliary account." ;
                                        rdfs:label "auxiliaryChargePayment" .


:TransactionKind.diversePayment uml:id "_67D0C643-F379-4c17-BD45-019906C1D72B" ;
                                rdfs:comment "Payment against an item other than an account." ;
                                rdfs:label "diversePayment" .


:TransactionKind.meterConfigurationToken uml:id "_CD4C6814-8926-476e-A037-15FDED5C581C" ;
                                         rdfs:comment "Issue of token that will alter the meter configuration." ;
                                         rdfs:label "meterConfigurationToken" .


:TransactionKind.other uml:id "_8E8D6006-5874-4a2d-AC8C-F197B63D0DBB" ;
                       rdfs:comment "Other kind of transaction." ;
                       rdfs:label "other" .


:TransactionKind.serviceChargePayment uml:id "_43AB867F-0D25-4618-9DA4-C2160EA1E91B" ;
                                      rdfs:comment "Payment for a service." ;
                                      rdfs:label "serviceChargePayment" .


:TransactionKind.taxChargePayment uml:id "_E90820C2-6C5F-4298-85B8-50CEC8E1FA9A" ;
                                  rdfs:comment "Payment for a tax." ;
                                  rdfs:label "taxChargePayment" .


:TransactionKind.tokenCancellation uml:id "_17BBAC42-3DEA-4be8-8F76-B1B3DB949148" ;
                                   rdfs:comment "Cancellation of a previously issued token." ;
                                   rdfs:label "tokenCancellation" .


:TransactionKind.tokenExchange uml:id "_73447643-6838-42f8-A7C0-DA1304CA3849" ;
                               rdfs:comment "Exchange of a previously issued token for a new token." ;
                               rdfs:label "tokenExchange" .


:TransactionKind.tokenFreeIssue uml:id "_7B64DDBC-C5C1-4f70-8205-848406680782" ;
                                rdfs:comment "Issue of a free credit token where the donor is the supplier." ;
                                rdfs:label "tokenFreeIssue" .


:TransactionKind.tokenGrant uml:id "_C54424FD-76CD-46d5-AECA-CD4362203D45" ;
                            rdfs:comment "Issue of a free credit token where the donor is a 3rd party." ;
                            rdfs:label "tokenGrant" .


:TransactionKind.tokenSalePayment uml:id "_6612C594-2FC1-4191-AB6C-0E4AE2A7F0C4" ;
                                  rdfs:comment "Payment for a credit token sale to a customer." ;
                                  rdfs:label "tokenSalePayment" .


:TransactionKind.transactionReversal uml:id "_2F1128AE-DA20-495f-AF3D-DFA9ADF66DC7" ;
                                     rdfs:comment "Reversal of a previous transaction." ;
                                     rdfs:label "transactionReversal" .


:TransformerApplicationKind.distribution uml:id "_8090DA52-12AF-4704-8B78-1C9C27FF05BD" ;
                                         rdfs:comment "Transformer between one distribution voltage level and another distribution voltage level." ;
                                         rdfs:label "distribution" .


:TransformerApplicationKind.generatorStepUp uml:id "_EB14DC9F-8667-4a55-AC96-FC9938358957" ;
                                            rdfs:comment "Transformer is generator step-up transformer." ;
                                            rdfs:label "generatorStepUp" .


:TransformerApplicationKind.transmissionBusToBus uml:id "_BBC6C67F-344C-4383-921A-6EEF35829419" ;
                                                 rdfs:comment "Transformer between bus at one transmission voltage level and a bus at another transmission voltage level." ;
                                                 rdfs:label "transmissionBusToBus" .


:TransformerApplicationKind.transmissionBusToDistribution uml:id "_7C0EDE59-1CCE-40a8-B719-1CD26C6E88F9" ;
                                                          rdfs:comment "Transformer between bus at transmission voltage level and bus at distribution voltage level." ;
                                                          rdfs:label "transmissionBusToDistribution" .


:TransformerConstructionKind.aerial uml:id "_D2C5029A-F5D2-48f0-BB2A-1727B7355C48" ;
                                    rdfs:label "aerial" .


:TransformerConstructionKind.dryType uml:id "_0B432449-9CF3-4593-A288-C5A417FC42A4" ;
                                     rdfs:label "dryType" .


:TransformerConstructionKind.network uml:id "_B22AA9A7-A6F9-4af7-AE3D-8B99DDFB98CF" ;
                                     rdfs:label "network" .


:TransformerConstructionKind.onePhase uml:id "_F169D0F5-5688-46ef-903E-7E00DA9E3173" ;
                                      rdfs:label "onePhase" .


:TransformerConstructionKind.overhead uml:id "_14EAE77C-1B3D-4942-A790-937E3B84476B" ;
                                      rdfs:label "overhead" .


:TransformerConstructionKind.padmountDeadFront uml:id "_523B0CB7-F3B0-40ac-8E54-AEE9778ADF80" ;
                                               rdfs:label "padmountDeadFront" .


:TransformerConstructionKind.padmountFeedThrough uml:id "_8C883EBA-574B-4d3d-8F99-5414BE00EF05" ;
                                                 rdfs:label "padmountFeedThrough" .


:TransformerConstructionKind.padmountLiveFront uml:id "_93F3FBA1-BDF2-4c3d-896E-B685586D099A" ;
                                               rdfs:label "padmountLiveFront" .


:TransformerConstructionKind.padmountLoopThrough uml:id "_D08D952F-48BE-4bb3-A653-C126F2522159" ;
                                                 rdfs:label "padmountLoopThrough" .


:TransformerConstructionKind.padmounted uml:id "_ABA1CB94-11D4-4cda-A13A-48CC6EEE12A8" ;
                                        rdfs:label "padmounted" .


:TransformerConstructionKind.subway uml:id "_4E88151A-3B4E-48ee-B37C-5AF70E93A2C7" ;
                                    rdfs:label "subway" .


:TransformerConstructionKind.threePhase uml:id "_37602A9A-DE94-440d-AE2B-8F7D95D549F0" ;
                                        rdfs:label "threePhase" .


:TransformerConstructionKind.underground uml:id "_A3059163-9E99-465c-A229-C763EC1CC1E3" ;
                                         rdfs:label "underground" .


:TransformerConstructionKind.unknown uml:id "_31313C0D-A923-47e9-AD3A-B2756894C575" ;
                                     rdfs:label "unknown" .


:TransformerConstructionKind.vault uml:id "_286CCE7F-E091-4bca-A9B0-D44AE5BAABA0" ;
                                   rdfs:label "vault" .


:TransformerConstructionKind.vaultThreePhase uml:id "_30ECF0EE-7DC8-4e63-B662-18C4897C7C84" ;
                                             rdfs:label "vaultThreePhase" .


:TransformerControlMode.reactive uml:id "_91A7C3F0-A2E6-4199-9B38-5EF91B1046A2" ;
                                 rdfs:comment "Reactive power flow control." ;
                                 rdfs:label "reactive" .


:TransformerControlMode.volt uml:id "_21799345-8131-44e5-90A0-6BC1BB534ABB" ;
                             rdfs:comment "Voltage control." ;
                             rdfs:label "volt" .


:TransformerCoreKind.core uml:id "_42FE2CEF-3FD8-4acb-8119-388DCE5A4006" ;
                          rdfs:label "core" .


:TransformerCoreKind.shell uml:id "_7E11FABD-CB5B-458a-9672-19DE58380E32" ;
                           rdfs:label "shell" .


:TransformerFailureReasonKind.bushingFailure uml:id "_3C0B66F6-B1E4-4231-A28F-FE0889D2F1F9" ;
                                             rdfs:comment "Bushing-caused failure." ;
                                             rdfs:label "bushingFailure" .


:TransformerFailureReasonKind.lossOfOil uml:id "_07F9AAB4-837B-44bc-B5AF-0481683DDBF1" ;
                                        rdfs:comment "Loss-of-oil-caused faliure." ;
                                        rdfs:label "lossOfOil" .


:TransformerFailureReasonKind.oilRelatedFailure uml:id "_7C0960AB-9A72-4a19-9ED9-D819CA491449" ;
                                                rdfs:comment "Oil-related failure." ;
                                                rdfs:label "oilRelatedFailure" .


:TransformerFailureReasonKind.poorOilQuality uml:id "_BBE4F5CA-38F8-4ffc-94ED-722F1523F0FB" ;
                                             rdfs:comment "Oil quality-related failure." ;
                                             rdfs:label "poorOilQuality" .


:TransformerFunctionKind.autotransformer uml:id "_FAFF03FE-3C7E-4cbc-90D5-0A1F20019505" ;
                                         rdfs:label "autotransformer" .


:TransformerFunctionKind.other uml:id "_AE18D8C5-355E-4cc7-A9B4-738871F729D8" ;
                               rdfs:label "other" .


:TransformerFunctionKind.powerTransformer uml:id "_2CD73C03-A1CB-4d74-A4DC-0A244B976231" ;
                                          rdfs:label "powerTransformer" .


:TransformerFunctionKind.secondaryTransformer uml:id "_7F9626DB-A1BB-4699-A3B7-FD6E7558C511" ;
                                              rdfs:label "secondaryTransformer" .


:TransformerFunctionKind.voltageRegulator uml:id "_C5B3CFA5-5A87-4b57-A536-1712F28D9A38" ;
                                          rdfs:label "voltageRegulator" .


:TransmissionModeKind.anonymous uml:id "_A75D62A0-7361-4c54-BA1A-7D68EC07F0FE" ;
                                rdfs:comment "Message transmission mode whereby messages or commands are broadcast to unspecified devices listening for such communications." ;
                                rdfs:label "anonymous" .


:TransmissionModeKind.both uml:id "_EE4F3450-0583-4ebe-B83F-A61D8CC609D0" ;
                           rdfs:comment "Message transmission mode whereby messages or commands are sent by both 'normal' and 'anonymous' methods." ;
                           rdfs:label "both" .


:TransmissionModeKind.normal uml:id "_8B33CD7F-F151-408b-B147-B5E2C9992550" ;
                             rdfs:comment "Message transmission mode whereby messages or commands are sent to specific devices." ;
                             rdfs:label "normal" .


:TroubleCallKind.lineDown uml:id "_32CD8B40-0684-4476-96DB-EB25EA135D0E" ;
                          rdfs:comment "The customer is reporting a line down" ;
                          rdfs:label "lineDown" .


:TroubleCallKind.powerOut uml:id "_0D243793-6AEE-48af-A4A1-D51FFE6B9762" ;
                          rdfs:comment "The customer is reporting an outage." ;
                          rdfs:label "powerOut" .


:TroubleReportingKind.app uml:id "_7BDEBC96-952F-4217-929C-1D0A48DBDE7F" ;
                          rdfs:label "app" .


:TroubleReportingKind.call uml:id "_082F4DA0-389D-4879-8BE5-F7103D5DB45A" ,
                                  "_E3DBCDD0-C040-4bb7-983D-CF2171EE375B" ;
                           rdfs:comment "Trouble call received by customer service representative." ;
                           rdfs:label "call" .


:TroubleReportingKind.email uml:id "_6A4F782D-C145-4228-AD70-333E39C40D08" ,
                                   "_C447B6E0-5BA5-49ca-A32B-A836324D5D47" ;
                            rdfs:comment "Trouble reported by email." ;
                            rdfs:label "email" .


:TroubleReportingKind.ivr uml:id "_37E8A66F-9052-4249-AE73-F0EDBD9C666B" ,
                                 "_F6A3821F-1FCE-498b-87B0-E3AF4A38ADDC" ;
                          rdfs:comment "Trouble reported through interactive voice response system." ;
                          rdfs:label "ivr" .


:TroubleReportingKind.letter uml:id "_5A807F00-9C57-4678-A748-FEE2CF766BF5" ,
                                    "_9B7EFA04-525A-4c2b-BBC8-807696DD7EE8" ;
                             rdfs:comment "Trouble reported by letter." ;
                             rdfs:label "letter" .


:TroubleReportingKind.other uml:id "_0FF97738-C280-4c67-B858-256038633AFE" ,
                                   "_53E43CD9-13AE-455f-A787-ED4B7B81A9E0" ;
                            rdfs:comment "Trouble reported by other means." ;
                            rdfs:label "other" .


:TroubleReportingKind.sms uml:id "_25553065-9062-4928-AD9B-B04F57941CA3" ;
                          rdfs:label "sms" .


:TroubleReportingKind.web uml:id "_6542B437-313E-4ffe-BC9A-9BD3D1C395C7" ;
                          rdfs:label "web" .


:TroubleSymptomsExtentKind.entireNeighbourhood uml:id "_1E251DA6-2A65-4dd2-B1BB-87C78CD1B52D" ;
                                               rdfs:label "entireNeighbourhood" .


:TroubleSymptomsExtentKind.neighbour uml:id "_77A29F2A-3B4E-4645-93F7-8EEEA8FE8C2D" ;
                                     rdfs:label "neighbour" .


:TroubleSymptomsExtentKind.ok uml:id "_DD4DE93E-BDC7-4021-A07E-E624D47DFCD1" ;
                              rdfs:label "ok" .


:TroubleSymptomsExtentKind.other uml:id "_BD51C1AA-00E2-49ce-8C8E-A67DBBEAE6E4" ;
                                 rdfs:label "other" .


:TroubleSymptomsExtentKind.singleCustomer uml:id "_45D6E8F8-A71E-4db7-9855-7803E5FC8B89" ;
                                          rdfs:label "singleCustomer" .


:TroubleSymptomsLightKind.allOut uml:id "_40F774B3-AC87-45a1-A761-5E8D3049DCB0" ;
                                 rdfs:label "allOut" .


:TroubleSymptomsLightKind.dim uml:id "_80FF3D1E-D0B6-46bc-8B89-BA1D697AB89F" ;
                              rdfs:label "dim" .


:TroubleSymptomsLightKind.flickering uml:id "_C024E0F8-3B63-4736-8BD4-D2C06EB81ED4" ;
                                     rdfs:label "flickering" .


:TroubleSymptomsLightKind.ok uml:id "_FFF40B77-DCC6-4920-9FE2-7F1BD61C42ED" ;
                             rdfs:label "ok" .


:TroubleSymptomsLightKind.other uml:id "_09489AEE-FD6F-4f8d-8174-BC02BF3E1CC2" ;
                                rdfs:label "other" .


:TroubleSymptomsLightKind.partOut uml:id "_4AC0A0A1-FC9A-4eb7-9F29-368FC647ABD9" ;
                                  rdfs:label "partOut" .


:TroubleSymptomsPoleKind.down uml:id "_555E3CB3-A700-44c8-9364-BC82BF7A6F72" ;
                              rdfs:label "down" .


:TroubleSymptomsPoleKind.hit uml:id "_36C309B7-7C0A-43f2-9000-45D53C6BE4BB" ;
                             rdfs:label "hit" .


:TroubleSymptomsPoleKind.leaning uml:id "_BAA451B5-C7C6-4258-B70A-D24909D09E9F" ;
                                 rdfs:label "leaning" .


:TroubleSymptomsPoleKind.ok uml:id "_D1E7C169-F893-4b25-8AD4-2CE2587607C0" ;
                            rdfs:label "ok" .


:TroubleSymptomsPoleKind.other uml:id "_11E9CFE2-7E9F-41b2-8202-EBCEC4530535" ;
                               rdfs:label "other" .


:TroubleSymptomsTransformerKind.burning uml:id "_4079A2A5-B8CA-43e0-B7FB-F510DD61E47C" ;
                                        rdfs:label "burning" .


:TroubleSymptomsTransformerKind.ok uml:id "_33FADF23-1213-4292-888B-0FB2BBAC5D18" ;
                                   rdfs:label "ok" .


:TroubleSymptomsTransformerKind.other uml:id "_ACD4467B-5260-4951-BD8C-9678D49CBAC5" ;
                                      rdfs:label "other" .


:TroubleSymptomsTree_Kind.limbOnService uml:id "_5516AA43-AD05-426e-A676-EC4D9CEB8C43" ;
                                        rdfs:label "limbOnService" .


:TroubleSymptomsTree_Kind.limbOnWire uml:id "_2D16AF9F-5DCC-47e2-B39A-6D52634D716C" ;
                                     rdfs:label "limbOnWire" .


:TroubleSymptomsTree_Kind.ok uml:id "_13FF5F78-8ED2-4108-8614-1D844A4C9184" ;
                             rdfs:label "ok" .


:TroubleSymptomsTree_Kind.other uml:id "_170371EF-B171-4cbd-B8DA-0351DFABE3AF" ;
                                rdfs:label "other" .


:TroubleSymptomsWireKind.digIn uml:id "_B25B33B8-0F35-4c52-B191-3F5131A3965E" ;
                               rdfs:label "digIn" .


:TroubleSymptomsWireKind.ok uml:id "_8D54DEF1-92B2-4c17-86B8-808AE1340DE2" ;
                            rdfs:label "ok" .


:TroubleSymptomsWireKind.other uml:id "_2E54A7DC-91BB-44cb-B9D9-B81BB48FEFBB" ;
                               rdfs:label "other" .


:TroubleSymptomsWireKind.serviceDown uml:id "_974750DB-D3BF-4cd6-943B-25873021AAB1" ;
                                     rdfs:label "serviceDown" .


:TroubleSymptomsWireKind.wireDown uml:id "_1228FDCA-A26C-4c45-B33F-DDA861371A91" ;
                                  rdfs:label "wireDown" .


:TroubleSymptomsWireKind.wireburning uml:id "_1EC52552-1D06-4ef2-9C14-8EB331A9B734" ;
                                     rdfs:label "wireburning" .


:UKMinistryOfDefenceStandardEditionKind.Issue_1 uml:id "_41908510-563A-4b57-9DF0-70D5DD632615" ;
                                                rdfs:comment "Issue 1 standard edition." ;
                                                rdfs:label "Issue 1" .


:UKMinistryOfDefenceStandardEditionKind.none uml:id "_6513F6BD-BE4F-476e-B757-32FB3A212825" ;
                                             rdfs:comment "No standard edition." ;
                                             rdfs:label "none" .


:UKMinistryOfDefenceStandardEditionKind.unknown uml:id "_94D658C2-8AD2-4c0b-8B07-B3BA329F5160" ;
                                                rdfs:comment "Unknown standard edition." ;
                                                rdfs:label "unknown" .


:UKMinistryofDefenceStandardKind._05-50__Part_65_ uml:id "_FAEFFDEB-AFE9-49a8-B9D4-B1F97AA6CB42" ;
                                                  rdfs:comment "Ministry of Defence, Defence Standard 05-50 (Part 65)/Issue 1 METHODS FOR TESTING FUELS, LUBRICANTS AND ASSOCIATED PRODUCTS." ;
                                                  rdfs:label "05-50 (Part 65)" .


:UOMType.FACTOR uml:id "_6A3BAC50-47DF-4eea-A4AB-12983425D0D8" ;
                rdfs:label "FACTOR" .


:UOMType.FLAG uml:id "_A0321D15-6C47-4fe1-AF34-E53C8C5CDA78" ;
              rdfs:label "FLAG" .


:UOMType.INTEGER uml:id "_2AAAB5CD-C589-4762-B435-BEC5EB398623" ;
                 rdfs:label "INTEGER" .


:UOMType.MW uml:id "_F17AA320-EF72-4b9a-AF9C-CB71DCFE1CA8" ;
            rdfs:label "MW" .


:UOMType.MWh uml:id "_F3876877-FCF6-4b60-BD26-1E30FC168250" ;
             rdfs:label "MWh" .


:UOMType.US_ uml:id "_54A6B44F-1629-4b9b-99AE-00A11BAD2A8E" ;
             rdfs:label "US$" .


:UOMType.US__MW uml:id "_911183F5-E1A7-4550-961C-E35A7CFC2053" ;
                rdfs:label "US$/MW" .


:UOMType.US__MWh uml:id "_02CDE6BC-CF46-4cb4-B62B-492A4CC4BC48" ;
                 rdfs:label "US$/MWh" .


:UOMType._ uml:id "_D63881DE-E79A-4c3c-BC21-F4C08FC5DD68" ;
           rdfs:label "%" .


:UOMType.__lb uml:id "_208BE661-4C4A-4f07-A89C-6EFB5E779134" ;
              rdfs:label "$/lb" .


:UOMType.__mmBTU uml:id "_53AD8C77-7160-4df3-9B85-4DDA4B1EDEBB" ;
                 rdfs:label "$/mmBTU" .


:UncertaintyKind.estimated uml:id "_C7AF5086-A42A-49ac-8765-7D59D8AF24D3" ;
                           rdfs:comment "The value is estimated." ;
                           rdfs:label "estimated" .


:UncertaintyKind.interpolated uml:id "_404AC095-654C-4202-B423-6E2C5B9EBD73" ;
                              rdfs:comment "The value is interpolated." ;
                              rdfs:label "interpolated" .


:UncertaintyKind.standard uml:id "_2F92A1B0-9D8D-44eb-A8F1-783B801E6B8D" ;
                          rdfs:comment "The value has standard uncertainty consistent with National Weather Service practises given the instrument and manner of observation." ;
                          rdfs:label "standard" .


:UncertaintyKind.unknown uml:id "_AEEB8600-47CB-482d-8718-3D3915667785" ;
                         rdfs:comment "The process of value calculation or measurement is unknown." ;
                         rdfs:label "unknown" .


:UndergroundStructureKind.burd uml:id "_ECBA1B04-6EDD-4378-87A9-489A2CC4D3F0" ;
                               rdfs:label "burd" .


:UndergroundStructureKind.enclosure uml:id "_549FB75A-0B49-4ff6-8442-D4D61BCCFAF4" ;
                                    rdfs:label "enclosure" .


:UndergroundStructureKind.handhole uml:id "_4E93AE2D-33DE-4d9a-8ED5-265823380E2C" ;
                                   rdfs:label "handhole" .


:UndergroundStructureKind.manhole uml:id "_C0C69252-1324-4966-8D72-7ADD56391659" ;
                                  rdfs:label "manhole" .


:UndergroundStructureKind.pad uml:id "_406ACAD2-B752-44d7-8811-96D5EAD8B930" ;
                              rdfs:label "pad" .


:UndergroundStructureKind.pullbox uml:id "_8EF36903-EDD0-4b3c-8B09-099AF5E71C24" ;
                                  rdfs:label "pullbox" .


:UndergroundStructureKind.subsurfaceEnclosure uml:id "_D5411441-F0C0-4827-A3AE-8F3D3610864D" ;
                                              rdfs:label "subsurfaceEnclosure" .


:UndergroundStructureKind.trench uml:id "_B4F6415B-86B3-482b-8A5D-905EA1E819AC" ;
                                 rdfs:label "trench" .


:UndergroundStructureKind.tunnel uml:id "_40653B9F-85A4-4b97-9731-914F0B76E155" ;
                                 rdfs:label "tunnel" .


:UndergroundStructureKind.vault uml:id "_EDA87E74-1A2E-41c4-88DB-F4027DD6D998" ;
                                rdfs:label "vault" .


:UnitMultiplier.E uml:hasInitialValue "18" ;
                  uml:id "_EADD578E-ADB6-4afc-989D-DCF868A74262" ;
                  rdfs:comment "Exa 10**18." ;
                  rdfs:label "E" .


:UnitMultiplier.G uml:hasInitialValue "9" ;
                  uml:id "_351B5D79-6203-48e5-9D9E-ECD7FB7CA8A6" ;
                  rdfs:comment "Giga 10**9." ;
                  rdfs:label "G" .


:UnitMultiplier.M uml:hasInitialValue "6" ;
                  uml:id "_F956FDD6-8C6E-427d-A51A-22A1D75BE1C3" ;
                  rdfs:comment "Mega 10**6." ;
                  rdfs:label "M" .


:UnitMultiplier.P uml:hasInitialValue "15" ;
                  uml:id "_F9AB8FD6-E2CB-4696-BDCE-16836A065FD4" ;
                  rdfs:comment "Peta 10**15." ;
                  rdfs:label "P" .


:UnitMultiplier.T uml:hasInitialValue "12" ;
                  uml:id "_F5185FB9-24E6-47c6-BB4D-259FDF678329" ;
                  rdfs:comment "Tera 10**12." ;
                  rdfs:label "T" .


:UnitMultiplier.Y uml:hasInitialValue "24" ;
                  uml:id "_B128FAC5-FF4E-48ae-BE52-0FF516C25214" ;
                  rdfs:comment "Yotta 10**24." ;
                  rdfs:label "Y" .


:UnitMultiplier.Z uml:hasInitialValue "21" ;
                  uml:id "_FCD1EF70-ACFA-4653-AEC4-086E460EA46C" ;
                  rdfs:comment "Zetta 10**21." ;
                  rdfs:label "Z" .


:UnitMultiplier.a uml:hasInitialValue "-18" ;
                  uml:id "_BBFD0505-6323-496c-95F7-818D6498EA5A" ;
                  rdfs:comment "Atto 10**-18." ;
                  rdfs:label "a" .


:UnitMultiplier.c uml:hasInitialValue "-2" ;
                  uml:id "_1219082C-9AED-439c-B862-8CA874195BA0" ;
                  rdfs:comment "Centi 10**-2." ;
                  rdfs:label "c" .


:UnitMultiplier.d uml:hasInitialValue "-1" ;
                  uml:id "_4E630955-DF5D-403d-A377-7ED5FF85978D" ;
                  rdfs:comment "Deci 10**-1." ;
                  rdfs:label "d" .


:UnitMultiplier.da uml:hasInitialValue "1" ;
                   uml:id "_EF522AAA-193D-4781-BDBD-4817C84E8558" ;
                   rdfs:comment "Deca 10**1." ;
                   rdfs:label "da" .


:UnitMultiplier.f uml:hasInitialValue "-15" ;
                  uml:id "_099282D3-03AC-4193-AB3D-71ABF7D63497" ;
                  rdfs:comment "Femto 10**-15." ;
                  rdfs:label "f" .


:UnitMultiplier.h uml:hasInitialValue "2" ;
                  uml:id "_A5B3106F-3B4E-4e44-A883-09DAE8804156" ;
                  rdfs:comment "Hecto 10**2." ;
                  rdfs:label "h" .


:UnitMultiplier.k uml:hasInitialValue "3" ;
                  uml:id "_C868627C-3B72-4bc8-879D-E177E9059A22" ;
                  rdfs:comment "Kilo 10**3." ;
                  rdfs:label "k" .


:UnitMultiplier.m uml:hasInitialValue "-3" ;
                  uml:id "_E7A60C22-3D12-49c5-8F18-870B1A39A1AA" ;
                  rdfs:comment "Milli 10**-3." ;
                  rdfs:label "m" .


:UnitMultiplier.micro uml:hasInitialValue "-6" ;
                      uml:id "_FF8E9CD6-A459-47ab-A71E-E69857742CE1" ;
                      rdfs:comment "Micro 10**-6." ;
                      rdfs:label "micro" .


:UnitMultiplier.n uml:hasInitialValue "-9" ;
                  uml:id "_EA61DA27-05DF-41c7-B459-F1194928062C" ;
                  rdfs:comment "Nano 10**-9." ;
                  rdfs:label "n" .


:UnitMultiplier.none uml:hasInitialValue "0" ;
                     uml:id "_C352D73C-B9DC-4e7d-B1DB-5BE6D4BAE868" ;
                     rdfs:comment "No multiplier or equivalently multiply by 1." ;
                     rdfs:label "none" .


:UnitMultiplier.p uml:hasInitialValue "-12" ;
                  uml:id "_90F83546-DD55-4cf8-9E01-DD8F69D74A8D" ;
                  rdfs:comment "Pico 10**-12." ;
                  rdfs:label "p" .


:UnitMultiplier.y uml:hasInitialValue "-24" ;
                  uml:id "_9AC37B70-6AC3-46ed-B408-8C4885FE483B" ;
                  rdfs:comment "Yocto 10**-24." ;
                  rdfs:label "y" .


:UnitMultiplier.z uml:hasInitialValue "-21" ;
                  uml:id "_78644DE9-99FB-4811-B5D9-B23A0DB2728D" ;
                  rdfs:comment "Zepto 10**-21." ;
                  rdfs:label "z" .


:UnitRegulationKind._0 uml:id "_F851FDDA-449A-44ee-B750-95A0DDE3AB91" ;
                       rdfs:comment "Unit is not on regulation." ;
                       rdfs:label "0" .


:UnitRegulationKind._1 uml:id "_A1950399-0868-43c3-959F-002E636C73EE" ;
                       rdfs:comment "Unit is on AGC and regulating." ;
                       rdfs:label "1" .


:UnitRegulationKind._2 uml:id "_512DC8F9-859C-4f12-AD97-2BDC6AE2110D" ;
                       rdfs:comment "Unit is suppose to be on regulation but it is not under regulation now." ;
                       rdfs:label "2" .


:UnitSymbol.A uml:hasInitialValue "5" ;
              uml:id "_EA92BC2E-3B95-470e-A50B-8BB500136F86" ;
              rdfs:comment "Current in amperes." ;
              rdfs:label "A" .


:UnitSymbol.A2 uml:hasInitialValue "69" ;
               uml:id "_D45ED57B-D0FD-4496-A516-CD82E8DCD2C0" ;
               rdfs:comment "Amperes squared (A²)." ;
               rdfs:label "A2" .


:UnitSymbol.A2h uml:hasInitialValue "105" ;
                uml:id "_0A2E81E6-2C43-43dd-A6CB-8915611FB6F2" ;
                rdfs:comment "Ampere-squared hour, ampere-squared hour." ;
                rdfs:label "A2h" .


:UnitSymbol.A2s uml:hasInitialValue "70" ;
                uml:id "_856A3A12-D5A5-4d1c-AC5F-2C618DE8BDB7" ;
                rdfs:comment "Ampere squared time in square amperes (A²s)." ;
                rdfs:label "A2s" .


:UnitSymbol.APerA uml:hasInitialValue "152" ;
                  uml:id "_84D9395E-1931-48aa-974A-43B3C1895E8F" ;
                  rdfs:comment "Current, ratio of amperages.   Note: Users may need to supply a prefix such as ‘m’ to show rates such as ‘mA/A’." ;
                  rdfs:label "APerA" .


:UnitSymbol.APerm uml:hasInitialValue "103" ;
                  uml:id "_27499686-8D79-40b7-9E0E-44D9212938E7" ;
                  rdfs:comment "A/m, magnetic field strength, amperes per metre." ;
                  rdfs:label "APerm" .


:UnitSymbol.Ah uml:hasInitialValue "106" ;
               uml:id "_4E2BC900-EA78-4b89-9479-A12680EC133B" ;
               rdfs:comment "Ampere-hours, ampere-hours." ;
               rdfs:label "Ah" .


:UnitSymbol.As uml:hasInitialValue "68" ;
               uml:id "_3FBD0254-1CEA-4fd9-9A11-EA68D8AD96D2" ;
               rdfs:comment "Ampere seconds (A·s)." ;
               rdfs:label "As" .


:UnitSymbol.Bq uml:hasInitialValue "22" ;
               uml:id "_6A58DADF-F9D2-4be4-BA67-51992495709D" ;
               rdfs:comment "Radioactivity in becquerels (1/s)." ;
               rdfs:label "Bq" .


:UnitSymbol.Btu uml:hasInitialValue "132" ;
                uml:id "_2C7C1B15-F2F1-463e-926B-90C565D92696" ;
                rdfs:comment "Energy, British Thermal Units." ;
                rdfs:label "Btu" .


:UnitSymbol.C uml:hasInitialValue "26" ;
              uml:id "_EC257654-B700-4c74-A3E0-FA2B685C13D5" ;
              rdfs:comment "Electric charge in coulombs (A·s)." ;
              rdfs:label "C" .


:UnitSymbol.CPerkg uml:hasInitialValue "189" ;
                   uml:id "_16EEBE18-1F4A-433c-AEDB-8542AAC26A6A" ;
                   rdfs:comment "Exposure (x rays), coulombs per kilogram." ;
                   rdfs:label "CPerkg" .


:UnitSymbol.CPerm2 uml:hasInitialValue "184" ;
                   uml:id "_78F3FB2B-9D65-4d98-BE54-D640D628ABB5" ;
                   rdfs:comment "Surface charge density, coulombs per square metre." ;
                   rdfs:label "CPerm2" .


:UnitSymbol.CPerm3 uml:hasInitialValue "183" ;
                   uml:id "_C372C81F-C15D-42a4-8CD7-42D8F243F69F" ;
                   rdfs:comment "Electric charge density, coulombs per cubic metre." ;
                   rdfs:label "CPerm3" .


:UnitSymbol.F uml:hasInitialValue "25" ;
              uml:id "_9D72A1D6-75D9-4e00-B3B4-42D7DD0990FE" ;
              rdfs:comment "Electric capacitance in farads (C/V)." ;
              rdfs:label "F" .


:UnitSymbol.FPerm uml:hasInitialValue "185" ;
                  uml:id "_EBCAD9B1-5855-460c-BE72-4577117C7A0B" ;
                  rdfs:comment "Permittivity, farads per metre." ;
                  rdfs:label "FPerm" .


:UnitSymbol.G uml:hasInitialValue "277" ;
              uml:id "_AD411764-B9AE-4720-B402-AE5C70F66A92" ;
              rdfs:comment "Magnetic flux density, gausses (1 G = 10-4 T)." ;
              rdfs:label "G" .


:UnitSymbol.Gy uml:hasInitialValue "21" ;
               uml:id "_60C8424D-7177-444c-BEF0-8E6AC1D1077B" ;
               rdfs:comment "Absorbed dose in grays (J/kg)." ;
               rdfs:label "Gy" .


:UnitSymbol.GyPers uml:hasInitialValue "190" ;
                   uml:id "_6C97FDC2-E63A-40ee-AF9E-361A9E4ADC3D" ;
                   rdfs:comment "Absorbed dose rate, grays per second." ;
                   rdfs:label "GyPers" .


:UnitSymbol.H uml:hasInitialValue "28" ;
              uml:id "_AE11FF61-9894-434b-AF7E-E30B3D6A4124" ;
              rdfs:comment "Electric inductance in henrys (Wb/A)." ;
              rdfs:label "H" .


:UnitSymbol.HPerm uml:hasInitialValue "186" ;
                  uml:id "_6CF0793D-A3E0-4f8f-863F-9C1032665065" ;
                  rdfs:comment "Permeability, henrys per metre." ;
                  rdfs:label "HPerm" .


:UnitSymbol.Hz uml:hasInitialValue "33" ;
               uml:id "_8E14F483-DBE2-46c3-9308-1DF800CD2FF2" ;
               rdfs:comment "Frequency in hertz (1/s)." ;
               rdfs:label "Hz" .


:UnitSymbol.HzPerHz uml:hasInitialValue "150" ;
                    uml:id "_12B11EAF-4BB5-4d5c-A2BB-D78A02327104" ;
                    rdfs:comment "Frequency, rate of frequency change.   Note: Users may need to supply a prefix such as ‘m’ to show rates such as ‘mHz/Hz’." ;
                    rdfs:label "HzPerHz" .


:UnitSymbol.HzPers uml:hasInitialValue "75" ;
                   uml:id "_98C8F3E1-139E-482e-8C78-EF21E8A15A38" ;
                   rdfs:comment "Rate of change of frequency in hertz per second." ;
                   rdfs:label "HzPers" .


:UnitSymbol.J uml:hasInitialValue "31" ;
              uml:id "_97A3FB98-8A5D-4b95-8473-5D3EDE289822" ;
              rdfs:comment "Energy in joules (N·m = C·V = W·s)." ;
              rdfs:label "J" .


:UnitSymbol.JPerK uml:hasInitialValue "51" ;
                  uml:id "_0A532BE2-CF36-4726-A14D-1EC97FD37B6D" ;
                  rdfs:comment "Heat capacity in joules/kelvin." ;
                  rdfs:label "JPerK" .


:UnitSymbol.JPerkg uml:hasInitialValue "165" ;
                   uml:id "_05214191-21C9-4b98-A8E5-CD63EAD7FB35" ;
                   rdfs:comment "Specific energy, Joules / kg." ;
                   rdfs:label "JPerkg" .


:UnitSymbol.JPerkgK uml:hasInitialValue "60" ;
                    uml:id "_5C1D5E18-724F-4348-A871-610428006C41" ;
                    rdfs:comment "Specific heat capacity, specific entropy, joules per kilogram Kelvin." ;
                    rdfs:label "JPerkgK" .


:UnitSymbol.JPerm2 uml:hasInitialValue "56" ;
                   uml:id "_1484901D-B114-4df8-8FBD-892ED2DDC36D" ;
                   rdfs:comment "Insulation energy density, joules per square metre or watt second per square metre." ;
                   rdfs:label "JPerm2" .


:UnitSymbol.JPerm3 uml:hasInitialValue "181" ;
                   uml:id "_643ABAE5-C491-445d-B0DA-FDD3381A7871" ;
                   rdfs:comment "Energy density, joules per cubic metre." ;
                   rdfs:label "JPerm3" .


:UnitSymbol.JPermol uml:hasInitialValue "187" ;
                    uml:id "_082C9B4F-A2B0-48b3-A976-4551C7B0B9D5" ;
                    rdfs:comment "Molar energy, joules per mole." ;
                    rdfs:label "JPermol" .


:UnitSymbol.JPermolK uml:hasInitialValue "188" ;
                     uml:id "_C86FC880-4592-4126-ACD6-C0CFE6151C19" ;
                     rdfs:comment "Molar entropy, molar heat capacity, joules per mole kelvin." ;
                     rdfs:label "JPermolK" .


:UnitSymbol.JPers uml:id "_8D0EFD06-CE71-454a-AF72-A37FF1988C0E" ;
                  rdfs:comment "Energy rate in joules per second (J/s)." ;
                  rdfs:label "JPers" .


:UnitSymbol.K uml:hasInitialValue "6" ;
              uml:id "_1E8C279F-B121-451f-B8D7-7B9F1EF080DF" ;
              rdfs:comment "Temperature in kelvins." ;
              rdfs:label "K" .


:UnitSymbol.KPers uml:hasInitialValue "58" ;
                  uml:id "_4AA28097-6E2C-4e6f-A7DE-F0813968DFAE" ;
                  rdfs:comment "Temperature change rate in kelvins per second." ;
                  rdfs:label "KPers" .


:UnitSymbol.M uml:hasInitialValue "217" ;
              uml:id "_95D59B4E-F7D2-4202-AEE3-BBE1602128E2" ;
              rdfs:comment "Length, nautical miles (1 M = 1852 m)." ;
              rdfs:label "M" .


:UnitSymbol.Mx uml:hasInitialValue "276" ;
               uml:id "_9D86ACE7-4F18-419a-B862-85D2D7165A51" ;
               rdfs:comment "Magnetic flux, maxwells (1 Mx = 10-8 Wb)." ;
               rdfs:label "Mx" .


:UnitSymbol.N uml:hasInitialValue "32" ;
              uml:id "_68AA121A-1847-446b-A6B2-F7180AC83772" ;
              rdfs:comment "Force in newtons (kg·m/s²)." ;
              rdfs:label "N" .


:UnitSymbol.NPerm uml:hasInitialValue "177" ;
                  uml:id "_05284484-23B5-4903-9FD7-2E7CF0E166B5" ;
                  rdfs:comment "Surface tension, newton per metre." ;
                  rdfs:label "NPerm" .


:UnitSymbol.Nm uml:hasInitialValue "176" ;
               uml:id "_62F46160-46EA-47c2-9E8D-DC44F5BCFEA7" ;
               rdfs:comment "Moment of force, newton metres." ;
               rdfs:label "Nm" .


:UnitSymbol.Oe uml:hasInitialValue "278" ;
               uml:id "_79B7C736-028D-4eab-9A0D-DEE3E6A963F8" ;
               rdfs:comment "Magnetic field in oersteds, (1 Oe = (103/4p) A/m)." ;
               rdfs:label "Oe" .


:UnitSymbol.Pa uml:hasInitialValue "39" ;
               uml:id "_BD782A7D-D539-4f4f-BAAF-44DFDC18CE40" ;
               rdfs:comment "Pressure in pascals (N/m²). Note: the absolute or relative measurement of pressure is implied with this entry. See below for more explicit forms." ;
               rdfs:label "Pa" .


:UnitSymbol.PaPers uml:hasInitialValue "59" ;
                   uml:id "_468B93E2-D504-4668-B698-6C438CC555FF" ;
                   rdfs:comment "Pressure change rate in pascals per second." ;
                   rdfs:label "PaPers" .


:UnitSymbol.Pas uml:hasInitialValue "175" ;
                uml:id "_2B45021A-F7A2-4f33-B105-918CA01B627D" ;
                rdfs:comment "Dynamic viscosity, pascal seconds." ;
                rdfs:label "Pas" .


:UnitSymbol.Q uml:hasInitialValue "100" ;
              uml:id "_67586835-9551-42fb-ABF8-3F4CFA5032F2" ;
              rdfs:comment "Quantity power, Q." ;
              rdfs:label "Q" .


:UnitSymbol.Qh uml:hasInitialValue "101" ;
               uml:id "_8908E051-4BDB-42f6-A2FB-126358F6952F" ;
               rdfs:comment "Quantity energy, Qh." ;
               rdfs:label "Qh" .


:UnitSymbol.S uml:hasInitialValue "27" ;
              uml:id "_C593555B-266C-4ac6-8F80-E91F045DFA89" ;
              rdfs:comment "Conductance in siemens." ;
              rdfs:label "S" .


:UnitSymbol.SPerm uml:hasInitialValue "57" ;
                  uml:id "_A1442E6B-3261-4ae2-B466-2788281713C6" ;
                  rdfs:comment "Conductance per length (F/m)." ;
                  rdfs:label "SPerm" .


:UnitSymbol.Sv uml:hasInitialValue "24" ;
               uml:id "_C408842C-136F-455f-B998-6A661EEA20AF" ;
               rdfs:comment "Dose equivalent in sieverts (J/kg)." ;
               rdfs:label "Sv" .


:UnitSymbol.T uml:hasInitialValue "37" ;
              uml:id "_12E9D418-34B0-4978-8012-CEBBB3154B37" ;
              rdfs:comment "Magnetic flux density in teslas (Wb/m2)." ;
              rdfs:label "T" .


:UnitSymbol.V uml:hasInitialValue "29" ;
              uml:id "_0A273035-181C-482c-9526-6673DE4AF59F" ;
              rdfs:comment "Electric potential in volts (W/A)." ;
              rdfs:label "V" .


:UnitSymbol.V2 uml:hasInitialValue "67" ;
               uml:id "_BADD342F-47DF-44a9-A9A2-C2923A48DBAB" ;
               rdfs:comment "Volt squared (W²/A²)." ;
               rdfs:label "V2" .


:UnitSymbol.V2h uml:hasInitialValue "104" ;
                uml:id "_AC926E85-C4E0-4512-84B1-8DFEC4D0C8E5" ;
                rdfs:comment "Volt-squared hour, volt-squared-hours." ;
                rdfs:label "V2h" .


:UnitSymbol.VA uml:hasInitialValue "61" ;
               uml:id "_D3EB929D-C57F-40a8-86DC-2F5CAACB6A71" ;
               rdfs:comment "Apparent power in volt amperes. See also real power and reactive power." ;
               rdfs:label "VA" .


:UnitSymbol.VAh uml:hasInitialValue "71" ;
                uml:id "_B65C6290-E53E-4bee-B674-A2E166EB4D77" ;
                rdfs:comment "Apparent energy in volt ampere hours." ;
                rdfs:label "VAh" .


:UnitSymbol.VAr uml:hasInitialValue "63" ;
                uml:id "_F38DF57D-7E97-4af9-984E-40820470C5EC" ;
                rdfs:comment """Reactive power in volt amperes reactive. The “reactive” or “imaginary” component of electrical power (VIsin(phi)). (See also real power and apparent power).
Note: Different meter designs use different methods to arrive at their results. Some meters may compute reactive power as an arithmetic value, while others compute the value vectorially. The data consumer should determine the method in use and the suitability of the measurement for the intended purpose.""" ;
                rdfs:label "VAr" .


:UnitSymbol.VArh uml:hasInitialValue "73" ;
                 uml:id "_DD5193A4-8564-4426-8FA1-98F3A50327FA" ;
                 rdfs:comment "Reactive energy in volt ampere reactive hours." ;
                 rdfs:label "VArh" .


:UnitSymbol.VPerHz uml:hasInitialValue "74" ;
                   uml:id "_18DE9C0C-CE23-4b20-8779-CEEB07E6BD9E" ;
                   rdfs:comment "Magnetic flux in volt per hertz." ;
                   rdfs:label "VPerHz" .


:UnitSymbol.VPerV uml:hasInitialValue "151" ;
                  uml:id "_E32A4356-EE83-4a56-A630-882387CC00C8" ;
                  rdfs:comment "Voltage, ratio of voltages.  Note: Users may need to supply a prefix such as ‘m’ to show rates such as ‘mV/V’." ;
                  rdfs:label "VPerV" .


:UnitSymbol.VPerVA uml:hasInitialValue "153" ;
                   uml:id "_F5914562-B809-455b-98A8-CECAA59EE125" ;
                   rdfs:comment "Power factor, PF, the ratio of the active power to the apparent power.  Note: The sign convention used for power factor will differ between IEC meters and EEI (ANSI) meters. It is assumed that the data consumers understand the type of meter being used and agree on the sign convention in use at any given utility." ;
                   rdfs:label "VPerVA" .


:UnitSymbol.VPerVAr uml:id "_F205CACD-712B-46f0-B7D7-170EEF3B59A3" ;
                    rdfs:comment "Power factor, PF, the ratio of the active power to the apparent power. Note: The sign convention used for power factor will differ between IEC meters and EEI (ANSI) meters. It is assumed that the data consumers understand the type of meter being used and agree on the sign convention in use at any given utility." ;
                    rdfs:label "VPerVAr" .


:UnitSymbol.VPerm uml:hasInitialValue "182" ;
                  uml:id "_72E72CF2-2E55-4c96-B72F-D2D0C602ED65" ;
                  rdfs:comment "Electric field strength, volts per metre." ;
                  rdfs:label "VPerm" .


:UnitSymbol.Vh uml:hasInitialValue "280" ;
               uml:id "_133A1DDB-6E5C-4edc-8788-0FEADD99F7AF" ;
               rdfs:comment "Volt-hour, Volt hours." ;
               rdfs:label "Vh" .


:UnitSymbol.Vs uml:hasInitialValue "66" ;
               uml:id "_4ADBB794-4439-4590-B83E-30CC81BB588F" ;
               rdfs:comment "Volt seconds (Ws/A)." ;
               rdfs:label "Vs" .


:UnitSymbol.W uml:hasInitialValue "38" ;
              uml:id "_41B0F1BC-E69B-4ca1-A565-ECBC27B49095" ;
              rdfs:comment "Real power in watts (J/s). Electrical power may have real and reactive components. The real portion of electrical power (I&#178;R or VIcos(phi)), is expressed in Watts. See also apparent power and reactive power." ;
              rdfs:label "W" .


:UnitSymbol.WPerA uml:id "_BD554F27-BD42-42e8-A102-327C8B95F611" ;
                  rdfs:comment "Active power per current flow, watts per Ampere." ;
                  rdfs:label "WPerA" .


:UnitSymbol.WPerW uml:hasInitialValue "168" ;
                  uml:id "_07C055AF-FF95-4a33-AFA4-CC2E9E87038C" ;
                  rdfs:comment "Signal Strength, ratio of power.   Note: Users may need to supply a prefix such as ‘m’ to show rates such as ‘mW/W’." ;
                  rdfs:label "WPerW" .


:UnitSymbol.WPerm2 uml:hasInitialValue "55" ;
                   uml:id "_74F16DEB-1187-4180-82E7-C9730606F991" ;
                   rdfs:comment "Heat flux density, irradiance, watts per square metre." ;
                   rdfs:label "WPerm2" .


:UnitSymbol.WPerm2sr uml:hasInitialValue "192" ;
                     uml:id "_09253D8A-34A7-49be-88AF-87147A5EAB64" ;
                     rdfs:comment "Radiance, watts per square metre steradian." ;
                     rdfs:label "WPerm2sr" .


:UnitSymbol.WPermK uml:hasInitialValue "50" ;
                   uml:id "_6A7D3263-4D03-4d39-B90C-38C100BD95FF" ;
                   rdfs:comment "Thermal conductivity in watt/metres kelvin." ;
                   rdfs:label "WPermK" .


:UnitSymbol.WPers uml:hasInitialValue "81" ;
                  uml:id "_35FB6E73-2730-4ae7-A67E-58DC67D68D70" ;
                  rdfs:comment "Ramp rate in watts per second." ;
                  rdfs:label "WPers" .


:UnitSymbol.WPersr uml:hasInitialValue "191" ;
                   uml:id "_9A57C4F9-ECB2-4273-8741-9A36085DA221" ;
                   rdfs:comment "Radiant intensity, watts per steradian." ;
                   rdfs:label "WPersr" .


:UnitSymbol.Wb uml:hasInitialValue "36" ;
               uml:id "_6F7B9EE5-AFA0-4cbc-B2A9-E3942BD3772F" ;
               rdfs:comment "Magnetic flux in webers (V·s)." ;
               rdfs:label "Wb" .


:UnitSymbol.Wh uml:hasInitialValue "72" ;
               uml:id "_D0065D4C-31BE-42b1-9588-806157D3000D" ;
               rdfs:comment "Real energy in watt hours." ;
               rdfs:label "Wh" .


:UnitSymbol.anglemin uml:hasInitialValue "196" ;
                     uml:id "_79557E1F-CC74-431a-8A0D-6BD70094B0B2" ;
                     rdfs:comment "Plane angle, minutes." ;
                     rdfs:label "anglemin" .


:UnitSymbol.anglesec uml:hasInitialValue "197" ;
                     uml:id "_9C734EB4-BFFF-482e-95B2-B7446E3D8FFB" ;
                     rdfs:comment "Plane angle, seconds." ;
                     rdfs:label "anglesec" .


:UnitSymbol.bar uml:hasInitialValue "214" ;
                uml:id "_9516CB35-2CC3-4b7a-8BBA-BB329514810B" ;
                rdfs:comment "Pressure in bars, (1 bar = 100 kPa)." ;
                rdfs:label "bar" .


:UnitSymbol.cd uml:hasInitialValue "8" ;
               uml:id "_E12E81A8-81B6-4286-B477-2A91F984C4FC" ;
               rdfs:comment "Luminous intensity in candelas." ;
               rdfs:label "cd" .


:UnitSymbol.charPers uml:hasInitialValue "77" ;
                     uml:id "_28E0BFBE-2F7A-43d1-BB99-DCCBF7ADC265" ;
                     rdfs:comment "Data rate (baud) in characters per second." ;
                     rdfs:label "charPers" .


:UnitSymbol.character uml:hasInitialValue "76" ;
                      uml:id "_8187AD67-24E6-4cc1-931D-FC0964171586" ;
                      rdfs:comment "Number of characters." ;
                      rdfs:label "character" .


:UnitSymbol.cosPhi uml:hasInitialValue "65" ;
                   uml:id "_3FF3E24E-53F5-45ae-8408-47C453D360C2" ;
                   rdfs:comment """Power factor, dimensionless.
Note 1: This definition of power factor only holds for balanced systems. See the alternative definition under code 153.
Note 2 : Beware of differing sign conventions in use between the IEC and EEI. It is assumed that the data consumer understands the type of meter in use and the sign convention in use by the utility.""" ;
                   rdfs:label "cosPhi" .


:UnitSymbol.count uml:hasInitialValue "111" ;
                  uml:id "_45989859-38C4-4d11-A5CF-7DD5EFB0E7F7" ;
                  rdfs:comment "Amount of substance, Counter value." ;
                  rdfs:label "count" .


:UnitSymbol.d uml:hasInitialValue "195" ;
              uml:id "_5A45829C-D0A2-45cc-A862-689B13D34708" ;
              rdfs:comment "Time in days, day = 24 h = 86400 s." ;
              rdfs:label "d" .


:UnitSymbol.dB uml:hasInitialValue "79" ;
               uml:id "_5FEFCFB2-EFE9-4969-8832-5AB856D1D9BC" ;
               rdfs:comment "Sound pressure level in decibels. Note:  multiplier “d” is included in this unit symbol for compatibility with IEC 61850-7-3." ;
               rdfs:label "dB" .


:UnitSymbol.dBm uml:hasInitialValue "83" ;
                uml:id "_D3D3EFF1-D398-4bbf-B71E-947636027C51" ;
                rdfs:comment "Power level (logarithmic ratio of signal strength , Bel-mW), normalized to 1mW. Note:  multiplier “d” is included in this unit symbol for compatibility with IEC 61850-7-3." ;
                rdfs:label "dBm" .


:UnitSymbol.deg uml:hasInitialValue "9" ;
                uml:id "_4FEE2708-57BD-4ab8-BF2C-504B62A5358F" ;
                rdfs:comment "Plane angle in degrees." ;
                rdfs:label "deg" .


:UnitSymbol.degC uml:hasInitialValue "23" ;
                 uml:id "_9266DB6A-744E-4939-896F-B84E928D14EE" ;
                 rdfs:comment """Relative temperature in degrees Celsius.
In the SI unit system the symbol is °C. Electric charge is measured in coulomb that has the unit symbol C. To distinguish degree Celsius from coulomb the symbol used in the UML is degC. The reason for not using °C is that the special character ° is difficult to manage in software.""" ;
                 rdfs:label "degC" .


:UnitSymbol.ft3 uml:hasInitialValue "119" ;
                uml:id "_CF1F601E-EF72-4b25-A464-82800437A9B1" ;
                rdfs:comment "Volume, cubic feet." ;
                rdfs:label "ft3" .


:UnitSymbol.gPerg uml:hasInitialValue "144" ;
                  uml:id "_E7AD0FC3-F546-4d24-AB93-27B09C22F271" ;
                  rdfs:comment "Concentration, The ratio of the mass of a solute divided by the mass of  the solution. Note: Users may need use a prefix such a ‘µ’ to express a quantity such as ‘µg/g’." ;
                  rdfs:label "gPerg" .


:UnitSymbol.gal uml:hasInitialValue "128" ;
                uml:id "_A1611ECE-DA95-4e1c-A2AD-AF799F5994BB" ;
                rdfs:comment "Volume in gallons, US gallon (1 gal = 231 in3 = 128 fl ounce)." ;
                rdfs:label "gal" .


:UnitSymbol.h uml:hasInitialValue "84" ;
              uml:id "_38CFF289-C542-4313-987C-62BAAB914148" ;
              rdfs:comment "Time in hours, hour = 60 min = 3600 s." ;
              rdfs:label "h" .


:UnitSymbol.ha uml:hasInitialValue "198" ;
               uml:id "_A0047B54-799B-4a83-BC4B-B34DE2214F66" ;
               rdfs:comment "Area, hectares." ;
               rdfs:label "ha" .


:UnitSymbol.kat uml:hasInitialValue "158" ;
                uml:id "_92141CD6-2C4A-4ecb-A300-08FC15945FFF" ;
                rdfs:comment "Catalytic activity, katal = mol / s." ;
                rdfs:label "kat" .


:UnitSymbol.katPerm3 uml:hasInitialValue "193" ;
                     uml:id "_2AA4DD24-932C-4726-9E04-2A190E13D25D" ;
                     rdfs:comment "Catalytic activity concentration, katals per cubic metre." ;
                     rdfs:label "katPerm3" .


:UnitSymbol.kg uml:hasInitialValue "3" ;
               uml:id "_E8CD3F4B-2301-4f19-BBDF-6D20CD945743" ;
               rdfs:comment "Mass in kilograms.  Note: multiplier “k” is included in this unit symbol for compatibility with IEC 61850-7-3." ;
               rdfs:label "kg" .


:UnitSymbol.kgPerJ uml:id "_9740266F-DE31-4a0a-B60E-5B341A44FDB3" ;
                   rdfs:comment "Weight per energy in kilograms per joule (kg/J). Note: multiplier “k” is included in this unit symbol for compatibility with IEC 61850-7-3." ;
                   rdfs:label "kgPerJ" .


:UnitSymbol.kgPerm3 uml:hasInitialValue "48" ;
                    uml:id "_BDA99721-EF6C-465b-A531-083BB5A339E7" ;
                    rdfs:comment "Density in kilogram/cubic metres (kg/m³). Note: multiplier “k” is included in this unit symbol for compatibility with IEC 61850-7-3." ;
                    rdfs:label "kgPerm3" .


:UnitSymbol.kgm uml:hasInitialValue "47" ;
                uml:id "_7EF2DD04-E97D-43d0-8EF5-A0C71B65B30F" ;
                rdfs:comment "Moment of mass in kilogram metres (kg·m) (first moment of mass). Note: multiplier “k” is included in this unit symbol for compatibility with IEC 61850-7-3." ;
                rdfs:label "kgm" .


:UnitSymbol.kgm2 uml:hasInitialValue "78" ;
                 uml:id "_D18A5CA3-5F86-4f15-AF52-313ED1C0FCA9" ;
                 rdfs:comment "Moment of mass in kilogram square metres (kg·m²) (Second moment of mass, commonly called the moment of inertia). Note: multiplier “k” is included in this unit symbol for compatibility with IEC 61850-7-3." ;
                 rdfs:label "kgm2" .


:UnitSymbol.kn uml:hasInitialValue "219" ;
               uml:id "_76B3AB3B-A772-48a3-87A9-CC2655C20055" ;
               rdfs:comment "Speed, knots (1 kn = 1852/3600) m/s." ;
               rdfs:label "kn" .


:UnitSymbol.l uml:hasInitialValue "134" ;
              uml:id "_3D491A25-7CCF-4251-9579-D569948EE574" ;
              rdfs:comment "Volume in litres, litre = dm3 = m3/1000." ;
              rdfs:label "l" .


:UnitSymbol.lPerh uml:hasInitialValue "137" ;
                  uml:id "_2611249E-07C4-481b-96AF-3912056F7A39" ;
                  rdfs:comment "Volumetric flow rate, litres per hour." ;
                  rdfs:label "lPerh" .


:UnitSymbol.lPerl uml:hasInitialValue "143" ;
                  uml:id "_3C51034A-1DF4-4f24-9021-DEFB86D27C69" ;
                  rdfs:comment "Concentration, The ratio of the volume of a solute divided by the volume of  the solution. Note: Users may need use a prefix such a ‘µ’ to express a quantity such as ‘µL/L’." ;
                  rdfs:label "lPerl" .


:UnitSymbol.lPers uml:hasInitialValue "82" ;
                  uml:id "_FEA615F0-27A6-43e5-AB75-C6C2954D09CC" ;
                  rdfs:comment "Volumetric flow rate in litres per second." ;
                  rdfs:label "lPers" .


:UnitSymbol.lm uml:hasInitialValue "35" ;
               uml:id "_593D68AB-754E-46e4-8BB0-56BE19944355" ;
               rdfs:comment "Luminous flux in lumens (cd·sr)." ;
               rdfs:label "lm" .


:UnitSymbol.lx uml:hasInitialValue "34" ;
               uml:id "_234076FB-B88A-4249-9CFF-8F30847685B6" ;
               rdfs:comment "Illuminance in lux (lm/m²)." ;
               rdfs:label "lx" .


:UnitSymbol.m uml:hasInitialValue "2" ;
              uml:id "_5D4DDF01-7840-42a2-9106-C5CA5D41D1F2" ;
              rdfs:comment "Length in metres." ;
              rdfs:label "m" .


:UnitSymbol.m2 uml:hasInitialValue "41" ;
               uml:id "_A675331A-7D99-4e64-910D-A537BB8CEAAA" ;
               rdfs:comment "Area in square metres (m²)." ;
               rdfs:label "m2" .


:UnitSymbol.m2Pers uml:hasInitialValue "49" ;
                   uml:id "_4C077318-15E4-40e9-81AF-94A22098B3AA" ;
                   rdfs:comment "Viscosity in square metres / second (m²/s)." ;
                   rdfs:label "m2Pers" .


:UnitSymbol.m3 uml:hasInitialValue "42" ;
               uml:id "_ACC84E95-39F4-4acf-A99C-F0F50B37A605" ;
               rdfs:comment "Volume in cubic metres (m³)." ;
               rdfs:label "m3" .


:UnitSymbol.m3Compensated uml:hasInitialValue "167" ;
                          uml:id "_232385E4-F5BB-4699-A93F-10C49C822329" ;
                          rdfs:comment "Volume, cubic metres, with the value compensated for weather effects." ;
                          rdfs:label "m3Compensated" .


:UnitSymbol.m3Perh uml:hasInitialValue "125" ;
                   uml:id "_D3CF2309-7272-4d0c-9977-D83D3FDA4054" ;
                   rdfs:comment "Volumetric flow rate, cubic metres per hour." ;
                   rdfs:label "m3Perh" .


:UnitSymbol.m3Perkg uml:hasInitialValue "174" ;
                    uml:id "_0E1D3CF6-01AC-4cd4-BBCE-19D25E34BE91" ;
                    rdfs:comment "Specific volume, cubic metres per kilogram, v." ;
                    rdfs:label "m3Perkg" .


:UnitSymbol.m3Pers uml:hasInitialValue "45" ;
                   uml:id "_49157E6B-5DF9-4c4a-91DF-A99100A9959A" ;
                   rdfs:comment "Volumetric flow rate in cubic metres per second (m³/s)." ;
                   rdfs:label "m3Pers" .


:UnitSymbol.m3Uncompensated uml:hasInitialValue "166" ;
                            uml:id "_EAA81876-9511-48ce-9CC1-8E744D558E43" ;
                            rdfs:comment "Volume, cubic metres, with the value uncompensated for weather effects." ;
                            rdfs:label "m3Uncompensated" .


:UnitSymbol.mPerm3 uml:hasInitialValue "46" ;
                   uml:id "_B76349C8-69F4-433e-A6F4-9A709F4BAEE3" ;
                   rdfs:comment "Fuel efficiency in metres per cubic metres (m/m³)." ;
                   rdfs:label "mPerm3" .


:UnitSymbol.mPers uml:hasInitialValue "43" ;
                  uml:id "_AA6472CE-DFB5-446a-A9E7-52A5CE50CEF8" ;
                  rdfs:comment "Velocity in metres per second (m/s)." ;
                  rdfs:label "mPers" .


:UnitSymbol.mPers2 uml:hasInitialValue "44" ;
                   uml:id "_57C47608-7060-4960-B368-B53B6FDE195C" ;
                   rdfs:comment "Acceleration in metres per second squared (m/s²)." ;
                   rdfs:label "mPers2" .


:UnitSymbol.min uml:hasInitialValue "85" ;
                uml:id "_5E4420E6-9C1E-4e9c-ABE3-CDDD28FEF17F" ;
                rdfs:comment "Time in minutes, minute  = 60 s." ;
                rdfs:label "min" .


:UnitSymbol.mmHg uml:hasInitialValue "215" ;
                 uml:id "_A3459B23-0BDB-4e8f-822B-1D0EDD223D18" ;
                 rdfs:comment "Pressure, millimetres of mercury (1 mmHg is approximately 133.3 Pa)." ;
                 rdfs:label "mmHg" .


:UnitSymbol.mol uml:hasInitialValue "7" ;
                uml:id "_AE67CF4C-C8D9-446d-AF20-8BFC19C17C18" ;
                rdfs:comment "Amount of substance in moles." ;
                rdfs:label "mol" .


:UnitSymbol.molPerkg uml:hasInitialValue "147" ;
                     uml:id "_6D617CFF-CBD4-4c43-B8DF-7356CB496160" ;
                     rdfs:comment "Concentration, Molality, the amount of solute in moles and the amount of solvent in kilograms." ;
                     rdfs:label "molPerkg" .


:UnitSymbol.molPerm3 uml:hasInitialValue "145" ;
                     uml:id "_6E337AE9-1E58-41d7-A865-080C8E7E029B" ;
                     rdfs:comment "Concentration, The amount of substance concentration, (c), the amount of solvent in moles divided by the volume of solution in m³." ;
                     rdfs:label "molPerm3" .


:UnitSymbol.molPermol uml:hasInitialValue "146" ;
                      uml:id "_9723639D-4BA1-4756-952E-605DBFAF2057" ;
                      rdfs:comment "Concentration, Molar fraction, the ratio of the molar amount of a solute divided by the molar amount of the solution." ;
                      rdfs:label "molPermol" .


:UnitSymbol.none uml:hasInitialValue "0" ;
                 uml:id "_F14E9D40-A805-4840-B04C-34CD7BD279CC" ;
                 rdfs:comment "Dimension less quantity, e.g. count, per unit, etc." ;
                 rdfs:label "none" .


:UnitSymbol.ohm uml:hasInitialValue "30" ;
                uml:id "_1DD847A9-4242-4c5d-98D6-8BF40A3F14C2" ;
                rdfs:comment "Electric resistance in ohms (V/A)." ;
                rdfs:label "ohm" .


:UnitSymbol.ohmPerm uml:hasInitialValue "86" ;
                    uml:id "_2BDD18E5-7E62-4f66-AF25-21B7AB95AA3A" ;
                    rdfs:comment "Electric resistance per length in ohms per metre ((V/A)/m)." ;
                    rdfs:label "ohmPerm" .


:UnitSymbol.ohmm uml:hasInitialValue "102" ;
                 uml:id "_D0950984-9A0E-482a-9DE1-16F420DAE9CC" ;
                 rdfs:comment "Resistivity, ohm metres, (rho)." ;
                 rdfs:label "ohmm" .


:UnitSymbol.onePerHz uml:id "_46A68760-C92B-49b5-9BED-F01BFEDAD997" ;
                     rdfs:comment "Reciprocal of frequency (1/Hz)." ;
                     rdfs:label "onePerHz" .


:UnitSymbol.onePerm uml:hasInitialValue "173" ;
                    uml:id "_B8367965-284B-4e08-8567-055B00DAEDBA" ;
                    rdfs:comment "Wavenumber, reciprocal metres,  (1/m)." ;
                    rdfs:label "onePerm" .


:UnitSymbol.ppm uml:hasInitialValue "52" ;
                uml:id "_EAC82D26-6F54-4556-90EE-430E28882551" ;
                rdfs:comment "Concentration in parts per million." ;
                rdfs:label "ppm" .


:UnitSymbol.rad uml:hasInitialValue "10" ;
                uml:id "_90D4CFED-C041-47b2-9BD3-B4F34BA5FD95" ;
                rdfs:comment "Plane angle in radians (m/m)." ;
                rdfs:label "rad" .


:UnitSymbol.radPers uml:hasInitialValue "54" ;
                    uml:id "_D02F038B-E180-44e1-94C9-0EF927B2FF01" ;
                    rdfs:comment "Angular velocity in radians per second (rad/s)." ;
                    rdfs:label "radPers" .


:UnitSymbol.radPers2 uml:hasInitialValue "178" ;
                     uml:id "_2C2CD44E-2697-496e-8976-75216FBF43F4" ;
                     rdfs:comment "Angular acceleration, radians per second squared." ;
                     rdfs:label "radPers2" .


:UnitSymbol.rev uml:hasInitialValue "154" ;
                uml:id "_67CE50F0-C29B-444d-AC79-8A344CFCD3D8" ;
                rdfs:comment "Amount of rotation, revolutions." ;
                rdfs:label "rev" .


:UnitSymbol.rotPers uml:hasInitialValue "53" ;
                    uml:id "_B1F4EE35-083B-4d1f-A153-F7C65D67770D" ;
                    rdfs:comment "Rotations per second (1/s). See also Hz (1/s)." ;
                    rdfs:label "rotPers" .


:UnitSymbol.s uml:hasInitialValue "4" ;
              uml:id "_D53EB49C-18D1-430f-BBB5-C7ED93CCFC2B" ;
              rdfs:comment "Time in seconds." ;
              rdfs:label "s" .


:UnitSymbol.sPers uml:hasInitialValue "149" ;
                  uml:id "_6536A446-4A67-45c0-A68E-517D8F75A6CF" ;
                  rdfs:comment "Time, Ratio of time.  Note: Users may need to supply a prefix such as ‘&#181;’ to show rates such as ‘&#181;s/s’." ;
                  rdfs:label "sPers" .


:UnitSymbol.sr uml:hasInitialValue "11" ;
               uml:id "_EDB8BF68-BB72-4cac-9576-DCC78C57DBB1" ;
               rdfs:comment "Solid angle in steradians (m2/m2)." ;
               rdfs:label "sr" .


:UnitSymbol.therm uml:hasInitialValue "169" ;
                  uml:id "_D9814FF0-29BF-4ccd-8F0F-0203764EDD8E" ;
                  rdfs:comment "Energy, therms." ;
                  rdfs:label "therm" .


:UnitSymbol.tonne uml:hasInitialValue "199" ;
                  uml:id "_13E05807-8D00-40c0-8826-9D508FD4E0DE" ;
                  rdfs:comment "Mass in tons, “tonne” or “metric  ton” (1000 kg = 1 Mg)." ;
                  rdfs:label "tonne" .


:UnitType.CCYC uml:id "_1BCD98DE-D22A-49d0-A306-3293748AEE95" ;
               rdfs:comment "Combined Cycle" ;
               rdfs:label "CCYC" .


:UnitType.GTUR uml:id "_28A92343-D74A-4f77-BF1E-7366E5B6977D" ;
               rdfs:comment "Gas Turbine" ;
               rdfs:label "GTUR" .


:UnitType.HYDR uml:id "_0EB0C43C-209C-4a8b-A2C0-38B00569598A" ;
               rdfs:comment "Hydro Turbine" ;
               rdfs:label "HYDR" .


:UnitType.OTHR uml:id "_7A3CA9A5-C61E-42c2-85F8-2929ABEF8BE7" ;
               rdfs:comment "Other" ;
               rdfs:label "OTHR" .


:UnitType.PHOT uml:id "_2ED6BB53-16D4-4196-8422-FDA15CA8AB1D" ;
               rdfs:comment "Photovoltaic" ;
               rdfs:label "PHOT" .


:UnitType.PTUR uml:id "_7B7D6AF2-5A24-4092-803F-858CBA938DEE" ;
               rdfs:comment "Hydro Pump-Turbine" ;
               rdfs:label "PTUR" .


:UnitType.RECP uml:id "_E735EFEF-208E-4896-8C82-BEB39E9CE84A" ;
               rdfs:comment "Reciprocating Engine" ;
               rdfs:label "RECP" .


:UnitType.STUR uml:id "_B487EB67-3DAB-4502-8153-3B5A4BDBE9D9" ;
               rdfs:comment "Steam Turbine" ;
               rdfs:label "STUR" .


:UnitType.SYNC uml:id "_2FC904CD-0592-47d3-9692-B5E20681C895" ;
               rdfs:comment "Synchronous Condenser" ;
               rdfs:label "SYNC" .


:UnitType.WIND uml:id "_73C0CADB-5893-4383-966A-B9AACA595028" ;
               rdfs:comment "Wind Turbine" ;
               rdfs:label "WIND" .


:UnitTypeEMS.FLAG uml:id "_AF663099-83AE-46a1-A806-E7FC1555CDFB" ;
                  rdfs:label "FLAG" .


:UnitTypeEMS.MW uml:id "_59027ED3-980B-41c7-B8F4-53E60E84BF5B" ;
                rdfs:label "MW" .


:UsagePointConnectedKind.connected uml:id "_17FA1E04-B8F5-4e75-A5AE-A4B9961AB9C2" ;
                                   rdfs:comment "The usage point is connected to the network and able to receive or send the applicable commodity (electricity, gas, water, etc.)." ;
                                   rdfs:label "connected" .


:UsagePointConnectedKind.logicallyDisconnected uml:id "_3B889020-3D2B-4c5b-8293-487E1DB4F11C" ;
                                               rdfs:comment "The usage point has been disconnected through operation of a disconnect function within the meter present at the usage point.  The usage point is unable to receive or send the applicable commodity (electricity, gas, water, etc.)  A logical disconnect can often be achieved without utilising a field crew." ;
                                               rdfs:label "logicallyDisconnected" .


:UsagePointConnectedKind.physicallyDisconnected uml:id "_FAF8C3E7-6CCD-4d51-B83D-E70FC1AB16F7" ;
                                                rdfs:comment "The usage point has been disconnected from the network at a point upstream of the meter. The usage point is unable to receive or send the applicable commodity (electricity, gas, water, etc.). A physical disconnect is often achieved by utilising a field crew." ;
                                                rdfs:label "physicallyDisconnected" .


:Validity.GOOD uml:id "_6929D040-2986-40d3-81FA-B02D410FDB69" ;
               rdfs:comment "The value is marked good if no abnormal condition of the acquisition function or the information source is detected." ;
               rdfs:label "GOOD" .


:Validity.INVALID uml:id "_44F0D4CA-67C3-42a2-9AD6-B4C7F032EE3A" ;
                  rdfs:comment "The value is marked invalid when a supervision function recognises abnormal conditions of the acquisition function or the information source (missing or non-operating updating devices). The value is not defined under this condition. The mark invalid is used to indicate to the client that the value may be incorrect and shall not be used." ;
                  rdfs:label "INVALID" .


:Validity.QUESTIONABLE uml:id "_ED216555-F577-4c42-9E86-FF8AFBA02D0A" ;
                       rdfs:comment "The value is marked questionable if a supervision function detects an abnormal behaviour, however the value could still be valid. The client is responsible for determining whether or not values marked \"questionable\" should be used." ;
                       rdfs:label "QUESTIONABLE" .


:VehicleUsageKind.contractor uml:id "_D97F5E8C-A431-495a-967C-0735426EE4F7" ;
                             rdfs:comment "Contractor vehicle." ;
                             rdfs:label "contractor" .


:VehicleUsageKind.crew uml:id "_8C670F08-5610-46a5-85C1-1AA8F5CB0F08" ;
                       rdfs:comment "Crew vehicle." ;
                       rdfs:label "crew" .


:VehicleUsageKind.other uml:id "_49A2B67C-734A-488e-96F1-FA84D1B5BA6B" ;
                        rdfs:comment "Other vehicle." ;
                        rdfs:label "other" .


:VehicleUsageKind.user uml:id "_D83E1081-541C-44d5-B87D-02107C9FBC12" ;
                       rdfs:comment "User vehicle." ;
                       rdfs:label "user" .


:VsPpccControlKind.pPcc uml:id "_1B0F9D15-341D-482a-92CA-2F87FD68CFD2" ;
                        rdfs:comment "Control is real power at point of common coupling. The target value is provided by ACDCConverter.targetPpcc." ;
                        rdfs:label "pPcc" .


:VsPpccControlKind.pPccAndUdcDroop uml:id "_1FAEF8C2-B58F-4a82-B07C-AF01ED672BB4" ;
                                   rdfs:comment "Control is active power at point of common coupling and local DC voltage, with the droop. Target values are provided by ACDCConverter.targetPpcc, ACDCConverter.targetUdc and VsConverter.droop." ;
                                   rdfs:label "pPccAndUdcDroop" .


:VsPpccControlKind.pPccAndUdcDroopPilot uml:id "_026AFB0C-5BA9-42fd-AC2D-C825D86EFA8E" ;
                                        rdfs:comment "Control is active power at point of common coupling and the pilot DC voltage, with the droop. The mode is used for Multi Terminal High Voltage DC (MTDC) systems where multiple HVDC Substations are connected to the HVDC transmission lines. The pilot voltage is then used to coordinate the control the DC voltage across the HVDC substations. Targets are provided by ACDCConverter.targetPpcc, ACDCConverter.targetUdc and  VsConverter.droop." ;
                                        rdfs:label "pPccAndUdcDroopPilot" .


:VsPpccControlKind.pPccAndUdcDroopWithCompensation uml:id "_5433041C-16FD-4f7e-BF43-1289EA1FC438" ;
                                                   rdfs:comment "Control is active power at point of common coupling and compensated DC voltage, with the droop. Compensation factor is the resistance, as an approximation of the DC voltage of a common (real or virtual) node in the DC network. Targets are provided by ACDCConverter.targetPpcc, ACDCConverter.targetUdc, VsConverter.droop and VsConverter.droopCompensation." ;
                                                   rdfs:label "pPccAndUdcDroopWithCompensation" .


:VsPpccControlKind.phasePcc uml:id "_EC265815-0658-4950-BF62-F505124EFCFD" ;
                            rdfs:comment "Control is phase at point of common coupling. Target is provided by VsConverter.targetPhasePcc." ;
                            rdfs:label "phasePcc" .


:VsPpccControlKind.udc uml:id "_DA24FCF6-C1CE-42c3-8138-A3788B84DA92" ;
                       rdfs:comment "Control is DC voltage  with target value provided by ACDCConverter.targetUdc." ;
                       rdfs:label "udc" .


:VsQpccControlKind.powerFactorPcc uml:id "_845E8692-0146-4b18-BBD0-8E17B26F5D9C" ;
                                  rdfs:comment "Control is power factor at point of common coupling. Target is provided by VsConverter.targetPowerFactorPcc." ;
                                  rdfs:label "powerFactorPcc" .


:VsQpccControlKind.pulseWidthModulation uml:id "_9B3E5597-1865-4cac-9211-2C407D533F36" ;
                                        rdfs:comment "No explicit control. Pulse-modulation factor is directly set in magnitude (VsConverter.targetPWMfactor) and phase (VsConverter.targetPhasePcc)." ;
                                        rdfs:label "pulseWidthModulation" .


:VsQpccControlKind.reactivePcc uml:id "_5E2A3C32-97E0-4c8e-AD27-9EA00490046B" ;
                               rdfs:comment "Control is reactive power at point of common coupling. Target is provided by VsConverter.targetQpcc." ;
                               rdfs:label "reactivePcc" .


:VsQpccControlKind.voltagePcc uml:id "_14625573-690D-425b-AA5B-9510C347DDD9" ;
                              rdfs:comment "Control is voltage at point of common coupling. Target is provided by VsConverter.targetUpcc." ;
                              rdfs:label "voltagePcc" .


:WEPStandardEditionKind.none uml:id "_E8ABE143-FBD6-4a9c-BB51-3945E126A644" ;
                             rdfs:comment "No edition." ;
                             rdfs:label "none" .


:WEPStandardEditionKind.unknown uml:id "_E87A1C28-FA6D-4850-92F3-1EDADC89E986" ;
                                rdfs:comment "Unknown edition." ;
                                rdfs:label "unknown" .


:WEPStandardKind._12__1254E uml:id "_4CA3075B-F105-4fa7-B804-C5269A6D5143" ;
                            rdfs:comment "Westinghouse Engineering Procedure 12,1254E." ;
                            rdfs:label "12, 1254E" .


:WeatherCodeKind.blowingDust uml:id "_E0F531C0-5044-42a8-BC6B-2DDF802FDF43" ;
                             rdfs:comment "\"BD\" weather code (\"Blowing Dust\")." ;
                             rdfs:label "blowingDust" .


:WeatherCodeKind.blowingSand uml:id "_2DC4BDEB-1736-460b-8B42-E58F401E9C73" ;
                             rdfs:comment "\"BN\" weather code (\"Blowing Sand\")." ;
                             rdfs:label "blowingSand" .


:WeatherCodeKind.blowingSnow uml:id "_7A468B9B-B623-4ff2-800F-5CDA34C0D9C9" ;
                             rdfs:comment "\"BS\" weather code (\"Blowing Snow\")." ;
                             rdfs:label "blowingSnow" .


:WeatherCodeKind.cloudy uml:id "_EFD8ED93-8155-4714-86B4-E48E0AD52096" ;
                        rdfs:label "cloudy" .


:WeatherCodeKind.drizzle uml:id "_F0151170-3B33-4e03-A328-A6418F7D42F9" ;
                         rdfs:comment "\"L\" weather code (\"Drizzle\")." ;
                         rdfs:label "drizzle" .


:WeatherCodeKind.fog uml:id "_45476FA6-93BC-4a48-A00F-D3BD5CFBCD7A" ;
                     rdfs:comment "\"F weather code (\"Fog" ;
                     rdfs:label "fog" .


:WeatherCodeKind.freezingDrizzle uml:id "_44A69511-3719-4fe1-A52B-A99845EB3820" ;
                                 rdfs:comment "\"ZL\" weather code (\"Freezing Drizzle\")." ;
                                 rdfs:label "freezingDrizzle" .


:WeatherCodeKind.freezingRain uml:id "_E01BBF5B-9957-40cf-B7F8-DC9405236771" ;
                              rdfs:comment "\"ZR\" weather code (\"Freezing Rain\")." ;
                              rdfs:label "freezingRain" .


:WeatherCodeKind.freezingSpray uml:id "_6ED0709C-E261-4848-A8AB-CC5F6ACFE9AA" ;
                               rdfs:comment "\"ZF\" weather code (\"Freezing Spray\")." ;
                               rdfs:label "freezingSpray" .


:WeatherCodeKind.frost uml:id "_2AA1FC87-E332-4e2b-A809-483FDB580470" ;
                       rdfs:comment "\"FR\" weather code (\"Frost\")." ;
                       rdfs:label "frost" .


:WeatherCodeKind.hail uml:id "_742B73D2-767D-4ead-8C13-741A65BEF5F4" ;
                      rdfs:comment "\"A\" weather code (\"Hail\")." ;
                      rdfs:label "hail" .


:WeatherCodeKind.haze uml:id "_07E7D561-3CC8-462a-B6E4-FC88A6BFCAB3" ;
                      rdfs:comment "\"H\" weather code (\"Haze\")." ;
                      rdfs:label "haze" .


:WeatherCodeKind.iceCrystals uml:id "_CE5A7979-58F6-4dd8-857B-04F5730AA689" ;
                             rdfs:comment "\"IC\" weather code (\"Ice Crystals\")." ;
                             rdfs:label "iceCrystals" .


:WeatherCodeKind.iceFog uml:id "_4DEC155B-1E90-4763-8801-D49430C0AA48" ;
                        rdfs:comment "\"IF\" weather code (\"Ice Fog\")." ;
                        rdfs:label "iceFog" .


:WeatherCodeKind.mist uml:id "_2D039197-0D46-4690-87B9-576677817FE5" ;
                      rdfs:comment "\"BR\" weather code (\"Mist\")," ;
                      rdfs:label "mist" .


:WeatherCodeKind.rain uml:id "_A8CA7E19-1018-49b3-85AA-22CE71A710C4" ;
                      rdfs:comment "\"R\" weather code (\"Rain\")." ;
                      rdfs:label "rain" .


:WeatherCodeKind.rainShowers uml:id "_F17519D7-E93E-4905-8C37-7E52A34B916F" ;
                             rdfs:comment "\"RW\" weather code (\"Rain Showers\")." ;
                             rdfs:label "rainShowers" .


:WeatherCodeKind.rainSnowMix uml:id "_D2DF3E7B-73CB-44e7-939F-3AF047AFAA07" ;
                             rdfs:comment "\"RS\" weather code (\"Rain/Snow Mix\")." ;
                             rdfs:label "rainSnowMix" .


:WeatherCodeKind.sleet uml:id "_28F215C8-D2BC-4517-81E3-9217CB8B34DE" ;
                       rdfs:comment "\"IP\" weather code (\"Ice Pellets/Sleet\")." ;
                       rdfs:label "sleet" .


:WeatherCodeKind.smoke uml:id "_2716FE7C-54E7-4eb5-8BA4-40EBBCD6BBF3" ;
                       rdfs:comment "\"K\" weather code (\"Smoke\")." ;
                       rdfs:label "smoke" .


:WeatherCodeKind.snow uml:id "_B65013C4-F0CC-417c-AA75-7FB0D67DE414" ;
                      rdfs:comment "\"S\" weather code (\"Snow\")." ;
                      rdfs:label "snow" .


:WeatherCodeKind.snowShowers uml:id "_AD6D8ECF-CDB2-405c-81D9-5539DC162EA0" ;
                             rdfs:comment "\"SW\" weather code (\"Snow Showers\")." ;
                             rdfs:label "snowShowers" .


:WeatherCodeKind.snowSleetMix uml:id "_CEA3B9B9-BDAE-4703-B2E5-CD0FD5F591E9" ;
                              rdfs:comment "\"SI\" weather code (\"Snow/Sleet Mix\")." ;
                              rdfs:label "snowSleetMix" .


:WeatherCodeKind.sunny uml:id "_048C1A03-785A-4a6c-A21A-830537499F49" ;
                       rdfs:label "sunny" .


:WeatherCodeKind.thunderStorms uml:id "_0C130E5A-6648-4302-A4FD-C6C263B47F59" ;
                               rdfs:comment "\"T\" weather code (\"Thunder Storms\")." ;
                               rdfs:label "thunderStorms" .


:WeatherCodeKind.volcanicAsh uml:id "_4729552E-6CC0-4021-AAC6-D6080DB92D9E" ;
                             rdfs:comment "\"VA\" weather code (\"Volcanic Ash\")." ;
                             rdfs:label "volcanicAsh" .


:WeatherCodeKind.waterSpouts uml:id "_F4BE6152-6379-4f1f-9ECF-EBB25B3C7852" ;
                             rdfs:comment "\"WP\" weather code (\"Water Spouts\")" ;
                             rdfs:label "waterSpouts" .


:WeatherCodeKind.wintryMix uml:id "_046461B0-656F-4468-843C-3DDFC9765B6A" ;
                           rdfs:comment "\"WS\" weather code (\"Wintry Mix\")." ;
                           rdfs:label "wintryMix" .


:WindGenUnitKind.offshore uml:id "_CAA438A7-EAA7-4595-809E-A1F07F043FFD" ;
                          rdfs:comment "The wind generating unit is located offshore." ;
                          rdfs:label "offshore" .


:WindGenUnitKind.onshore uml:id "_BDE56A86-D849-42ab-8F4B-97BD16312617" ;
                         rdfs:comment "The wind generating unit is located onshore." ;
                         rdfs:label "onshore" .


:WindLookupTableFunctionKind.ipmax uml:id "_1B14E732-2D2F-42b6-A00A-432346B25E31" ;
                                   rdfs:comment "Lookup table for voltage dependency of active current limits (i<sub>pmax</sub>(u<sub>WT</sub>)). It is used for the current limitation model, IEC 61400-27-1:2015, 5.6.5.8." ;
                                   rdfs:label "ipmax" .


:WindLookupTableFunctionKind.iqmax uml:id "_36FEFE58-B86F-4eb1-8FD8-E43156818740" ;
                                   rdfs:comment "Lookup table for voltage dependency of reactive current limits (i<sub>qmax</sub>(u<sub>WT</sub>)). It is used for the current limitation model, IEC 61400-27-1:2015, 5.6.5.8." ;
                                   rdfs:label "iqmax" .


:WindLookupTableFunctionKind.omegap uml:id "_66683139-71CE-4174-B0E2-CD8ACC10862A" ;
                                    rdfs:comment "Power vs. speed lookup table (omega(p)). It is used for the P control model type 3, IEC 61400-27-1:2015, 5.6.5.4." ;
                                    rdfs:label "omegap" .


:WindLookupTableFunctionKind.prr uml:id "_B748FE52-33B7-4d36-9921-3A03A7B89E1A" ;
                                 rdfs:comment "Power versus speed change (negative slip) lookup table (p<sub>rr</sub>(deltaomega)). It is used for the rotor resistance control model, IEC 61400-27-1:2015, 5.6.5.3." ;
                                 rdfs:label "prr" .


:WindLookupTableFunctionKind.pwp uml:id "_9D027ECB-7A49-433a-9DE5-09918986DA1C" ;
                                 rdfs:comment "Power vs. frequency lookup table (p<sub>WPbias</sub>(f)). It is used for the wind power plant frequency and active power control model, IEC 61400-27-1:2015, Annex D." ;
                                 rdfs:label "pwp" .


:WindLookupTableFunctionKind.qmaxp uml:id "_E6370B95-DC95-494c-B457-8D67EAB70295" ;
                                   rdfs:comment "Lookup table for active power dependency of reactive power maximum limit (q<sub>maxp</sub>(p)). It is used for the QP and QU limitation model, IEC 61400-27-1:2015, 5.6.5.10." ;
                                   rdfs:label "qmaxp" .


:WindLookupTableFunctionKind.qmaxu uml:id "_690E4283-8B00-40f5-86EB-E4E18E6C497B" ;
                                   rdfs:comment "Lookup table for voltage dependency of reactive power maximum limit (q<sub>maxu</sub>(p)). It is used for the QP and QU limitation model, IEC 61400-27-1:2015, 5.6.5.10." ;
                                   rdfs:label "qmaxu" .


:WindLookupTableFunctionKind.qminp uml:id "_23F94943-3723-4277-943C-3D57681DDD5F" ;
                                   rdfs:comment "Lookup table for active power dependency of reactive power minimum limit (q<sub>minp</sub>(p)). It is used for the QP and QU limitation model, IEC 61400-27-1:2015, 5.6.5.10." ;
                                   rdfs:label "qminp" .


:WindLookupTableFunctionKind.qminu uml:id "_36C3CF45-F5C9-4914-9D6D-766DF38E805F" ;
                                   rdfs:comment "Lookup table for voltage dependency of reactive power minimum limit (q<sub>minu</sub>(p)). It is used for the QP and QU limitation model, IEC 61400-27-1:2015, 5.6.5.10." ;
                                   rdfs:label "qminu" .


:WindLookupTableFunctionKind.qwp uml:id "_D2A36A3B-2056-41d1-897D-6B8F821716FE" ;
                                 rdfs:comment "Look up table for the UQ static mode (q<sub>WP</sub>(u<sub>err</sub>)). It is used for the voltage and reactive power control model, IEC 61400-27-1:2015, Annex D." ;
                                 rdfs:label "qwp" .


:WindLookupTableFunctionKind.tcwdu uml:id "_282BB811-4873-4a71-91B7-7934CD548ABE" ;
                                   rdfs:comment "Crowbar duration versus voltage variation look-up table (T<sub>CW</sub>(du)). It is a case-dependent parameter. It is used for the type 3B generator set model, IEC 61400-27-1:2015, 5.6.3.3." ;
                                   rdfs:label "tcwdu" .


:WindLookupTableFunctionKind.tduwt uml:id "_176DA674-D6E3-4806-B463-BFD90B8DABDF" ;
                                   rdfs:comment "Lookup table to determine the duration of the power reduction after a voltage dip, depending on the size of the voltage dip (T<sub>d</sub>(u<sub>WT</sub>)). It is a type-dependent parameter. It is used for the pitch control power model, IEC 61400-27-1:2015, 5.6.5.1." ;
                                   rdfs:label "tduwt" .


:WindLookupTableFunctionKind.tfover uml:id "_9A943F84-5C84-47e0-B4DF-9D984C2231D6" ;
                                    rdfs:comment "Disconnection time versus over-frequency lookup table (T<sub>fover</sub>(f<sub>WT</sub>)). It is used for the grid protection model, IEC 61400-27-1:2015, 5.6.6." ;
                                    rdfs:label "tfover" .


:WindLookupTableFunctionKind.tfunder uml:id "_5C8F9AB5-4885-4232-9719-E9A3DB66F802" ;
                                     rdfs:comment "Disconnection time versus under-frequency lookup table (T<sub>funder</sub>(f<sub>WT</sub>)). It is used for the grid protection model, IEC 61400-27-1:2015, 5.6.6." ;
                                     rdfs:label "tfunder" .


:WindLookupTableFunctionKind.tuover uml:id "_1747CDAB-23E9-46c5-838D-70F6BF628D61" ;
                                    rdfs:comment "Disconnection time versus over-voltage lookup table (T<sub>uover</sub>(u<sub>WT</sub>)). It is used for the grid protection model, IEC 61400-27-1:2015, 5.6.6." ;
                                    rdfs:label "tuover" .


:WindLookupTableFunctionKind.tuunder uml:id "_8B0C6E5C-9164-4cc6-9E24-1BCA284CEF9A" ;
                                     rdfs:comment "Disconnection time versus under-voltage lookup table (T<sub>uunder</sub>(u<sub>WT</sub>)). It is used for the grid protection model, IEC 61400-27-1:2015, 5.6.6." ;
                                     rdfs:label "tuunder" .


:WindPlantQcontrolModeKind.powerFactor uml:id "_59D81CFD-D491-4d68-9E89-62DCB57FFFFF" ;
                                       rdfs:comment "Power factor reference." ;
                                       rdfs:label "powerFactor" .


:WindPlantQcontrolModeKind.reactivePower uml:id "_8748EB26-424E-4d1d-9276-F92E7AAC8286" ;
                                         rdfs:comment "Reactive power reference." ;
                                         rdfs:label "reactivePower" .


:WindPlantQcontrolModeKind.uqStatic uml:id "_F4C3853A-1AED-4286-8CE6-4E6C4375B803" ;
                                    rdfs:comment "UQ static." ;
                                    rdfs:label "uqStatic" .


:WindPlantQcontrolModeKind.voltageControl uml:id "_2E7704D8-5D74-4eb1-8EF2-3F7F213800DF" ;
                                          rdfs:comment "Voltage control." ;
                                          rdfs:label "voltageControl" .


:WindQcontrolModeKind.openLoopReactivePower uml:id "_6494681E-5E28-467b-85C6-46C752181AFF" ;
                                            rdfs:comment "Open loop reactive power control (only used with closed loop at plant level) (<i>M</i><i><sub>qG</sub></i><sub> </sub>equals 2)." ;
                                            rdfs:label "openLoopReactivePower" .


:WindQcontrolModeKind.openLooppowerFactor uml:id "_D4C1AF17-29B7-4ce7-8D62-9D6BF4D945A4" ;
                                          rdfs:comment "Open loop power factor control (<i>M</i><i><sub>qG</sub></i><sub> </sub>equals 4)." ;
                                          rdfs:label "openLooppowerFactor" .


:WindQcontrolModeKind.powerFactor uml:id "_25ED6E82-C16F-4cac-B91D-E54B0D0AE271" ;
                                  rdfs:comment "Power factor control (<i>M</i><i><sub>qG</sub></i><sub> </sub>equals 3)." ;
                                  rdfs:label "powerFactor" .


:WindQcontrolModeKind.reactivePower uml:id "_B57EAEC9-8F65-495e-8807-23746951BB08" ;
                                    rdfs:comment "Reactive power control (<i>M</i><i><sub>qG</sub></i> equals 1)." ;
                                    rdfs:label "reactivePower" .


:WindQcontrolModeKind.voltage uml:id "_3FD39FB0-3F40-42a6-899D-5A8120A15EFD" ;
                              rdfs:comment "Voltage control (<i>M</i><i><sub>qG</sub></i> equals 0)." ;
                              rdfs:label "voltage" .


:WindUVRTQcontrolModeKind.mode0 uml:id "_EE1CFEEC-B6FE-4121-914F-2048E4E2B1C9" ;
                                rdfs:comment "Voltage-dependent reactive current injection (<i>M</i><i><sub>qUVRT</sub></i> <sub> </sub>equals 0)." ;
                                rdfs:label "mode0" .


:WindUVRTQcontrolModeKind.mode1 uml:id "_6AEDB696-9494-4d56-AF04-5683FA0929F1" ;
                                rdfs:comment "Reactive current injection controlled as the pre-fault value plus an additional voltage dependent reactive current injection (<i>M</i><i><sub>qUVRT</sub></i> equals 1)." ;
                                rdfs:label "mode1" .


:WindUVRTQcontrolModeKind.mode2 uml:id "_9F30B7A5-E21A-4739-91FA-A9A94E53EFD3" ;
                                rdfs:comment "Reactive current injection controlled as the pre-fault value plus an additional voltage-dependent reactive current injection during fault, and as the pre-fault value plus an additional constant reactive current injection post fault (<i>M</i><i><sub>qUVRT</sub></i><sub>  </sub>equals 2)." ;
                                rdfs:label "mode2" .


:WindingConnection.A uml:id "_473A99ED-036B-405f-A0A4-EBED23928C49" ;
                     rdfs:comment "Autotransformer common winding." ;
                     rdfs:label "A" .


:WindingConnection.D uml:id "_B17A24C7-3B0F-4024-AC56-16CA61D533E6" ;
                     rdfs:comment "Delta." ;
                     rdfs:label "D" .


:WindingConnection.I uml:id "_FF8C5784-060C-4954-B55D-43105F992714" ;
                     rdfs:comment "Independent winding, for single-phase connections." ;
                     rdfs:label "I" .


:WindingConnection.Y uml:id "_CEEF48C7-F053-4f14-92EA-5D90C5DC84CA" ;
                     rdfs:comment "Wye." ;
                     rdfs:label "Y" .


:WindingConnection.Yn uml:id "_BBAF2E36-E868-4c4f-BFB9-00666ED78C08" ;
                      rdfs:comment "Wye, with neutral brought out for grounding." ;
                      rdfs:label "Yn" .


:WindingConnection.Z uml:id "_E5F532C8-F2D1-43c4-92D4-4E9EE6DA107D" ;
                     rdfs:comment "ZigZag." ;
                     rdfs:label "Z" .


:WindingConnection.Zn uml:id "_FFDB7590-ADFD-4c08-9BFC-84349F427C0A" ;
                      rdfs:comment "ZigZag, with neutral brought out for grounding." ;
                      rdfs:label "Zn" .


:WindingInsulationKind.nomex uml:id "_509B53BA-6E56-4101-A477-FA94D70E5103" ;
                             rdfs:label "nomex" .


:WindingInsulationKind.other uml:id "_7187EF04-71F4-4748-91E6-E515722C4D4B" ;
                             rdfs:label "other" .


:WindingInsulationKind.paper uml:id "_1CD6E7B1-7CCA-43f0-A857-1F18F72D6B84" ;
                             rdfs:label "paper" .


:WindingInsulationKind.thermallyUpgradedPaper uml:id "_8EF25822-D7C1-48c8-A97B-5E033ACFC16C" ;
                                              rdfs:label "thermallyUpgradedPaper" .


:WireInsulationKind.asbestosAndVarnishedCambric uml:id "_30E375BA-C4B3-4505-968E-B8BA20914E5E" ;
                                                rdfs:comment "Asbestos and varnished cambric wire insulation." ;
                                                rdfs:label "asbestosAndVarnishedCambric" .


:WireInsulationKind.beltedPilc uml:id "_62F9A2B8-02B3-4b5a-9AA6-B99CEC1EB596" ;
                               rdfs:comment "Belted pilc wire insulation." ;
                               rdfs:label "beltedPilc" .


:WireInsulationKind.butyl uml:id "_A5F33528-CC25-4812-9088-E60D3BFA49AF" ;
                          rdfs:comment "Butyl wire insulation." ;
                          rdfs:label "butyl" .


:WireInsulationKind.crosslinkedPolyethylene uml:id "_E912D943-F76D-46a4-B7FF-BF3871515F13" ;
                                            rdfs:comment "Crosslinked polyethylene wire insulation." ;
                                            rdfs:label "crosslinkedPolyethylene" .


:WireInsulationKind.ethylenePropyleneRubber uml:id "_4A0619A9-20BD-4ad4-BB89-E88F7E74C948" ;
                                            rdfs:comment "Ethylene propylene rubber wire insulation." ;
                                            rdfs:label "ethylenePropyleneRubber" .


:WireInsulationKind.highMolecularWeightPolyethylene uml:id "_0030F678-8470-4671-9E25-968B0DE137CF" ;
                                                    rdfs:comment "High nolecular weight polyethylene wire insulation." ;
                                                    rdfs:label "highMolecularWeightPolyethylene" .


:WireInsulationKind.highPressureFluidFilled uml:id "_D5DDABAF-1CA9-454f-A87C-F361B7E6A72D" ;
                                            rdfs:comment "High pressure fluid filled wire insulation." ;
                                            rdfs:label "highPressureFluidFilled" .


:WireInsulationKind.lowCapacitanceRubber uml:id "_5E43F710-8E6F-4fd0-AF8E-472D3E02EB4A" ;
                                         rdfs:comment "Low capacitance rubber wire insulation." ;
                                         rdfs:label "lowCapacitanceRubber" .


:WireInsulationKind.oilPaper uml:id "_74E898D3-1C82-4efd-9AD9-9405B755DC60" ;
                             rdfs:comment "Oil paper wire insulation." ;
                             rdfs:label "oilPaper" .


:WireInsulationKind.other uml:id "_7B2FF0B3-BBC2-4bfd-B2BA-96566F74904E" ;
                          rdfs:comment "Other kind of wire insulation." ;
                          rdfs:label "other" .


:WireInsulationKind.ozoneResistantRubber uml:id "_A345779F-3C98-4c51-AED3-A9FF9B9C9A55" ;
                                         rdfs:comment "Ozone resistant rubber wire insulation." ;
                                         rdfs:label "ozoneResistantRubber" .


:WireInsulationKind.rubber uml:id "_A9074515-1B3D-4b1e-99CA-5A869A2D844D" ;
                           rdfs:comment "Rubber wire insulation." ;
                           rdfs:label "rubber" .


:WireInsulationKind.siliconRubber uml:id "_D0FAEC04-3EEF-4020-AA92-FD1C7735718D" ;
                                  rdfs:comment "Silicon rubber wire insulation." ;
                                  rdfs:label "siliconRubber" .


:WireInsulationKind.treeResistantHighMolecularWeightPolyethylene uml:id "_D79DA710-F1DE-403e-9677-E4E201D8D310" ;
                                                                 rdfs:comment "Tree resistant high molecular weight polyethylene wire insulation." ;
                                                                 rdfs:label "treeResistantHighMolecularWeightPolyethylene" .


:WireInsulationKind.treeRetardantCrosslinkedPolyethylene uml:id "_B1222D86-1336-4d6d-A202-D418B9EF825C" ;
                                                         rdfs:comment "Tree retardant crosslinked polyethylene wire insulation." ;
                                                         rdfs:label "treeRetardantCrosslinkedPolyethylene" .


:WireInsulationKind.unbeltedPilc uml:id "_8FC1D561-1C31-408d-A2C9-7DF76D85010B" ;
                                 rdfs:comment "Unbelted pilc wire insulation." ;
                                 rdfs:label "unbeltedPilc" .


:WireInsulationKind.varnishedCambricCloth uml:id "_B0089617-3C80-4a82-8986-4EF1D2D92106" ;
                                          rdfs:comment "Varnished cambric cloth wire insulation." ;
                                          rdfs:label "varnishedCambricCloth" .


:WireInsulationKind.varnishedDacronGlass uml:id "_6DD767E3-93CA-46df-9E4C-2073C8E8574B" ;
                                         rdfs:comment "Varnished dacron glass wire insulation." ;
                                         rdfs:label "varnishedDacronGlass" .


:WireMaterialKind.aaac uml:id "_39B47590-4B8E-4006-933C-BB396BA23217" ;
                       rdfs:comment "Aluminum-alloy conductor steel reinforced." ;
                       rdfs:label "aaac" .


:WireMaterialKind.acsr uml:id "_95FD7B5D-209E-4eec-ACF6-E5387757BD08" ;
                       rdfs:comment "Aluminum conductor steel reinforced." ;
                       rdfs:label "acsr" .


:WireMaterialKind.aluminum uml:id "_433A8D99-E844-4f17-B01B-966253FB305B" ;
                           rdfs:comment "Aluminum wire." ;
                           rdfs:label "aluminum" .


:WireMaterialKind.aluminumAlloy uml:id "_2DF0A3CB-A604-4590-937D-226D68C40908" ;
                                rdfs:comment "Aluminum-alloy wire." ;
                                rdfs:label "aluminumAlloy" .


:WireMaterialKind.aluminumAlloySteel uml:id "_815E84F9-FF5C-4af3-9991-24FE3D56F69B" ;
                                     rdfs:comment "Aluminum-alloy-steel wire." ;
                                     rdfs:label "aluminumAlloySteel" .


:WireMaterialKind.aluminumSteel uml:id "_3D69894B-4569-4d20-87C9-1FC3311C6A63" ;
                                rdfs:comment "Aluminum-steel wire." ;
                                rdfs:label "aluminumSteel" .


:WireMaterialKind.copper uml:id "_5A0B6132-86F0-4609-B74F-6F758C8D48EF" ;
                         rdfs:comment "Copper wire." ;
                         rdfs:label "copper" .


:WireMaterialKind.other uml:id "_8399FECD-92B0-4ba6-B8B4-A9E6BFEE034D" ;
                        rdfs:comment "Other wire material." ;
                        rdfs:label "other" .


:WireMaterialKind.steel uml:id "_EE3F58B1-30B5-4cdd-922B-787F07F820D8" ;
                        rdfs:comment "Steel wire." ;
                        rdfs:label "steel" .


:WireUsageKind.distribution uml:id "_1D3D45DD-FA7F-4b23-A21B-1D58DFD712C5" ;
                            rdfs:comment "Wire is used in medium voltage network." ;
                            rdfs:label "distribution" .


:WireUsageKind.other uml:id "_2839FD65-EDFD-4f48-BA7B-BC43D0E31CA7" ;
                     rdfs:comment "Other kind of wire usage." ;
                     rdfs:label "other" .


:WireUsageKind.secondary uml:id "_0A9700A4-0FA1-46c8-A160-215D1948D37B" ;
                         rdfs:comment "Wire is used in low voltage circuit." ;
                         rdfs:label "secondary" .


:WireUsageKind.transmission uml:id "_251491DC-9AA3-40ff-B7BF-EBDDB07F0FF6" ;
                            rdfs:comment "Wire is used in extra-high voltage or high voltage network." ;
                            rdfs:label "transmission" .


:WorkActionKind.abandon uml:id "_7FA3F3CC-3E4E-420b-9615-2DFD8BB74777" ;
                        rdfs:comment "Leave it in place but not use it." ;
                        rdfs:label "abandon" .


:WorkActionKind.install uml:id "_40169EBA-0A02-44f3-92F7-F8259E78710A" ;
                        rdfs:comment "Install." ;
                        rdfs:label "install" .


:WorkActionKind.remove uml:id "_9324515E-CCC0-43f4-9EC3-34E7485652B5" ;
                       rdfs:comment "Remove." ;
                       rdfs:label "remove" .


:WorkActionKind.transfer uml:id "_0897113E-B76D-431d-9267-9D696261C8EF" ;
                         rdfs:comment "Remove from one and install at another loctation." ;
                         rdfs:label "transfer" .


:WorkStatusKind.approved uml:id "_5057A818-AA07-42cc-B8D9-5161B3184BA2" ;
                         rdfs:comment "Work has been approved." ;
                         rdfs:label "approved" .


:WorkStatusKind.cancelled uml:id "_339A9CC2-A20C-4f36-A400-DC0A4DA4DC7D" ;
                          rdfs:comment "Work has been canceled." ;
                          rdfs:label "cancelled" .


:WorkStatusKind.closed uml:id "_94C97DAF-02F0-4272-9CD6-05474493D9F3" ;
                       rdfs:comment "Work has been closed (typically by a person responsible for work management) and is ready for billing." ;
                       rdfs:label "closed" .


:WorkStatusKind.completed uml:id "_0EC9B67B-F060-4a1b-B467-B49B39A923EE" ;
                          rdfs:comment "Work has been completed, i.e., crew can leave the work location and is available for another work." ;
                          rdfs:label "completed" .


:WorkStatusKind.dispatched uml:id "_2B5AD67C-0F2A-4df4-A7BC-7E474A0ACF41" ;
                           rdfs:comment "Crew has been dispatched." ;
                           rdfs:label "dispatched" .


:WorkStatusKind.enroute uml:id "_138C75A7-0B81-4d97-B8DD-400537A3F2CE" ;
                        rdfs:comment "Crew is 'en route'." ;
                        rdfs:label "enroute" .


:WorkStatusKind.inProgress uml:id "_F93942E8-4EB4-44e2-9554-AC8608E6B90F" ;
                           rdfs:comment "Work is in progress." ;
                           rdfs:label "inProgress" .


:WorkStatusKind.onSite uml:id "_88CA861D-1421-4b0d-95D4-8544F332671F" ;
                       rdfs:comment "Crew is on the site." ;
                       rdfs:label "onSite" .


:WorkStatusKind.scheduled uml:id "_2040A7AE-92D2-4cf3-B314-9FA9B71CE87F" ;
                          rdfs:comment "Work has been scheduled." ;
                          rdfs:label "scheduled" .


:WorkStatusKind.waitingOnApproval uml:id "_155E917C-9579-4a94-B495-8778F313BD20" ;
                                  rdfs:comment "Work approval is pending." ;
                                  rdfs:label "waitingOnApproval" .


:WorkStatusKind.waitingOnMaterial uml:id "_9E154373-CA89-4d23-A4E8-35E02879B016" ;
                                  rdfs:comment "Work has been waiting on material." ;
                                  rdfs:label "waitingOnMaterial" .


:WorkStatusKind.waitingToBeScheduled uml:id "_F6D6D000-2B03-4ea3-B407-BD24173C98FA" ;
                                     rdfs:comment "Work needs to be scheduled." ;
                                     rdfs:label "waitingToBeScheduled" .


:WorkTaskKind.exchange uml:id "_621F815D-BDFD-4146-B45B-2B89546DD621" ;
                       rdfs:comment "Work task deals with exchange of assets." ;
                       rdfs:label "exchange" .


:WorkTaskKind.install uml:id "_C1B2174E-EDB4-4f10-94AC-2B0D2D8D93CA" ;
                      rdfs:comment "Work task deals with installation of assets." ;
                      rdfs:label "install" .


:WorkTaskKind.investigate uml:id "_8F3A049B-17B4-459a-90C0-B09C9EC8914C" ;
                          rdfs:comment "Work task deals with investigation about assets." ;
                          rdfs:label "investigate" .


:WorkTaskKind.remove uml:id "_BC9FE20F-8CD0-41a8-9F75-A4DFC190B9B2" ;
                     rdfs:comment "Work task deals with removal of assets." ;
                     rdfs:label "remove" .


:WorkTimeScheduleKind.actual uml:id "_4A7DDC08-A33B-496a-8109-F9DEDDED28BD" ;
                             rdfs:comment "Actual work time schedule." ;
                             rdfs:label "actual" .


:WorkTimeScheduleKind.earliest uml:id "_D71C72B0-9ADF-4a16-98E1-633DC4710A26" ;
                               rdfs:comment "Earliest work time schedule." ;
                               rdfs:label "earliest" .


:WorkTimeScheduleKind.estimate uml:id "_B3081235-198B-47da-8187-C425BA576FDE" ;
                               rdfs:comment "Estimate work time schedule." ;
                               rdfs:label "estimate" .


:WorkTimeScheduleKind.immediate uml:id "_486D7F9D-18E4-4630-9AAA-7659CDD82270" ;
                                rdfs:comment "??." ;
                                rdfs:label "immediate" .


:WorkTimeScheduleKind.latest uml:id "_BF0E733C-C6F7-4251-988E-7C83746A2957" ;
                             rdfs:comment "Latest work time schedule." ;
                             rdfs:label "latest" .


:WorkTimeScheduleKind.request uml:id "_EA40C9ED-10B3-4898-B316-F6ABB82C3AD6" ;
                              rdfs:comment "Request work time schedule." ;
                              rdfs:label "request" .


:YesNo.NO uml:id "_C27DE8FD-732D-43d2-8898-B8547130FB91" ;
          rdfs:label "NO" .


:YesNo.YES uml:id "_54A6BEC9-5CFC-4269-B252-C9637B123FF1" ;
           rdfs:label "YES" .


:ZoneKind.electricalNetwork uml:id "_3AFEA97D-AD07-41a9-ACFD-16E587A739F0" ;
                            rdfs:label "electricalNetwork" .


:ZoneKind.other uml:id "_E6101D62-B54A-477f-AFF4-0272B089D193" ;
                rdfs:label "other" .


:ZoneKind.specialRestrictionLand uml:id "_A32EA834-850F-4f37-AA6C-A22D845D5E8F" ;
                                 rdfs:label "specialRestrictionLand" .


:ZoneKind.weatherZone uml:id "_358B578F-209E-4907-92C5-24125B55397D" ;
                      rdfs:label "weatherZone" .


:ZoneType.ASREGION uml:id "_FC92FB19-420E-4a12-AEFF-E983621A8366" ;
                   rdfs:comment "ancillary service region" ;
                   rdfs:label "ASREGION" .


:ZoneType.DCA uml:id "_AC9A4301-6B37-4f8a-9FF7-CEA88CFEACD5" ;
              rdfs:comment "designated congestion area" ;
              rdfs:label "DCA" .


:ZoneType.LOADZONE uml:id "_E61398DB-F658-455f-82D1-922521ED8DC6" ;
                   rdfs:comment "load zone" ;
                   rdfs:label "LOADZONE" .


:ZoneType.RUCZONE uml:id "_4F49BEA5-63C7-4056-A767-FBCBEA225868" ;
                  rdfs:comment "RUC zone" ;
                  rdfs:label "RUCZONE" .


:ZoneType.TRADINGHUB uml:id "_C9AD4D89-E529-4224-B327-E34939FA7C10" ;
                     rdfs:comment "trading hub" ;
                     rdfs:label "TRADINGHUB" .


:runTypeCAISO.P uml:id "_B597DE19-45A9-465c-9EE2-78E4E364093B" ;
                rdfs:label "P" .


:runTypeCAISO.S uml:id "_3FB723A8-1F76-4af7-8BDA-40C03E71A11F" ;
                rdfs:label "S" .


###  Generated by the OWL API (version 4.5.26.2023-07-17T20:34:13Z) https://github.com/owlcs/owlapi
