<?xml version="1.0"?>
<rdf:RDF xmlns="http://iec.ch/TC57/CIM100#"
     xml:base="http://iec.ch/TC57/CIM100"
     xmlns:dc="http://purl.org/dc/elements/1.1/"
     xmlns:msg="http://langdale.com.au/2005/Message#"
     xmlns:owl="http://www.w3.org/2002/07/owl#"
     xmlns:rdf="http://www.w3.org/1999/02/22-rdf-syntax-ns#"
     xmlns:uml="http://langdale.com.au/2005/UML#"
     xmlns:xml="http://www.w3.org/XML/1998/namespace"
     xmlns:xsd="http://www.w3.org/2001/XMLSchema#"
     xmlns:rdfs="http://www.w3.org/2000/01/rdf-schema#">
    <owl:Ontology rdf:about="http://iec.ch/TC57/CIM100"/>
    


    <!-- 
    ///////////////////////////////////////////////////////////////////////////////////////
    //
    // Annotation properties
    //
    ///////////////////////////////////////////////////////////////////////////////////////
     -->

    


    <!-- http://langdale.com.au/2005/UML#baseprefix -->

    <owl:AnnotationProperty rdf:about="http://langdale.com.au/2005/UML#baseprefix"/>
    


    <!-- http://langdale.com.au/2005/UML#baseuri -->

    <owl:AnnotationProperty rdf:about="http://langdale.com.au/2005/UML#baseuri"/>
    


    <!-- http://langdale.com.au/2005/UML#hasInitialValue -->

    <owl:AnnotationProperty rdf:about="http://langdale.com.au/2005/UML#hasInitialValue"/>
    


    <!-- http://langdale.com.au/2005/UML#hasMaxCardinality -->

    <owl:AnnotationProperty rdf:about="http://langdale.com.au/2005/UML#hasMaxCardinality"/>
    


    <!-- http://langdale.com.au/2005/UML#hasMinCardinality -->

    <owl:AnnotationProperty rdf:about="http://langdale.com.au/2005/UML#hasMinCardinality"/>
    


    <!-- http://langdale.com.au/2005/UML#hasMultiplier -->

    <owl:AnnotationProperty rdf:about="http://langdale.com.au/2005/UML#hasMultiplier"/>
    


    <!-- http://langdale.com.au/2005/UML#hasStereotype -->

    <owl:AnnotationProperty rdf:about="http://langdale.com.au/2005/UML#hasStereotype"/>
    


    <!-- http://langdale.com.au/2005/UML#hasUnits -->

    <owl:AnnotationProperty rdf:about="http://langdale.com.au/2005/UML#hasUnits"/>
    


    <!-- http://langdale.com.au/2005/UML#id -->

    <owl:AnnotationProperty rdf:about="http://langdale.com.au/2005/UML#id"/>
    


    <!-- http://langdale.com.au/2005/UML#roleALabel -->

    <owl:AnnotationProperty rdf:about="http://langdale.com.au/2005/UML#roleALabel"/>
    


    <!-- http://langdale.com.au/2005/UML#roleAOf -->

    <owl:AnnotationProperty rdf:about="http://langdale.com.au/2005/UML#roleAOf"/>
    


    <!-- http://langdale.com.au/2005/UML#roleBLabel -->

    <owl:AnnotationProperty rdf:about="http://langdale.com.au/2005/UML#roleBLabel"/>
    


    <!-- http://langdale.com.au/2005/UML#roleBOf -->

    <owl:AnnotationProperty rdf:about="http://langdale.com.au/2005/UML#roleBOf"/>
    


    <!-- http://langdale.com.au/2005/UML#uriHasPrefix -->

    <owl:AnnotationProperty rdf:about="http://langdale.com.au/2005/UML#uriHasPrefix"/>
    


    <!-- 
    ///////////////////////////////////////////////////////////////////////////////////////
    //
    // Object Properties
    //
    ///////////////////////////////////////////////////////////////////////////////////////
     -->

    


    <!-- http://iec.ch/TC57/CIM100#BaseVoltage.ConductingEquipment -->

    <owl:ObjectProperty rdf:about="http://iec.ch/TC57/CIM100#BaseVoltage.ConductingEquipment">
        <owl:inverseOf rdf:resource="http://iec.ch/TC57/CIM100#ConductingEquipment.BaseVoltage"/>
        <rdfs:domain rdf:resource="http://iec.ch/TC57/CIM100#BaseVoltage"/>
        <rdfs:range rdf:resource="http://iec.ch/TC57/CIM100#ConductingEquipment"/>
        <uml:id>EAID_B21687D9_2B46_4880_B016_06CCFA215EC3-B</uml:id>
        <rdfs:comment>All conducting equipment with this base voltage.  Use only when there is no voltage level container used and only one base voltage applies.  For example, not used for transformers.</rdfs:comment>
        <rdfs:isDefinedBy rdf:resource="http://iec.ch/TC57/CIM100#Package_Core"/>
        <rdfs:label>ConductingEquipment</rdfs:label>
    </owl:ObjectProperty>
    


    <!-- http://iec.ch/TC57/CIM100#BaseVoltage.VoltageLevel -->

    <owl:ObjectProperty rdf:about="http://iec.ch/TC57/CIM100#BaseVoltage.VoltageLevel">
        <owl:inverseOf rdf:resource="http://iec.ch/TC57/CIM100#VoltageLevel.BaseVoltage"/>
        <rdfs:domain rdf:resource="http://iec.ch/TC57/CIM100#BaseVoltage"/>
        <rdfs:range rdf:resource="http://iec.ch/TC57/CIM100#VoltageLevel"/>
        <uml:id>EAID_F610FDC8_D98D_4367_99A9_E9CA1C8A8CC5-A</uml:id>
        <rdfs:comment>The voltage levels having this base voltage.</rdfs:comment>
        <rdfs:isDefinedBy rdf:resource="http://iec.ch/TC57/CIM100#Package_Core"/>
        <rdfs:label>VoltageLevel</rdfs:label>
    </owl:ObjectProperty>
    


    <!-- http://iec.ch/TC57/CIM100#Bay.Substation -->

    <owl:ObjectProperty rdf:about="http://iec.ch/TC57/CIM100#Bay.Substation">
        <owl:inverseOf rdf:resource="http://iec.ch/TC57/CIM100#Substation.Bays"/>
        <rdfs:domain rdf:resource="http://iec.ch/TC57/CIM100#Bay"/>
        <rdfs:range rdf:resource="http://iec.ch/TC57/CIM100#Substation"/>
        <uml:id>EAID_51152F4A_1B03_451f_BA84_6A05A6AE1630-B</uml:id>
        <rdfs:comment>Substation containing the bay.</rdfs:comment>
        <rdfs:isDefinedBy rdf:resource="http://iec.ch/TC57/CIM100#Package_Core"/>
        <rdfs:label>Substation</rdfs:label>
    </owl:ObjectProperty>
    


    <!-- http://iec.ch/TC57/CIM100#Bay.VoltageLevel -->

    <owl:ObjectProperty rdf:about="http://iec.ch/TC57/CIM100#Bay.VoltageLevel">
        <owl:inverseOf rdf:resource="http://iec.ch/TC57/CIM100#VoltageLevel.Bays"/>
        <rdfs:domain rdf:resource="http://iec.ch/TC57/CIM100#Bay"/>
        <rdfs:range rdf:resource="http://iec.ch/TC57/CIM100#VoltageLevel"/>
        <uml:id>EAID_5E328091_5BC1_4fa8_9BA3_F087A215492A-A</uml:id>
        <rdfs:comment>The voltage level containing this bay.</rdfs:comment>
        <rdfs:isDefinedBy rdf:resource="http://iec.ch/TC57/CIM100#Package_Core"/>
        <rdfs:label>VoltageLevel</rdfs:label>
    </owl:ObjectProperty>
    


    <!-- http://iec.ch/TC57/CIM100#ConductingEquipment.BaseVoltage -->

    <owl:ObjectProperty rdf:about="http://iec.ch/TC57/CIM100#ConductingEquipment.BaseVoltage">
        <rdfs:domain rdf:resource="http://iec.ch/TC57/CIM100#ConductingEquipment"/>
        <rdfs:range rdf:resource="http://iec.ch/TC57/CIM100#BaseVoltage"/>
        <uml:id>EAID_B21687D9_2B46_4880_B016_06CCFA215EC3-A</uml:id>
        <rdfs:comment>Base voltage of this conducting equipment.  Use only when there is no voltage level container used and only one base voltage applies.  For example, not used for transformers.</rdfs:comment>
        <rdfs:isDefinedBy rdf:resource="http://iec.ch/TC57/CIM100#Package_Core"/>
        <rdfs:label>BaseVoltage</rdfs:label>
    </owl:ObjectProperty>
    


    <!-- http://iec.ch/TC57/CIM100#ConductingEquipment.Terminals -->

    <owl:ObjectProperty rdf:about="http://iec.ch/TC57/CIM100#ConductingEquipment.Terminals">
        <owl:inverseOf rdf:resource="http://iec.ch/TC57/CIM100#Terminal.ConductingEquipment"/>
        <rdfs:domain rdf:resource="http://iec.ch/TC57/CIM100#ConductingEquipment"/>
        <rdfs:range rdf:resource="http://iec.ch/TC57/CIM100#Terminal"/>
        <uml:id>EAID_5FEF5186_7804_4dad_8E18_8C5DB7FCE6B2-A</uml:id>
        <rdfs:comment>Conducting equipment have terminals that may be connected to other conducting equipment terminals via connectivity nodes or topological nodes.</rdfs:comment>
        <rdfs:isDefinedBy rdf:resource="http://iec.ch/TC57/CIM100#Package_Core"/>
        <rdfs:label>Terminals</rdfs:label>
    </owl:ObjectProperty>
    


    <!-- http://iec.ch/TC57/CIM100#ConnectivityNode.ConnectivityNodeContainer -->

    <owl:ObjectProperty rdf:about="http://iec.ch/TC57/CIM100#ConnectivityNode.ConnectivityNodeContainer">
        <owl:inverseOf rdf:resource="http://iec.ch/TC57/CIM100#ConnectivityNodeContainer.ConnectivityNodes"/>
        <rdfs:domain rdf:resource="http://iec.ch/TC57/CIM100#ConnectivityNode"/>
        <rdfs:range rdf:resource="http://iec.ch/TC57/CIM100#ConnectivityNodeContainer"/>
        <uml:id>EAID_08EEABA6_269C_44a7_8F82_7BBEFE71ADD6-B</uml:id>
        <rdfs:comment>Container of this connectivity node.</rdfs:comment>
        <rdfs:isDefinedBy rdf:resource="http://iec.ch/TC57/CIM100#Package_Core"/>
        <rdfs:label>ConnectivityNodeContainer</rdfs:label>
    </owl:ObjectProperty>
    


    <!-- http://iec.ch/TC57/CIM100#ConnectivityNode.Terminals -->

    <owl:ObjectProperty rdf:about="http://iec.ch/TC57/CIM100#ConnectivityNode.Terminals">
        <owl:inverseOf rdf:resource="http://iec.ch/TC57/CIM100#Terminal.ConnectivityNode"/>
        <rdfs:domain rdf:resource="http://iec.ch/TC57/CIM100#ConnectivityNode"/>
        <rdfs:range rdf:resource="http://iec.ch/TC57/CIM100#Terminal"/>
        <uml:id>EAID_C7E01609_F4E6_4a6e_8ACF_BDD413E62DE3-A</uml:id>
        <rdfs:comment>Terminals interconnected with zero impedance at a this connectivity node.</rdfs:comment>
        <rdfs:isDefinedBy rdf:resource="http://iec.ch/TC57/CIM100#Package_Core"/>
        <rdfs:label>Terminals</rdfs:label>
    </owl:ObjectProperty>
    


    <!-- http://iec.ch/TC57/CIM100#ConnectivityNodeContainer.ConnectivityNodes -->

    <owl:ObjectProperty rdf:about="http://iec.ch/TC57/CIM100#ConnectivityNodeContainer.ConnectivityNodes">
        <rdfs:domain rdf:resource="http://iec.ch/TC57/CIM100#ConnectivityNodeContainer"/>
        <rdfs:range rdf:resource="http://iec.ch/TC57/CIM100#ConnectivityNode"/>
        <uml:id>EAID_08EEABA6_269C_44a7_8F82_7BBEFE71ADD6-A</uml:id>
        <rdfs:comment>Connectivity nodes which belong to this connectivity node container.</rdfs:comment>
        <rdfs:isDefinedBy rdf:resource="http://iec.ch/TC57/CIM100#Package_Core"/>
        <rdfs:label>ConnectivityNodes</rdfs:label>
    </owl:ObjectProperty>
    


    <!-- http://iec.ch/TC57/CIM100#Equipment.AdditionalEquipmentContainer -->

    <owl:ObjectProperty rdf:about="http://iec.ch/TC57/CIM100#Equipment.AdditionalEquipmentContainer">
        <owl:inverseOf rdf:resource="http://iec.ch/TC57/CIM100#EquipmentContainer.AdditionalGroupedEquipment"/>
        <rdfs:domain rdf:resource="http://iec.ch/TC57/CIM100#Equipment"/>
        <rdfs:range rdf:resource="http://iec.ch/TC57/CIM100#EquipmentContainer"/>
        <uml:id>EAID_43EA076F_F51B_4617_BC39_6D3939D5CEFD-A</uml:id>
        <rdfs:comment>Additional equipment container beyond the primary equipment container.  The equipment is contained in another equipment container, but also grouped with this equipment container.</rdfs:comment>
        <rdfs:isDefinedBy rdf:resource="http://iec.ch/TC57/CIM100#Package_Core"/>
        <rdfs:label>AdditionalEquipmentContainer</rdfs:label>
    </owl:ObjectProperty>
    


    <!-- http://iec.ch/TC57/CIM100#Equipment.EquipmentContainer -->

    <owl:ObjectProperty rdf:about="http://iec.ch/TC57/CIM100#Equipment.EquipmentContainer">
        <owl:inverseOf rdf:resource="http://iec.ch/TC57/CIM100#EquipmentContainer.Equipments"/>
        <rdfs:domain rdf:resource="http://iec.ch/TC57/CIM100#Equipment"/>
        <rdfs:range rdf:resource="http://iec.ch/TC57/CIM100#EquipmentContainer"/>
        <uml:id>EAID_68BA73EF_8533_48ba_964A_DE0F722292D2-A</uml:id>
        <rdfs:comment>Container of this equipment.</rdfs:comment>
        <rdfs:isDefinedBy rdf:resource="http://iec.ch/TC57/CIM100#Package_Core"/>
        <rdfs:label>EquipmentContainer</rdfs:label>
    </owl:ObjectProperty>
    


    <!-- http://iec.ch/TC57/CIM100#EquipmentContainer.AdditionalGroupedEquipment -->

    <owl:ObjectProperty rdf:about="http://iec.ch/TC57/CIM100#EquipmentContainer.AdditionalGroupedEquipment">
        <rdfs:domain rdf:resource="http://iec.ch/TC57/CIM100#EquipmentContainer"/>
        <rdfs:range rdf:resource="http://iec.ch/TC57/CIM100#Equipment"/>
        <uml:id>EAID_43EA076F_F51B_4617_BC39_6D3939D5CEFD-B</uml:id>
        <rdfs:comment>The additonal contained equipment.  The equipment belong to the equipment container. The equipment is contained in another equipment container, but also grouped with this equipment container.  Examples include when a switch contained in a substation is also desired to be grouped with a line contianer or when a switch is included in a secondary substation and also grouped in a feeder.</rdfs:comment>
        <rdfs:isDefinedBy rdf:resource="http://iec.ch/TC57/CIM100#Package_Core"/>
        <rdfs:label>AdditionalGroupedEquipment</rdfs:label>
    </owl:ObjectProperty>
    


    <!-- http://iec.ch/TC57/CIM100#EquipmentContainer.Equipments -->

    <owl:ObjectProperty rdf:about="http://iec.ch/TC57/CIM100#EquipmentContainer.Equipments">
        <rdfs:domain rdf:resource="http://iec.ch/TC57/CIM100#EquipmentContainer"/>
        <rdfs:range rdf:resource="http://iec.ch/TC57/CIM100#Equipment"/>
        <uml:id>EAID_68BA73EF_8533_48ba_964A_DE0F722292D2-B</uml:id>
        <rdfs:comment>Contained equipment.</rdfs:comment>
        <rdfs:isDefinedBy rdf:resource="http://iec.ch/TC57/CIM100#Package_Core"/>
        <rdfs:label>Equipments</rdfs:label>
    </owl:ObjectProperty>
    


    <!-- http://iec.ch/TC57/CIM100#GeographicalRegion.Regions -->

    <owl:ObjectProperty rdf:about="http://iec.ch/TC57/CIM100#GeographicalRegion.Regions">
        <owl:inverseOf rdf:resource="http://iec.ch/TC57/CIM100#SubGeographicalRegion.Region"/>
        <rdfs:domain rdf:resource="http://iec.ch/TC57/CIM100#GeographicalRegion"/>
        <rdfs:range rdf:resource="http://iec.ch/TC57/CIM100#SubGeographicalRegion"/>
        <uml:id>EAID_023E20DF_DF02_4ffb_A047_E5BBDB18AB59-B</uml:id>
        <rdfs:comment>All sub-geographical regions within this geographical region.</rdfs:comment>
        <rdfs:isDefinedBy rdf:resource="http://iec.ch/TC57/CIM100#Package_Core"/>
        <rdfs:label>Regions</rdfs:label>
    </owl:ObjectProperty>
    


    <!-- http://iec.ch/TC57/CIM100#IdentifiedObject.Names -->

    <owl:ObjectProperty rdf:about="http://iec.ch/TC57/CIM100#IdentifiedObject.Names">
        <owl:inverseOf rdf:resource="http://iec.ch/TC57/CIM100#Name.IdentifiedObject"/>
        <rdfs:domain rdf:resource="http://iec.ch/TC57/CIM100#IdentifiedObject"/>
        <rdfs:range rdf:resource="http://iec.ch/TC57/CIM100#Name"/>
        <uml:id>EAID_203C47E2_30FB_4c8f_ABEA_1661621CC0A7-A</uml:id>
        <rdfs:comment>All names of this identified object.</rdfs:comment>
        <rdfs:isDefinedBy rdf:resource="http://iec.ch/TC57/CIM100#Package_Core"/>
        <rdfs:label>Names</rdfs:label>
    </owl:ObjectProperty>
    


    <!-- http://iec.ch/TC57/CIM100#Line.Region -->

    <owl:ObjectProperty rdf:about="http://iec.ch/TC57/CIM100#Line.Region">
        <owl:inverseOf rdf:resource="http://iec.ch/TC57/CIM100#SubGeographicalRegion.Lines"/>
        <rdfs:domain rdf:resource="http://iec.ch/TC57/CIM100#Line"/>
        <rdfs:range rdf:resource="http://iec.ch/TC57/CIM100#SubGeographicalRegion"/>
        <uml:id>EAID_BAB73169_D3BE_43c3_A58B_F1B87EAA1239-A</uml:id>
        <rdfs:comment>The sub-geographical region of the line.</rdfs:comment>
        <rdfs:isDefinedBy rdf:resource="http://iec.ch/TC57/CIM100#Package_Core"/>
        <rdfs:label>Region</rdfs:label>
    </owl:ObjectProperty>
    


    <!-- http://iec.ch/TC57/CIM100#Name.IdentifiedObject -->

    <owl:ObjectProperty rdf:about="http://iec.ch/TC57/CIM100#Name.IdentifiedObject">
        <rdfs:domain rdf:resource="http://iec.ch/TC57/CIM100#Name"/>
        <rdfs:range rdf:resource="http://iec.ch/TC57/CIM100#IdentifiedObject"/>
        <uml:id>EAID_203C47E2_30FB_4c8f_ABEA_1661621CC0A7-B</uml:id>
        <rdfs:comment>Identified object that this name designates.</rdfs:comment>
        <rdfs:isDefinedBy rdf:resource="http://iec.ch/TC57/CIM100#Package_Core"/>
        <rdfs:label>IdentifiedObject</rdfs:label>
    </owl:ObjectProperty>
    


    <!-- http://iec.ch/TC57/CIM100#Name.NameType -->

    <owl:ObjectProperty rdf:about="http://iec.ch/TC57/CIM100#Name.NameType">
        <owl:inverseOf rdf:resource="http://iec.ch/TC57/CIM100#NameType.Names"/>
        <rdfs:domain rdf:resource="http://iec.ch/TC57/CIM100#Name"/>
        <rdfs:range rdf:resource="http://iec.ch/TC57/CIM100#NameType"/>
        <uml:id>EAID_2DF559F1_C2F0_43ff_B7E0_654C3E738FDE-B</uml:id>
        <rdfs:comment>Type of this name.</rdfs:comment>
        <rdfs:isDefinedBy rdf:resource="http://iec.ch/TC57/CIM100#Package_Core"/>
        <rdfs:label>NameType</rdfs:label>
    </owl:ObjectProperty>
    


    <!-- http://iec.ch/TC57/CIM100#NameType.Names -->

    <owl:ObjectProperty rdf:about="http://iec.ch/TC57/CIM100#NameType.Names">
        <rdfs:domain rdf:resource="http://iec.ch/TC57/CIM100#NameType"/>
        <rdfs:range rdf:resource="http://iec.ch/TC57/CIM100#Name"/>
        <uml:id>EAID_2DF559F1_C2F0_43ff_B7E0_654C3E738FDE-A</uml:id>
        <rdfs:comment>All names of this type.</rdfs:comment>
        <rdfs:isDefinedBy rdf:resource="http://iec.ch/TC57/CIM100#Package_Core"/>
        <rdfs:label>Names</rdfs:label>
    </owl:ObjectProperty>
    


    <!-- http://iec.ch/TC57/CIM100#PSRType.PowerSystemResources -->

    <owl:ObjectProperty rdf:about="http://iec.ch/TC57/CIM100#PSRType.PowerSystemResources">
        <owl:inverseOf rdf:resource="http://iec.ch/TC57/CIM100#PowerSystemResource.PSRType"/>
        <rdfs:domain rdf:resource="http://iec.ch/TC57/CIM100#PSRType"/>
        <rdfs:range rdf:resource="http://iec.ch/TC57/CIM100#PowerSystemResource"/>
        <uml:id>EAID_739158B5_6CE8_473f_87FF_1CDA17078612-A</uml:id>
        <rdfs:comment>Power system resources classified with this power system resource type.</rdfs:comment>
        <rdfs:isDefinedBy rdf:resource="http://iec.ch/TC57/CIM100#Package_Core"/>
        <rdfs:label>PowerSystemResources</rdfs:label>
    </owl:ObjectProperty>
    


    <!-- http://iec.ch/TC57/CIM100#PowerSystemResource.PSRType -->

    <owl:ObjectProperty rdf:about="http://iec.ch/TC57/CIM100#PowerSystemResource.PSRType">
        <rdfs:domain rdf:resource="http://iec.ch/TC57/CIM100#PowerSystemResource"/>
        <rdfs:range rdf:resource="http://iec.ch/TC57/CIM100#PSRType"/>
        <uml:id>EAID_739158B5_6CE8_473f_87FF_1CDA17078612-B</uml:id>
        <rdfs:comment>Custom classification for this power system resource.</rdfs:comment>
        <rdfs:isDefinedBy rdf:resource="http://iec.ch/TC57/CIM100#Package_Core"/>
        <rdfs:label>PSRType</rdfs:label>
    </owl:ObjectProperty>
    


    <!-- http://iec.ch/TC57/CIM100#SubGeographicalRegion.Lines -->

    <owl:ObjectProperty rdf:about="http://iec.ch/TC57/CIM100#SubGeographicalRegion.Lines">
        <rdfs:domain rdf:resource="http://iec.ch/TC57/CIM100#SubGeographicalRegion"/>
        <rdfs:range rdf:resource="http://iec.ch/TC57/CIM100#Line"/>
        <uml:id>EAID_BAB73169_D3BE_43c3_A58B_F1B87EAA1239-B</uml:id>
        <rdfs:comment>The lines within the sub-geographical region.</rdfs:comment>
        <rdfs:isDefinedBy rdf:resource="http://iec.ch/TC57/CIM100#Package_Core"/>
        <rdfs:label>Lines</rdfs:label>
    </owl:ObjectProperty>
    


    <!-- http://iec.ch/TC57/CIM100#SubGeographicalRegion.Region -->

    <owl:ObjectProperty rdf:about="http://iec.ch/TC57/CIM100#SubGeographicalRegion.Region">
        <rdfs:domain rdf:resource="http://iec.ch/TC57/CIM100#SubGeographicalRegion"/>
        <rdfs:range rdf:resource="http://iec.ch/TC57/CIM100#GeographicalRegion"/>
        <uml:id>EAID_023E20DF_DF02_4ffb_A047_E5BBDB18AB59-A</uml:id>
        <rdfs:comment>The geographical region which this sub-geographical region is within.</rdfs:comment>
        <rdfs:isDefinedBy rdf:resource="http://iec.ch/TC57/CIM100#Package_Core"/>
        <rdfs:label>Region</rdfs:label>
    </owl:ObjectProperty>
    


    <!-- http://iec.ch/TC57/CIM100#SubGeographicalRegion.Substations -->

    <owl:ObjectProperty rdf:about="http://iec.ch/TC57/CIM100#SubGeographicalRegion.Substations">
        <owl:inverseOf rdf:resource="http://iec.ch/TC57/CIM100#Substation.Region"/>
        <rdfs:domain rdf:resource="http://iec.ch/TC57/CIM100#SubGeographicalRegion"/>
        <rdfs:range rdf:resource="http://iec.ch/TC57/CIM100#Substation"/>
        <uml:id>EAID_66E7D72B_2889_483c_80A2_2E51B283F2B1-B</uml:id>
        <rdfs:comment>The substations in this sub-geographical region.</rdfs:comment>
        <rdfs:isDefinedBy rdf:resource="http://iec.ch/TC57/CIM100#Package_Core"/>
        <rdfs:label>Substations</rdfs:label>
    </owl:ObjectProperty>
    


    <!-- http://iec.ch/TC57/CIM100#Substation.Bays -->

    <owl:ObjectProperty rdf:about="http://iec.ch/TC57/CIM100#Substation.Bays">
        <rdfs:domain rdf:resource="http://iec.ch/TC57/CIM100#Substation"/>
        <rdfs:range rdf:resource="http://iec.ch/TC57/CIM100#Bay"/>
        <uml:id>EAID_51152F4A_1B03_451f_BA84_6A05A6AE1630-A</uml:id>
        <rdfs:comment>Bays contained in the substation.</rdfs:comment>
        <rdfs:isDefinedBy rdf:resource="http://iec.ch/TC57/CIM100#Package_Core"/>
        <rdfs:label>Bays</rdfs:label>
    </owl:ObjectProperty>
    


    <!-- http://iec.ch/TC57/CIM100#Substation.Region -->

    <owl:ObjectProperty rdf:about="http://iec.ch/TC57/CIM100#Substation.Region">
        <rdfs:domain rdf:resource="http://iec.ch/TC57/CIM100#Substation"/>
        <rdfs:range rdf:resource="http://iec.ch/TC57/CIM100#SubGeographicalRegion"/>
        <uml:id>EAID_66E7D72B_2889_483c_80A2_2E51B283F2B1-A</uml:id>
        <rdfs:comment>The SubGeographicalRegion containing the substation.</rdfs:comment>
        <rdfs:isDefinedBy rdf:resource="http://iec.ch/TC57/CIM100#Package_Core"/>
        <rdfs:label>Region</rdfs:label>
    </owl:ObjectProperty>
    


    <!-- http://iec.ch/TC57/CIM100#Substation.VoltageLevels -->

    <owl:ObjectProperty rdf:about="http://iec.ch/TC57/CIM100#Substation.VoltageLevels">
        <owl:inverseOf rdf:resource="http://iec.ch/TC57/CIM100#VoltageLevel.Substation"/>
        <rdfs:domain rdf:resource="http://iec.ch/TC57/CIM100#Substation"/>
        <rdfs:range rdf:resource="http://iec.ch/TC57/CIM100#VoltageLevel"/>
        <uml:id>EAID_0E9E9E28_C575_47c5_BF01_7F4EB8B36D16-B</uml:id>
        <rdfs:comment>The voltage levels within this substation.</rdfs:comment>
        <rdfs:isDefinedBy rdf:resource="http://iec.ch/TC57/CIM100#Package_Core"/>
        <rdfs:label>VoltageLevels</rdfs:label>
    </owl:ObjectProperty>
    


    <!-- http://iec.ch/TC57/CIM100#Terminal.ConductingEquipment -->

    <owl:ObjectProperty rdf:about="http://iec.ch/TC57/CIM100#Terminal.ConductingEquipment">
        <rdfs:domain rdf:resource="http://iec.ch/TC57/CIM100#Terminal"/>
        <rdfs:range rdf:resource="http://iec.ch/TC57/CIM100#ConductingEquipment"/>
        <uml:id>EAID_5FEF5186_7804_4dad_8E18_8C5DB7FCE6B2-B</uml:id>
        <rdfs:comment>The conducting equipment of the terminal.  Conducting equipment have  terminals that may be connected to other conducting equipment terminals via connectivity nodes or topological nodes.</rdfs:comment>
        <rdfs:isDefinedBy rdf:resource="http://iec.ch/TC57/CIM100#Package_Core"/>
        <rdfs:label>ConductingEquipment</rdfs:label>
    </owl:ObjectProperty>
    


    <!-- http://iec.ch/TC57/CIM100#Terminal.ConnectivityNode -->

    <owl:ObjectProperty rdf:about="http://iec.ch/TC57/CIM100#Terminal.ConnectivityNode">
        <rdfs:domain rdf:resource="http://iec.ch/TC57/CIM100#Terminal"/>
        <rdfs:range rdf:resource="http://iec.ch/TC57/CIM100#ConnectivityNode"/>
        <uml:id>EAID_C7E01609_F4E6_4a6e_8ACF_BDD413E62DE3-B</uml:id>
        <rdfs:comment>The connectivity node to which this terminal connects with zero impedance.</rdfs:comment>
        <rdfs:isDefinedBy rdf:resource="http://iec.ch/TC57/CIM100#Package_Core"/>
        <rdfs:label>ConnectivityNode</rdfs:label>
    </owl:ObjectProperty>
    


    <!-- http://iec.ch/TC57/CIM100#TopologicalNode.ConnectivityNodeContainer -->

    <owl:ObjectProperty rdf:about="http://iec.ch/TC57/CIM100#TopologicalNode.ConnectivityNodeContainer">
        <rdfs:range rdf:resource="http://iec.ch/TC57/CIM100#ConnectivityNodeContainer"/>
        <uml:id>EAID_88BD0C47_4CB3_44db_9A6B_20C783A24478-B</uml:id>
        <rdfs:comment>The connectivity node container to which the topological node belongs.</rdfs:comment>
        <rdfs:isDefinedBy rdf:resource="http://iec.ch/TC57/CIM100#Package_Core"/>
        <rdfs:label>ConnectivityNodeContainer</rdfs:label>
    </owl:ObjectProperty>
    


    <!-- http://iec.ch/TC57/CIM100#VoltageLevel.BaseVoltage -->

    <owl:ObjectProperty rdf:about="http://iec.ch/TC57/CIM100#VoltageLevel.BaseVoltage">
        <rdfs:domain rdf:resource="http://iec.ch/TC57/CIM100#VoltageLevel"/>
        <rdfs:range rdf:resource="http://iec.ch/TC57/CIM100#BaseVoltage"/>
        <uml:id>EAID_F610FDC8_D98D_4367_99A9_E9CA1C8A8CC5-B</uml:id>
        <rdfs:comment>The base voltage used for all equipment within the voltage level.</rdfs:comment>
        <rdfs:isDefinedBy rdf:resource="http://iec.ch/TC57/CIM100#Package_Core"/>
        <rdfs:label>BaseVoltage</rdfs:label>
    </owl:ObjectProperty>
    


    <!-- http://iec.ch/TC57/CIM100#VoltageLevel.Bays -->

    <owl:ObjectProperty rdf:about="http://iec.ch/TC57/CIM100#VoltageLevel.Bays">
        <rdfs:domain rdf:resource="http://iec.ch/TC57/CIM100#VoltageLevel"/>
        <rdfs:range rdf:resource="http://iec.ch/TC57/CIM100#Bay"/>
        <uml:id>EAID_5E328091_5BC1_4fa8_9BA3_F087A215492A-B</uml:id>
        <rdfs:comment>The bays within this voltage level.</rdfs:comment>
        <rdfs:isDefinedBy rdf:resource="http://iec.ch/TC57/CIM100#Package_Core"/>
        <rdfs:label>Bays</rdfs:label>
    </owl:ObjectProperty>
    


    <!-- http://iec.ch/TC57/CIM100#VoltageLevel.Substation -->

    <owl:ObjectProperty rdf:about="http://iec.ch/TC57/CIM100#VoltageLevel.Substation">
        <rdfs:domain rdf:resource="http://iec.ch/TC57/CIM100#VoltageLevel"/>
        <rdfs:range rdf:resource="http://iec.ch/TC57/CIM100#Substation"/>
        <uml:id>EAID_0E9E9E28_C575_47c5_BF01_7F4EB8B36D16-A</uml:id>
        <rdfs:comment>The substation of the voltage level.</rdfs:comment>
        <rdfs:isDefinedBy rdf:resource="http://iec.ch/TC57/CIM100#Package_Core"/>
        <rdfs:label>Substation</rdfs:label>
    </owl:ObjectProperty>
    


    <!-- 
    ///////////////////////////////////////////////////////////////////////////////////////
    //
    // Classes
    //
    ///////////////////////////////////////////////////////////////////////////////////////
     -->

    


    <!-- http://iec.ch/TC57/CIM100#ACDCTerminal -->

    <owl:Class rdf:about="http://iec.ch/TC57/CIM100#ACDCTerminal">
        <uml:id>EAID_D37077B9_3B0C_4c16_8F5F_9A6F2C83A7F2</uml:id>
        <rdfs:comment>An electrical connection point (AC or DC) to a piece of conducting equipment. Terminals are connected at physical connection points called connectivity nodes.</rdfs:comment>
        <rdfs:comment>The connected status is related to a bus-branch model and the topological node to terminal relation.  True implies the terminal is connected to the related topological node and false implies it is not. 
In a bus-branch model, the connected status is used to tell if equipment is disconnected without having to change the connectivity described by the topological node to terminal relation. A valid case is that conducting equipment can be connected in one end and open in the other. In particular for an AC line segment, where the reactive line charging can be significant, this is a relevant case.</rdfs:comment>
        <rdfs:comment>The orientation of the terminal connections for a multiple terminal conducting equipment.  The sequence numbering starts with 1 and additional terminals should follow in increasing order.   The first terminal is the &quot;starting point&quot; for a two terminal branch.</rdfs:comment>
        <rdfs:isDefinedBy rdf:resource="http://iec.ch/TC57/CIM100#Package_Core"/>
        <rdfs:label>ACDCTerminal</rdfs:label>
    </owl:Class>
    


    <!-- http://iec.ch/TC57/CIM100#BaseFrequency -->

    <owl:Class rdf:about="http://iec.ch/TC57/CIM100#BaseFrequency">
        <uml:id>EAID_2FA6A39A_A920_4ab7_92DC_D005DDDBB348</uml:id>
        <rdfs:comment>The BaseFrequency class describes a base frequency for a power system network. In case of multiple power networks with different frequencies, e.g. 50 Hz or 60 Hz each network will have its own base frequency class. Hence it is assumed that power system objects having different base frequencies appear in separate documents where each document has a single base frequency instance.</rdfs:comment>
        <rdfs:comment>The base frequency.</rdfs:comment>
        <rdfs:isDefinedBy rdf:resource="http://iec.ch/TC57/CIM100#Package_Core"/>
        <rdfs:label>BaseFrequency</rdfs:label>
    </owl:Class>
    


    <!-- http://iec.ch/TC57/CIM100#BasePower -->

    <owl:Class rdf:about="http://iec.ch/TC57/CIM100#BasePower">
        <uml:id>EAID_A10836E5_09FC_4862_B3C3_96D52298E21B</uml:id>
        <rdfs:comment>The BasePower class defines the base power used in the per unit calculations.</rdfs:comment>
        <rdfs:comment>Value used as base power.</rdfs:comment>
        <rdfs:isDefinedBy rdf:resource="http://iec.ch/TC57/CIM100#Package_Core"/>
        <rdfs:label>BasePower</rdfs:label>
    </owl:Class>
    


    <!-- http://iec.ch/TC57/CIM100#BaseVoltage -->

    <owl:Class rdf:about="http://iec.ch/TC57/CIM100#BaseVoltage">
        <uml:id>EAID_2E70DC9D_AEAE_46cc_B20A_C20A636AE9B0</uml:id>
        <rdfs:comment>Defines a system base voltage which is referenced.</rdfs:comment>
        <rdfs:comment>The power system resource&apos;s base voltage.  Shall be a positive value and not zero.</rdfs:comment>
        <rdfs:isDefinedBy rdf:resource="http://iec.ch/TC57/CIM100#Package_Core"/>
        <rdfs:label>BaseVoltage</rdfs:label>
    </owl:Class>
    


    <!-- http://iec.ch/TC57/CIM100#Bay -->

    <owl:Class rdf:about="http://iec.ch/TC57/CIM100#Bay">
        <uml:id>EAID_45910062_D4E8_40ee_99EB_FEC14DD9FAB0</uml:id>
        <rdfs:comment>A collection of power system resources (within a given substation) including conducting equipment, protection relays, measurements, and telemetry.  A bay typically represents a physical grouping related to modularization of equipment.</rdfs:comment>
        <rdfs:comment>Breaker configuration.</rdfs:comment>
        <rdfs:comment>Busbar configuration.</rdfs:comment>
        <rdfs:comment>Indicates the presence/absence of active/reactive power measurements.</rdfs:comment>
        <rdfs:comment>Indicates the presence/absence of energy measurements.</rdfs:comment>
        <rdfs:isDefinedBy rdf:resource="http://iec.ch/TC57/CIM100#Package_Core"/>
        <rdfs:label>Bay</rdfs:label>
    </owl:Class>
    


    <!-- http://iec.ch/TC57/CIM100#Boolean -->

    <owl:Class rdf:about="http://iec.ch/TC57/CIM100#Boolean">
        <uml:id>EAID_9F8964F1_6C32_465b_A83D_F5A201A291C3</uml:id>
        <rdfs:comment>A type with the value space &quot;true&quot; and &quot;false&quot;.</rdfs:comment>
        <rdfs:isDefinedBy rdf:resource="http://iec.ch/TC57/CIM100#Package_Domain"/>
        <rdfs:label>Boolean</rdfs:label>
    </owl:Class>
    


    <!-- http://iec.ch/TC57/CIM100#Breaker -->

    <owl:Class rdf:about="http://iec.ch/TC57/CIM100#Breaker">
        <uml:id>EAID_380D92AA_1D80_4e84_A8EE_843DACEB59DD</uml:id>
        <rdfs:comment>A mechanical switching device capable of making, carrying, and breaking currents under normal circuit conditions and also making, carrying for a specified time, and breaking currents under specified abnormal circuit conditions e.g.  those of short circuit.</rdfs:comment>
        <rdfs:comment>The transition time from open to close.</rdfs:comment>
        <rdfs:isDefinedBy rdf:resource="http://iec.ch/TC57/CIM100#Package_Wires"/>
        <rdfs:label>Breaker</rdfs:label>
    </owl:Class>
    


    <!-- http://iec.ch/TC57/CIM100#ConductingEquipment -->

    <owl:Class rdf:about="http://iec.ch/TC57/CIM100#ConductingEquipment">
        <uml:id>EAID_7C5F19FB_5253_430c_8E53_BDCF7EBCE4C1</uml:id>
        <rdfs:comment>The parts of the AC power system that are designed to carry current or that are conductively connected through terminals.</rdfs:comment>
        <rdfs:isDefinedBy rdf:resource="http://iec.ch/TC57/CIM100#Package_Core"/>
        <rdfs:label>ConductingEquipment</rdfs:label>
    </owl:Class>
    


    <!-- http://iec.ch/TC57/CIM100#ConnectivityNode -->

    <owl:Class rdf:about="http://iec.ch/TC57/CIM100#ConnectivityNode">
        <uml:id>EAID_8BCACC36_B2DD_4c2a_A2AE_CFDF43731FC2</uml:id>
        <rdfs:comment>Connectivity nodes are points where terminals of AC conducting equipment are connected together with zero impedance.</rdfs:comment>
        <rdfs:isDefinedBy rdf:resource="http://iec.ch/TC57/CIM100#Package_Core"/>
        <rdfs:label>ConnectivityNode</rdfs:label>
    </owl:Class>
    


    <!-- http://iec.ch/TC57/CIM100#ConnectivityNodeContainer -->

    <owl:Class rdf:about="http://iec.ch/TC57/CIM100#ConnectivityNodeContainer">
        <uml:id>EAID_B985C03E_46A3_4aec_B5B6_FDD983EBE621</uml:id>
        <rdfs:comment>A base class for all objects that may contain connectivity nodes or topological nodes.</rdfs:comment>
        <rdfs:isDefinedBy rdf:resource="http://iec.ch/TC57/CIM100#Package_Core"/>
        <rdfs:label>ConnectivityNodeContainer</rdfs:label>
    </owl:Class>
    


    <!-- http://iec.ch/TC57/CIM100#Date -->

    <owl:Class rdf:about="http://iec.ch/TC57/CIM100#Date">
        <uml:id>EAID_C724EF94_9D38_4673_A889_46E7C5C6321C</uml:id>
        <rdfs:comment>Date as &quot;yyyy-mm-dd&quot;, which conforms with ISO 8601. UTC time zone is specified as &quot;yyyy-mm-ddZ&quot;. A local timezone relative UTC is specified as &quot;yyyy-mm-dd(+/-)hh:mm&quot;.</rdfs:comment>
        <rdfs:isDefinedBy rdf:resource="http://iec.ch/TC57/CIM100#Package_Domain"/>
        <rdfs:label>Date</rdfs:label>
    </owl:Class>
    


    <!-- http://iec.ch/TC57/CIM100#DateAndOrTime -->

    <owl:Class rdf:about="http://iec.ch/TC57/CIM100#DateAndOrTime">
        <uml:id>EAID_209EDF47_74BC_4a80_BCF8_42F3960FFE71</uml:id>
        <rdfs:comment>Date as &quot;yyyy-mm-dd&quot;, which conforms with ISO 8601</rdfs:comment>
        <rdfs:comment>The date and/or the time.</rdfs:comment>
        <rdfs:comment>Time as &quot;hh:mm:ss.sssZ&quot;, which conforms with ISO 8601.</rdfs:comment>
        <rdfs:isDefinedBy rdf:resource="http://iec.ch/TC57/CIM100#Package_MarketManagement"/>
        <rdfs:label>DateAndOrTime</rdfs:label>
    </owl:Class>
    


    <!-- http://iec.ch/TC57/CIM100#DateInterval -->

    <owl:Class rdf:about="http://iec.ch/TC57/CIM100#DateInterval">
        <uml:id>EAID_28B6A229_F6A8_4d93_BD50_F337824B5C8F</uml:id>
        <rdfs:comment>End date of this interval.</rdfs:comment>
        <rdfs:comment>Interval between two dates.</rdfs:comment>
        <rdfs:comment>Start date of this interval.</rdfs:comment>
        <rdfs:isDefinedBy rdf:resource="http://iec.ch/TC57/CIM100#Package_Domain"/>
        <rdfs:label>DateInterval</rdfs:label>
    </owl:Class>
    


    <!-- http://iec.ch/TC57/CIM100#DateTime -->

    <owl:Class rdf:about="http://iec.ch/TC57/CIM100#DateTime">
        <uml:id>EAID_EEAE6E83_944C_489c_8E25_CFB85F80C3EB</uml:id>
        <rdfs:comment>Date and time as &quot;yyyy-mm-ddThh:mm:ss.sss&quot;, which conforms with ISO 8601. UTC time zone is specified as &quot;yyyy-mm-ddThh:mm:ss.sssZ&quot;. A local timezone relative UTC is specified as &quot;yyyy-mm-ddThh:mm:ss.sss-hh:mm&quot;. The second component (shown here as &quot;ss.sss&quot;) could have any number of digits in its fractional part to allow any kind of precision beyond seconds.</rdfs:comment>
        <rdfs:isDefinedBy rdf:resource="http://iec.ch/TC57/CIM100#Package_Domain"/>
        <rdfs:label>DateTime</rdfs:label>
    </owl:Class>
    


    <!-- http://iec.ch/TC57/CIM100#Decimal -->

    <owl:Class rdf:about="http://iec.ch/TC57/CIM100#Decimal">
        <uml:id>EAID_9CD33DFD_D5FD_46a0_A320_11DFA5341F73</uml:id>
        <rdfs:comment>Decimal is the base-10 notational system for representing real numbers.</rdfs:comment>
        <rdfs:isDefinedBy rdf:resource="http://iec.ch/TC57/CIM100#Package_Domain"/>
        <rdfs:label>Decimal</rdfs:label>
    </owl:Class>
    


    <!-- http://iec.ch/TC57/CIM100#Discrete -->

    <owl:Class rdf:about="http://iec.ch/TC57/CIM100#Discrete">
        <uml:id>EAID_57AFC760_6CA7_42c5_B988_36221A805D38</uml:id>
        <rdfs:comment>Discrete represents a discrete Measurement, i.e. a Measurement representing discrete values, e.g. a Breaker position.</rdfs:comment>
        <rdfs:comment>Normal measurement value, e.g., used for percentage calculations.</rdfs:comment>
        <rdfs:comment>Normal value range maximum for any of the MeasurementValue.values. Used for scaling, e.g. in bar graphs or of telemetered raw values.</rdfs:comment>
        <rdfs:comment>Normal value range minimum for any of the MeasurementValue.values. Used for scaling, e.g. in bar graphs or of telemetered raw values.</rdfs:comment>
        <rdfs:isDefinedBy rdf:resource="http://iec.ch/TC57/CIM100#Package_Meas"/>
        <rdfs:label>Discrete</rdfs:label>
    </owl:Class>
    


    <!-- http://iec.ch/TC57/CIM100#Equipment -->

    <owl:Class rdf:about="http://iec.ch/TC57/CIM100#Equipment">
        <uml:id>EAID_F8DD8DAC_3545_4660_9CA5_794881CC6591</uml:id>
        <rdfs:comment>Specifies the availability of the equipment under normal operating conditions. True means the equipment is available for topology processing, which determines if the equipment is energized or not. False means that the equipment is treated by network applications as if it is not in the model.</rdfs:comment>
        <rdfs:comment>Specifies the availability of the equipment. True means the equipment is available for topology processing, which determines if the equipment is energized or not. False means that the equipment is treated by network applications as if it is not in the model.</rdfs:comment>
        <rdfs:comment>The aggregate flag provides an alternative way of representing an aggregated (equivalent) element. It is applicable in cases when the dedicated classes for equivalent equipment do not have all of the attributes necessary to represent the required level of detail.  In case the flag is set to “true” the single instance of equipment represents multiple pieces of equipment that have been modelled together as an aggregate equivalent obtained by a network reduction procedure. Examples would be power transformers or synchronous machines operating in parallel modelled as a single aggregate power transformer or aggregate synchronous machine.  
The attribute is not used for EquivalentBranch, EquivalentShunt and EquivalentInjection.</rdfs:comment>
        <rdfs:comment>The equipment is enabled to participate in network analysis.  If unspecified, the value is assumed to be true.</rdfs:comment>
        <rdfs:comment>The parts of a power system that are physical devices, electronic or mechanical.</rdfs:comment>
        <rdfs:isDefinedBy rdf:resource="http://iec.ch/TC57/CIM100#Package_Core"/>
        <rdfs:label>Equipment</rdfs:label>
    </owl:Class>
    


    <!-- http://iec.ch/TC57/CIM100#EquipmentContainer -->

    <owl:Class rdf:about="http://iec.ch/TC57/CIM100#EquipmentContainer">
        <uml:id>EAID_F465B7B4_B488_46c5_8D05_8036F09A03A0</uml:id>
        <rdfs:comment>A modelling construct to provide a root class for containing equipment.</rdfs:comment>
        <rdfs:isDefinedBy rdf:resource="http://iec.ch/TC57/CIM100#Package_Core"/>
        <rdfs:label>EquipmentContainer</rdfs:label>
    </owl:Class>
    


    <!-- http://iec.ch/TC57/CIM100#Float -->

    <owl:Class rdf:about="http://iec.ch/TC57/CIM100#Float">
        <uml:id>EAID_921A00A7_D33C_43ea_9DE4_70A026CBA70F</uml:id>
        <rdfs:comment>A floating point number. The range is unspecified and not limited.</rdfs:comment>
        <rdfs:isDefinedBy rdf:resource="http://iec.ch/TC57/CIM100#Package_Domain"/>
        <rdfs:label>Float</rdfs:label>
    </owl:Class>
    


    <!-- http://iec.ch/TC57/CIM100#Frequency -->

    <owl:Class rdf:about="http://iec.ch/TC57/CIM100#Frequency">
        <uml:id>EAID_DD71FE93_4683_440c_8622_A8AA2EB44F6F</uml:id>
        <rdfs:comment>Cycles per second.</rdfs:comment>
        <rdfs:isDefinedBy rdf:resource="http://iec.ch/TC57/CIM100#Package_Domain"/>
        <rdfs:label>Frequency</rdfs:label>
    </owl:Class>
    


    <!-- http://iec.ch/TC57/CIM100#GeographicalRegion -->

    <owl:Class rdf:about="http://iec.ch/TC57/CIM100#GeographicalRegion">
        <uml:id>EAID_F935232D_65FF_4720_BAFB_50639B7CA0AB</uml:id>
        <rdfs:comment>A geographical region of a power system network model.</rdfs:comment>
        <rdfs:isDefinedBy rdf:resource="http://iec.ch/TC57/CIM100#Package_Core"/>
        <rdfs:label>GeographicalRegion</rdfs:label>
    </owl:Class>
    


    <!-- http://iec.ch/TC57/CIM100#Hours -->

    <owl:Class rdf:about="http://iec.ch/TC57/CIM100#Hours">
        <uml:id>EAID_C8C67111_A8BF_46d8_B8DB_F0336CD201D1</uml:id>
        <rdfs:comment>Time specified in hours.</rdfs:comment>
        <rdfs:isDefinedBy rdf:resource="http://iec.ch/TC57/CIM100#Package_Domain"/>
        <rdfs:label>Hours</rdfs:label>
    </owl:Class>
    


    <!-- http://iec.ch/TC57/CIM100#IEC61970CIMVersion -->

    <owl:Class rdf:about="http://iec.ch/TC57/CIM100#IEC61970CIMVersion">
        <uml:id>EAID_990AB50C_5CF8_46d2_B5FF_887BBBD3346F</uml:id>
        <rdfs:comment>Form is IEC61970CIMXXvYY where XX is the major CIM package version and the YY is the minor version. For example IEC61970CIM13v18.</rdfs:comment>
        <rdfs:comment>Form is YYYY-MM-DD for example for January 5, 2009 it is 2009-01-05.</rdfs:comment>
        <rdfs:comment>This is the IEC 61970 CIM version number assigned to this UML model.</rdfs:comment>
        <rdfs:isDefinedBy rdf:resource="http://iec.ch/TC57/CIM100#Package_IEC61970"/>
        <rdfs:label>IEC61970CIMVersion</rdfs:label>
    </owl:Class>
    


    <!-- http://iec.ch/TC57/CIM100#IdentifiedObject -->

    <owl:Class rdf:about="http://iec.ch/TC57/CIM100#IdentifiedObject">
        <uml:id>EAID_055C5806_E9D8_4a7a_9307_DAF7C31763C7</uml:id>
        <rdfs:comment>Master resource identifier issued by a model authority. The mRID is unique within an exchange context. Global uniqueness is easily achieved by using a UUID, as specified in RFC 4122, for the mRID. The use of UUID is strongly recommended.
For CIMXML data files in RDF syntax conforming to IEC 61970-552, the mRID is mapped to rdf:ID or rdf:about attributes that identify CIM object elements.</rdfs:comment>
        <rdfs:comment>The aliasName is free text human readable name of the object alternative to IdentifiedObject.name. It may be non unique and may not correlate to a naming hierarchy.
The attribute aliasName is retained because of backwards compatibility between CIM relases. It is however recommended to replace aliasName with the Name class as aliasName is planned for retirement at a future time.</rdfs:comment>
        <rdfs:comment>The description is a free human readable text describing or naming the object. It may be non unique and may not correlate to a naming hierarchy.</rdfs:comment>
        <rdfs:comment>The name is any free human readable and possibly non unique text naming the object.</rdfs:comment>
        <rdfs:comment>This is a root class to provide common identification for all classes needing identification and naming attributes.</rdfs:comment>
        <rdfs:isDefinedBy rdf:resource="http://iec.ch/TC57/CIM100#Package_Core"/>
        <rdfs:label>IdentifiedObject</rdfs:label>
    </owl:Class>
    


    <!-- http://iec.ch/TC57/CIM100#Integer -->

    <owl:Class rdf:about="http://iec.ch/TC57/CIM100#Integer">
        <uml:id>EAID_5F6B613B_C31A_4476_8050_E600FBD5F789</uml:id>
        <rdfs:comment>An integer number. The range is unspecified and not limited.</rdfs:comment>
        <rdfs:isDefinedBy rdf:resource="http://iec.ch/TC57/CIM100#Package_Domain"/>
        <rdfs:label>Integer</rdfs:label>
    </owl:Class>
    


    <!-- http://iec.ch/TC57/CIM100#Length -->

    <owl:Class rdf:about="http://iec.ch/TC57/CIM100#Length">
        <uml:id>EAID_06F9A3F0_3AE3_4ad1_88F8_06C207238C3B</uml:id>
        <rdfs:comment>Unit of length. It shall be a positive value or zero.</rdfs:comment>
        <rdfs:isDefinedBy rdf:resource="http://iec.ch/TC57/CIM100#Package_Domain"/>
        <rdfs:label>Length</rdfs:label>
    </owl:Class>
    


    <!-- http://iec.ch/TC57/CIM100#Line -->

    <owl:Class rdf:about="http://iec.ch/TC57/CIM100#Line">
        <uml:id>EAID_43D9D2B8_DA1E_45c4_B99D_EC28FCAB742B</uml:id>
        <rdfs:comment>Contains equipment beyond a substation belonging to a power transmission line.</rdfs:comment>
        <rdfs:isDefinedBy rdf:resource="http://iec.ch/TC57/CIM100#Package_Wires"/>
        <rdfs:label>Line</rdfs:label>
    </owl:Class>
    


    <!-- http://iec.ch/TC57/CIM100#Minutes -->

    <owl:Class rdf:about="http://iec.ch/TC57/CIM100#Minutes">
        <uml:id>EAID_68F89418_6302_42a8_8177_5637B46ED1DB</uml:id>
        <rdfs:comment>Time in minutes.</rdfs:comment>
        <rdfs:isDefinedBy rdf:resource="http://iec.ch/TC57/CIM100#Package_Domain"/>
        <rdfs:label>Minutes</rdfs:label>
    </owl:Class>
    


    <!-- http://iec.ch/TC57/CIM100#Name -->

    <owl:Class rdf:about="http://iec.ch/TC57/CIM100#Name">
        <uml:id>EAID_D6F3DF4E_3363_48d2_AB61_7872E337C422</uml:id>
        <rdfs:comment>Any free text that name the object.</rdfs:comment>
        <rdfs:comment>The Name class provides the means to define any number of human readable  names for an object. A name is &lt;b&gt;not&lt;/b&gt; to be used for defining inter-object relationships. For inter-object relationships instead use the object identification &apos;mRID&apos;.</rdfs:comment>
        <rdfs:isDefinedBy rdf:resource="http://iec.ch/TC57/CIM100#Package_Core"/>
        <rdfs:label>Name</rdfs:label>
    </owl:Class>
    


    <!-- http://iec.ch/TC57/CIM100#NameType -->

    <owl:Class rdf:about="http://iec.ch/TC57/CIM100#NameType">
        <uml:id>EAID_666F94BF_13E3_4947_830F_3A2D4E7CC9FC</uml:id>
        <rdfs:comment>Description of the name type.</rdfs:comment>
        <rdfs:comment>Name of the name type.</rdfs:comment>
        <rdfs:comment>Type of name. Possible values for attribute &apos;name&apos; are implementation dependent but standard profiles may specify types. An enterprise may have multiple IT systems each having its own local name for the same object, e.g. a planning system may have different names from an EMS. An object may also have different names within the same IT system, e.g. localName as defined in CIM version 14. The definition from CIM14 is:
The localName is a human readable name of the object. It is a free text name local to a node in a naming hierarchy similar to a file directory structure. A power system related naming hierarchy may be: Substation, VoltageLevel, Equipment etc. Children of the same parent in such a hierarchy have names that typically are unique among them.</rdfs:comment>
        <rdfs:isDefinedBy rdf:resource="http://iec.ch/TC57/CIM100#Package_Core"/>
        <rdfs:label>NameType</rdfs:label>
    </owl:Class>
    


    <!-- http://iec.ch/TC57/CIM100#PSRType -->

    <owl:Class rdf:about="http://iec.ch/TC57/CIM100#PSRType">
        <uml:id>EAID_CF59539F_A910_4af6_A84D_A52BBA7300CB</uml:id>
        <rdfs:comment>Classifying instances of the same class, e.g. overhead and underground ACLineSegments. This classification mechanism is intended to provide flexibility outside the scope of this document, i.e. provide customisation that is non standard.</rdfs:comment>
        <rdfs:isDefinedBy rdf:resource="http://iec.ch/TC57/CIM100#Package_Core"/>
        <rdfs:label>PSRType</rdfs:label>
    </owl:Class>
    


    <!-- http://iec.ch/TC57/CIM100#PhaseCode -->

    <owl:Class rdf:about="http://iec.ch/TC57/CIM100#PhaseCode">
        <uml:id>EAID_3687AEED_A1B1_4557_899E_5985D184FCE9</uml:id>
        <rdfs:comment>An unordered enumeration of phase identifiers.  Allows designation of phases for both transmission and distribution equipment, circuits and loads.   The enumeration, by itself, does not describe how the phases are connected together or connected to ground.  Ground is not explicitly denoted as a phase.
Residential and small commercial loads are often served from single-phase, or split-phase, secondary circuits. For the example of s12N, phases 1 and 2 refer to hot wires that are 180 degrees out of phase, while N refers to the neutral wire. Through single-phase transformer connections, these secondary circuits may be served from one or two of the primary phases A, B, and C. For three-phase loads, use the A, B, C phase codes instead of s12N.
The integer values are from IEC 61968-9 to support revenue metering applications.</rdfs:comment>
        <rdfs:comment>Neutral phase.</rdfs:comment>
        <rdfs:comment>No phases specified.</rdfs:comment>
        <rdfs:comment>Phase A.</rdfs:comment>
        <rdfs:comment>Phase B.</rdfs:comment>
        <rdfs:comment>Phase C.</rdfs:comment>
        <rdfs:comment>Phases A and B.</rdfs:comment>
        <rdfs:comment>Phases A and C.</rdfs:comment>
        <rdfs:comment>Phases A and neutral.</rdfs:comment>
        <rdfs:comment>Phases A, B, C, and N.</rdfs:comment>
        <rdfs:comment>Phases A, B, and C.</rdfs:comment>
        <rdfs:comment>Phases A, B, and neutral.</rdfs:comment>
        <rdfs:comment>Phases A, C and neutral.</rdfs:comment>
        <rdfs:comment>Phases B and C.</rdfs:comment>
        <rdfs:comment>Phases B and neutral.</rdfs:comment>
        <rdfs:comment>Phases B, C, and neutral.</rdfs:comment>
        <rdfs:comment>Phases C and neutral.</rdfs:comment>
        <rdfs:comment>Secondary phase 1 and 2.</rdfs:comment>
        <rdfs:comment>Secondary phase 1 and neutral.</rdfs:comment>
        <rdfs:comment>Secondary phase 1.</rdfs:comment>
        <rdfs:comment>Secondary phase 2 and neutral.</rdfs:comment>
        <rdfs:comment>Secondary phase 2.</rdfs:comment>
        <rdfs:comment>Secondary phases 1, 2, and neutral.</rdfs:comment>
        <rdfs:comment>Two unknown non-neutral phases plus neutral.</rdfs:comment>
        <rdfs:comment>Two unknown non-neutral phases.</rdfs:comment>
        <rdfs:comment>Unknown non-neutral phase plus neutral.</rdfs:comment>
        <rdfs:comment>Unknown non-neutral phase.</rdfs:comment>
        <rdfs:isDefinedBy rdf:resource="http://iec.ch/TC57/CIM100#Package_Core"/>
        <rdfs:label>PhaseCode</rdfs:label>
    </owl:Class>
    


    <!-- http://iec.ch/TC57/CIM100#PowerSystemResource -->

    <owl:Class rdf:about="http://iec.ch/TC57/CIM100#PowerSystemResource">
        <uml:id>EAID_0340C084_3759_40cc_AAF2_386101DE842F</uml:id>
        <rdfs:comment>A power system resource (PSR) can be an item of equipment such as a switch, an equipment container containing many individual items of equipment such as a substation, or an organisational entity such as sub-control area. Power system resources can have measurements associated.</rdfs:comment>
        <rdfs:isDefinedBy rdf:resource="http://iec.ch/TC57/CIM100#Package_Core"/>
        <rdfs:label>PowerSystemResource</rdfs:label>
    </owl:Class>
    


    <!-- http://iec.ch/TC57/CIM100#ProtectedSwitch -->

    <owl:Class rdf:about="http://iec.ch/TC57/CIM100#ProtectedSwitch">
        <uml:id>EAID_BADE2A18_37F4_49bf_87BC_A087E4D2E4F7</uml:id>
        <rdfs:comment>A ProtectedSwitch is a switching device that can be operated by ProtectionEquipment.</rdfs:comment>
        <rdfs:comment>The maximum fault current a breaking device can break safely under prescribed conditions of use.</rdfs:comment>
        <rdfs:isDefinedBy rdf:resource="http://iec.ch/TC57/CIM100#Package_Wires"/>
        <rdfs:label>ProtectedSwitch</rdfs:label>
    </owl:Class>
    


    <!-- http://iec.ch/TC57/CIM100#Seconds -->

    <owl:Class rdf:about="http://iec.ch/TC57/CIM100#Seconds">
        <uml:id>EAID_A2008978_193D_4955_8102_599E43C7CFE4</uml:id>
        <rdfs:comment>Time, in seconds</rdfs:comment>
        <rdfs:comment>Time, in seconds.</rdfs:comment>
        <rdfs:isDefinedBy rdf:resource="http://iec.ch/TC57/CIM100#Package_Domain"/>
        <rdfs:label>Seconds</rdfs:label>
    </owl:Class>
    


    <!-- http://iec.ch/TC57/CIM100#String -->

    <owl:Class rdf:about="http://iec.ch/TC57/CIM100#String">
        <uml:id>EAID_E50DF78B_84CE_42e9_A275_A956DEF45490</uml:id>
        <rdfs:comment>A string consisting of a sequence of characters. The character encoding is UTF-8. The string length is unspecified and unlimited.</rdfs:comment>
        <rdfs:isDefinedBy rdf:resource="http://iec.ch/TC57/CIM100#Package_Domain"/>
        <rdfs:label>String</rdfs:label>
    </owl:Class>
    


    <!-- http://iec.ch/TC57/CIM100#SubGeographicalRegion -->

    <owl:Class rdf:about="http://iec.ch/TC57/CIM100#SubGeographicalRegion">
        <uml:id>EAID_D3CE44CA_5AED_484b_92A3_89F156425204</uml:id>
        <rdfs:comment>A subset of a geographical region of a power system network model.</rdfs:comment>
        <rdfs:isDefinedBy rdf:resource="http://iec.ch/TC57/CIM100#Package_Core"/>
        <rdfs:label>SubGeographicalRegion</rdfs:label>
    </owl:Class>
    


    <!-- http://iec.ch/TC57/CIM100#Substation -->

    <owl:Class rdf:about="http://iec.ch/TC57/CIM100#Substation">
        <uml:id>EAID_D8A14AC5_D17B_4d42_8F12_1B674E5D12D7</uml:id>
        <rdfs:comment>A collection of equipment for purposes other than generation or utilization, through which electric energy in bulk is passed for the purposes of switching or modifying its characteristics.</rdfs:comment>
        <rdfs:isDefinedBy rdf:resource="http://iec.ch/TC57/CIM100#Package_Core"/>
        <rdfs:label>Substation</rdfs:label>
    </owl:Class>
    


    <!-- http://iec.ch/TC57/CIM100#Switch -->

    <owl:Class rdf:about="http://iec.ch/TC57/CIM100#Switch">
        <uml:id>EAID_ACE2DDBB_536E_489a_A3A8_22589256302D</uml:id>
        <rdfs:comment>A generic device designed to close, or open, or both, one or more electric circuits.  All switches are two terminal devices including grounding switches. The ACDCTerminal.connected at the two sides of the switch shall not be considered for assessing switch connectivity, i.e. only Switch.open, .normalOpen and .locked are relevant.</rdfs:comment>
        <rdfs:comment>Branch is retained in the topological solution.  The flow through retained switches will normally be calculated in power flow.</rdfs:comment>
        <rdfs:comment>If true, the switch is locked. The resulting switch state is a combination of locked and Switch.open attributes as follows:
&lt;ul&gt;
	&lt;li&gt;locked=true and Switch.open=true. The resulting state is open and locked;&lt;/li&gt;
	&lt;li&gt;locked=false and Switch.open=true. The resulting state is open;&lt;/li&gt;
	&lt;li&gt;locked=false and Switch.open=false. The resulting state is closed.&lt;/li&gt;
&lt;/ul&gt;</rdfs:comment>
        <rdfs:comment>The attribute is used in cases when no Measurement for the status value is present. If the Switch has a status measurement the Discrete.normalValue is expected to match with the Switch.normalOpen.</rdfs:comment>
        <rdfs:comment>The attribute tells if the switch is considered open when used as input to topology processing.</rdfs:comment>
        <rdfs:comment>The date and time when the switch was last switched on.</rdfs:comment>
        <rdfs:comment>The maximum continuous current carrying capacity in amps governed by the device material and construction.
The attribute shall be a positive value.</rdfs:comment>
        <rdfs:comment>The switch on count since the switch was last reset or initialized.</rdfs:comment>
        <rdfs:isDefinedBy rdf:resource="http://iec.ch/TC57/CIM100#Package_Wires"/>
        <rdfs:label>Switch</rdfs:label>
    </owl:Class>
    


    <!-- http://iec.ch/TC57/CIM100#TapChanger -->

    <owl:Class rdf:about="http://iec.ch/TC57/CIM100#TapChanger">
        <uml:id>EAID_F43099C0_90EA_47f1_B038_EDE831744C07</uml:id>
        <rdfs:comment>For an LTC, the delay for initial tap changer operation (first step change).</rdfs:comment>
        <rdfs:comment>For an LTC, the delay for subsequent tap changer operation (second and later step changes).</rdfs:comment>
        <rdfs:comment>Highest possible tap step position, advance from neutral.
The attribute shall be greater than lowStep.</rdfs:comment>
        <rdfs:comment>Lowest possible tap step position, retard from neutral.</rdfs:comment>
        <rdfs:comment>Mechanism for changing transformer winding tap positions.</rdfs:comment>
        <rdfs:comment>Specifies the regulation status of the equipment.  True is regulating, false is not regulating.</rdfs:comment>
        <rdfs:comment>Specifies whether or not a TapChanger has load tap changing capabilities.</rdfs:comment>
        <rdfs:comment>Tap changer position.
Starting step for a steady state solution. Non integer values are allowed to support continuous tap variables. The reasons for continuous value are to support study cases where no discrete tap changer has yet been designed, a solution where a narrow voltage band forces the tap step to oscillate or to accommodate for a continuous solution as input.
The attribute shall be equal to or greater than lowStep and equal to or less than highStep.</rdfs:comment>
        <rdfs:comment>The neutral tap step position for this winding.
The attribute shall be equal to or greater than lowStep and equal or less than highStep.
It is the step position where the voltage is neutralU when the other terminals of the transformer are at the ratedU.  If there are other tap changers on the transformer those taps are kept constant at their neutralStep.</rdfs:comment>
        <rdfs:comment>The tap step position used in &quot;normal&quot; network operation for this winding. For a &quot;Fixed&quot; tap changer indicates the current physical tap setting.
The attribute shall be equal to or greater than lowStep and equal to or less than highStep.</rdfs:comment>
        <rdfs:comment>Voltage at which the winding operates at the neutral tap setting. It is the voltage at the terminal of the PowerTransformerEnd associated with the tap changer when all tap changers on the transformer are at their neutralStep position.  Normally neutralU of the tap changer is the same as ratedU of the PowerTransformerEnd, but it can differ in special cases such as when the tapping mechanism is separate from the winding more common on lower voltage transformers.
This attribute is not relevant for PhaseTapChangerAsymmetrical, PhaseTapChangerSymmetrical and PhaseTapChangerLinear.</rdfs:comment>
        <rdfs:isDefinedBy rdf:resource="http://iec.ch/TC57/CIM100#Package_Wires"/>
        <rdfs:label>TapChanger</rdfs:label>
    </owl:Class>
    


    <!-- http://iec.ch/TC57/CIM100#Terminal -->

    <owl:Class rdf:about="http://iec.ch/TC57/CIM100#Terminal">
        <uml:id>EAID_1A0F8321_5E77_4d68_BE29_B36FA31549DC</uml:id>
        <rdfs:comment>An AC electrical connection point to a piece of conducting equipment. Terminals are connected at physical connection points called connectivity nodes.</rdfs:comment>
        <rdfs:comment>Represents the normal network phasing condition. If the attribute is missing, three phases (ABC) shall be assumed, except for terminals of grounding classes (specializations of EarthFaultCompensator, GroundDisconnector, and Ground) which will be assumed to be N. Therefore, phase code ABCN is explicitly declared when needed, e.g. for star point grounding equipment.
The phase code on terminals connecting same ConnectivityNode or same TopologicalNode as well as for equipment between two terminals shall be consistent.</rdfs:comment>
        <rdfs:isDefinedBy rdf:resource="http://iec.ch/TC57/CIM100#Package_Core"/>
        <rdfs:label>Terminal</rdfs:label>
    </owl:Class>
    


    <!-- http://iec.ch/TC57/CIM100#Voltage -->

    <owl:Class rdf:about="http://iec.ch/TC57/CIM100#Voltage">
        <uml:id>EAID_233C330A_11B8_4705_879C_5497380F1D82</uml:id>
        <rdfs:comment>Electrical voltage, can be both AC and DC.</rdfs:comment>
        <rdfs:isDefinedBy rdf:resource="http://iec.ch/TC57/CIM100#Package_Domain"/>
        <rdfs:label>Voltage</rdfs:label>
    </owl:Class>
    


    <!-- http://iec.ch/TC57/CIM100#VoltageLevel -->

    <owl:Class rdf:about="http://iec.ch/TC57/CIM100#VoltageLevel">
        <uml:id>EAID_B147BAEA_7339_406b_A8C3_47F85EA0E82A</uml:id>
        <rdfs:comment>A collection of equipment at one common system voltage forming a switchgear. The equipment typically consists of breakers, busbars, instrumentation, control, regulation and protection devices as well as assemblies of all these.</rdfs:comment>
        <rdfs:comment>The bus bar&apos;s high voltage limit.
The limit applies to all equipment and nodes contained in a given VoltageLevel. It is not required that it is exchanged in pair with lowVoltageLimit. It is preferable to use operational VoltageLimit, which prevails, if present.</rdfs:comment>
        <rdfs:comment>The bus bar&apos;s low voltage limit.
The limit applies to all equipment and nodes contained in a given VoltageLevel. It is not required that it is exchanged in pair with highVoltageLimit. It is preferable to use operational VoltageLimit, which prevails, if present.</rdfs:comment>
        <rdfs:isDefinedBy rdf:resource="http://iec.ch/TC57/CIM100#Package_Core"/>
        <rdfs:label>VoltageLevel</rdfs:label>
    </owl:Class>
    


    <!-- http://langdale.com.au/2005/UML#Package -->

    <owl:Class rdf:about="http://langdale.com.au/2005/UML#Package"/>
    


    <!-- http://langdale.com.au/2005/UML#Stereotype -->

    <owl:Class rdf:about="http://langdale.com.au/2005/UML#Stereotype"/>
    


    <!-- 
    ///////////////////////////////////////////////////////////////////////////////////////
    //
    // Individuals
    //
    ///////////////////////////////////////////////////////////////////////////////////////
     -->

    


    <!-- http://iec.ch/TC57/CIM100#Package_AlternateModels -->

    <owl:NamedIndividual rdf:about="http://iec.ch/TC57/CIM100#Package_AlternateModels">
        <rdf:type rdf:resource="http://langdale.com.au/2005/UML#Package"/>
        <uml:id>EAPK_6FE4A0B4_282A_41c9_AEB3_11E1155C0840</uml:id>
        <rdfs:isDefinedBy rdf:resource="http://iec.ch/TC57/CIM100#Package_InfPart303"/>
        <rdfs:label>AlternateModels</rdfs:label>
    </owl:NamedIndividual>
    


    <!-- http://iec.ch/TC57/CIM100#Package_AssetInfo -->

    <owl:NamedIndividual rdf:about="http://iec.ch/TC57/CIM100#Package_AssetInfo">
        <rdf:type rdf:resource="http://langdale.com.au/2005/UML#Package"/>
        <uml:id>EAPK_DE6246EF_E71A_46da_BE5A_6A296C03DADD</uml:id>
        <rdfs:comment>This package is an extension of Assets package and contains the core information classes that support asset management and different network and work planning applications with specialized AssetInfo subclasses. They hold attributes that can be referenced by not only Asset-s or AssetModel-s but also by ConductingEquipment-s.</rdfs:comment>
        <rdfs:isDefinedBy rdf:resource="http://iec.ch/TC57/CIM100#Package_IEC61968"/>
        <rdfs:label>AssetInfo</rdfs:label>
    </owl:NamedIndividual>
    


    <!-- http://iec.ch/TC57/CIM100#Package_AssetMeas -->

    <owl:NamedIndividual rdf:about="http://iec.ch/TC57/CIM100#Package_AssetMeas">
        <rdf:type rdf:resource="http://langdale.com.au/2005/UML#Package"/>
        <uml:id>EAPK_3E9FBFDD_879C_4a70_862F_A3506421B44E</uml:id>
        <rdfs:comment>ClcSrc</rdfs:comment>
        <rdfs:isDefinedBy rdf:resource="http://iec.ch/TC57/CIM100#Package_IEC61968"/>
        <rdfs:label>AssetMeas</rdfs:label>
    </owl:NamedIndividual>
    


    <!-- http://iec.ch/TC57/CIM100#Package_Assets -->

    <owl:NamedIndividual rdf:about="http://iec.ch/TC57/CIM100#Package_Assets">
        <rdf:type rdf:resource="http://langdale.com.au/2005/UML#Package"/>
        <uml:id>EAPK_6518C7D6_2509_431c_AB1A_02EFAFCE7A51</uml:id>
        <rdfs:comment>This package contains the core information classes that support asset management applications that deal with the physical and lifecycle aspects of various network resources (as opposed to power system resource models defined in IEC61970::Wires package, which support network applications).</rdfs:comment>
        <rdfs:isDefinedBy rdf:resource="http://iec.ch/TC57/CIM100#Package_IEC61968"/>
        <rdfs:label>Assets</rdfs:label>
    </owl:NamedIndividual>
    


    <!-- http://iec.ch/TC57/CIM100#Package_AsynchronousMachineDynamics -->

    <owl:NamedIndividual rdf:about="http://iec.ch/TC57/CIM100#Package_AsynchronousMachineDynamics">
        <rdf:type rdf:resource="http://langdale.com.au/2005/UML#Package"/>
        <uml:id>EAPK_5D284657_A8B5_4b22_A1BE_60220021422B</uml:id>
        <rdfs:comment>An asynchronous machine model represents a (induction) generator or motor with no external connection to the rotor windings, e.g. a squirrel-cage induction machine. 
The interconnection with the electrical network equations can differ among simulation tools.  The program only needs to know the terminal to which this asynchronous machine is connected in order to establish the correct interconnection.  The interconnection with the motor’s equipment could also differ due to input and output signals required by standard models.
The asynchronous machine model is used to model wind generators type 1 and type 2.  For these, normal practice is to include the rotor flux transients and neglect the stator flux transients.</rdfs:comment>
        <rdfs:isDefinedBy rdf:resource="http://iec.ch/TC57/CIM100#Package_StandardModels"/>
        <rdfs:label>AsynchronousMachineDynamics</rdfs:label>
    </owl:NamedIndividual>
    


    <!-- http://iec.ch/TC57/CIM100#Package_AuxiliaryEquipment -->

    <owl:NamedIndividual rdf:about="http://iec.ch/TC57/CIM100#Package_AuxiliaryEquipment">
        <rdf:type rdf:resource="http://langdale.com.au/2005/UML#Package"/>
        <uml:id>EAPK_FF7DBBED_8801_4db6_A94B_3AE5E6FFFE95</uml:id>
        <rdfs:comment>Contains equipment which is not normal conducting equipment such as sensors, fault locators, and surge protectors.  These devices do not define power carrying topological connections as conducting equipment, but are associated to terminals of other conducting equipment.</rdfs:comment>
        <rdfs:isDefinedBy rdf:resource="http://iec.ch/TC57/CIM100#Package_Base"/>
        <rdfs:label>AuxiliaryEquipment</rdfs:label>
    </owl:NamedIndividual>
    


    <!-- http://iec.ch/TC57/CIM100#Package_Base -->

    <owl:NamedIndividual rdf:about="http://iec.ch/TC57/CIM100#Package_Base">
        <rdf:type rdf:resource="http://langdale.com.au/2005/UML#Package"/>
        <uml:id>EAPK_20A2C6D8_4765_466f_AD75_5E1B3CAF4E8D</uml:id>
        <rdfs:comment>An extension to the Core Package that, in association with the Terminal class, models Connectivity, that is the physical definition of how equipment is connected together. In addition it models Topology, that is the logical definition of how equipment is connected via closed switches. The Topology definition is independent of the other electrical characteristics.</rdfs:comment>
        <rdfs:comment>An extension to the Core and Topology package that models information on the electrical characteristics of Transmission and Distribution networks. This package is used by network applications such as State Estimation, Load Flow and Optimal Power Flow.</rdfs:comment>
        <rdfs:comment>An extension to the Core and Wires packages that models information for protection equipment such as relays. These entities are used within training simulators and distribution network fault location applications.</rdfs:comment>
        <rdfs:comment>Contains entities that describe dynamic measurement data exchanged between applications.</rdfs:comment>
        <rdfs:comment>Contains entities to model information used by Supervisory Control and Data Acquisition (SCADA) applications. Supervisory control supports operator control of equipment, such as opening or closing a breaker. Data acquisition gathers telemetered data from various sources.  The subtypes of the Telemetry entity deliberately match the UCA and IEC 61850 definitions. 
This package also supports alarm presentation but it is not expected to be used by other applications.</rdfs:comment>
        <rdfs:comment>Contains equipment which is not normal conducting equipment such as sensors, fault locators, and surge protectors.  These devices do not define power carrying topological connections as conducting equipment, but are associated to terminals of other conducting equipment.</rdfs:comment>
        <rdfs:comment>Contains the core PowerSystemResource and ConductingEquipment entities shared by all applications plus common collections of those entities. Not all applications require all the Core entities.  This package does not depend on any other package except the Domain package, but most of the other packages have associations and generalizations that depend on it.</rdfs:comment>
        <rdfs:comment>Content of the base CIM published as IEC 61970-301.</rdfs:comment>
        <rdfs:comment>Contingencies to be studied.</rdfs:comment>
        <rdfs:comment>State variables for analysis solutions such as powerflow.</rdfs:comment>
        <rdfs:comment>The ControlArea package models area specifications which can be used for a variety of purposes.  The package as a whole models potentially overlapping control area specifications for the purpose of actual generation control, load forecast area load capture, or powerflow based analysis.</rdfs:comment>
        <rdfs:comment>The domain package defines primitive datatypes that are used by classes in other packages. Stereotypes are used to describe the datatypes. The following stereotypes are defined:
&amp;lt;&amp;lt;enumeration&amp;gt;&amp;gt; A list of permissible constant values.
&amp;lt;&amp;lt;Primitive&amp;gt;&amp;gt; The most basic data types used to compose all other data types.
&amp;lt;&amp;lt;CIMDatatype&amp;gt;&amp;gt; A datatype that contains a value attribute, an optional unit of measure and a unit multiplier. The unit and multiplier may be specified as a static variable initialized to the allowed value.
&amp;lt;&amp;lt;Compound&amp;gt;&amp;gt; A composite of Primitive, enumeration, CIMDatatype or other Compound classes, as long as the Compound classes do not recurse.
For all datatypes both positive and negative values are allowed unless stated otherwise for a particular datatype.</rdfs:comment>
        <rdfs:comment>The equivalents package models equivalent networks.</rdfs:comment>
        <rdfs:comment>The package describes faults that may happen to conducting equipment, e.g. tree falling on a power line.</rdfs:comment>
        <rdfs:comment>This package contains example documentation diagrams not intended to be documented in IEC61970-301 with the rest of the normative packages.  The diagrams within this package are individually included in this document.</rdfs:comment>
        <rdfs:comment>This package contains model for direct current equipment and controls.</rdfs:comment>
        <rdfs:comment>This package contains packages that have information for Unit Commitment and Economic Dispatch of hydro and thermal generating units, Load Forecasting, Automatic Generation Control, and unit modeling for Training Simulation.</rdfs:comment>
        <rdfs:comment>This package describes diagram layout. This describes how objects are arranged in a coordinate system rather than how they are rendered.</rdfs:comment>
        <rdfs:comment>This package is responsible for modelling the energy consumers and the system load as curves and associated curve data. Special circumstances that may affect the load, such as seasons and day types, are also included here.

This information is used by Load Forecasting and Load Management.</rdfs:comment>
        <rdfs:comment>This package models a specification of limits associated with equipment and other operational entities.</rdfs:comment>
        <rdfs:comment>This package models configuration of ICCP required for bilateral exchanges.</rdfs:comment>
        <rdfs:isDefinedBy rdf:resource="http://iec.ch/TC57/CIM100#Package_IEC61970"/>
        <rdfs:label>Base</rdfs:label>
    </owl:NamedIndividual>
    


    <!-- http://iec.ch/TC57/CIM100#Package_CSC -->

    <owl:NamedIndividual rdf:about="http://iec.ch/TC57/CIM100#Package_CSC">
        <rdf:type rdf:resource="http://langdale.com.au/2005/UML#Package"/>
        <uml:id>EAPK_C29F669A_3BFC_42d7_9AB1_6F8337D8BA79</uml:id>
        <rdfs:isDefinedBy rdf:resource="http://iec.ch/TC57/CIM100#Package_InfHVDCDynamics"/>
        <rdfs:label>CSC</rdfs:label>
    </owl:NamedIndividual>
    


    <!-- http://iec.ch/TC57/CIM100#Package_Common -->

    <owl:NamedIndividual rdf:about="http://iec.ch/TC57/CIM100#Package_Common">
        <rdf:type rdf:resource="http://langdale.com.au/2005/UML#Package"/>
        <uml:id>EAPK_EE877146_D323_4066_AB0A_FCE1513C20A4</uml:id>
        <rdfs:comment>This package contains the information classes that support distribution management in general.</rdfs:comment>
        <rdfs:isDefinedBy rdf:resource="http://iec.ch/TC57/CIM100#Package_IEC61968"/>
        <rdfs:label>Common</rdfs:label>
    </owl:NamedIndividual>
    


    <!-- http://iec.ch/TC57/CIM100#Package_CongestionRevenueRights -->

    <owl:NamedIndividual rdf:about="http://iec.ch/TC57/CIM100#Package_CongestionRevenueRights">
        <rdf:type rdf:resource="http://langdale.com.au/2005/UML#Package"/>
        <uml:id>EAPK_183825EA_CEBE_4df4_902F_35523ED8F6D7</uml:id>
        <rdfs:comment>Congestion rent is a major, highly volatile charge currently faced by many participants in the LMP-based electrical energy markets. For this reason, the ISOs offer congestion revenue rights (CRR), also known as financial transmission rights or transmission congestion contracts. These are financial instruments that allow market participants to hedge against congestion charges when they schedule their generation, load and bilateral energy transactions.</rdfs:comment>
        <rdfs:isDefinedBy rdf:resource="http://iec.ch/TC57/CIM100#Package_MarketOperations"/>
        <rdfs:label>CongestionRevenueRights</rdfs:label>
    </owl:NamedIndividual>
    


    <!-- http://iec.ch/TC57/CIM100#Package_Contingency -->

    <owl:NamedIndividual rdf:about="http://iec.ch/TC57/CIM100#Package_Contingency">
        <rdf:type rdf:resource="http://langdale.com.au/2005/UML#Package"/>
        <uml:id>EAPK_5AFF4730_5CFE_48e6_961A_077143DE2082</uml:id>
        <rdfs:comment>Contingencies to be studied.</rdfs:comment>
        <rdfs:isDefinedBy rdf:resource="http://iec.ch/TC57/CIM100#Package_Base"/>
        <rdfs:label>Contingency</rdfs:label>
    </owl:NamedIndividual>
    


    <!-- http://iec.ch/TC57/CIM100#Package_ControlArea -->

    <owl:NamedIndividual rdf:about="http://iec.ch/TC57/CIM100#Package_ControlArea">
        <rdf:type rdf:resource="http://langdale.com.au/2005/UML#Package"/>
        <uml:id>EAPK_3A4198A2_F8DC_4ff1_B669_3064688AF4DD</uml:id>
        <rdfs:comment>The ControlArea package models area specifications which can be used for a variety of purposes.  The package as a whole models potentially overlapping control area specifications for the purpose of actual generation control, load forecast area load capture, or powerflow based analysis.</rdfs:comment>
        <rdfs:isDefinedBy rdf:resource="http://iec.ch/TC57/CIM100#Package_Base"/>
        <rdfs:label>ControlArea</rdfs:label>
    </owl:NamedIndividual>
    


    <!-- http://iec.ch/TC57/CIM100#Package_Core -->

    <owl:NamedIndividual rdf:about="http://iec.ch/TC57/CIM100#Package_Core">
        <rdf:type rdf:resource="http://langdale.com.au/2005/UML#Package"/>
        <uml:id>EAPK_6A503B72_6E15_4cd1_B92D_DDF6D14DBE29</uml:id>
        <rdfs:comment>Contains the core PowerSystemResource and ConductingEquipment entities shared by all applications plus common collections of those entities. Not all applications require all the Core entities.  This package does not depend on any other package except the Domain package, but most of the other packages have associations and generalizations that depend on it.</rdfs:comment>
        <rdfs:isDefinedBy rdf:resource="http://iec.ch/TC57/CIM100#Package_Base"/>
        <rdfs:label>Core</rdfs:label>
    </owl:NamedIndividual>
    


    <!-- http://iec.ch/TC57/CIM100#Package_Customers -->

    <owl:NamedIndividual rdf:about="http://iec.ch/TC57/CIM100#Package_Customers">
        <rdf:type rdf:resource="http://langdale.com.au/2005/UML#Package"/>
        <uml:id>EAPK_09D51F52_B40C_44cf_88CE_EB44B9E4EB9E</uml:id>
        <rdfs:comment>This package contains the core information classes that support customer billing applications.</rdfs:comment>
        <rdfs:isDefinedBy rdf:resource="http://iec.ch/TC57/CIM100#Package_IEC61968"/>
        <rdfs:label>Customers</rdfs:label>
    </owl:NamedIndividual>
    


    <!-- http://iec.ch/TC57/CIM100#Package_DC -->

    <owl:NamedIndividual rdf:about="http://iec.ch/TC57/CIM100#Package_DC">
        <rdf:type rdf:resource="http://langdale.com.au/2005/UML#Package"/>
        <uml:id>EAPK_6CA575E7_020B_40d8_B841_027BF8B51BE9</uml:id>
        <rdfs:comment>This package contains diagrams that will not be printed from the package context (within DC package), but you can and should use diagram placeholders in the 61970-301 template for documentation of examples and comments on modelling principles.</rdfs:comment>
        <rdfs:comment>This package contains instances used in instance diagrams for DC sample modelling.</rdfs:comment>
        <rdfs:comment>This package contains model for direct current equipment and controls.</rdfs:comment>
        <rdfs:isDefinedBy rdf:resource="http://iec.ch/TC57/CIM100#Package_Base"/>
        <rdfs:label>DC</rdfs:label>
    </owl:NamedIndividual>
    


    <!-- http://iec.ch/TC57/CIM100#Package_DER -->

    <owl:NamedIndividual rdf:about="http://iec.ch/TC57/CIM100#Package_DER">
        <rdf:type rdf:resource="http://langdale.com.au/2005/UML#Package"/>
        <uml:id>EAPK_9EF99BBA_443D_4383_9B81_5E50218D0209</uml:id>
        <rdfs:isDefinedBy rdf:resource="http://iec.ch/TC57/CIM100#Package_IEC61968"/>
        <rdfs:label>DER</rdfs:label>
    </owl:NamedIndividual>
    


    <!-- http://iec.ch/TC57/CIM100#Package_DiagramLayout -->

    <owl:NamedIndividual rdf:about="http://iec.ch/TC57/CIM100#Package_DiagramLayout">
        <rdf:type rdf:resource="http://langdale.com.au/2005/UML#Package"/>
        <uml:id>EAPK_BD6471E7_9929_4251_A731_BB65A6ABD2BF</uml:id>
        <rdfs:comment>This package describes diagram layout. This describes how objects are arranged in a coordinate system rather than how they are rendered.</rdfs:comment>
        <rdfs:isDefinedBy rdf:resource="http://iec.ch/TC57/CIM100#Package_Base"/>
        <rdfs:label>DiagramLayout</rdfs:label>
    </owl:NamedIndividual>
    


    <!-- http://iec.ch/TC57/CIM100#Package_DiscontinuousExcitationControlDynamics -->

    <owl:NamedIndividual rdf:about="http://iec.ch/TC57/CIM100#Package_DiscontinuousExcitationControlDynamics">
        <rdf:type rdf:resource="http://langdale.com.au/2005/UML#Package"/>
        <uml:id>EAPK_510FA576_60DA_4709_96D0_60C754D1875E</uml:id>
        <rdfs:comment>In certain system configurations, continuous excitation control with terminal voltage and power system stabilizing regulator input signals does not ensure that the potential of the excitation system for improving system stability is fully exploited. For these situations, discontinuous excitation control signals can be employed to enhance stability following large transient disturbances.
&lt;font color=&quot;#0f0f0f&quot;&gt;For additional information please refer to IEEE 421.5-2005, 12.&lt;/font&gt;</rdfs:comment>
        <rdfs:isDefinedBy rdf:resource="http://iec.ch/TC57/CIM100#Package_StandardModels"/>
        <rdfs:label>DiscontinuousExcitationControlDynamics</rdfs:label>
    </owl:NamedIndividual>
    


    <!-- http://iec.ch/TC57/CIM100#Package_DocIEC61968 -->

    <owl:NamedIndividual rdf:about="http://iec.ch/TC57/CIM100#Package_DocIEC61968">
        <rdf:type rdf:resource="http://langdale.com.au/2005/UML#Package"/>
        <uml:id>EAPK_5A92CCC8_D463_4af2_BDD1_EE82064CB8CD</uml:id>
        <rdfs:comment>This package contains only diagrams that are used in the introduction of IEC61968-11 and that should not be printed in its Clause 6 describing the UML model (due to the naming convention, this package will be considered as informative).
Other specifications may freely reuse some of these diagrams from their templates.</rdfs:comment>
        <rdfs:isDefinedBy rdf:resource="http://iec.ch/TC57/CIM100#Package_IEC61968"/>
        <rdfs:label>DocIEC61968</rdfs:label>
    </owl:NamedIndividual>
    


    <!-- http://iec.ch/TC57/CIM100#Package_Domain -->

    <owl:NamedIndividual rdf:about="http://iec.ch/TC57/CIM100#Package_Domain">
        <rdf:type rdf:resource="http://langdale.com.au/2005/UML#Package"/>
        <uml:id>EAPK_0134E45C_F32A_4522_A725_E07B0AE4CB57</uml:id>
        <rdfs:comment>The domain package defines primitive datatypes that are used by classes in other packages. Stereotypes are used to describe the datatypes. The following stereotypes are defined:
&amp;lt;&amp;lt;enumeration&amp;gt;&amp;gt; A list of permissible constant values.
&amp;lt;&amp;lt;Primitive&amp;gt;&amp;gt; The most basic data types used to compose all other data types.
&amp;lt;&amp;lt;CIMDatatype&amp;gt;&amp;gt; A datatype that contains a value attribute, an optional unit of measure and a unit multiplier. The unit and multiplier may be specified as a static variable initialized to the allowed value.
&amp;lt;&amp;lt;Compound&amp;gt;&amp;gt; A composite of Primitive, enumeration, CIMDatatype or other Compound classes, as long as the Compound classes do not recurse.
For all datatypes both positive and negative values are allowed unless stated otherwise for a particular datatype.</rdfs:comment>
        <rdfs:isDefinedBy rdf:resource="http://iec.ch/TC57/CIM100#Package_Base"/>
        <rdfs:label>Domain</rdfs:label>
    </owl:NamedIndividual>
    


    <!-- http://iec.ch/TC57/CIM100#Package_Dynamics -->

    <owl:NamedIndividual rdf:about="http://iec.ch/TC57/CIM100#Package_Dynamics">
        <rdf:type rdf:resource="http://langdale.com.au/2005/UML#Package"/>
        <uml:id>EAPK_A71B9185_6D48_40f4_B618_485C08C4F269</uml:id>
        <rdfs:comment>Examples illustrating the use of dynamic behaviour models are given in the following diagrams.</rdfs:comment>
        <rdfs:comment>The CIM dynamic model definitions reflect the most common IEEE or, in the case of wind models, IEC, representations of models as well as models included in some of the transient stability software widely used by utilities. 
These dynamic models are intended to ensure interoperability between different vendors’ software products currently in use by electric utility energy companies, utilities, Transmission System Operators (TSOs), Regional Transmission Organizations (RTOs), and Independent System Operators (ISOs).  It is important to note that each vendor is free to select its own internal implementation of these models.  Differences in vendor results, as long as they are within accepted engineering practice, caused by different internal representations, are acceptable.
Unless explicitly stated otherwise, the following modelling conventions are followed:
- limited integrators are of the non-windup type;
- it shall be possible to enter a time constant of zero (where it makes sense).</rdfs:comment>
        <rdfs:comment>This subclause contains standard dynamic model specifications grouped into packages by standard function block (type of equipment being modelled).
In the CIM, standard dynamic models are expressed by means of a class named with the standard model name and attributes reflecting each of the parameters necessary to describe the behaviour of an instance of the standard model.</rdfs:comment>
        <rdfs:comment>This subclause contains user-defined dynamic model classes to support the exchange of both proprietary and explicitly defined user-defined models.  
&lt;u&gt;Proprietary models&lt;/u&gt; represent behaviour which, while not defined by a standard model class, is mutually understood by the sending and receiving applications based on the name passed in the .name attribute of the appropriate xxxUserDefined class.  Proprietary model parameters are passed as general attributes using as many instances of the ProprietaryParameterDynamics class as there are parameters.
&lt;u&gt;Explicitly defined models&lt;/u&gt; describe dynamic behaviour in detail in terms of control blocks and their input and output signals.  Note that the classes to support explicitly defined modelling are not currently defined - it is future work intended to also be supported by the family of xxxUserDefined classes.
Both types of user-defined models use the family of xxxUserDefined classes, which allow a user-defined model to be used:
- as the model for an individual standard function block (such as a turbine-governor or power system stabilizer) in a standard interconnection model whose other function blocks could be either standard or user-defined.  For an illustration of this form of usage for a proprietary model, see the ExampleFunctionBlockProprietaryModel diagram in subclause 5.5.
- as the complete representation of a dynamic behaviour model (for an entire synchronous machine, for example) where standard function blocks and standard interconnections are not used at all. For an illustration of this form of usage for a proprietary model, see the ExampleCompleteProprietaryModel diagram in subclause 5.5.</rdfs:comment>
        <rdfs:comment>This subclause describes the standard interconnections for various types of equipment. These interconnections are understood by the application programs and can be identified based on the presence of one of the key classes with a relationship to the static power flow model: SynchronousMachineDynamics, AsynchronousMachineDynamics, EnergyConsumerDynamics or WindTurbineType3or4Dynamics. 
The relationships between classes expressed in the interconnection diagrams are intended to support dynamic behaviour described by either standard models or user-defined models.
In the interconnection diagrams, boxes which are black in colour represent function blocks whose functionality can be provided by one of many standard models or by a user-defined model. Blue boxes represent specific standard models.  A dashed box means that the function block or specific standard model is optional.</rdfs:comment>
        <rdfs:isDefinedBy rdf:resource="http://iec.ch/TC57/CIM100#Package_IEC61970"/>
        <rdfs:label>Dynamics</rdfs:label>
    </owl:NamedIndividual>
    


    <!-- http://iec.ch/TC57/CIM100#Package_EnergyArea -->

    <owl:NamedIndividual rdf:about="http://iec.ch/TC57/CIM100#Package_EnergyArea">
        <rdf:type rdf:resource="http://langdale.com.au/2005/UML#Package"/>
        <uml:id>EAPK_1B32681C_A297_4a09_9DFC_C7C1C07AACFC</uml:id>
        <rdfs:isDefinedBy rdf:resource="http://iec.ch/TC57/CIM100#Package_InfIEC61970"/>
        <rdfs:label>EnergyArea</rdfs:label>
    </owl:NamedIndividual>
    


    <!-- http://iec.ch/TC57/CIM100#Package_EnvDomain -->

    <owl:NamedIndividual rdf:about="http://iec.ch/TC57/CIM100#Package_EnvDomain">
        <rdf:type rdf:resource="http://langdale.com.au/2005/UML#Package"/>
        <uml:id>EAPK_02E1C073_74BE_457f_B0A6_FC8AE00A1681</uml:id>
        <rdfs:isDefinedBy rdf:resource="http://iec.ch/TC57/CIM100#Package_Environmental"/>
        <rdfs:label>EnvDomain</rdfs:label>
    </owl:NamedIndividual>
    


    <!-- http://iec.ch/TC57/CIM100#Package_Environmental -->

    <owl:NamedIndividual rdf:about="http://iec.ch/TC57/CIM100#Package_Environmental">
        <rdf:type rdf:resource="http://langdale.com.au/2005/UML#Package"/>
        <uml:id>EAPK_4F65E356_1F62_4781_A4B2_857643E94ADB</uml:id>
        <rdfs:isDefinedBy rdf:resource="http://iec.ch/TC57/CIM100#Package_IEC62325"/>
        <rdfs:label>Environmental</rdfs:label>
    </owl:NamedIndividual>
    


    <!-- http://iec.ch/TC57/CIM100#Package_Equivalents -->

    <owl:NamedIndividual rdf:about="http://iec.ch/TC57/CIM100#Package_Equivalents">
        <rdf:type rdf:resource="http://langdale.com.au/2005/UML#Package"/>
        <uml:id>EAPK_32F75AB7_7839_4933_BE8C_F162A464FE41</uml:id>
        <rdfs:comment>The equivalents package models equivalent networks.</rdfs:comment>
        <rdfs:isDefinedBy rdf:resource="http://iec.ch/TC57/CIM100#Package_Base"/>
        <rdfs:label>Equivalents</rdfs:label>
    </owl:NamedIndividual>
    


    <!-- http://iec.ch/TC57/CIM100#Package_ExcitationSystemDynamics -->

    <owl:NamedIndividual rdf:about="http://iec.ch/TC57/CIM100#Package_ExcitationSystemDynamics">
        <rdf:type rdf:resource="http://langdale.com.au/2005/UML#Package"/>
        <uml:id>EAPK_829F67E7_F698_4aa7_95C2_13C616AB6B78</uml:id>
        <rdfs:comment>The excitation system model provides the field voltage (&lt;i&gt;Efd&lt;/i&gt;) for a synchronous machine model.  It is linked to a specific generator (synchronous machine). 
The representation of all limits used by the models (not including IEEE standard models) shall comply with the representation defined in the Annex E of the IEEE 421.5-2005, unless specified differently in the documentation of the model.
The parameters are different for each excitation system model; the same parameter name can have different meaning in different models.</rdfs:comment>
        <rdfs:isDefinedBy rdf:resource="http://iec.ch/TC57/CIM100#Package_StandardModels"/>
        <rdfs:label>ExcitationSystemDynamics</rdfs:label>
    </owl:NamedIndividual>
    


    <!-- http://iec.ch/TC57/CIM100#Package_ExternalInputs -->

    <owl:NamedIndividual rdf:about="http://iec.ch/TC57/CIM100#Package_ExternalInputs">
        <rdf:type rdf:resource="http://langdale.com.au/2005/UML#Package"/>
        <uml:id>EAPK_60C81C80_9E0F_4484_95EC_4DBA653914B7</uml:id>
        <rdfs:comment>Inputs to the market system from external sources.</rdfs:comment>
        <rdfs:isDefinedBy rdf:resource="http://iec.ch/TC57/CIM100#Package_MarketSystem"/>
        <rdfs:label>ExternalInputs</rdfs:label>
    </owl:NamedIndividual>
    


    <!-- http://iec.ch/TC57/CIM100#Package_Faults -->

    <owl:NamedIndividual rdf:about="http://iec.ch/TC57/CIM100#Package_Faults">
        <rdf:type rdf:resource="http://langdale.com.au/2005/UML#Package"/>
        <uml:id>EAPK_59BC9A2E_B8E4_4c5f_B1D8_2C6502296346</uml:id>
        <rdfs:comment>The package describes faults that may happen to conducting equipment, e.g. tree falling on a power line.</rdfs:comment>
        <rdfs:isDefinedBy rdf:resource="http://iec.ch/TC57/CIM100#Package_Base"/>
        <rdfs:label>Faults</rdfs:label>
    </owl:NamedIndividual>
    


    <!-- http://iec.ch/TC57/CIM100#Package_Feeder -->

    <owl:NamedIndividual rdf:about="http://iec.ch/TC57/CIM100#Package_Feeder">
        <rdf:type rdf:resource="http://langdale.com.au/2005/UML#Package"/>
        <uml:id>EAPK_4CD4EBB9_E213_44df_9BD9_20ECAE4160A8</uml:id>
        <rdfs:isDefinedBy rdf:resource="http://iec.ch/TC57/CIM100#Package_InfIEC61970"/>
        <rdfs:label>Feeder</rdfs:label>
    </owl:NamedIndividual>
    


    <!-- http://iec.ch/TC57/CIM100#Package_Generation -->

    <owl:NamedIndividual rdf:about="http://iec.ch/TC57/CIM100#Package_Generation">
        <rdf:type rdf:resource="http://langdale.com.au/2005/UML#Package"/>
        <uml:id>EAPK_6B50A1FD_22E9_4abc_B0B7_F46BBD8B33AE</uml:id>
        <rdfs:comment>The GenerationTrainingSimululation package contains prime movers, such as turbines and boilers, which are needed for simulation and educational purposes.</rdfs:comment>
        <rdfs:comment>The production package is responsible for classes which describe various kinds of generators. These classes also provide production costing information which is used to economically allocate demand among committed units and calculate reserve quantities.</rdfs:comment>
        <rdfs:comment>This package contains packages that have information for Unit Commitment and Economic Dispatch of hydro and thermal generating units, Load Forecasting, Automatic Generation Control, and unit modeling for Training Simulation.</rdfs:comment>
        <rdfs:isDefinedBy rdf:resource="http://iec.ch/TC57/CIM100#Package_Base"/>
        <rdfs:label>Generation</rdfs:label>
    </owl:NamedIndividual>
    


    <!-- http://iec.ch/TC57/CIM100#Package_GenerationTrainingSimulation -->

    <owl:NamedIndividual rdf:about="http://iec.ch/TC57/CIM100#Package_GenerationTrainingSimulation">
        <rdf:type rdf:resource="http://langdale.com.au/2005/UML#Package"/>
        <uml:id>EAPK_D3C36399_A1D6_4491_A975_06B94A5A1258</uml:id>
        <rdfs:comment>The GenerationTrainingSimululation package contains prime movers, such as turbines and boilers, which are needed for simulation and educational purposes.</rdfs:comment>
        <rdfs:isDefinedBy rdf:resource="http://iec.ch/TC57/CIM100#Package_Generation"/>
        <rdfs:label>GenerationTrainingSimulation</rdfs:label>
    </owl:NamedIndividual>
    


    <!-- http://iec.ch/TC57/CIM100#Package_GenericDataSet -->

    <owl:NamedIndividual rdf:about="http://iec.ch/TC57/CIM100#Package_GenericDataSet">
        <rdf:type rdf:resource="http://langdale.com.au/2005/UML#Package"/>
        <uml:id>EAPK_8FF85768_B48A_4be5_9113_0DD28B347634</uml:id>
        <rdfs:comment>Contains classes used for generic dataset modelling.</rdfs:comment>
        <rdfs:isDefinedBy rdf:resource="http://iec.ch/TC57/CIM100#Package_Part303"/>
        <rdfs:label>GenericDataSet</rdfs:label>
    </owl:NamedIndividual>
    


    <!-- http://iec.ch/TC57/CIM100#Package_HVDCDynamics -->

    <owl:NamedIndividual rdf:about="http://iec.ch/TC57/CIM100#Package_HVDCDynamics">
        <rdf:type rdf:resource="http://langdale.com.au/2005/UML#Package"/>
        <uml:id>EAPK_7C62349B_D355_4ba0_BE12_91068427292A</uml:id>
        <rdfs:comment>High voltage direct current (HVDC) models.</rdfs:comment>
        <rdfs:isDefinedBy rdf:resource="http://iec.ch/TC57/CIM100#Package_StandardModels"/>
        <rdfs:label>HVDCDynamics</rdfs:label>
    </owl:NamedIndividual>
    


    <!-- http://iec.ch/TC57/CIM100#Package_ICCPConfiguration -->

    <owl:NamedIndividual rdf:about="http://iec.ch/TC57/CIM100#Package_ICCPConfiguration">
        <rdf:type rdf:resource="http://langdale.com.au/2005/UML#Package"/>
        <uml:id>EAPK_423B82DE_E83D_40a8_A4C8_8EA08513C297</uml:id>
        <rdfs:comment>This package models configuration of ICCP required for bilateral exchanges.</rdfs:comment>
        <rdfs:isDefinedBy rdf:resource="http://iec.ch/TC57/CIM100#Package_Base"/>
        <rdfs:label>ICCPConfiguration</rdfs:label>
    </owl:NamedIndividual>
    


    <!-- http://iec.ch/TC57/CIM100#Package_IEC61968 -->

    <owl:NamedIndividual rdf:about="http://iec.ch/TC57/CIM100#Package_IEC61968">
        <rdf:type rdf:resource="http://langdale.com.au/2005/UML#Package"/>
        <uml:id>EAPK_F020E775_00E6_4716_A216_BDD5E2FF16F5</uml:id>
        <rdfs:comment>The IEC 61968 subpackages of the CIM are developed, standardized and maintained by the UCA community including its working groups and task forces.
Currently, normative parts of the model support the needs of information exchange defined in IEC 61968-3, IEC 61968-4, IEC 61968-5, IEC 61968-6, IEC 61968-8, IEC 61968-9 and in IEC 61968-13.</rdfs:comment>
        <rdfs:comment>This package and its subpackages contain informative (unstable) elements of the model, expected to evolve a lot or to be removed, and not published as IEC document yet. Some portions of it will be reworked and moved to normative packages as the need arises, and some portions may be removed.
WG14 does not generate documentation for this informative portion of the model.</rdfs:comment>
        <rdfs:comment>This package contains only diagrams that are used in the introduction of IEC61968-11 and that should not be printed in its Clause 6 describing the UML model (due to the naming convention, this package will be considered as informative).
Other specifications may freely reuse some of these diagrams from their templates.</rdfs:comment>
        <rdfs:comment>This package contains the core information classes that support asset management applications that deal with the physical and lifecycle aspects of various network resources (as opposed to power system resource models defined in IEC61970::Wires package, which support network applications).</rdfs:comment>
        <rdfs:comment>This package contains the core information classes that support customer billing applications.</rdfs:comment>
        <rdfs:comment>This package contains the core information classes that support end device applications with specialized classes for metering and premises area network devices, and remote reading functions. These classes are generally associated with the point where a service is delivered to the customer.</rdfs:comment>
        <rdfs:comment>This package contains the core information classes that support operations and outage management applications.</rdfs:comment>
        <rdfs:comment>This package contains the core information classes that support work management and network extension planning applications.</rdfs:comment>
        <rdfs:comment>This package contains the information classes that support distribution management in general.</rdfs:comment>
        <rdfs:comment>This package is an extension of Assets package and contains the core information classes that support asset management and different network and work planning applications with specialized AssetInfo subclasses. They hold attributes that can be referenced by not only Asset-s or AssetModel-s but also by ConductingEquipment-s.</rdfs:comment>
        <rdfs:comment>This package is an extension of the Metering package and contains the information classes that support specialised applications such as demand-side management using load control equipment. These classes are generally associated with the point where a service is delivered to the customer.</rdfs:comment>
        <rdfs:comment>This package is an extension of the Metering package and contains the information classes that support specialised applications such as prepayment metering. These classes are generally associated with the collection and control of revenue from the customer for a delivered service.</rdfs:comment>
        <rdfs:isDefinedBy rdf:resource="http://iec.ch/TC57/CIM100#Package_TC57CIM"/>
        <rdfs:label>IEC61968</rdfs:label>
    </owl:NamedIndividual>
    


    <!-- http://iec.ch/TC57/CIM100#Package_IEC61970 -->

    <owl:NamedIndividual rdf:about="http://iec.ch/TC57/CIM100#Package_IEC61970">
        <rdf:type rdf:resource="http://langdale.com.au/2005/UML#Package"/>
        <uml:id>EAPK_21D32832_FF64_4213_B81C_55ACE35EEBFF</uml:id>
        <rdfs:comment>Content of the base CIM published as IEC 61970-301.</rdfs:comment>
        <rdfs:comment>The CIM dynamic model definitions reflect the most common IEEE or, in the case of wind models, IEC, representations of models as well as models included in some of the transient stability software widely used by utilities. 
These dynamic models are intended to ensure interoperability between different vendors’ software products currently in use by electric utility energy companies, utilities, Transmission System Operators (TSOs), Regional Transmission Organizations (RTOs), and Independent System Operators (ISOs).  It is important to note that each vendor is free to select its own internal implementation of these models.  Differences in vendor results, as long as they are within accepted engineering practice, caused by different internal representations, are acceptable.
Unless explicitly stated otherwise, the following modelling conventions are followed:
- limited integrators are of the non-windup type;
- it shall be possible to enter a time constant of zero (where it makes sense).</rdfs:comment>
        <rdfs:comment>This package and its subpackages contain informative (unstable) elements of the model, expected to evolve a lot or to be removed, and not published as IEC document yet. Some portions of it will be reworked and moved to normative packages as the need arises, and some portions may be removed.
WG13 does not generate documentation for this informative portion of the model.</rdfs:comment>
        <rdfs:comment>Top package for IEC 61970.</rdfs:comment>
        <rdfs:isDefinedBy rdf:resource="http://iec.ch/TC57/CIM100#Package_TC57CIM"/>
        <rdfs:label>IEC61970</rdfs:label>
    </owl:NamedIndividual>
    


    <!-- http://iec.ch/TC57/CIM100#Package_IEC62325 -->

    <owl:NamedIndividual rdf:about="http://iec.ch/TC57/CIM100#Package_IEC62325">
        <rdf:type rdf:resource="http://langdale.com.au/2005/UML#Package"/>
        <uml:id>EAPK_7E17978D_C3C1_419d_ACA8_48AC1E690B51</uml:id>
        <rdfs:comment>The IEC 62325 subpackages of the CIM are developed, standardized and maintained by the IEC TC57.</rdfs:comment>
        <rdfs:comment>This package contains all core CIM Market Extensions required for market management systems.</rdfs:comment>
        <rdfs:comment>This package contains all core CIM Market Extensions required for market operations systems.</rdfs:comment>
        <rdfs:comment>This package contains the common objects shared by MarketManagement, MarketOperations and Environmental packages.</rdfs:comment>
        <rdfs:isDefinedBy rdf:resource="http://iec.ch/TC57/CIM100#Package_TC57CIM"/>
        <rdfs:label>IEC62325</rdfs:label>
    </owl:NamedIndividual>
    


    <!-- http://iec.ch/TC57/CIM100#Package_InfAssetInfo -->

    <owl:NamedIndividual rdf:about="http://iec.ch/TC57/CIM100#Package_InfAssetInfo">
        <rdf:type rdf:resource="http://langdale.com.au/2005/UML#Package"/>
        <uml:id>EAPK_64B41E47_775F_4ec7_A068_4204B9810D7E</uml:id>
        <rdfs:isDefinedBy rdf:resource="http://iec.ch/TC57/CIM100#Package_InfIEC61968"/>
        <rdfs:label>InfAssetInfo</rdfs:label>
    </owl:NamedIndividual>
    


    <!-- http://iec.ch/TC57/CIM100#Package_InfAssets -->

    <owl:NamedIndividual rdf:about="http://iec.ch/TC57/CIM100#Package_InfAssets">
        <rdf:type rdf:resource="http://langdale.com.au/2005/UML#Package"/>
        <uml:id>EAPK_E9801E7A_D817_48da_B8F0_8328EA11731F</uml:id>
        <rdfs:comment>The package is used to define asset-level models for objects. Assets may be comprised of other assets and may have relationships to other assets. Assets also have owners and values. Assets may also have a relationship to a PowerSystemResource in the Wires model.

TODO: The following has been copied from a very old version of draft Part 11, so the references are wrong, but we store the knowledge here to reuse later:
&quot;Assets are the basic units which define a physical infrastructure. PowerSystemResources are logical objects meaningful to operations which are constructed from one or more Assets, although PowerSystemResources are not required to specifiy their component Assets.
The Asset package is comprosed of several packages. The key concepts of an Asset are as follows:
&lt;ul&gt;
	&lt;li&gt;Assets can have names, through inheritance to the Naming package&lt;/li&gt;
	&lt;li&gt;Assets are physical entities which have a lifecycle&lt;/li&gt;
	&lt;li&gt;One or more assets can be associated to create a PowerSystemResource&lt;/li&gt;
	&lt;li&gt;Assets can be grouped (aggregated) with other Assets&lt;/li&gt;
	&lt;li&gt;Assets are typically either &apos;point&apos; or &apos;linear&apos; assets, which relate to physical geometry&lt;/li&gt;
	&lt;li&gt;Assets have a close relationship to Work as a consequence of their lifecycle&lt;/li&gt;
&lt;/ul&gt;
The following sections describe the packages in the Assets package.
The AssetBasics package defines the relationship between Asset and other classes, such as Organization, PowerSystemResource and Document.
Point assets are those assets whose physical location can be described in terms of a single coordinate, such as a pole or a switch.
Linear assets are those assets whose physical location is best described in terms of a line, plyline or polygon.
Asset work triggers are used to determine when inspection and/or maintenance are required for assets&quot;.</rdfs:comment>
        <rdfs:isDefinedBy rdf:resource="http://iec.ch/TC57/CIM100#Package_InfIEC61968"/>
        <rdfs:label>InfAssets</rdfs:label>
    </owl:NamedIndividual>
    


    <!-- http://iec.ch/TC57/CIM100#Package_InfAvailabilityPlans -->

    <owl:NamedIndividual rdf:about="http://iec.ch/TC57/CIM100#Package_InfAvailabilityPlans">
        <rdf:type rdf:resource="http://langdale.com.au/2005/UML#Package"/>
        <uml:id>EAPK_F2BCFC39_B533_4a36_B116_464719DAC88A</uml:id>
        <rdfs:comment>Contains the planned schedules for equipment availability, primarily intended for future studies.</rdfs:comment>
        <rdfs:isDefinedBy rdf:resource="http://iec.ch/TC57/CIM100#Package_InfIEC61970"/>
        <rdfs:label>InfAvailabilityPlans</rdfs:label>
    </owl:NamedIndividual>
    


    <!-- http://iec.ch/TC57/CIM100#Package_InfCommon -->

    <owl:NamedIndividual rdf:about="http://iec.ch/TC57/CIM100#Package_InfCommon">
        <rdf:type rdf:resource="http://langdale.com.au/2005/UML#Package"/>
        <uml:id>EAPK_3E8BAB84_78CC_4863_9826_B143EDCFFBB1</uml:id>
        <rdfs:comment>This package contains functions common for distribution management.</rdfs:comment>
        <rdfs:isDefinedBy rdf:resource="http://iec.ch/TC57/CIM100#Package_InfIEC61968"/>
        <rdfs:label>InfCommon</rdfs:label>
    </owl:NamedIndividual>
    


    <!-- http://iec.ch/TC57/CIM100#Package_InfCongestionRevenueRights -->

    <owl:NamedIndividual rdf:about="http://iec.ch/TC57/CIM100#Package_InfCongestionRevenueRights">
        <rdf:type rdf:resource="http://langdale.com.au/2005/UML#Package"/>
        <uml:id>EAPK_78694811_BA98_46d0_8240_F7474E3AA214</uml:id>
        <rdfs:isDefinedBy rdf:resource="http://iec.ch/TC57/CIM100#Package_InfIEC62325"/>
        <rdfs:label>InfCongestionRevenueRights</rdfs:label>
    </owl:NamedIndividual>
    


    <!-- http://iec.ch/TC57/CIM100#Package_InfCustomers -->

    <owl:NamedIndividual rdf:about="http://iec.ch/TC57/CIM100#Package_InfCustomers">
        <rdf:type rdf:resource="http://langdale.com.au/2005/UML#Package"/>
        <uml:id>EAPK_74D05A57_F7EC_4a08_8CF8_969FC5C422CA</uml:id>
        <rdfs:comment>The package is used to define detailed customer models.</rdfs:comment>
        <rdfs:isDefinedBy rdf:resource="http://iec.ch/TC57/CIM100#Package_InfIEC61968"/>
        <rdfs:label>InfCustomers</rdfs:label>
    </owl:NamedIndividual>
    


    <!-- http://iec.ch/TC57/CIM100#Package_InfDomain -->

    <owl:NamedIndividual rdf:about="http://iec.ch/TC57/CIM100#Package_InfDomain">
        <rdf:type rdf:resource="http://langdale.com.au/2005/UML#Package"/>
        <uml:id>EAPK_B9EE7EDA_E0CD_4c34_8FDC_5888CE1D50E0</uml:id>
        <rdfs:isDefinedBy rdf:resource="http://iec.ch/TC57/CIM100#Package_InfIEC62325"/>
        <rdfs:label>InfDomain</rdfs:label>
    </owl:NamedIndividual>
    


    <!-- http://iec.ch/TC57/CIM100#Package_InfERPSupport -->

    <owl:NamedIndividual rdf:about="http://iec.ch/TC57/CIM100#Package_InfERPSupport">
        <rdf:type rdf:resource="http://langdale.com.au/2005/UML#Package"/>
        <uml:id>EAPK_2548BF66_BC1B_4349_9BAA_BAC4204952F4</uml:id>
        <rdfs:comment>The package contains portions of the model defined byEnterprise Resource Planning (ERP) standards like those proposed by the Open Applications Group (OAG). It is provided to facilitate integration among electric utility applications (CIM) and enterprise resource planning (ERP) applications (as defined by OAG). Rather than inventing new CIM classes that accomplish similar functionality as in existing ERP models, the preferred approach is to use and extend ERP classes as appropriate in other packages.
If a model other that the OAG standard is used as a basis for ERP integration, the utility classes labeld &quot;Erp...&quot; should be associated with the appropriate classes of that standard. In fact, definitions of &quot;Erp...&quot; classes are based on OAG Nouns to facilitate this process.

TODO: The following has been copied from a very old version of draft Part 11, so the references are wrong, but we store the knowledge here to reuse later:
&quot;The Enterprise Resource Planning (ERP) Support Package contains portions of the model defined by ERP standards like those proposed by the Open Applications Group (OAG). This package is provided to facilitate integration among electric utility applications (CIM) and enterprise resource planning (ERP) applications (OAG). Rather than inventing new CIM classes that accomplish similar functionality as in existing ERP models, the preferred approach is to use and extend ERP classes as appropriate in other packages.
If a model other that the OAG standard is used as a basis for ERP integration, the utility classes labeled &quot;Erp...&quot; should be associated with the appropriate classes of that standard&quot;.</rdfs:comment>
        <rdfs:isDefinedBy rdf:resource="http://iec.ch/TC57/CIM100#Package_InfIEC61968"/>
        <rdfs:label>InfERPSupport</rdfs:label>
    </owl:NamedIndividual>
    


    <!-- http://iec.ch/TC57/CIM100#Package_InfEnergyScheduling -->

    <owl:NamedIndividual rdf:about="http://iec.ch/TC57/CIM100#Package_InfEnergyScheduling">
        <rdf:type rdf:resource="http://langdale.com.au/2005/UML#Package"/>
        <uml:id>EAPK_A08EDD43_307E_49c0_8A6C_667ACCD9CAC1</uml:id>
        <rdfs:comment>This package provides the capability to schedule and account for transactions for the exchange of electric power between companies. It includes transations for megawatts which are generated, consumed, lost, passed through, sold and purchased. These classes are used by Accounting and Billing for Energy, Generation Capacity, Transmission, and Ancillary Services.</rdfs:comment>
        <rdfs:isDefinedBy rdf:resource="http://iec.ch/TC57/CIM100#Package_InfIEC62325"/>
        <rdfs:label>InfEnergyScheduling</rdfs:label>
    </owl:NamedIndividual>
    


    <!-- http://iec.ch/TC57/CIM100#Package_InfExternalInputs -->

    <owl:NamedIndividual rdf:about="http://iec.ch/TC57/CIM100#Package_InfExternalInputs">
        <rdf:type rdf:resource="http://langdale.com.au/2005/UML#Package"/>
        <uml:id>EAPK_E1115CC9_35BB_493e_A4C4_B7E41F25A0AC</uml:id>
        <rdfs:isDefinedBy rdf:resource="http://iec.ch/TC57/CIM100#Package_InfIEC62325"/>
        <rdfs:label>InfExternalInputs</rdfs:label>
    </owl:NamedIndividual>
    


    <!-- http://iec.ch/TC57/CIM100#Package_InfFinancial -->

    <owl:NamedIndividual rdf:about="http://iec.ch/TC57/CIM100#Package_InfFinancial">
        <rdf:type rdf:resource="http://langdale.com.au/2005/UML#Package"/>
        <uml:id>EAPK_C2A5377E_AC73_4b31_BA05_7C6D8900F469</uml:id>
        <rdfs:comment>This package is responsible for Settlement and Billing. These classes represent the legal entities who participate in formal or informal agreements.</rdfs:comment>
        <rdfs:isDefinedBy rdf:resource="http://iec.ch/TC57/CIM100#Package_InfIEC62325"/>
        <rdfs:label>InfFinancial</rdfs:label>
    </owl:NamedIndividual>
    


    <!-- http://iec.ch/TC57/CIM100#Package_InfHVDCDynamics -->

    <owl:NamedIndividual rdf:about="http://iec.ch/TC57/CIM100#Package_InfHVDCDynamics">
        <rdf:type rdf:resource="http://langdale.com.au/2005/UML#Package"/>
        <uml:id>EAPK_4DF22A50_ED55_4083_A159_4BA058A50CD6</uml:id>
        <rdfs:isDefinedBy rdf:resource="http://iec.ch/TC57/CIM100#Package_StandardModels"/>
        <rdfs:label>InfHVDCDynamics</rdfs:label>
    </owl:NamedIndividual>
    


    <!-- http://iec.ch/TC57/CIM100#Package_InfIEC61968 -->

    <owl:NamedIndividual rdf:about="http://iec.ch/TC57/CIM100#Package_InfIEC61968">
        <rdf:type rdf:resource="http://langdale.com.au/2005/UML#Package"/>
        <uml:id>EAPK_6D361F11_F6D2_4e79_972E_9E34AA663CA4</uml:id>
        <rdfs:comment>The package contains portions of the model defined byEnterprise Resource Planning (ERP) standards like those proposed by the Open Applications Group (OAG). It is provided to facilitate integration among electric utility applications (CIM) and enterprise resource planning (ERP) applications (as defined by OAG). Rather than inventing new CIM classes that accomplish similar functionality as in existing ERP models, the preferred approach is to use and extend ERP classes as appropriate in other packages.
If a model other that the OAG standard is used as a basis for ERP integration, the utility classes labeld &quot;Erp...&quot; should be associated with the appropriate classes of that standard. In fact, definitions of &quot;Erp...&quot; classes are based on OAG Nouns to facilitate this process.

TODO: The following has been copied from a very old version of draft Part 11, so the references are wrong, but we store the knowledge here to reuse later:
&quot;The Enterprise Resource Planning (ERP) Support Package contains portions of the model defined by ERP standards like those proposed by the Open Applications Group (OAG). This package is provided to facilitate integration among electric utility applications (CIM) and enterprise resource planning (ERP) applications (OAG). Rather than inventing new CIM classes that accomplish similar functionality as in existing ERP models, the preferred approach is to use and extend ERP classes as appropriate in other packages.
If a model other that the OAG standard is used as a basis for ERP integration, the utility classes labeled &quot;Erp...&quot; should be associated with the appropriate classes of that standard&quot;.</rdfs:comment>
        <rdfs:comment>The package covers all types of work, including inspection, maintenance, repair, restoration, and construction. It covers the full life cycle including request, initiate, track and record work. Standardized designs (compatible units) are used where possible.

TODO: The following has been copied from a very old version of draft Part 11, so the references are wrong, but we store the knowledge here to reuse later:
&quot;The Work package is used to define classes related to work. There are several different aspects of work.
The Work Initiation (Work, Project, Request).
The Work Design package is used for managing designs (CompatibleUnit, Design, DesignLocation, WorkTask).
The Work Schedule package is used for the scheduling and coordination of work (AccessPermit, MaterialItem, OneCallRequest, Regulation).
The Work Closing package is used for tracking costs of work (CostType, LaborItem, WorkCostDetail, VehicleItem).
The Work Standards package is used for the definition of compatible units (CULaborItem, CUVehicleItem, CUGroup).
This package is used for inspection and maintenance (InspectionDataSet, Procedure).
The WorkService package defines Appointment class&quot;.</rdfs:comment>
        <rdfs:comment>The package is used to define asset-level models for objects. Assets may be comprised of other assets and may have relationships to other assets. Assets also have owners and values. Assets may also have a relationship to a PowerSystemResource in the Wires model.

TODO: The following has been copied from a very old version of draft Part 11, so the references are wrong, but we store the knowledge here to reuse later:
&quot;Assets are the basic units which define a physical infrastructure. PowerSystemResources are logical objects meaningful to operations which are constructed from one or more Assets, although PowerSystemResources are not required to specifiy their component Assets.
The Asset package is comprosed of several packages. The key concepts of an Asset are as follows:
&lt;ul&gt;
	&lt;li&gt;Assets can have names, through inheritance to the Naming package&lt;/li&gt;
	&lt;li&gt;Assets are physical entities which have a lifecycle&lt;/li&gt;
	&lt;li&gt;One or more assets can be associated to create a PowerSystemResource&lt;/li&gt;
	&lt;li&gt;Assets can be grouped (aggregated) with other Assets&lt;/li&gt;
	&lt;li&gt;Assets are typically either &apos;point&apos; or &apos;linear&apos; assets, which relate to physical geometry&lt;/li&gt;
	&lt;li&gt;Assets have a close relationship to Work as a consequence of their lifecycle&lt;/li&gt;
&lt;/ul&gt;
The following sections describe the packages in the Assets package.
The AssetBasics package defines the relationship between Asset and other classes, such as Organization, PowerSystemResource and Document.
Point assets are those assets whose physical location can be described in terms of a single coordinate, such as a pole or a switch.
Linear assets are those assets whose physical location is best described in terms of a line, plyline or polygon.
Asset work triggers are used to determine when inspection and/or maintenance are required for assets&quot;.</rdfs:comment>
        <rdfs:comment>The package is used to define detailed customer models.</rdfs:comment>
        <rdfs:comment>This package and its subpackages contain informative (unstable) elements of the model, expected to evolve a lot or to be removed, and not published as IEC document yet. Some portions of it will be reworked and moved to normative packages as the need arises, and some portions may be removed.
WG14 does not generate documentation for this informative portion of the model.</rdfs:comment>
        <rdfs:comment>This package contains functions common for distribution management.</rdfs:comment>
        <rdfs:comment>This package contains informative classes (new and old) that we are working on in DCIM12 and that should be promoted to normative as soon as we deem them stable enough.
We did not rename existing Inf*** packages on purpose, because we sometimes refer to them and their classes in issues. Package below this sandbox will disappear, as soon as their content moves to normative.</rdfs:comment>
        <rdfs:isDefinedBy rdf:resource="http://iec.ch/TC57/CIM100#Package_IEC61968"/>
        <rdfs:label>InfIEC61968</rdfs:label>
    </owl:NamedIndividual>
    


    <!-- http://iec.ch/TC57/CIM100#Package_InfIEC61970 -->

    <owl:NamedIndividual rdf:about="http://iec.ch/TC57/CIM100#Package_InfIEC61970">
        <rdf:type rdf:resource="http://langdale.com.au/2005/UML#Package"/>
        <uml:id>EAPK_D2DD87AA_AF0C_477c_8E65_69D543D76521</uml:id>
        <rdfs:comment>Contains the planned schedules for equipment availability, primarily intended for future studies.</rdfs:comment>
        <rdfs:comment>Part of the canonical CIM published as IEC 61970-303.</rdfs:comment>
        <rdfs:comment>System Integrity Protection Schemes (SIPS) (IEC terminology). Other names used are: Remedial Action Schemes (RAS) or System Protection Schemes (SPS).</rdfs:comment>
        <rdfs:comment>The description of computed or dynamic limits.
These classes would likely go into the OperationalLimits package.</rdfs:comment>
        <rdfs:comment>This package and its subpackages contain informative (unstable) elements of the model, expected to evolve a lot or to be removed, and not published as IEC document yet. Some portions of it will be reworked and moved to normative packages as the need arises, and some portions may be removed.
WG13 does not generate documentation for this informative portion of the model.</rdfs:comment>
        <rdfs:isDefinedBy rdf:resource="http://iec.ch/TC57/CIM100#Package_IEC61970"/>
        <rdfs:label>InfIEC61970</rdfs:label>
    </owl:NamedIndividual>
    


    <!-- http://iec.ch/TC57/CIM100#Package_InfIEC62325 -->

    <owl:NamedIndividual rdf:about="http://iec.ch/TC57/CIM100#Package_InfIEC62325">
        <rdf:type rdf:resource="http://langdale.com.au/2005/UML#Package"/>
        <uml:id>EAPK_24305F28_EA82_4ffd_B4E1_454FDB3E2C36</uml:id>
        <rdfs:comment>This package is responsible for Settlement and Billing. These classes represent the legal entities who participate in formal or informal agreements.</rdfs:comment>
        <rdfs:comment>This package provides the capability to schedule and account for transactions for the exchange of electric power between companies. It includes transations for megawatts which are generated, consumed, lost, passed through, sold and purchased. These classes are used by Accounting and Billing for Energy, Generation Capacity, Transmission, and Ancillary Services.</rdfs:comment>
        <rdfs:isDefinedBy rdf:resource="http://iec.ch/TC57/CIM100#Package_IEC62325"/>
        <rdfs:label>InfIEC62325</rdfs:label>
    </owl:NamedIndividual>
    


    <!-- http://iec.ch/TC57/CIM100#Package_InfLocations -->

    <owl:NamedIndividual rdf:about="http://iec.ch/TC57/CIM100#Package_InfLocations">
        <rdf:type rdf:resource="http://langdale.com.au/2005/UML#Package"/>
        <uml:id>EAPK_3C223F3D_264E_410e_898C_82E54A1FC379</uml:id>
        <rdfs:isDefinedBy rdf:resource="http://iec.ch/TC57/CIM100#Package_InfIEC61968"/>
        <rdfs:label>InfLocations</rdfs:label>
    </owl:NamedIndividual>
    


    <!-- http://iec.ch/TC57/CIM100#Package_InfMarketOpCommon -->

    <owl:NamedIndividual rdf:about="http://iec.ch/TC57/CIM100#Package_InfMarketOpCommon">
        <rdf:type rdf:resource="http://langdale.com.au/2005/UML#Package"/>
        <uml:id>EAPK_63434AB3_A3E0_4853_9CB4_3432FD9EA2F5</uml:id>
        <rdfs:isDefinedBy rdf:resource="http://iec.ch/TC57/CIM100#Package_InfIEC62325"/>
        <rdfs:label>InfMarketOpCommon</rdfs:label>
    </owl:NamedIndividual>
    


    <!-- http://iec.ch/TC57/CIM100#Package_InfMarketOperations -->

    <owl:NamedIndividual rdf:about="http://iec.ch/TC57/CIM100#Package_InfMarketOperations">
        <rdf:type rdf:resource="http://langdale.com.au/2005/UML#Package"/>
        <uml:id>EAPK_25E6DE52_C4E1_4f13_9B34_95F06129D6A1</uml:id>
        <rdfs:isDefinedBy rdf:resource="http://iec.ch/TC57/CIM100#Package_InfIEC62325"/>
        <rdfs:label>InfMarketOperations</rdfs:label>
    </owl:NamedIndividual>
    


    <!-- http://iec.ch/TC57/CIM100#Package_InfMarketResults -->

    <owl:NamedIndividual rdf:about="http://iec.ch/TC57/CIM100#Package_InfMarketResults">
        <rdf:type rdf:resource="http://langdale.com.au/2005/UML#Package"/>
        <uml:id>EAPK_70940F3E_04B0_4747_8EF6_0E222B29C2FE</uml:id>
        <rdfs:isDefinedBy rdf:resource="http://iec.ch/TC57/CIM100#Package_InfIEC62325"/>
        <rdfs:label>InfMarketResults</rdfs:label>
    </owl:NamedIndividual>
    


    <!-- http://iec.ch/TC57/CIM100#Package_InfOperationalLimits -->

    <owl:NamedIndividual rdf:about="http://iec.ch/TC57/CIM100#Package_InfOperationalLimits">
        <rdf:type rdf:resource="http://langdale.com.au/2005/UML#Package"/>
        <uml:id>EAPK_33B38556_EE8E_4641_811C_0BC1AA73C764</uml:id>
        <rdfs:comment>The description of computed or dynamic limits.
These classes would likely go into the OperationalLimits package.</rdfs:comment>
        <rdfs:isDefinedBy rdf:resource="http://iec.ch/TC57/CIM100#Package_InfIEC61970"/>
        <rdfs:label>InfOperationalLimits</rdfs:label>
    </owl:NamedIndividual>
    


    <!-- http://iec.ch/TC57/CIM100#Package_InfPart303 -->

    <owl:NamedIndividual rdf:about="http://iec.ch/TC57/CIM100#Package_InfPart303">
        <rdf:type rdf:resource="http://langdale.com.au/2005/UML#Package"/>
        <uml:id>EAPK_500389E9_5C8C_40f4_9EB4_19613576509E</uml:id>
        <rdfs:comment>Defining meta-data for a change set in the functional Power System model.</rdfs:comment>
        <rdfs:comment>Generic descriptions of how domain data participates in datasets and alternate datasets.</rdfs:comment>
        <rdfs:isDefinedBy rdf:resource="http://iec.ch/TC57/CIM100#Package_InfIEC61970"/>
        <rdfs:label>InfPart303</rdfs:label>
    </owl:NamedIndividual>
    


    <!-- http://iec.ch/TC57/CIM100#Package_InfParticipantInterfaces -->

    <owl:NamedIndividual rdf:about="http://iec.ch/TC57/CIM100#Package_InfParticipantInterfaces">
        <rdf:type rdf:resource="http://langdale.com.au/2005/UML#Package"/>
        <uml:id>EAPK_B7690580_EDC9_4a72_831E_F41D6CF75D4A</uml:id>
        <rdfs:isDefinedBy rdf:resource="http://iec.ch/TC57/CIM100#Package_InfIEC62325"/>
        <rdfs:label>InfParticipantInterfaces</rdfs:label>
    </owl:NamedIndividual>
    


    <!-- http://iec.ch/TC57/CIM100#Package_InfReferenceData -->

    <owl:NamedIndividual rdf:about="http://iec.ch/TC57/CIM100#Package_InfReferenceData">
        <rdf:type rdf:resource="http://langdale.com.au/2005/UML#Package"/>
        <uml:id>EAPK_84D0D686_974E_4e70_8A25_93EEE6A54988</uml:id>
        <rdfs:isDefinedBy rdf:resource="http://iec.ch/TC57/CIM100#Package_InfIEC62325"/>
        <rdfs:label>InfReferenceData</rdfs:label>
    </owl:NamedIndividual>
    


    <!-- http://iec.ch/TC57/CIM100#Package_InfReservation -->

    <owl:NamedIndividual rdf:about="http://iec.ch/TC57/CIM100#Package_InfReservation">
        <rdf:type rdf:resource="http://langdale.com.au/2005/UML#Package"/>
        <uml:id>EAPK_B5F2CF0F_D405_4ca5_866A_6EB093CA37F8</uml:id>
        <rdfs:isDefinedBy rdf:resource="http://iec.ch/TC57/CIM100#Package_InfIEC62325"/>
        <rdfs:label>InfReservation</rdfs:label>
    </owl:NamedIndividual>
    


    <!-- http://iec.ch/TC57/CIM100#Package_InfSIPS -->

    <owl:NamedIndividual rdf:about="http://iec.ch/TC57/CIM100#Package_InfSIPS">
        <rdf:type rdf:resource="http://langdale.com.au/2005/UML#Package"/>
        <uml:id>EAPK_BB903AB3_D08C_4d30_A5AE_E3FA868711FA</uml:id>
        <rdfs:comment>System Integrity Protection Schemes (SIPS) (IEC terminology). Other names used are: Remedial Action Schemes (RAS) or System Protection Schemes (SPS).</rdfs:comment>
        <rdfs:isDefinedBy rdf:resource="http://iec.ch/TC57/CIM100#Package_InfIEC61970"/>
        <rdfs:label>InfSIPS</rdfs:label>
    </owl:NamedIndividual>
    


    <!-- http://iec.ch/TC57/CIM100#Package_InfTypeAsset -->

    <owl:NamedIndividual rdf:about="http://iec.ch/TC57/CIM100#Package_InfTypeAsset">
        <rdf:type rdf:resource="http://langdale.com.au/2005/UML#Package"/>
        <uml:id>EAPK_126D6C14_74BA_454d_86CC_F4E22C8E1448</uml:id>
        <rdfs:isDefinedBy rdf:resource="http://iec.ch/TC57/CIM100#Package_InfIEC61968"/>
        <rdfs:label>InfTypeAsset</rdfs:label>
    </owl:NamedIndividual>
    


    <!-- http://iec.ch/TC57/CIM100#Package_InfWiresExt -->

    <owl:NamedIndividual rdf:about="http://iec.ch/TC57/CIM100#Package_InfWiresExt">
        <rdf:type rdf:resource="http://langdale.com.au/2005/UML#Package"/>
        <uml:id>EAPK_C5B06802_9987_4648_AB20_57391B09A164</uml:id>
        <rdfs:isDefinedBy rdf:resource="http://iec.ch/TC57/CIM100#Package_InfIEC61968"/>
        <rdfs:label>InfWiresExt</rdfs:label>
    </owl:NamedIndividual>
    


    <!-- http://iec.ch/TC57/CIM100#Package_InfWork -->

    <owl:NamedIndividual rdf:about="http://iec.ch/TC57/CIM100#Package_InfWork">
        <rdf:type rdf:resource="http://langdale.com.au/2005/UML#Package"/>
        <uml:id>EAPK_17E519D6_0834_4012_A020_D6C99BC3AC25</uml:id>
        <rdfs:comment>The package covers all types of work, including inspection, maintenance, repair, restoration, and construction. It covers the full life cycle including request, initiate, track and record work. Standardized designs (compatible units) are used where possible.

TODO: The following has been copied from a very old version of draft Part 11, so the references are wrong, but we store the knowledge here to reuse later:
&quot;The Work package is used to define classes related to work. There are several different aspects of work.
The Work Initiation (Work, Project, Request).
The Work Design package is used for managing designs (CompatibleUnit, Design, DesignLocation, WorkTask).
The Work Schedule package is used for the scheduling and coordination of work (AccessPermit, MaterialItem, OneCallRequest, Regulation).
The Work Closing package is used for tracking costs of work (CostType, LaborItem, WorkCostDetail, VehicleItem).
The Work Standards package is used for the definition of compatible units (CULaborItem, CUVehicleItem, CUGroup).
This package is used for inspection and maintenance (InspectionDataSet, Procedure).
The WorkService package defines Appointment class&quot;.</rdfs:comment>
        <rdfs:isDefinedBy rdf:resource="http://iec.ch/TC57/CIM100#Package_InfIEC61968"/>
        <rdfs:label>InfWork</rdfs:label>
    </owl:NamedIndividual>
    


    <!-- http://iec.ch/TC57/CIM100#Package_LoadControl -->

    <owl:NamedIndividual rdf:about="http://iec.ch/TC57/CIM100#Package_LoadControl">
        <rdf:type rdf:resource="http://langdale.com.au/2005/UML#Package"/>
        <uml:id>EAPK_2C8E7660_0AE1_49fc_A5A4_854129CB9826</uml:id>
        <rdfs:comment>This package is an extension of the Metering package and contains the information classes that support specialised applications such as demand-side management using load control equipment. These classes are generally associated with the point where a service is delivered to the customer.</rdfs:comment>
        <rdfs:isDefinedBy rdf:resource="http://iec.ch/TC57/CIM100#Package_IEC61968"/>
        <rdfs:label>LoadControl</rdfs:label>
    </owl:NamedIndividual>
    


    <!-- http://iec.ch/TC57/CIM100#Package_LoadDynamics -->

    <owl:NamedIndividual rdf:about="http://iec.ch/TC57/CIM100#Package_LoadDynamics">
        <rdf:type rdf:resource="http://langdale.com.au/2005/UML#Package"/>
        <uml:id>EAPK_4B245477_75CE_4d8d_BBFE_0471D2D7A63D</uml:id>
        <rdfs:comment>Dynamic load models are used to represent the dynamic real and reactive load behaviour of a load from the static power flow model.  
Dynamic load models can be defined as applying either to a single load (energy consumer) or to a group of energy consumers.  
Large industrial motors or groups of similar motors can be represented by a synchronous machine model (SynchronousMachineDynamics) or an asynchronous machine model (AsynchronousMachineDynamics), which are usually represented as generators with negative active power output in the static (power flow) data.</rdfs:comment>
        <rdfs:isDefinedBy rdf:resource="http://iec.ch/TC57/CIM100#Package_StandardModels"/>
        <rdfs:label>LoadDynamics</rdfs:label>
    </owl:NamedIndividual>
    


    <!-- http://iec.ch/TC57/CIM100#Package_LoadModel -->

    <owl:NamedIndividual rdf:about="http://iec.ch/TC57/CIM100#Package_LoadModel">
        <rdf:type rdf:resource="http://langdale.com.au/2005/UML#Package"/>
        <uml:id>EAPK_427D9D64_CDA2_4070_AAC6_04A32F290872</uml:id>
        <rdfs:comment>This package is responsible for modelling the energy consumers and the system load as curves and associated curve data. Special circumstances that may affect the load, such as seasons and day types, are also included here.

This information is used by Load Forecasting and Load Management.</rdfs:comment>
        <rdfs:isDefinedBy rdf:resource="http://iec.ch/TC57/CIM100#Package_Base"/>
        <rdfs:label>LoadModel</rdfs:label>
    </owl:NamedIndividual>
    


    <!-- http://iec.ch/TC57/CIM100#Package_MarketCommon -->

    <owl:NamedIndividual rdf:about="http://iec.ch/TC57/CIM100#Package_MarketCommon">
        <rdf:type rdf:resource="http://langdale.com.au/2005/UML#Package"/>
        <uml:id>EAPK_2194B080_D2C6_41dc_99F4_9FF3984EC186</uml:id>
        <rdfs:comment>This package contains the common objects shared by MarketManagement, MarketOperations and Environmental packages.</rdfs:comment>
        <rdfs:isDefinedBy rdf:resource="http://iec.ch/TC57/CIM100#Package_IEC62325"/>
        <rdfs:label>MarketCommon</rdfs:label>
    </owl:NamedIndividual>
    


    <!-- http://iec.ch/TC57/CIM100#Package_MarketManagement -->

    <owl:NamedIndividual rdf:about="http://iec.ch/TC57/CIM100#Package_MarketManagement">
        <rdf:type rdf:resource="http://langdale.com.au/2005/UML#Package"/>
        <uml:id>EAPK_CB54CF00_9A30_4481_A696_FCB1BB1841E4</uml:id>
        <rdfs:comment>This package contains all core CIM Market Extensions required for market management systems.</rdfs:comment>
        <rdfs:isDefinedBy rdf:resource="http://iec.ch/TC57/CIM100#Package_IEC62325"/>
        <rdfs:label>MarketManagement</rdfs:label>
    </owl:NamedIndividual>
    


    <!-- http://iec.ch/TC57/CIM100#Package_MarketOpCommon -->

    <owl:NamedIndividual rdf:about="http://iec.ch/TC57/CIM100#Package_MarketOpCommon">
        <rdf:type rdf:resource="http://langdale.com.au/2005/UML#Package"/>
        <uml:id>EAPK_FCAD9A25_8D61_4b14_8D18_D988C0D98E52</uml:id>
        <rdfs:comment>This package contains the common objects shared by MarketOperations packages.</rdfs:comment>
        <rdfs:isDefinedBy rdf:resource="http://iec.ch/TC57/CIM100#Package_MarketOperations"/>
        <rdfs:label>MarketOpCommon</rdfs:label>
    </owl:NamedIndividual>
    


    <!-- http://iec.ch/TC57/CIM100#Package_MarketOperations -->

    <owl:NamedIndividual rdf:about="http://iec.ch/TC57/CIM100#Package_MarketOperations">
        <rdf:type rdf:resource="http://langdale.com.au/2005/UML#Package"/>
        <uml:id>EAPK_2D65E587_B530_4ca3_AF8F_86C72F1D5D50</uml:id>
        <rdfs:comment>Congestion rent is a major, highly volatile charge currently faced by many participants in the LMP-based electrical energy markets. For this reason, the ISOs offer congestion revenue rights (CRR), also known as financial transmission rights or transmission congestion contracts. These are financial instruments that allow market participants to hedge against congestion charges when they schedule their generation, load and bilateral energy transactions.</rdfs:comment>
        <rdfs:comment>Market participant interfaces for bids and trades.</rdfs:comment>
        <rdfs:comment>Market plan definitions for planned markets, planned market events, actual market runs, actual market events.</rdfs:comment>
        <rdfs:comment>Market results and external inputs consumed by markets.</rdfs:comment>
        <rdfs:comment>Market static reference data.</rdfs:comment>
        <rdfs:comment>Post-market accounting, calculation and meter data corrections to reduce invoicing errors and disputes. Reduces manual validation, verification and correction of transactional data that could affect market settlements. Republishing of market results with affected data corrected.</rdfs:comment>
        <rdfs:comment>The MktDomain package is a data dictionary of quantities and units that define datatypes for attributes (properties) that may be used by any class in any other package within MarketOperations.</rdfs:comment>
        <rdfs:comment>This package contains all core CIM Market Extensions required for market operations systems.</rdfs:comment>
        <rdfs:comment>This package contains the common objects shared by MarketOperations packages.</rdfs:comment>
        <rdfs:isDefinedBy rdf:resource="http://iec.ch/TC57/CIM100#Package_IEC62325"/>
        <rdfs:label>MarketOperations</rdfs:label>
    </owl:NamedIndividual>
    


    <!-- http://iec.ch/TC57/CIM100#Package_MarketPlan -->

    <owl:NamedIndividual rdf:about="http://iec.ch/TC57/CIM100#Package_MarketPlan">
        <rdf:type rdf:resource="http://langdale.com.au/2005/UML#Package"/>
        <uml:id>EAPK_78334671_413D_45ef_9151_795D865E6E26</uml:id>
        <rdfs:comment>Market plan definitions for planned markets, planned market events, actual market runs, actual market events.</rdfs:comment>
        <rdfs:isDefinedBy rdf:resource="http://iec.ch/TC57/CIM100#Package_MarketOperations"/>
        <rdfs:label>MarketPlan</rdfs:label>
    </owl:NamedIndividual>
    


    <!-- http://iec.ch/TC57/CIM100#Package_MarketQualitySystem -->

    <owl:NamedIndividual rdf:about="http://iec.ch/TC57/CIM100#Package_MarketQualitySystem">
        <rdf:type rdf:resource="http://langdale.com.au/2005/UML#Package"/>
        <uml:id>EAPK_2E615271_FBED_4feb_B966_C26B1134823F</uml:id>
        <rdfs:comment>Post-market accounting, calculation and meter data corrections to reduce invoicing errors and disputes. Reduces manual validation, verification and correction of transactional data that could affect market settlements. Republishing of market results with affected data corrected.</rdfs:comment>
        <rdfs:isDefinedBy rdf:resource="http://iec.ch/TC57/CIM100#Package_MarketOperations"/>
        <rdfs:label>MarketQualitySystem</rdfs:label>
    </owl:NamedIndividual>
    


    <!-- http://iec.ch/TC57/CIM100#Package_MarketResults -->

    <owl:NamedIndividual rdf:about="http://iec.ch/TC57/CIM100#Package_MarketResults">
        <rdf:type rdf:resource="http://langdale.com.au/2005/UML#Package"/>
        <uml:id>EAPK_DE03C327_EA1F_43be_9490_41A7C740FA0A</uml:id>
        <rdfs:comment>Results from the execution of a market.</rdfs:comment>
        <rdfs:isDefinedBy rdf:resource="http://iec.ch/TC57/CIM100#Package_MarketSystem"/>
        <rdfs:label>MarketResults</rdfs:label>
    </owl:NamedIndividual>
    


    <!-- http://iec.ch/TC57/CIM100#Package_MarketSystem -->

    <owl:NamedIndividual rdf:about="http://iec.ch/TC57/CIM100#Package_MarketSystem">
        <rdf:type rdf:resource="http://langdale.com.au/2005/UML#Package"/>
        <uml:id>EAPK_7710FAF5_3EB3_45aa_8719_083DE43F0A7A</uml:id>
        <rdfs:comment>Inputs to the market system from external sources.</rdfs:comment>
        <rdfs:comment>Market results and external inputs consumed by markets.</rdfs:comment>
        <rdfs:comment>Results from the execution of a market.</rdfs:comment>
        <rdfs:isDefinedBy rdf:resource="http://iec.ch/TC57/CIM100#Package_MarketOperations"/>
        <rdfs:label>MarketSystem</rdfs:label>
    </owl:NamedIndividual>
    


    <!-- http://iec.ch/TC57/CIM100#Package_Meas -->

    <owl:NamedIndividual rdf:about="http://iec.ch/TC57/CIM100#Package_Meas">
        <rdf:type rdf:resource="http://langdale.com.au/2005/UML#Package"/>
        <uml:id>EAPK_6B58A5C3_5CC1_4320_A9D3_2CABB8F9399E</uml:id>
        <rdfs:comment>Contains entities that describe dynamic measurement data exchanged between applications.</rdfs:comment>
        <rdfs:isDefinedBy rdf:resource="http://iec.ch/TC57/CIM100#Package_Base"/>
        <rdfs:label>Meas</rdfs:label>
    </owl:NamedIndividual>
    


    <!-- http://iec.ch/TC57/CIM100#Package_MechanicalLoadDynamics -->

    <owl:NamedIndividual rdf:about="http://iec.ch/TC57/CIM100#Package_MechanicalLoadDynamics">
        <rdf:type rdf:resource="http://langdale.com.au/2005/UML#Package"/>
        <uml:id>EAPK_54ED4DD8_2593_43f5_9A32_43679D605D36</uml:id>
        <rdfs:comment>A mechanical load represents the variation in a motor&apos;s shaft torque or power as a function of shaft speed.</rdfs:comment>
        <rdfs:isDefinedBy rdf:resource="http://iec.ch/TC57/CIM100#Package_StandardModels"/>
        <rdfs:label>MechanicalLoadDynamics</rdfs:label>
    </owl:NamedIndividual>
    


    <!-- http://iec.ch/TC57/CIM100#Package_Metering -->

    <owl:NamedIndividual rdf:about="http://iec.ch/TC57/CIM100#Package_Metering">
        <rdf:type rdf:resource="http://langdale.com.au/2005/UML#Package"/>
        <uml:id>EAPK_D6DF2C49_9FF2_428e_97B0_B5F4709BE7BE</uml:id>
        <rdfs:comment>This package contains only diagrams that are never printed in official documents.
Some are related to pending CIM issues, but the majority are drawn by hand from Metering-related XSDs that are in Part 9 document (Ed.1). Entry points into the schema are filled with green. Non-used associations are light grey.</rdfs:comment>
        <rdfs:comment>This package contains the core information classes that support end device applications with specialized classes for metering and premises area network devices, and remote reading functions. These classes are generally associated with the point where a service is delivered to the customer.</rdfs:comment>
        <rdfs:isDefinedBy rdf:resource="http://iec.ch/TC57/CIM100#Package_IEC61968"/>
        <rdfs:label>Metering</rdfs:label>
    </owl:NamedIndividual>
    


    <!-- http://iec.ch/TC57/CIM100#Package_MktDomain -->

    <owl:NamedIndividual rdf:about="http://iec.ch/TC57/CIM100#Package_MktDomain">
        <rdf:type rdf:resource="http://langdale.com.au/2005/UML#Package"/>
        <uml:id>EAPK_21A49697_6B5A_4e13_8499_8A2191CFCE84</uml:id>
        <rdfs:comment>The MktDomain package is a data dictionary of quantities and units that define datatypes for attributes (properties) that may be used by any class in any other package within MarketOperations.</rdfs:comment>
        <rdfs:isDefinedBy rdf:resource="http://iec.ch/TC57/CIM100#Package_MarketOperations"/>
        <rdfs:label>MktDomain</rdfs:label>
    </owl:NamedIndividual>
    


    <!-- http://iec.ch/TC57/CIM100#Package_ModelOperations -->

    <owl:NamedIndividual rdf:about="http://iec.ch/TC57/CIM100#Package_ModelOperations">
        <rdf:type rdf:resource="http://langdale.com.au/2005/UML#Package"/>
        <uml:id>EAPK_0FA4D827_B897_47bb_9BF8_B514908D372A</uml:id>
        <rdfs:isDefinedBy rdf:resource="http://iec.ch/TC57/CIM100#Package_InfPart303"/>
        <rdfs:label>ModelOperations</rdfs:label>
    </owl:NamedIndividual>
    


    <!-- http://iec.ch/TC57/CIM100#Package_NetworkModelFrames -->

    <owl:NamedIndividual rdf:about="http://iec.ch/TC57/CIM100#Package_NetworkModelFrames">
        <rdf:type rdf:resource="http://langdale.com.au/2005/UML#Package"/>
        <uml:id>EAPK_2C9E3B69_563C_4663_96DD_0E1074BE5F73</uml:id>
        <rdfs:isDefinedBy rdf:resource="http://iec.ch/TC57/CIM100#Package_InfPart303"/>
        <rdfs:label>NetworkModelFrames</rdfs:label>
    </owl:NamedIndividual>
    


    <!-- http://iec.ch/TC57/CIM100#Package_NetworkModelProjects -->

    <owl:NamedIndividual rdf:about="http://iec.ch/TC57/CIM100#Package_NetworkModelProjects">
        <rdf:type rdf:resource="http://langdale.com.au/2005/UML#Package"/>
        <uml:id>EAPK_0090ED2A_A4A9_40f2_B6AC_02BBFADFE48D</uml:id>
        <rdfs:comment>Defining meta-data for a change set in the functional Power System model.</rdfs:comment>
        <rdfs:isDefinedBy rdf:resource="http://iec.ch/TC57/CIM100#Package_InfPart303"/>
        <rdfs:label>NetworkModelProjects</rdfs:label>
    </owl:NamedIndividual>
    


    <!-- http://iec.ch/TC57/CIM100#Package_OperationalLimits -->

    <owl:NamedIndividual rdf:about="http://iec.ch/TC57/CIM100#Package_OperationalLimits">
        <rdf:type rdf:resource="http://langdale.com.au/2005/UML#Package"/>
        <uml:id>EAPK_CCAAF4EA_4C50_4438_86F9_63852950B3CA</uml:id>
        <rdfs:comment>This package models a specification of limits associated with equipment and other operational entities.</rdfs:comment>
        <rdfs:isDefinedBy rdf:resource="http://iec.ch/TC57/CIM100#Package_Base"/>
        <rdfs:label>OperationalLimits</rdfs:label>
    </owl:NamedIndividual>
    


    <!-- http://iec.ch/TC57/CIM100#Package_Operations -->

    <owl:NamedIndividual rdf:about="http://iec.ch/TC57/CIM100#Package_Operations">
        <rdf:type rdf:resource="http://langdale.com.au/2005/UML#Package"/>
        <uml:id>EAPK_CE6EBADC_B316_4fe1_AC5C_D4888139657D</uml:id>
        <rdfs:comment>This package contains the core information classes that support operations and outage management applications.</rdfs:comment>
        <rdfs:isDefinedBy rdf:resource="http://iec.ch/TC57/CIM100#Package_IEC61968"/>
        <rdfs:label>Operations</rdfs:label>
    </owl:NamedIndividual>
    


    <!-- http://iec.ch/TC57/CIM100#Package_OverexcitationLimiterDynamics -->

    <owl:NamedIndividual rdf:about="http://iec.ch/TC57/CIM100#Package_OverexcitationLimiterDynamics">
        <rdf:type rdf:resource="http://langdale.com.au/2005/UML#Package"/>
        <uml:id>EAPK_CB5C7172_23DD_4cc0_ACF3_557E0496AFCD</uml:id>
        <rdfs:comment>Overexcitation limiters (OELs) are also referred to as &lt;i&gt;maximum excitation limiters &lt;/i&gt;and &lt;i&gt;field current limiters. &lt;/i&gt;The possibility of voltage collapse in stressed power systems increases the importance of modelling these limiters in studies of system conditions that cause machines to operate at high levels of excitation for a sustained period, such as voltage collapse or system-islanding. Such events typically occur over a long time frame compared with transient or small-signal stability simulations.</rdfs:comment>
        <rdfs:isDefinedBy rdf:resource="http://iec.ch/TC57/CIM100#Package_StandardModels"/>
        <rdfs:label>OverexcitationLimiterDynamics</rdfs:label>
    </owl:NamedIndividual>
    


    <!-- http://iec.ch/TC57/CIM100#Package_PFVArControllerType1Dynamics -->

    <owl:NamedIndividual rdf:about="http://iec.ch/TC57/CIM100#Package_PFVArControllerType1Dynamics">
        <rdf:type rdf:resource="http://langdale.com.au/2005/UML#Package"/>
        <uml:id>EAPK_DB4B66D7_C753_481b_9C15_D0753561B765</uml:id>
        <rdfs:comment>&lt;font color=&quot;#0f0f0f&quot;&gt;Excitation systems for synchronous machines are sometimes supplied with an optional means of automatically adjusting generator output reactive power (VAr) or power factor (PF) to a user-specified value. This can be accomplished with either a reactive power or power factor controller or regulator.  A reactive power or power factor controller is defined as a PF/VAr controller in IEEE 421.1 as “a control function that acts through the reference adjuster to modify the voltage regulator set point to maintain the synchronous machine steady-state power factor or reactive power at a predetermined value.” &lt;/font&gt;
&lt;font color=&quot;#0f0f0f&quot;&gt;For additional information please refer to IEEE 421.5-2005, 11.&lt;/font&gt;</rdfs:comment>
        <rdfs:isDefinedBy rdf:resource="http://iec.ch/TC57/CIM100#Package_StandardModels"/>
        <rdfs:label>PFVArControllerType1Dynamics</rdfs:label>
    </owl:NamedIndividual>
    


    <!-- http://iec.ch/TC57/CIM100#Package_PFVArControllerType2Dynamics -->

    <owl:NamedIndividual rdf:about="http://iec.ch/TC57/CIM100#Package_PFVArControllerType2Dynamics">
        <rdf:type rdf:resource="http://langdale.com.au/2005/UML#Package"/>
        <uml:id>EAPK_9AF74EDB_FFF5_4083_A7D5_48644244A045</uml:id>
        <rdfs:comment>&lt;font color=&quot;#0f0f0f&quot;&gt;A var/pf regulator is defined as “a synchronous machine regulator that functions to maintain the power factor or reactive component of power at a predetermined value.”  &lt;/font&gt;
&lt;font color=&quot;#0f0f0f&quot;&gt;For additional information please refer to IEEE 421.5-2005, 11.&lt;/font&gt;
&lt;font color=&quot;#0f0f0f&quot;&gt;
&lt;/font&gt;</rdfs:comment>
        <rdfs:isDefinedBy rdf:resource="http://iec.ch/TC57/CIM100#Package_StandardModels"/>
        <rdfs:label>PFVArControllerType2Dynamics</rdfs:label>
    </owl:NamedIndividual>
    


    <!-- http://iec.ch/TC57/CIM100#Package_PackageDependencies -->

    <owl:NamedIndividual rdf:about="http://iec.ch/TC57/CIM100#Package_PackageDependencies">
        <rdf:type rdf:resource="http://langdale.com.au/2005/UML#Package"/>
        <uml:id>EAPK_FDFFB5A3_38EB_404f_83EC_1F62FC479DC2</uml:id>
        <rdfs:comment>This package shows all the root level subpackage dependencies of the combined CIM model.</rdfs:comment>
        <rdfs:isDefinedBy rdf:resource="http://iec.ch/TC57/CIM100#Package_TC57CIM"/>
        <rdfs:label>PackageDependencies</rdfs:label>
    </owl:NamedIndividual>
    


    <!-- http://iec.ch/TC57/CIM100#Package_Part303 -->

    <owl:NamedIndividual rdf:about="http://iec.ch/TC57/CIM100#Package_Part303">
        <rdf:type rdf:resource="http://langdale.com.au/2005/UML#Package"/>
        <uml:id>EAPK_097BFA4A_EAE9_4618_B4D1_896C3B3BB77D</uml:id>
        <rdfs:comment>Contains classes used for generic dataset modelling.</rdfs:comment>
        <rdfs:comment>Part of the canonical CIM published as IEC 61970-303.</rdfs:comment>
        <rdfs:isDefinedBy rdf:resource="http://iec.ch/TC57/CIM100#Package_InfIEC61970"/>
        <rdfs:label>Part303</rdfs:label>
    </owl:NamedIndividual>
    


    <!-- http://iec.ch/TC57/CIM100#Package_ParticipantInterfaces -->

    <owl:NamedIndividual rdf:about="http://iec.ch/TC57/CIM100#Package_ParticipantInterfaces">
        <rdf:type rdf:resource="http://langdale.com.au/2005/UML#Package"/>
        <uml:id>EAPK_3A7DCF28_B7A5_424f_BB0A_560014D3974A</uml:id>
        <rdfs:comment>Market participant interfaces for bids and trades.</rdfs:comment>
        <rdfs:isDefinedBy rdf:resource="http://iec.ch/TC57/CIM100#Package_MarketOperations"/>
        <rdfs:label>ParticipantInterfaces</rdfs:label>
    </owl:NamedIndividual>
    


    <!-- http://iec.ch/TC57/CIM100#Package_PaymentMetering -->

    <owl:NamedIndividual rdf:about="http://iec.ch/TC57/CIM100#Package_PaymentMetering">
        <rdf:type rdf:resource="http://langdale.com.au/2005/UML#Package"/>
        <uml:id>EAPK_027D3F98_0C2D_4ba2_84A8_3DB60760C72A</uml:id>
        <rdfs:comment>This package contains only diagrams that are never printed in official documents.
Diagrams are drawn by hand from PaymentMetering-related XSDs that are in Part 9 Ed.1 document. Entry points into the schema are filled with green. Non-used associations are light grey.</rdfs:comment>
        <rdfs:comment>This package is an extension of the Metering package and contains the information classes that support specialised applications such as prepayment metering. These classes are generally associated with the collection and control of revenue from the customer for a delivered service.</rdfs:comment>
        <rdfs:isDefinedBy rdf:resource="http://iec.ch/TC57/CIM100#Package_IEC61968"/>
        <rdfs:label>PaymentMetering</rdfs:label>
    </owl:NamedIndividual>
    


    <!-- http://iec.ch/TC57/CIM100#Package_PowerSystemStabilizerDynamics -->

    <owl:NamedIndividual rdf:about="http://iec.ch/TC57/CIM100#Package_PowerSystemStabilizerDynamics">
        <rdf:type rdf:resource="http://langdale.com.au/2005/UML#Package"/>
        <uml:id>EAPK_15788FE9_6C55_412c_8AB7_F3F1EB004BDF</uml:id>
        <rdfs:comment>The power system stabilizer (PSS) model provides an input (&lt;i&gt;Vs&lt;/i&gt;) to the excitation system model to improve damping of system oscillations.  A variety of input signals can be used depending on the particular design.</rdfs:comment>
        <rdfs:isDefinedBy rdf:resource="http://iec.ch/TC57/CIM100#Package_StandardModels"/>
        <rdfs:label>PowerSystemStabilizerDynamics</rdfs:label>
    </owl:NamedIndividual>
    


    <!-- http://iec.ch/TC57/CIM100#Package_Production -->

    <owl:NamedIndividual rdf:about="http://iec.ch/TC57/CIM100#Package_Production">
        <rdf:type rdf:resource="http://langdale.com.au/2005/UML#Package"/>
        <uml:id>EAPK_39719C4D_64F6_4704_8202_8CAEF5179709</uml:id>
        <rdfs:comment>The production package is responsible for classes which describe various kinds of generators. These classes also provide production costing information which is used to economically allocate demand among committed units and calculate reserve quantities.</rdfs:comment>
        <rdfs:isDefinedBy rdf:resource="http://iec.ch/TC57/CIM100#Package_Generation"/>
        <rdfs:label>Production</rdfs:label>
    </owl:NamedIndividual>
    


    <!-- http://iec.ch/TC57/CIM100#Package_Protection -->

    <owl:NamedIndividual rdf:about="http://iec.ch/TC57/CIM100#Package_Protection">
        <rdf:type rdf:resource="http://langdale.com.au/2005/UML#Package"/>
        <uml:id>EAPK_3F02E213_ECF8_4f14_9AD5_D4A252FE300A</uml:id>
        <rdfs:comment>An extension to the Core and Wires packages that models information for protection equipment such as relays. These entities are used within training simulators and distribution network fault location applications.</rdfs:comment>
        <rdfs:isDefinedBy rdf:resource="http://iec.ch/TC57/CIM100#Package_Base"/>
        <rdfs:label>Protection</rdfs:label>
    </owl:NamedIndividual>
    


    <!-- http://iec.ch/TC57/CIM100#Package_ReferenceData -->

    <owl:NamedIndividual rdf:about="http://iec.ch/TC57/CIM100#Package_ReferenceData">
        <rdf:type rdf:resource="http://langdale.com.au/2005/UML#Package"/>
        <uml:id>EAPK_B6A20E36_8969_4657_B90F_000277DAC6C4</uml:id>
        <rdfs:comment>Market static reference data.</rdfs:comment>
        <rdfs:isDefinedBy rdf:resource="http://iec.ch/TC57/CIM100#Package_MarketOperations"/>
        <rdfs:label>ReferenceData</rdfs:label>
    </owl:NamedIndividual>
    


    <!-- http://iec.ch/TC57/CIM100#Package_SCADA -->

    <owl:NamedIndividual rdf:about="http://iec.ch/TC57/CIM100#Package_SCADA">
        <rdf:type rdf:resource="http://langdale.com.au/2005/UML#Package"/>
        <uml:id>EAPK_C397A471_682D_4757_89C3_C65DCE1842A7</uml:id>
        <rdfs:comment>Contains entities to model information used by Supervisory Control and Data Acquisition (SCADA) applications. Supervisory control supports operator control of equipment, such as opening or closing a breaker. Data acquisition gathers telemetered data from various sources.  The subtypes of the Telemetry entity deliberately match the UCA and IEC 61850 definitions. 
This package also supports alarm presentation but it is not expected to be used by other applications.</rdfs:comment>
        <rdfs:isDefinedBy rdf:resource="http://iec.ch/TC57/CIM100#Package_Base"/>
        <rdfs:label>SCADA</rdfs:label>
    </owl:NamedIndividual>
    


    <!-- http://iec.ch/TC57/CIM100#Package_StandardInterconnections -->

    <owl:NamedIndividual rdf:about="http://iec.ch/TC57/CIM100#Package_StandardInterconnections">
        <rdf:type rdf:resource="http://langdale.com.au/2005/UML#Package"/>
        <uml:id>EAPK_9E32B79D_9C05_4fe4_9518_A32B1C67637A</uml:id>
        <rdfs:comment>This subclause describes the standard interconnections for various types of equipment. These interconnections are understood by the application programs and can be identified based on the presence of one of the key classes with a relationship to the static power flow model: SynchronousMachineDynamics, AsynchronousMachineDynamics, EnergyConsumerDynamics or WindTurbineType3or4Dynamics. 
The relationships between classes expressed in the interconnection diagrams are intended to support dynamic behaviour described by either standard models or user-defined models.
In the interconnection diagrams, boxes which are black in colour represent function blocks whose functionality can be provided by one of many standard models or by a user-defined model. Blue boxes represent specific standard models.  A dashed box means that the function block or specific standard model is optional.</rdfs:comment>
        <rdfs:isDefinedBy rdf:resource="http://iec.ch/TC57/CIM100#Package_Dynamics"/>
        <rdfs:label>StandardInterconnections</rdfs:label>
    </owl:NamedIndividual>
    


    <!-- http://iec.ch/TC57/CIM100#Package_StandardModels -->

    <owl:NamedIndividual rdf:about="http://iec.ch/TC57/CIM100#Package_StandardModels">
        <rdf:type rdf:resource="http://langdale.com.au/2005/UML#Package"/>
        <uml:id>EAPK_1BEB429C_BFD0_49c6_9556_AC7BA58C2202</uml:id>
        <rdfs:comment>&lt;font color=&quot;#0f0f0f&quot;&gt;A var/pf regulator is defined as “a synchronous machine regulator that functions to maintain the power factor or reactive component of power at a predetermined value.”  &lt;/font&gt;
&lt;font color=&quot;#0f0f0f&quot;&gt;For additional information please refer to IEEE 421.5-2005, 11.&lt;/font&gt;
&lt;font color=&quot;#0f0f0f&quot;&gt;
&lt;/font&gt;</rdfs:comment>
        <rdfs:comment>&lt;font color=&quot;#0f0f0f&quot;&gt;A voltage adjuster is a reference adjuster that uses inputs from a reactive power or power factor controller to modify the voltage regulator set point to maintain the synchronous machine steady-state power factor or reactive power at a predetermined value. &lt;/font&gt;
&lt;font color=&quot;#0f0f0f&quot;&gt;For additional information please refer to IEEE 421.5-2005, 11.&lt;/font&gt;</rdfs:comment>
        <rdfs:comment>&lt;font color=&quot;#0f0f0f&quot;&gt;Excitation systems for synchronous machines are sometimes supplied with an optional means of automatically adjusting generator output reactive power (VAr) or power factor (PF) to a user-specified value. This can be accomplished with either a reactive power or power factor controller or regulator.  A reactive power or power factor controller is defined as a PF/VAr controller in IEEE 421.1 as “a control function that acts through the reference adjuster to modify the voltage regulator set point to maintain the synchronous machine steady-state power factor or reactive power at a predetermined value.” &lt;/font&gt;
&lt;font color=&quot;#0f0f0f&quot;&gt;For additional information please refer to IEEE 421.5-2005, 11.&lt;/font&gt;</rdfs:comment>
        <rdfs:comment>&lt;font color=&quot;#0f0f0f&quot;&gt;Synchronous machine terminal voltage transducer and current compensator models&lt;/font&gt; adjust the terminal voltage feedback to the excitation system by adding a quantity that is proportional to the terminal current of the generator.  It is linked to a specific generator (synchronous machine).
&lt;font color=&quot;#0f0f0f&quot;&gt;Several types of compensation are available on most excitation systems. Synchronous machine active and reactive current compensation are the most common. Either reactive droop compensation and/or line-drop compensation can be used, simulating an impedance drop and effectively regulating at some point other than the terminals of the machine. The impedance or range of adjustment and type of compensation should be specified for different types. &lt;/font&gt;
&lt;font color=&quot;#0f0f0f&quot;&gt;Care shall be taken to ensure that a consistent PU system is utilized for the compensator parameters and the synchronous machine current base.&lt;/font&gt;
&lt;font color=&quot;#0f0f0f&quot;&gt;For further information see IEEE 421.5-2005, 4.&lt;/font&gt;


&lt;font color=&quot;#0f0f0f&quot;&gt;
&lt;/font&gt;</rdfs:comment>
        <rdfs:comment>A mechanical load represents the variation in a motor&apos;s shaft torque or power as a function of shaft speed.</rdfs:comment>
        <rdfs:comment>A turbine load controller acts to maintain turbine power at a set value by continuous adjustment of the turbine governor speed-load reference.</rdfs:comment>
        <rdfs:comment>An asynchronous machine model represents a (induction) generator or motor with no external connection to the rotor windings, e.g. a squirrel-cage induction machine. 
The interconnection with the electrical network equations can differ among simulation tools.  The program only needs to know the terminal to which this asynchronous machine is connected in order to establish the correct interconnection.  The interconnection with the motor’s equipment could also differ due to input and output signals required by standard models.
The asynchronous machine model is used to model wind generators type 1 and type 2.  For these, normal practice is to include the rotor flux transients and neglect the stator flux transients.</rdfs:comment>
        <rdfs:comment>Dynamic load models are used to represent the dynamic real and reactive load behaviour of a load from the static power flow model.  
Dynamic load models can be defined as applying either to a single load (energy consumer) or to a group of energy consumers.  
Large industrial motors or groups of similar motors can be represented by a synchronous machine model (SynchronousMachineDynamics) or an asynchronous machine model (AsynchronousMachineDynamics), which are usually represented as generators with negative active power output in the static (power flow) data.</rdfs:comment>
        <rdfs:comment>For conventional power generating units (e.g., thermal, hydro, combustion turbine), a synchronous machine model represents the electrical characteristics of the generator and the mechanical characteristics of the turbine-generator rotational inertia.  Large industrial motors or groups of similar motors can be represented by individual motor models which are represented as generators with negative active power in the static (power flow) data.  
The interconnection with the electrical network equations can differ among simulation tools.  The tool only needs to know the synchronous machine to establish the correct interconnection.  The interconnection with the motor’s equipment could also differ due to input and output signals required by standard models.</rdfs:comment>
        <rdfs:comment>High voltage direct current (HVDC) models.</rdfs:comment>
        <rdfs:comment>In certain system configurations, continuous excitation control with terminal voltage and power system stabilizing regulator input signals does not ensure that the potential of the excitation system for improving system stability is fully exploited. For these situations, discontinuous excitation control signals can be employed to enhance stability following large transient disturbances.
&lt;font color=&quot;#0f0f0f&quot;&gt;For additional information please refer to IEEE 421.5-2005, 12.&lt;/font&gt;</rdfs:comment>
        <rdfs:comment>Overexcitation limiters (OELs) are also referred to as &lt;i&gt;maximum excitation limiters &lt;/i&gt;and &lt;i&gt;field current limiters. &lt;/i&gt;The possibility of voltage collapse in stressed power systems increases the importance of modelling these limiters in studies of system conditions that cause machines to operate at high levels of excitation for a sustained period, such as voltage collapse or system-islanding. Such events typically occur over a long time frame compared with transient or small-signal stability simulations.</rdfs:comment>
        <rdfs:comment>Static var compensator (SVC) models.</rdfs:comment>
        <rdfs:comment>The excitation system model provides the field voltage (&lt;i&gt;Efd&lt;/i&gt;) for a synchronous machine model.  It is linked to a specific generator (synchronous machine). 
The representation of all limits used by the models (not including IEEE standard models) shall comply with the representation defined in the Annex E of the IEEE 421.5-2005, unless specified differently in the documentation of the model.
The parameters are different for each excitation system model; the same parameter name can have different meaning in different models.</rdfs:comment>
        <rdfs:comment>The power system stabilizer (PSS) model provides an input (&lt;i&gt;Vs&lt;/i&gt;) to the excitation system model to improve damping of system oscillations.  A variety of input signals can be used depending on the particular design.</rdfs:comment>
        <rdfs:comment>The turbine-governor model is linked to one or two synchronous generators and determines the shaft mechanical power (&lt;i&gt;Pm&lt;/i&gt;) or torque (&lt;i&gt;Tm&lt;/i&gt;) for the generator model.  
Unlike IEEE standard models for other function blocks, the three IEEE turbine-governor standard models (GovHydroIEEE0, GovHydroIEEE2, and GovSteamIEEE1) are documented in IEEE Transactions, not in IEEE standards. For that reason, diagrams are supplied for those models.
A 2012 IEEE report, &lt;i&gt;&lt;u&gt;Dynamic Models for Turbine-Governors in Power System Studies&lt;/u&gt;&lt;/i&gt;, provides updated information on a variety of models including IEEE, vendor and reliability authority models.  Fully incorporating the results of that report into the CIM dynamics model is a future effort.</rdfs:comment>
        <rdfs:comment>This subclause contains standard dynamic model specifications grouped into packages by standard function block (type of equipment being modelled).
In the CIM, standard dynamic models are expressed by means of a class named with the standard model name and attributes reflecting each of the parameters necessary to describe the behaviour of an instance of the standard model.</rdfs:comment>
        <rdfs:comment>Underexcitation limiters (UELs) act to boost excitation. The UEL typically senses either a combination of voltage and current of the synchronous machine or a combination of real and reactive power. Some UELs utilize a temperature or pressure recalibration feature, in which the UEL characteristic is shifted depending upon the generator cooling gas temperature or pressure.</rdfs:comment>
        <rdfs:comment>Wind turbines are generally divided into four types, which are currently significant in power systems.  The four types have the following characteristics:
- type 1: wind turbine with directly grid connected asynchronous generator with fixed rotor resistance (typically squirrel cage);
- type 2: wind turbine with directly grid connected asynchronous generator with variable rotor resistance;
- type 3: wind turbines with doubly-fed asynchronous generators (directly connected stator and rotor connected through power converter);
- type 4: wind turbines connected to the grid through a full size power converter.
Models included in this package are according to IEC 61400-27-1:2015.</rdfs:comment>
        <rdfs:isDefinedBy rdf:resource="http://iec.ch/TC57/CIM100#Package_Dynamics"/>
        <rdfs:label>StandardModels</rdfs:label>
    </owl:NamedIndividual>
    


    <!-- http://iec.ch/TC57/CIM100#Package_StateVariables -->

    <owl:NamedIndividual rdf:about="http://iec.ch/TC57/CIM100#Package_StateVariables">
        <rdf:type rdf:resource="http://langdale.com.au/2005/UML#Package"/>
        <uml:id>EAPK_968842F7_ED9B_4b20_A08E_C8ECAAC5DB25</uml:id>
        <rdfs:comment>State variables for analysis solutions such as powerflow.</rdfs:comment>
        <rdfs:isDefinedBy rdf:resource="http://iec.ch/TC57/CIM100#Package_Base"/>
        <rdfs:label>StateVariables</rdfs:label>
    </owl:NamedIndividual>
    


    <!-- http://iec.ch/TC57/CIM100#Package_StaticVarCompensatorDynamics -->

    <owl:NamedIndividual rdf:about="http://iec.ch/TC57/CIM100#Package_StaticVarCompensatorDynamics">
        <rdf:type rdf:resource="http://langdale.com.au/2005/UML#Package"/>
        <uml:id>EAPK_97871C31_9D61_4b9b_A49A_F63A7DC2DBA5</uml:id>
        <rdfs:comment>Static var compensator (SVC) models.</rdfs:comment>
        <rdfs:isDefinedBy rdf:resource="http://iec.ch/TC57/CIM100#Package_StandardModels"/>
        <rdfs:label>StaticVarCompensatorDynamics</rdfs:label>
    </owl:NamedIndividual>
    


    <!-- http://iec.ch/TC57/CIM100#Package_SynchronousMachineDynamics -->

    <owl:NamedIndividual rdf:about="http://iec.ch/TC57/CIM100#Package_SynchronousMachineDynamics">
        <rdf:type rdf:resource="http://langdale.com.au/2005/UML#Package"/>
        <uml:id>EAPK_448F8675_D39C_4fe0_9450_2791AE603EFC</uml:id>
        <rdfs:comment>For conventional power generating units (e.g., thermal, hydro, combustion turbine), a synchronous machine model represents the electrical characteristics of the generator and the mechanical characteristics of the turbine-generator rotational inertia.  Large industrial motors or groups of similar motors can be represented by individual motor models which are represented as generators with negative active power in the static (power flow) data.  
The interconnection with the electrical network equations can differ among simulation tools.  The tool only needs to know the synchronous machine to establish the correct interconnection.  The interconnection with the motor’s equipment could also differ due to input and output signals required by standard models.</rdfs:comment>
        <rdfs:isDefinedBy rdf:resource="http://iec.ch/TC57/CIM100#Package_StandardModels"/>
        <rdfs:label>SynchronousMachineDynamics</rdfs:label>
    </owl:NamedIndividual>
    


    <!-- http://iec.ch/TC57/CIM100#Package_TC57CIM -->

    <owl:NamedIndividual rdf:about="http://iec.ch/TC57/CIM100#Package_TC57CIM">
        <rdf:type rdf:resource="http://langdale.com.au/2005/UML#Package"/>
        <uml:id>EAPK_39AA7E64_A03A_4934_AF09_E74943F7E6C0</uml:id>
        <rdfs:comment>The IEC 61968 subpackages of the CIM are developed, standardized and maintained by the UCA community including its working groups and task forces.
Currently, normative parts of the model support the needs of information exchange defined in IEC 61968-3, IEC 61968-4, IEC 61968-5, IEC 61968-6, IEC 61968-8, IEC 61968-9 and in IEC 61968-13.</rdfs:comment>
        <rdfs:comment>The IEC 62325 subpackages of the CIM are developed, standardized and maintained by the IEC TC57.</rdfs:comment>
        <rdfs:comment>This package shows all the root level subpackage dependencies of the combined CIM model.</rdfs:comment>
        <rdfs:comment>Top package for IEC 61970.</rdfs:comment>
        <rdfs:comment>Top package for IEC TC57 CIM.</rdfs:comment>
        <rdfs:label>TC57CIM</rdfs:label>
    </owl:NamedIndividual>
    


    <!-- http://iec.ch/TC57/CIM100#Package_Topology -->

    <owl:NamedIndividual rdf:about="http://iec.ch/TC57/CIM100#Package_Topology">
        <rdf:type rdf:resource="http://langdale.com.au/2005/UML#Package"/>
        <uml:id>EAPK_E44AA599_D1DD_4d0c_8487_AE8BE9E6FEEB</uml:id>
        <rdfs:comment>An extension to the Core Package that, in association with the Terminal class, models Connectivity, that is the physical definition of how equipment is connected together. In addition it models Topology, that is the logical definition of how equipment is connected via closed switches. The Topology definition is independent of the other electrical characteristics.</rdfs:comment>
        <rdfs:isDefinedBy rdf:resource="http://iec.ch/TC57/CIM100#Package_Base"/>
        <rdfs:label>Topology</rdfs:label>
    </owl:NamedIndividual>
    


    <!-- http://iec.ch/TC57/CIM100#Package_TurbineGovernorDynamics -->

    <owl:NamedIndividual rdf:about="http://iec.ch/TC57/CIM100#Package_TurbineGovernorDynamics">
        <rdf:type rdf:resource="http://langdale.com.au/2005/UML#Package"/>
        <uml:id>EAPK_40DA7439_D5DD_4608_85C0_87CF5444B24E</uml:id>
        <rdfs:comment>The turbine-governor model is linked to one or two synchronous generators and determines the shaft mechanical power (&lt;i&gt;Pm&lt;/i&gt;) or torque (&lt;i&gt;Tm&lt;/i&gt;) for the generator model.  
Unlike IEEE standard models for other function blocks, the three IEEE turbine-governor standard models (GovHydroIEEE0, GovHydroIEEE2, and GovSteamIEEE1) are documented in IEEE Transactions, not in IEEE standards. For that reason, diagrams are supplied for those models.
A 2012 IEEE report, &lt;i&gt;&lt;u&gt;Dynamic Models for Turbine-Governors in Power System Studies&lt;/u&gt;&lt;/i&gt;, provides updated information on a variety of models including IEEE, vendor and reliability authority models.  Fully incorporating the results of that report into the CIM dynamics model is a future effort.</rdfs:comment>
        <rdfs:isDefinedBy rdf:resource="http://iec.ch/TC57/CIM100#Package_StandardModels"/>
        <rdfs:label>TurbineGovernorDynamics</rdfs:label>
    </owl:NamedIndividual>
    


    <!-- http://iec.ch/TC57/CIM100#Package_TurbineLoadControllerDynamics -->

    <owl:NamedIndividual rdf:about="http://iec.ch/TC57/CIM100#Package_TurbineLoadControllerDynamics">
        <rdf:type rdf:resource="http://langdale.com.au/2005/UML#Package"/>
        <uml:id>EAPK_F0E43C7F_6E03_4b93_B0AF_2111023CA155</uml:id>
        <rdfs:comment>A turbine load controller acts to maintain turbine power at a set value by continuous adjustment of the turbine governor speed-load reference.</rdfs:comment>
        <rdfs:isDefinedBy rdf:resource="http://iec.ch/TC57/CIM100#Package_StandardModels"/>
        <rdfs:label>TurbineLoadControllerDynamics</rdfs:label>
    </owl:NamedIndividual>
    


    <!-- http://iec.ch/TC57/CIM100#Package_UnderexcitationLimiterDynamics -->

    <owl:NamedIndividual rdf:about="http://iec.ch/TC57/CIM100#Package_UnderexcitationLimiterDynamics">
        <rdf:type rdf:resource="http://langdale.com.au/2005/UML#Package"/>
        <uml:id>EAPK_6601D8F5_D2D3_4743_A9D8_51CADC84A53A</uml:id>
        <rdfs:comment>Underexcitation limiters (UELs) act to boost excitation. The UEL typically senses either a combination of voltage and current of the synchronous machine or a combination of real and reactive power. Some UELs utilize a temperature or pressure recalibration feature, in which the UEL characteristic is shifted depending upon the generator cooling gas temperature or pressure.</rdfs:comment>
        <rdfs:isDefinedBy rdf:resource="http://iec.ch/TC57/CIM100#Package_StandardModels"/>
        <rdfs:label>UnderexcitationLimiterDynamics</rdfs:label>
    </owl:NamedIndividual>
    


    <!-- http://iec.ch/TC57/CIM100#Package_UserDefinedModels -->

    <owl:NamedIndividual rdf:about="http://iec.ch/TC57/CIM100#Package_UserDefinedModels">
        <rdf:type rdf:resource="http://langdale.com.au/2005/UML#Package"/>
        <uml:id>EAPK_93B7FCE7_E22B_45f5_81C9_BF67091B1825</uml:id>
        <rdfs:comment>This subclause contains user-defined dynamic model classes to support the exchange of both proprietary and explicitly defined user-defined models.  
&lt;u&gt;Proprietary models&lt;/u&gt; represent behaviour which, while not defined by a standard model class, is mutually understood by the sending and receiving applications based on the name passed in the .name attribute of the appropriate xxxUserDefined class.  Proprietary model parameters are passed as general attributes using as many instances of the ProprietaryParameterDynamics class as there are parameters.
&lt;u&gt;Explicitly defined models&lt;/u&gt; describe dynamic behaviour in detail in terms of control blocks and their input and output signals.  Note that the classes to support explicitly defined modelling are not currently defined - it is future work intended to also be supported by the family of xxxUserDefined classes.
Both types of user-defined models use the family of xxxUserDefined classes, which allow a user-defined model to be used:
- as the model for an individual standard function block (such as a turbine-governor or power system stabilizer) in a standard interconnection model whose other function blocks could be either standard or user-defined.  For an illustration of this form of usage for a proprietary model, see the ExampleFunctionBlockProprietaryModel diagram in subclause 5.5.
- as the complete representation of a dynamic behaviour model (for an entire synchronous machine, for example) where standard function blocks and standard interconnections are not used at all. For an illustration of this form of usage for a proprietary model, see the ExampleCompleteProprietaryModel diagram in subclause 5.5.</rdfs:comment>
        <rdfs:isDefinedBy rdf:resource="http://iec.ch/TC57/CIM100#Package_Dynamics"/>
        <rdfs:label>UserDefinedModels</rdfs:label>
    </owl:NamedIndividual>
    


    <!-- http://iec.ch/TC57/CIM100#Package_VSC -->

    <owl:NamedIndividual rdf:about="http://iec.ch/TC57/CIM100#Package_VSC">
        <rdf:type rdf:resource="http://langdale.com.au/2005/UML#Package"/>
        <uml:id>EAPK_B0381296_1B6B_45de_8B97_702885B06E17</uml:id>
        <rdfs:isDefinedBy rdf:resource="http://iec.ch/TC57/CIM100#Package_InfHVDCDynamics"/>
        <rdfs:label>VSC</rdfs:label>
    </owl:NamedIndividual>
    


    <!-- http://iec.ch/TC57/CIM100#Package_VoltageAdjusterDynamics -->

    <owl:NamedIndividual rdf:about="http://iec.ch/TC57/CIM100#Package_VoltageAdjusterDynamics">
        <rdf:type rdf:resource="http://langdale.com.au/2005/UML#Package"/>
        <uml:id>EAPK_35B78447_A031_4927_A915_5C69304A72D2</uml:id>
        <rdfs:comment>&lt;font color=&quot;#0f0f0f&quot;&gt;A voltage adjuster is a reference adjuster that uses inputs from a reactive power or power factor controller to modify the voltage regulator set point to maintain the synchronous machine steady-state power factor or reactive power at a predetermined value. &lt;/font&gt;
&lt;font color=&quot;#0f0f0f&quot;&gt;For additional information please refer to IEEE 421.5-2005, 11.&lt;/font&gt;</rdfs:comment>
        <rdfs:isDefinedBy rdf:resource="http://iec.ch/TC57/CIM100#Package_StandardModels"/>
        <rdfs:label>VoltageAdjusterDynamics</rdfs:label>
    </owl:NamedIndividual>
    


    <!-- http://iec.ch/TC57/CIM100#Package_VoltageCompensatorDynamics -->

    <owl:NamedIndividual rdf:about="http://iec.ch/TC57/CIM100#Package_VoltageCompensatorDynamics">
        <rdf:type rdf:resource="http://langdale.com.au/2005/UML#Package"/>
        <uml:id>EAPK_7FD04580_1444_4ea3_A69D_D2D00000A4A9</uml:id>
        <rdfs:comment>&lt;font color=&quot;#0f0f0f&quot;&gt;Synchronous machine terminal voltage transducer and current compensator models&lt;/font&gt; adjust the terminal voltage feedback to the excitation system by adding a quantity that is proportional to the terminal current of the generator.  It is linked to a specific generator (synchronous machine).
&lt;font color=&quot;#0f0f0f&quot;&gt;Several types of compensation are available on most excitation systems. Synchronous machine active and reactive current compensation are the most common. Either reactive droop compensation and/or line-drop compensation can be used, simulating an impedance drop and effectively regulating at some point other than the terminals of the machine. The impedance or range of adjustment and type of compensation should be specified for different types. &lt;/font&gt;
&lt;font color=&quot;#0f0f0f&quot;&gt;Care shall be taken to ensure that a consistent PU system is utilized for the compensator parameters and the synchronous machine current base.&lt;/font&gt;
&lt;font color=&quot;#0f0f0f&quot;&gt;For further information see IEEE 421.5-2005, 4.&lt;/font&gt;


&lt;font color=&quot;#0f0f0f&quot;&gt;
&lt;/font&gt;</rdfs:comment>
        <rdfs:isDefinedBy rdf:resource="http://iec.ch/TC57/CIM100#Package_StandardModels"/>
        <rdfs:label>VoltageCompensatorDynamics</rdfs:label>
    </owl:NamedIndividual>
    


    <!-- http://iec.ch/TC57/CIM100#Package_WindDynamics -->

    <owl:NamedIndividual rdf:about="http://iec.ch/TC57/CIM100#Package_WindDynamics">
        <rdf:type rdf:resource="http://langdale.com.au/2005/UML#Package"/>
        <uml:id>EAPK_6EA4C7E4_FDDC_4438_8A1C_12346215E0FA</uml:id>
        <rdfs:comment>Wind turbines are generally divided into four types, which are currently significant in power systems.  The four types have the following characteristics:
- type 1: wind turbine with directly grid connected asynchronous generator with fixed rotor resistance (typically squirrel cage);
- type 2: wind turbine with directly grid connected asynchronous generator with variable rotor resistance;
- type 3: wind turbines with doubly-fed asynchronous generators (directly connected stator and rotor connected through power converter);
- type 4: wind turbines connected to the grid through a full size power converter.
Models included in this package are according to IEC 61400-27-1:2015.</rdfs:comment>
        <rdfs:isDefinedBy rdf:resource="http://iec.ch/TC57/CIM100#Package_StandardModels"/>
        <rdfs:label>WindDynamics</rdfs:label>
    </owl:NamedIndividual>
    


    <!-- http://iec.ch/TC57/CIM100#Package_Wires -->

    <owl:NamedIndividual rdf:about="http://iec.ch/TC57/CIM100#Package_Wires">
        <rdf:type rdf:resource="http://langdale.com.au/2005/UML#Package"/>
        <uml:id>EAPK_6C99E9CA_2035_4035_B77F_9217E17D86F4</uml:id>
        <rdfs:comment>An extension to the Core and Topology package that models information on the electrical characteristics of Transmission and Distribution networks. This package is used by network applications such as State Estimation, Load Flow and Optimal Power Flow.</rdfs:comment>
        <rdfs:isDefinedBy rdf:resource="http://iec.ch/TC57/CIM100#Package_Base"/>
        <rdfs:label>Wires</rdfs:label>
    </owl:NamedIndividual>
    


    <!-- http://iec.ch/TC57/CIM100#Package_Work -->

    <owl:NamedIndividual rdf:about="http://iec.ch/TC57/CIM100#Package_Work">
        <rdf:type rdf:resource="http://langdale.com.au/2005/UML#Package"/>
        <uml:id>EAPK_B70CA547_A79D_4aac_BBDC_74DAE769AE67</uml:id>
        <rdfs:comment>This package contains the core information classes that support work management and network extension planning applications.</rdfs:comment>
        <rdfs:isDefinedBy rdf:resource="http://iec.ch/TC57/CIM100#Package_IEC61968"/>
        <rdfs:label>Work</rdfs:label>
    </owl:NamedIndividual>
    


    <!-- http://iec.ch/TC57/CIM100#Package_unused -->

    <owl:NamedIndividual rdf:about="http://iec.ch/TC57/CIM100#Package_unused">
        <rdf:type rdf:resource="http://langdale.com.au/2005/UML#Package"/>
        <uml:id>EAPK_DC6CD8C2_B2CE_4849_AB47_760BEA0ACA18</uml:id>
        <rdfs:isDefinedBy rdf:resource="http://iec.ch/TC57/CIM100#Package_NetworkModelFrames"/>
        <rdfs:label>unused</rdfs:label>
    </owl:NamedIndividual>
    


    <!-- http://langdale.com.au/2005/UML#aggregateOf -->

    <owl:NamedIndividual rdf:about="http://langdale.com.au/2005/UML#aggregateOf">
        <rdf:type rdf:resource="http://langdale.com.au/2005/UML#Stereotype"/>
        <rdfs:label>Aggregate Of</rdfs:label>
    </owl:NamedIndividual>
    


    <!-- http://langdale.com.au/2005/UML#attribute -->

    <owl:NamedIndividual rdf:about="http://langdale.com.au/2005/UML#attribute">
        <rdf:type rdf:resource="http://langdale.com.au/2005/UML#Stereotype"/>
        <rdfs:label>Attribute</rdfs:label>
    </owl:NamedIndividual>
    


    <!-- http://langdale.com.au/2005/UML#base -->

    <owl:NamedIndividual rdf:about="http://langdale.com.au/2005/UML#base">
        <rdf:type rdf:resource="http://langdale.com.au/2005/UML#Stereotype"/>
        <rdfs:label>Base</rdfs:label>
    </owl:NamedIndividual>
    


    <!-- http://langdale.com.au/2005/UML#byreference -->

    <owl:NamedIndividual rdf:about="http://langdale.com.au/2005/UML#byreference">
        <rdf:type rdf:resource="http://langdale.com.au/2005/UML#Stereotype"/>
        <rdfs:label>By Reference</rdfs:label>
    </owl:NamedIndividual>
    


    <!-- http://langdale.com.au/2005/UML#cimdatatype -->

    <owl:NamedIndividual rdf:about="http://langdale.com.au/2005/UML#cimdatatype">
        <rdf:type rdf:resource="http://langdale.com.au/2005/UML#Stereotype"/>
        <rdfs:label>CIMDatatype</rdfs:label>
    </owl:NamedIndividual>
    


    <!-- http://langdale.com.au/2005/UML#compositeOf -->

    <owl:NamedIndividual rdf:about="http://langdale.com.au/2005/UML#compositeOf">
        <rdf:type rdf:resource="http://langdale.com.au/2005/UML#Stereotype"/>
        <rdfs:label>Composite Of</rdfs:label>
    </owl:NamedIndividual>
    


    <!-- http://langdale.com.au/2005/UML#compound -->

    <owl:NamedIndividual rdf:about="http://langdale.com.au/2005/UML#compound">
        <rdf:type rdf:resource="http://langdale.com.au/2005/UML#Stereotype"/>
        <rdfs:label>Compound Datatype</rdfs:label>
    </owl:NamedIndividual>
    


    <!-- http://langdale.com.au/2005/UML#concrete -->

    <owl:NamedIndividual rdf:about="http://langdale.com.au/2005/UML#concrete">
        <rdf:type rdf:resource="http://langdale.com.au/2005/UML#Stereotype"/>
        <rdfs:label>Concrete</rdfs:label>
    </owl:NamedIndividual>
    


    <!-- http://langdale.com.au/2005/UML#datatype -->

    <owl:NamedIndividual rdf:about="http://langdale.com.au/2005/UML#datatype">
        <rdf:type rdf:resource="http://langdale.com.au/2005/UML#Stereotype"/>
        <rdfs:label>Datatype</rdfs:label>
    </owl:NamedIndividual>
    


    <!-- http://langdale.com.au/2005/UML#enumeration -->

    <owl:NamedIndividual rdf:about="http://langdale.com.au/2005/UML#enumeration">
        <rdf:type rdf:resource="http://langdale.com.au/2005/UML#Stereotype"/>
        <rdfs:label>Enumeration</rdfs:label>
    </owl:NamedIndividual>
    


    <!-- http://langdale.com.au/2005/UML#extendedby -->

    <owl:NamedIndividual rdf:about="http://langdale.com.au/2005/UML#extendedby">
        <rdf:type rdf:resource="http://langdale.com.au/2005/UML#Stereotype"/>
        <rdfs:label>Extended By</rdfs:label>
    </owl:NamedIndividual>
    


    <!-- http://langdale.com.au/2005/UML#extension -->

    <owl:NamedIndividual rdf:about="http://langdale.com.au/2005/UML#extension">
        <rdf:type rdf:resource="http://langdale.com.au/2005/UML#Stereotype"/>
        <rdfs:label>Extension Class</rdfs:label>
    </owl:NamedIndividual>
    


    <!-- http://langdale.com.au/2005/UML#ofAggregate -->

    <owl:NamedIndividual rdf:about="http://langdale.com.au/2005/UML#ofAggregate">
        <rdf:type rdf:resource="http://langdale.com.au/2005/UML#Stereotype"/>
        <rdfs:label>Of Aggregate</rdfs:label>
    </owl:NamedIndividual>
    


    <!-- http://langdale.com.au/2005/UML#ofComposite -->

    <owl:NamedIndividual rdf:about="http://langdale.com.au/2005/UML#ofComposite">
        <rdf:type rdf:resource="http://langdale.com.au/2005/UML#Stereotype"/>
        <rdfs:label>Of Composite</rdfs:label>
    </owl:NamedIndividual>
    


    <!-- http://langdale.com.au/2005/UML#preserve -->

    <owl:NamedIndividual rdf:about="http://langdale.com.au/2005/UML#preserve">
        <rdf:type rdf:resource="http://langdale.com.au/2005/UML#Stereotype"/>
        <rdfs:label>Preserve</rdfs:label>
    </owl:NamedIndividual>
    


    <!-- http://langdale.com.au/2005/UML#primitive -->

    <owl:NamedIndividual rdf:about="http://langdale.com.au/2005/UML#primitive">
        <rdf:type rdf:resource="http://langdale.com.au/2005/UML#Stereotype"/>
        <rdfs:label>Primitive</rdfs:label>
    </owl:NamedIndividual>
    


    <!-- http://langdale.com.au/2005/UML#union -->

    <owl:NamedIndividual rdf:about="http://langdale.com.au/2005/UML#union">
        <rdf:type rdf:resource="http://langdale.com.au/2005/UML#Stereotype"/>
        <rdfs:label>Union</rdfs:label>
    </owl:NamedIndividual>
    


    <!-- http://langdale.com.au/2005/UML#xmlattribute -->

    <owl:NamedIndividual rdf:about="http://langdale.com.au/2005/UML#xmlattribute">
        <rdf:type rdf:resource="http://langdale.com.au/2005/UML#Stereotype"/>
        <rdfs:label>XML Attribute</rdfs:label>
    </owl:NamedIndividual>
    


    <!-- http://langdale.com.au/2005/UML#xmlelement -->

    <owl:NamedIndividual rdf:about="http://langdale.com.au/2005/UML#xmlelement">
        <rdf:type rdf:resource="http://langdale.com.au/2005/UML#Stereotype"/>
        <rdfs:label>XML Element</rdfs:label>
    </owl:NamedIndividual>
</rdf:RDF>



<!-- Generated by the OWL API (version 4.5.26.2023-07-17T20:34:13Z) https://github.com/owlcs/owlapi -->

